@prefix dbo: <http://dbpedia.org/ontology/> .
@prefix dbprop: <http://dbpedia.org/property/> .
@prefix dct: <http://purl.org/dc/terms/> .
@prefix foaf: <http://xmlns.com/foaf/0.1/> .
@prefix glosis_cl: <http://w3id.org/glosis/model/codelists/> .
@prefix owl: <http://www.w3.org/2002/07/owl#> .
@prefix rdf: <http://www.w3.org/1999/02/22-rdf-syntax-ns#> .
@prefix rdfs: <http://www.w3.org/2000/01/rdf-schema#> .
@prefix schema: <https://schema.org/> .
@prefix skos: <http://www.w3.org/2004/02/skos/core#> .
@prefix sosa: <http://www.w3.org/ns/sosa/> .

<http://w3id.org/glosis/model/codelists> a owl:Ontology ;
    dct:creator [ rdfs:seeAlso <http://orcid.org/0000-0003-4289-4922> ;
            foaf:name "Raul Palma" ;
            schema:affiliation [ foaf:name "PSNC" ] ],
        [ foaf:name "Bogusz Janiak" ;
            schema:affiliation [ foaf:name "PSNC" ] ],
        [ rdfs:seeAlso <http://orcid.org/0000-0002-5851-2071> ;
            foaf:name "Luís Moreira de Sousa" ;
            schema:affiliation [ foaf:name "Técnico ULisboa" ] ] ;
    dct:description "This ontology represents GLOSIS code lists extracted from the data model for the Global Soil Information System (GloSIS) v1.0, edited by Tomas Reznik and Katharina Schleidt"@en ;
    dct:rights "This ontology is distributed under Creative Commons Attribution-NonCommercial-ShareAlike 3.0 IGO License - https://creativecommons.org/licenses/by-nc-sa/3.0/igo/"@en ;
    dct:source "Data model for the Global Soil Information System (GloSIS) v1.0, edited by Tomas Reznik and Katharina Schleidt"@en ;
    dct:title "GLOSIS code lists"@en ;
    rdfs:comment "This module contains all the code lists of observable properties and results codes."@en ;
    owl:versionIRI glosis_cl:v1.5.1 ;
    owl:versionInfo "v1.5.1" .

glosis_cl:biologicalAbundanceValueCode a skos:ConceptScheme ;
    rdfs:label "Code list for biologicalAbundanceValue - codelist scheme"@en ;
    rdfs:seeAlso glosis_cl:BiologicalAbundanceValueCode ;
    skos:definition "Classification of the abundance of biological activity. See more in Guidelines for Soil Description issued by the FAO: table 81" ;
    skos:note "This code list provides possible values for biologicalAbundance."@en ;
    skos:prefLabel "Code list for biologicalAbundanceValue - codelist scheme"@en .

glosis_cl:biologicalFeaturesValueCode a skos:ConceptScheme ;
    rdfs:label "Code list for biologicalFeaturesValue - codelist scheme"@en ;
    rdfs:seeAlso glosis_cl:BiologicalFeaturesValueCode ;
    skos:definition "Examples of biological features. See more in Guidelines for Soil Description issued by the FAO: table 82" ;
    skos:note "This code list provides possible values for biologicalFeatures."@en ;
    skos:prefLabel "Code list for biologicalFeaturesValue - codelist scheme"@en .

glosis_cl:bleachedSandValueCode a skos:ConceptScheme ;
    rdfs:label "Code list for bleachedSandValue - codelist scheme"@en ;
    rdfs:seeAlso glosis_cl:BleachedSandValueCode ;
    skos:definition "Classification of bleached sand characteristics based on the percentage of surface covered. See more in Guidelines for Soil Description issued by the FAO: table 23" ;
    skos:note "This code list provides possible values for bleachedSand."@en ;
    skos:prefLabel "Code list for bleachedSandValue - codelist scheme"@en .

glosis_cl:boundaryClassificationValueCode a skos:ConceptScheme ;
    rdfs:label "Code list for boundaryClassificationValue - codelist scheme"@en ;
    rdfs:seeAlso glosis_cl:BoundaryClassificationValueCode ;
    skos:definition "The boundary between mottle and matrix is described as the thickness of the zone within which the colour transition can be located without being in either the mottle or matrix. See more in guidelines for Soil Description issued by the FAO: table 35" ;
    skos:note "This code list provides possible values for boundaryClassification."@en ;
    skos:prefLabel "Code list for boundaryClassificationValue - codelist scheme"@en .

glosis_cl:boundaryDistinctnessValueCode a skos:ConceptScheme ;
    rdfs:label "Code list for boundaryDistinctnessValue - codelist scheme"@en ;
    rdfs:seeAlso glosis_cl:BoundaryDistinctnessValueCode ;
    skos:definition "The distinctness of the boundary refers to the thickness of the zone in which the horizon boundary can be located without being in one of the adjacent horizons. See more in the  Guidelines for Soil Description issued by the FAO: table 24.1" ;
    skos:note "This code list provides possible values for boundaryDistinctness."@en ;
    skos:prefLabel "Code list for boundaryDistinctnessValue - codelist scheme"@en .

glosis_cl:boundaryTopographyValueCode a skos:ConceptScheme ;
    rdfs:label "Code list for boundaryTopographyValue - codelist scheme"@en ;
    rdfs:seeAlso glosis_cl:BoundaryTopographyValueCode ;
    skos:definition "Classification of horizon boundaries by topography. See more in Guidelines for Soil Description issued by the FAO: table 24,2" ;
    skos:note "This code list provides possible values for boundaryTopography."@en ;
    skos:prefLabel "Code list for boundaryTopographyValue - codelist scheme"@en .

glosis_cl:bulkDensityMineralValueCode a skos:ConceptScheme ;
    rdfs:label "Code list for bulkDensityMineralValue - codelist scheme"@en ;
    rdfs:seeAlso glosis_cl:BulkDensityMineralValueCode ;
    skos:definition "Field determinations of bulk density may be obtained by estimating the force required to push a knife into a soil horizon exposed at a field moist pit wall. See more in Guidelines for Soil Description issued by the FAO: table 58" ;
    skos:note "This code list provides possible values for bulkDensityMineral."@en ;
    skos:prefLabel "Code list for bulkDensityMineralValue - codelist scheme"@en .

glosis_cl:bulkDensityPeatValueCode a skos:ConceptScheme ;
    rdfs:label "Code list for bulkDensityPeatValue - codelist scheme"@en ;
    rdfs:seeAlso glosis_cl:BulkDensityPeatValueCode ;
    skos:definition "Bulk density and volume of solids of organic soils can be estimated after the decomposition stage or the extent of peat drainage. See more in guidelines for Soil Description issued by the FAO: table 59,3" ;
    skos:note "This code list provides possible values for bulkDensityPeat."@en ;
    skos:prefLabel "Code list for bulkDensityPeatValue - codelist scheme"@en .

glosis_cl:carbonatesContentValueCode a skos:ConceptScheme ;
    rdfs:label "Code list for carbonatesContentValue - codelist scheme"@en ;
    rdfs:seeAlso glosis_cl:CarbonatesContentValueCode ;
    skos:definition "Classes for the reaction of carbonates in the soil matrix. See more in Guidelines for Soil Description issued by the FAO: table 38" ;
    skos:note "This code list provides possible values for carbonatesContent."@en ;
    skos:prefLabel "Code list for carbonatesContentValue - codelist scheme"@en .

glosis_cl:carbonatesFormsValueCode a skos:ConceptScheme ;
    rdfs:label "Code list for carbonatesFormsValue - codelist scheme"@en ;
    rdfs:seeAlso glosis_cl:CarbonatesFormsValueCode ;
    skos:definition "The forms of secondary carbonates in soils are diverse and are considered to be informative for diagnostics of soil genesis. See more in guidelines for Soil Description issued by the FAO: table 39" ;
    skos:note "This code list provides possible values for carbonatesForms."@en ;
    skos:prefLabel "Code list for carbonatesFormsValue - codelist scheme"@en .

glosis_cl:cementationContinuityValueCode a skos:ConceptScheme ;
    rdfs:label "Code list for cementationContinuityValue - codelist scheme"@en ;
    rdfs:seeAlso glosis_cl:CementationContinuityValueCode ;
    skos:definition "The occurrence of cementation or compaction in pans or otherwise is described according to its nature, continuity, structure, agent and degree. See more in the guidelines for Soil Description issued by the FAO: table 69" ;
    skos:note "This code list provides possible values for cementationContinuity."@en ;
    skos:prefLabel "Code list for cementationContinuityValue - codelist scheme"@en .

glosis_cl:cementationDegreeValueCode a skos:ConceptScheme ;
    rdfs:label "Code list for cementationDegreeValue - codelist scheme"@en ;
    rdfs:seeAlso glosis_cl:CementationDegreeValueCode ;
    skos:definition "The classification of the degree of cementation/compaction. See more in Guidelines for Soil Description issued by the FAO: table 72" ;
    skos:note "This code list provides possible values for cementationDegree."@en ;
    skos:prefLabel "Code list for cementationDegreeValue - codelist scheme"@en .

glosis_cl:cementationFabricValueCode a skos:ConceptScheme ;
    rdfs:label "Code list for cementationFabricValue - codelist scheme"@en ;
    rdfs:seeAlso glosis_cl:CementationFabricValueCode ;
    skos:definition "Classification of the fabric of the cemented/compacted layer. See more in Guidelines for Soil Description issued by the FAO: table 70" ;
    skos:note "This code list provides possible values for cementationFabric."@en ;
    skos:prefLabel "Code list for cementationFabricValue - codelist scheme"@en .

glosis_cl:cementationNatureValueCode a skos:ConceptScheme ;
    rdfs:label "Code list for cementationNatureValue - codelist scheme"@en ;
    rdfs:seeAlso glosis_cl:CementationNatureValueCode ;
    skos:definition "Classification of the nature of cementation/compaction. See more in Guidelines for Soil Description issued by the FAO: table 71" ;
    skos:note "This code list provides possible values for cementationNature."@en ;
    skos:prefLabel "Code list for cementationNatureValue - codelist scheme"@en .

glosis_cl:clayPropertyCode a skos:ConceptScheme ;
    rdfs:label "Code list for clayProperty - codelist scheme"@en ;
    rdfs:seeAlso glosis_cl:ClayPropertyCode ;
    skos:definition "ISRIC Report 2019/01: Tier 1 and Tier 2 data in the context of the federated Global Soil Information System. Appendix 3" ;
    skos:note "This code list provides possible values for clay."@en ;
    skos:prefLabel "Code list for clayProperty - codelist scheme"@en .

glosis_cl:coatingAbundanceValueCode a skos:ConceptScheme ;
    rdfs:label "Code list for coatingAbundanceValue - codelist scheme"@en ;
    rdfs:seeAlso glosis_cl:CoatingAbundanceValueCode ;
    skos:definition "Classification of abundance of coatings. See more in Guidelines for Soil Description issued by the FAO: table 64" ;
    skos:note "This code list provides possible values for coatingAbundance."@en ;
    skos:prefLabel "Code list for coatingAbundanceValue - codelist scheme"@en .

glosis_cl:coatingContrastValueCode a skos:ConceptScheme ;
    rdfs:label "Code list for coatingContrastValue - codelist scheme"@en ;
    rdfs:seeAlso glosis_cl:CoatingContrastValueCode ;
    skos:definition "Classification of the contrast of coatings. See more in Guidelines for Soil Description issued by the FAO: table 65" ;
    skos:note "This code list provides possible values for coatingContrast."@en ;
    skos:prefLabel "Code list for coatingContrastValue - codelist scheme"@en .

glosis_cl:coatingFormValueCode a skos:ConceptScheme ;
    rdfs:label "Code list for coatingFormValue - codelist scheme"@en ;
    rdfs:seeAlso glosis_cl:CoatingFormValueCode ;
    skos:definition "Classification of the form of coatings. See more in Guidelines for Soil Description issued by the FAO: table 67" ;
    skos:note "This code list provides possible values for coatingForm."@en ;
    skos:prefLabel "Code list for coatingFormValue - codelist scheme"@en .

glosis_cl:coatingLocationValueCode a skos:ConceptScheme ;
    rdfs:label "Code list for coatingLocationValue - codelist scheme"@en ;
    rdfs:seeAlso glosis_cl:CoatingLocationValueCode ;
    skos:definition "Classification of the location of coatings and clay accumulation. See more in Guidelines for Soil Description issued by the FAO: table 68" ;
    skos:note "This code list provides possible values for coatingLocation."@en ;
    skos:prefLabel "Code list for coatingLocationValue - codelist scheme"@en .

glosis_cl:coatingNatureValueCode a skos:ConceptScheme ;
    rdfs:label "Code list for coatingNatureValue - codelist scheme"@en ;
    rdfs:seeAlso glosis_cl:CoatingNatureValueCode ;
    skos:definition "Classification of the nature of coatings. See more in Guidelines for Soil Description issued by the FAO: table 66" ;
    skos:note "This code list provides possible values for coatingNature."@en ;
    skos:prefLabel "Code list for coatingNatureValue - codelist scheme"@en .

glosis_cl:consistenceDryValueCode a skos:ConceptScheme ;
    rdfs:label "Code list for consistenceDryValue - codelist scheme"@en ;
    rdfs:seeAlso glosis_cl:ConsistenceDryValueCode ;
    skos:definition "The consistence when dry is determined by breaking an air-dried mass of soil between thumb and forefinger or in the hand. See more in the guidelines for Soil Description issued by the FAO: table 53" ;
    skos:note "This code list provides possible values for consistenceDry."@en ;
    skos:prefLabel "Code list for consistenceDryValue - codelist scheme"@en .

glosis_cl:consistenceMoistValueCode a skos:ConceptScheme ;
    rdfs:label "Code list for consistenceMoistValue - codelist scheme"@en ;
    rdfs:seeAlso glosis_cl:ConsistenceMoistValueCode ;
    skos:definition "Guidelines for Soil Description issued by the FAO: table 54;Consistence when moist is determined by attempting to crush a mass of moist or slightly moist soil material. See more in Guidelines for Soil Description issued by the FAO: table 54" ;
    skos:note "This code list provides possible values for consistenceMoist."@en ;
    skos:prefLabel "Code list for consistenceMoistValue - codelist scheme"@en .

glosis_cl:contrastValueCode a skos:ConceptScheme ;
    rdfs:label "Code list for contrastValue - codelist scheme"@en ;
    rdfs:seeAlso glosis_cl:ContrastValueCode ;
    skos:definition "The colour contrast between mottles and soil matrix. See more in Guidelines for Soil Description issued by the FAO: table 34" ;
    skos:note "This code list provides possible values for contrast."@en ;
    skos:prefLabel "Code list for contrastValue - codelist scheme"@en .

glosis_cl:cracksDepthValueCode a skos:ConceptScheme ;
    rdfs:label "Code list for cracksDepthValue - codelist scheme"@en ;
    rdfs:seeAlso glosis_cl:CracksDepthValueCode ;
    skos:definition "List of suggested classes of surface cracks in shrink–swell clay-rich soils after they dry out. See more in guidelines for Soil Description issued by the FAO: table 21,2" ;
    skos:note "This code list provides possible values for cracksDepth."@en ;
    skos:prefLabel "Code list for cracksDepthValue - codelist scheme"@en .

glosis_cl:cracksDistanceValueCode a skos:ConceptScheme ;
    rdfs:label "Code list for cracksDistanceValue - codelist scheme"@en ;
    rdfs:seeAlso glosis_cl:CracksDistanceValueCode ;
    skos:definition "Classification of the surface cracks based on distance between the cracks measured in meters. See more in Guidelines for Soil Description issued by the FAO: table 21,3" ;
    skos:note "This code list provides possible values for cracksDistance."@en ;
    skos:prefLabel "Code list for cracksDistanceValue - codelist scheme"@en .

glosis_cl:cracksWidthValueCode a skos:ConceptScheme ;
    rdfs:label "Code list for cracksWidthValue - codelist scheme"@en ;
    rdfs:seeAlso glosis_cl:CracksWidthValueCode ;
    skos:definition "Classification of surface cracks based on the width. See more in Guidelines for Soil Description issued by the FAO: table 21,1" ;
    skos:note "This code list provides possible values for cracksWidth."@en ;
    skos:prefLabel "Code list for cracksWidthValue - codelist scheme"@en .

glosis_cl:cropClassValueCode a skos:ConceptScheme ;
    rdfs:label "Code list for cropClassValue - codelist scheme"@en ;
    rdfs:seeAlso glosis_cl:CropClassValueCode ;
    skos:definition "Examples for the most common crops with their recommended codes. See more in guidelines for Soil Description issued by the FAO: table 9" ;
    skos:note "This code list provides possible values for cropClass."@en ;
    skos:prefLabel "Code list for cropClassValue - codelist scheme"@en .

glosis_cl:erosionActivityPeriodValueCode a skos:ConceptScheme ;
    rdfs:label "Code list for erosionActivityPeriodValue - codelist scheme"@en ;
    rdfs:seeAlso glosis_cl:ErosionActivityPeriodValueCode ;
    skos:definition "The period of activity of accelerated erosion or deposition is described using the recommended classes. See more in Guidelines for Soil Description issued by the FAO: table 19" ;
    skos:note "This code list provides possible values for erosionActivityPeriod."@en ;
    skos:prefLabel "Code list for erosionActivityPeriodValue - codelist scheme"@en .

glosis_cl:erosionAreaAffectedValueCode a skos:ConceptScheme ;
    rdfs:label "Code list for erosionAreaAffectedValue - codelist scheme"@en ;
    rdfs:seeAlso glosis_cl:ErosionAreaAffectedValueCode ;
    skos:definition "Classification of total area affected by erosion and deposition. See more in Guidelines for Soil Description issued by the FAO: table 17" ;
    skos:note "This code list provides possible values for erosionAreaAffected."@en ;
    skos:prefLabel "Code list for erosionAreaAffectedValue - codelist scheme"@en .

glosis_cl:erosionCategoryValueCode a skos:ConceptScheme ;
    rdfs:label "Code list for erosionCategoryValue - codelist scheme"@en ;
    rdfs:seeAlso glosis_cl:ErosionCategoryValueCode ;
    skos:definition "Erosion can be classified as water or wind erosion and include off-site effects such as deposition; a third major category is mass movements (landslides and related phenomena). See more in Guidelines for Soil Description issued by the FAO: table 16" ;
    skos:note "This code list provides possible values for erosionCategory."@en ;
    skos:prefLabel "Code list for erosionCategoryValue - codelist scheme"@en .

glosis_cl:erosionDegreeValueCode a skos:ConceptScheme ;
    rdfs:label "Code list for erosionDegreeValue - codelist scheme"@en ;
    rdfs:seeAlso glosis_cl:ErosionDegreeValueCode ;
    skos:definition "Classification of erosion, by degree. See more in guidelines for Soil Description issued by the FAO: table 18" ;
    skos:note "This code list provides possible values for erosionDegree."@en ;
    skos:prefLabel "Code list for erosionDegreeValue - codelist scheme"@en .

glosis_cl:erosionTotalAreaAffectedValueCode a skos:ConceptScheme ;
    rdfs:label "Code list for erosionTotalAreaAffectedValue - codelist scheme"@en ;
    rdfs:seeAlso glosis_cl:ErosionTotalAreaAffectedValueCode ;
    skos:definition "The total area affected by erosion and deposition is estimated following the classes defined by SOTER (FAO, 1995). See more in the Guidelines for Soil Description issued by the FAO: table 17" ;
    skos:note "This code list provides possible values for erosionTotalAreaAffected."@en ;
    skos:prefLabel "Code list for erosionTotalAreaAffectedValue - codelist scheme"@en .

glosis_cl:floodDurationValueCode a skos:ConceptScheme ;
    rdfs:label "Code list for floodDurationValue - codelist scheme"@en ;
    rdfs:seeAlso glosis_cl:FloodDurationValueCode ;
    skos:definition "Related to the amount of time an area remains inundated by floodwater.  This metric is important because it helps assess the extent of waterlogging and its impact on soil properties, particularly in terms of oxygen availability and soil aeration. Flood duration affects the mobility of nutrients and contaminants within the soil, influencing both agricultural productivity and environmental quality. Longer flood durations can also lead to changes in soil texture and structure due to the continuous movement and deposition of particles during inundation​. Source: Guidance for Flood Risk Analysis and Mapping" ;
    skos:note "This code list provides possible values for floodDuration."@en ;
    skos:prefLabel "Code list for floodDurationValue - codelist scheme"@en .

glosis_cl:floodFrequencyValueCode a skos:ConceptScheme ;
    rdfs:label "Code list for floodFrequencyValue - codelist scheme"@en ;
    rdfs:seeAlso glosis_cl:FloodFrequencyValueCode ;
    skos:definition "Refers to the statistical analysis of the occurrence of floods at a particular location over a defined time period. It often involves calculating the recurrence intervals or return periods of flood events, which are typically used to understand how often a specific flood magnitude (like a 100-year flood) is likely to occur. Source: Introduction to Flood Frequency Analysis" ;
    skos:note "This code list provides possible values for floodFrequency."@en ;
    skos:prefLabel "Code list for floodFrequencyValue - codelist scheme"@en .

glosis_cl:fragmentCoverValueCode a skos:ConceptScheme ;
    rdfs:label "Code list for fragmentCoverValue - codelist scheme"@en ;
    rdfs:seeAlso glosis_cl:FragmentCoverValueCode ;
    skos:definition "Coarse surface fragments, including those partially exposed, should be described in terms of percentage of surface coverage and of size of the fragments. See more in Guidelines for Soil Description issued by the FAO: table 15,1" ;
    skos:note "This code list provides possible values for fragmentCover."@en ;
    skos:prefLabel "Code list for fragmentCoverValue - codelist scheme"@en .

glosis_cl:fragmentsClassValueCode a skos:ConceptScheme ;
    rdfs:label "Code list for fragmentsClassValue - codelist scheme"@en ;
    rdfs:seeAlso glosis_cl:FragmentsClassValueCode ;
    skos:definition "Horizon properties encountered in a global data compilation programme. See more in ISRIC Report 2019/01: Tier 1 and Tier 2 data in the context of the federated Global Soil Information System. Appendix 3" ;
    skos:note "This code list provides possible values for fragmentsClass."@en ;
    skos:prefLabel "Code list for fragmentsClassValue - codelist scheme"@en .

glosis_cl:fragmentsSizeValueCode a skos:ConceptScheme ;
    rdfs:label "Code list for fragmentsSizeValue - codelist scheme"@en ;
    rdfs:seeAlso glosis_cl:FragmentsSizeValueCode ;
    skos:definition "Classes of occurrence of coarse surface fragments are correlated with the ones for rock outcrop. See more in guidelines for Soil Description issued by the FAO: table 15,2" ;
    skos:note "This code list provides possible values for fragmentsSize."@en ;
    skos:prefLabel "Code list for fragmentsSizeValue - codelist scheme"@en .

glosis_cl:gypsumContentValueCode a skos:ConceptScheme ;
    rdfs:label "Code list for gypsumContentValue - codelist scheme"@en ;
    rdfs:seeAlso glosis_cl:GypsumContentValueCode ;
    skos:definition "Where more readily soluble salts are absent, gypsum can be estimated in the field by measurements of electrical conductivity. More in the guidelines for Soil Description issued by the FAO: table 40" ;
    skos:note "This code list provides possible values for gypsumContent."@en ;
    skos:prefLabel "Code list for gypsumContentValue - codelist scheme"@en .

glosis_cl:gypsumFormsValueCode a skos:ConceptScheme ;
    rdfs:label "Code list for gypsumFormsValue - codelist scheme"@en ;
    rdfs:seeAlso glosis_cl:GypsumFormsValueCode ;
    skos:definition "The forms of secondary gypsum in soils are diverse and are considered to be informative for diagnostics of soil genesis. See more information in the Guidelines for Soil Description issued by the FAO: table 41" ;
    skos:note "This code list provides possible values for gypsumForms."@en ;
    skos:prefLabel "Code list for gypsumFormsValue - codelist scheme"@en .

glosis_cl:humanInfluenceClassValueCode a skos:ConceptScheme ;
    rdfs:label "Code list for humanInfluenceClassValue - codelist scheme"@en ;
    rdfs:seeAlso glosis_cl:HumanInfluenceClassValueCode ;
    skos:definition "This item refers to any evidence of human activity that is likely to have affected the landscape or the physical and chemical properties of the soil. See more in the Guidelines for Soil Description issued by the FAO: table 10" ;
    skos:note "This code list provides possible values for humanInfluenceClass."@en ;
    skos:prefLabel "Code list for humanInfluenceClassValue - codelist scheme"@en .

glosis_cl:landUseClassValueCode a skos:ConceptScheme ;
    rdfs:label "Code list for landUseClassValue - codelist scheme"@en ;
    rdfs:seeAlso glosis_cl:LandUseClassValueCode ;
    skos:definition "Land use applies to the current use of the land, whether agricultural or nonagricultural, in which the soil is located. See more in the guidelines for Soil Description issued by the FAO: table 8" ;
    skos:note "This code list provides possible values for landUseClass."@en ;
    skos:prefLabel "Code list for landUseClassValue - codelist scheme"@en .

glosis_cl:landformComplexValueCode a skos:ConceptScheme ;
    rdfs:label "Code list for landformComplexValue - codelist scheme"@en ;
    rdfs:seeAlso glosis_cl:LandformComplexValueCode ;
    skos:definition "Subdivisions for complex landforms. See more in Guidelines for Soil Description issued by the FAO: table 5" ;
    skos:note "This code list provides possible values for landformComplex."@en ;
    skos:prefLabel "Code list for landformComplexValue - codelist scheme"@en .

glosis_cl:lithologyValueCode a skos:ConceptScheme ;
    rdfs:label "Code list for lithologyValue - codelist scheme"@en ;
    rdfs:seeAlso glosis_cl:LithologyValueCode ;
    skos:definition "In order to be able to work in smaller scales, some additional natural and anthropogenic parent materials are used for the identification of rocks  in the field, the keys to the most important rock types are provided in the hierarchical SOTER list. See more in the guidelines for Soil Description issued by the FAO: table 12" ;
    skos:note "This code list provides possible values for lithology."@en ;
    skos:prefLabel "Code list for lithologyValue - codelist scheme"@en .

glosis_cl:majorLandFormValueCode a skos:ConceptScheme ;
    rdfs:label "Code list for majorLandFormValue - codelist scheme"@en ;
    rdfs:seeAlso glosis_cl:MajorLandFormValueCode ;
    skos:definition "Hierarchy of major landforms. See more in Guidelines for Soil Description issued by the FAO: table 4" ;
    skos:note "This code list provides possible values for majorLandForm."@en ;
    skos:prefLabel "Code list for majorLandFormValue - codelist scheme"@en .

glosis_cl:mineralConcColourValueCode a skos:ConceptScheme ;
    rdfs:label "Code list for mineralConcColourValue - codelist scheme"@en ;
    rdfs:seeAlso glosis_cl:MineralConcColourValueCode ;
    skos:definition "The general colour names are usually sufficient to describe the colour of the nodules (similar to mottles) or of artefacts. See more in Guidelines for Soil Description issued by the FAO: table 78" ;
    skos:note "This code list provides possible values for mineralConcColour."@en ;
    skos:prefLabel "Code list for mineralConcColourValue - codelist scheme"@en .

glosis_cl:mineralConcHardnessValueCode a skos:ConceptScheme ;
    rdfs:label "Code list for mineralConcHardnessValue - codelist scheme"@en ;
    rdfs:seeAlso glosis_cl:MineralConcHardnessValueCode ;
    skos:definition "Classification of the hardness of mineral concentrations. More in the Guidelines for Soil Description issued by the FAO: table 76" ;
    skos:note "This code list provides possible values for mineralConcHardness."@en ;
    skos:prefLabel "Code list for mineralConcHardnessValue - codelist scheme"@en .

glosis_cl:mineralConcKindValueCode a skos:ConceptScheme ;
    rdfs:label "Code list for mineralConcKindValue - codelist scheme"@en ;
    rdfs:seeAlso glosis_cl:MineralConcKindValueCode ;
    skos:definition "Classification of the kinds of mineral concentrations. See more in guidelines for Soil Description issued by the FAO: table 74" ;
    skos:note "This code list provides possible values for mineralConcKind."@en ;
    skos:prefLabel "Code list for mineralConcKindValue - codelist scheme"@en .

glosis_cl:mineralConcNatureValueCode a skos:ConceptScheme ;
    rdfs:label "Code list for mineralConcNatureValue - codelist scheme"@en ;
    rdfs:seeAlso glosis_cl:MineralConcNatureValueCode ;
    skos:definition "Mineral concentrations are described according to the composition or impregnating substance.See more in Guidelines for Soil Description issued by the FAO: 77" ;
    skos:note "This code list provides possible values for mineralConcNature."@en ;
    skos:prefLabel "Code list for mineralConcNatureValue - codelist scheme"@en .

glosis_cl:mineralConcShapeValueCode a skos:ConceptScheme ;
    rdfs:label "Code list for mineralConcShapeValue - codelist scheme"@en ;
    rdfs:seeAlso glosis_cl:MineralConcShapeValueCode ;
    skos:definition "Classification of the size and shape of mineral concentrations. See more in Guidelines for Soil Description issued by the FAO: table 75,2" ;
    skos:note "This code list provides possible values for mineralConcShape."@en ;
    skos:prefLabel "Code list for mineralConcShapeValue - codelist scheme"@en .

glosis_cl:mineralConcSizeValueCode a skos:ConceptScheme ;
    rdfs:label "Code list for mineralConcSizeValue - codelist scheme"@en ;
    rdfs:seeAlso glosis_cl:MineralConcSizeValueCode ;
    skos:definition "Classification of mineral concentrations based on size. See more in Guidelines for Soil Description issued by the FAO: table 75,1" ;
    skos:note "This code list provides possible values for mineralConcSize."@en ;
    skos:prefLabel "Code list for mineralConcSizeValue - codelist scheme"@en .

glosis_cl:mineralConcVolumeValueCode a skos:ConceptScheme ;
    rdfs:label "Code list for mineralConcVolumeValue - codelist scheme"@en ;
    rdfs:seeAlso glosis_cl:MineralConcVolumeValueCode ;
    skos:definition "The mineral concentrations are described according to their abundance, kind, size, shape, hardness, nature and colour. See more onGuidelines for Soil Description issued by the FAO: table 73" ;
    skos:note "This code list provides possible values for mineralConcVolume."@en ;
    skos:prefLabel "Code list for mineralConcVolumeValue - codelist scheme"@en .

glosis_cl:mineralFragmentsValueCode a skos:ConceptScheme ;
    rdfs:label "Code list for mineralFragmentsValue - codelist scheme"@en ;
    rdfs:seeAlso glosis_cl:MineralFragmentsValueCode ;
    skos:definition "Codes for primary mineral fragments. See more in Guidelines for Soil Description issued by the FAO: table 30" ;
    skos:note "This code list provides possible values for mineralFragments."@en ;
    skos:prefLabel "Code list for mineralFragmentsValue - codelist scheme"@en .

glosis_cl:mottlesAbundanceValueCode a skos:ConceptScheme ;
    rdfs:label "Code list for mottlesAbundanceValue - codelist scheme"@en ;
    rdfs:seeAlso glosis_cl:MottlesAbundanceValueCode ;
    skos:definition "The abundance of mottles is described in terms of classes indicating the percentage of the exposed surface that the mottles occupy. See more in the Guidelines for Soil Description issued by the FAO: table 32" ;
    skos:note "This code list provides possible values for mottlesAbundance."@en ;
    skos:prefLabel "Code list for mottlesAbundanceValue - codelist scheme"@en .

glosis_cl:mottlesSizeValueCode a skos:ConceptScheme ;
    rdfs:label "Code list for mottlesSizeValue - codelist scheme"@en ;
    rdfs:seeAlso glosis_cl:MottlesSizeValueCode ;
    skos:definition "The individual classes of the mottle nodules according to their diameter size. See more in the guidelines for Soil Description issued by the FAO: table 33" ;
    skos:note "This code list provides possible values for mottlesSize."@en ;
    skos:prefLabel "Code list for mottlesSizeValue - codelist scheme"@en .

glosis_cl:organicMatterClassValueCode a skos:ConceptScheme ;
    rdfs:label "Code list for organicMatterClassValue - codelist scheme"@en ;
    rdfs:seeAlso glosis_cl:OrganicMatterClassValueCode ;
    skos:definition "Refers to the categorization or classification of soil based on the quality, quantity, and composition of organic matter present, influencing soil properties such as fertility, water retention, and microbial activity. Source: Source: FAO, Soil Organic Matter and Soil Health, Land and Water Development Division." ;
    skos:note "This code list provides possible values for organicMatterClass."@en ;
    skos:prefLabel "Code list for organicMatterClassValue - codelist scheme"@en .

glosis_cl:peatDecompostionValueCode a skos:ConceptScheme ;
    rdfs:label "Code list for peatDecompostionValue - codelist scheme"@en ;
    rdfs:seeAlso glosis_cl:PeatDecompostionValueCode ;
    skos:definition "In most organic layers of rocks the determination of the texture class is done by estimating of the degree of decomposition and humification of the organic material.See more in Guidelines for Soil Description issued by the FAO: table 31" ;
    skos:note "This code list provides possible values for peatDecompostion."@en ;
    skos:prefLabel "Code list for peatDecompostionValue - codelist scheme"@en .

glosis_cl:peatDrainageValueCode a skos:ConceptScheme ;
    rdfs:label "Code list for peatDrainageValue - codelist scheme"@en ;
    rdfs:seeAlso glosis_cl:PeatDrainageValueCode ;
    skos:definition "Bulk density and volume of solids of organic soils may be estimated after the decomposition stage or the extent of peat drainage. More information is in the guidelines for Soil Description issued by the FAO: table 59,1" ;
    skos:note "This code list provides possible values for peatDrainage."@en ;
    skos:prefLabel "Code list for peatDrainageValue - codelist scheme"@en .

glosis_cl:peatVolumeValueCode a skos:ConceptScheme ;
    rdfs:label "Code list for peatVolumeValue - codelist scheme"@en ;
    rdfs:seeAlso glosis_cl:PeatVolumeValueCode ;
    skos:definition "Field estimation of volume of solids and bulk density of peat soils. See more in Guidelines for Soil Description issued by the FAO: table 59,2" ;
    skos:note "This code list provides possible values for peatVolume."@en ;
    skos:prefLabel "Code list for peatVolumeValue - codelist scheme"@en .

glosis_cl:physioChemicalPropertyCode a skos:ConceptScheme ;
    rdfs:label "Code list for physioChemicalProperty - codelist scheme"@en ;
    rdfs:seeAlso glosis_cl:PhysioChemicalPropertyCode ;
    skos:definition "ISRIC Report 2019/01: Tier 1 and Tier 2 data in the context of the federated Global Soil Information System. Appendix 3;ISRIC Report 2014/01: Africa Soil Profiles Database Version 1.2. Annex 3a" ;
    skos:note "This code list provides possible values for physioChemical."@en ;
    skos:prefLabel "Code list for physioChemicalProperty - codelist scheme"@en .

glosis_cl:physiographyValueCode a skos:ConceptScheme ;
    rdfs:label "Code list for physiographyValue - codelist scheme"@en ;
    rdfs:seeAlso glosis_cl:PhysiographyValueCode ;
    skos:definition "The relative position of the site within the land should be indicated. The position affects the hydrological conditions of the site. See more in the Guidelines for Soil Description issued by the FAO: figure 2" ;
    skos:note "This code list provides possible values for physiography."@en ;
    skos:prefLabel "Code list for physiographyValue - codelist scheme"@en .

glosis_cl:plasticityValueCode a skos:ConceptScheme ;
    rdfs:label "Code list for plasticityValue - codelist scheme"@en ;
    rdfs:seeAlso glosis_cl:PlasticityValueCode ;
    skos:definition "Plasticity is the ability of soil material to change shape continuously under the influence of an applied stress and to retain the compressed shape on removal of stress. See more in Guidelines for Soil Description issued by the FAO: Guidelines for Soil Description issued by the FAO: table 56" ;
    skos:note "This code list provides possible values for plasticity."@en ;
    skos:prefLabel "Code list for plasticityValue - codelist scheme"@en .

glosis_cl:poresAbundanceValueCode a skos:ConceptScheme ;
    rdfs:label "Code list for poresAbundanceValue - codelist scheme"@en ;
    rdfs:seeAlso glosis_cl:PoresAbundanceValueCode ;
    skos:definition "Classification of abundance of pores. See more in Guidelines for Soil Description issued by the FAO: table 63" ;
    skos:note "This code list provides possible values for poresAbundance."@en ;
    skos:prefLabel "Code list for poresAbundanceValue - codelist scheme"@en .

glosis_cl:porosityClassValueCode a skos:ConceptScheme ;
    rdfs:label "Code list for porosityClassValue - codelist scheme"@en ;
    rdfs:seeAlso glosis_cl:PorosityClassValueCode ;
    skos:definition "The porosity is an indication of the total volume of voids discernible with a ×10 hand-lens measured by area and recorded as the percentage of the surface occupied by pores. See more in guidelines for Soil Description issued by the FAO: table 60" ;
    skos:note "This code list provides possible values for porosityClass."@en ;
    skos:prefLabel "Code list for porosityClassValue - codelist scheme"@en .

glosis_cl:profileDescriptionStatusValueCode a skos:ConceptScheme ;
    rdfs:label "Code list for profileDescriptionStatusValue - codelist scheme"@en ;
    rdfs:seeAlso glosis_cl:ProfileDescriptionStatusValueCode ;
    skos:definition "Soil profile description status. See more in Guidelines for Soil Description issued by the FAO: table 1" ;
    skos:note "This code list provides possible values for profileDescriptionStatus."@en ;
    skos:prefLabel "Code list for profileDescriptionStatusValue - codelist scheme"@en .

glosis_cl:rockAbundanceValueCode a skos:ConceptScheme ;
    rdfs:label "Code list for rockAbundanceValue - codelist scheme"@en ;
    rdfs:seeAlso glosis_cl:RockAbundanceValueCode ;
    skos:definition "Abundance of rock fragments and artefacts, by volume. See more in Guidelines for Soil Description issued by the FAO: table 26" ;
    skos:note "This code list provides possible values for rockAbundance."@en ;
    skos:prefLabel "Code list for rockAbundanceValue - codelist scheme"@en .

glosis_cl:rockOutcropsCoverValueCode a skos:ConceptScheme ;
    rdfs:label "Code list for rockOutcropsCoverValue - codelist scheme"@en ;
    rdfs:seeAlso glosis_cl:RockOutcropsCoverValueCode ;
    skos:definition "Recommended classes of percentage of surface cover and of average distance between rock outcrops. See more in Guidelines for Soil Description issued by the FAO: table 14,1" ;
    skos:note "This code list provides possible values for rockOutcropsCover."@en ;
    skos:prefLabel "Code list for rockOutcropsCoverValue - codelist scheme"@en .

glosis_cl:rockOutcropsDistanceValueCode a skos:ConceptScheme ;
    rdfs:label "Code list for rockOutcropsDistanceValue - codelist scheme"@en ;
    rdfs:seeAlso glosis_cl:RockOutcropsDistanceValueCode ;
    skos:definition "Recommended classes of percentage of surface cover and of average distance between rock outcrops. See more in Guidelines for Soil Description issued by the FAO: table 14,2" ;
    skos:note "This code list provides possible values for rockOutcropsDistance."@en ;
    skos:prefLabel "Code list for rockOutcropsDistanceValue - codelist scheme"@en .

glosis_cl:rockShapeValueCode a skos:ConceptScheme ;
    rdfs:label "Code list for rockShapeValue - codelist scheme"@en ;
    rdfs:seeAlso glosis_cl:RockShapeValueCode ;
    skos:definition "The general shape or roundness of rock fragments. See more on Guidelines for Soil Description issued by the FAO: table 28" ;
    skos:note "This code list provides possible values for rockShape."@en ;
    skos:prefLabel "Code list for rockShapeValue - codelist scheme"@en .

glosis_cl:rockSizeValueCode a skos:ConceptScheme ;
    rdfs:label "Code list for rockSizeValue - codelist scheme"@en ;
    rdfs:seeAlso glosis_cl:RockSizeValueCode ;
    skos:definition "Classification for rock fragments and artefacts influences the nutrient status, water movement, use and management of the soil. See more in guidelines for Soil Description issued by the FAO: table 27" ;
    skos:note "This code list provides possible values for rockSize."@en ;
    skos:prefLabel "Code list for rockSizeValue - codelist scheme"@en .

glosis_cl:rootsAbundanceValueCode a skos:ConceptScheme ;
    rdfs:label "Code list for rootsAbundanceValue - codelist scheme"@en ;
    rdfs:seeAlso glosis_cl:RootsAbundanceValueCode ;
    skos:definition "classification of the abundance of roots.. See more in Guidelines for Soil Description issued by the FAO: table 80" ;
    skos:note "This code list provides possible values for rootsAbundance."@en ;
    skos:prefLabel "Code list for rootsAbundanceValue - codelist scheme"@en .

glosis_cl:saltContentValueCode a skos:ConceptScheme ;
    rdfs:label "Code list for saltContentValue - codelist scheme"@en ;
    rdfs:seeAlso glosis_cl:SaltContentValueCode ;
    skos:definition "Classification of salt content of soil. See more in Guidelines for Soil Description issued by the FAO: table 42" ;
    skos:note "This code list provides possible values for saltContent."@en ;
    skos:prefLabel "Code list for saltContentValue - codelist scheme"@en .

glosis_cl:saltCoverValueCode a skos:ConceptScheme ;
    rdfs:label "Code list for saltCoverValue - codelist scheme"@en ;
    rdfs:seeAlso glosis_cl:SaltCoverValueCode ;
    skos:definition "The occurrence of salt at the surface may be described in terms of cover, appearance and type of salt. See more in the guidelines for Soil Description issued by the FAO: table 22,1" ;
    skos:note "This code list provides possible values for saltCover."@en ;
    skos:prefLabel "Code list for saltCoverValue - codelist scheme"@en .

glosis_cl:saltThicknessValueCode a skos:ConceptScheme ;
    rdfs:label "Code list for saltThicknessValue - codelist scheme"@en ;
    rdfs:seeAlso glosis_cl:SaltThicknessValueCode ;
    skos:definition "The occurrence of salt at the surface may be described in terms of cover, appearance and type of salt. See more in the Guidelines for Soil Description issued by the FAO: table 22,2" ;
    skos:note "This code list provides possible values for saltThickness."@en ;
    skos:prefLabel "Code list for saltThicknessValue - codelist scheme"@en .

glosis_cl:sandPropertyCode a skos:ConceptScheme ;
    rdfs:label "Code list for sandProperty - codelist scheme"@en ;
    rdfs:seeAlso glosis_cl:SandPropertyCode ;
    skos:definition "ISRIC Report 2019/01: Tier 1 and Tier 2 data in the context of the federated Global Soil Information System. Appendix 3" ;
    skos:note "This code list provides possible values for sand."@en ;
    skos:prefLabel "Code list for sandProperty - codelist scheme"@en .

glosis_cl:sandyTextureValueCode a skos:ConceptScheme ;
    rdfs:label "Code list for sandyTextureValue - codelist scheme"@en ;
    rdfs:seeAlso glosis_cl:SandyTextureValueCode ;
    skos:definition "Relation of constituents of fine earth by size, defining textural classes and sand subclasses. See more in Guidelines for Soil Description issued by the FAO: figure 4,3" ;
    skos:note "This code list provides possible values for sandyTexture."@en ;
    skos:prefLabel "Code list for sandyTextureValue - codelist scheme"@en .

glosis_cl:sealingConsistenceValueCode a skos:ConceptScheme ;
    rdfs:label "Code list for sealingConsistenceValue - codelist scheme"@en ;
    rdfs:seeAlso glosis_cl:SealingConsistenceValueCode ;
    skos:definition "Classification of the attributes of surface sealing based on consistency. See more in Guidelines for Soil Description issued by the FAO: table 20,2" ;
    skos:note "This code list provides possible values for sealingConsistence."@en ;
    skos:prefLabel "Code list for sealingConsistenceValue - codelist scheme"@en .

glosis_cl:sealingThicknessValueCode a skos:ConceptScheme ;
    rdfs:label "Code list for sealingThicknessValue - codelist scheme"@en ;
    rdfs:seeAlso glosis_cl:SealingThicknessValueCode ;
    skos:definition "Surface sealing is used to describe crusts that develop at the soil surface after the topsoil dries out. See more in Guidelines for Soil Description issued by the FAO: 20,1" ;
    skos:note "This code list provides possible values for sealingThickness."@en ;
    skos:prefLabel "Code list for sealingThicknessValue - codelist scheme"@en .

glosis_cl:siltPropertyCode a skos:ConceptScheme ;
    rdfs:label "Code list for siltProperty - codelist scheme"@en ;
    rdfs:seeAlso glosis_cl:SiltPropertyCode ;
    skos:definition "ISRIC Report 2019/01: Tier 1 and Tier 2 data in the context of the federated Global Soil Information System. Appendix 3" ;
    skos:note "This code list provides possible values for silt."@en ;
    skos:prefLabel "Code list for siltProperty - codelist scheme"@en .

glosis_cl:slopeFormValueCode a skos:ConceptScheme ;
    rdfs:label "Code list for slopeFormValue - codelist scheme"@en ;
    rdfs:seeAlso glosis_cl:SlopeFormValueCode ;
    skos:definition "The slope form refers to the general shape of the slope in both the vertical and horizontal directions. See more in Guidelines for Soil Description issued by the FAO: table 6" ;
    skos:note "This code list provides possible values for slopeForm."@en ;
    skos:prefLabel "Code list for slopeFormValue - codelist scheme"@en .

glosis_cl:slopeGradientClassValueCode a skos:ConceptScheme ;
    rdfs:label "Code list for slopeGradientClassValue - codelist scheme"@en ;
    rdfs:seeAlso glosis_cl:SlopeGradientClassValueCode ;
    skos:definition "Slope gradient classes measured on the percentage of slope. See more in Guidelines for Soil Description issued by the FAO: table 7" ;
    skos:note "This code list provides possible values for slopeGradientClass."@en ;
    skos:prefLabel "Code list for slopeGradientClassValue - codelist scheme"@en .

glosis_cl:slopePathwaysValueCode a skos:ConceptScheme ;
    rdfs:label "Code list for slopePathwaysValue - codelist scheme"@en ;
    rdfs:seeAlso glosis_cl:SlopePathwaysValueCode ;
    skos:definition "The slope form refers to the general shape of the slope in both the vertical and horizontal directions. See more in guidelines for Soil Description issued by the FAO: figure 3" ;
    skos:note "This code list provides possible values for slopePathways."@en ;
    skos:prefLabel "Code list for slopePathwaysValue - codelist scheme"@en .

glosis_cl:stickinessValueCode a skos:ConceptScheme ;
    rdfs:label "Code list for stickinessValue - codelist scheme"@en ;
    rdfs:seeAlso glosis_cl:StickinessValueCode ;
    skos:definition "Stickiness is the quality of adhesion of the soil material to other objects determined by noting the adherence of soil material when it is pressed between thumb and finger. See more in the Guidelines for Soil Description issued by the FAO: table 55" ;
    skos:note "This code list provides possible values for stickiness."@en ;
    skos:prefLabel "Code list for stickinessValue - codelist scheme"@en .

glosis_cl:structureGradeValueCode a skos:ConceptScheme ;
    rdfs:label "Code list for structureGradeValue - codelist scheme"@en ;
    rdfs:seeAlso glosis_cl:StructureGradeValueCode ;
    skos:definition "Guidelines for Soil Description issued by the FAO: table 47; Classification of structure of pedal soil materials. See more in Guidelines for Soil Description issued by the FAO: table 47" ;
    skos:note "This code list provides possible values for structureGrade."@en ;
    skos:prefLabel "Code list for structureGradeValue - codelist scheme"@en .

glosis_cl:structureSizeValueCode a skos:ConceptScheme ;
    rdfs:label "Code list for structureSizeValue - codelist scheme"@en ;
    rdfs:seeAlso glosis_cl:StructureSizeValueCode ;
    skos:definition "Size classes for soil structure types. See more in guidelines for Soil Description issued by the FAO: table 50" ;
    skos:note "This code list provides possible values for structureSize."@en ;
    skos:prefLabel "Code list for structureSizeValue - codelist scheme"@en .

glosis_cl:surfaceAgeValueCode a skos:ConceptScheme ;
    rdfs:label "Code list for surfaceAgeValue - codelist scheme"@en ;
    rdfs:seeAlso glosis_cl:SurfaceAgeValueCode ;
    skos:definition "The age of the landscape is important information from which the possible duration of the occurrence of soil formation processes can be derived. See more in guidelines for Soil Description issued by the FAO: table 13" ;
    skos:note "This code list provides possible values for surfaceAge."@en ;
    skos:prefLabel "Code list for surfaceAgeValue - codelist scheme"@en .

glosis_cl:textClayPropertyCode a skos:ConceptScheme ;
    rdfs:label "Code list for textClayProperty - codelist scheme"@en ;
    rdfs:seeAlso glosis_cl:TextClayPropertyCode ;
    skos:definition "Eva Corral-Pazos-de-Provens, Ígor Rapp-Arrarás and Juan M. Domingo-Santos, Estimating textural fractions of the USDA using those of the International System: A quantile approach, Geoderma, Volume 416, 2022." ;
    skos:note "This code list provides possible values for textClay."@en ;
    skos:prefLabel "Code list for textClayProperty - codelist scheme"@en .

glosis_cl:textSandPropertyCode a skos:ConceptScheme ;
    rdfs:label "Code list for textSandProperty - codelist scheme"@en ;
    rdfs:seeAlso glosis_cl:TextSandPropertyCode ;
    skos:definition "ISO 14688-1:2017 Geotechnical investigation and testing — Identification and classification of soil ;S.J. Blott and K. Pye, Particle size scales and classification of sediment types based on particle size distributions: Review and recommended procedures, Sedimentology, 59 (7) (2012), pp. 2071-2096.  ;International Society of Soil Science (ISSS), 1929. The minutes of the First Commission meetings, International Congress of Soil Science, Washington 1927. Proc. Int. Soc. Soil Sci. 4 (3), pp. 215–222." ;
    skos:note "This code list provides possible values for textSand."@en ;
    skos:prefLabel "Code list for textSandProperty - codelist scheme"@en .

glosis_cl:textSiltPropertyCode a skos:ConceptScheme ;
    rdfs:label "Code list for textSiltProperty - codelist scheme"@en ;
    rdfs:seeAlso glosis_cl:TextSiltPropertyCode ;
    skos:definition "ISO 14688-1:2017 Geotechnical investigation and testing — Identification and classification of soil ;S.J. Blott and K. Pye, Particle size scales and classification of sediment types based on particle size distributions: Review and recommended procedures, Sedimentology, 59 (7) (2012), pp. 2071-2096.  " ;
    skos:note "This code list provides possible values for textSilt."@en ;
    skos:prefLabel "Code list for textSiltProperty - codelist scheme"@en .

glosis_cl:textureUnconsolidatedValueCode a skos:ConceptScheme ;
    rdfs:label "Code list for textureUnconsolidatedValue - codelist scheme"@en ;
    rdfs:seeAlso glosis_cl:TextureUnconsolidatedValueCode ;
    skos:definition "Texture of a soil that is unconsolidated or loose, typically not bound into a compact mass. It describes the proportions of sand, silt, and clay in the soil, which directly influences the soil's physical properties such as water retention, aeration, and fertility. This texture classification can impact various soil management practices, such as tillage, irrigation, and erosion control. Source: Canadian Soil Information Service - chapter 17 & Geosciences libretexts - 3.1: Soil Texture and Structure. Possible values include unconsolidated Sand,Silt, Clay, Loam. Silty Sand, Clayey Sand" ;
    skos:note "This code list provides possible values for textureUnconsolidated."@en ;
    skos:prefLabel "Code list for textureUnconsolidatedValue - codelist scheme"@en .

glosis_cl:vegetationClassValueCode a skos:ConceptScheme ;
    rdfs:label "Code list for vegetationClassValue - codelist scheme"@en ;
    rdfs:seeAlso glosis_cl:VegetationClassValueCode ;
    skos:definition "Classification of vegetation.See more in Guidelines for Soil Description issued by the FAO: table 11" ;
    skos:note "This code list provides possible values for vegetationClass."@en ;
    skos:prefLabel "Code list for vegetationClassValue - codelist scheme"@en .

glosis_cl:voidsClassificationValueCode a skos:ConceptScheme ;
    rdfs:label "Code list for voidsClassificationValue - codelist scheme"@en ;
    rdfs:seeAlso glosis_cl:VoidsClassificationValueCode ;
    skos:definition "Voids include all empty spaces in the soil. They are related to the arrangement of the primary soil constituents, rooting patterns, burrowing of animals or any other soil-forming processes, such as cracking, translocation and leaching. See more in Guidelines for Soil Description issued by the FAO: table 61" ;
    skos:note "This code list provides possible values for voidsClassification."@en ;
    skos:prefLabel "Code list for voidsClassificationValue - codelist scheme"@en .

glosis_cl:voidsDiameterValueCode a skos:ConceptScheme ;
    rdfs:label "Code list for voidsDiameterValue - codelist scheme"@en ;
    rdfs:seeAlso glosis_cl:VoidsDiameterValueCode ;
    skos:definition "Voids include all empty spaces in the soil. They are related to the arrangement of the primary soil constituents, rooting patterns, burrowing of animals or any other soil-forming processes, such as cracking, translocation and leaching. See more in Guidelines for Soil Description issued by the FAO: table 62" ;
    skos:note "This code list provides possible values for voidsDiameter."@en ;
    skos:prefLabel "Code list for voidsDiameterValue - codelist scheme"@en .

glosis_cl:waterRetentionPropertyCode a skos:ConceptScheme ;
    rdfs:label "Code list for waterRetentionProperty - codelist scheme"@en ;
    rdfs:seeAlso glosis_cl:WaterRetentionPropertyCode ;
    skos:definition "ISRIC Report 2019/01: Tier 1 and Tier 2 data in the context of the federated Global Soil Information System. Appendix 3" ;
    skos:note "This code list provides possible values for waterRetention."@en ;
    skos:prefLabel "Code list for waterRetentionProperty - codelist scheme"@en .

glosis_cl:weatherConditionsValueCode a skos:ConceptScheme ;
    rdfs:label "Code list for weatherConditionsValue - codelist scheme"@en ;
    rdfs:seeAlso glosis_cl:WeatherConditionsValueCode ;
    skos:definition "Codes for weather conditions.See in Guidelines for Soil Description issued by the FAO: table 2" ;
    skos:note "This code list provides possible values for weatherConditions."@en ;
    skos:prefLabel "Code list for weatherConditionsValue - codelist scheme"@en .

glosis_cl:weatheringValueCode a skos:ConceptScheme ;
    rdfs:label "Code list for weatheringValue - codelist scheme"@en ;
    rdfs:seeAlso glosis_cl:WeatheringValueCode ;
    skos:definition "Classification of weathering of coarse fragments. See more in Guidelines for Soil Description issued by the FAO: table 29" ;
    skos:note "This code list provides possible values for weathering."@en ;
    skos:prefLabel "Code list for weatheringValue - codelist scheme"@en .

glosis_cl:BiologicalAbundanceValueCode a owl:Class ;
    rdfs:label "Code list for BiologicalAbundanceValue - codelist class"@en ;
    rdfs:comment "This code list provides the BiologicalAbundanceValue codes."@en ;
    rdfs:seeAlso glosis_cl:biologicalAbundanceValueCode ;
    rdfs:subClassOf skos:Concept ;
    owl:oneOf ( glosis_cl:biologicalAbundanceValueCode-C glosis_cl:biologicalAbundanceValueCode-M glosis_cl:biologicalAbundanceValueCode-F glosis_cl:biologicalAbundanceValueCode-N ) ;
    skos:definition "Classification of the abundance of biological activity. See more in Guidelines for Soil Description issued by the FAO: table 81" .

glosis_cl:BiologicalFeaturesValueCode a owl:Class ;
    rdfs:label "Code list for BiologicalFeaturesValue - codelist class"@en ;
    rdfs:comment "This code list provides the BiologicalFeaturesValue codes."@en ;
    rdfs:seeAlso glosis_cl:biologicalFeaturesValueCode ;
    rdfs:subClassOf skos:Concept ;
    owl:oneOf ( glosis_cl:biologicalFeaturesValueCode-BO glosis_cl:biologicalFeaturesValueCode-BI glosis_cl:biologicalFeaturesValueCode-T glosis_cl:biologicalFeaturesValueCode-P glosis_cl:biologicalFeaturesValueCode-E glosis_cl:biologicalFeaturesValueCode-C glosis_cl:biologicalFeaturesValueCode-A glosis_cl:biologicalFeaturesValueCode-B glosis_cl:biologicalFeaturesValueCode-I ) ;
    skos:definition "Examples of biological features. See more in Guidelines for Soil Description issued by the FAO: table 82" .

glosis_cl:BleachedSandValueCode a owl:Class ;
    rdfs:label "Code list for BleachedSandValue - codelist class"@en ;
    rdfs:comment "This code list provides the BleachedSandValue codes."@en ;
    rdfs:seeAlso glosis_cl:bleachedSandValueCode ;
    rdfs:subClassOf skos:Concept ;
    owl:oneOf ( glosis_cl:bleachedSandValueCode-4 glosis_cl:bleachedSandValueCode-1 glosis_cl:bleachedSandValueCode-2 glosis_cl:bleachedSandValueCode-3 glosis_cl:bleachedSandValueCode-0 ) ;
    skos:definition "Classification of bleached sand characteristics based on the percentage of surface covered. See more in Guidelines for Soil Description issued by the FAO: table 23" .

glosis_cl:BoundaryClassificationValueCode a owl:Class ;
    rdfs:label "Code list for BoundaryClassificationValue - codelist class"@en ;
    rdfs:comment "This code list provides the BoundaryClassificationValue codes."@en ;
    rdfs:seeAlso glosis_cl:boundaryClassificationValueCode ;
    rdfs:subClassOf skos:Concept ;
    owl:oneOf ( glosis_cl:boundaryClassificationValueCode-C glosis_cl:boundaryClassificationValueCode-S glosis_cl:boundaryClassificationValueCode-D ) ;
    skos:definition "The boundary between mottle and matrix is described as the thickness of the zone within which the colour transition can be located without being in either the mottle or matrix. See more in guidelines for Soil Description issued by the FAO: table 35" .

glosis_cl:BoundaryDistinctnessValueCode a owl:Class ;
    rdfs:label "Code list for BoundaryDistinctnessValue - codelist class"@en ;
    rdfs:comment "This code list provides the BoundaryDistinctnessValue codes."@en ;
    rdfs:seeAlso glosis_cl:boundaryDistinctnessValueCode ;
    rdfs:subClassOf skos:Concept ;
    owl:oneOf ( glosis_cl:boundaryDistinctnessValueCode-C glosis_cl:boundaryDistinctnessValueCode-D glosis_cl:boundaryDistinctnessValueCode-A glosis_cl:boundaryDistinctnessValueCode-G ) ;
    skos:definition "The distinctness of the boundary refers to the thickness of the zone in which the horizon boundary can be located without being in one of the adjacent horizons. See more in the  Guidelines for Soil Description issued by the FAO: table 24.1" .

glosis_cl:BoundaryTopographyValueCode a owl:Class ;
    rdfs:label "Code list for BoundaryTopographyValue - codelist class"@en ;
    rdfs:comment "This code list provides the BoundaryTopographyValue codes."@en ;
    rdfs:seeAlso glosis_cl:boundaryTopographyValueCode ;
    rdfs:subClassOf skos:Concept ;
    owl:oneOf ( glosis_cl:boundaryTopographyValueCode-W glosis_cl:boundaryTopographyValueCode-I glosis_cl:boundaryTopographyValueCode-B glosis_cl:boundaryTopographyValueCode-S ) ;
    skos:definition "Classification of horizon boundaries by topography. See more in Guidelines for Soil Description issued by the FAO: table 24,2" .

glosis_cl:BulkDensityMineralValueCode a owl:Class ;
    rdfs:label "Code list for BulkDensityMineralValue - codelist class"@en ;
    rdfs:comment "This code list provides the BulkDensityMineralValue codes."@en ;
    rdfs:seeAlso glosis_cl:bulkDensityMineralValueCode ;
    rdfs:subClassOf skos:Concept ;
    owl:oneOf ( glosis_cl:bulkDensityMineralValueCode-BD3 glosis_cl:bulkDensityMineralValueCode-BD4 glosis_cl:bulkDensityMineralValueCode-BD2 glosis_cl:bulkDensityMineralValueCode-BD5 glosis_cl:bulkDensityMineralValueCode-BD1 ) ;
    skos:definition "Field determinations of bulk density may be obtained by estimating the force required to push a knife into a soil horizon exposed at a field moist pit wall. See more in Guidelines for Soil Description issued by the FAO: table 58" .

glosis_cl:BulkDensityPeatValueCode a owl:Class ;
    rdfs:label "Code list for BulkDensityPeatValue - codelist class"@en ;
    rdfs:comment "This code list provides the BulkDensityPeatValue codes."@en ;
    rdfs:seeAlso glosis_cl:bulkDensityPeatValueCode ;
    rdfs:subClassOf skos:Concept ;
    owl:oneOf ( glosis_cl:bulkDensityPeatValueCode-BD5 glosis_cl:bulkDensityPeatValueCode-BD4 glosis_cl:bulkDensityPeatValueCode-BD1 glosis_cl:bulkDensityPeatValueCode-BD3 glosis_cl:bulkDensityPeatValueCode-BD2 ) ;
    skos:definition "Bulk density and volume of solids of organic soils can be estimated after the decomposition stage or the extent of peat drainage. See more in guidelines for Soil Description issued by the FAO: table 59,3" .

glosis_cl:CarbonatesContentValueCode a owl:Class ;
    rdfs:label "Code list for CarbonatesContentValue - codelist class"@en ;
    rdfs:comment "This code list provides the CarbonatesContentValue codes."@en ;
    rdfs:seeAlso glosis_cl:carbonatesContentValueCode ;
    rdfs:subClassOf skos:Concept ;
    owl:oneOf ( glosis_cl:carbonatesContentValueCode-MO glosis_cl:carbonatesContentValueCode-N glosis_cl:carbonatesContentValueCode-ST glosis_cl:carbonatesContentValueCode-EX glosis_cl:carbonatesContentValueCode-SL ) ;
    skos:definition "Classes for the reaction of carbonates in the soil matrix. See more in Guidelines for Soil Description issued by the FAO: table 38" .

glosis_cl:CarbonatesFormsValueCode a owl:Class ;
    rdfs:label "Code list for CarbonatesFormsValue - codelist class"@en ;
    rdfs:comment "This code list provides the CarbonatesFormsValue codes."@en ;
    rdfs:seeAlso glosis_cl:carbonatesFormsValueCode ;
    rdfs:subClassOf skos:Concept ;
    owl:oneOf ( glosis_cl:carbonatesFormsValueCode-HHC glosis_cl:carbonatesFormsValueCode-HL glosis_cl:carbonatesFormsValueCode-PM glosis_cl:carbonatesFormsValueCode-D glosis_cl:carbonatesFormsValueCode-M glosis_cl:carbonatesFormsValueCode-SC glosis_cl:carbonatesFormsValueCode-HC ) ;
    skos:definition "The forms of secondary carbonates in soils are diverse and are considered to be informative for diagnostics of soil genesis. See more in guidelines for Soil Description issued by the FAO: table 39" .

glosis_cl:CementationContinuityValueCode a owl:Class ;
    rdfs:label "Code list for CementationContinuityValue - codelist class"@en ;
    rdfs:comment "This code list provides the CementationContinuityValue codes."@en ;
    rdfs:seeAlso glosis_cl:cementationContinuityValueCode ;
    rdfs:subClassOf skos:Concept ;
    owl:oneOf ( glosis_cl:cementationContinuityValueCode-C glosis_cl:cementationContinuityValueCode-B glosis_cl:cementationContinuityValueCode-D ) ;
    skos:definition "The occurrence of cementation or compaction in pans or otherwise is described according to its nature, continuity, structure, agent and degree. See more in the guidelines for Soil Description issued by the FAO: table 69" .

glosis_cl:CementationDegreeValueCode a owl:Class ;
    rdfs:label "Code list for CementationDegreeValue - codelist class"@en ;
    rdfs:comment "This code list provides the CementationDegreeValue codes."@en ;
    rdfs:seeAlso glosis_cl:cementationDegreeValueCode ;
    rdfs:subClassOf skos:Concept ;
    owl:oneOf ( glosis_cl:cementationDegreeValueCode-N glosis_cl:cementationDegreeValueCode-I glosis_cl:cementationDegreeValueCode-Y glosis_cl:cementationDegreeValueCode-M glosis_cl:cementationDegreeValueCode-C glosis_cl:cementationDegreeValueCode-W ) ;
    skos:definition "The classification of the degree of cementation/compaction. See more in Guidelines for Soil Description issued by the FAO: table 72" .

glosis_cl:CementationFabricValueCode a owl:Class ;
    rdfs:label "Code list for CementationFabricValue - codelist class"@en ;
    rdfs:comment "This code list provides the CementationFabricValue codes."@en ;
    rdfs:seeAlso glosis_cl:cementationFabricValueCode ;
    rdfs:subClassOf skos:Concept ;
    owl:oneOf ( glosis_cl:cementationFabricValueCode-Pi glosis_cl:cementationFabricValueCode-Pl glosis_cl:cementationFabricValueCode-D glosis_cl:cementationFabricValueCode-V ) ;
    skos:definition "Classification of the fabric of the cemented/compacted layer. See more in Guidelines for Soil Description issued by the FAO: table 70" .

glosis_cl:CementationNatureValueCode a owl:Class ;
    rdfs:label "Code list for CementationNatureValue - codelist class"@en ;
    rdfs:comment "This code list provides the CementationNatureValue codes."@en ;
    rdfs:seeAlso glosis_cl:cementationNatureValueCode ;
    rdfs:subClassOf skos:Concept ;
    owl:oneOf ( glosis_cl:cementationNatureValueCode-Q glosis_cl:cementationNatureValueCode-CS glosis_cl:cementationNatureValueCode-C glosis_cl:cementationNatureValueCode-F glosis_cl:cementationNatureValueCode-I glosis_cl:cementationNatureValueCode-GY glosis_cl:cementationNatureValueCode-FO glosis_cl:cementationNatureValueCode-FM glosis_cl:cementationNatureValueCode-NK glosis_cl:cementationNatureValueCode-P glosis_cl:cementationNatureValueCode-K glosis_cl:cementationNatureValueCode-KQ glosis_cl:cementationNatureValueCode-M ) ;
    skos:definition "Classification of the nature of cementation/compaction. See more in Guidelines for Soil Description issued by the FAO: table 71" .

glosis_cl:ClayPropertyCode a owl:Class ;
    rdfs:label "Code list for ClayProperty - codelist class"@en ;
    rdfs:comment "This code list provides the ClayProperty codes."@en ;
    rdfs:seeAlso glosis_cl:clayPropertyCode ;
    rdfs:subClassOf skos:Concept,
        sosa:ObservableProperty ;
    owl:oneOf ( glosis_cl:clayPropertyCode-CC glosis_cl:clayPropertyCode-CNC glosis_cl:clayPropertyCode-CWT ) ;
    skos:definition "ISRIC Report 2019/01: Tier 1 and Tier 2 data in the context of the federated Global Soil Information System. Appendix 3" .

glosis_cl:CoatingAbundanceValueCode a owl:Class ;
    rdfs:label "Code list for CoatingAbundanceValue - codelist class"@en ;
    rdfs:comment "This code list provides the CoatingAbundanceValue codes."@en ;
    rdfs:seeAlso glosis_cl:coatingAbundanceValueCode ;
    rdfs:subClassOf skos:Concept ;
    owl:oneOf ( glosis_cl:coatingAbundanceValueCode-A glosis_cl:coatingAbundanceValueCode-M glosis_cl:coatingAbundanceValueCode-D glosis_cl:coatingAbundanceValueCode-F glosis_cl:coatingAbundanceValueCode-V glosis_cl:coatingAbundanceValueCode-C glosis_cl:coatingAbundanceValueCode-N ) ;
    skos:definition "Classification of abundance of coatings. See more in Guidelines for Soil Description issued by the FAO: table 64" .

glosis_cl:CoatingContrastValueCode a owl:Class ;
    rdfs:label "Code list for CoatingContrastValue - codelist class"@en ;
    rdfs:comment "This code list provides the CoatingContrastValue codes."@en ;
    rdfs:seeAlso glosis_cl:coatingContrastValueCode ;
    rdfs:subClassOf skos:Concept ;
    owl:oneOf ( glosis_cl:coatingContrastValueCode-F glosis_cl:coatingContrastValueCode-P glosis_cl:coatingContrastValueCode-D ) ;
    skos:definition "Classification of the contrast of coatings. See more in Guidelines for Soil Description issued by the FAO: table 65" .

glosis_cl:CoatingFormValueCode a owl:Class ;
    rdfs:label "Code list for CoatingFormValue - codelist class"@en ;
    rdfs:comment "This code list provides the CoatingFormValue codes."@en ;
    rdfs:seeAlso glosis_cl:coatingFormValueCode ;
    rdfs:subClassOf skos:Concept ;
    owl:oneOf ( glosis_cl:coatingFormValueCode-O glosis_cl:coatingFormValueCode-DI glosis_cl:coatingFormValueCode-DC glosis_cl:coatingFormValueCode-CI glosis_cl:coatingFormValueCode-C glosis_cl:coatingFormValueCode-DE ) ;
    skos:definition "Classification of the form of coatings. See more in Guidelines for Soil Description issued by the FAO: table 67" .

glosis_cl:CoatingLocationValueCode a owl:Class ;
    rdfs:label "Code list for CoatingLocationValue - codelist class"@en ;
    rdfs:comment "This code list provides the CoatingLocationValue codes."@en ;
    rdfs:seeAlso glosis_cl:coatingLocationValueCode ;
    rdfs:subClassOf skos:Concept ;
    owl:oneOf ( glosis_cl:coatingLocationValueCode-LA glosis_cl:coatingLocationValueCode-PH glosis_cl:coatingLocationValueCode-PV glosis_cl:coatingLocationValueCode-BR glosis_cl:coatingLocationValueCode-CF glosis_cl:coatingLocationValueCode-P glosis_cl:coatingLocationValueCode-VO glosis_cl:coatingLocationValueCode-NS ) ;
    skos:definition "Classification of the location of coatings and clay accumulation. See more in Guidelines for Soil Description issued by the FAO: table 68" .

glosis_cl:CoatingNatureValueCode a owl:Class ;
    rdfs:label "Code list for CoatingNatureValue - codelist class"@en ;
    rdfs:comment "This code list provides the CoatingNatureValue codes."@en ;
    rdfs:seeAlso glosis_cl:coatingNatureValueCode ;
    rdfs:subClassOf skos:Concept ;
    owl:oneOf ( glosis_cl:coatingNatureValueCode-C glosis_cl:coatingNatureValueCode-CC glosis_cl:coatingNatureValueCode-CS glosis_cl:coatingNatureValueCode-SP glosis_cl:coatingNatureValueCode-SF glosis_cl:coatingNatureValueCode-HC glosis_cl:coatingNatureValueCode-S glosis_cl:coatingNatureValueCode-SL glosis_cl:coatingNatureValueCode-MN glosis_cl:coatingNatureValueCode-PF glosis_cl:coatingNatureValueCode-GB glosis_cl:coatingNatureValueCode-CH glosis_cl:coatingNatureValueCode-JA glosis_cl:coatingNatureValueCode-ST glosis_cl:coatingNatureValueCode-SN glosis_cl:coatingNatureValueCode-SI glosis_cl:coatingNatureValueCode-SA glosis_cl:coatingNatureValueCode-H ) ;
    skos:definition "Classification of the nature of coatings. See more in Guidelines for Soil Description issued by the FAO: table 66" .

glosis_cl:ConsistenceDryValueCode a owl:Class ;
    rdfs:label "Code list for ConsistenceDryValue - codelist class"@en ;
    rdfs:comment "This code list provides the ConsistenceDryValue codes."@en ;
    rdfs:seeAlso glosis_cl:consistenceDryValueCode ;
    rdfs:subClassOf skos:Concept ;
    owl:oneOf ( glosis_cl:consistenceDryValueCode-HA glosis_cl:consistenceDryValueCode-HVH glosis_cl:consistenceDryValueCode-VHA glosis_cl:consistenceDryValueCode-SSH glosis_cl:consistenceDryValueCode-SO glosis_cl:consistenceDryValueCode-LO glosis_cl:consistenceDryValueCode-SHH glosis_cl:consistenceDryValueCode-SHA glosis_cl:consistenceDryValueCode-EHA ) ;
    skos:definition "The consistence when dry is determined by breaking an air-dried mass of soil between thumb and forefinger or in the hand. See more in the guidelines for Soil Description issued by the FAO: table 53" .

glosis_cl:ConsistenceMoistValueCode a owl:Class ;
    rdfs:label "Code list for ConsistenceMoistValue - codelist class"@en ;
    rdfs:comment "This code list provides the ConsistenceMoistValue codes."@en ;
    rdfs:seeAlso glosis_cl:consistenceMoistValueCode ;
    rdfs:subClassOf skos:Concept ;
    owl:oneOf ( glosis_cl:consistenceMoistValueCode-LO glosis_cl:consistenceMoistValueCode-EFI glosis_cl:consistenceMoistValueCode-FI glosis_cl:consistenceMoistValueCode-VFR glosis_cl:consistenceMoistValueCode-VFI glosis_cl:consistenceMoistValueCode-FR ) ;
    skos:definition "Guidelines for Soil Description issued by the FAO: table 54;Consistence when moist is determined by attempting to crush a mass of moist or slightly moist soil material. See more in Guidelines for Soil Description issued by the FAO: table 54" .

glosis_cl:ContrastValueCode a owl:Class ;
    rdfs:label "Code list for ContrastValue - codelist class"@en ;
    rdfs:comment "This code list provides the ContrastValue codes."@en ;
    rdfs:seeAlso glosis_cl:contrastValueCode ;
    rdfs:subClassOf skos:Concept ;
    owl:oneOf ( glosis_cl:contrastValueCode-D glosis_cl:contrastValueCode-F glosis_cl:contrastValueCode-P ) ;
    skos:definition "The colour contrast between mottles and soil matrix. See more in Guidelines for Soil Description issued by the FAO: table 34" .

glosis_cl:CracksDepthValueCode a owl:Class ;
    rdfs:label "Code list for CracksDepthValue - codelist class"@en ;
    rdfs:comment "This code list provides the CracksDepthValue codes."@en ;
    rdfs:seeAlso glosis_cl:cracksDepthValueCode ;
    rdfs:subClassOf skos:Concept ;
    owl:oneOf ( glosis_cl:cracksDepthValueCode-D glosis_cl:cracksDepthValueCode-M glosis_cl:cracksDepthValueCode-S glosis_cl:cracksDepthValueCode-V ) ;
    skos:definition "List of suggested classes of surface cracks in shrink–swell clay-rich soils after they dry out. See more in guidelines for Soil Description issued by the FAO: table 21,2" .

glosis_cl:CracksDistanceValueCode a owl:Class ;
    rdfs:label "Code list for CracksDistanceValue - codelist class"@en ;
    rdfs:comment "This code list provides the CracksDistanceValue codes."@en ;
    rdfs:seeAlso glosis_cl:cracksDistanceValueCode ;
    rdfs:subClassOf skos:Concept ;
    owl:oneOf ( glosis_cl:cracksDistanceValueCode-D glosis_cl:cracksDistanceValueCode-V glosis_cl:cracksDistanceValueCode-C glosis_cl:cracksDistanceValueCode-W glosis_cl:cracksDistanceValueCode-M ) ;
    skos:definition "Classification of the surface cracks based on distance between the cracks measured in meters. See more in Guidelines for Soil Description issued by the FAO: table 21,3" .

glosis_cl:CracksWidthValueCode a owl:Class ;
    rdfs:label "Code list for CracksWidthValue - codelist class"@en ;
    rdfs:comment "This code list provides the CracksWidthValue codes."@en ;
    rdfs:seeAlso glosis_cl:cracksWidthValueCode ;
    rdfs:subClassOf skos:Concept ;
    owl:oneOf ( glosis_cl:cracksWidthValueCode-F glosis_cl:cracksWidthValueCode-M glosis_cl:cracksWidthValueCode-W glosis_cl:cracksWidthValueCode-V glosis_cl:cracksWidthValueCode-E ) ;
    skos:definition "Classification of surface cracks based on the width. See more in Guidelines for Soil Description issued by the FAO: table 21,1" .

glosis_cl:CropClassValueCode a owl:Class ;
    rdfs:label "Code list for CropClassValue - codelist class"@en ;
    rdfs:comment "This code list provides the CropClassValue codes."@en ;
    rdfs:seeAlso glosis_cl:cropClassValueCode ;
    rdfs:subClassOf skos:Concept ;
    owl:oneOf ( glosis_cl:cropClassValueCode-Ce_Ba glosis_cl:cropClassValueCode-Fr glosis_cl:cropClassValueCode-Lu_Te glosis_cl:cropClassValueCode-Ce_Ri glosis_cl:cropClassValueCode-Fo_Pu glosis_cl:cropClassValueCode-Ro_Po glosis_cl:cropClassValueCode-Fr_Me glosis_cl:cropClassValueCode-Oi_Su glosis_cl:cropClassValueCode-Ce_Wh glosis_cl:cropClassValueCode-Lu_Cc glosis_cl:cropClassValueCode-Ce glosis_cl:cropClassValueCode-Lu_Co glosis_cl:cropClassValueCode-Ot_Sc glosis_cl:cropClassValueCode-Fr_Ma glosis_cl:cropClassValueCode-Pu_Le glosis_cl:cropClassValueCode-Fo_Ma glosis_cl:cropClassValueCode-Oi_Se glosis_cl:cropClassValueCode-Ro_Ca glosis_cl:cropClassValueCode-Pu_Be glosis_cl:cropClassValueCode-Fr_Ba glosis_cl:cropClassValueCode-Ro glosis_cl:cropClassValueCode-Pu glosis_cl:cropClassValueCode-Ce_So glosis_cl:cropClassValueCode-Lu glosis_cl:cropClassValueCode-Ce_Ry glosis_cl:cropClassValueCode-Oi_So glosis_cl:cropClassValueCode-Fo_Ha glosis_cl:cropClassValueCode-Lu_To glosis_cl:cropClassValueCode-Ve glosis_cl:cropClassValueCode-Fo_Le glosis_cl:cropClassValueCode-Fr_Ap glosis_cl:cropClassValueCode-Oi_Op glosis_cl:cropClassValueCode-Fi_Ju glosis_cl:cropClassValueCode-Fr_Ci glosis_cl:cropClassValueCode-Ol glosis_cl:cropClassValueCode-Ot_Pa glosis_cl:cropClassValueCode-Oi_Li glosis_cl:cropClassValueCode-Oi_Gr glosis_cl:cropClassValueCode-Fo_Gr glosis_cl:cropClassValueCode-Ot_Ru glosis_cl:cropClassValueCode-Oi_Cc glosis_cl:cropClassValueCode-Ro_Su glosis_cl:cropClassValueCode-Ce_Mi glosis_cl:cropClassValueCode-Fo glosis_cl:cropClassValueCode-Fo_Cl glosis_cl:cropClassValueCode-Ce_Oa glosis_cl:cropClassValueCode-Ce_Pa glosis_cl:cropClassValueCode-Fr_Gr glosis_cl:cropClassValueCode-Fi_Co glosis_cl:cropClassValueCode-Fi glosis_cl:cropClassValueCode-Ro_Ya glosis_cl:cropClassValueCode-Ot glosis_cl:cropClassValueCode-Oi_Ra glosis_cl:cropClassValueCode-Oi glosis_cl:cropClassValueCode-Ce_Ma glosis_cl:cropClassValueCode-Pu_Pe glosis_cl:cropClassValueCode-Fo_Al ) ;
    skos:definition "Examples for the most common crops with their recommended codes. See more in guidelines for Soil Description issued by the FAO: table 9" .

glosis_cl:ErosionActivityPeriodValueCode a owl:Class ;
    rdfs:label "Code list for ErosionActivityPeriodValue - codelist class"@en ;
    rdfs:comment "This code list provides the ErosionActivityPeriodValue codes."@en ;
    rdfs:seeAlso glosis_cl:erosionActivityPeriodValueCode ;
    rdfs:subClassOf skos:Concept ;
    owl:oneOf ( glosis_cl:erosionActivityPeriodValueCode-N glosis_cl:erosionActivityPeriodValueCode-X glosis_cl:erosionActivityPeriodValueCode-A glosis_cl:erosionActivityPeriodValueCode-H glosis_cl:erosionActivityPeriodValueCode-R ) ;
    skos:definition "The period of activity of accelerated erosion or deposition is described using the recommended classes. See more in Guidelines for Soil Description issued by the FAO: table 19" .

glosis_cl:ErosionAreaAffectedValueCode a owl:Class ;
    rdfs:label "Code list for ErosionAreaAffectedValue - codelist class"@en ;
    rdfs:comment "This code list provides the ErosionAreaAffectedValue codes."@en ;
    rdfs:seeAlso glosis_cl:erosionAreaAffectedValueCode ;
    rdfs:subClassOf skos:Concept ;
    owl:oneOf ( glosis_cl:erosionAreaAffectedValueCode-5 glosis_cl:erosionAreaAffectedValueCode-4 glosis_cl:erosionAreaAffectedValueCode-2 glosis_cl:erosionAreaAffectedValueCode-1 glosis_cl:erosionAreaAffectedValueCode-3 glosis_cl:erosionAreaAffectedValueCode-0 ) ;
    skos:definition "Classification of total area affected by erosion and deposition. See more in Guidelines for Soil Description issued by the FAO: table 17" .

glosis_cl:ErosionCategoryValueCode a owl:Class ;
    rdfs:label "Code list for ErosionCategoryValue - codelist class"@en ;
    rdfs:comment "This code list provides the ErosionCategoryValue codes."@en ;
    rdfs:seeAlso glosis_cl:erosionCategoryValueCode ;
    rdfs:subClassOf skos:Concept ;
    owl:oneOf ( glosis_cl:erosionCategoryValueCode-WD glosis_cl:erosionCategoryValueCode-M glosis_cl:erosionCategoryValueCode-AM glosis_cl:erosionCategoryValueCode-WG glosis_cl:erosionCategoryValueCode-WA glosis_cl:erosionCategoryValueCode-A glosis_cl:erosionCategoryValueCode-NK glosis_cl:erosionCategoryValueCode-AZ glosis_cl:erosionCategoryValueCode-WS glosis_cl:erosionCategoryValueCode-AD glosis_cl:erosionCategoryValueCode-WT glosis_cl:erosionCategoryValueCode-AS glosis_cl:erosionCategoryValueCode-N glosis_cl:erosionCategoryValueCode-WR glosis_cl:erosionCategoryValueCode-W ) ;
    skos:definition "Erosion can be classified as water or wind erosion and include off-site effects such as deposition; a third major category is mass movements (landslides and related phenomena). See more in Guidelines for Soil Description issued by the FAO: table 16" .

glosis_cl:ErosionDegreeValueCode a owl:Class ;
    rdfs:label "Code list for ErosionDegreeValue - codelist class"@en ;
    rdfs:comment "This code list provides the ErosionDegreeValue codes."@en ;
    rdfs:seeAlso glosis_cl:erosionDegreeValueCode ;
    rdfs:subClassOf skos:Concept ;
    owl:oneOf ( glosis_cl:erosionDegreeValueCode-S glosis_cl:erosionDegreeValueCode-V glosis_cl:erosionDegreeValueCode-E glosis_cl:erosionDegreeValueCode-M ) ;
    skos:definition "Classification of erosion, by degree. See more in guidelines for Soil Description issued by the FAO: table 18" .

glosis_cl:ErosionTotalAreaAffectedValueCode a owl:Class ;
    rdfs:label "Code list for ErosionTotalAreaAffectedValue - codelist class"@en ;
    rdfs:comment "This code list provides the ErosionTotalAreaAffectedValue codes."@en ;
    rdfs:seeAlso glosis_cl:erosionTotalAreaAffectedValueCode ;
    rdfs:subClassOf skos:Concept ;
    owl:oneOf ( glosis_cl:erosionTotalAreaAffectedValueCode-4 glosis_cl:erosionTotalAreaAffectedValueCode-0 glosis_cl:erosionTotalAreaAffectedValueCode-2 glosis_cl:erosionTotalAreaAffectedValueCode-1 glosis_cl:erosionTotalAreaAffectedValueCode-5 glosis_cl:erosionTotalAreaAffectedValueCode-3 ) ;
    skos:definition "The total area affected by erosion and deposition is estimated following the classes defined by SOTER (FAO, 1995). See more in the Guidelines for Soil Description issued by the FAO: table 17" .

glosis_cl:FloodDurationValueCode a owl:Class ;
    rdfs:label "Code list for FloodDurationValue - codelist class"@en ;
    rdfs:comment "This code list provides the FloodDurationValue codes."@en ;
    rdfs:seeAlso glosis_cl:floodDurationValueCode ;
    rdfs:subClassOf skos:Concept ;
    skos:definition "Related to the amount of time an area remains inundated by floodwater.  This metric is important because it helps assess the extent of waterlogging and its impact on soil properties, particularly in terms of oxygen availability and soil aeration. Flood duration affects the mobility of nutrients and contaminants within the soil, influencing both agricultural productivity and environmental quality. Longer flood durations can also lead to changes in soil texture and structure due to the continuous movement and deposition of particles during inundation​. Source: Guidance for Flood Risk Analysis and Mapping" .

glosis_cl:FloodFrequencyValueCode a owl:Class ;
    rdfs:label "Code list for FloodFrequencyValue - codelist class"@en ;
    rdfs:comment "This code list provides the FloodFrequencyValue codes."@en ;
    rdfs:seeAlso glosis_cl:floodFrequencyValueCode ;
    rdfs:subClassOf skos:Concept ;
    skos:definition "Refers to the statistical analysis of the occurrence of floods at a particular location over a defined time period. It often involves calculating the recurrence intervals or return periods of flood events, which are typically used to understand how often a specific flood magnitude (like a 100-year flood) is likely to occur. Source: Introduction to Flood Frequency Analysis" .

glosis_cl:FragmentCoverValueCode a owl:Class ;
    rdfs:label "Code list for FragmentCoverValue - codelist class"@en ;
    rdfs:comment "This code list provides the FragmentCoverValue codes."@en ;
    rdfs:seeAlso glosis_cl:fragmentCoverValueCode ;
    rdfs:subClassOf skos:Concept ;
    owl:oneOf ( glosis_cl:fragmentCoverValueCode-A glosis_cl:fragmentCoverValueCode-D glosis_cl:fragmentCoverValueCode-C glosis_cl:fragmentCoverValueCode-M glosis_cl:fragmentCoverValueCode-N glosis_cl:fragmentCoverValueCode-F glosis_cl:fragmentCoverValueCode-V ) ;
    skos:definition "Coarse surface fragments, including those partially exposed, should be described in terms of percentage of surface coverage and of size of the fragments. See more in Guidelines for Soil Description issued by the FAO: table 15,1" .

glosis_cl:FragmentsClassValueCode a owl:Class ;
    rdfs:label "Code list for FragmentsClassValue - codelist class"@en ;
    rdfs:comment "This code list provides the FragmentsClassValue codes."@en ;
    rdfs:seeAlso glosis_cl:fragmentsClassValueCode ;
    rdfs:subClassOf skos:Concept ;
    owl:oneOf ( glosis_cl:fragmentsClassValueCode-FGF3 glosis_cl:fragmentsClassValueCode-FVE glosis_cl:fragmentsClassValueCode-FV2 glosis_cl:fragmentsClassValueCode-FV3 glosis_cl:fragmentsClassValueCode-FGT glosis_cl:fragmentsClassValueCode-FGF2 glosis_cl:fragmentsClassValueCode-FGF1 glosis_cl:fragmentsClassValueCode-FV1 glosis_cl:fragmentsClassValueCode-FGF4 glosis_cl:fragmentsClassValueCode-FVT ) ;
    skos:definition "Horizon properties encountered in a global data compilation programme. See more in ISRIC Report 2019/01: Tier 1 and Tier 2 data in the context of the federated Global Soil Information System. Appendix 3" .

glosis_cl:FragmentsSizeValueCode a owl:Class ;
    rdfs:label "Code list for FragmentsSizeValue - codelist class"@en ;
    rdfs:comment "This code list provides the FragmentsSizeValue codes."@en ;
    rdfs:seeAlso glosis_cl:fragmentsSizeValueCode ;
    rdfs:subClassOf skos:Concept ;
    owl:oneOf ( glosis_cl:fragmentsSizeValueCode-B glosis_cl:fragmentsSizeValueCode-M glosis_cl:fragmentsSizeValueCode-F glosis_cl:fragmentsSizeValueCode-C glosis_cl:fragmentsSizeValueCode-S glosis_cl:fragmentsSizeValueCode-L ) ;
    skos:definition "Classes of occurrence of coarse surface fragments are correlated with the ones for rock outcrop. See more in guidelines for Soil Description issued by the FAO: table 15,2" .

glosis_cl:GypsumContentValueCode a owl:Class ;
    rdfs:label "Code list for GypsumContentValue - codelist class"@en ;
    rdfs:comment "This code list provides the GypsumContentValue codes."@en ;
    rdfs:seeAlso glosis_cl:gypsumContentValueCode ;
    rdfs:subClassOf skos:Concept ;
    owl:oneOf ( glosis_cl:gypsumContentValueCode-MO glosis_cl:gypsumContentValueCode-EX glosis_cl:gypsumContentValueCode-SL glosis_cl:gypsumContentValueCode-ST glosis_cl:gypsumContentValueCode-N ) ;
    skos:definition "Where more readily soluble salts are absent, gypsum can be estimated in the field by measurements of electrical conductivity. More in the guidelines for Soil Description issued by the FAO: table 40" .

glosis_cl:GypsumFormsValueCode a owl:Class ;
    rdfs:label "Code list for GypsumFormsValue - codelist class"@en ;
    rdfs:comment "This code list provides the GypsumFormsValue codes."@en ;
    rdfs:seeAlso glosis_cl:gypsumFormsValueCode ;
    rdfs:subClassOf skos:Concept ;
    owl:oneOf ( glosis_cl:gypsumFormsValueCode-SC glosis_cl:gypsumFormsValueCode-D glosis_cl:gypsumFormsValueCode-HL glosis_cl:gypsumFormsValueCode-G ) ;
    skos:definition "The forms of secondary gypsum in soils are diverse and are considered to be informative for diagnostics of soil genesis. See more information in the Guidelines for Soil Description issued by the FAO: table 41" .

glosis_cl:HumanInfluenceClassValueCode a owl:Class ;
    rdfs:label "Code list for HumanInfluenceClassValue - codelist class"@en ;
    rdfs:comment "This code list provides the HumanInfluenceClassValue codes."@en ;
    rdfs:seeAlso glosis_cl:humanInfluenceClassValueCode ;
    rdfs:subClassOf skos:Concept ;
    owl:oneOf ( glosis_cl:humanInfluenceClassValueCode-SA glosis_cl:humanInfluenceClassValueCode-AC glosis_cl:humanInfluenceClassValueCode-N glosis_cl:humanInfluenceClassValueCode-CR glosis_cl:humanInfluenceClassValueCode-BP glosis_cl:humanInfluenceClassValueCode-CL glosis_cl:humanInfluenceClassValueCode-PL glosis_cl:humanInfluenceClassValueCode-DU glosis_cl:humanInfluenceClassValueCode-VM glosis_cl:humanInfluenceClassValueCode-ID glosis_cl:humanInfluenceClassValueCode-IF glosis_cl:humanInfluenceClassValueCode-MI glosis_cl:humanInfluenceClassValueCode-MS glosis_cl:humanInfluenceClassValueCode-VU glosis_cl:humanInfluenceClassValueCode-PO glosis_cl:humanInfluenceClassValueCode-MR glosis_cl:humanInfluenceClassValueCode-TE glosis_cl:humanInfluenceClassValueCode-NK glosis_cl:humanInfluenceClassValueCode-ME glosis_cl:humanInfluenceClassValueCode-AD glosis_cl:humanInfluenceClassValueCode-LF glosis_cl:humanInfluenceClassValueCode-IS glosis_cl:humanInfluenceClassValueCode-VS glosis_cl:humanInfluenceClassValueCode-LV glosis_cl:humanInfluenceClassValueCode-BR glosis_cl:humanInfluenceClassValueCode-IB glosis_cl:humanInfluenceClassValueCode-MU glosis_cl:humanInfluenceClassValueCode-BU glosis_cl:humanInfluenceClassValueCode-IP glosis_cl:humanInfluenceClassValueCode-IU glosis_cl:humanInfluenceClassValueCode-MO glosis_cl:humanInfluenceClassValueCode-MP glosis_cl:humanInfluenceClassValueCode-SC glosis_cl:humanInfluenceClassValueCode-FE glosis_cl:humanInfluenceClassValueCode-VE ) ;
    skos:definition "This item refers to any evidence of human activity that is likely to have affected the landscape or the physical and chemical properties of the soil. See more in the Guidelines for Soil Description issued by the FAO: table 10" .

glosis_cl:LandUseClassValueCode a owl:Class ;
    rdfs:label "Code list for LandUseClassValue - codelist class"@en ;
    rdfs:comment "This code list provides the LandUseClassValue codes."@en ;
    rdfs:seeAlso glosis_cl:landUseClassValueCode ;
    rdfs:subClassOf skos:Concept ;
    owl:oneOf ( glosis_cl:landUseClassValueCode-S glosis_cl:landUseClassValueCode-AT2 glosis_cl:landUseClassValueCode-H glosis_cl:landUseClassValueCode-PD glosis_cl:landUseClassValueCode-AA1 glosis_cl:landUseClassValueCode-PN glosis_cl:landUseClassValueCode-MP glosis_cl:landUseClassValueCode-U glosis_cl:landUseClassValueCode-AT3 glosis_cl:landUseClassValueCode-AA glosis_cl:landUseClassValueCode-HE3 glosis_cl:landUseClassValueCode-FN1 glosis_cl:landUseClassValueCode-SD glosis_cl:landUseClassValueCode-SC glosis_cl:landUseClassValueCode-HE1 glosis_cl:landUseClassValueCode-AP1 glosis_cl:landUseClassValueCode-Y glosis_cl:landUseClassValueCode-AA2 glosis_cl:landUseClassValueCode-HI1 glosis_cl:landUseClassValueCode-MF glosis_cl:landUseClassValueCode-AT4 glosis_cl:landUseClassValueCode-HE glosis_cl:landUseClassValueCode-FP glosis_cl:landUseClassValueCode-AA4 glosis_cl:landUseClassValueCode-FN2 glosis_cl:landUseClassValueCode-AT1 glosis_cl:landUseClassValueCode-A glosis_cl:landUseClassValueCode-PN1 glosis_cl:landUseClassValueCode-HI2 glosis_cl:landUseClassValueCode-Oi glosis_cl:landUseClassValueCode-AT glosis_cl:landUseClassValueCode-AP2 glosis_cl:landUseClassValueCode-AA5 glosis_cl:landUseClassValueCode-PD1 glosis_cl:landUseClassValueCode-PN2 glosis_cl:landUseClassValueCode-AA3 glosis_cl:landUseClassValueCode-SR glosis_cl:landUseClassValueCode-ST glosis_cl:landUseClassValueCode-M glosis_cl:landUseClassValueCode-PD2 glosis_cl:landUseClassValueCode-AA6 glosis_cl:landUseClassValueCode-F glosis_cl:landUseClassValueCode-SI glosis_cl:landUseClassValueCode-FN glosis_cl:landUseClassValueCode-HE2 glosis_cl:landUseClassValueCode-PN3 glosis_cl:landUseClassValueCode-AP glosis_cl:landUseClassValueCode-HI glosis_cl:landUseClassValueCode-SX glosis_cl:landUseClassValueCode-P ) ;
    skos:definition "Land use applies to the current use of the land, whether agricultural or nonagricultural, in which the soil is located. See more in the guidelines for Soil Description issued by the FAO: table 8" .

glosis_cl:LandformComplexValueCode a owl:Class ;
    rdfs:label "Code list for LandformComplexValue - codelist class"@en ;
    rdfs:comment "This code list provides the LandformComplexValue codes."@en ;
    rdfs:seeAlso glosis_cl:landformComplexValueCode ;
    rdfs:subClassOf skos:Concept ;
    owl:oneOf ( glosis_cl:landformComplexValueCode-DU glosis_cl:landformComplexValueCode-RI glosis_cl:landformComplexValueCode-CU glosis_cl:landformComplexValueCode-KA glosis_cl:landformComplexValueCode-WE glosis_cl:landformComplexValueCode-IM glosis_cl:landformComplexValueCode-TE glosis_cl:landformComplexValueCode-DO glosis_cl:landformComplexValueCode-IN ) ;
    skos:definition "Subdivisions for complex landforms. See more in Guidelines for Soil Description issued by the FAO: table 5" .

glosis_cl:LithologyValueCode a owl:Class ;
    rdfs:label "Code list for LithologyValue - codelist class"@en ;
    rdfs:comment "This code list provides the LithologyValue codes."@en ;
    rdfs:seeAlso glosis_cl:lithologyValueCode ;
    rdfs:subClassOf skos:Concept ;
    owl:oneOf ( glosis_cl:lithologyValueCode-IU glosis_cl:lithologyValueCode-IP1 glosis_cl:lithologyValueCode-IP glosis_cl:lithologyValueCode-UO glosis_cl:lithologyValueCode-UK2 glosis_cl:lithologyValueCode-I glosis_cl:lithologyValueCode-UE glosis_cl:lithologyValueCode-SC3 glosis_cl:lithologyValueCode-UF2 glosis_cl:lithologyValueCode-UR glosis_cl:lithologyValueCode-UU4 glosis_cl:lithologyValueCode-MU glosis_cl:lithologyValueCode-IA2 glosis_cl:lithologyValueCode-SC5 glosis_cl:lithologyValueCode-UG2 glosis_cl:lithologyValueCode-MA glosis_cl:lithologyValueCode-UG1 glosis_cl:lithologyValueCode-UM glosis_cl:lithologyValueCode-IA1 glosis_cl:lithologyValueCode-UU1 glosis_cl:lithologyValueCode-MB3 glosis_cl:lithologyValueCode-II1 glosis_cl:lithologyValueCode-UA glosis_cl:lithologyValueCode-UC1 glosis_cl:lithologyValueCode-SO2 glosis_cl:lithologyValueCode-UU5 glosis_cl:lithologyValueCode-IB1 glosis_cl:lithologyValueCode-IA glosis_cl:lithologyValueCode-IA4 glosis_cl:lithologyValueCode-MB2 glosis_cl:lithologyValueCode-IU2 glosis_cl:lithologyValueCode-UF1 glosis_cl:lithologyValueCode-SC4 glosis_cl:lithologyValueCode-MA3 glosis_cl:lithologyValueCode-UC glosis_cl:lithologyValueCode-UE2 glosis_cl:lithologyValueCode-IP2 glosis_cl:lithologyValueCode-MB glosis_cl:lithologyValueCode-UE1 glosis_cl:lithologyValueCode-IB3 glosis_cl:lithologyValueCode-SC2 glosis_cl:lithologyValueCode-IP4 glosis_cl:lithologyValueCode-IU1 glosis_cl:lithologyValueCode-UL glosis_cl:lithologyValueCode-MB5 glosis_cl:lithologyValueCode-MA1 glosis_cl:lithologyValueCode-UU3 glosis_cl:lithologyValueCode-UK glosis_cl:lithologyValueCode-UL1 glosis_cl:lithologyValueCode-UO1 glosis_cl:lithologyValueCode-UK1 glosis_cl:lithologyValueCode-UG3 glosis_cl:lithologyValueCode-SO3 glosis_cl:lithologyValueCode-UA1 glosis_cl:lithologyValueCode-UO2 glosis_cl:lithologyValueCode-UR1 glosis_cl:lithologyValueCode-SE glosis_cl:lithologyValueCode-SC1 glosis_cl:lithologyValueCode-IA3 glosis_cl:lithologyValueCode-UM1 glosis_cl:lithologyValueCode-MB4 glosis_cl:lithologyValueCode-UM2 glosis_cl:lithologyValueCode-SE1 glosis_cl:lithologyValueCode-SO1 glosis_cl:lithologyValueCode-SE2 glosis_cl:lithologyValueCode-MA2 glosis_cl:lithologyValueCode-UF glosis_cl:lithologyValueCode-IP3 glosis_cl:lithologyValueCode-UU2 glosis_cl:lithologyValueCode-UA2 glosis_cl:lithologyValueCode-UU glosis_cl:lithologyValueCode-MB1 glosis_cl:lithologyValueCode-UG glosis_cl:lithologyValueCode-SC glosis_cl:lithologyValueCode-II glosis_cl:lithologyValueCode-U glosis_cl:lithologyValueCode-MU1 glosis_cl:lithologyValueCode-UL2 glosis_cl:lithologyValueCode-IB2 glosis_cl:lithologyValueCode-IU3 glosis_cl:lithologyValueCode-S glosis_cl:lithologyValueCode-UC2 glosis_cl:lithologyValueCode-IB glosis_cl:lithologyValueCode-MA4 glosis_cl:lithologyValueCode-MB6 glosis_cl:lithologyValueCode-II2 glosis_cl:lithologyValueCode-M glosis_cl:lithologyValueCode-SO ) ;
    skos:definition "In order to be able to work in smaller scales, some additional natural and anthropogenic parent materials are used for the identification of rocks  in the field, the keys to the most important rock types are provided in the hierarchical SOTER list. See more in the guidelines for Soil Description issued by the FAO: table 12" .

glosis_cl:MajorLandFormValueCode a owl:Class ;
    rdfs:label "Code list for MajorLandFormValue - codelist class"@en ;
    rdfs:comment "This code list provides the MajorLandFormValue codes."@en ;
    rdfs:seeAlso glosis_cl:majorLandFormValueCode ;
    rdfs:subClassOf skos:Concept ;
    owl:oneOf ( glosis_cl:majorLandFormValueCode-LP glosis_cl:majorLandFormValueCode-TV glosis_cl:majorLandFormValueCode-LD glosis_cl:majorLandFormValueCode-SM glosis_cl:majorLandFormValueCode-T glosis_cl:majorLandFormValueCode-TH glosis_cl:majorLandFormValueCode-TE glosis_cl:majorLandFormValueCode-LV glosis_cl:majorLandFormValueCode-L glosis_cl:majorLandFormValueCode-SH glosis_cl:majorLandFormValueCode-SE glosis_cl:majorLandFormValueCode-LL glosis_cl:majorLandFormValueCode-TM glosis_cl:majorLandFormValueCode-S glosis_cl:majorLandFormValueCode-SP glosis_cl:majorLandFormValueCode-SV ) ;
    skos:definition "Hierarchy of major landforms. See more in Guidelines for Soil Description issued by the FAO: table 4" .

glosis_cl:MineralConcColourValueCode a owl:Class ;
    rdfs:label "Code list for MineralConcColourValue - codelist class"@en ;
    rdfs:comment "This code list provides the MineralConcColourValue codes."@en ;
    rdfs:seeAlso glosis_cl:mineralConcColourValueCode ;
    rdfs:subClassOf skos:Concept ;
    owl:oneOf ( glosis_cl:mineralConcColourValueCode-BS glosis_cl:mineralConcColourValueCode-RY glosis_cl:mineralConcColourValueCode-BL glosis_cl:mineralConcColourValueCode-WH glosis_cl:mineralConcColourValueCode-YR glosis_cl:mineralConcColourValueCode-GS glosis_cl:mineralConcColourValueCode-YB glosis_cl:mineralConcColourValueCode-BB glosis_cl:mineralConcColourValueCode-MC glosis_cl:mineralConcColourValueCode-GR glosis_cl:mineralConcColourValueCode-GE glosis_cl:mineralConcColourValueCode-RS glosis_cl:mineralConcColourValueCode-RB glosis_cl:mineralConcColourValueCode-BR glosis_cl:mineralConcColourValueCode-BU glosis_cl:mineralConcColourValueCode-RE glosis_cl:mineralConcColourValueCode-YE ) ;
    skos:definition "The general colour names are usually sufficient to describe the colour of the nodules (similar to mottles) or of artefacts. See more in Guidelines for Soil Description issued by the FAO: table 78" .

glosis_cl:MineralConcHardnessValueCode a owl:Class ;
    rdfs:label "Code list for MineralConcHardnessValue - codelist class"@en ;
    rdfs:comment "This code list provides the MineralConcHardnessValue codes."@en ;
    rdfs:seeAlso glosis_cl:mineralConcHardnessValueCode ;
    rdfs:subClassOf skos:Concept ;
    owl:oneOf ( glosis_cl:mineralConcHardnessValueCode-S glosis_cl:mineralConcHardnessValueCode-B glosis_cl:mineralConcHardnessValueCode-H ) ;
    skos:definition "Classification of the hardness of mineral concentrations. More in the Guidelines for Soil Description issued by the FAO: table 76" .

glosis_cl:MineralConcKindValueCode a owl:Class ;
    rdfs:label "Code list for MineralConcKindValue - codelist class"@en ;
    rdfs:comment "This code list provides the MineralConcKindValue codes."@en ;
    rdfs:seeAlso glosis_cl:mineralConcKindValueCode ;
    rdfs:subClassOf skos:Concept ;
    owl:oneOf ( glosis_cl:mineralConcKindValueCode-SC glosis_cl:mineralConcKindValueCode-IC glosis_cl:mineralConcKindValueCode-R glosis_cl:mineralConcKindValueCode-O glosis_cl:mineralConcKindValueCode-IP glosis_cl:mineralConcKindValueCode-N glosis_cl:mineralConcKindValueCode-T glosis_cl:mineralConcKindValueCode-S glosis_cl:mineralConcKindValueCode-C ) ;
    skos:definition "Classification of the kinds of mineral concentrations. See more in guidelines for Soil Description issued by the FAO: table 74" .

glosis_cl:MineralConcNatureValueCode a owl:Class ;
    rdfs:label "Code list for MineralConcNatureValue - codelist class"@en ;
    rdfs:comment "This code list provides the MineralConcNatureValue codes."@en ;
    rdfs:seeAlso glosis_cl:mineralConcNatureValueCode ;
    rdfs:subClassOf skos:Concept ;
    owl:oneOf ( glosis_cl:mineralConcNatureValueCode-KQ glosis_cl:mineralConcNatureValueCode-FM glosis_cl:mineralConcNatureValueCode-F glosis_cl:mineralConcNatureValueCode-NK glosis_cl:mineralConcNatureValueCode-SA glosis_cl:mineralConcNatureValueCode-S glosis_cl:mineralConcNatureValueCode-CS glosis_cl:mineralConcNatureValueCode-Q glosis_cl:mineralConcNatureValueCode-GB glosis_cl:mineralConcNatureValueCode-C glosis_cl:mineralConcNatureValueCode-M glosis_cl:mineralConcNatureValueCode-K glosis_cl:mineralConcNatureValueCode-GY glosis_cl:mineralConcNatureValueCode-JA ) ;
    skos:definition "Mineral concentrations are described according to the composition or impregnating substance.See more in Guidelines for Soil Description issued by the FAO: 77" .

glosis_cl:MineralConcShapeValueCode a owl:Class ;
    rdfs:label "Code list for MineralConcShapeValue - codelist class"@en ;
    rdfs:comment "This code list provides the MineralConcShapeValue codes."@en ;
    rdfs:seeAlso glosis_cl:mineralConcShapeValueCode ;
    rdfs:subClassOf skos:Concept ;
    owl:oneOf ( glosis_cl:mineralConcShapeValueCode-R glosis_cl:mineralConcShapeValueCode-E glosis_cl:mineralConcShapeValueCode-A glosis_cl:mineralConcShapeValueCode-I glosis_cl:mineralConcShapeValueCode-F ) ;
    skos:definition "Classification of the size and shape of mineral concentrations. See more in Guidelines for Soil Description issued by the FAO: table 75,2" .

glosis_cl:MineralConcSizeValueCode a owl:Class ;
    rdfs:label "Code list for MineralConcSizeValue - codelist class"@en ;
    rdfs:comment "This code list provides the MineralConcSizeValue codes."@en ;
    rdfs:seeAlso glosis_cl:mineralConcSizeValueCode ;
    rdfs:subClassOf skos:Concept ;
    owl:oneOf ( glosis_cl:mineralConcSizeValueCode-V glosis_cl:mineralConcSizeValueCode-C glosis_cl:mineralConcSizeValueCode-F glosis_cl:mineralConcSizeValueCode-M ) ;
    skos:definition "Classification of mineral concentrations based on size. See more in Guidelines for Soil Description issued by the FAO: table 75,1" .

glosis_cl:MineralConcVolumeValueCode a owl:Class ;
    rdfs:label "Code list for MineralConcVolumeValue - codelist class"@en ;
    rdfs:comment "This code list provides the MineralConcVolumeValue codes."@en ;
    rdfs:seeAlso glosis_cl:mineralConcVolumeValueCode ;
    rdfs:subClassOf skos:Concept ;
    owl:oneOf ( glosis_cl:mineralConcVolumeValueCode-C glosis_cl:mineralConcVolumeValueCode-F glosis_cl:mineralConcVolumeValueCode-V glosis_cl:mineralConcVolumeValueCode-N glosis_cl:mineralConcVolumeValueCode-M glosis_cl:mineralConcVolumeValueCode-A glosis_cl:mineralConcVolumeValueCode-D ) ;
    skos:definition "The mineral concentrations are described according to their abundance, kind, size, shape, hardness, nature and colour. See more onGuidelines for Soil Description issued by the FAO: table 73" .

glosis_cl:MineralFragmentsValueCode a owl:Class ;
    rdfs:label "Code list for MineralFragmentsValue - codelist class"@en ;
    rdfs:comment "This code list provides the MineralFragmentsValue codes."@en ;
    rdfs:seeAlso glosis_cl:mineralFragmentsValueCode ;
    rdfs:subClassOf skos:Concept ;
    owl:oneOf ( glosis_cl:mineralFragmentsValueCode-QU glosis_cl:mineralFragmentsValueCode-FE glosis_cl:mineralFragmentsValueCode-MI ) ;
    skos:definition "Codes for primary mineral fragments. See more in Guidelines for Soil Description issued by the FAO: table 30" .

glosis_cl:MottlesAbundanceValueCode a owl:Class ;
    rdfs:label "Code list for MottlesAbundanceValue - codelist class"@en ;
    rdfs:comment "This code list provides the MottlesAbundanceValue codes."@en ;
    rdfs:seeAlso glosis_cl:mottlesAbundanceValueCode ;
    rdfs:subClassOf skos:Concept ;
    owl:oneOf ( glosis_cl:mottlesAbundanceValueCode-N glosis_cl:mottlesAbundanceValueCode-M glosis_cl:mottlesAbundanceValueCode-C glosis_cl:mottlesAbundanceValueCode-V glosis_cl:mottlesAbundanceValueCode-A glosis_cl:mottlesAbundanceValueCode-F ) ;
    skos:definition "The abundance of mottles is described in terms of classes indicating the percentage of the exposed surface that the mottles occupy. See more in the Guidelines for Soil Description issued by the FAO: table 32" .

glosis_cl:MottlesSizeValueCode a owl:Class ;
    rdfs:label "Code list for MottlesSizeValue - codelist class"@en ;
    rdfs:comment "This code list provides the MottlesSizeValue codes."@en ;
    rdfs:seeAlso glosis_cl:mottlesSizeValueCode ;
    rdfs:subClassOf skos:Concept ;
    owl:oneOf ( glosis_cl:mottlesSizeValueCode-M glosis_cl:mottlesSizeValueCode-A glosis_cl:mottlesSizeValueCode-F glosis_cl:mottlesSizeValueCode-V ) ;
    skos:definition "The individual classes of the mottle nodules according to their diameter size. See more in the guidelines for Soil Description issued by the FAO: table 33" .

glosis_cl:OrganicMatterClassValueCode a owl:Class ;
    rdfs:label "Code list for OrganicMatterClassValue - codelist class"@en ;
    rdfs:comment "This code list provides the OrganicMatterClassValue codes."@en ;
    rdfs:seeAlso glosis_cl:organicMatterClassValueCode ;
    rdfs:subClassOf skos:Concept ;
    skos:definition "Refers to the categorization or classification of soil based on the quality, quantity, and composition of organic matter present, influencing soil properties such as fertility, water retention, and microbial activity. Source: Source: FAO, Soil Organic Matter and Soil Health, Land and Water Development Division." .

glosis_cl:PeatDecompostionValueCode a owl:Class ;
    rdfs:label "Code list for PeatDecompostionValue - codelist class"@en ;
    rdfs:comment "This code list provides the PeatDecompostionValue codes."@en ;
    rdfs:seeAlso glosis_cl:peatDecompostionValueCode ;
    rdfs:subClassOf skos:Concept ;
    owl:oneOf ( glosis_cl:peatDecompostionValueCode-Fibric glosis_cl:peatDecompostionValueCode-Hemic glosis_cl:peatDecompostionValueCode-D3 glosis_cl:peatDecompostionValueCode-Sapric glosis_cl:peatDecompostionValueCode-D5.2 glosis_cl:peatDecompostionValueCode-D4 glosis_cl:peatDecompostionValueCode-D5.1 glosis_cl:peatDecompostionValueCode-D2 glosis_cl:peatDecompostionValueCode-D1 ) ;
    skos:definition "In most organic layers of rocks the determination of the texture class is done by estimating of the degree of decomposition and humification of the organic material.See more in Guidelines for Soil Description issued by the FAO: table 31" .

glosis_cl:PeatDrainageValueCode a owl:Class ;
    rdfs:label "Code list for PeatDrainageValue - codelist class"@en ;
    rdfs:comment "This code list provides the PeatDrainageValue codes."@en ;
    rdfs:seeAlso glosis_cl:peatDrainageValueCode ;
    rdfs:subClassOf skos:Concept ;
    owl:oneOf ( glosis_cl:peatDrainageValueCode-DC4 glosis_cl:peatDrainageValueCode-DC3 glosis_cl:peatDrainageValueCode-DC2 glosis_cl:peatDrainageValueCode-DC1 ) ;
    skos:definition "Bulk density and volume of solids of organic soils may be estimated after the decomposition stage or the extent of peat drainage. More information is in the guidelines for Soil Description issued by the FAO: table 59,1" .

glosis_cl:PeatVolumeValueCode a owl:Class ;
    rdfs:label "Code list for PeatVolumeValue - codelist class"@en ;
    rdfs:comment "This code list provides the PeatVolumeValue codes."@en ;
    rdfs:seeAlso glosis_cl:peatVolumeValueCode ;
    rdfs:subClassOf skos:Concept ;
    owl:oneOf ( glosis_cl:peatVolumeValueCode-SV2 glosis_cl:peatVolumeValueCode-SV5 glosis_cl:peatVolumeValueCode-SV1 glosis_cl:peatVolumeValueCode-SV3 glosis_cl:peatVolumeValueCode-SV4 ) ;
    skos:definition "Field estimation of volume of solids and bulk density of peat soils. See more in Guidelines for Soil Description issued by the FAO: table 59,2" .

glosis_cl:PhysioChemicalPropertyCode a owl:Class ;
    rdfs:label "Code list for PhysioChemicalProperty - codelist class"@en ;
    rdfs:comment "This code list provides the PhysioChemicalProperty codes."@en ;
    rdfs:seeAlso glosis_cl:physioChemicalPropertyCode ;
    rdfs:subClassOf skos:Concept,
        sosa:ObservableProperty ;
    owl:oneOf ( glosis_cl:physioChemicalPropertyCode-Alusat glosis_cl:physioChemicalPropertyCode-Mandit glosis_cl:physioChemicalPropertyCode-Irodit glosis_cl:physioChemicalPropertyCode-Aluext glosis_cl:physioChemicalPropertyCode-Gyp glosis_cl:physioChemicalPropertyCode-Pottot glosis_cl:physioChemicalPropertyCode-Photot glosis_cl:physioChemicalPropertyCode-Basexc glosis_cl:physioChemicalPropertyCode-Bassum glosis_cl:physioChemicalPropertyCode-Aluoxa glosis_cl:physioChemicalPropertyCode-CaN glosis_cl:physioChemicalPropertyCode-Manpyr glosis_cl:physioChemicalPropertyCode-ManKCl glosis_cl:physioChemicalPropertyCode-Mol glosis_cl:physioChemicalPropertyCode-pH glosis_cl:physioChemicalPropertyCode-Manext glosis_cl:physioChemicalPropertyCode-Borext glosis_cl:physioChemicalPropertyCode-Sul glosis_cl:physioChemicalPropertyCode-Brot glosis_cl:physioChemicalPropertyCode-Calsol glosis_cl:physioChemicalPropertyCode-Sulext glosis_cl:physioChemicalPropertyCode-Alu glosis_cl:physioChemicalPropertyCode-Por glosis_cl:physioChemicalPropertyCode-Copext glosis_cl:physioChemicalPropertyCode-Irotot glosis_cl:physioChemicalPropertyCode-Aluexc glosis_cl:physioChemicalPropertyCode-Cartot glosis_cl:physioChemicalPropertyCode-Car glosis_cl:physioChemicalPropertyCode-Hyd glosis_cl:physioChemicalPropertyCode-Magext glosis_cl:physioChemicalPropertyCode-Caltot glosis_cl:physioChemicalPropertyCode-Phoret glosis_cl:physioChemicalPropertyCode-Aciexc glosis_cl:physioChemicalPropertyCode-Carpyr glosis_cl:physioChemicalPropertyCode-Potexc glosis_cl:physioChemicalPropertyCode-Avavol glosis_cl:physioChemicalPropertyCode-Cad glosis_cl:physioChemicalPropertyCode-Nittot glosis_cl:physioChemicalPropertyCode-Hydcond glosis_cl:physioChemicalPropertyCode-Nit2 glosis_cl:physioChemicalPropertyCode-Ccetot glosis_cl:physioChemicalPropertyCode-Siloxa glosis_cl:physioChemicalPropertyCode-Aciext glosis_cl:physioChemicalPropertyCode-Selext glosis_cl:physioChemicalPropertyCode-Hydexc glosis_cl:physioChemicalPropertyCode-Irooxa glosis_cl:physioChemicalPropertyCode-Seltot glosis_cl:physioChemicalPropertyCode-BulDwhole glosis_cl:physioChemicalPropertyCode-Sodexc glosis_cl:physioChemicalPropertyCode-Magtot glosis_cl:physioChemicalPropertyCode-Carhum glosis_cl:physioChemicalPropertyCode-Calext glosis_cl:physioChemicalPropertyCode-Potsol glosis_cl:physioChemicalPropertyCode-Eleccond glosis_cl:physioChemicalPropertyCode-Iropyr glosis_cl:physioChemicalPropertyCode-Carorg glosis_cl:physioChemicalPropertyCode-Cartoh glosis_cl:physioChemicalPropertyCode-Calfra glosis_cl:physioChemicalPropertyCode-Carinorg glosis_cl:physioChemicalPropertyCode-Sodsol glosis_cl:physioChemicalPropertyCode-Alutot glosis_cl:physioChemicalPropertyCode-BulDfine glosis_cl:physioChemicalPropertyCode-Sodexp glosis_cl:physioChemicalPropertyCode-Sultot glosis_cl:physioChemicalPropertyCode-Zin glosis_cl:physioChemicalPropertyCode-Bascal glosis_cl:physioChemicalPropertyCode-Phooxa glosis_cl:physioChemicalPropertyCode-Manoxa glosis_cl:physioChemicalPropertyCode-Pho glosis_cl:physioChemicalPropertyCode-Magexc glosis_cl:physioChemicalPropertyCode-Solsal glosis_cl:physioChemicalPropertyCode-Calexc glosis_cl:physioChemicalPropertyCode-Carful glosis_cl:physioChemicalPropertyCode-Potext glosis_cl:physioChemicalPropertyCode-Brod glosis_cl:physioChemicalPropertyCode-Aludit glosis_cl:physioChemicalPropertyCode-Zinext glosis_cl:physioChemicalPropertyCode-Iroext glosis_cl:physioChemicalPropertyCode-Sodext glosis_cl:physioChemicalPropertyCode-Alupyr glosis_cl:physioChemicalPropertyCode-CEC glosis_cl:physioChemicalPropertyCode-Chl glosis_cl:physioChemicalPropertyCode-Bortot glosis_cl:physioChemicalPropertyCode-Nit3 glosis_cl:physioChemicalPropertyCode-Orgmat glosis_cl:physioChemicalPropertyCode-Sodtot glosis_cl:physioChemicalPropertyCode-Phoext glosis_cl:physioChemicalPropertyCode-Mantot glosis_cl:physioChemicalPropertyCode-Coptot glosis_cl:physioChemicalPropertyCode-ECEC glosis_cl:physioChemicalPropertyCode-Magsol ) ;
    skos:definition "ISRIC Report 2019/01: Tier 1 and Tier 2 data in the context of the federated Global Soil Information System. Appendix 3;ISRIC Report 2014/01: Africa Soil Profiles Database Version 1.2. Annex 3a" .

glosis_cl:PhysiographyValueCode a owl:Class ;
    rdfs:label "Code list for PhysiographyValue - codelist class"@en ;
    rdfs:comment "This code list provides the PhysiographyValue codes."@en ;
    rdfs:seeAlso glosis_cl:physiographyValueCode ;
    rdfs:subClassOf skos:Concept ;
    owl:oneOf ( glosis_cl:physiographyValueCode-HI glosis_cl:physiographyValueCode-MS glosis_cl:physiographyValueCode-LO glosis_cl:physiographyValueCode-IN glosis_cl:physiographyValueCode-TS glosis_cl:physiographyValueCode-UP glosis_cl:physiographyValueCode-LS glosis_cl:physiographyValueCode-CR glosis_cl:physiographyValueCode-BOdl glosis_cl:physiographyValueCode-BOf ) ;
    skos:definition "The relative position of the site within the land should be indicated. The position affects the hydrological conditions of the site. See more in the Guidelines for Soil Description issued by the FAO: figure 2" .

glosis_cl:PlasticityValueCode a owl:Class ;
    rdfs:label "Code list for PlasticityValue - codelist class"@en ;
    rdfs:comment "This code list provides the PlasticityValue codes."@en ;
    rdfs:seeAlso glosis_cl:plasticityValueCode ;
    rdfs:subClassOf skos:Concept ;
    owl:oneOf ( glosis_cl:plasticityValueCode-PL glosis_cl:plasticityValueCode-PVP glosis_cl:plasticityValueCode-SPP glosis_cl:plasticityValueCode-NPL glosis_cl:plasticityValueCode-VPL glosis_cl:plasticityValueCode-SPL ) ;
    skos:definition "Plasticity is the ability of soil material to change shape continuously under the influence of an applied stress and to retain the compressed shape on removal of stress. See more in Guidelines for Soil Description issued by the FAO: Guidelines for Soil Description issued by the FAO: table 56" .

glosis_cl:PoresAbundanceValueCode a owl:Class ;
    rdfs:label "Code list for PoresAbundanceValue - codelist class"@en ;
    rdfs:comment "This code list provides the PoresAbundanceValue codes."@en ;
    rdfs:seeAlso glosis_cl:poresAbundanceValueCode ;
    rdfs:subClassOf skos:Concept ;
    owl:oneOf ( glosis_cl:poresAbundanceValueCode-F glosis_cl:poresAbundanceValueCode-N glosis_cl:poresAbundanceValueCode-V glosis_cl:poresAbundanceValueCode-M glosis_cl:poresAbundanceValueCode-C ) ;
    skos:definition "Classification of abundance of pores. See more in Guidelines for Soil Description issued by the FAO: table 63" .

glosis_cl:PorosityClassValueCode a owl:Class ;
    rdfs:label "Code list for PorosityClassValue - codelist class"@en ;
    rdfs:comment "This code list provides the PorosityClassValue codes."@en ;
    rdfs:seeAlso glosis_cl:porosityClassValueCode ;
    rdfs:subClassOf skos:Concept ;
    owl:oneOf ( glosis_cl:porosityClassValueCode-1 glosis_cl:porosityClassValueCode-3 glosis_cl:porosityClassValueCode-4 glosis_cl:porosityClassValueCode-2 glosis_cl:porosityClassValueCode-5 ) ;
    skos:definition "The porosity is an indication of the total volume of voids discernible with a ×10 hand-lens measured by area and recorded as the percentage of the surface occupied by pores. See more in guidelines for Soil Description issued by the FAO: table 60" .

glosis_cl:ProfileDescriptionStatusValueCode a owl:Class ;
    rdfs:label "Code list for ProfileDescriptionStatusValue - codelist class"@en ;
    rdfs:comment "This code list provides the ProfileDescriptionStatusValue codes."@en ;
    rdfs:seeAlso glosis_cl:profileDescriptionStatusValueCode ;
    rdfs:subClassOf skos:Concept ;
    owl:oneOf ( glosis_cl:profileDescriptionStatusValueCode-4.1 glosis_cl:profileDescriptionStatusValueCode-3.1 glosis_cl:profileDescriptionStatusValueCode-2 glosis_cl:profileDescriptionStatusValueCode-3 glosis_cl:profileDescriptionStatusValueCode-5 glosis_cl:profileDescriptionStatusValueCode-2.1 glosis_cl:profileDescriptionStatusValueCode-1 glosis_cl:profileDescriptionStatusValueCode-1.1 glosis_cl:profileDescriptionStatusValueCode-4 ) ;
    skos:definition "Soil profile description status. See more in Guidelines for Soil Description issued by the FAO: table 1" .

glosis_cl:RockAbundanceValueCode a owl:Class ;
    rdfs:label "Code list for RockAbundanceValue - codelist class"@en ;
    rdfs:comment "This code list provides the RockAbundanceValue codes."@en ;
    rdfs:seeAlso glosis_cl:rockAbundanceValueCode ;
    rdfs:subClassOf skos:Concept ;
    owl:oneOf ( glosis_cl:rockAbundanceValueCode-C glosis_cl:rockAbundanceValueCode-D glosis_cl:rockAbundanceValueCode-N glosis_cl:rockAbundanceValueCode-F glosis_cl:rockAbundanceValueCode-M glosis_cl:rockAbundanceValueCode-A glosis_cl:rockAbundanceValueCode-S glosis_cl:rockAbundanceValueCode-V ) ;
    skos:definition "Abundance of rock fragments and artefacts, by volume. See more in Guidelines for Soil Description issued by the FAO: table 26" .

glosis_cl:RockOutcropsCoverValueCode a owl:Class ;
    rdfs:label "Code list for RockOutcropsCoverValue - codelist class"@en ;
    rdfs:comment "This code list provides the RockOutcropsCoverValue codes."@en ;
    rdfs:seeAlso glosis_cl:rockOutcropsCoverValueCode ;
    rdfs:subClassOf skos:Concept ;
    owl:oneOf ( glosis_cl:rockOutcropsCoverValueCode-M glosis_cl:rockOutcropsCoverValueCode-C glosis_cl:rockOutcropsCoverValueCode-V glosis_cl:rockOutcropsCoverValueCode-A glosis_cl:rockOutcropsCoverValueCode-N glosis_cl:rockOutcropsCoverValueCode-F glosis_cl:rockOutcropsCoverValueCode-D ) ;
    skos:definition "Recommended classes of percentage of surface cover and of average distance between rock outcrops. See more in Guidelines for Soil Description issued by the FAO: table 14,1" .

glosis_cl:RockOutcropsDistanceValueCode a owl:Class ;
    rdfs:label "Code list for RockOutcropsDistanceValue - codelist class"@en ;
    rdfs:comment "This code list provides the RockOutcropsDistanceValue codes."@en ;
    rdfs:seeAlso glosis_cl:rockOutcropsDistanceValueCode ;
    rdfs:subClassOf skos:Concept ;
    owl:oneOf ( glosis_cl:rockOutcropsDistanceValueCode-3 glosis_cl:rockOutcropsDistanceValueCode-5 glosis_cl:rockOutcropsDistanceValueCode-1 glosis_cl:rockOutcropsDistanceValueCode-2 glosis_cl:rockOutcropsDistanceValueCode-4 ) ;
    skos:definition "Recommended classes of percentage of surface cover and of average distance between rock outcrops. See more in Guidelines for Soil Description issued by the FAO: table 14,2" .

glosis_cl:RockShapeValueCode a owl:Class ;
    rdfs:label "Code list for RockShapeValue - codelist class"@en ;
    rdfs:comment "This code list provides the RockShapeValue codes."@en ;
    rdfs:seeAlso glosis_cl:rockShapeValueCode ;
    rdfs:subClassOf skos:Concept ;
    owl:oneOf ( glosis_cl:rockShapeValueCode-A glosis_cl:rockShapeValueCode-S glosis_cl:rockShapeValueCode-R glosis_cl:rockShapeValueCode-F ) ;
    skos:definition "The general shape or roundness of rock fragments. See more on Guidelines for Soil Description issued by the FAO: table 28" .

glosis_cl:RockSizeValueCode a owl:Class ;
    rdfs:label "Code list for RockSizeValue - codelist class"@en ;
    rdfs:comment "This code list provides the RockSizeValue codes."@en ;
    rdfs:seeAlso glosis_cl:rockSizeValueCode ;
    rdfs:subClassOf skos:Concept ;
    owl:oneOf ( glosis_cl:rockSizeValueCode-A glosis_cl:rockSizeValueCode-AC glosis_cl:rockSizeValueCode-AM glosis_cl:rockSizeValueCode-R glosis_cl:rockSizeValueCode-RM glosis_cl:rockSizeValueCode-RL glosis_cl:rockSizeValueCode-BL glosis_cl:rockSizeValueCode-FM glosis_cl:rockSizeValueCode-C glosis_cl:rockSizeValueCode-SB glosis_cl:rockSizeValueCode-RB glosis_cl:rockSizeValueCode-AF glosis_cl:rockSizeValueCode-MC glosis_cl:rockSizeValueCode-RF glosis_cl:rockSizeValueCode-RC glosis_cl:rockSizeValueCode-AV glosis_cl:rockSizeValueCode-RS glosis_cl:rockSizeValueCode-CS ) ;
    skos:definition "Classification for rock fragments and artefacts influences the nutrient status, water movement, use and management of the soil. See more in guidelines for Soil Description issued by the FAO: table 27" .

glosis_cl:RootsAbundanceValueCode a owl:Class ;
    rdfs:label "Code list for RootsAbundanceValue - codelist class"@en ;
    rdfs:comment "This code list provides the RootsAbundanceValue codes."@en ;
    rdfs:seeAlso glosis_cl:rootsAbundanceValueCode ;
    rdfs:subClassOf skos:Concept ;
    owl:oneOf ( glosis_cl:rootsAbundanceValueCode-M glosis_cl:rootsAbundanceValueCode-F glosis_cl:rootsAbundanceValueCode-C glosis_cl:rootsAbundanceValueCode-V glosis_cl:rootsAbundanceValueCode-N ) ;
    skos:definition "classification of the abundance of roots.. See more in Guidelines for Soil Description issued by the FAO: table 80" .

glosis_cl:SaltContentValueCode a owl:Class ;
    rdfs:label "Code list for SaltContentValue - codelist class"@en ;
    rdfs:comment "This code list provides the SaltContentValue codes."@en ;
    rdfs:seeAlso glosis_cl:saltContentValueCode ;
    rdfs:subClassOf skos:Concept ;
    owl:oneOf ( glosis_cl:saltContentValueCode-EX glosis_cl:saltContentValueCode-SL glosis_cl:saltContentValueCode-N glosis_cl:saltContentValueCode-ST glosis_cl:saltContentValueCode-VST glosis_cl:saltContentValueCode-MO ) ;
    skos:definition "Classification of salt content of soil. See more in Guidelines for Soil Description issued by the FAO: table 42" .

glosis_cl:SaltCoverValueCode a owl:Class ;
    rdfs:label "Code list for SaltCoverValue - codelist class"@en ;
    rdfs:comment "This code list provides the SaltCoverValue codes."@en ;
    rdfs:seeAlso glosis_cl:saltCoverValueCode ;
    rdfs:subClassOf skos:Concept ;
    owl:oneOf ( glosis_cl:saltCoverValueCode-2 glosis_cl:saltCoverValueCode-1 glosis_cl:saltCoverValueCode-3 glosis_cl:saltCoverValueCode-0 glosis_cl:saltCoverValueCode-4 ) ;
    skos:definition "The occurrence of salt at the surface may be described in terms of cover, appearance and type of salt. See more in the guidelines for Soil Description issued by the FAO: table 22,1" .

glosis_cl:SaltThicknessValueCode a owl:Class ;
    rdfs:label "Code list for SaltThicknessValue - codelist class"@en ;
    rdfs:comment "This code list provides the SaltThicknessValue codes."@en ;
    rdfs:seeAlso glosis_cl:saltThicknessValueCode ;
    rdfs:subClassOf skos:Concept ;
    owl:oneOf ( glosis_cl:saltThicknessValueCode-N glosis_cl:saltThicknessValueCode-V glosis_cl:saltThicknessValueCode-F glosis_cl:saltThicknessValueCode-M glosis_cl:saltThicknessValueCode-C ) ;
    skos:definition "The occurrence of salt at the surface may be described in terms of cover, appearance and type of salt. See more in the Guidelines for Soil Description issued by the FAO: table 22,2" .

glosis_cl:SandPropertyCode a owl:Class ;
    rdfs:label "Code list for SandProperty - codelist class"@en ;
    rdfs:comment "This code list provides the SandProperty codes."@en ;
    rdfs:seeAlso glosis_cl:sandPropertyCode ;
    rdfs:subClassOf skos:Concept,
        sosa:ObservableProperty ;
    owl:oneOf ( glosis_cl:sandPropertyCode-SWD3 glosis_cl:sandPropertyCode-SWDT glosis_cl:sandPropertyCode-SWD2 glosis_cl:sandPropertyCode-SWD4 glosis_cl:sandPropertyCode-SWD1 glosis_cl:sandPropertyCode-SWD5 ) ;
    skos:definition "ISRIC Report 2019/01: Tier 1 and Tier 2 data in the context of the federated Global Soil Information System. Appendix 3" .

glosis_cl:SandyTextureValueCode a owl:Class ;
    rdfs:label "Code list for SandyTextureValue - codelist class"@en ;
    rdfs:comment "This code list provides the SandyTextureValue codes."@en ;
    rdfs:seeAlso glosis_cl:sandyTextureValueCode ;
    rdfs:subClassOf skos:Concept ;
    owl:oneOf ( glosis_cl:sandyTextureValueCode-FS glosis_cl:sandyTextureValueCode-LFS glosis_cl:sandyTextureValueCode-LCS glosis_cl:sandyTextureValueCode-MS glosis_cl:sandyTextureValueCode-CSL glosis_cl:sandyTextureValueCode-US glosis_cl:sandyTextureValueCode-CS glosis_cl:sandyTextureValueCode-FSL glosis_cl:sandyTextureValueCode-LVFS glosis_cl:sandyTextureValueCode-VFS ) ;
    skos:definition "Relation of constituents of fine earth by size, defining textural classes and sand subclasses. See more in Guidelines for Soil Description issued by the FAO: figure 4,3" .

glosis_cl:SealingConsistenceValueCode a owl:Class ;
    rdfs:label "Code list for SealingConsistenceValue - codelist class"@en ;
    rdfs:comment "This code list provides the SealingConsistenceValue codes."@en ;
    rdfs:seeAlso glosis_cl:sealingConsistenceValueCode ;
    rdfs:subClassOf skos:Concept ;
    owl:oneOf ( glosis_cl:sealingConsistenceValueCode-H glosis_cl:sealingConsistenceValueCode-V glosis_cl:sealingConsistenceValueCode-E glosis_cl:sealingConsistenceValueCode-S ) ;
    skos:definition "Classification of the attributes of surface sealing based on consistency. See more in Guidelines for Soil Description issued by the FAO: table 20,2" .

glosis_cl:SealingThicknessValueCode a owl:Class ;
    rdfs:label "Code list for SealingThicknessValue - codelist class"@en ;
    rdfs:comment "This code list provides the SealingThicknessValue codes."@en ;
    rdfs:seeAlso glosis_cl:sealingThicknessValueCode ;
    rdfs:subClassOf skos:Concept ;
    owl:oneOf ( glosis_cl:sealingThicknessValueCode-F glosis_cl:sealingThicknessValueCode-N glosis_cl:sealingThicknessValueCode-M glosis_cl:sealingThicknessValueCode-V glosis_cl:sealingThicknessValueCode-C ) ;
    skos:definition "Surface sealing is used to describe crusts that develop at the soil surface after the topsoil dries out. See more in Guidelines for Soil Description issued by the FAO: 20,1" .

glosis_cl:SiltPropertyCode a owl:Class ;
    rdfs:label "Code list for SiltProperty - codelist class"@en ;
    rdfs:comment "This code list provides the SiltProperty codes."@en ;
    rdfs:seeAlso glosis_cl:siltPropertyCode ;
    rdfs:subClassOf skos:Concept,
        sosa:ObservableProperty ;
    owl:oneOf ( glosis_cl:siltPropertyCode-SWDF2 glosis_cl:siltPropertyCode-SWDF1 glosis_cl:siltPropertyCode-SWDFT ) ;
    skos:definition "ISRIC Report 2019/01: Tier 1 and Tier 2 data in the context of the federated Global Soil Information System. Appendix 3" .

glosis_cl:SlopeFormValueCode a owl:Class ;
    rdfs:label "Code list for SlopeFormValue - codelist class"@en ;
    rdfs:comment "This code list provides the SlopeFormValue codes."@en ;
    rdfs:seeAlso glosis_cl:slopeFormValueCode ;
    rdfs:subClassOf skos:Concept ;
    owl:oneOf ( glosis_cl:slopeFormValueCode-T glosis_cl:slopeFormValueCode-S glosis_cl:slopeFormValueCode-X glosis_cl:slopeFormValueCode-C glosis_cl:slopeFormValueCode-V ) ;
    skos:definition "The slope form refers to the general shape of the slope in both the vertical and horizontal directions. See more in Guidelines for Soil Description issued by the FAO: table 6" .

glosis_cl:SlopeGradientClassValueCode a owl:Class ;
    rdfs:label "Code list for SlopeGradientClassValue - codelist class"@en ;
    rdfs:comment "This code list provides the SlopeGradientClassValue codes."@en ;
    rdfs:seeAlso glosis_cl:slopeGradientClassValueCode ;
    rdfs:subClassOf skos:Concept ;
    owl:oneOf ( glosis_cl:slopeGradientClassValueCode-10 glosis_cl:slopeGradientClassValueCode-7 glosis_cl:slopeGradientClassValueCode-5 glosis_cl:slopeGradientClassValueCode-3 glosis_cl:slopeGradientClassValueCode-4 glosis_cl:slopeGradientClassValueCode-6 glosis_cl:slopeGradientClassValueCode-1 glosis_cl:slopeGradientClassValueCode-2 glosis_cl:slopeGradientClassValueCode-9 glosis_cl:slopeGradientClassValueCode-8 ) ;
    skos:definition "Slope gradient classes measured on the percentage of slope. See more in Guidelines for Soil Description issued by the FAO: table 7" .

glosis_cl:SlopePathwaysValueCode a owl:Class ;
    rdfs:label "Code list for SlopePathwaysValue - codelist class"@en ;
    rdfs:comment "This code list provides the SlopePathwaysValue codes."@en ;
    rdfs:seeAlso glosis_cl:slopePathwaysValueCode ;
    rdfs:subClassOf skos:Concept ;
    owl:oneOf ( glosis_cl:slopePathwaysValueCode-VS glosis_cl:slopePathwaysValueCode-SC glosis_cl:slopePathwaysValueCode-VV glosis_cl:slopePathwaysValueCode-SV glosis_cl:slopePathwaysValueCode-CS glosis_cl:slopePathwaysValueCode-VC glosis_cl:slopePathwaysValueCode-CV glosis_cl:slopePathwaysValueCode-SS glosis_cl:slopePathwaysValueCode-CC ) ;
    skos:definition "The slope form refers to the general shape of the slope in both the vertical and horizontal directions. See more in guidelines for Soil Description issued by the FAO: figure 3" .

glosis_cl:StickinessValueCode a owl:Class ;
    rdfs:label "Code list for StickinessValue - codelist class"@en ;
    rdfs:comment "This code list provides the StickinessValue codes."@en ;
    rdfs:seeAlso glosis_cl:stickinessValueCode ;
    rdfs:subClassOf skos:Concept ;
    owl:oneOf ( glosis_cl:stickinessValueCode-ST glosis_cl:stickinessValueCode-SST glosis_cl:stickinessValueCode-VST glosis_cl:stickinessValueCode-SVS glosis_cl:stickinessValueCode-NST glosis_cl:stickinessValueCode-SSS ) ;
    skos:definition "Stickiness is the quality of adhesion of the soil material to other objects determined by noting the adherence of soil material when it is pressed between thumb and finger. See more in the Guidelines for Soil Description issued by the FAO: table 55" .

glosis_cl:StructureGradeValueCode a owl:Class ;
    rdfs:label "Code list for StructureGradeValue - codelist class"@en ;
    rdfs:comment "This code list provides the StructureGradeValue codes."@en ;
    rdfs:seeAlso glosis_cl:structureGradeValueCode ;
    rdfs:subClassOf skos:Concept ;
    owl:oneOf ( glosis_cl:structureGradeValueCode-WM glosis_cl:structureGradeValueCode-ST glosis_cl:structureGradeValueCode-MO glosis_cl:structureGradeValueCode-MS glosis_cl:structureGradeValueCode-WE ) ;
    skos:definition "Guidelines for Soil Description issued by the FAO: table 47; Classification of structure of pedal soil materials. See more in Guidelines for Soil Description issued by the FAO: table 47" .

glosis_cl:StructureSizeValueCode a owl:Class ;
    rdfs:label "Code list for StructureSizeValue - codelist class"@en ;
    rdfs:comment "This code list provides the StructureSizeValue codes."@en ;
    rdfs:seeAlso glosis_cl:structureSizeValueCode ;
    rdfs:subClassOf skos:Concept ;
    owl:oneOf ( glosis_cl:structureSizeValueCode-VC glosis_cl:structureSizeValueCode-ME glosis_cl:structureSizeValueCode-FI glosis_cl:structureSizeValueCode-VF glosis_cl:structureSizeValueCode-CO glosis_cl:structureSizeValueCode-EC ) ;
    skos:definition "Size classes for soil structure types. See more in guidelines for Soil Description issued by the FAO: table 50" .

glosis_cl:SurfaceAgeValueCode a owl:Class ;
    rdfs:label "Code list for SurfaceAgeValue - codelist class"@en ;
    rdfs:comment "This code list provides the SurfaceAgeValue codes."@en ;
    rdfs:seeAlso glosis_cl:surfaceAgeValueCode ;
    rdfs:subClassOf skos:Concept ;
    owl:oneOf ( glosis_cl:surfaceAgeValueCode-T glosis_cl:surfaceAgeValueCode-oPf glosis_cl:surfaceAgeValueCode-Ha glosis_cl:surfaceAgeValueCode-Ya glosis_cl:surfaceAgeValueCode-oPp glosis_cl:surfaceAgeValueCode-Yn glosis_cl:surfaceAgeValueCode-lPi glosis_cl:surfaceAgeValueCode-oPi glosis_cl:surfaceAgeValueCode-lPp glosis_cl:surfaceAgeValueCode-O glosis_cl:surfaceAgeValueCode-vYa glosis_cl:surfaceAgeValueCode-vYn glosis_cl:surfaceAgeValueCode-lPf glosis_cl:surfaceAgeValueCode-Hn ) ;
    skos:definition "The age of the landscape is important information from which the possible duration of the occurrence of soil formation processes can be derived. See more in guidelines for Soil Description issued by the FAO: table 13" .

glosis_cl:TextClayPropertyCode a owl:Class ;
    rdfs:label "Code list for TextClayProperty - codelist class"@en ;
    rdfs:comment "This code list provides the TextClayProperty codes."@en ;
    rdfs:seeAlso glosis_cl:textClayPropertyCode ;
    rdfs:subClassOf skos:Concept,
        sosa:ObservableProperty ;
    owl:oneOf ( glosis_cl:textClayPropertyCode-Cl ) ;
    skos:definition "Eva Corral-Pazos-de-Provens, Ígor Rapp-Arrarás and Juan M. Domingo-Santos, Estimating textural fractions of the USDA using those of the International System: A quantile approach, Geoderma, Volume 416, 2022." .

glosis_cl:TextSandPropertyCode a owl:Class ;
    rdfs:label "Code list for TextSandProperty - codelist class"@en ;
    rdfs:comment "This code list provides the TextSandProperty codes."@en ;
    rdfs:seeAlso glosis_cl:textSandPropertyCode ;
    rdfs:subClassOf skos:Concept,
        sosa:ObservableProperty ;
    owl:oneOf ( glosis_cl:textSandPropertyCode-fSa_ISSS glosis_cl:textSandPropertyCode-mSa_ISSS glosis_cl:textSandPropertyCode-cSa_USDA glosis_cl:textSandPropertyCode-vfSa_ISSS glosis_cl:textSandPropertyCode-vcSa_ISSS glosis_cl:textSandPropertyCode-cSa_ISO glosis_cl:textSandPropertyCode-fSa_ISO glosis_cl:textSandPropertyCode-Sa_ISSS glosis_cl:textSandPropertyCode-cSa_ISSS glosis_cl:textSandPropertyCode-mSa_USDA glosis_cl:textSandPropertyCode-vcSa_USDA glosis_cl:textSandPropertyCode-vfSa_USDA glosis_cl:textSandPropertyCode-Sa_ISO glosis_cl:textSandPropertyCode-Sa_USDA glosis_cl:textSandPropertyCode-mSa_ISO glosis_cl:textSandPropertyCode-fSa_USDA ) ;
    skos:definition "ISO 14688-1:2017 Geotechnical investigation and testing — Identification and classification of soil ;S.J. Blott and K. Pye, Particle size scales and classification of sediment types based on particle size distributions: Review and recommended procedures, Sedimentology, 59 (7) (2012), pp. 2071-2096.  ;International Society of Soil Science (ISSS), 1929. The minutes of the First Commission meetings, International Congress of Soil Science, Washington 1927. Proc. Int. Soc. Soil Sci. 4 (3), pp. 215–222." .

glosis_cl:TextSiltPropertyCode a owl:Class ;
    rdfs:label "Code list for TextSiltProperty - codelist class"@en ;
    rdfs:comment "This code list provides the TextSiltProperty codes."@en ;
    rdfs:seeAlso glosis_cl:textSiltPropertyCode ;
    rdfs:subClassOf skos:Concept,
        sosa:ObservableProperty ;
    owl:oneOf ( glosis_cl:textSiltPropertyCode-mSi_ISO glosis_cl:textSiltPropertyCode-fSi_ISO glosis_cl:textSiltPropertyCode-cSi_ISO glosis_cl:textSiltPropertyCode-Si_ISSS glosis_cl:textSiltPropertyCode-Si_USDA glosis_cl:textSiltPropertyCode-Si_ISO glosis_cl:textSiltPropertyCode-cSi_USDA glosis_cl:textSiltPropertyCode-fSi_USDA ) ;
    skos:definition "ISO 14688-1:2017 Geotechnical investigation and testing — Identification and classification of soil ;S.J. Blott and K. Pye, Particle size scales and classification of sediment types based on particle size distributions: Review and recommended procedures, Sedimentology, 59 (7) (2012), pp. 2071-2096.  " .

glosis_cl:TextureUnconsolidatedValueCode a owl:Class ;
    rdfs:label "Code list for TextureUnconsolidatedValue - codelist class"@en ;
    rdfs:comment "This code list provides the TextureUnconsolidatedValue codes."@en ;
    rdfs:seeAlso glosis_cl:textureUnconsolidatedValueCode ;
    rdfs:subClassOf skos:Concept ;
    skos:definition "Texture of a soil that is unconsolidated or loose, typically not bound into a compact mass. It describes the proportions of sand, silt, and clay in the soil, which directly influences the soil's physical properties such as water retention, aeration, and fertility. This texture classification can impact various soil management practices, such as tillage, irrigation, and erosion control. Source: Canadian Soil Information Service - chapter 17 & Geosciences libretexts - 3.1: Soil Texture and Structure. Possible values include unconsolidated Sand,Silt, Clay, Loam. Silty Sand, Clayey Sand" .

glosis_cl:VegetationClassValueCode a owl:Class ;
    rdfs:label "Code list for VegetationClassValue - codelist class"@en ;
    rdfs:comment "This code list provides the VegetationClassValue codes."@en ;
    rdfs:seeAlso glosis_cl:vegetationClassValueCode ;
    rdfs:subClassOf skos:Concept ;
    owl:oneOf ( glosis_cl:vegetationClassValueCode-FS glosis_cl:vegetationClassValueCode-WD glosis_cl:vegetationClassValueCode-WX glosis_cl:vegetationClassValueCode-FX glosis_cl:vegetationClassValueCode-SS glosis_cl:vegetationClassValueCode-F glosis_cl:vegetationClassValueCode-HS glosis_cl:vegetationClassValueCode-D glosis_cl:vegetationClassValueCode-SE glosis_cl:vegetationClassValueCode-DS glosis_cl:vegetationClassValueCode-FE glosis_cl:vegetationClassValueCode-HT glosis_cl:vegetationClassValueCode-SX glosis_cl:vegetationClassValueCode-FD glosis_cl:vegetationClassValueCode-SD glosis_cl:vegetationClassValueCode-H glosis_cl:vegetationClassValueCode-FC glosis_cl:vegetationClassValueCode-HF glosis_cl:vegetationClassValueCode-DE glosis_cl:vegetationClassValueCode-S glosis_cl:vegetationClassValueCode-B glosis_cl:vegetationClassValueCode-M glosis_cl:vegetationClassValueCode-DX glosis_cl:vegetationClassValueCode-DD glosis_cl:vegetationClassValueCode-DT glosis_cl:vegetationClassValueCode-WE glosis_cl:vegetationClassValueCode-HM glosis_cl:vegetationClassValueCode-W glosis_cl:vegetationClassValueCode-WS ) ;
    skos:definition "Classification of vegetation.See more in Guidelines for Soil Description issued by the FAO: table 11" .

glosis_cl:VoidsClassificationValueCode a owl:Class ;
    rdfs:label "Code list for VoidsClassificationValue - codelist class"@en ;
    rdfs:comment "This code list provides the VoidsClassificationValue codes."@en ;
    rdfs:seeAlso glosis_cl:voidsClassificationValueCode ;
    rdfs:subClassOf skos:Concept ;
    owl:oneOf ( glosis_cl:voidsClassificationValueCode-C glosis_cl:voidsClassificationValueCode-I glosis_cl:voidsClassificationValueCode-P glosis_cl:voidsClassificationValueCode-B glosis_cl:voidsClassificationValueCode-V ) ;
    skos:definition "Voids include all empty spaces in the soil. They are related to the arrangement of the primary soil constituents, rooting patterns, burrowing of animals or any other soil-forming processes, such as cracking, translocation and leaching. See more in Guidelines for Soil Description issued by the FAO: table 61" .

glosis_cl:VoidsDiameterValueCode a owl:Class ;
    rdfs:label "Code list for VoidsDiameterValue - codelist class"@en ;
    rdfs:comment "This code list provides the VoidsDiameterValue codes."@en ;
    rdfs:seeAlso glosis_cl:voidsDiameterValueCode ;
    rdfs:subClassOf skos:Concept ;
    owl:oneOf ( glosis_cl:voidsDiameterValueCode-MC glosis_cl:voidsDiameterValueCode-VC glosis_cl:voidsDiameterValueCode-M glosis_cl:voidsDiameterValueCode-FM glosis_cl:voidsDiameterValueCode-V glosis_cl:voidsDiameterValueCode-FF glosis_cl:voidsDiameterValueCode-C glosis_cl:voidsDiameterValueCode-F ) ;
    skos:definition "Voids include all empty spaces in the soil. They are related to the arrangement of the primary soil constituents, rooting patterns, burrowing of animals or any other soil-forming processes, such as cracking, translocation and leaching. See more in Guidelines for Soil Description issued by the FAO: table 62" .

glosis_cl:WaterRetentionPropertyCode a owl:Class ;
    rdfs:label "Code list for WaterRetentionProperty - codelist class"@en ;
    rdfs:comment "This code list provides the WaterRetentionProperty codes."@en ;
    rdfs:seeAlso glosis_cl:waterRetentionPropertyCode ;
    rdfs:subClassOf skos:Concept,
        sosa:ObservableProperty ;
    owl:oneOf ( glosis_cl:waterRetentionPropertyCode-WRG100 glosis_cl:waterRetentionPropertyCode-WRG33 glosis_cl:waterRetentionPropertyCode-WRG1500 glosis_cl:waterRetentionPropertyCode-WRV10 glosis_cl:waterRetentionPropertyCode-WRV1500 glosis_cl:waterRetentionPropertyCode-WRV33 glosis_cl:waterRetentionPropertyCode-WRV glosis_cl:waterRetentionPropertyCode-WRG6 glosis_cl:waterRetentionPropertyCode-WRV200 glosis_cl:waterRetentionPropertyCode-WRG10 glosis_cl:waterRetentionPropertyCode-WRG glosis_cl:waterRetentionPropertyCode-WRV6 glosis_cl:waterRetentionPropertyCode-WRG500 glosis_cl:waterRetentionPropertyCode-WRG200 glosis_cl:waterRetentionPropertyCode-WRV100 glosis_cl:waterRetentionPropertyCode-WRV500 ) ;
    skos:definition "ISRIC Report 2019/01: Tier 1 and Tier 2 data in the context of the federated Global Soil Information System. Appendix 3" .

glosis_cl:WeatherConditionsValueCode a owl:Class ;
    rdfs:label "Code list for WeatherConditionsValue - codelist class"@en ;
    rdfs:comment "This code list provides the WeatherConditionsValue codes."@en ;
    rdfs:seeAlso glosis_cl:weatherConditionsValueCode ;
    rdfs:subClassOf skos:Concept ;
    owl:oneOf ( glosis_cl:weatherConditionsValueCode-PC glosis_cl:weatherConditionsValueCode-WC1 glosis_cl:weatherConditionsValueCode-WC5 glosis_cl:weatherConditionsValueCode-WC4 glosis_cl:weatherConditionsValueCode-OV glosis_cl:weatherConditionsValueCode-SU glosis_cl:weatherConditionsValueCode-RA glosis_cl:weatherConditionsValueCode-SL glosis_cl:weatherConditionsValueCode-SN glosis_cl:weatherConditionsValueCode-WC6 glosis_cl:weatherConditionsValueCode-WC3 glosis_cl:weatherConditionsValueCode-WC2 ) ;
    skos:definition "Codes for weather conditions.See in Guidelines for Soil Description issued by the FAO: table 2" .

glosis_cl:WeatheringValueCode a owl:Class ;
    rdfs:label "Code list for WeatheringValue - codelist class"@en ;
    rdfs:comment "This code list provides the WeatheringValue codes."@en ;
    rdfs:seeAlso glosis_cl:weatheringValueCode ;
    rdfs:subClassOf skos:Concept ;
    owl:oneOf ( glosis_cl:weatheringValueCode-S glosis_cl:weatheringValueCode-F glosis_cl:weatheringValueCode-W ) ;
    skos:definition "Classification of weathering of coarse fragments. See more in Guidelines for Soil Description issued by the FAO: table 29" .

glosis_cl:biologicalAbundanceValueCode-C a glosis_cl:BiologicalAbundanceValueCode,
        skos:Concept ;
    skos:definition "Common biological activity in soil" ;
    skos:inScheme glosis_cl:biologicalAbundanceValueCode ;
    skos:notation "C" ;
    skos:prefLabel "Common"@en ;
    skos:topConceptOf glosis_cl:biologicalAbundanceValueCode .

glosis_cl:biologicalAbundanceValueCode-F a glosis_cl:BiologicalAbundanceValueCode,
        skos:Concept ;
    skos:definition "Few biological activity in soil" ;
    skos:inScheme glosis_cl:biologicalAbundanceValueCode ;
    skos:notation "F" ;
    skos:prefLabel "Few"@en ;
    skos:topConceptOf glosis_cl:biologicalAbundanceValueCode .

glosis_cl:biologicalAbundanceValueCode-M a glosis_cl:BiologicalAbundanceValueCode,
        skos:Concept ;
    skos:definition "Many biological activity in soil" ;
    skos:inScheme glosis_cl:biologicalAbundanceValueCode ;
    skos:notation "M" ;
    skos:prefLabel "Many"@en ;
    skos:topConceptOf glosis_cl:biologicalAbundanceValueCode .

glosis_cl:biologicalAbundanceValueCode-N a glosis_cl:BiologicalAbundanceValueCode,
        skos:Concept ;
    skos:definition "No biological activity in soil" ;
    skos:inScheme glosis_cl:biologicalAbundanceValueCode ;
    skos:notation "N" ;
    skos:prefLabel "None"@en ;
    skos:topConceptOf glosis_cl:biologicalAbundanceValueCode .

glosis_cl:biologicalFeaturesValueCode-A a glosis_cl:BiologicalFeaturesValueCode,
        skos:Concept ;
    skos:definition "Biological feature of  Artefacts" ;
    skos:inScheme glosis_cl:biologicalFeaturesValueCode ;
    skos:notation "A" ;
    skos:prefLabel "Artefacts"@en ;
    skos:topConceptOf glosis_cl:biologicalFeaturesValueCode .

glosis_cl:biologicalFeaturesValueCode-B a glosis_cl:BiologicalFeaturesValueCode,
        skos:Concept ;
    skos:definition "Biological feature of Burrows (unspecified)" ;
    skos:inScheme glosis_cl:biologicalFeaturesValueCode ;
    skos:notation "B" ;
    skos:prefLabel "Burrows (unspecified)"@en ;
    skos:topConceptOf glosis_cl:biologicalFeaturesValueCode .

glosis_cl:biologicalFeaturesValueCode-BI a glosis_cl:BiologicalFeaturesValueCode,
        skos:Concept ;
    skos:definition "Biological feature of  Infilled large burrows" ;
    skos:inScheme glosis_cl:biologicalFeaturesValueCode ;
    skos:notation "BI" ;
    skos:prefLabel "Infilled large burrows"@en ;
    skos:topConceptOf glosis_cl:biologicalFeaturesValueCode .

glosis_cl:biologicalFeaturesValueCode-BO a glosis_cl:BiologicalFeaturesValueCode,
        skos:Concept ;
    skos:definition "Biological feature of  Open large burrows" ;
    skos:inScheme glosis_cl:biologicalFeaturesValueCode ;
    skos:notation "BO" ;
    skos:prefLabel "Open large burrows"@en ;
    skos:topConceptOf glosis_cl:biologicalFeaturesValueCode .

glosis_cl:biologicalFeaturesValueCode-C a glosis_cl:BiologicalFeaturesValueCode,
        skos:Concept ;
    skos:definition "Biological feature of  Charcoal" ;
    skos:inScheme glosis_cl:biologicalFeaturesValueCode ;
    skos:notation "C" ;
    skos:prefLabel "Charcoal"@en ;
    skos:topConceptOf glosis_cl:biologicalFeaturesValueCode .

glosis_cl:biologicalFeaturesValueCode-E a glosis_cl:BiologicalFeaturesValueCode,
        skos:Concept ;
    skos:definition "Biological feature of Earthworm channels" ;
    skos:inScheme glosis_cl:biologicalFeaturesValueCode ;
    skos:notation "E" ;
    skos:prefLabel "Earthworm channels"@en ;
    skos:topConceptOf glosis_cl:biologicalFeaturesValueCode .

glosis_cl:biologicalFeaturesValueCode-I a glosis_cl:BiologicalFeaturesValueCode,
        skos:Concept ;
    skos:definition "Biological feature of Other insect activity" ;
    skos:inScheme glosis_cl:biologicalFeaturesValueCode ;
    skos:notation "I" ;
    skos:prefLabel "Other insect activity"@en ;
    skos:topConceptOf glosis_cl:biologicalFeaturesValueCode .

glosis_cl:biologicalFeaturesValueCode-P a glosis_cl:BiologicalFeaturesValueCode,
        skos:Concept ;
    skos:definition "Biological feature of  Pedotubules" ;
    skos:inScheme glosis_cl:biologicalFeaturesValueCode ;
    skos:notation "P" ;
    skos:prefLabel "Pedotubules"@en ;
    skos:topConceptOf glosis_cl:biologicalFeaturesValueCode .

glosis_cl:biologicalFeaturesValueCode-T a glosis_cl:BiologicalFeaturesValueCode,
        skos:Concept ;
    skos:definition "Biological feature of Termite or ant channels and nests" ;
    skos:inScheme glosis_cl:biologicalFeaturesValueCode ;
    skos:notation "T" ;
    skos:prefLabel "Termite or ant channels and nests"@en ;
    skos:topConceptOf glosis_cl:biologicalFeaturesValueCode .

glosis_cl:bleachedSandValueCode-0 a glosis_cl:BleachedSandValueCode,
        skos:Concept ;
    skos:definition "Bleached sand of surface coverage 0-2%" ;
    skos:inScheme glosis_cl:bleachedSandValueCode ;
    skos:notation "None" ;
    skos:prefLabel "Bleached sand of surface coverage 0-2%"@en ;
    skos:topConceptOf glosis_cl:bleachedSandValueCode .

glosis_cl:bleachedSandValueCode-1 a glosis_cl:BleachedSandValueCode,
        skos:Concept ;
    skos:definition "Bleached sand of surface coverage 2-15%" ;
    skos:inScheme glosis_cl:bleachedSandValueCode ;
    skos:notation "Low" ;
    skos:prefLabel "Bleached sand of surface coverage 2-15%"@en ;
    skos:topConceptOf glosis_cl:bleachedSandValueCode .

glosis_cl:bleachedSandValueCode-2 a glosis_cl:BleachedSandValueCode,
        skos:Concept ;
    skos:definition "Bleached sand of surface coverage 15-40%" ;
    skos:inScheme glosis_cl:bleachedSandValueCode ;
    skos:notation "Moderate" ;
    skos:prefLabel "Bleached sand of surface coverage 15-40%"@en ;
    skos:topConceptOf glosis_cl:bleachedSandValueCode .

glosis_cl:bleachedSandValueCode-3 a glosis_cl:BleachedSandValueCode,
        skos:Concept ;
    skos:definition "Bleached sand of surface coverage  40-80%" ;
    skos:inScheme glosis_cl:bleachedSandValueCode ;
    skos:notation "High" ;
    skos:prefLabel "Bleached sand of surface coverage  40-80%"@en ;
    skos:topConceptOf glosis_cl:bleachedSandValueCode .

glosis_cl:bleachedSandValueCode-4 a glosis_cl:BleachedSandValueCode,
        skos:Concept ;
    skos:definition "Bleached sand of surface coverage more than 80%" ;
    skos:inScheme glosis_cl:bleachedSandValueCode ;
    skos:notation "Dominant" ;
    skos:prefLabel "Bleached sand of surface coverage more than 80%"@en ;
    skos:topConceptOf glosis_cl:bleachedSandValueCode .

glosis_cl:boundaryClassificationValueCode-C a glosis_cl:BoundaryClassificationValueCode,
        skos:Concept ;
    skos:definition "Boundary of mottles 0.5–2 mm" ;
    skos:inScheme glosis_cl:boundaryClassificationValueCode ;
    skos:notation "C" ;
    skos:prefLabel "Clear"@en ;
    skos:topConceptOf glosis_cl:boundaryClassificationValueCode .

glosis_cl:boundaryClassificationValueCode-D a glosis_cl:BoundaryClassificationValueCode,
        skos:Concept ;
    skos:definition "Boundary of mottles > 2 mm" ;
    skos:inScheme glosis_cl:boundaryClassificationValueCode ;
    skos:notation "D" ;
    skos:prefLabel "Diffuse"@en ;
    skos:topConceptOf glosis_cl:boundaryClassificationValueCode .

glosis_cl:boundaryClassificationValueCode-S a glosis_cl:BoundaryClassificationValueCode,
        skos:Concept ;
    skos:definition "Boundary of mottles < 0.5" ;
    skos:inScheme glosis_cl:boundaryClassificationValueCode ;
    skos:notation "S" ;
    skos:prefLabel "Sharp"@en ;
    skos:topConceptOf glosis_cl:boundaryClassificationValueCode .

glosis_cl:boundaryDistinctnessValueCode-A a glosis_cl:BoundaryDistinctnessValueCode,
        skos:Concept ;
    skos:definition "0cm–2cm" ;
    skos:inScheme glosis_cl:boundaryDistinctnessValueCode ;
    skos:notation "A" ;
    skos:prefLabel "Abrupt"@en ;
    skos:topConceptOf glosis_cl:boundaryDistinctnessValueCode .

glosis_cl:boundaryDistinctnessValueCode-C a glosis_cl:BoundaryDistinctnessValueCode,
        skos:Concept ;
    skos:definition "2cm–5cm" ;
    skos:inScheme glosis_cl:boundaryDistinctnessValueCode ;
    skos:notation "C" ;
    skos:prefLabel "Clear"@en ;
    skos:topConceptOf glosis_cl:boundaryDistinctnessValueCode .

glosis_cl:boundaryDistinctnessValueCode-D a glosis_cl:BoundaryDistinctnessValueCode,
        skos:Concept ;
    skos:definition "> 15cm" ;
    skos:inScheme glosis_cl:boundaryDistinctnessValueCode ;
    skos:notation "D" ;
    skos:prefLabel "Diffuse"@en ;
    skos:topConceptOf glosis_cl:boundaryDistinctnessValueCode .

glosis_cl:boundaryDistinctnessValueCode-G a glosis_cl:BoundaryDistinctnessValueCode,
        skos:Concept ;
    skos:definition "5cm–15cm" ;
    skos:inScheme glosis_cl:boundaryDistinctnessValueCode ;
    skos:notation "G" ;
    skos:prefLabel "Gradual"@en ;
    skos:topConceptOf glosis_cl:boundaryDistinctnessValueCode .

glosis_cl:boundaryTopographyValueCode-B a glosis_cl:BoundaryTopographyValueCode,
        skos:Concept ;
    skos:definition "Discontinuous" ;
    skos:inScheme glosis_cl:boundaryTopographyValueCode ;
    skos:notation "B" ;
    skos:prefLabel "Broken"@en ;
    skos:topConceptOf glosis_cl:boundaryTopographyValueCode .

glosis_cl:boundaryTopographyValueCode-I a glosis_cl:BoundaryTopographyValueCode,
        skos:Concept ;
    skos:definition "Pockets more deep than wide" ;
    skos:inScheme glosis_cl:boundaryTopographyValueCode ;
    skos:notation "I" ;
    skos:prefLabel "Irregular"@en ;
    skos:topConceptOf glosis_cl:boundaryTopographyValueCode .

glosis_cl:boundaryTopographyValueCode-S a glosis_cl:BoundaryTopographyValueCode,
        skos:Concept ;
    skos:definition "Nearly plane surface" ;
    skos:inScheme glosis_cl:boundaryTopographyValueCode ;
    skos:notation "S" ;
    skos:prefLabel "Smooth"@en ;
    skos:topConceptOf glosis_cl:boundaryTopographyValueCode .

glosis_cl:boundaryTopographyValueCode-W a glosis_cl:BoundaryTopographyValueCode,
        skos:Concept ;
    skos:definition "Pockets less deep than wide" ;
    skos:inScheme glosis_cl:boundaryTopographyValueCode ;
    skos:notation "W" ;
    skos:prefLabel "Wavy"@en ;
    skos:topConceptOf glosis_cl:boundaryTopographyValueCode .

glosis_cl:bulkDensityMineralValueCode-BD1 a glosis_cl:BulkDensityMineralValueCode,
        skos:Concept ;
    skos:definition "materials with vesicular pores, mineral soils with andic properties. Sample disintegrates at the instant of sampling, many pores visible onthe pit wall. Sample disintegrates at the instant of sampling, many pores visible on the pit wall. Loamy soils with high clay content, clayey soils When dropped, sample disintegrates into numerous fragments, further disintegration of subfragments after application of weak pressure." ;
    skos:inScheme glosis_cl:bulkDensityMineralValueCode ;
    skos:notation "BD1" ;
    skos:prefLabel "Many pores, moist materials drop easily out of the auger."@en ;
    skos:topConceptOf glosis_cl:bulkDensityMineralValueCode .

glosis_cl:bulkDensityMineralValueCode-BD2 a glosis_cl:BulkDensityMineralValueCode,
        skos:Concept ;
    skos:definition "Loamy soils with high clay content, clayey soils. When dropped, sample disintegrates into few fragments, further disintegration of subfragments after application of mild pressure." ;
    skos:inScheme glosis_cl:bulkDensityMineralValueCode ;
    skos:notation "BD2" ;
    skos:prefLabel "Sample disintegrates into numerous fragments after application of weak pressure."@en ;
    skos:topConceptOf glosis_cl:bulkDensityMineralValueCode .

glosis_cl:bulkDensityMineralValueCode-BD3 a glosis_cl:BulkDensityMineralValueCode,
        skos:Concept ;
    skos:definition "Loamy soils with high clay content, clayey soils. Sample remains mostly intact when dropped, further disintegration possible after application of large pressure." ;
    skos:inScheme glosis_cl:bulkDensityMineralValueCode ;
    skos:notation "BD3" ;
    skos:prefLabel "Knife can be pushed into the moist soil with weak pressure, sample disintegrates into few fragments, which may be further divided."@en ;
    skos:topConceptOf glosis_cl:bulkDensityMineralValueCode .

glosis_cl:bulkDensityMineralValueCode-BD4 a glosis_cl:BulkDensityMineralValueCode,
        skos:Concept ;
    skos:definition "Loamy soils with high clay content, clayey soils. Sample remains intact when dropped, no further disintegration after application of very large pressure." ;
    skos:inScheme glosis_cl:bulkDensityMineralValueCode ;
    skos:notation "BD4" ;
    skos:prefLabel "Knife penetrates only 1–2 cm into the moist soil, some effort required, sample disintegrates into few fragments, which cannot be subdivided further."@en ;
    skos:topConceptOf glosis_cl:bulkDensityMineralValueCode .

glosis_cl:bulkDensityMineralValueCode-BD5 a glosis_cl:BulkDensityMineralValueCode,
        skos:Concept ;
    skos:definition "Loamy soils with high clay content, clayey soils. Sample remains intact when dropped, no further disintegration after application of very large pressure." ;
    skos:inScheme glosis_cl:bulkDensityMineralValueCode ;
    skos:notation "BD5" ;
    skos:prefLabel "Very large pressure necessary to force knife into the soil, no further disintegration of sample."@en ;
    skos:topConceptOf glosis_cl:bulkDensityMineralValueCode .

glosis_cl:bulkDensityPeatValueCode-BD1 a glosis_cl:BulkDensityPeatValueCode,
        skos:Concept ;
    skos:definition "Very low (fibric) class of decomposition: < 0.04g cm-3" ;
    skos:inScheme glosis_cl:bulkDensityPeatValueCode ;
    skos:notation "BD1" ;
    skos:prefLabel "Very low"@en ;
    skos:topConceptOf glosis_cl:bulkDensityPeatValueCode .

glosis_cl:bulkDensityPeatValueCode-BD2 a glosis_cl:BulkDensityPeatValueCode,
        skos:Concept ;
    skos:definition "Low (fibric) class of decomposition: 0.04–0.07g cm-3" ;
    skos:inScheme glosis_cl:bulkDensityPeatValueCode ;
    skos:notation "BD2" ;
    skos:prefLabel "Low"@en ;
    skos:topConceptOf glosis_cl:bulkDensityPeatValueCode .

glosis_cl:bulkDensityPeatValueCode-BD3 a glosis_cl:BulkDensityPeatValueCode,
        skos:Concept ;
    skos:definition "Moderate(fibric) class of decomposition: 0.07–0.11g cm-3" ;
    skos:inScheme glosis_cl:bulkDensityPeatValueCode ;
    skos:notation "BD3" ;
    skos:prefLabel "Moderate low"@en ;
    skos:topConceptOf glosis_cl:bulkDensityPeatValueCode .

glosis_cl:bulkDensityPeatValueCode-BD4 a glosis_cl:BulkDensityPeatValueCode,
        skos:Concept ;
    skos:definition "Moderate(fibric) class of decomposition: 0.11–0.17g cm-3" ;
    skos:inScheme glosis_cl:bulkDensityPeatValueCode ;
    skos:notation "BD4" ;
    skos:prefLabel "Moderate high"@en ;
    skos:topConceptOf glosis_cl:bulkDensityPeatValueCode .

glosis_cl:bulkDensityPeatValueCode-BD5 a glosis_cl:BulkDensityPeatValueCode,
        skos:Concept ;
    skos:definition "Strong (hemic) class of decomposition: > 0.17g cm-3" ;
    skos:inScheme glosis_cl:bulkDensityPeatValueCode ;
    skos:notation "BD5" ;
    skos:prefLabel "Strong (hemic)"@en ;
    skos:topConceptOf glosis_cl:bulkDensityPeatValueCode .

glosis_cl:carbonatesContentValueCode-EX a glosis_cl:CarbonatesContentValueCode,
        skos:Concept ;
    skos:definition "Extremely strong reaction forming thick foam forms quickly: ≈ > 25" ;
    skos:inScheme glosis_cl:carbonatesContentValueCode ;
    skos:notation "EX" ;
    skos:prefLabel "Extremely calcareous"@en ;
    skos:topConceptOf glosis_cl:carbonatesContentValueCode .

glosis_cl:carbonatesContentValueCode-MO a glosis_cl:CarbonatesContentValueCode,
        skos:Concept ;
    skos:definition "Visible effervescence: ≈ 2–10" ;
    skos:inScheme glosis_cl:carbonatesContentValueCode ;
    skos:notation "MO" ;
    skos:prefLabel "Moderately calcareous"@en ;
    skos:topConceptOf glosis_cl:carbonatesContentValueCode .

glosis_cl:carbonatesContentValueCode-N a glosis_cl:CarbonatesContentValueCode,
        skos:Concept ;
    skos:definition "No detectable visible or audible effervescence." ;
    skos:inScheme glosis_cl:carbonatesContentValueCode ;
    skos:notation "N" ;
    skos:prefLabel "Non-calcareous"@en ;
    skos:topConceptOf glosis_cl:carbonatesContentValueCode .

glosis_cl:carbonatesContentValueCode-SL a glosis_cl:CarbonatesContentValueCode,
        skos:Concept ;
    skos:definition "Audible effervescence but not visible: ≈ 0–2" ;
    skos:inScheme glosis_cl:carbonatesContentValueCode ;
    skos:notation "SL" ;
    skos:prefLabel "Slightly calcareous"@en ;
    skos:topConceptOf glosis_cl:carbonatesContentValueCode .

glosis_cl:carbonatesContentValueCode-ST a glosis_cl:CarbonatesContentValueCode,
        skos:Concept ;
    skos:definition "Strong visible effervescence. Bubbles form a low foam: ≈ 10–25" ;
    skos:inScheme glosis_cl:carbonatesContentValueCode ;
    skos:notation "ST" ;
    skos:prefLabel "Strongly calcareous"@en ;
    skos:topConceptOf glosis_cl:carbonatesContentValueCode .

glosis_cl:carbonatesFormsValueCode-D a glosis_cl:CarbonatesFormsValueCode,
        skos:Concept ;
    skos:definition "Secondary carbonates in soil in the form of disperse powdery lime" ;
    skos:inScheme glosis_cl:carbonatesFormsValueCode ;
    skos:notation "D" ;
    skos:prefLabel "disperse powdery lime"@en ;
    skos:topConceptOf glosis_cl:carbonatesFormsValueCode .

glosis_cl:carbonatesFormsValueCode-HC a glosis_cl:CarbonatesFormsValueCode,
        skos:Concept ;
    skos:definition "Secondary carbonates in soil in the form of hard concretions" ;
    skos:inScheme glosis_cl:carbonatesFormsValueCode ;
    skos:notation "HC" ;
    skos:prefLabel "hard concretions"@en ;
    skos:topConceptOf glosis_cl:carbonatesFormsValueCode .

glosis_cl:carbonatesFormsValueCode-HHC a glosis_cl:CarbonatesFormsValueCode,
        skos:Concept ;
    skos:definition "Secondary carbonates in soil in the form of hard hollow concretions" ;
    skos:inScheme glosis_cl:carbonatesFormsValueCode ;
    skos:notation "HHC" ;
    skos:prefLabel "hard hollow concretions"@en ;
    skos:topConceptOf glosis_cl:carbonatesFormsValueCode .

glosis_cl:carbonatesFormsValueCode-HL a glosis_cl:CarbonatesFormsValueCode,
        skos:Concept ;
    skos:definition "Secondary carbonates in soil in the form of hard cemented layer or layers of carbonates" ;
    skos:inScheme glosis_cl:carbonatesFormsValueCode ;
    skos:notation "HL" ;
    skos:prefLabel "hard cemented layer or layers of carbonates (less than 10 cm thick)"@en ;
    skos:topConceptOf glosis_cl:carbonatesFormsValueCode .

glosis_cl:carbonatesFormsValueCode-M a glosis_cl:CarbonatesFormsValueCode,
        skos:Concept ;
    skos:definition "Secondary carbonates in soil in the form of marl layer" ;
    skos:inScheme glosis_cl:carbonatesFormsValueCode ;
    skos:notation "M" ;
    skos:prefLabel "marl layer"@en ;
    skos:topConceptOf glosis_cl:carbonatesFormsValueCode .

glosis_cl:carbonatesFormsValueCode-PM a glosis_cl:CarbonatesFormsValueCode,
        skos:Concept ;
    skos:definition "Secondary carbonates in soil in the form of pseudomycelia i.e. carbonate infillings in pores, resembling mycelia" ;
    skos:inScheme glosis_cl:carbonatesFormsValueCode ;
    skos:notation "PM" ;
    skos:prefLabel "pseudomycelia* (carbonate infillings in pores, resembling mycelia)"@en ;
    skos:topConceptOf glosis_cl:carbonatesFormsValueCode .

glosis_cl:carbonatesFormsValueCode-SC a glosis_cl:CarbonatesFormsValueCode,
        skos:Concept ;
    skos:definition "Secondary carbonates in soil in the form of soft concretions" ;
    skos:inScheme glosis_cl:carbonatesFormsValueCode ;
    skos:notation "SC" ;
    skos:prefLabel "soft concretions"@en ;
    skos:topConceptOf glosis_cl:carbonatesFormsValueCode .

glosis_cl:cementationContinuityValueCode-B a glosis_cl:CementationContinuityValueCode,
        skos:Concept ;
    skos:definition "The layer is less than 50 percent cemented or compacted, and shows a rather irregular appearance." ;
    skos:inScheme glosis_cl:cementationContinuityValueCode ;
    skos:notation "B" ;
    skos:prefLabel "Broken"@en ;
    skos:topConceptOf glosis_cl:cementationContinuityValueCode .

glosis_cl:cementationContinuityValueCode-C a glosis_cl:CementationContinuityValueCode,
        skos:Concept ;
    skos:definition "The layer is more than 90 percent cemented or compacted, and is only interrupted in places by cracks or fissures." ;
    skos:inScheme glosis_cl:cementationContinuityValueCode ;
    skos:notation "C" ;
    skos:prefLabel "Continuous"@en ;
    skos:topConceptOf glosis_cl:cementationContinuityValueCode .

glosis_cl:cementationContinuityValueCode-D a glosis_cl:CementationContinuityValueCode,
        skos:Concept ;
    skos:definition "The layer is 50–90 percent cemented or compacted, and in general shows a regular appearance." ;
    skos:inScheme glosis_cl:cementationContinuityValueCode ;
    skos:notation "D" ;
    skos:prefLabel "Discontinuous"@en ;
    skos:topConceptOf glosis_cl:cementationContinuityValueCode .

glosis_cl:cementationDegreeValueCode-C a glosis_cl:CementationDegreeValueCode,
        skos:Concept ;
    skos:definition "Cemented mass cannot be broken in the hands and is continuous (more than 90 percent of soil mass)." ;
    skos:inScheme glosis_cl:cementationDegreeValueCode ;
    skos:notation "C" ;
    skos:prefLabel "Cemented"@en ;
    skos:topConceptOf glosis_cl:cementationDegreeValueCode .

glosis_cl:cementationDegreeValueCode-I a glosis_cl:CementationDegreeValueCode,
        skos:Concept ;
    skos:definition "Cemented mass cannot be broken by body weight (75-kg standard soil scientist) (more than 90 percent of soil mass)." ;
    skos:inScheme glosis_cl:cementationDegreeValueCode ;
    skos:notation "I" ;
    skos:prefLabel "Indurated"@en ;
    skos:topConceptOf glosis_cl:cementationDegreeValueCode .

glosis_cl:cementationDegreeValueCode-M a glosis_cl:CementationDegreeValueCode,
        skos:Concept ;
    skos:definition "Cemented mass cannot be broken in the hands but is discontinuous (less than 90 percent of soil mass)." ;
    skos:inScheme glosis_cl:cementationDegreeValueCode ;
    skos:notation "M" ;
    skos:prefLabel "Moderately cemented"@en ;
    skos:topConceptOf glosis_cl:cementationDegreeValueCode .

glosis_cl:cementationDegreeValueCode-N a glosis_cl:CementationDegreeValueCode,
        skos:Concept ;
    skos:definition "Neither cementation nor compaction observed (slakes in water)." ;
    skos:inScheme glosis_cl:cementationDegreeValueCode ;
    skos:notation "N" ;
    skos:prefLabel "Non-cemented and non-compacted"@en ;
    skos:topConceptOf glosis_cl:cementationDegreeValueCode .

glosis_cl:cementationDegreeValueCode-W a glosis_cl:CementationDegreeValueCode,
        skos:Concept ;
    skos:definition "Cemented mass is brittle and hard, but can be broken in the hands." ;
    skos:inScheme glosis_cl:cementationDegreeValueCode ;
    skos:notation "W" ;
    skos:prefLabel "Weakly cemented"@en ;
    skos:topConceptOf glosis_cl:cementationDegreeValueCode .

glosis_cl:cementationDegreeValueCode-Y a glosis_cl:CementationDegreeValueCode,
        skos:Concept ;
    skos:definition "Compacted mass is appreciably harder or more brittle than other comparable soil mass (slakes in water)." ;
    skos:inScheme glosis_cl:cementationDegreeValueCode ;
    skos:notation "Y" ;
    skos:prefLabel "Compacted but non-cemented"@en ;
    skos:topConceptOf glosis_cl:cementationDegreeValueCode .

glosis_cl:cementationFabricValueCode-D a glosis_cl:CementationFabricValueCode,
        skos:Concept ;
    skos:definition "The layer is largely constructed from cemented nodules or concretions of irregular shape." ;
    skos:inScheme glosis_cl:cementationFabricValueCode ;
    skos:notation "D" ;
    skos:prefLabel "Nodular"@en ;
    skos:topConceptOf glosis_cl:cementationFabricValueCode .

glosis_cl:cementationFabricValueCode-Pi a glosis_cl:CementationFabricValueCode,
        skos:Concept ;
    skos:definition "The layer is largely constructed from cemented spherical nodules." ;
    skos:inScheme glosis_cl:cementationFabricValueCode ;
    skos:notation "Pi" ;
    skos:prefLabel "Pisolithic"@en ;
    skos:topConceptOf glosis_cl:cementationFabricValueCode .

glosis_cl:cementationFabricValueCode-Pl a glosis_cl:CementationFabricValueCode,
        skos:Concept ;
    skos:definition "The compacted or cemented parts are platelike and have a horizontal or subhorizontal orientation." ;
    skos:inScheme glosis_cl:cementationFabricValueCode ;
    skos:notation "Pl" ;
    skos:prefLabel "Platy"@en ;
    skos:topConceptOf glosis_cl:cementationFabricValueCode .

glosis_cl:cementationFabricValueCode-V a glosis_cl:CementationFabricValueCode,
        skos:Concept ;
    skos:definition "The layer has large, equidimensional voids that may be filled with uncemented material." ;
    skos:inScheme glosis_cl:cementationFabricValueCode ;
    skos:notation "V" ;
    skos:prefLabel "Vesicular"@en ;
    skos:topConceptOf glosis_cl:cementationFabricValueCode .

glosis_cl:cementationNatureValueCode-C a glosis_cl:CementationNatureValueCode,
        skos:Concept ;
    skos:definition "Primary cementing material containing Clay" ;
    skos:inScheme glosis_cl:cementationNatureValueCode ;
    skos:notation "C" ;
    skos:prefLabel "Clay"@en ;
    skos:topConceptOf glosis_cl:cementationNatureValueCode .

glosis_cl:cementationNatureValueCode-CS a glosis_cl:CementationNatureValueCode,
        skos:Concept ;
    skos:definition "Primary cementing material containing Clay–sesquioxides" ;
    skos:inScheme glosis_cl:cementationNatureValueCode ;
    skos:notation "CS" ;
    skos:prefLabel "Clay–sesquioxides"@en ;
    skos:topConceptOf glosis_cl:cementationNatureValueCode .

glosis_cl:cementationNatureValueCode-F a glosis_cl:CementationNatureValueCode,
        skos:Concept ;
    skos:definition "Primary cementing material containing Iron" ;
    skos:inScheme glosis_cl:cementationNatureValueCode ;
    skos:notation "F" ;
    skos:prefLabel "Iron"@en ;
    skos:topConceptOf glosis_cl:cementationNatureValueCode .

glosis_cl:cementationNatureValueCode-FM a glosis_cl:CementationNatureValueCode,
        skos:Concept ;
    skos:definition "Primary cementing material containing Iron–manganese (sesquioxides)" ;
    skos:inScheme glosis_cl:cementationNatureValueCode ;
    skos:notation "FM" ;
    skos:prefLabel "Iron–manganese (sesquioxides)"@en ;
    skos:topConceptOf glosis_cl:cementationNatureValueCode .

glosis_cl:cementationNatureValueCode-FO a glosis_cl:CementationNatureValueCode,
        skos:Concept ;
    skos:definition "Primary cementing material containing Iron–organic matter" ;
    skos:inScheme glosis_cl:cementationNatureValueCode ;
    skos:notation "FO" ;
    skos:prefLabel "Iron–organic matter"@en ;
    skos:topConceptOf glosis_cl:cementationNatureValueCode .

glosis_cl:cementationNatureValueCode-GY a glosis_cl:CementationNatureValueCode,
        skos:Concept ;
    skos:definition "Primary cementing material containing Gypsum" ;
    skos:inScheme glosis_cl:cementationNatureValueCode ;
    skos:notation "GY" ;
    skos:prefLabel "Gypsum"@en ;
    skos:topConceptOf glosis_cl:cementationNatureValueCode .

glosis_cl:cementationNatureValueCode-I a glosis_cl:CementationNatureValueCode,
        skos:Concept ;
    skos:definition "Primary cementing material containing Ice" ;
    skos:inScheme glosis_cl:cementationNatureValueCode ;
    skos:notation "I" ;
    skos:prefLabel "Ice"@en ;
    skos:topConceptOf glosis_cl:cementationNatureValueCode .

glosis_cl:cementationNatureValueCode-K a glosis_cl:CementationNatureValueCode,
        skos:Concept ;
    skos:definition "Primary cementing material containing Carbonates" ;
    skos:inScheme glosis_cl:cementationNatureValueCode ;
    skos:notation "K" ;
    skos:prefLabel "Carbonates"@en ;
    skos:topConceptOf glosis_cl:cementationNatureValueCode .

glosis_cl:cementationNatureValueCode-KQ a glosis_cl:CementationNatureValueCode,
        skos:Concept ;
    skos:definition "Primary cementing material containing Carbonates–silica" ;
    skos:inScheme glosis_cl:cementationNatureValueCode ;
    skos:notation "KQ" ;
    skos:prefLabel "Carbonates–silica"@en ;
    skos:topConceptOf glosis_cl:cementationNatureValueCode .

glosis_cl:cementationNatureValueCode-M a glosis_cl:CementationNatureValueCode,
        skos:Concept ;
    skos:definition "Primary cementing material containing Mechanical" ;
    skos:inScheme glosis_cl:cementationNatureValueCode ;
    skos:notation "M" ;
    skos:prefLabel "Mechanical"@en ;
    skos:topConceptOf glosis_cl:cementationNatureValueCode .

glosis_cl:cementationNatureValueCode-NK a glosis_cl:CementationNatureValueCode,
        skos:Concept ;
    skos:definition "Primary cementing material containing Not known contents" ;
    skos:inScheme glosis_cl:cementationNatureValueCode ;
    skos:notation "NK" ;
    skos:prefLabel "Not known"@en ;
    skos:topConceptOf glosis_cl:cementationNatureValueCode .

glosis_cl:cementationNatureValueCode-P a glosis_cl:CementationNatureValueCode,
        skos:Concept ;
    skos:definition "Primary cementing material containing Ploughing" ;
    skos:inScheme glosis_cl:cementationNatureValueCode ;
    skos:notation "P" ;
    skos:prefLabel "Ploughing"@en ;
    skos:topConceptOf glosis_cl:cementationNatureValueCode .

glosis_cl:cementationNatureValueCode-Q a glosis_cl:CementationNatureValueCode,
        skos:Concept ;
    skos:definition "Primary cementing material containing Silica" ;
    skos:inScheme glosis_cl:cementationNatureValueCode ;
    skos:notation "Q" ;
    skos:prefLabel "Silica"@en ;
    skos:topConceptOf glosis_cl:cementationNatureValueCode .

glosis_cl:clayPropertyCode-CC a glosis_cl:ClayPropertyCode,
        skos:Concept ;
    skos:definition "Clay carbonate refers to clay particles that are associated with or contain carbonate minerals, particularly calcium carbonate (CaCO₃). These carbonates are typically present in soils with higher pH (alkaline soils), and they play a significant role in buffering soil acidity. Clay-carbonate soils are found in regions with semi-arid and arid climates, where evaporation exceeds precipitation. These soils can have distinct properties, including a lower cation exchange capacity compared to non-carbonate soils and an ability to neutralize soil acidity, influencing both soil fertility and plant growth. Source: Brady & Weil (2017), The Nature and Properties of Soils." ;
    skos:inScheme glosis_cl:clayPropertyCode ;
    skos:notation "CC" ;
    skos:prefLabel "Clay Carbonate"@en ;
    skos:topConceptOf glosis_cl:clayPropertyCode .

glosis_cl:clayPropertyCode-CNC a glosis_cl:ClayPropertyCode,
        skos:Concept ;
    skos:definition "Clay non-carbonate refers to the fraction of clay particles in soil that do not contain carbonates. Clay particles are very fine mineral components that contribute to the soil's texture and are typically smaller than 0.002 mm in diameter. The term non-carbonate implies that these clay particles are not associated with carbonate minerals, such as calcium carbonate (lime), which are commonly found in soils in arid or semi-arid regions. Non-carbonate clay soils are often more acidic, with higher cation exchange capacity, and may require different management practices, especially for nutrient availability and soil pH control. Source: Brady & Weil (2017), The Nature and Properties of Soils." ;
    skos:inScheme glosis_cl:clayPropertyCode ;
    skos:notation "CNC" ;
    skos:prefLabel "Clay Non-Carbonate"@en ;
    skos:topConceptOf glosis_cl:clayPropertyCode .

glosis_cl:clayPropertyCode-CWT a glosis_cl:ClayPropertyCode,
        skos:Concept ;
    skos:definition "Clay water dispersible refers to the portion of clay particles in soil that can be dispersed into water, forming a suspension when the soil is wetted. This characteristic is significant in assessing soil stability, particularly in the presence of water. Water-dispersible clays can lead to erosion problems, as the particles are more easily detached and transported by water. This term is important in understanding soil erodibility, especially in soils with high clay content that are prone to degradation when subjected to rainfall or irrigation. The dispersibility of clay affects both the physical structure and water-holding capacity of the soil. Source: Soil Science Society of America." ;
    skos:inScheme glosis_cl:clayPropertyCode ;
    skos:notation "CWT" ;
    skos:prefLabel "Clay Water Dispersible"@en ;
    skos:topConceptOf glosis_cl:clayPropertyCode .

glosis_cl:coatingAbundanceValueCode-A a glosis_cl:CoatingAbundanceValueCode,
        skos:Concept ;
    skos:definition "40–80% of coating abundance" ;
    skos:inScheme glosis_cl:coatingAbundanceValueCode ;
    skos:notation "A" ;
    skos:prefLabel "Abundant"@en ;
    skos:topConceptOf glosis_cl:coatingAbundanceValueCode .

glosis_cl:coatingAbundanceValueCode-C a glosis_cl:CoatingAbundanceValueCode,
        skos:Concept ;
    skos:definition "5–15% of coating abundance" ;
    skos:inScheme glosis_cl:coatingAbundanceValueCode ;
    skos:notation "C" ;
    skos:prefLabel "Common"@en ;
    skos:topConceptOf glosis_cl:coatingAbundanceValueCode .

glosis_cl:coatingAbundanceValueCode-D a glosis_cl:CoatingAbundanceValueCode,
        skos:Concept ;
    skos:definition "> 80% of coating abundance" ;
    skos:inScheme glosis_cl:coatingAbundanceValueCode ;
    skos:notation "D" ;
    skos:prefLabel "Dominant"@en ;
    skos:topConceptOf glosis_cl:coatingAbundanceValueCode .

glosis_cl:coatingAbundanceValueCode-F a glosis_cl:CoatingAbundanceValueCode,
        skos:Concept ;
    skos:definition "2–5% of coating abundance" ;
    skos:inScheme glosis_cl:coatingAbundanceValueCode ;
    skos:notation "F" ;
    skos:prefLabel "Few"@en ;
    skos:topConceptOf glosis_cl:coatingAbundanceValueCode .

glosis_cl:coatingAbundanceValueCode-M a glosis_cl:CoatingAbundanceValueCode,
        skos:Concept ;
    skos:definition "15–40% of coating abundance" ;
    skos:inScheme glosis_cl:coatingAbundanceValueCode ;
    skos:notation "M" ;
    skos:prefLabel "Many"@en ;
    skos:topConceptOf glosis_cl:coatingAbundanceValueCode .

glosis_cl:coatingAbundanceValueCode-N a glosis_cl:CoatingAbundanceValueCode,
        skos:Concept ;
    skos:definition "0% of coating abundance" ;
    skos:inScheme glosis_cl:coatingAbundanceValueCode ;
    skos:notation "N" ;
    skos:prefLabel "None"@en ;
    skos:topConceptOf glosis_cl:coatingAbundanceValueCode .

glosis_cl:coatingAbundanceValueCode-V a glosis_cl:CoatingAbundanceValueCode,
        skos:Concept ;
    skos:definition "0–2 % of coating abundance" ;
    skos:inScheme glosis_cl:coatingAbundanceValueCode ;
    skos:notation "V" ;
    skos:prefLabel "Very few"@en ;
    skos:topConceptOf glosis_cl:coatingAbundanceValueCode .

glosis_cl:coatingContrastValueCode-D a glosis_cl:CoatingContrastValueCode,
        skos:Concept ;
    skos:definition "Surface of coating is distinctly smoother or different in colour from the adjacent surface. Fine sand grains are enveloped in the coating but their outlines are still visible. Lamellae are 2–5 mm thick." ;
    skos:inScheme glosis_cl:coatingContrastValueCode ;
    skos:notation "D" ;
    skos:prefLabel "Distinct"@en ;
    skos:topConceptOf glosis_cl:coatingContrastValueCode .

glosis_cl:coatingContrastValueCode-F a glosis_cl:CoatingContrastValueCode,
        skos:Concept ;
    skos:definition "Surface of coating shows only little contrast in colour, smoothness or any other property to the adjacent surface. Fine sand grains are readily apparent in the cutan. Lamellae are less than 2 mm thick." ;
    skos:inScheme glosis_cl:coatingContrastValueCode ;
    skos:notation "F" ;
    skos:prefLabel "Faint"@en ;
    skos:topConceptOf glosis_cl:coatingContrastValueCode .

glosis_cl:coatingContrastValueCode-P a glosis_cl:CoatingContrastValueCode,
        skos:Concept ;
    skos:definition "Surface of coatings contrasts strongly in smoothness or colour with the adjacent surfaces. Outlines of fine sand grains are not visible. Lamellae are more than 5 mm thick." ;
    skos:inScheme glosis_cl:coatingContrastValueCode ;
    skos:notation "P" ;
    skos:prefLabel "Prominent"@en ;
    skos:topConceptOf glosis_cl:coatingContrastValueCode .

glosis_cl:coatingFormValueCode-C a glosis_cl:CoatingFormValueCode,
        skos:Concept ;
    skos:definition "Continuous form coatings" ;
    skos:inScheme glosis_cl:coatingFormValueCode ;
    skos:notation "C" ;
    skos:prefLabel "Continuous"@en ;
    skos:topConceptOf glosis_cl:coatingFormValueCode .

glosis_cl:coatingFormValueCode-CI a glosis_cl:CoatingFormValueCode,
        skos:Concept ;
    skos:definition "Continuous irregular (non-uniform, heterogeneous)form coatings" ;
    skos:inScheme glosis_cl:coatingFormValueCode ;
    skos:notation "CI" ;
    skos:prefLabel "Continuous irregular (non-uniform, heterogeneous)"@en ;
    skos:topConceptOf glosis_cl:coatingFormValueCode .

glosis_cl:coatingFormValueCode-DC a glosis_cl:CoatingFormValueCode,
        skos:Concept ;
    skos:definition "Discontinuous circular form coatings" ;
    skos:inScheme glosis_cl:coatingFormValueCode ;
    skos:notation "DC" ;
    skos:prefLabel "Discontinuous circular"@en ;
    skos:topConceptOf glosis_cl:coatingFormValueCode .

glosis_cl:coatingFormValueCode-DE a glosis_cl:CoatingFormValueCode,
        skos:Concept ;
    skos:definition "Dendroidal form coatings" ;
    skos:inScheme glosis_cl:coatingFormValueCode ;
    skos:notation "DE" ;
    skos:prefLabel "Dendroidal"@en ;
    skos:topConceptOf glosis_cl:coatingFormValueCode .

glosis_cl:coatingFormValueCode-DI a glosis_cl:CoatingFormValueCode,
        skos:Concept ;
    skos:definition "Discontinuous irregular form coatings" ;
    skos:inScheme glosis_cl:coatingFormValueCode ;
    skos:notation "DI" ;
    skos:prefLabel "Discontinuous irregular"@en ;
    skos:topConceptOf glosis_cl:coatingFormValueCode .

glosis_cl:coatingFormValueCode-O a glosis_cl:CoatingFormValueCode,
        skos:Concept ;
    skos:definition "Other kind of form coatings" ;
    skos:inScheme glosis_cl:coatingFormValueCode ;
    skos:notation "O" ;
    skos:prefLabel "Other"@en ;
    skos:topConceptOf glosis_cl:coatingFormValueCode .

glosis_cl:coatingLocationValueCode-BR a glosis_cl:CoatingLocationValueCode,
        skos:Concept ;
    skos:definition "Location of coatings and clay accumulation in the form of bridges between sand grains" ;
    skos:inScheme glosis_cl:coatingLocationValueCode ;
    skos:notation "BR" ;
    skos:prefLabel "Bridges between sand grains"@en ;
    skos:topConceptOf glosis_cl:coatingLocationValueCode .

glosis_cl:coatingLocationValueCode-CF a glosis_cl:CoatingLocationValueCode,
        skos:Concept ;
    skos:definition "Location of coatings and clay accumulation in the form of coarse fragments" ;
    skos:inScheme glosis_cl:coatingLocationValueCode ;
    skos:notation "CF" ;
    skos:prefLabel "Coarse fragments"@en ;
    skos:topConceptOf glosis_cl:coatingLocationValueCode .

glosis_cl:coatingLocationValueCode-LA a glosis_cl:CoatingLocationValueCode,
        skos:Concept ;
    skos:definition "Location of coatings and clay accumulation in the form of Lamellae (clay bands)" ;
    skos:inScheme glosis_cl:coatingLocationValueCode ;
    skos:notation "LA" ;
    skos:prefLabel "Lamellae (clay bands)"@en ;
    skos:topConceptOf glosis_cl:coatingLocationValueCode .

glosis_cl:coatingLocationValueCode-NS a glosis_cl:CoatingLocationValueCode,
        skos:Concept ;
    skos:definition "No specific location of coatings and clay accumulation" ;
    skos:inScheme glosis_cl:coatingLocationValueCode ;
    skos:notation "NS" ;
    skos:prefLabel "No specific location"@en ;
    skos:topConceptOf glosis_cl:coatingLocationValueCode .

glosis_cl:coatingLocationValueCode-P a glosis_cl:CoatingLocationValueCode,
        skos:Concept ;
    skos:definition "Location of coatings and clay accumulation in the form of Pedfaces" ;
    skos:inScheme glosis_cl:coatingLocationValueCode ;
    skos:notation "P" ;
    skos:prefLabel "Pedfaces"@en ;
    skos:topConceptOf glosis_cl:coatingLocationValueCode .

glosis_cl:coatingLocationValueCode-PH a glosis_cl:CoatingLocationValueCode,
        skos:Concept ;
    skos:definition "Location of coatings and clay accumulation in the form of horizontal pedfaces" ;
    skos:inScheme glosis_cl:coatingLocationValueCode ;
    skos:notation "PH" ;
    skos:prefLabel "Horizontal pedfaces"@en ;
    skos:topConceptOf glosis_cl:coatingLocationValueCode .

glosis_cl:coatingLocationValueCode-PV a glosis_cl:CoatingLocationValueCode,
        skos:Concept ;
    skos:definition "Location of coatings and clay accumulation in the form of vertical pedfaces" ;
    skos:inScheme glosis_cl:coatingLocationValueCode ;
    skos:notation "PV" ;
    skos:prefLabel "Vertical pedfaces"@en ;
    skos:topConceptOf glosis_cl:coatingLocationValueCode .

glosis_cl:coatingLocationValueCode-VO a glosis_cl:CoatingLocationValueCode,
        skos:Concept ;
    skos:definition "Location of coatings and clay accumulation in the form of voids" ;
    skos:inScheme glosis_cl:coatingLocationValueCode ;
    skos:notation "VO" ;
    skos:prefLabel "Voids"@en ;
    skos:topConceptOf glosis_cl:coatingLocationValueCode .

glosis_cl:coatingNatureValueCode-C a glosis_cl:CoatingNatureValueCode,
        skos:Concept ;
    skos:definition "Clay" ;
    skos:inScheme glosis_cl:coatingNatureValueCode ;
    skos:notation "C" ;
    skos:prefLabel "Clay"@en ;
    skos:topConceptOf glosis_cl:coatingNatureValueCode .

glosis_cl:coatingNatureValueCode-CC a glosis_cl:CoatingNatureValueCode,
        skos:Concept ;
    skos:definition "Calcium carbonate" ;
    skos:inScheme glosis_cl:coatingNatureValueCode ;
    skos:notation "CC" ;
    skos:prefLabel "Calcium carbonate"@en ;
    skos:topConceptOf glosis_cl:coatingNatureValueCode .

glosis_cl:coatingNatureValueCode-CH a glosis_cl:CoatingNatureValueCode,
        skos:Concept ;
    skos:definition "Clay and humus (organic matter)" ;
    skos:inScheme glosis_cl:coatingNatureValueCode ;
    skos:notation "CH" ;
    skos:prefLabel "Clay and humus (organic matter)"@en ;
    skos:topConceptOf glosis_cl:coatingNatureValueCode .

glosis_cl:coatingNatureValueCode-CS a glosis_cl:CoatingNatureValueCode,
        skos:Concept ;
    skos:definition "Clay and sesquioxides" ;
    skos:inScheme glosis_cl:coatingNatureValueCode ;
    skos:notation "CS" ;
    skos:prefLabel "Clay and sesquioxides"@en ;
    skos:topConceptOf glosis_cl:coatingNatureValueCode .

glosis_cl:coatingNatureValueCode-GB a glosis_cl:CoatingNatureValueCode,
        skos:Concept ;
    skos:definition "Gibbsite" ;
    skos:inScheme glosis_cl:coatingNatureValueCode ;
    skos:notation "GB" ;
    skos:prefLabel "Gibbsite"@en ;
    skos:topConceptOf glosis_cl:coatingNatureValueCode .

glosis_cl:coatingNatureValueCode-H a glosis_cl:CoatingNatureValueCode,
        skos:Concept ;
    skos:definition "Humus" ;
    skos:inScheme glosis_cl:coatingNatureValueCode ;
    skos:notation "H" ;
    skos:prefLabel "Humus"@en ;
    skos:topConceptOf glosis_cl:coatingNatureValueCode .

glosis_cl:coatingNatureValueCode-HC a glosis_cl:CoatingNatureValueCode,
        skos:Concept ;
    skos:definition "Hypodermic coatings (Hypodermic coatings, as used here, are field-scale features, commonly only expressed as hydromorphic features. Micromorphological hypodermic coatings include non-redox features [Bullock et al., 1985].)" ;
    skos:inScheme glosis_cl:coatingNatureValueCode ;
    skos:notation "HC" ;
    skos:prefLabel "Hypodermic coatings (Hypodermic coatings, as used here, are field-scale features, commonly only expressed as hydromorphic features. Micromorphological hypodermic coatings include non-redox features [Bullock et al., 1985].)"@en ;
    skos:topConceptOf glosis_cl:coatingNatureValueCode .

glosis_cl:coatingNatureValueCode-JA a glosis_cl:CoatingNatureValueCode,
        skos:Concept ;
    skos:definition "Jarosite" ;
    skos:inScheme glosis_cl:coatingNatureValueCode ;
    skos:notation "JA" ;
    skos:prefLabel "Jarosite"@en ;
    skos:topConceptOf glosis_cl:coatingNatureValueCode .

glosis_cl:coatingNatureValueCode-MN a glosis_cl:CoatingNatureValueCode,
        skos:Concept ;
    skos:definition "Manganese" ;
    skos:inScheme glosis_cl:coatingNatureValueCode ;
    skos:notation "MN" ;
    skos:prefLabel "Manganese"@en ;
    skos:topConceptOf glosis_cl:coatingNatureValueCode .

glosis_cl:coatingNatureValueCode-PF a glosis_cl:CoatingNatureValueCode,
        skos:Concept ;
    skos:definition "Pressure faces" ;
    skos:inScheme glosis_cl:coatingNatureValueCode ;
    skos:notation "PF" ;
    skos:prefLabel "Pressure faces"@en ;
    skos:topConceptOf glosis_cl:coatingNatureValueCode .

glosis_cl:coatingNatureValueCode-S a glosis_cl:CoatingNatureValueCode,
        skos:Concept ;
    skos:definition "Sesquioxides" ;
    skos:inScheme glosis_cl:coatingNatureValueCode ;
    skos:notation "S" ;
    skos:prefLabel "Sesquioxides"@en ;
    skos:topConceptOf glosis_cl:coatingNatureValueCode .

glosis_cl:coatingNatureValueCode-SA a glosis_cl:CoatingNatureValueCode,
        skos:Concept ;
    skos:definition "Sand coatings" ;
    skos:inScheme glosis_cl:coatingNatureValueCode ;
    skos:notation "SA" ;
    skos:prefLabel "Sand coatings"@en ;
    skos:topConceptOf glosis_cl:coatingNatureValueCode .

glosis_cl:coatingNatureValueCode-SF a glosis_cl:CoatingNatureValueCode,
        skos:Concept ;
    skos:definition "Shiny faces (as in nitic horizon)" ;
    skos:inScheme glosis_cl:coatingNatureValueCode ;
    skos:notation "SF" ;
    skos:prefLabel "Shiny faces (as in nitic horizon)"@en ;
    skos:topConceptOf glosis_cl:coatingNatureValueCode .

glosis_cl:coatingNatureValueCode-SI a glosis_cl:CoatingNatureValueCode,
        skos:Concept ;
    skos:definition "Slickensides, predominantly intersecting (Slickensides are polished and grooved ped surfaces that are produced by aggregates sliding one past another.)" ;
    skos:inScheme glosis_cl:coatingNatureValueCode ;
    skos:notation "SI" ;
    skos:prefLabel "Slickensides, predominantly intersecting (Slickensides are polished and grooved ped surfaces that are produced by aggregates sliding one past another.)"@en ;
    skos:topConceptOf glosis_cl:coatingNatureValueCode .

glosis_cl:coatingNatureValueCode-SL a glosis_cl:CoatingNatureValueCode,
        skos:Concept ;
    skos:definition "Silica (opal)" ;
    skos:inScheme glosis_cl:coatingNatureValueCode ;
    skos:notation "SL" ;
    skos:prefLabel "Silica (opal)"@en ;
    skos:topConceptOf glosis_cl:coatingNatureValueCode .

glosis_cl:coatingNatureValueCode-SN a glosis_cl:CoatingNatureValueCode,
        skos:Concept ;
    skos:definition "Slickensides, non intersecting" ;
    skos:inScheme glosis_cl:coatingNatureValueCode ;
    skos:notation "SN" ;
    skos:prefLabel "Slickensides, non intersecting"@en ;
    skos:topConceptOf glosis_cl:coatingNatureValueCode .

glosis_cl:coatingNatureValueCode-SP a glosis_cl:CoatingNatureValueCode,
        skos:Concept ;
    skos:definition "Slickensides, partly intersecting" ;
    skos:inScheme glosis_cl:coatingNatureValueCode ;
    skos:notation "SP" ;
    skos:prefLabel "Slickensides, partly intersecting"@en ;
    skos:topConceptOf glosis_cl:coatingNatureValueCode .

glosis_cl:coatingNatureValueCode-ST a glosis_cl:CoatingNatureValueCode,
        skos:Concept ;
    skos:definition "Silt coatings" ;
    skos:inScheme glosis_cl:coatingNatureValueCode ;
    skos:notation "ST" ;
    skos:prefLabel "Silt coatings"@en ;
    skos:topConceptOf glosis_cl:coatingNatureValueCode .

glosis_cl:consistenceDryValueCode-EHA a glosis_cl:ConsistenceDryValueCode,
        skos:Concept ;
    skos:definition "Extremely resistant to pressure; cannot be broken in the hands." ;
    skos:inScheme glosis_cl:consistenceDryValueCode ;
    skos:notation "EHA" ;
    skos:prefLabel "Extremely hard"@en ;
    skos:topConceptOf glosis_cl:consistenceDryValueCode .

glosis_cl:consistenceDryValueCode-HA a glosis_cl:ConsistenceDryValueCode,
        skos:Concept ;
    skos:definition "Moderately resistant to pressure; can be broken in the hands; not breakable between thumb and forefinger." ;
    skos:inScheme glosis_cl:consistenceDryValueCode ;
    skos:notation "HA" ;
    skos:prefLabel "Hard"@en ;
    skos:topConceptOf glosis_cl:consistenceDryValueCode .

glosis_cl:consistenceDryValueCode-HVH a glosis_cl:ConsistenceDryValueCode,
        skos:Concept ;
    skos:definition "Additional code formed by combining HA and VHA" ;
    skos:inScheme glosis_cl:consistenceDryValueCode ;
    skos:notation "HVH" ;
    skos:prefLabel "hard to very hard"@en ;
    skos:topConceptOf glosis_cl:consistenceDryValueCode .

glosis_cl:consistenceDryValueCode-LO a glosis_cl:ConsistenceDryValueCode,
        skos:Concept ;
    skos:definition "Non-coherent." ;
    skos:inScheme glosis_cl:consistenceDryValueCode ;
    skos:notation "LO" ;
    skos:prefLabel "Loose"@en ;
    skos:topConceptOf glosis_cl:consistenceDryValueCode .

glosis_cl:consistenceDryValueCode-SHA a glosis_cl:ConsistenceDryValueCode,
        skos:Concept ;
    skos:definition "Weakly resistant to pressure; easily broken between thumb and forefinger." ;
    skos:inScheme glosis_cl:consistenceDryValueCode ;
    skos:notation "SHA" ;
    skos:prefLabel "Slightly hard"@en ;
    skos:topConceptOf glosis_cl:consistenceDryValueCode .

glosis_cl:consistenceDryValueCode-SHH a glosis_cl:ConsistenceDryValueCode,
        skos:Concept ;
    skos:definition "slightly hard to hard" ;
    skos:inScheme glosis_cl:consistenceDryValueCode ;
    skos:notation "SHH" ;
    skos:prefLabel "slightly hard to hard"@en ;
    skos:topConceptOf glosis_cl:consistenceDryValueCode .

glosis_cl:consistenceDryValueCode-SO a glosis_cl:ConsistenceDryValueCode,
        skos:Concept ;
    skos:definition "Soil mass is very weakly coherent and fragile; breaks to powder or individual grains under very slight pressure." ;
    skos:inScheme glosis_cl:consistenceDryValueCode ;
    skos:notation "SO" ;
    skos:prefLabel "Soft"@en ;
    skos:topConceptOf glosis_cl:consistenceDryValueCode .

glosis_cl:consistenceDryValueCode-SSH a glosis_cl:ConsistenceDryValueCode,
        skos:Concept ;
    skos:definition "soft to slightly hard" ;
    skos:inScheme glosis_cl:consistenceDryValueCode ;
    skos:notation "SSH" ;
    skos:prefLabel "soft to slightly hard"@en ;
    skos:topConceptOf glosis_cl:consistenceDryValueCode .

glosis_cl:consistenceDryValueCode-VHA a glosis_cl:ConsistenceDryValueCode,
        skos:Concept ;
    skos:definition "Very hard Very resistant to pressure; can be broken in the hands only with difficulty." ;
    skos:inScheme glosis_cl:consistenceDryValueCode ;
    skos:notation "VHA" ;
    skos:prefLabel "Very hard"@en ;
    skos:topConceptOf glosis_cl:consistenceDryValueCode .

glosis_cl:consistenceMoistValueCode-EFI a glosis_cl:ConsistenceMoistValueCode,
        skos:Concept ;
    skos:definition "Soil material crushes only under very strong pressure; cannot be crushed between thumb and forefinger." ;
    skos:inScheme glosis_cl:consistenceMoistValueCode ;
    skos:notation "EFI" ;
    skos:prefLabel "Extremely firm"@en ;
    skos:topConceptOf glosis_cl:consistenceMoistValueCode .

glosis_cl:consistenceMoistValueCode-FI a glosis_cl:ConsistenceMoistValueCode,
        skos:Concept ;
    skos:definition "Soil material crushes under moderate pressure between thumb and forefinger, but resistance is distinctly noticeable." ;
    skos:inScheme glosis_cl:consistenceMoistValueCode ;
    skos:notation "FI" ;
    skos:prefLabel "Firm"@en ;
    skos:topConceptOf glosis_cl:consistenceMoistValueCode .

glosis_cl:consistenceMoistValueCode-FR a glosis_cl:ConsistenceMoistValueCode,
        skos:Concept ;
    skos:definition "Soil material crushes easily under gentle to moderate pressure between thumb and forefinger, and coheres when pressed together." ;
    skos:inScheme glosis_cl:consistenceMoistValueCode ;
    skos:notation "FR" ;
    skos:prefLabel "Friable"@en ;
    skos:topConceptOf glosis_cl:consistenceMoistValueCode .

glosis_cl:consistenceMoistValueCode-LO a glosis_cl:ConsistenceMoistValueCode,
        skos:Concept ;
    skos:definition "Non-coherent." ;
    skos:inScheme glosis_cl:consistenceMoistValueCode ;
    skos:notation "LO" ;
    skos:prefLabel "Loose"@en ;
    skos:topConceptOf glosis_cl:consistenceMoistValueCode .

glosis_cl:consistenceMoistValueCode-VFI a glosis_cl:ConsistenceMoistValueCode,
        skos:Concept ;
    skos:definition "Soil material crushes under strong pressures; barely crushable between thumb and forefinger." ;
    skos:inScheme glosis_cl:consistenceMoistValueCode ;
    skos:notation "VFI" ;
    skos:prefLabel "Very firm"@en ;
    skos:topConceptOf glosis_cl:consistenceMoistValueCode .

glosis_cl:consistenceMoistValueCode-VFR a glosis_cl:ConsistenceMoistValueCode,
        skos:Concept ;
    skos:definition "Soil material crushes under very gentle pressure, but coheres when pressed together." ;
    skos:inScheme glosis_cl:consistenceMoistValueCode ;
    skos:notation "VFR" ;
    skos:prefLabel "Very friable"@en ;
    skos:topConceptOf glosis_cl:consistenceMoistValueCode .

glosis_cl:contrastValueCode-D a glosis_cl:ContrastValueCode,
        skos:Concept ;
    skos:definition "Although not striking, the mottles are readily seen. The hue, chroma and value of the matrix are easily distinguished from those of the mottles. They may vary by as much as 2.5 units of hue or several units in chroma or value." ;
    skos:inScheme glosis_cl:contrastValueCode ;
    skos:notation "D" ;
    skos:prefLabel "Distinct"@en ;
    skos:topConceptOf glosis_cl:contrastValueCode .

glosis_cl:contrastValueCode-F a glosis_cl:ContrastValueCode,
        skos:Concept ;
    skos:definition "The mottles are evident only on close examination. Soil colours in both the matrix and mottles have closely related hues, chromas and values." ;
    skos:inScheme glosis_cl:contrastValueCode ;
    skos:notation "F" ;
    skos:prefLabel "Faint"@en ;
    skos:topConceptOf glosis_cl:contrastValueCode .

glosis_cl:contrastValueCode-P a glosis_cl:ContrastValueCode,
        skos:Concept ;
    skos:definition "The mottles are conspicuous and mottling is one of the outstanding features of the horizon. Hue, chroma and value alone or in combination are at least several units apart." ;
    skos:inScheme glosis_cl:contrastValueCode ;
    skos:notation "P" ;
    skos:prefLabel "Prominent"@en ;
    skos:topConceptOf glosis_cl:contrastValueCode .

glosis_cl:cracksDepthValueCode-D a glosis_cl:CracksDepthValueCode,
        skos:Concept ;
    skos:definition "Deep surface crack of 10 - 20 cm in depth" ;
    skos:inScheme glosis_cl:cracksDepthValueCode ;
    skos:notation "D" ;
    skos:prefLabel "Deep 10–20"@en ;
    skos:topConceptOf glosis_cl:cracksDepthValueCode .

glosis_cl:cracksDepthValueCode-M a glosis_cl:CracksDepthValueCode,
        skos:Concept ;
    skos:definition "Medium surface crack of 2 - 10 cm in depth" ;
    skos:inScheme glosis_cl:cracksDepthValueCode ;
    skos:notation "M" ;
    skos:prefLabel "Medium 2–10"@en ;
    skos:topConceptOf glosis_cl:cracksDepthValueCode .

glosis_cl:cracksDepthValueCode-S a glosis_cl:CracksDepthValueCode,
        skos:Concept ;
    skos:definition "Surface crack less than 2 cm in depth" ;
    skos:inScheme glosis_cl:cracksDepthValueCode ;
    skos:notation "S" ;
    skos:prefLabel "Surface < 2"@en ;
    skos:topConceptOf glosis_cl:cracksDepthValueCode .

glosis_cl:cracksDepthValueCode-V a glosis_cl:CracksDepthValueCode,
        skos:Concept ;
    skos:definition "Very deep surface crack of more than 20 cm in depth" ;
    skos:inScheme glosis_cl:cracksDepthValueCode ;
    skos:notation "V" ;
    skos:prefLabel "Very deep > 20"@en ;
    skos:topConceptOf glosis_cl:cracksDepthValueCode .

glosis_cl:cracksDistanceValueCode-C a glosis_cl:CracksDistanceValueCode,
        skos:Concept ;
    skos:definition "Very closely spaced surface crack with distance less than 0.2 m" ;
    skos:inScheme glosis_cl:cracksDistanceValueCode ;
    skos:notation "C" ;
    skos:prefLabel "Very closely spaced < 0.2"@en ;
    skos:topConceptOf glosis_cl:cracksDistanceValueCode .

glosis_cl:cracksDistanceValueCode-D a glosis_cl:CracksDistanceValueCode,
        skos:Concept ;
    skos:definition "Closely spaced surface crack with distance between 0.2 - 0.5 m" ;
    skos:inScheme glosis_cl:cracksDistanceValueCode ;
    skos:notation "D" ;
    skos:prefLabel "Closely spaced 0.2–0.5"@en ;
    skos:topConceptOf glosis_cl:cracksDistanceValueCode .

glosis_cl:cracksDistanceValueCode-M a glosis_cl:CracksDistanceValueCode,
        skos:Concept ;
    skos:definition "Moderately widely spaced surface crack with distance between 0.5–2 m" ;
    skos:inScheme glosis_cl:cracksDistanceValueCode ;
    skos:notation "M" ;
    skos:prefLabel "Moderately widely spaced 0.5–2"@en ;
    skos:topConceptOf glosis_cl:cracksDistanceValueCode .

glosis_cl:cracksDistanceValueCode-V a glosis_cl:CracksDistanceValueCode,
        skos:Concept ;
    skos:definition "Very widely spaced surface crack with distance more than 5 m" ;
    skos:inScheme glosis_cl:cracksDistanceValueCode ;
    skos:notation "V" ;
    skos:prefLabel "Very widely spaced > 5"@en ;
    skos:topConceptOf glosis_cl:cracksDistanceValueCode .

glosis_cl:cracksDistanceValueCode-W a glosis_cl:CracksDistanceValueCode,
        skos:Concept ;
    skos:definition "Widely spaced surface crack with distance between 2–5 m" ;
    skos:inScheme glosis_cl:cracksDistanceValueCode ;
    skos:notation "W" ;
    skos:prefLabel "Widely spaced 2–5"@en ;
    skos:topConceptOf glosis_cl:cracksDistanceValueCode .

glosis_cl:cracksWidthValueCode-E a glosis_cl:CracksWidthValueCode,
        skos:Concept ;
    skos:definition "Extremely wide surface crack with width more than 10cm" ;
    skos:inScheme glosis_cl:cracksWidthValueCode ;
    skos:notation "E" ;
    skos:prefLabel "Extremely wide > 10cm"@en ;
    skos:topConceptOf glosis_cl:cracksWidthValueCode .

glosis_cl:cracksWidthValueCode-F a glosis_cl:CracksWidthValueCode,
        skos:Concept ;
    skos:definition "Fine surface crack with width less than 1 cm" ;
    skos:inScheme glosis_cl:cracksWidthValueCode ;
    skos:notation "F" ;
    skos:prefLabel "Fine < 1cm"@en ;
    skos:topConceptOf glosis_cl:cracksWidthValueCode .

glosis_cl:cracksWidthValueCode-M a glosis_cl:CracksWidthValueCode,
        skos:Concept ;
    skos:definition "Medium surface crack with width 1 - 2 cm" ;
    skos:inScheme glosis_cl:cracksWidthValueCode ;
    skos:notation "M" ;
    skos:prefLabel "Medium 1cm–2cm"@en ;
    skos:topConceptOf glosis_cl:cracksWidthValueCode .

glosis_cl:cracksWidthValueCode-V a glosis_cl:CracksWidthValueCode,
        skos:Concept ;
    skos:definition "Very wide surface crack with width 5cm - 10 cm" ;
    skos:inScheme glosis_cl:cracksWidthValueCode ;
    skos:notation "V" ;
    skos:prefLabel "Very wide 5cm–10cm"@en ;
    skos:topConceptOf glosis_cl:cracksWidthValueCode .

glosis_cl:cracksWidthValueCode-W a glosis_cl:CracksWidthValueCode,
        skos:Concept ;
    skos:definition "Wide surface crack with width 2 - 5 cm" ;
    skos:inScheme glosis_cl:cracksWidthValueCode ;
    skos:notation "W" ;
    skos:prefLabel "Wide 2cm–5cm"@en ;
    skos:topConceptOf glosis_cl:cracksWidthValueCode .

glosis_cl:cropClassValueCode-Ce a glosis_cl:CropClassValueCode,
        skos:Concept ;
    skos:definition "Crop code for Cereals class" ;
    skos:inScheme glosis_cl:cropClassValueCode ;
    skos:narrower glosis_cl:cropClassValueCode-Ce_Ba,
        glosis_cl:cropClassValueCode-Ce_Ma,
        glosis_cl:cropClassValueCode-Ce_Mi,
        glosis_cl:cropClassValueCode-Ce_Oa,
        glosis_cl:cropClassValueCode-Ce_Pa,
        glosis_cl:cropClassValueCode-Ce_Ri,
        glosis_cl:cropClassValueCode-Ce_Ry,
        glosis_cl:cropClassValueCode-Ce_So,
        glosis_cl:cropClassValueCode-Ce_Wh ;
    skos:notation "Ce" ;
    skos:prefLabel "Cereals"@en ;
    skos:topConceptOf glosis_cl:cropClassValueCode .

glosis_cl:cropClassValueCode-Ce_Ba a glosis_cl:CropClassValueCode,
        skos:Concept ;
    skos:broader glosis_cl:cropClassValueCode-Ce ;
    skos:definition "Crop code for Barley from Cereal class" ;
    skos:inScheme glosis_cl:cropClassValueCode ;
    skos:notation "Ce_Ba" ;
    skos:prefLabel "Barley"@en .

glosis_cl:cropClassValueCode-Ce_Ma a glosis_cl:CropClassValueCode,
        skos:Concept ;
    skos:broader glosis_cl:cropClassValueCode-Ce ;
    skos:definition "Crop code for Maize from Cereals class" ;
    skos:inScheme glosis_cl:cropClassValueCode ;
    skos:notation "Ce_Ma" ;
    skos:prefLabel "Maize"@en .

glosis_cl:cropClassValueCode-Ce_Mi a glosis_cl:CropClassValueCode,
        skos:Concept ;
    skos:broader glosis_cl:cropClassValueCode-Ce ;
    skos:definition "Crop code for Millet from Cereal class" ;
    skos:inScheme glosis_cl:cropClassValueCode ;
    skos:notation "Ce_Mi" ;
    skos:prefLabel "Millet"@en .

glosis_cl:cropClassValueCode-Ce_Oa a glosis_cl:CropClassValueCode,
        skos:Concept ;
    skos:broader glosis_cl:cropClassValueCode-Ce ;
    skos:definition "Crop code for Oats from Cereals class" ;
    skos:inScheme glosis_cl:cropClassValueCode ;
    skos:notation "Ce_Oa" ;
    skos:prefLabel "Oats"@en .

glosis_cl:cropClassValueCode-Ce_Pa a glosis_cl:CropClassValueCode,
        skos:Concept ;
    skos:broader glosis_cl:cropClassValueCode-Ce ;
    skos:definition "Crop code for Rice and paddy from Cereal class" ;
    skos:inScheme glosis_cl:cropClassValueCode ;
    skos:notation "Ce_Pa" ;
    skos:prefLabel "Rice, paddy"@en .

glosis_cl:cropClassValueCode-Ce_Ri a glosis_cl:CropClassValueCode,
        skos:Concept ;
    skos:broader glosis_cl:cropClassValueCode-Ce ;
    skos:definition "Crop code for Rice(dry) from Cereal class" ;
    skos:inScheme glosis_cl:cropClassValueCode ;
    skos:notation "Ce_Ra" ;
    skos:prefLabel "Rice, dry"@en .

glosis_cl:cropClassValueCode-Ce_Ry a glosis_cl:CropClassValueCode,
        skos:Concept ;
    skos:broader glosis_cl:cropClassValueCode-Ce ;
    skos:definition "Crop code for Rye from Cereal class" ;
    skos:inScheme glosis_cl:cropClassValueCode ;
    skos:notation "Ce_Ry" ;
    skos:prefLabel "Rye"@en .

glosis_cl:cropClassValueCode-Ce_So a glosis_cl:CropClassValueCode,
        skos:Concept ;
    skos:broader glosis_cl:cropClassValueCode-Ce ;
    skos:definition "Crop code for Sorghum from Cereals class" ;
    skos:inScheme glosis_cl:cropClassValueCode ;
    skos:notation "Ce_So" ;
    skos:prefLabel "Sorghum"@en .

glosis_cl:cropClassValueCode-Ce_Wh a glosis_cl:CropClassValueCode,
        skos:Concept ;
    skos:broader glosis_cl:cropClassValueCode-Ce ;
    skos:definition "Crop code for Wheat from Cereal class" ;
    skos:inScheme glosis_cl:cropClassValueCode ;
    skos:notation "Ce_Wh" ;
    skos:prefLabel "Wheat"@en .

glosis_cl:cropClassValueCode-Fi a glosis_cl:CropClassValueCode,
        skos:Concept ;
    skos:definition "Crop code for Fibre crops class" ;
    skos:inScheme glosis_cl:cropClassValueCode ;
    skos:narrower glosis_cl:cropClassValueCode-Fi_Co,
        glosis_cl:cropClassValueCode-Fi_Ju ;
    skos:notation "Fi" ;
    skos:prefLabel "Fibre crops"@en ;
    skos:topConceptOf glosis_cl:cropClassValueCode .

glosis_cl:cropClassValueCode-Fi_Co a glosis_cl:CropClassValueCode,
        skos:Concept ;
    skos:broader glosis_cl:cropClassValueCode-Fi ;
    skos:definition "Crop code for Cotton from Fiber crops class" ;
    skos:inScheme glosis_cl:cropClassValueCode ;
    skos:notation "Fi_Co" ;
    skos:prefLabel "Cotton"@en .

glosis_cl:cropClassValueCode-Fi_Ju a glosis_cl:CropClassValueCode,
        skos:Concept ;
    skos:broader glosis_cl:cropClassValueCode-Fi ;
    skos:definition "Crop code for Jute from Fiber crops class" ;
    skos:inScheme glosis_cl:cropClassValueCode ;
    skos:notation "Fi_Ju" ;
    skos:prefLabel "Jute"@en .

glosis_cl:cropClassValueCode-Fo a glosis_cl:CropClassValueCode,
        skos:Concept ;
    skos:definition "Crop code for Fodder plants class" ;
    skos:inScheme glosis_cl:cropClassValueCode ;
    skos:narrower glosis_cl:cropClassValueCode-Fo_Al,
        glosis_cl:cropClassValueCode-Fo_Cl,
        glosis_cl:cropClassValueCode-Fo_Gr,
        glosis_cl:cropClassValueCode-Fo_Ha,
        glosis_cl:cropClassValueCode-Fo_Le,
        glosis_cl:cropClassValueCode-Fo_Ma,
        glosis_cl:cropClassValueCode-Fo_Pu ;
    skos:notation "Fo" ;
    skos:prefLabel "Fodder plants"@en ;
    skos:topConceptOf glosis_cl:cropClassValueCode .

glosis_cl:cropClassValueCode-Fo_Al a glosis_cl:CropClassValueCode,
        skos:Concept ;
    skos:broader glosis_cl:cropClassValueCode-Fo ;
    skos:definition "Crop code for Alfalfa from fodder plants class" ;
    skos:inScheme glosis_cl:cropClassValueCode ;
    skos:notation "Fo_Al" ;
    skos:prefLabel "Alfalfa"@en .

glosis_cl:cropClassValueCode-Fo_Cl a glosis_cl:CropClassValueCode,
        skos:Concept ;
    skos:broader glosis_cl:cropClassValueCode-Fo ;
    skos:definition "Crop code for Clover from Fodder class" ;
    skos:inScheme glosis_cl:cropClassValueCode ;
    skos:notation "Fo_Cl" ;
    skos:prefLabel "Clover"@en .

glosis_cl:cropClassValueCode-Fo_Gr a glosis_cl:CropClassValueCode,
        skos:Concept ;
    skos:broader glosis_cl:cropClassValueCode-Fo ;
    skos:definition "Crop code for Grasses from Fodder plants class" ;
    skos:inScheme glosis_cl:cropClassValueCode ;
    skos:notation "Fo_Gr" ;
    skos:prefLabel "Grasses"@en .

glosis_cl:cropClassValueCode-Fo_Ha a glosis_cl:CropClassValueCode,
        skos:Concept ;
    skos:broader glosis_cl:cropClassValueCode-Fo ;
    skos:definition "Crop code for Hay from Fodder class" ;
    skos:inScheme glosis_cl:cropClassValueCode ;
    skos:notation "Fo_Ha" ;
    skos:prefLabel "Hay"@en .

glosis_cl:cropClassValueCode-Fo_Le a glosis_cl:CropClassValueCode,
        skos:Concept ;
    skos:broader glosis_cl:cropClassValueCode-Fo ;
    skos:definition "Crop code for Leguminous from fodder plants class" ;
    skos:inScheme glosis_cl:cropClassValueCode ;
    skos:notation "Fo_Le" ;
    skos:prefLabel "Leguminous"@en .

glosis_cl:cropClassValueCode-Fo_Ma a glosis_cl:CropClassValueCode,
        skos:Concept ;
    skos:broader glosis_cl:cropClassValueCode-Fo ;
    skos:definition "Crop code for Maize from Fodder plants class" ;
    skos:inScheme glosis_cl:cropClassValueCode ;
    skos:notation "Fo_Ma" ;
    skos:prefLabel "Maize"@en .

glosis_cl:cropClassValueCode-Fo_Pu a glosis_cl:CropClassValueCode,
        skos:Concept ;
    skos:broader glosis_cl:cropClassValueCode-Fo ;
    skos:definition "Crop code for Pumpkins from Fruits and melons class" ;
    skos:inScheme glosis_cl:cropClassValueCode ;
    skos:notation "Fo_Pu" ;
    skos:prefLabel "Pumpkins"@en .

glosis_cl:cropClassValueCode-Fr a glosis_cl:CropClassValueCode,
        skos:Concept ;
    skos:definition "Crop code for Fruits and melons class" ;
    skos:inScheme glosis_cl:cropClassValueCode ;
    skos:narrower glosis_cl:cropClassValueCode-Fr_Ap,
        glosis_cl:cropClassValueCode-Fr_Ba,
        glosis_cl:cropClassValueCode-Fr_Ci,
        glosis_cl:cropClassValueCode-Fr_Gr,
        glosis_cl:cropClassValueCode-Fr_Ma,
        glosis_cl:cropClassValueCode-Fr_Me ;
    skos:notation "Fr" ;
    skos:prefLabel "Fruits and melons"@en ;
    skos:topConceptOf glosis_cl:cropClassValueCode .

glosis_cl:cropClassValueCode-Fr_Ap a glosis_cl:CropClassValueCode,
        skos:Concept ;
    skos:broader glosis_cl:cropClassValueCode-Fr ;
    skos:definition "Crop code for Apples from Fruits and melons class" ;
    skos:inScheme glosis_cl:cropClassValueCode ;
    skos:notation "Fr_Ap" ;
    skos:prefLabel "Apples"@en .

glosis_cl:cropClassValueCode-Fr_Ba a glosis_cl:CropClassValueCode,
        skos:Concept ;
    skos:broader glosis_cl:cropClassValueCode-Fr ;
    skos:definition "Crop code for Bananas from Fruits and melons class" ;
    skos:inScheme glosis_cl:cropClassValueCode ;
    skos:notation "Fr_Ba" ;
    skos:prefLabel "Bananas"@en .

glosis_cl:cropClassValueCode-Fr_Ci a glosis_cl:CropClassValueCode,
        skos:Concept ;
    skos:broader glosis_cl:cropClassValueCode-Fr ;
    skos:definition "Crop code for Citrus from Fruits and melons class" ;
    skos:inScheme glosis_cl:cropClassValueCode ;
    skos:notation "Fr_Ci" ;
    skos:prefLabel "Citrus"@en .

glosis_cl:cropClassValueCode-Fr_Gr a glosis_cl:CropClassValueCode,
        skos:Concept ;
    skos:broader glosis_cl:cropClassValueCode-Fr ;
    skos:definition "Crop code for Grapes, Wine, Raisins from fruits and melons class" ;
    skos:inScheme glosis_cl:cropClassValueCode ;
    skos:notation "Fr_Gr" ;
    skos:prefLabel "Grapes, Wine, Raisins"@en .

glosis_cl:cropClassValueCode-Fr_Ma a glosis_cl:CropClassValueCode,
        skos:Concept ;
    skos:broader glosis_cl:cropClassValueCode-Fr ;
    skos:definition "Crop code for Mangoes from Fruits and melons class" ;
    skos:inScheme glosis_cl:cropClassValueCode ;
    skos:notation "Fr_Ma" ;
    skos:prefLabel "Mangoes"@en .

glosis_cl:cropClassValueCode-Fr_Me a glosis_cl:CropClassValueCode,
        skos:Concept ;
    skos:broader glosis_cl:cropClassValueCode-Fr ;
    skos:definition "Crop code for Melons from Fruits and melons class" ;
    skos:inScheme glosis_cl:cropClassValueCode ;
    skos:notation "Fr_Me" ;
    skos:prefLabel "Melons"@en .

glosis_cl:cropClassValueCode-Lu a glosis_cl:CropClassValueCode,
        skos:Concept ;
    skos:definition "Crop code for Semi-luxury foods and tobacco class" ;
    skos:inScheme glosis_cl:cropClassValueCode ;
    skos:narrower glosis_cl:cropClassValueCode-Lu_Cc,
        glosis_cl:cropClassValueCode-Lu_Co,
        glosis_cl:cropClassValueCode-Lu_Te,
        glosis_cl:cropClassValueCode-Lu_To ;
    skos:notation "Lu" ;
    skos:prefLabel "Semi-luxury foods and tobacco"@en ;
    skos:topConceptOf glosis_cl:cropClassValueCode .

glosis_cl:cropClassValueCode-Lu_Cc a glosis_cl:CropClassValueCode,
        skos:Concept ;
    skos:broader glosis_cl:cropClassValueCode-Lu ;
    skos:definition "Crop code for Cocoa from Semi-luxury foods and tobacco class" ;
    skos:inScheme glosis_cl:cropClassValueCode ;
    skos:notation "Lu_Cc" ;
    skos:prefLabel "Cocoa"@en .

glosis_cl:cropClassValueCode-Lu_Co a glosis_cl:CropClassValueCode,
        skos:Concept ;
    skos:broader glosis_cl:cropClassValueCode-Lu ;
    skos:definition "Crop code for Coffee from Semi-luxury foods and tobacco class" ;
    skos:inScheme glosis_cl:cropClassValueCode ;
    skos:notation "Lu_Co" ;
    skos:prefLabel "Coffee"@en .

glosis_cl:cropClassValueCode-Lu_Te a glosis_cl:CropClassValueCode,
        skos:Concept ;
    skos:broader glosis_cl:cropClassValueCode-Lu ;
    skos:definition "Crop code for Tea from Semi-luxury foods and tobacco class" ;
    skos:inScheme glosis_cl:cropClassValueCode ;
    skos:notation "Lu_Te" ;
    skos:prefLabel "Tea"@en .

glosis_cl:cropClassValueCode-Lu_To a glosis_cl:CropClassValueCode,
        skos:Concept ;
    skos:broader glosis_cl:cropClassValueCode-Lu ;
    skos:definition "Crop code for Tobacco from Semi-luxury foods and tobacco class" ;
    skos:inScheme glosis_cl:cropClassValueCode ;
    skos:notation "Lu_To" ;
    skos:prefLabel "Tobacco"@en .

glosis_cl:cropClassValueCode-Oi a glosis_cl:CropClassValueCode,
        skos:Concept ;
    skos:definition "Crop code for Oilcrops class" ;
    skos:inScheme glosis_cl:cropClassValueCode ;
    skos:narrower glosis_cl:cropClassValueCode-Oi_Cc,
        glosis_cl:cropClassValueCode-Oi_Gr,
        glosis_cl:cropClassValueCode-Oi_Li,
        glosis_cl:cropClassValueCode-Oi_Op,
        glosis_cl:cropClassValueCode-Oi_Ra,
        glosis_cl:cropClassValueCode-Oi_Se,
        glosis_cl:cropClassValueCode-Oi_So,
        glosis_cl:cropClassValueCode-Oi_Su,
        glosis_cl:cropClassValueCode-Ol ;
    skos:notation "Oi" ;
    skos:prefLabel "Oilcrops"@en ;
    skos:topConceptOf glosis_cl:cropClassValueCode .

glosis_cl:cropClassValueCode-Oi_Cc a glosis_cl:CropClassValueCode,
        skos:Concept ;
    skos:broader glosis_cl:cropClassValueCode-Oi ;
    skos:definition "Crop code for Coconuts from Oilcrops class" ;
    skos:inScheme glosis_cl:cropClassValueCode ;
    skos:notation "Oi_Cc" ;
    skos:prefLabel "Coconuts"@en .

glosis_cl:cropClassValueCode-Oi_Gr a glosis_cl:CropClassValueCode,
        skos:Concept ;
    skos:broader glosis_cl:cropClassValueCode-Oi ;
    skos:definition "Crop code for Groundnuts from Oilcrops class" ;
    skos:inScheme glosis_cl:cropClassValueCode ;
    skos:notation "Oi_Gr" ;
    skos:prefLabel "Groundnuts"@en .

glosis_cl:cropClassValueCode-Oi_Li a glosis_cl:CropClassValueCode,
        skos:Concept ;
    skos:broader glosis_cl:cropClassValueCode-Oi ;
    skos:definition "Crop code for Linseed class" ;
    skos:inScheme glosis_cl:cropClassValueCode ;
    skos:notation "Li" ;
    skos:prefLabel "Linseed"@en .

glosis_cl:cropClassValueCode-Oi_Op a glosis_cl:CropClassValueCode,
        skos:Concept ;
    skos:broader glosis_cl:cropClassValueCode-Oi ;
    skos:definition "Crop code for Oil-palm from Oilcrops class" ;
    skos:inScheme glosis_cl:cropClassValueCode ;
    skos:notation "Oi_Op" ;
    skos:prefLabel "Oil-palm"@en .

glosis_cl:cropClassValueCode-Oi_Ra a glosis_cl:CropClassValueCode,
        skos:Concept ;
    skos:broader glosis_cl:cropClassValueCode-Oi ;
    skos:definition "Crop code for Rape from Oilcrops class" ;
    skos:inScheme glosis_cl:cropClassValueCode ;
    skos:notation "Oi_Ra" ;
    skos:prefLabel "Rape"@en .

glosis_cl:cropClassValueCode-Oi_Se a glosis_cl:CropClassValueCode,
        skos:Concept ;
    skos:broader glosis_cl:cropClassValueCode-Oi ;
    skos:definition "Crop code for Sesame from Oilcrops class" ;
    skos:inScheme glosis_cl:cropClassValueCode ;
    skos:notation "Oi_Se" ;
    skos:prefLabel "Sesame"@en .

glosis_cl:cropClassValueCode-Oi_So a glosis_cl:CropClassValueCode,
        skos:Concept ;
    skos:broader glosis_cl:cropClassValueCode-Oi ;
    skos:definition "Crop code for Soybeans from Oilcrops class" ;
    skos:inScheme glosis_cl:cropClassValueCode ;
    skos:notation "Oi_So" ;
    skos:prefLabel "Soybeans"@en .

glosis_cl:cropClassValueCode-Oi_Su a glosis_cl:CropClassValueCode,
        skos:Concept ;
    skos:broader glosis_cl:cropClassValueCode-Oi ;
    skos:definition "Crop code for Sunflower from Oilcrops class" ;
    skos:inScheme glosis_cl:cropClassValueCode ;
    skos:notation "Oi_Su" ;
    skos:prefLabel "Sunflower"@en .

glosis_cl:cropClassValueCode-Ol a glosis_cl:CropClassValueCode,
        skos:Concept ;
    skos:broader glosis_cl:cropClassValueCode-Oi ;
    skos:definition "Crop code for Olives from Oilcrops class" ;
    skos:inScheme glosis_cl:cropClassValueCode ;
    skos:notation "Oi_Ol" ;
    skos:prefLabel "Olives"@en .

glosis_cl:cropClassValueCode-Ot a glosis_cl:CropClassValueCode,
        skos:Concept ;
    skos:definition "Crop code for Other crops class" ;
    skos:inScheme glosis_cl:cropClassValueCode ;
    skos:narrower glosis_cl:cropClassValueCode-Ot_Pa,
        glosis_cl:cropClassValueCode-Ot_Ru,
        glosis_cl:cropClassValueCode-Ot_Sc ;
    skos:notation "Ot" ;
    skos:prefLabel "Other crops"@en ;
    skos:topConceptOf glosis_cl:cropClassValueCode .

glosis_cl:cropClassValueCode-Ot_Pa a glosis_cl:CropClassValueCode,
        skos:Concept ;
    skos:broader glosis_cl:cropClassValueCode-Ot ;
    skos:definition "Crop code for Palm (fibres, kernels) from other crops class" ;
    skos:inScheme glosis_cl:cropClassValueCode ;
    skos:notation "Ot_Pa" ;
    skos:prefLabel "Palm (fibres, kernels)"@en .

glosis_cl:cropClassValueCode-Ot_Ru a glosis_cl:CropClassValueCode,
        skos:Concept ;
    skos:broader glosis_cl:cropClassValueCode-Ot ;
    skos:definition "Crop code for Rubber from Other crops class" ;
    skos:inScheme glosis_cl:cropClassValueCode ;
    skos:notation "Ot_Ru" ;
    skos:prefLabel "Rubber"@en .

glosis_cl:cropClassValueCode-Ot_Sc a glosis_cl:CropClassValueCode,
        skos:Concept ;
    skos:broader glosis_cl:cropClassValueCode-Ot ;
    skos:definition "Crop code for Sugar cane from other crops class" ;
    skos:inScheme glosis_cl:cropClassValueCode ;
    skos:notation "Ot_Sc" ;
    skos:prefLabel "Sugar cane"@en .

glosis_cl:cropClassValueCode-Pu a glosis_cl:CropClassValueCode,
        skos:Concept ;
    skos:definition "Crop code for Pulses class" ;
    skos:inScheme glosis_cl:cropClassValueCode ;
    skos:narrower glosis_cl:cropClassValueCode-Pu_Be,
        glosis_cl:cropClassValueCode-Pu_Le,
        glosis_cl:cropClassValueCode-Pu_Pe ;
    skos:notation "Pu" ;
    skos:prefLabel "Pulses"@en ;
    skos:topConceptOf glosis_cl:cropClassValueCode .

glosis_cl:cropClassValueCode-Pu_Be a glosis_cl:CropClassValueCode,
        skos:Concept ;
    skos:broader glosis_cl:cropClassValueCode-Pu ;
    skos:definition "Crop code for Beans from Pulses class" ;
    skos:inScheme glosis_cl:cropClassValueCode ;
    skos:notation "Pu_Be" ;
    skos:prefLabel "Beans"@en .

glosis_cl:cropClassValueCode-Pu_Le a glosis_cl:CropClassValueCode,
        skos:Concept ;
    skos:broader glosis_cl:cropClassValueCode-Pu ;
    skos:definition "Crop code for Lentils from Pulses class" ;
    skos:inScheme glosis_cl:cropClassValueCode ;
    skos:notation "Pu_Le" ;
    skos:prefLabel "Lentils"@en .

glosis_cl:cropClassValueCode-Pu_Pe a glosis_cl:CropClassValueCode,
        skos:Concept ;
    skos:broader glosis_cl:cropClassValueCode-Pu ;
    skos:definition "Crop code for Peas from Pulses class" ;
    skos:inScheme glosis_cl:cropClassValueCode ;
    skos:notation "Pu_Pe" ;
    skos:prefLabel "Peas"@en .

glosis_cl:cropClassValueCode-Ro a glosis_cl:CropClassValueCode,
        skos:Concept ;
    skos:definition "Crop code for Roots and tubers class" ;
    skos:inScheme glosis_cl:cropClassValueCode ;
    skos:narrower glosis_cl:cropClassValueCode-Ro_Ca,
        glosis_cl:cropClassValueCode-Ro_Po,
        glosis_cl:cropClassValueCode-Ro_Su,
        glosis_cl:cropClassValueCode-Ro_Ya ;
    skos:notation "Ro" ;
    skos:prefLabel "Roots and tubers"@en ;
    skos:topConceptOf glosis_cl:cropClassValueCode .

glosis_cl:cropClassValueCode-Ro_Ca a glosis_cl:CropClassValueCode,
        skos:Concept ;
    skos:broader glosis_cl:cropClassValueCode-Ro ;
    skos:definition "Crop code for Cassava from Roots and tubers class" ;
    skos:inScheme glosis_cl:cropClassValueCode ;
    skos:notation "Ro_Ca" ;
    skos:prefLabel "Cassava"@en .

glosis_cl:cropClassValueCode-Ro_Po a glosis_cl:CropClassValueCode,
        skos:Concept ;
    skos:broader glosis_cl:cropClassValueCode-Ro ;
    skos:definition "Crop code for Potatoes from Roots and tubers class" ;
    skos:inScheme glosis_cl:cropClassValueCode ;
    skos:notation "Ro_Po" ;
    skos:prefLabel "Potatoes"@en .

glosis_cl:cropClassValueCode-Ro_Su a glosis_cl:CropClassValueCode,
        skos:Concept ;
    skos:broader glosis_cl:cropClassValueCode-Ro ;
    skos:definition "Crop code for Sugar beets from Roots and tubers class" ;
    skos:inScheme glosis_cl:cropClassValueCode ;
    skos:notation "Ro_Su" ;
    skos:prefLabel "Sugar beets"@en .

glosis_cl:cropClassValueCode-Ro_Ya a glosis_cl:CropClassValueCode,
        skos:Concept ;
    skos:broader glosis_cl:cropClassValueCode-Ro ;
    skos:definition "Crop code for Yams from Roots and tubers class" ;
    skos:inScheme glosis_cl:cropClassValueCode ;
    skos:notation "Ro_Ya" ;
    skos:prefLabel "Yams"@en .

glosis_cl:cropClassValueCode-Ve a glosis_cl:CropClassValueCode,
        skos:Concept ;
    skos:definition "Crop code for Vegetables class" ;
    skos:inScheme glosis_cl:cropClassValueCode ;
    skos:notation "Ve" ;
    skos:prefLabel "Vegetables"@en ;
    skos:topConceptOf glosis_cl:cropClassValueCode .

glosis_cl:erosionActivityPeriodValueCode-A a glosis_cl:ErosionActivityPeriodValueCode,
        skos:Concept ;
    skos:definition "Active at present" ;
    skos:inScheme glosis_cl:erosionActivityPeriodValueCode ;
    skos:notation "A" ;
    skos:prefLabel "Active at present"@en ;
    skos:topConceptOf glosis_cl:erosionActivityPeriodValueCode .

glosis_cl:erosionActivityPeriodValueCode-H a glosis_cl:ErosionActivityPeriodValueCode,
        skos:Concept ;
    skos:definition "Active in historical times" ;
    skos:inScheme glosis_cl:erosionActivityPeriodValueCode ;
    skos:notation "H" ;
    skos:prefLabel "Active in historical times"@en ;
    skos:topConceptOf glosis_cl:erosionActivityPeriodValueCode .

glosis_cl:erosionActivityPeriodValueCode-N a glosis_cl:ErosionActivityPeriodValueCode,
        skos:Concept ;
    skos:definition "Period of activity not known" ;
    skos:inScheme glosis_cl:erosionActivityPeriodValueCode ;
    skos:notation "N" ;
    skos:prefLabel "Period of activity not known"@en ;
    skos:topConceptOf glosis_cl:erosionActivityPeriodValueCode .

glosis_cl:erosionActivityPeriodValueCode-R a glosis_cl:ErosionActivityPeriodValueCode,
        skos:Concept ;
    skos:definition "Active in recent past (previous 50–100 years)" ;
    skos:inScheme glosis_cl:erosionActivityPeriodValueCode ;
    skos:notation "R" ;
    skos:prefLabel "Active in recent past"@en ;
    skos:topConceptOf glosis_cl:erosionActivityPeriodValueCode .

glosis_cl:erosionActivityPeriodValueCode-X a glosis_cl:ErosionActivityPeriodValueCode,
        skos:Concept ;
    skos:definition "Accelerated and natural erosion not distinguished" ;
    skos:inScheme glosis_cl:erosionActivityPeriodValueCode ;
    skos:notation "X" ;
    skos:prefLabel "Accelerated and natural erosion not distinguished"@en ;
    skos:topConceptOf glosis_cl:erosionActivityPeriodValueCode .

glosis_cl:erosionAreaAffectedValueCode-0 a glosis_cl:ErosionAreaAffectedValueCode,
        skos:Concept ;
    skos:definition "0%" ;
    skos:inScheme glosis_cl:erosionAreaAffectedValueCode ;
    skos:notation "0" ;
    skos:prefLabel "Zero"@en ;
    skos:topConceptOf glosis_cl:erosionAreaAffectedValueCode .

glosis_cl:erosionAreaAffectedValueCode-1 a glosis_cl:ErosionAreaAffectedValueCode,
        skos:Concept ;
    skos:definition "0-5(%)" ;
    skos:inScheme glosis_cl:erosionAreaAffectedValueCode ;
    skos:notation "1" ;
    skos:prefLabel "Between 0% and 5%"@en ;
    skos:topConceptOf glosis_cl:erosionAreaAffectedValueCode .

glosis_cl:erosionAreaAffectedValueCode-2 a glosis_cl:ErosionAreaAffectedValueCode,
        skos:Concept ;
    skos:definition "5-10(%)" ;
    skos:inScheme glosis_cl:erosionAreaAffectedValueCode ;
    skos:notation "2" ;
    skos:prefLabel "Between 5% and 10%"@en ;
    skos:topConceptOf glosis_cl:erosionAreaAffectedValueCode .

glosis_cl:erosionAreaAffectedValueCode-3 a glosis_cl:ErosionAreaAffectedValueCode,
        skos:Concept ;
    skos:definition "10-25(%)" ;
    skos:inScheme glosis_cl:erosionAreaAffectedValueCode ;
    skos:notation "3" ;
    skos:prefLabel "Between 10% and 25%"@en ;
    skos:topConceptOf glosis_cl:erosionAreaAffectedValueCode .

glosis_cl:erosionAreaAffectedValueCode-4 a glosis_cl:ErosionAreaAffectedValueCode,
        skos:Concept ;
    skos:definition "25-50(%)" ;
    skos:inScheme glosis_cl:erosionAreaAffectedValueCode ;
    skos:notation "4" ;
    skos:prefLabel "Between 25% and 50%"@en ;
    skos:topConceptOf glosis_cl:erosionAreaAffectedValueCode .

glosis_cl:erosionAreaAffectedValueCode-5 a glosis_cl:ErosionAreaAffectedValueCode,
        skos:Concept ;
    skos:definition "> 50%" ;
    skos:inScheme glosis_cl:erosionAreaAffectedValueCode ;
    skos:notation "5" ;
    skos:prefLabel "More than 50%"@en ;
    skos:topConceptOf glosis_cl:erosionAreaAffectedValueCode .

glosis_cl:erosionCategoryValueCode-A a glosis_cl:ErosionCategoryValueCode,
        skos:Concept ;
    skos:definition "Erosion caused by wind" ;
    skos:inScheme glosis_cl:erosionCategoryValueCode ;
    skos:narrower glosis_cl:erosionCategoryValueCode-AD,
        glosis_cl:erosionCategoryValueCode-AM,
        glosis_cl:erosionCategoryValueCode-AS,
        glosis_cl:erosionCategoryValueCode-AZ ;
    skos:notation "A" ;
    skos:prefLabel "Wind (aeolian) erosion or deposition"@en ;
    skos:topConceptOf glosis_cl:erosionCategoryValueCode .

glosis_cl:erosionCategoryValueCode-AD a glosis_cl:ErosionCategoryValueCode,
        skos:Concept ;
    skos:broader glosis_cl:erosionCategoryValueCode-A ;
    skos:definition "Soil deposition caused by wind" ;
    skos:inScheme glosis_cl:erosionCategoryValueCode ;
    skos:notation "AD" ;
    skos:prefLabel "Wind deposition"@en .

glosis_cl:erosionCategoryValueCode-AM a glosis_cl:ErosionCategoryValueCode,
        skos:Concept ;
    skos:broader glosis_cl:erosionCategoryValueCode-A ;
    skos:definition "Erosion and deposition caused by wind" ;
    skos:inScheme glosis_cl:erosionCategoryValueCode ;
    skos:notation "AM" ;
    skos:prefLabel "Wind erosion and deposition"@en .

glosis_cl:erosionCategoryValueCode-AS a glosis_cl:ErosionCategoryValueCode,
        skos:Concept ;
    skos:broader glosis_cl:erosionCategoryValueCode-A ;
    skos:definition "Erosion caused by shifting of sands" ;
    skos:inScheme glosis_cl:erosionCategoryValueCode ;
    skos:notation "AS" ;
    skos:prefLabel "Shifting sands"@en .

glosis_cl:erosionCategoryValueCode-AZ a glosis_cl:ErosionCategoryValueCode,
        skos:Concept ;
    skos:broader glosis_cl:erosionCategoryValueCode-A ;
    skos:definition "Erosion caused by salt deposition" ;
    skos:inScheme glosis_cl:erosionCategoryValueCode ;
    skos:notation "AZ" ;
    skos:prefLabel "Salt deposition"@en .

glosis_cl:erosionCategoryValueCode-M a glosis_cl:ErosionCategoryValueCode,
        skos:Concept ;
    skos:definition "Mass movements are defined as processes of erosion, transport and accumulation of material that occur on both gentle and steep slopes mainly owing to gravitational forces." ;
    skos:inScheme glosis_cl:erosionCategoryValueCode ;
    skos:notation "N" ;
    skos:prefLabel "Mass movement"@en ;
    skos:topConceptOf glosis_cl:erosionCategoryValueCode .

glosis_cl:erosionCategoryValueCode-N a glosis_cl:ErosionCategoryValueCode,
        skos:Concept ;
    skos:definition "Refers to a condition in which the soil shows no visible signs of erosion, indicating that the surface is intact and not undergoing significant degradation due to physical forces like water, wind, or human activity. This category is often used in soil conservation and land management to evaluate the stability of soil. It suggests that soil properties are being maintained, and there is no noticeable loss of topsoil or alteration in the soil structure that would be indicative of erosion processes such as rill, sheet, or gully erosion. In agricultural and ecological contexts, the absence of erosion is a positive indicator that the land is being properly managed, with adequate vegetation cover or protective measures in place to prevent soil degradation​. Source: Soil Erosion from Intro to Environmental Science" ;
    skos:inScheme glosis_cl:erosionCategoryValueCode ;
    skos:notation "N" ;
    skos:prefLabel "No evidence of erosion"@en ;
    skos:topConceptOf glosis_cl:erosionCategoryValueCode .

glosis_cl:erosionCategoryValueCode-NK a glosis_cl:ErosionCategoryValueCode,
        skos:Concept ;
    skos:definition "Unknown causes of Soil erosion" ;
    skos:inScheme glosis_cl:erosionCategoryValueCode ;
    skos:notation "N" ;
    skos:prefLabel "Not known"@en ;
    skos:topConceptOf glosis_cl:erosionCategoryValueCode .

glosis_cl:erosionCategoryValueCode-W a glosis_cl:ErosionCategoryValueCode,
        skos:Concept ;
    skos:definition "Erosion and decposition caused by flowing surface water" ;
    skos:inScheme glosis_cl:erosionCategoryValueCode ;
    skos:narrower glosis_cl:erosionCategoryValueCode-WA,
        glosis_cl:erosionCategoryValueCode-WD,
        glosis_cl:erosionCategoryValueCode-WG,
        glosis_cl:erosionCategoryValueCode-WR,
        glosis_cl:erosionCategoryValueCode-WS,
        glosis_cl:erosionCategoryValueCode-WT ;
    skos:notation "W" ;
    skos:prefLabel "Water erosion or deposition"@en ;
    skos:topConceptOf glosis_cl:erosionCategoryValueCode .

glosis_cl:erosionCategoryValueCode-WA a glosis_cl:ErosionCategoryValueCode,
        skos:Concept ;
    skos:broader glosis_cl:erosionCategoryValueCode-W ;
    skos:definition "Erosion and deposition caused by wind" ;
    skos:inScheme glosis_cl:erosionCategoryValueCode ;
    skos:notation "WA" ;
    skos:prefLabel "Water and wind erosion"@en .

glosis_cl:erosionCategoryValueCode-WD a glosis_cl:ErosionCategoryValueCode,
        skos:Concept ;
    skos:broader glosis_cl:erosionCategoryValueCode-W ;
    skos:definition "Soil deposition caused by water" ;
    skos:inScheme glosis_cl:erosionCategoryValueCode ;
    skos:notation "WD" ;
    skos:prefLabel "Deposition by water"@en .

glosis_cl:erosionCategoryValueCode-WG a glosis_cl:ErosionCategoryValueCode,
        skos:Concept ;
    skos:broader glosis_cl:erosionCategoryValueCode-W ;
    skos:definition "Erosion caused by flowing surface water" ;
    skos:inScheme glosis_cl:erosionCategoryValueCode ;
    skos:notation "WG" ;
    skos:prefLabel "Gully erosion"@en .

glosis_cl:erosionCategoryValueCode-WR a glosis_cl:ErosionCategoryValueCode,
        skos:Concept ;
    skos:broader glosis_cl:erosionCategoryValueCode-W ;
    skos:definition "Rill erosion is the type of erosion that occurs as water flows over a hillslope and cuts shallow, curvy channels into the top soil." ;
    skos:inScheme glosis_cl:erosionCategoryValueCode ;
    skos:notation "WR" ;
    skos:prefLabel "Rill erosion"@en .

glosis_cl:erosionCategoryValueCode-WS a glosis_cl:ErosionCategoryValueCode,
        skos:Concept ;
    skos:broader glosis_cl:erosionCategoryValueCode-W ;
    skos:definition "Uniform erosion of soil in the form of thin layers or sheets." ;
    skos:inScheme glosis_cl:erosionCategoryValueCode ;
    skos:notation "WS" ;
    skos:prefLabel "Sheet erosion"@en .

glosis_cl:erosionCategoryValueCode-WT a glosis_cl:ErosionCategoryValueCode,
        skos:Concept ;
    skos:broader glosis_cl:erosionCategoryValueCode-W ;
    skos:definition "Erosion caused by the movement of excess water through a dispersive subsoil." ;
    skos:inScheme glosis_cl:erosionCategoryValueCode ;
    skos:notation "WT" ;
    skos:prefLabel "Tunnel erosion"@en .

glosis_cl:erosionDegreeValueCode-E a glosis_cl:ErosionDegreeValueCode,
        skos:Concept ;
    skos:definition "Extreme Substantial removal of deeper subsurface horizons (badlands). Original biotic functions fully destroyed." ;
    skos:inScheme glosis_cl:erosionDegreeValueCode ;
    skos:notation "E" ;
    skos:prefLabel "Extreme"@en ;
    skos:topConceptOf glosis_cl:erosionDegreeValueCode .

glosis_cl:erosionDegreeValueCode-M a glosis_cl:ErosionDegreeValueCode,
        skos:Concept ;
    skos:definition "Moderate Clear evidence of removal of surface horizons. Original biotic functions partly destroyed." ;
    skos:inScheme glosis_cl:erosionDegreeValueCode ;
    skos:notation "M" ;
    skos:prefLabel "Moderate"@en ;
    skos:topConceptOf glosis_cl:erosionDegreeValueCode .

glosis_cl:erosionDegreeValueCode-S a glosis_cl:ErosionDegreeValueCode,
        skos:Concept ;
    skos:definition "Slight Some evidence of damage to surface horizons. Original biotic functions largely intact." ;
    skos:inScheme glosis_cl:erosionDegreeValueCode ;
    skos:notation "S" ;
    skos:prefLabel "Slight"@en ;
    skos:topConceptOf glosis_cl:erosionDegreeValueCode .

glosis_cl:erosionDegreeValueCode-V a glosis_cl:ErosionDegreeValueCode,
        skos:Concept ;
    skos:definition "Severe Surface horizons completely removed and subsurface horizons exposed. Original biotic functions largely destroyed." ;
    skos:inScheme glosis_cl:erosionDegreeValueCode ;
    skos:notation "V" ;
    skos:prefLabel "Severe"@en ;
    skos:topConceptOf glosis_cl:erosionDegreeValueCode .

glosis_cl:erosionTotalAreaAffectedValueCode-0 a glosis_cl:ErosionTotalAreaAffectedValueCode,
        skos:Concept ;
    skos:definition "The total area affected by erosion is zero" ;
    skos:inScheme glosis_cl:erosionTotalAreaAffectedValueCode ;
    skos:notation "0" ;
    skos:prefLabel "Zero"@en ;
    skos:topConceptOf glosis_cl:erosionTotalAreaAffectedValueCode .

glosis_cl:erosionTotalAreaAffectedValueCode-1 a glosis_cl:ErosionTotalAreaAffectedValueCode,
        skos:Concept ;
    skos:definition "The total percentage of area affected by erosion is between 0 to 5" ;
    skos:inScheme glosis_cl:erosionTotalAreaAffectedValueCode ;
    skos:notation "1" ;
    skos:prefLabel "Between 0% and 5%"@en ;
    skos:topConceptOf glosis_cl:erosionTotalAreaAffectedValueCode .

glosis_cl:erosionTotalAreaAffectedValueCode-2 a glosis_cl:ErosionTotalAreaAffectedValueCode,
        skos:Concept ;
    skos:definition "The total percentage of area affected by erosion is between 5 - 10" ;
    skos:inScheme glosis_cl:erosionTotalAreaAffectedValueCode ;
    skos:notation "2" ;
    skos:prefLabel "Between 5% and 10%"@en ;
    skos:topConceptOf glosis_cl:erosionTotalAreaAffectedValueCode .

glosis_cl:erosionTotalAreaAffectedValueCode-3 a glosis_cl:ErosionTotalAreaAffectedValueCode,
        skos:Concept ;
    skos:definition "The total percentage of area affected by erosion is between 10 to 25" ;
    skos:inScheme glosis_cl:erosionTotalAreaAffectedValueCode ;
    skos:notation "3" ;
    skos:prefLabel "Between 10% and 25%"@en ;
    skos:topConceptOf glosis_cl:erosionTotalAreaAffectedValueCode .

glosis_cl:erosionTotalAreaAffectedValueCode-4 a glosis_cl:ErosionTotalAreaAffectedValueCode,
        skos:Concept ;
    skos:definition "The total percentage of area affected by erosion is between 25 to 50" ;
    skos:inScheme glosis_cl:erosionTotalAreaAffectedValueCode ;
    skos:notation "4" ;
    skos:prefLabel "Between 25% and 50%"@en ;
    skos:topConceptOf glosis_cl:erosionTotalAreaAffectedValueCode .

glosis_cl:erosionTotalAreaAffectedValueCode-5 a glosis_cl:ErosionTotalAreaAffectedValueCode,
        skos:Concept ;
    skos:definition "The total percentage of area affected by erosion is more than 50: >50%" ;
    skos:inScheme glosis_cl:erosionTotalAreaAffectedValueCode ;
    skos:notation "5" ;
    skos:prefLabel "More than 50%"@en ;
    skos:topConceptOf glosis_cl:erosionTotalAreaAffectedValueCode .

glosis_cl:fragmentCoverValueCode-A a glosis_cl:FragmentCoverValueCode,
        skos:Concept ;
    skos:definition "40%–80% of coarse surface fragments" ;
    skos:inScheme glosis_cl:fragmentCoverValueCode ;
    skos:notation "A" ;
    skos:prefLabel "Abundant"@en ;
    skos:topConceptOf glosis_cl:fragmentCoverValueCode .

glosis_cl:fragmentCoverValueCode-C a glosis_cl:FragmentCoverValueCode,
        skos:Concept ;
    skos:definition "5%–15% of coarse surface fragments" ;
    skos:inScheme glosis_cl:fragmentCoverValueCode ;
    skos:notation "C" ;
    skos:prefLabel "Common"@en ;
    skos:topConceptOf glosis_cl:fragmentCoverValueCode .

glosis_cl:fragmentCoverValueCode-D a glosis_cl:FragmentCoverValueCode,
        skos:Concept ;
    skos:definition "> 80% of coarse surface fragments" ;
    skos:inScheme glosis_cl:fragmentCoverValueCode ;
    skos:notation "D" ;
    skos:prefLabel "Dominant"@en ;
    skos:topConceptOf glosis_cl:fragmentCoverValueCode .

glosis_cl:fragmentCoverValueCode-F a glosis_cl:FragmentCoverValueCode,
        skos:Concept ;
    skos:definition "2%–5% of coarse surface fragments" ;
    skos:inScheme glosis_cl:fragmentCoverValueCode ;
    skos:notation "F" ;
    skos:prefLabel "Few"@en ;
    skos:topConceptOf glosis_cl:fragmentCoverValueCode .

glosis_cl:fragmentCoverValueCode-M a glosis_cl:FragmentCoverValueCode,
        skos:Concept ;
    skos:definition "15%–40% of coarse surface fragments" ;
    skos:inScheme glosis_cl:fragmentCoverValueCode ;
    skos:notation "M" ;
    skos:prefLabel "Many"@en ;
    skos:topConceptOf glosis_cl:fragmentCoverValueCode .

glosis_cl:fragmentCoverValueCode-N a glosis_cl:FragmentCoverValueCode,
        skos:Concept ;
    skos:definition "0% of coarse surface fragments" ;
    skos:inScheme glosis_cl:fragmentCoverValueCode ;
    skos:notation "N" ;
    skos:prefLabel "None"@en ;
    skos:topConceptOf glosis_cl:fragmentCoverValueCode .

glosis_cl:fragmentCoverValueCode-V a glosis_cl:FragmentCoverValueCode,
        skos:Concept ;
    skos:definition "0%–2% of coarse surface fragments" ;
    skos:inScheme glosis_cl:fragmentCoverValueCode ;
    skos:notation "V" ;
    skos:prefLabel "Very few"@en ;
    skos:topConceptOf glosis_cl:fragmentCoverValueCode .

glosis_cl:fragmentsClassValueCode-FGF1 a glosis_cl:FragmentsClassValueCode,
        skos:Concept ;
    skos:definition "Horizon layer property of Coarse fragments - gravimetric fraction 01" ;
    skos:inScheme glosis_cl:fragmentsClassValueCode ;
    skos:notation "FGF1" ;
    skos:prefLabel "FragmentsGravimetricFraction01"@en ;
    skos:topConceptOf glosis_cl:fragmentsClassValueCode .

glosis_cl:fragmentsClassValueCode-FGF2 a glosis_cl:FragmentsClassValueCode,
        skos:Concept ;
    skos:definition "Horizon layer property of Coarse fragments - gravimetric fraction 02" ;
    skos:inScheme glosis_cl:fragmentsClassValueCode ;
    skos:notation "FGF2" ;
    skos:prefLabel "FragmentsGravimetricFraction02"@en ;
    skos:topConceptOf glosis_cl:fragmentsClassValueCode .

glosis_cl:fragmentsClassValueCode-FGF3 a glosis_cl:FragmentsClassValueCode,
        skos:Concept ;
    skos:definition "Horizon layer property of Coarse fragments - gravimetric fraction 03" ;
    skos:inScheme glosis_cl:fragmentsClassValueCode ;
    skos:notation "FGF3" ;
    skos:prefLabel "FragmentsGravimetricFraction03"@en ;
    skos:topConceptOf glosis_cl:fragmentsClassValueCode .

glosis_cl:fragmentsClassValueCode-FGF4 a glosis_cl:FragmentsClassValueCode,
        skos:Concept ;
    skos:definition "Horizon layer property of Coarse fragments - gravimetric fraction 04" ;
    skos:inScheme glosis_cl:fragmentsClassValueCode ;
    skos:notation "FGF4" ;
    skos:prefLabel "FragmentsGravimetricFraction04"@en ;
    skos:topConceptOf glosis_cl:fragmentsClassValueCode .

glosis_cl:fragmentsClassValueCode-FGT a glosis_cl:FragmentsClassValueCode,
        skos:Concept ;
    skos:definition "Horizon layer property of Coarse fragments - gravimetric total" ;
    skos:inScheme glosis_cl:fragmentsClassValueCode ;
    skos:notation "FGT" ;
    skos:prefLabel "FragmentsGravimetricTotal"@en ;
    skos:topConceptOf glosis_cl:fragmentsClassValueCode .

glosis_cl:fragmentsClassValueCode-FV1 a glosis_cl:FragmentsClassValueCode,
        skos:Concept ;
    skos:definition "Horizon layer property of Coarse fragments - volumetric fraction 01" ;
    skos:inScheme glosis_cl:fragmentsClassValueCode ;
    skos:notation "FV1" ;
    skos:prefLabel "FragmentsVolumetric01"@en ;
    skos:topConceptOf glosis_cl:fragmentsClassValueCode .

glosis_cl:fragmentsClassValueCode-FV2 a glosis_cl:FragmentsClassValueCode,
        skos:Concept ;
    skos:definition "Horizon layer property of Coarse fragments - volumetric fraction 02" ;
    skos:inScheme glosis_cl:fragmentsClassValueCode ;
    skos:notation "FV2" ;
    skos:prefLabel "FragmentsVolumetric02"@en ;
    skos:topConceptOf glosis_cl:fragmentsClassValueCode .

glosis_cl:fragmentsClassValueCode-FV3 a glosis_cl:FragmentsClassValueCode,
        skos:Concept ;
    skos:definition "Horizon layer property of Coarse fragments - volumetric fraction 03" ;
    skos:inScheme glosis_cl:fragmentsClassValueCode ;
    skos:notation "FV3" ;
    skos:prefLabel "FragmentsVolumetric03"@en ;
    skos:topConceptOf glosis_cl:fragmentsClassValueCode .

glosis_cl:fragmentsClassValueCode-FVE a glosis_cl:FragmentsClassValueCode,
        skos:Concept ;
    skos:definition "Horizon layer property of Coarse fragments - volumetric total, field estimated " ;
    skos:inScheme glosis_cl:fragmentsClassValueCode ;
    skos:notation "FVE" ;
    skos:prefLabel "FragmentsVolumetricEstimate"@en ;
    skos:topConceptOf glosis_cl:fragmentsClassValueCode .

glosis_cl:fragmentsClassValueCode-FVT a glosis_cl:FragmentsClassValueCode,
        skos:Concept ;
    skos:definition "Horizon layer property of Coarse fragments - volumetric total" ;
    skos:inScheme glosis_cl:fragmentsClassValueCode ;
    skos:notation "FVT" ;
    skos:prefLabel "FragmentsVolumetricTotal"@en ;
    skos:topConceptOf glosis_cl:fragmentsClassValueCode .

glosis_cl:fragmentsSizeValueCode-B a glosis_cl:FragmentsSizeValueCode,
        skos:Concept ;
    skos:definition "Boulders of coarse size of 20cm–60cm" ;
    skos:inScheme glosis_cl:fragmentsSizeValueCode ;
    skos:notation "B" ;
    skos:prefLabel "Boulders"@en ;
    skos:topConceptOf glosis_cl:fragmentsSizeValueCode .

glosis_cl:fragmentsSizeValueCode-C a glosis_cl:FragmentsSizeValueCode,
        skos:Concept ;
    skos:definition "Coarse gravel of size 2cm–6cm" ;
    skos:inScheme glosis_cl:fragmentsSizeValueCode ;
    skos:notation "C" ;
    skos:prefLabel "Coarse gravel"@en ;
    skos:topConceptOf glosis_cl:fragmentsSizeValueCode .

glosis_cl:fragmentsSizeValueCode-F a glosis_cl:FragmentsSizeValueCode,
        skos:Concept ;
    skos:definition "Fine gravel coarse size of 0.2cm–0.6cm" ;
    skos:inScheme glosis_cl:fragmentsSizeValueCode ;
    skos:notation "F" ;
    skos:prefLabel "Fine gravel"@en ;
    skos:topConceptOf glosis_cl:fragmentsSizeValueCode .

glosis_cl:fragmentsSizeValueCode-L a glosis_cl:FragmentsSizeValueCode,
        skos:Concept ;
    skos:definition "Large boulders of coarse size 60cm–200cm" ;
    skos:inScheme glosis_cl:fragmentsSizeValueCode ;
    skos:notation "L" ;
    skos:prefLabel "Large boulders"@en ;
    skos:topConceptOf glosis_cl:fragmentsSizeValueCode .

glosis_cl:fragmentsSizeValueCode-M a glosis_cl:FragmentsSizeValueCode,
        skos:Concept ;
    skos:definition "Medium gravel coarse size of 0.6cm–2.0cm" ;
    skos:inScheme glosis_cl:fragmentsSizeValueCode ;
    skos:notation "M" ;
    skos:prefLabel "Medium gravel"@en ;
    skos:topConceptOf glosis_cl:fragmentsSizeValueCode .

glosis_cl:fragmentsSizeValueCode-S a glosis_cl:FragmentsSizeValueCode,
        skos:Concept ;
    skos:definition "Stones of coarse size 6cm–20cm" ;
    skos:inScheme glosis_cl:fragmentsSizeValueCode ;
    skos:notation "S" ;
    skos:prefLabel "Stones"@en ;
    skos:topConceptOf glosis_cl:fragmentsSizeValueCode .

glosis_cl:gypsumContentValueCode-EX a glosis_cl:GypsumContentValueCode,
        skos:Concept ;
    skos:definition "≈ > 60" ;
    skos:inScheme glosis_cl:gypsumContentValueCode ;
    skos:notation "EX" ;
    skos:prefLabel "Extremely gypsiric"@en ;
    skos:topConceptOf glosis_cl:gypsumContentValueCode .

glosis_cl:gypsumContentValueCode-MO a glosis_cl:GypsumContentValueCode,
        skos:Concept ;
    skos:definition "≈ 5–15 EC = > 1.8 dS m-1 in 10 g soil/250 ml H2O" ;
    skos:inScheme glosis_cl:gypsumContentValueCode ;
    skos:notation "MO" ;
    skos:prefLabel "Moderately gypsiric"@en ;
    skos:topConceptOf glosis_cl:gypsumContentValueCode .

glosis_cl:gypsumContentValueCode-N a glosis_cl:GypsumContentValueCode,
        skos:Concept ;
    skos:definition "0 EC = < 0.18 dS m-1 in 10 g soil/250 ml H2O" ;
    skos:inScheme glosis_cl:gypsumContentValueCode ;
    skos:notation "N" ;
    skos:prefLabel "Non-gypsiric"@en ;
    skos:topConceptOf glosis_cl:gypsumContentValueCode .

glosis_cl:gypsumContentValueCode-SL a glosis_cl:GypsumContentValueCode,
        skos:Concept ;
    skos:definition "≈ 0–5 EC = < 1.8 dS m-1 in 10 g soil/250 ml H2O" ;
    skos:inScheme glosis_cl:gypsumContentValueCode ;
    skos:notation "SL" ;
    skos:prefLabel "Slightly gypsiric"@en ;
    skos:topConceptOf glosis_cl:gypsumContentValueCode .

glosis_cl:gypsumContentValueCode-ST a glosis_cl:GypsumContentValueCode,
        skos:Concept ;
    skos:definition "≈ 15–60 higher amounts may be differentiated by abundance of H2O-soluble pseudomycelia/crystals and soil colour" ;
    skos:inScheme glosis_cl:gypsumContentValueCode ;
    skos:notation "ST" ;
    skos:prefLabel "Strongly gypsiric"@en ;
    skos:topConceptOf glosis_cl:gypsumContentValueCode .

glosis_cl:gypsumFormsValueCode-D a glosis_cl:GypsumFormsValueCode,
        skos:Concept ;
    skos:definition "Secondary gypson in the form of disperse powdery gypsum" ;
    skos:inScheme glosis_cl:gypsumFormsValueCode ;
    skos:notation "D" ;
    skos:prefLabel "disperse powdery gypsum"@en ;
    skos:topConceptOf glosis_cl:gypsumFormsValueCode .

glosis_cl:gypsumFormsValueCode-G a glosis_cl:GypsumFormsValueCode,
        skos:Concept ;
    skos:definition "Secondary gypson in the form of gazha (clayey water-saturated layer with high gypsum content)" ;
    skos:inScheme glosis_cl:gypsumFormsValueCode ;
    skos:notation "G" ;
    skos:prefLabel "gazha"@en ;
    skos:topConceptOf glosis_cl:gypsumFormsValueCode .

glosis_cl:gypsumFormsValueCode-HL a glosis_cl:GypsumFormsValueCode,
        skos:Concept ;
    skos:definition "Secondary gypson in the form of hard cemented layer or layers of gypsum less than 10 cm thick" ;
    skos:inScheme glosis_cl:gypsumFormsValueCode ;
    skos:notation "HL" ;
    skos:prefLabel "hard cemented layer or layers of gypsum"@en ;
    skos:topConceptOf glosis_cl:gypsumFormsValueCode .

glosis_cl:gypsumFormsValueCode-SC a glosis_cl:GypsumFormsValueCode,
        skos:Concept ;
    skos:definition "Secondary gypsum in the form of soft concretions" ;
    skos:inScheme glosis_cl:gypsumFormsValueCode ;
    skos:notation "SC" ;
    skos:prefLabel "soft concretions"@en ;
    skos:topConceptOf glosis_cl:gypsumFormsValueCode .

glosis_cl:humanInfluenceClassValueCode-AC a glosis_cl:HumanInfluenceClassValueCode,
        skos:Concept ;
    skos:definition "Human Influence on landsacpe affected by archeological activities i.e burial mound, midden etc" ;
    skos:inScheme glosis_cl:humanInfluenceClassValueCode ;
    skos:notation "AC" ;
    skos:prefLabel "Archaeological (burial mound, midden)"@en ;
    skos:topConceptOf glosis_cl:humanInfluenceClassValueCode .

glosis_cl:humanInfluenceClassValueCode-AD a glosis_cl:HumanInfluenceClassValueCode,
        skos:Concept ;
    skos:definition "Human Influence on landsacpe affected by artificial drainage" ;
    skos:inScheme glosis_cl:humanInfluenceClassValueCode ;
    skos:notation "AD" ;
    skos:prefLabel "Artificial drainage"@en ;
    skos:topConceptOf glosis_cl:humanInfluenceClassValueCode .

glosis_cl:humanInfluenceClassValueCode-BP a glosis_cl:HumanInfluenceClassValueCode,
        skos:Concept ;
    skos:definition "Human Influence on landsacpe affected by borrow pit" ;
    skos:inScheme glosis_cl:humanInfluenceClassValueCode ;
    skos:notation "BP" ;
    skos:prefLabel "Borrow pit"@en ;
    skos:topConceptOf glosis_cl:humanInfluenceClassValueCode .

glosis_cl:humanInfluenceClassValueCode-BR a glosis_cl:HumanInfluenceClassValueCode,
        skos:Concept ;
    skos:definition "Human Influence on landsacpe affected by burning" ;
    skos:inScheme glosis_cl:humanInfluenceClassValueCode ;
    skos:notation "BR" ;
    skos:prefLabel "Burning"@en ;
    skos:topConceptOf glosis_cl:humanInfluenceClassValueCode .

glosis_cl:humanInfluenceClassValueCode-BU a glosis_cl:HumanInfluenceClassValueCode,
        skos:Concept ;
    skos:definition "Human Influence on landsacpe affected by bunding" ;
    skos:inScheme glosis_cl:humanInfluenceClassValueCode ;
    skos:notation "BU" ;
    skos:prefLabel "Bunding"@en ;
    skos:topConceptOf glosis_cl:humanInfluenceClassValueCode .

glosis_cl:humanInfluenceClassValueCode-CL a glosis_cl:HumanInfluenceClassValueCode,
        skos:Concept ;
    skos:definition "Human Influence on landsacpe affected by clearing" ;
    skos:inScheme glosis_cl:humanInfluenceClassValueCode ;
    skos:notation "CL" ;
    skos:prefLabel "Clearing"@en ;
    skos:topConceptOf glosis_cl:humanInfluenceClassValueCode .

glosis_cl:humanInfluenceClassValueCode-CR a glosis_cl:HumanInfluenceClassValueCode,
        skos:Concept ;
    skos:definition "Human Influence on landsacpe affected by impact factors" ;
    skos:inScheme glosis_cl:humanInfluenceClassValueCode ;
    skos:notation "CR" ;
    skos:prefLabel "Impact crater"@en ;
    skos:topConceptOf glosis_cl:humanInfluenceClassValueCode .

glosis_cl:humanInfluenceClassValueCode-DU a glosis_cl:HumanInfluenceClassValueCode,
        skos:Concept ;
    skos:definition "Human Influence on landsacpe affected by unspecified dumpings" ;
    skos:inScheme glosis_cl:humanInfluenceClassValueCode ;
    skos:notation "DU" ;
    skos:prefLabel "Dump (not specified)"@en ;
    skos:topConceptOf glosis_cl:humanInfluenceClassValueCode .

glosis_cl:humanInfluenceClassValueCode-FE a glosis_cl:HumanInfluenceClassValueCode,
        skos:Concept ;
    skos:definition "Human Influence on landsacpe affected by application of fertilizers" ;
    skos:inScheme glosis_cl:humanInfluenceClassValueCode ;
    skos:notation "FE" ;
    skos:prefLabel "Application of fertilizers"@en ;
    skos:topConceptOf glosis_cl:humanInfluenceClassValueCode .

glosis_cl:humanInfluenceClassValueCode-IB a glosis_cl:HumanInfluenceClassValueCode,
        skos:Concept ;
    skos:definition "Human Influence on landsacpe affected by border irrigation" ;
    skos:inScheme glosis_cl:humanInfluenceClassValueCode ;
    skos:notation "IB" ;
    skos:prefLabel "Border irrigation"@en ;
    skos:topConceptOf glosis_cl:humanInfluenceClassValueCode .

glosis_cl:humanInfluenceClassValueCode-ID a glosis_cl:HumanInfluenceClassValueCode,
        skos:Concept ;
    skos:definition "Human Influence on landsacpe affected by drip irrigation" ;
    skos:inScheme glosis_cl:humanInfluenceClassValueCode ;
    skos:notation "ID" ;
    skos:prefLabel "Drip irrigation"@en ;
    skos:topConceptOf glosis_cl:humanInfluenceClassValueCode .

glosis_cl:humanInfluenceClassValueCode-IF a glosis_cl:HumanInfluenceClassValueCode,
        skos:Concept ;
    skos:definition "Human Influence on landsacpe affected by furrow irrigation" ;
    skos:inScheme glosis_cl:humanInfluenceClassValueCode ;
    skos:notation "IF" ;
    skos:prefLabel "Furrow irrigation"@en ;
    skos:topConceptOf glosis_cl:humanInfluenceClassValueCode .

glosis_cl:humanInfluenceClassValueCode-IP a glosis_cl:HumanInfluenceClassValueCode,
        skos:Concept ;
    skos:definition "Human Influence on landsacpe affected by flood irrigation" ;
    skos:inScheme glosis_cl:humanInfluenceClassValueCode ;
    skos:notation "IP" ;
    skos:prefLabel "Flood irrigation"@en ;
    skos:topConceptOf glosis_cl:humanInfluenceClassValueCode .

glosis_cl:humanInfluenceClassValueCode-IS a glosis_cl:HumanInfluenceClassValueCode,
        skos:Concept ;
    skos:definition "Human Influence on landsacpe affected by sprinkler irrigation" ;
    skos:inScheme glosis_cl:humanInfluenceClassValueCode ;
    skos:notation "IS" ;
    skos:prefLabel "Sprinkler irrigation"@en ;
    skos:topConceptOf glosis_cl:humanInfluenceClassValueCode .

glosis_cl:humanInfluenceClassValueCode-IU a glosis_cl:HumanInfluenceClassValueCode,
        skos:Concept ;
    skos:definition "Human Influence on landsacpe affected by unspecified irrgation" ;
    skos:inScheme glosis_cl:humanInfluenceClassValueCode ;
    skos:notation "IU" ;
    skos:prefLabel "Irrigation (not specified)"@en ;
    skos:topConceptOf glosis_cl:humanInfluenceClassValueCode .

glosis_cl:humanInfluenceClassValueCode-LF a glosis_cl:HumanInfluenceClassValueCode,
        skos:Concept ;
    skos:definition "Human Influence on landsacpe affected by sanitary activities like landfills" ;
    skos:inScheme glosis_cl:humanInfluenceClassValueCode ;
    skos:notation "LF" ;
    skos:prefLabel "Landfill (also sanitary)"@en ;
    skos:topConceptOf glosis_cl:humanInfluenceClassValueCode .

glosis_cl:humanInfluenceClassValueCode-LV a glosis_cl:HumanInfluenceClassValueCode,
        skos:Concept ;
    skos:definition "Human Influence on landsacpe affected by levelling" ;
    skos:inScheme glosis_cl:humanInfluenceClassValueCode ;
    skos:notation "LV" ;
    skos:prefLabel "Levelling"@en ;
    skos:topConceptOf glosis_cl:humanInfluenceClassValueCode .

glosis_cl:humanInfluenceClassValueCode-ME a glosis_cl:HumanInfluenceClassValueCode,
        skos:Concept ;
    skos:definition "Human Influence on landsacpe affected by engineering activites like raised beds" ;
    skos:inScheme glosis_cl:humanInfluenceClassValueCode ;
    skos:notation "ME" ;
    skos:prefLabel "Raised beds (engineering purposes)"@en ;
    skos:topConceptOf glosis_cl:humanInfluenceClassValueCode .

glosis_cl:humanInfluenceClassValueCode-MI a glosis_cl:HumanInfluenceClassValueCode,
        skos:Concept ;
    skos:definition "Human Influence on landsacpe affected by mining activities e.g. surface mining, openpit mining, gravel and quarries" ;
    skos:inScheme glosis_cl:humanInfluenceClassValueCode ;
    skos:notation "MI" ;
    skos:prefLabel "Mine (surface, including openpit, gravel and quarries)"@en ;
    skos:topConceptOf glosis_cl:humanInfluenceClassValueCode .

glosis_cl:humanInfluenceClassValueCode-MO a glosis_cl:HumanInfluenceClassValueCode,
        skos:Concept ;
    skos:definition "Human Influence on landsacpe affected by unspecified Organic additions" ;
    skos:inScheme glosis_cl:humanInfluenceClassValueCode ;
    skos:notation "MO" ;
    skos:prefLabel "Organic additions (not specified)"@en ;
    skos:topConceptOf glosis_cl:humanInfluenceClassValueCode .

glosis_cl:humanInfluenceClassValueCode-MP a glosis_cl:HumanInfluenceClassValueCode,
        skos:Concept ;
    skos:definition "Human Influence on landsacpe affected by plaggen" ;
    skos:inScheme glosis_cl:humanInfluenceClassValueCode ;
    skos:notation "MP" ;
    skos:prefLabel "Plaggen"@en ;
    skos:topConceptOf glosis_cl:humanInfluenceClassValueCode .

glosis_cl:humanInfluenceClassValueCode-MR a glosis_cl:HumanInfluenceClassValueCode,
        skos:Concept ;
    skos:definition "Human Influence on landsacpe affected by raised bed due to agricultural activity" ;
    skos:inScheme glosis_cl:humanInfluenceClassValueCode ;
    skos:notation "MR" ;
    skos:prefLabel "Raised beds (agricultural purposes)"@en ;
    skos:topConceptOf glosis_cl:humanInfluenceClassValueCode .

glosis_cl:humanInfluenceClassValueCode-MS a glosis_cl:HumanInfluenceClassValueCode,
        skos:Concept ;
    skos:definition "Human Influence on landsacpe affected by sand additions" ;
    skos:inScheme glosis_cl:humanInfluenceClassValueCode ;
    skos:notation "MS" ;
    skos:prefLabel "Sand additions"@en ;
    skos:topConceptOf glosis_cl:humanInfluenceClassValueCode .

glosis_cl:humanInfluenceClassValueCode-MU a glosis_cl:HumanInfluenceClassValueCode,
        skos:Concept ;
    skos:definition "Human Influence on landsacpe affected by unspecified addition of minerals" ;
    skos:inScheme glosis_cl:humanInfluenceClassValueCode ;
    skos:notation "MU" ;
    skos:prefLabel "Mineral additions (not specified)"@en ;
    skos:topConceptOf glosis_cl:humanInfluenceClassValueCode .

glosis_cl:humanInfluenceClassValueCode-N a glosis_cl:HumanInfluenceClassValueCode,
        skos:Concept ;
    skos:definition "No visible human influence on landscape" ;
    skos:inScheme glosis_cl:humanInfluenceClassValueCode ;
    skos:notation "N" ;
    skos:prefLabel "No influence"@en ;
    skos:topConceptOf glosis_cl:humanInfluenceClassValueCode .

glosis_cl:humanInfluenceClassValueCode-NK a glosis_cl:HumanInfluenceClassValueCode,
        skos:Concept ;
    skos:definition "Human Influence on landsacpe affected by unkown reasons" ;
    skos:inScheme glosis_cl:humanInfluenceClassValueCode ;
    skos:notation "NK" ;
    skos:prefLabel "Not known"@en ;
    skos:topConceptOf glosis_cl:humanInfluenceClassValueCode .

glosis_cl:humanInfluenceClassValueCode-PL a glosis_cl:HumanInfluenceClassValueCode,
        skos:Concept ;
    skos:definition "Human Influence on landsacpe affected by ploughing" ;
    skos:inScheme glosis_cl:humanInfluenceClassValueCode ;
    skos:notation "PL" ;
    skos:prefLabel "Ploughing"@en ;
    skos:topConceptOf glosis_cl:humanInfluenceClassValueCode .

glosis_cl:humanInfluenceClassValueCode-PO a glosis_cl:HumanInfluenceClassValueCode,
        skos:Concept ;
    skos:definition "Human Influence on landsacpe affected by pollution" ;
    skos:inScheme glosis_cl:humanInfluenceClassValueCode ;
    skos:notation "PO" ;
    skos:prefLabel "Pollution"@en ;
    skos:topConceptOf glosis_cl:humanInfluenceClassValueCode .

glosis_cl:humanInfluenceClassValueCode-SA a glosis_cl:HumanInfluenceClassValueCode,
        skos:Concept ;
    skos:definition "Human Influence on landsacpe affected by scalped area" ;
    skos:inScheme glosis_cl:humanInfluenceClassValueCode ;
    skos:notation "SA" ;
    skos:prefLabel "Scalped area"@en ;
    skos:topConceptOf glosis_cl:humanInfluenceClassValueCode .

glosis_cl:humanInfluenceClassValueCode-SC a glosis_cl:HumanInfluenceClassValueCode,
        skos:Concept ;
    skos:definition "Human Influence on landsacpe affected by surface compaction" ;
    skos:inScheme glosis_cl:humanInfluenceClassValueCode ;
    skos:notation "SC" ;
    skos:prefLabel "Surface compaction"@en ;
    skos:topConceptOf glosis_cl:humanInfluenceClassValueCode .

glosis_cl:humanInfluenceClassValueCode-TE a glosis_cl:HumanInfluenceClassValueCode,
        skos:Concept ;
    skos:definition "Human Influence on landsacpe affected by terracing" ;
    skos:inScheme glosis_cl:humanInfluenceClassValueCode ;
    skos:notation "TE" ;
    skos:prefLabel "Terracing"@en ;
    skos:topConceptOf glosis_cl:humanInfluenceClassValueCode .

glosis_cl:humanInfluenceClassValueCode-VE a glosis_cl:HumanInfluenceClassValueCode,
        skos:Concept ;
    skos:definition "Human Influence on landsacpe affected by strongly disturbed vegetation" ;
    skos:inScheme glosis_cl:humanInfluenceClassValueCode ;
    skos:notation "VE" ;
    skos:prefLabel "Vegetation strongly disturbed"@en ;
    skos:topConceptOf glosis_cl:humanInfluenceClassValueCode .

glosis_cl:humanInfluenceClassValueCode-VM a glosis_cl:HumanInfluenceClassValueCode,
        skos:Concept ;
    skos:definition "Human Influence on landsacpe affected by moderately disturbed vegetation" ;
    skos:inScheme glosis_cl:humanInfluenceClassValueCode ;
    skos:notation "VM" ;
    skos:prefLabel "Vegetation moderately disturbed"@en ;
    skos:topConceptOf glosis_cl:humanInfluenceClassValueCode .

glosis_cl:humanInfluenceClassValueCode-VS a glosis_cl:HumanInfluenceClassValueCode,
        skos:Concept ;
    skos:definition "Human Influence on landsacpe affected by slightly disturbed vegetation" ;
    skos:inScheme glosis_cl:humanInfluenceClassValueCode ;
    skos:notation "VS" ;
    skos:prefLabel "Vegetation slightly disturbed"@en ;
    skos:topConceptOf glosis_cl:humanInfluenceClassValueCode .

glosis_cl:humanInfluenceClassValueCode-VU a glosis_cl:HumanInfluenceClassValueCode,
        skos:Concept ;
    skos:definition "Human Influence on landsacpe affected by unspecified disturbed vegitation" ;
    skos:inScheme glosis_cl:humanInfluenceClassValueCode ;
    skos:notation "VU" ;
    skos:prefLabel "Vegetation disturbed (not specified)"@en ;
    skos:topConceptOf glosis_cl:humanInfluenceClassValueCode .

glosis_cl:landUseClassValueCode-A a glosis_cl:LandUseClassValueCode,
        skos:Concept ;
    skos:definition "Land-use classification of main class Crop agriculture (cropping)" ;
    skos:inScheme glosis_cl:landUseClassValueCode ;
    skos:narrower glosis_cl:landUseClassValueCode-AA,
        glosis_cl:landUseClassValueCode-AP,
        glosis_cl:landUseClassValueCode-AT ;
    skos:notation "A" ;
    skos:prefLabel "Crop agriculture (cropping)"@en ;
    skos:topConceptOf glosis_cl:landUseClassValueCode .

glosis_cl:landUseClassValueCode-AA a glosis_cl:LandUseClassValueCode,
        skos:Concept ;
    skos:broader glosis_cl:landUseClassValueCode-A ;
    skos:definition "Land-use classification of main class Crop agriculture and of subclass Annual field cropping" ;
    skos:inScheme glosis_cl:landUseClassValueCode ;
    skos:narrower glosis_cl:landUseClassValueCode-AA1,
        glosis_cl:landUseClassValueCode-AA2,
        glosis_cl:landUseClassValueCode-AA3,
        glosis_cl:landUseClassValueCode-AA4,
        glosis_cl:landUseClassValueCode-AA5,
        glosis_cl:landUseClassValueCode-AA6 ;
    skos:notation "AA" ;
    skos:prefLabel "Annual field cropping"@en .

glosis_cl:landUseClassValueCode-AA1 a glosis_cl:LandUseClassValueCode,
        skos:Concept ;
    skos:broader glosis_cl:landUseClassValueCode-AA ;
    skos:definition "Land-use classification of main class Crop agriculture and of subclass Annual field cropping and of type Shifting cultivation" ;
    skos:inScheme glosis_cl:landUseClassValueCode ;
    skos:notation "AA1" ;
    skos:prefLabel "Shifting cultivation"@en .

glosis_cl:landUseClassValueCode-AA2 a glosis_cl:LandUseClassValueCode,
        skos:Concept ;
    skos:broader glosis_cl:landUseClassValueCode-AA ;
    skos:definition "Land-use classification of main class Crop agriculture and of sub-class Annual field cropping and of type Fallow system cultivation" ;
    skos:inScheme glosis_cl:landUseClassValueCode ;
    skos:notation "AA2" ;
    skos:prefLabel "Fallow system cultivation"@en .

glosis_cl:landUseClassValueCode-AA3 a glosis_cl:LandUseClassValueCode,
        skos:Concept ;
    skos:broader glosis_cl:landUseClassValueCode-AA ;
    skos:definition "Land-use classification of main class Crop agriculture and of subclass Annual field cropping and of type Ley system cultivation" ;
    skos:inScheme glosis_cl:landUseClassValueCode ;
    skos:notation "AA3" ;
    skos:prefLabel "Ley system cultivation"@en .

glosis_cl:landUseClassValueCode-AA4 a glosis_cl:LandUseClassValueCode,
        skos:Concept ;
    skos:broader glosis_cl:landUseClassValueCode-AA ;
    skos:definition "Land-use classification of main class Crop agriculture and of subclass Annual field cropping and of type Rainfed arable cultivation" ;
    skos:inScheme glosis_cl:landUseClassValueCode ;
    skos:notation "AA4" ;
    skos:prefLabel "Rainfed arable cultivation"@en .

glosis_cl:landUseClassValueCode-AA5 a glosis_cl:LandUseClassValueCode,
        skos:Concept ;
    skos:broader glosis_cl:landUseClassValueCode-AA ;
    skos:definition "Land-use classification of mainclass Crop agriculture and of class Annual field cropping and of type Wet rice cultivation" ;
    skos:inScheme glosis_cl:landUseClassValueCode ;
    skos:notation "AA5" ;
    skos:prefLabel "Wet rice cultivation"@en .

glosis_cl:landUseClassValueCode-AA6 a glosis_cl:LandUseClassValueCode,
        skos:Concept ;
    skos:broader glosis_cl:landUseClassValueCode-AA ;
    skos:definition "Land-use classification of main class Crop agriculture and of subclass Annual field cropping and of type Irrigated cultivation" ;
    skos:inScheme glosis_cl:landUseClassValueCode ;
    skos:notation "AA6" ;
    skos:prefLabel "Irrigated cultivation"@en .

glosis_cl:landUseClassValueCode-AP a glosis_cl:LandUseClassValueCode,
        skos:Concept ;
    skos:broader glosis_cl:landUseClassValueCode-A ;
    skos:definition "Land-use classification of main class Crop agriculture and of subclass Perennial field cropping" ;
    skos:inScheme glosis_cl:landUseClassValueCode ;
    skos:narrower glosis_cl:landUseClassValueCode-AP1,
        glosis_cl:landUseClassValueCode-AP2 ;
    skos:notation "AP" ;
    skos:prefLabel "Perennial field cropping"@en .

glosis_cl:landUseClassValueCode-AP1 a glosis_cl:LandUseClassValueCode,
        skos:Concept ;
    skos:broader glosis_cl:landUseClassValueCode-AP ;
    skos:definition "Land-use classification of main class Crop agriculture and of subclass Perennial field cropping and of type Non-irrigated cultivation" ;
    skos:inScheme glosis_cl:landUseClassValueCode ;
    skos:notation "AP1" ;
    skos:prefLabel "Non-irrigated cultivation"@en .

glosis_cl:landUseClassValueCode-AP2 a glosis_cl:LandUseClassValueCode,
        skos:Concept ;
    skos:broader glosis_cl:landUseClassValueCode-AP ;
    skos:definition "Land-use classification of main class Crop agriculture and of subclass Perennial field cropping and of type Irrigated cultivation" ;
    skos:inScheme glosis_cl:landUseClassValueCode ;
    skos:notation "AP2" ;
    skos:prefLabel "Irrigated cultivation"@en .

glosis_cl:landUseClassValueCode-AT a glosis_cl:LandUseClassValueCode,
        skos:Concept ;
    skos:broader glosis_cl:landUseClassValueCode-A ;
    skos:definition "Land-use classification of main class Crop agriculture and of subclass Tree and shrub cropping" ;
    skos:inScheme glosis_cl:landUseClassValueCode ;
    skos:narrower glosis_cl:landUseClassValueCode-AT1,
        glosis_cl:landUseClassValueCode-AT2,
        glosis_cl:landUseClassValueCode-AT3,
        glosis_cl:landUseClassValueCode-AT4 ;
    skos:notation "AT" ;
    skos:prefLabel "Tree and shrub cropping"@en .

glosis_cl:landUseClassValueCode-AT1 a glosis_cl:LandUseClassValueCode,
        skos:Concept ;
    skos:broader glosis_cl:landUseClassValueCode-AT ;
    skos:definition "Land-use classification of main class Crop agriculture and of subclass Tree and shrub cropping and of type Non-irrigated shrub crop cultivation" ;
    skos:inScheme glosis_cl:landUseClassValueCode ;
    skos:notation "AT1" ;
    skos:prefLabel "Non-irrigated tree crop cultivation"@en .

glosis_cl:landUseClassValueCode-AT2 a glosis_cl:LandUseClassValueCode,
        skos:Concept ;
    skos:broader glosis_cl:landUseClassValueCode-AT ;
    skos:definition "Land-use classification of main class Crop agriculture and of subclass Tree and shrub cropping and of type Irrigated tree crop cultivation" ;
    skos:inScheme glosis_cl:landUseClassValueCode ;
    skos:notation "AT2" ;
    skos:prefLabel "Irrigated tree crop cultivation"@en .

glosis_cl:landUseClassValueCode-AT3 a glosis_cl:LandUseClassValueCode,
        skos:Concept ;
    skos:broader glosis_cl:landUseClassValueCode-AT ;
    skos:definition "Land-use classification of main class Crop agriculture and of subclass Tree and shrub cropping and of type Non-irrigated shrub crop cultivation" ;
    skos:inScheme glosis_cl:landUseClassValueCode ;
    skos:notation "AT3" ;
    skos:prefLabel "Non-irrigated shrub crop cultivation"@en .

glosis_cl:landUseClassValueCode-AT4 a glosis_cl:LandUseClassValueCode,
        skos:Concept ;
    skos:broader glosis_cl:landUseClassValueCode-AT ;
    skos:definition "Land-use classification of main class Crop agriculture and of subclass Tree and shrub cropping and of type Irrigated shrub crop cultivation" ;
    skos:inScheme glosis_cl:landUseClassValueCode ;
    skos:notation "AT4" ;
    skos:prefLabel "Irrigated shrub crop cultivation"@en .

glosis_cl:landUseClassValueCode-F a glosis_cl:LandUseClassValueCode,
        skos:Concept ;
    skos:definition "Land-use classification of main class Forestry" ;
    skos:inScheme glosis_cl:landUseClassValueCode ;
    skos:narrower glosis_cl:landUseClassValueCode-FN,
        glosis_cl:landUseClassValueCode-FP ;
    skos:notation "F" ;
    skos:prefLabel "F = Forestry"@en ;
    skos:topConceptOf glosis_cl:landUseClassValueCode .

glosis_cl:landUseClassValueCode-FN a glosis_cl:LandUseClassValueCode,
        skos:Concept ;
    skos:broader glosis_cl:landUseClassValueCode-F ;
    skos:definition "Land-use classification of main class Forestry and of subclass Natural forest and woodland" ;
    skos:inScheme glosis_cl:landUseClassValueCode ;
    skos:narrower glosis_cl:landUseClassValueCode-FN1,
        glosis_cl:landUseClassValueCode-FN2 ;
    skos:notation "FN" ;
    skos:prefLabel "Natural forest and woodland"@en .

glosis_cl:landUseClassValueCode-FN1 a glosis_cl:LandUseClassValueCode,
        skos:Concept ;
    skos:broader glosis_cl:landUseClassValueCode-FN ;
    skos:definition "Land-use classification of main class Forestry and of subclass Natural forest and woodland and of type Selective felling" ;
    skos:inScheme glosis_cl:landUseClassValueCode ;
    skos:notation "FN1" ;
    skos:prefLabel "Selective felling"@en .

glosis_cl:landUseClassValueCode-FN2 a glosis_cl:LandUseClassValueCode,
        skos:Concept ;
    skos:broader glosis_cl:landUseClassValueCode-FN ;
    skos:definition "Land-use classification of main class Forestry and of subclass Natural forest and woodland and of type Clear felling" ;
    skos:inScheme glosis_cl:landUseClassValueCode ;
    skos:notation "FN2" ;
    skos:prefLabel "Clear felling"@en .

glosis_cl:landUseClassValueCode-FP a glosis_cl:LandUseClassValueCode,
        skos:Concept ;
    skos:broader glosis_cl:landUseClassValueCode-F ;
    skos:definition "Land-use classification of main class Forestry and of subclass Plantation forestry" ;
    skos:inScheme glosis_cl:landUseClassValueCode ;
    skos:notation "FP" ;
    skos:prefLabel "Plantation forestry"@en .

glosis_cl:landUseClassValueCode-H a glosis_cl:LandUseClassValueCode,
        skos:Concept ;
    skos:definition "Land-use classification of main class Animal husbandry" ;
    skos:inScheme glosis_cl:landUseClassValueCode ;
    skos:narrower glosis_cl:landUseClassValueCode-HE,
        glosis_cl:landUseClassValueCode-HI ;
    skos:notation "H" ;
    skos:prefLabel "Animal husbandry"@en ;
    skos:topConceptOf glosis_cl:landUseClassValueCode .

glosis_cl:landUseClassValueCode-HE a glosis_cl:LandUseClassValueCode,
        skos:Concept ;
    skos:broader glosis_cl:landUseClassValueCode-H ;
    skos:definition "Land-use classification of main class Animal husbandry and of subclass Extensive grazing" ;
    skos:inScheme glosis_cl:landUseClassValueCode ;
    skos:narrower glosis_cl:landUseClassValueCode-HE1,
        glosis_cl:landUseClassValueCode-HE2,
        glosis_cl:landUseClassValueCode-HE3 ;
    skos:notation "HE" ;
    skos:prefLabel "Extensive grazing"@en .

glosis_cl:landUseClassValueCode-HE1 a glosis_cl:LandUseClassValueCode,
        skos:Concept ;
    skos:broader glosis_cl:landUseClassValueCode-HE ;
    skos:definition "Land-use classification of main class Animal husbandry and of subclass Extensive grazing and of type Nomadism" ;
    skos:inScheme glosis_cl:landUseClassValueCode ;
    skos:notation "HE1" ;
    skos:prefLabel "Nomadism"@en .

glosis_cl:landUseClassValueCode-HE2 a glosis_cl:LandUseClassValueCode,
        skos:Concept ;
    skos:broader glosis_cl:landUseClassValueCode-HE ;
    skos:definition "Land-use classification of main class Animal husbandry and of subclass Extensive grazing and of type Semi-nomadism" ;
    skos:inScheme glosis_cl:landUseClassValueCode ;
    skos:notation "HE2" ;
    skos:prefLabel "Semi-nomadism"@en .

glosis_cl:landUseClassValueCode-HE3 a glosis_cl:LandUseClassValueCode,
        skos:Concept ;
    skos:broader glosis_cl:landUseClassValueCode-HE ;
    skos:definition "Land-use classification of main class Animal husbandry and of subclass Extensive grazing and of type Ranching" ;
    skos:inScheme glosis_cl:landUseClassValueCode ;
    skos:notation "HE3" ;
    skos:prefLabel "Ranching"@en .

glosis_cl:landUseClassValueCode-HI a glosis_cl:LandUseClassValueCode,
        skos:Concept ;
    skos:broader glosis_cl:landUseClassValueCode-H ;
    skos:definition "Land-use classification of main class Animal husbandry and of subclass Intensive grazing" ;
    skos:inScheme glosis_cl:landUseClassValueCode ;
    skos:narrower glosis_cl:landUseClassValueCode-HI1,
        glosis_cl:landUseClassValueCode-HI2 ;
    skos:notation "HI" ;
    skos:prefLabel "Intensive grazing"@en .

glosis_cl:landUseClassValueCode-HI1 a glosis_cl:LandUseClassValueCode,
        skos:Concept ;
    skos:broader glosis_cl:landUseClassValueCode-HI ;
    skos:definition "Land-use classification of main class Animal husbandry and of subclass Intensive grazing and of type Animal production" ;
    skos:inScheme glosis_cl:landUseClassValueCode ;
    skos:notation "HI1" ;
    skos:prefLabel "Animal production"@en .

glosis_cl:landUseClassValueCode-HI2 a glosis_cl:LandUseClassValueCode,
        skos:Concept ;
    skos:broader glosis_cl:landUseClassValueCode-HI ;
    skos:definition "Land-use classification of main class Animal husbandry and of subclass Intensive grazing and of type Dairying" ;
    skos:inScheme glosis_cl:landUseClassValueCode ;
    skos:notation "HI2" ;
    skos:prefLabel "Dairying"@en .

glosis_cl:landUseClassValueCode-M a glosis_cl:LandUseClassValueCode,
        skos:Concept ;
    skos:definition "Land-use classification of main class Mixed farming" ;
    skos:inScheme glosis_cl:landUseClassValueCode ;
    skos:narrower glosis_cl:landUseClassValueCode-MF,
        glosis_cl:landUseClassValueCode-MP ;
    skos:notation "M" ;
    skos:prefLabel "M = Mixed farming"@en ;
    skos:topConceptOf glosis_cl:landUseClassValueCode .

glosis_cl:landUseClassValueCode-MF a glosis_cl:LandUseClassValueCode,
        skos:Concept ;
    skos:broader glosis_cl:landUseClassValueCode-M ;
    skos:definition "Land-use classification of main class Mixed farming and of subclass Agroforestry" ;
    skos:inScheme glosis_cl:landUseClassValueCode ;
    skos:notation "MF" ;
    skos:prefLabel "Agroforestry"@en .

glosis_cl:landUseClassValueCode-MP a glosis_cl:LandUseClassValueCode,
        skos:Concept ;
    skos:broader glosis_cl:landUseClassValueCode-M ;
    skos:definition "Land-use classification of main class Mixed farming and of subclass Agropastoralism" ;
    skos:inScheme glosis_cl:landUseClassValueCode ;
    skos:notation "MP" ;
    skos:prefLabel "Agropastoralism"@en .

glosis_cl:landUseClassValueCode-Oi a glosis_cl:LandUseClassValueCode,
        skos:Concept ;
    skos:definition "Land-use classification of main class Other land uses" ;
    skos:inScheme glosis_cl:landUseClassValueCode ;
    skos:notation "O" ;
    skos:prefLabel "Other land uses"@en ;
    skos:topConceptOf glosis_cl:landUseClassValueCode .

glosis_cl:landUseClassValueCode-P a glosis_cl:LandUseClassValueCode,
        skos:Concept ;
    skos:definition "Land-use classification of main class Nature protection" ;
    skos:inScheme glosis_cl:landUseClassValueCode ;
    skos:narrower glosis_cl:landUseClassValueCode-PD,
        glosis_cl:landUseClassValueCode-PN ;
    skos:notation "P" ;
    skos:prefLabel "P = Nature protection"@en ;
    skos:topConceptOf glosis_cl:landUseClassValueCode .

glosis_cl:landUseClassValueCode-PD a glosis_cl:LandUseClassValueCode,
        skos:Concept ;
    skos:broader glosis_cl:landUseClassValueCode-P ;
    skos:definition "Land-use classification of main class Nature protection and of subclass Degradation control" ;
    skos:inScheme glosis_cl:landUseClassValueCode ;
    skos:narrower glosis_cl:landUseClassValueCode-PD1,
        glosis_cl:landUseClassValueCode-PD2 ;
    skos:notation "PD" ;
    skos:prefLabel "Degradation control"@en .

glosis_cl:landUseClassValueCode-PD1 a glosis_cl:LandUseClassValueCode,
        skos:Concept ;
    skos:broader glosis_cl:landUseClassValueCode-PD ;
    skos:definition "Land-use classification of main class Nature protection and of subclass Degradation control and of type Without interference" ;
    skos:inScheme glosis_cl:landUseClassValueCode ;
    skos:notation "PD1" ;
    skos:prefLabel "Without interference"@en .

glosis_cl:landUseClassValueCode-PD2 a glosis_cl:LandUseClassValueCode,
        skos:Concept ;
    skos:broader glosis_cl:landUseClassValueCode-PD ;
    skos:definition "Land-use classification of main class Nature protection and of subclass Degradation control and of type With interference" ;
    skos:inScheme glosis_cl:landUseClassValueCode ;
    skos:notation "PD2" ;
    skos:prefLabel "With interference"@en .

glosis_cl:landUseClassValueCode-PN a glosis_cl:LandUseClassValueCode,
        skos:Concept ;
    skos:broader glosis_cl:landUseClassValueCode-P ;
    skos:definition "Land-use classification of main class Nature protection and of subclass Nature and game preservation" ;
    skos:inScheme glosis_cl:landUseClassValueCode ;
    skos:narrower glosis_cl:landUseClassValueCode-PN1,
        glosis_cl:landUseClassValueCode-PN2,
        glosis_cl:landUseClassValueCode-PN3 ;
    skos:notation "PN" ;
    skos:prefLabel "Nature and game preservation"@en .

glosis_cl:landUseClassValueCode-PN1 a glosis_cl:LandUseClassValueCode,
        skos:Concept ;
    skos:broader glosis_cl:landUseClassValueCode-PN ;
    skos:definition "Land-use classification of main class Nature protection and of subclass Nature and game preservationand of type Reserves" ;
    skos:inScheme glosis_cl:landUseClassValueCode ;
    skos:notation "PN1" ;
    skos:prefLabel "Reserves"@en .

glosis_cl:landUseClassValueCode-PN2 a glosis_cl:LandUseClassValueCode,
        skos:Concept ;
    skos:broader glosis_cl:landUseClassValueCode-PN ;
    skos:definition "Land-use classification of main class Nature protection and of subclass Nature and game preservation and of type Parks" ;
    skos:inScheme glosis_cl:landUseClassValueCode ;
    skos:notation "PN2" ;
    skos:prefLabel "Parks"@en .

glosis_cl:landUseClassValueCode-PN3 a glosis_cl:LandUseClassValueCode,
        skos:Concept ;
    skos:broader glosis_cl:landUseClassValueCode-PN ;
    skos:definition "Land-use classification of main class Nature protection and of subclass Nature and game preservation and of type Wildlife management" ;
    skos:inScheme glosis_cl:landUseClassValueCode ;
    skos:notation "PN3" ;
    skos:prefLabel "Wildlife management"@en .

glosis_cl:landUseClassValueCode-S a glosis_cl:LandUseClassValueCode,
        skos:Concept ;
    skos:definition "Land-use classification of main class Settlement, industry" ;
    skos:inScheme glosis_cl:landUseClassValueCode ;
    skos:narrower glosis_cl:landUseClassValueCode-SC,
        glosis_cl:landUseClassValueCode-SD,
        glosis_cl:landUseClassValueCode-SI,
        glosis_cl:landUseClassValueCode-SR,
        glosis_cl:landUseClassValueCode-ST,
        glosis_cl:landUseClassValueCode-SX ;
    skos:notation "S" ;
    skos:prefLabel "S = Settlement, industry"@en ;
    skos:topConceptOf glosis_cl:landUseClassValueCode .

glosis_cl:landUseClassValueCode-SC a glosis_cl:LandUseClassValueCode,
        skos:Concept ;
    skos:broader glosis_cl:landUseClassValueCode-S ;
    skos:definition "Land-use classification of main class Settlement, industry and of subclass Recreational use" ;
    skos:inScheme glosis_cl:landUseClassValueCode ;
    skos:notation "SC" ;
    skos:prefLabel "Recreational use"@en .

glosis_cl:landUseClassValueCode-SD a glosis_cl:LandUseClassValueCode,
        skos:Concept ;
    skos:broader glosis_cl:landUseClassValueCode-S ;
    skos:definition "Land-use classification of main class Settlement, industry and of subclass Disposal sites" ;
    skos:inScheme glosis_cl:landUseClassValueCode ;
    skos:notation "SD" ;
    skos:prefLabel "Disposal sites"@en .

glosis_cl:landUseClassValueCode-SI a glosis_cl:LandUseClassValueCode,
        skos:Concept ;
    skos:broader glosis_cl:landUseClassValueCode-S ;
    skos:definition "Land-use classification of main class Settlement, industry and of subclass Industrial use" ;
    skos:inScheme glosis_cl:landUseClassValueCode ;
    skos:notation "SI" ;
    skos:prefLabel "Industrial use"@en .

glosis_cl:landUseClassValueCode-SR a glosis_cl:LandUseClassValueCode,
        skos:Concept ;
    skos:broader glosis_cl:landUseClassValueCode-S ;
    skos:definition "Land-use classification of main class Settlement or industry and of subclass Residential use" ;
    skos:inScheme glosis_cl:landUseClassValueCode ;
    skos:notation "SR" ;
    skos:prefLabel "Residential use"@en .

glosis_cl:landUseClassValueCode-ST a glosis_cl:LandUseClassValueCode,
        skos:Concept ;
    skos:broader glosis_cl:landUseClassValueCode-S ;
    skos:definition "Land-use classification of main class Settlement, industry and of subclass Transport" ;
    skos:inScheme glosis_cl:landUseClassValueCode ;
    skos:notation "ST" ;
    skos:prefLabel "Transport"@en .

glosis_cl:landUseClassValueCode-SX a glosis_cl:LandUseClassValueCode,
        skos:Concept ;
    skos:broader glosis_cl:landUseClassValueCode-S ;
    skos:definition "Land-use classification of main class Settlement, industry and of subclass Excavations" ;
    skos:inScheme glosis_cl:landUseClassValueCode ;
    skos:notation "SX" ;
    skos:prefLabel "Excavations"@en .

glosis_cl:landUseClassValueCode-U a glosis_cl:LandUseClassValueCode,
        skos:Concept ;
    skos:definition "Land-use classification of main class Not used and not managed" ;
    skos:inScheme glosis_cl:landUseClassValueCode ;
    skos:notation "U" ;
    skos:prefLabel "Not used and not managed"@en ;
    skos:topConceptOf glosis_cl:landUseClassValueCode .

glosis_cl:landUseClassValueCode-Y a glosis_cl:LandUseClassValueCode,
        skos:Concept ;
    skos:definition "Land-use classification of main class Military area" ;
    skos:inScheme glosis_cl:landUseClassValueCode ;
    skos:notation "Y" ;
    skos:prefLabel "Military area"@en ;
    skos:topConceptOf glosis_cl:landUseClassValueCode .

glosis_cl:landformComplexValueCode-CU a glosis_cl:LandformComplexValueCode,
        skos:Concept ;
    skos:definition "Cuesta-shaped lanform" ;
    skos:inScheme glosis_cl:landformComplexValueCode ;
    skos:notation "CU" ;
    skos:prefLabel "Cuesta-shaped"@en ;
    skos:topConceptOf glosis_cl:landformComplexValueCode .

glosis_cl:landformComplexValueCode-DO a glosis_cl:LandformComplexValueCode,
        skos:Concept ;
    skos:definition "Dome-shaped landform" ;
    skos:inScheme glosis_cl:landformComplexValueCode ;
    skos:notation "DO" ;
    skos:prefLabel "Dome-shaped"@en ;
    skos:topConceptOf glosis_cl:landformComplexValueCode .

glosis_cl:landformComplexValueCode-DU a glosis_cl:LandformComplexValueCode,
        skos:Concept ;
    skos:definition "Dune-shaped landform" ;
    skos:inScheme glosis_cl:landformComplexValueCode ;
    skos:notation "DU" ;
    skos:prefLabel "Dune-shaped"@en ;
    skos:topConceptOf glosis_cl:landformComplexValueCode .

glosis_cl:landformComplexValueCode-IM a glosis_cl:LandformComplexValueCode,
        skos:Concept ;
    skos:definition "With intermontane plains landform(occupying > 15%)" ;
    skos:inScheme glosis_cl:landformComplexValueCode ;
    skos:notation "IM" ;
    skos:prefLabel "With intermontane plains (occupying > 15%)"@en ;
    skos:topConceptOf glosis_cl:landformComplexValueCode .

glosis_cl:landformComplexValueCode-IN a glosis_cl:LandformComplexValueCode,
        skos:Concept ;
    skos:definition "Inselberg covered (occupying > 1% of level land)" ;
    skos:inScheme glosis_cl:landformComplexValueCode ;
    skos:notation "IN" ;
    skos:prefLabel "Inselberg covered (occupying > 1% of level land)"@en ;
    skos:topConceptOf glosis_cl:landformComplexValueCode .

glosis_cl:landformComplexValueCode-KA a glosis_cl:LandformComplexValueCode,
        skos:Concept ;
    skos:definition "Strong karst landform" ;
    skos:inScheme glosis_cl:landformComplexValueCode ;
    skos:notation "KA" ;
    skos:prefLabel "Strong karst"@en ;
    skos:topConceptOf glosis_cl:landformComplexValueCode .

glosis_cl:landformComplexValueCode-RI a glosis_cl:LandformComplexValueCode,
        skos:Concept ;
    skos:definition "Ridged Landform" ;
    skos:inScheme glosis_cl:landformComplexValueCode ;
    skos:notation "RI" ;
    skos:prefLabel "Ridged"@en ;
    skos:topConceptOf glosis_cl:landformComplexValueCode .

glosis_cl:landformComplexValueCode-TE a glosis_cl:LandformComplexValueCode,
        skos:Concept ;
    skos:definition "Terraced landform" ;
    skos:inScheme glosis_cl:landformComplexValueCode ;
    skos:notation "TE" ;
    skos:prefLabel "Terraced"@en ;
    skos:topConceptOf glosis_cl:landformComplexValueCode .

glosis_cl:landformComplexValueCode-WE a glosis_cl:LandformComplexValueCode,
        skos:Concept ;
    skos:definition "With wetlands landform (occupying > 15%)" ;
    skos:inScheme glosis_cl:landformComplexValueCode ;
    skos:notation "WE" ;
    skos:prefLabel "With wetlands (occupying > 15%)"@en ;
    skos:topConceptOf glosis_cl:landformComplexValueCode .

glosis_cl:lithologyValueCode-I a glosis_cl:LithologyValueCode,
        skos:Concept ;
    skos:definition "Hierarchy of lithology from the major class of igneous rock" ;
    skos:inScheme glosis_cl:lithologyValueCode ;
    skos:narrower glosis_cl:lithologyValueCode-IA,
        glosis_cl:lithologyValueCode-IB,
        glosis_cl:lithologyValueCode-II,
        glosis_cl:lithologyValueCode-IP,
        glosis_cl:lithologyValueCode-IU ;
    skos:notation "I" ;
    skos:prefLabel "igneous rock"@en ;
    skos:topConceptOf glosis_cl:lithologyValueCode .

glosis_cl:lithologyValueCode-IA a glosis_cl:LithologyValueCode,
        skos:Concept ;
    skos:broader glosis_cl:lithologyValueCode-I ;
    skos:definition "Hierarchy of lithology from the major class of igneous rock and the group of acid igneous" ;
    skos:inScheme glosis_cl:lithologyValueCode ;
    skos:narrower glosis_cl:lithologyValueCode-IA1,
        glosis_cl:lithologyValueCode-IA2,
        glosis_cl:lithologyValueCode-IA3,
        glosis_cl:lithologyValueCode-IA4 ;
    skos:notation "IA" ;
    skos:prefLabel "acid igneous"@en .

glosis_cl:lithologyValueCode-IA1 a glosis_cl:LithologyValueCode,
        skos:Concept ;
    skos:broader glosis_cl:lithologyValueCode-IA ;
    skos:definition "Hierarchy of lithology from the major class of igneous rock and the group of acid igneous of type diorite" ;
    skos:inScheme glosis_cl:lithologyValueCode ;
    skos:notation "IA1" ;
    skos:prefLabel "diorite"@en .

glosis_cl:lithologyValueCode-IA2 a glosis_cl:LithologyValueCode,
        skos:Concept ;
    skos:broader glosis_cl:lithologyValueCode-IA ;
    skos:definition "Hierarchy of lithology from the major class of igneous rock and the group of acid igneous of type grano-diorite" ;
    skos:inScheme glosis_cl:lithologyValueCode ;
    skos:notation "IA2" ;
    skos:prefLabel "grano-diorite"@en .

glosis_cl:lithologyValueCode-IA3 a glosis_cl:LithologyValueCode,
        skos:Concept ;
    skos:broader glosis_cl:lithologyValueCode-IA ;
    skos:definition "Hierarchy of lithology from the major class of igneous rock and the group of acid igneous of type quartz-diorite" ;
    skos:inScheme glosis_cl:lithologyValueCode ;
    skos:notation "IA3" ;
    skos:prefLabel "quartz-diorite"@en .

glosis_cl:lithologyValueCode-IA4 a glosis_cl:LithologyValueCode,
        skos:Concept ;
    skos:broader glosis_cl:lithologyValueCode-IA ;
    skos:definition "Hierarchy of lithology from the major class of sedimentary rock (unconsolidated) and the group of acid igneous of type rhyolite" ;
    skos:inScheme glosis_cl:lithologyValueCode ;
    skos:notation "IA4" ;
    skos:prefLabel "rhyolite"@en .

glosis_cl:lithologyValueCode-IB a glosis_cl:LithologyValueCode,
        skos:Concept ;
    skos:broader glosis_cl:lithologyValueCode-I ;
    skos:definition "Hierarchy of lithology from the major class of igneous rock and the group of basic igneous" ;
    skos:inScheme glosis_cl:lithologyValueCode ;
    skos:narrower glosis_cl:lithologyValueCode-IB1,
        glosis_cl:lithologyValueCode-IB2,
        glosis_cl:lithologyValueCode-IB3 ;
    skos:notation "IB" ;
    skos:prefLabel "basic igneous"@en .

glosis_cl:lithologyValueCode-IB1 a glosis_cl:LithologyValueCode,
        skos:Concept ;
    skos:broader glosis_cl:lithologyValueCode-IB ;
    skos:definition "Hierarchy of lithology from the major class of igneous rock and the group of basic igneous of type gabbro" ;
    skos:inScheme glosis_cl:lithologyValueCode ;
    skos:notation "IB1" ;
    skos:prefLabel "gabbro"@en .

glosis_cl:lithologyValueCode-IB2 a glosis_cl:LithologyValueCode,
        skos:Concept ;
    skos:broader glosis_cl:lithologyValueCode-IB ;
    skos:definition "Hierarchy of lithology from the major class of igneous rock and the group of basic igneous of type basalt" ;
    skos:inScheme glosis_cl:lithologyValueCode ;
    skos:notation "IB2" ;
    skos:prefLabel "basalt"@en .

glosis_cl:lithologyValueCode-IB3 a glosis_cl:LithologyValueCode,
        skos:Concept ;
    skos:broader glosis_cl:lithologyValueCode-IB ;
    skos:definition "Hierarchy of lithology from the major class of igneous rock and the group of basic igneous of type dolerite" ;
    skos:inScheme glosis_cl:lithologyValueCode ;
    skos:notation "IB3" ;
    skos:prefLabel "dolerite"@en .

glosis_cl:lithologyValueCode-II a glosis_cl:LithologyValueCode,
        skos:Concept ;
    skos:broader glosis_cl:lithologyValueCode-I ;
    skos:definition "Hierarchy of lithology from the major class of igneous rock and the group of intermediate igneous" ;
    skos:inScheme glosis_cl:lithologyValueCode ;
    skos:narrower glosis_cl:lithologyValueCode-II1,
        glosis_cl:lithologyValueCode-II2 ;
    skos:notation "II" ;
    skos:prefLabel "intermediate igneous"@en .

glosis_cl:lithologyValueCode-II1 a glosis_cl:LithologyValueCode,
        skos:Concept ;
    skos:broader glosis_cl:lithologyValueCode-II ;
    skos:definition "Hierarchy of lithology from the major class of igneous rock and the group of intermediate igneous of type andesite, trachyte, phonolite" ;
    skos:inScheme glosis_cl:lithologyValueCode ;
    skos:notation "II1" ;
    skos:prefLabel "andesite, trachyte, phonolite"@en .

glosis_cl:lithologyValueCode-II2 a glosis_cl:LithologyValueCode,
        skos:Concept ;
    skos:broader glosis_cl:lithologyValueCode-II ;
    skos:definition "Hierarchy of lithology from the major class of igneous rock and the group of intermediate igneous of type diorite-syenite" ;
    skos:inScheme glosis_cl:lithologyValueCode ;
    skos:notation "II2" ;
    skos:prefLabel "diorite-syenite"@en .

glosis_cl:lithologyValueCode-IP a glosis_cl:LithologyValueCode,
        skos:Concept ;
    skos:broader glosis_cl:lithologyValueCode-I ;
    skos:definition "Hierarchy of lithology from the major class of igneous rock and the group of pyroclastic" ;
    skos:inScheme glosis_cl:lithologyValueCode ;
    skos:narrower glosis_cl:lithologyValueCode-IP1,
        glosis_cl:lithologyValueCode-IP2,
        glosis_cl:lithologyValueCode-IP3,
        glosis_cl:lithologyValueCode-IP4 ;
    skos:notation "IP" ;
    skos:prefLabel "pyroclastic"@en .

glosis_cl:lithologyValueCode-IP1 a glosis_cl:LithologyValueCode,
        skos:Concept ;
    skos:broader glosis_cl:lithologyValueCode-IP ;
    skos:definition "Hierarchy of lithology from the major class of igneous rock and the group of pyroclastic of type tuff, tuffite" ;
    skos:inScheme glosis_cl:lithologyValueCode ;
    skos:notation "IP1" ;
    skos:prefLabel "tuff, tuffite"@en .

glosis_cl:lithologyValueCode-IP2 a glosis_cl:LithologyValueCode,
        skos:Concept ;
    skos:broader glosis_cl:lithologyValueCode-IP ;
    skos:definition "Hierarchy of lithology from the major class of igneous rock and the group of pyroclastic of type volcanic scoria/breccia" ;
    skos:inScheme glosis_cl:lithologyValueCode ;
    skos:notation "IP2" ;
    skos:prefLabel "volcanic scoria/breccia"@en .

glosis_cl:lithologyValueCode-IP3 a glosis_cl:LithologyValueCode,
        skos:Concept ;
    skos:broader glosis_cl:lithologyValueCode-IP ;
    skos:definition "Hierarchy of lithology from the major class of igneous rock and the group of pyroclastic of type volcanic ash" ;
    skos:inScheme glosis_cl:lithologyValueCode ;
    skos:notation "IP3" ;
    skos:prefLabel "volcanic ash"@en .

glosis_cl:lithologyValueCode-IP4 a glosis_cl:LithologyValueCode,
        skos:Concept ;
    skos:broader glosis_cl:lithologyValueCode-IP ;
    skos:definition "Hierarchy of lithology from the major class of metamorphic rock and the group of acid metamorphic of type ignimbrite" ;
    skos:inScheme glosis_cl:lithologyValueCode ;
    skos:notation "IP4" ;
    skos:prefLabel "ignimbrite"@en .

glosis_cl:lithologyValueCode-IU a glosis_cl:LithologyValueCode,
        skos:Concept ;
    skos:broader glosis_cl:lithologyValueCode-I ;
    skos:definition "Hierarchy of lithology from the major class of igneous rock and the group of ultrabasic igneous" ;
    skos:inScheme glosis_cl:lithologyValueCode ;
    skos:narrower glosis_cl:lithologyValueCode-IU1,
        glosis_cl:lithologyValueCode-IU2,
        glosis_cl:lithologyValueCode-IU3 ;
    skos:notation "IU" ;
    skos:prefLabel "ultrabasic igneous"@en .

glosis_cl:lithologyValueCode-IU1 a glosis_cl:LithologyValueCode,
        skos:Concept ;
    skos:broader glosis_cl:lithologyValueCode-IU ;
    skos:definition "Hierarchy of lithology from the major class of igneous rock and the group of ultrabasic igneous of type peridotite" ;
    skos:inScheme glosis_cl:lithologyValueCode ;
    skos:notation "IU1" ;
    skos:prefLabel "peridotite"@en .

glosis_cl:lithologyValueCode-IU2 a glosis_cl:LithologyValueCode,
        skos:Concept ;
    skos:broader glosis_cl:lithologyValueCode-IU ;
    skos:definition "Hierarchy of lithology from the major class of igneous rock and the group of ultrabasic igneous of type pyroxenite" ;
    skos:inScheme glosis_cl:lithologyValueCode ;
    skos:notation "IU2" ;
    skos:prefLabel "pyroxenite"@en .

glosis_cl:lithologyValueCode-IU3 a glosis_cl:LithologyValueCode,
        skos:Concept ;
    skos:broader glosis_cl:lithologyValueCode-IU ;
    skos:definition "Hierarchy of lithology from the major class of igneous rock and the group of ultrabasic igneous of type ilmenite, magnetite, ironstone, serpentine" ;
    skos:inScheme glosis_cl:lithologyValueCode ;
    skos:notation "IU3" ;
    skos:prefLabel "ilmenite, magnetite, ironstone, serpentine"@en .

glosis_cl:lithologyValueCode-M a glosis_cl:LithologyValueCode,
        skos:Concept ;
    skos:definition "Hierarchy of lithology from the major class of metamorphic rock" ;
    skos:inScheme glosis_cl:lithologyValueCode ;
    skos:narrower glosis_cl:lithologyValueCode-MA,
        glosis_cl:lithologyValueCode-MB,
        glosis_cl:lithologyValueCode-MU ;
    skos:notation "M" ;
    skos:prefLabel "metamorphic rock"@en ;
    skos:topConceptOf glosis_cl:lithologyValueCode .

glosis_cl:lithologyValueCode-MA a glosis_cl:LithologyValueCode,
        skos:Concept ;
    skos:broader glosis_cl:lithologyValueCode-M ;
    skos:definition "Hierarchy of lithology from the major class of metamorphic rock and the group of acid metamorphic" ;
    skos:inScheme glosis_cl:lithologyValueCode ;
    skos:narrower glosis_cl:lithologyValueCode-MA1,
        glosis_cl:lithologyValueCode-MA2,
        glosis_cl:lithologyValueCode-MA3,
        glosis_cl:lithologyValueCode-MA4 ;
    skos:notation "MA" ;
    skos:prefLabel "acid metamorphic"@en .

glosis_cl:lithologyValueCode-MA1 a glosis_cl:LithologyValueCode,
        skos:Concept ;
    skos:broader glosis_cl:lithologyValueCode-MA ;
    skos:definition "Hierarchy of lithology from the major class of metamorphic rock and the group of acid metamorphic of type quartzite" ;
    skos:inScheme glosis_cl:lithologyValueCode ;
    skos:notation "MA1" ;
    skos:prefLabel "quartzite"@en .

glosis_cl:lithologyValueCode-MA2 a glosis_cl:LithologyValueCode,
        skos:Concept ;
    skos:broader glosis_cl:lithologyValueCode-MA ;
    skos:definition "Hierarchy of lithology from the major class of metamorphic rock and the group of acid metamorphic of type gneiss, migmatite" ;
    skos:inScheme glosis_cl:lithologyValueCode ;
    skos:notation "MA2" ;
    skos:prefLabel "gneiss, migmatite"@en .

glosis_cl:lithologyValueCode-MA3 a glosis_cl:LithologyValueCode,
        skos:Concept ;
    skos:broader glosis_cl:lithologyValueCode-MA ;
    skos:definition "Hierarchy of lithology from the major class of metamorphic rock and the group of acid metamorphic of type slate, phyllite (pelitic rocks)" ;
    skos:inScheme glosis_cl:lithologyValueCode ;
    skos:notation "MA3" ;
    skos:prefLabel "slate, phyllite (pelitic rocks)"@en .

glosis_cl:lithologyValueCode-MA4 a glosis_cl:LithologyValueCode,
        skos:Concept ;
    skos:broader glosis_cl:lithologyValueCode-MA ;
    skos:definition "Hierarchy of lithology from the major class of metamorphic rock and the group of acid metamorphic of type schist" ;
    skos:inScheme glosis_cl:lithologyValueCode ;
    skos:notation "MA4" ;
    skos:prefLabel "schist"@en .

glosis_cl:lithologyValueCode-MB a glosis_cl:LithologyValueCode,
        skos:Concept ;
    skos:broader glosis_cl:lithologyValueCode-M ;
    skos:definition "Hierarchy of lithology from the major class of metamorphic rock and the group of basic metamorphic" ;
    skos:inScheme glosis_cl:lithologyValueCode ;
    skos:narrower glosis_cl:lithologyValueCode-MB1,
        glosis_cl:lithologyValueCode-MB2,
        glosis_cl:lithologyValueCode-MB3,
        glosis_cl:lithologyValueCode-MB4,
        glosis_cl:lithologyValueCode-MB5,
        glosis_cl:lithologyValueCode-MB6 ;
    skos:notation "MB" ;
    skos:prefLabel "basic metamorphic"@en .

glosis_cl:lithologyValueCode-MB1 a glosis_cl:LithologyValueCode,
        skos:Concept ;
    skos:broader glosis_cl:lithologyValueCode-MB ;
    skos:definition "Hierarchy of lithology from the major class of metamorphic rock and the group of acid metamorphic of type slate, phyllite (pelitic rocks)" ;
    skos:inScheme glosis_cl:lithologyValueCode ;
    skos:notation "MB1" ;
    skos:prefLabel "slate, phyllite (pelitic rocks)"@en .

glosis_cl:lithologyValueCode-MB2 a glosis_cl:LithologyValueCode,
        skos:Concept ;
    skos:broader glosis_cl:lithologyValueCode-MB ;
    skos:definition "Hierarchy of lithology from the major class of metamorphic rock and the group of acid metamorphic of type (green)schist" ;
    skos:inScheme glosis_cl:lithologyValueCode ;
    skos:notation "MB2" ;
    skos:prefLabel "(green)schist"@en .

glosis_cl:lithologyValueCode-MB3 a glosis_cl:LithologyValueCode,
        skos:Concept ;
    skos:broader glosis_cl:lithologyValueCode-MB ;
    skos:definition "Hierarchy of lithology from the major class of metamorphic rock and the group of basic metamorphic of type gneiss rich in Fe–Mg minerals" ;
    skos:inScheme glosis_cl:lithologyValueCode ;
    skos:notation "MB3" ;
    skos:prefLabel "gneiss rich in Fe–Mg minerals"@en .

glosis_cl:lithologyValueCode-MB4 a glosis_cl:LithologyValueCode,
        skos:Concept ;
    skos:broader glosis_cl:lithologyValueCode-MB ;
    skos:definition "Hierarchy of lithology from the major class of metamorphic rock and the group of basic metamorphic of type metamorphic limestone (marble)" ;
    skos:inScheme glosis_cl:lithologyValueCode ;
    skos:notation "MB4" ;
    skos:prefLabel "metamorphic limestone (marble)"@en .

glosis_cl:lithologyValueCode-MB5 a glosis_cl:LithologyValueCode,
        skos:Concept ;
    skos:broader glosis_cl:lithologyValueCode-MB ;
    skos:definition "Hierarchy of lithology from the major class of metamorphic rock and the group of basic metamorphic of type amphibolite" ;
    skos:inScheme glosis_cl:lithologyValueCode ;
    skos:notation "MB5" ;
    skos:prefLabel "amphibolite"@en .

glosis_cl:lithologyValueCode-MB6 a glosis_cl:LithologyValueCode,
        skos:Concept ;
    skos:broader glosis_cl:lithologyValueCode-MB ;
    skos:definition "Hierarchy of lithology from the major class of metamorphic rock and the group of basic metamorphic of type eclogite" ;
    skos:inScheme glosis_cl:lithologyValueCode ;
    skos:notation "MB6" ;
    skos:prefLabel "eclogite"@en .

glosis_cl:lithologyValueCode-MU a glosis_cl:LithologyValueCode,
        skos:Concept ;
    skos:broader glosis_cl:lithologyValueCode-M ;
    skos:definition "Hierarchy of lithology from the major class of metamorphic rock and the group of ultrabasic metamorphic" ;
    skos:inScheme glosis_cl:lithologyValueCode ;
    skos:narrower glosis_cl:lithologyValueCode-MU1 ;
    skos:notation "MU" ;
    skos:prefLabel "ultrabasic metamorphic"@en .

glosis_cl:lithologyValueCode-MU1 a glosis_cl:LithologyValueCode,
        skos:Concept ;
    skos:broader glosis_cl:lithologyValueCode-MU ;
    skos:definition "Hierarchy of lithology from the major class of metamorphic rock and the group of ultrabasic metamorphic of type serpentinite, greenstone" ;
    skos:inScheme glosis_cl:lithologyValueCode ;
    skos:notation "MU1" ;
    skos:prefLabel "serpentinite, greenstone"@en .

glosis_cl:lithologyValueCode-S a glosis_cl:LithologyValueCode,
        skos:Concept ;
    skos:definition "Hierarchy of lithology from the major class of sedimentary rock (consolidated)" ;
    skos:inScheme glosis_cl:lithologyValueCode ;
    skos:narrower glosis_cl:lithologyValueCode-SC,
        glosis_cl:lithologyValueCode-SE,
        glosis_cl:lithologyValueCode-SO ;
    skos:notation "S" ;
    skos:prefLabel "sedimentary rock (consolidated)"@en ;
    skos:topConceptOf glosis_cl:lithologyValueCode .

glosis_cl:lithologyValueCode-SC a glosis_cl:LithologyValueCode,
        skos:Concept ;
    skos:broader glosis_cl:lithologyValueCode-S ;
    skos:definition "Hierarchy of lithology from the major class of sedimentary rock (consolidated) and the group of clastic sediments" ;
    skos:inScheme glosis_cl:lithologyValueCode ;
    skos:narrower glosis_cl:lithologyValueCode-SC1,
        glosis_cl:lithologyValueCode-SC2,
        glosis_cl:lithologyValueCode-SC3,
        glosis_cl:lithologyValueCode-SC4,
        glosis_cl:lithologyValueCode-SC5 ;
    skos:notation "SC" ;
    skos:prefLabel "clastic sediments"@en .

glosis_cl:lithologyValueCode-SC1 a glosis_cl:LithologyValueCode,
        skos:Concept ;
    skos:broader glosis_cl:lithologyValueCode-SC ;
    skos:definition "Hierarchy of lithology from the major class of sedimentary rock (consolidated) and the group of clastic sediments of type conglomerate, breccia" ;
    skos:inScheme glosis_cl:lithologyValueCode ;
    skos:notation "SC1" ;
    skos:prefLabel "conglomerate, breccia"@en .

glosis_cl:lithologyValueCode-SC2 a glosis_cl:LithologyValueCode,
        skos:Concept ;
    skos:broader glosis_cl:lithologyValueCode-SC ;
    skos:definition "Hierarchy of lithology from the major class of sedimentary rock (unconsolidated) and the group of clastic sediments of type sandstone, greywacke, arkose" ;
    skos:inScheme glosis_cl:lithologyValueCode ;
    skos:notation "SC2" ;
    skos:prefLabel "sandstone, greywacke, arkose"@en .

glosis_cl:lithologyValueCode-SC3 a glosis_cl:LithologyValueCode,
        skos:Concept ;
    skos:broader glosis_cl:lithologyValueCode-SC ;
    skos:definition "Hierarchy of lithology from the major class of sedimentary rock (consolidated) and the group of clastic sediments of type silt-, mud-, claystone" ;
    skos:inScheme glosis_cl:lithologyValueCode ;
    skos:notation "SC3" ;
    skos:prefLabel "silt-, mud-, claystone"@en .

glosis_cl:lithologyValueCode-SC4 a glosis_cl:LithologyValueCode,
        skos:Concept ;
    skos:broader glosis_cl:lithologyValueCode-SC ;
    skos:definition "Hierarchy of lithology from the major class of sedimentary rock (consolidated) and the group of clastic sediments of type shale" ;
    skos:inScheme glosis_cl:lithologyValueCode ;
    skos:notation "SC4" ;
    skos:prefLabel "shale"@en .

glosis_cl:lithologyValueCode-SC5 a glosis_cl:LithologyValueCode,
        skos:Concept ;
    skos:broader glosis_cl:lithologyValueCode-SC ;
    skos:definition "Hierarchy of lithology from the major class of sedimentary rock (consolidated)and the group of acid metamorphic of type ironstone" ;
    skos:inScheme glosis_cl:lithologyValueCode ;
    skos:notation "SC5" ;
    skos:prefLabel "ironstone"@en .

glosis_cl:lithologyValueCode-SE a glosis_cl:LithologyValueCode,
        skos:Concept ;
    skos:broader glosis_cl:lithologyValueCode-S ;
    skos:definition "Hierarchy of lithology from the major class of sedimentary rock (consolidated) and the group of evaporites" ;
    skos:inScheme glosis_cl:lithologyValueCode ;
    skos:narrower glosis_cl:lithologyValueCode-SE1,
        glosis_cl:lithologyValueCode-SE2 ;
    skos:notation "SE" ;
    skos:prefLabel "evaporites"@en .

glosis_cl:lithologyValueCode-SE1 a glosis_cl:LithologyValueCode,
        skos:Concept ;
    skos:broader glosis_cl:lithologyValueCode-SE ;
    skos:definition "Hierarchy of lithology from the major class of sedimentary rock (consolidated) and the group of acid evaporites of type anhydrite, gypsum" ;
    skos:inScheme glosis_cl:lithologyValueCode ;
    skos:notation "SE1" ;
    skos:prefLabel "anhydrite, gypsum"@en .

glosis_cl:lithologyValueCode-SE2 a glosis_cl:LithologyValueCode,
        skos:Concept ;
    skos:broader glosis_cl:lithologyValueCode-SE ;
    skos:definition "Hierarchy of lithology from the major class of sedimentary rock (consolidated) and the group of evaporites of type halite" ;
    skos:inScheme glosis_cl:lithologyValueCode ;
    skos:notation "SE2" ;
    skos:prefLabel "halite"@en .

glosis_cl:lithologyValueCode-SO a glosis_cl:LithologyValueCode,
        skos:Concept ;
    skos:broader glosis_cl:lithologyValueCode-S ;
    skos:definition "Hierarchy of lithology from the major class of sedimentary rock (unconsolidated) and the group of carbonatic, organic" ;
    skos:inScheme glosis_cl:lithologyValueCode ;
    skos:narrower glosis_cl:lithologyValueCode-SO1,
        glosis_cl:lithologyValueCode-SO2,
        glosis_cl:lithologyValueCode-SO3 ;
    skos:notation "SO" ;
    skos:prefLabel "carbonatic, organic"@en .

glosis_cl:lithologyValueCode-SO1 a glosis_cl:LithologyValueCode,
        skos:Concept ;
    skos:broader glosis_cl:lithologyValueCode-SO ;
    skos:definition "Hierarchy of lithology from the major class of sedimentary rock (unconsolidated) and the group of carbonatic, organic of type limestone, other carbonate rock" ;
    skos:inScheme glosis_cl:lithologyValueCode ;
    skos:notation "SO1" ;
    skos:prefLabel "limestone, other carbonate rock"@en .

glosis_cl:lithologyValueCode-SO2 a glosis_cl:LithologyValueCode,
        skos:Concept ;
    skos:broader glosis_cl:lithologyValueCode-SO ;
    skos:definition "Hierarchy of lithology from the major class of sedimentary rock (unconsolidated) and the group of carbonatic, organic of type marl and other mixtures" ;
    skos:inScheme glosis_cl:lithologyValueCode ;
    skos:notation "SO2" ;
    skos:prefLabel "marl and other mixtures"@en .

glosis_cl:lithologyValueCode-SO3 a glosis_cl:LithologyValueCode,
        skos:Concept ;
    skos:broader glosis_cl:lithologyValueCode-SO ;
    skos:definition "Hierarchy of lithology from the major class of sedimentary rock (consolidated) and the group of carbonatic, organic of type coals, bitumen and related rocks" ;
    skos:inScheme glosis_cl:lithologyValueCode ;
    skos:notation "SO3" ;
    skos:prefLabel "coals, bitumen and related rocks"@en .

glosis_cl:lithologyValueCode-U a glosis_cl:LithologyValueCode,
        skos:Concept ;
    skos:definition "Hierarchy of lithology from the major class of sedimentary rock (unconsolidated)" ;
    skos:inScheme glosis_cl:lithologyValueCode ;
    skos:narrower glosis_cl:lithologyValueCode-UA,
        glosis_cl:lithologyValueCode-UC,
        glosis_cl:lithologyValueCode-UE,
        glosis_cl:lithologyValueCode-UF,
        glosis_cl:lithologyValueCode-UG,
        glosis_cl:lithologyValueCode-UK,
        glosis_cl:lithologyValueCode-UL,
        glosis_cl:lithologyValueCode-UM,
        glosis_cl:lithologyValueCode-UO,
        glosis_cl:lithologyValueCode-UR,
        glosis_cl:lithologyValueCode-UU ;
    skos:notation "U" ;
    skos:prefLabel "sedimentary rock (unconsolidated)"@en ;
    skos:topConceptOf glosis_cl:lithologyValueCode .

glosis_cl:lithologyValueCode-UA a glosis_cl:LithologyValueCode,
        skos:Concept ;
    skos:broader glosis_cl:lithologyValueCode-U ;
    skos:definition "Hierarchy of lithology from the group of anthropogenic/technogenic" ;
    skos:inScheme glosis_cl:lithologyValueCode ;
    skos:narrower glosis_cl:lithologyValueCode-UA1,
        glosis_cl:lithologyValueCode-UA2 ;
    skos:notation "UA" ;
    skos:prefLabel "anthropogenic/technogenic"@en .

glosis_cl:lithologyValueCode-UA1 a glosis_cl:LithologyValueCode,
        skos:Concept ;
    skos:broader glosis_cl:lithologyValueCode-UA ;
    skos:definition "Hierarchy of lithology from the group of anthropogenic/technogenic of type redeposited natural material" ;
    skos:inScheme glosis_cl:lithologyValueCode ;
    skos:notation "UA1" ;
    skos:prefLabel "redeposited natural material"@en .

glosis_cl:lithologyValueCode-UA2 a glosis_cl:LithologyValueCode,
        skos:Concept ;
    skos:broader glosis_cl:lithologyValueCode-UA ;
    skos:definition "Hierarchy of lithology from the group of unspecified deposits of type industrial/artisanal deposits" ;
    skos:inScheme glosis_cl:lithologyValueCode ;
    skos:notation "UA2" ;
    skos:prefLabel "industrial/artisanal deposits"@en .

glosis_cl:lithologyValueCode-UC a glosis_cl:LithologyValueCode,
        skos:Concept ;
    skos:broader glosis_cl:lithologyValueCode-U ;
    skos:definition "Hierarchy of lithology from the major class of sedimentary rock (unconsolidated) and the group of colluvial" ;
    skos:inScheme glosis_cl:lithologyValueCode ;
    skos:narrower glosis_cl:lithologyValueCode-UC1,
        glosis_cl:lithologyValueCode-UC2 ;
    skos:notation "UC" ;
    skos:prefLabel "colluvial"@en .

glosis_cl:lithologyValueCode-UC1 a glosis_cl:LithologyValueCode,
        skos:Concept ;
    skos:broader glosis_cl:lithologyValueCode-UC ;
    skos:definition "Hierarchy of lithology from the major class of sedimentary rock (consolidated) and the group of colluvial of type slope deposits" ;
    skos:inScheme glosis_cl:lithologyValueCode ;
    skos:notation "UC1" ;
    skos:prefLabel "slope deposits"@en .

glosis_cl:lithologyValueCode-UC2 a glosis_cl:LithologyValueCode,
        skos:Concept ;
    skos:broader glosis_cl:lithologyValueCode-UC ;
    skos:definition "Hierarchy of lithology from the major class of sedimentary rock (consolidated) and the group of colluvial of type lahar" ;
    skos:inScheme glosis_cl:lithologyValueCode ;
    skos:notation "UC2" ;
    skos:prefLabel "lahar"@en .

glosis_cl:lithologyValueCode-UE a glosis_cl:LithologyValueCode,
        skos:Concept ;
    skos:broader glosis_cl:lithologyValueCode-U ;
    skos:definition "Hierarchy of lithology from the major class of sedimentary rock (unconsolidated) and the group of eolian" ;
    skos:inScheme glosis_cl:lithologyValueCode ;
    skos:narrower glosis_cl:lithologyValueCode-UE1,
        glosis_cl:lithologyValueCode-UE2 ;
    skos:notation "UE" ;
    skos:prefLabel "eolian"@en .

glosis_cl:lithologyValueCode-UE1 a glosis_cl:LithologyValueCode,
        skos:Concept ;
    skos:broader glosis_cl:lithologyValueCode-UE ;
    skos:definition "Hierarchy of lithology from the major class of sedimentary rock (consolidated) and the group of eolian of type loess" ;
    skos:inScheme glosis_cl:lithologyValueCode ;
    skos:notation "UE1" ;
    skos:prefLabel "loess"@en .

glosis_cl:lithologyValueCode-UE2 a glosis_cl:LithologyValueCode,
        skos:Concept ;
    skos:broader glosis_cl:lithologyValueCode-UE ;
    skos:definition "Hierarchy of lithology from the major class of sedimentary rock (consolidated) and the group of lacustrine of type sand" ;
    skos:inScheme glosis_cl:lithologyValueCode ;
    skos:notation "UE2" ;
    skos:prefLabel "sand"@en .

glosis_cl:lithologyValueCode-UF a glosis_cl:LithologyValueCode,
        skos:Concept ;
    skos:broader glosis_cl:lithologyValueCode-U ;
    skos:definition "Hierarchy of lithology from the major class of sedimentary rock (consolidated) and the group of fluvial" ;
    skos:inScheme glosis_cl:lithologyValueCode ;
    skos:narrower glosis_cl:lithologyValueCode-UF1,
        glosis_cl:lithologyValueCode-UF2 ;
    skos:notation "UF" ;
    skos:prefLabel "fluvial"@en .

glosis_cl:lithologyValueCode-UF1 a glosis_cl:LithologyValueCode,
        skos:Concept ;
    skos:broader glosis_cl:lithologyValueCode-UF ;
    skos:definition "Hierarchy of lithology from the major class of sedimentary rock (unconsolidated) and the group of fluvial of type sand and gravel" ;
    skos:inScheme glosis_cl:lithologyValueCode ;
    skos:notation "UF1" ;
    skos:prefLabel "sand and gravel"@en .

glosis_cl:lithologyValueCode-UF2 a glosis_cl:LithologyValueCode,
        skos:Concept ;
    skos:broader glosis_cl:lithologyValueCode-UF ;
    skos:definition "Hierarchy of lithology from the major class of sedimentary rock (consolidated) and the group of fluvial of type clay, silt and loam" ;
    skos:inScheme glosis_cl:lithologyValueCode ;
    skos:notation "UF2" ;
    skos:prefLabel "clay, silt and loam"@en .

glosis_cl:lithologyValueCode-UG a glosis_cl:LithologyValueCode,
        skos:Concept ;
    skos:broader glosis_cl:lithologyValueCode-U ;
    skos:definition "Hierarchy of lithology from the major class of sedimentary rock (unconsolidated) and the group of glacial" ;
    skos:inScheme glosis_cl:lithologyValueCode ;
    skos:narrower glosis_cl:lithologyValueCode-UG1,
        glosis_cl:lithologyValueCode-UG2,
        glosis_cl:lithologyValueCode-UG3 ;
    skos:notation "UG" ;
    skos:prefLabel "glacial"@en .

glosis_cl:lithologyValueCode-UG1 a glosis_cl:LithologyValueCode,
        skos:Concept ;
    skos:broader glosis_cl:lithologyValueCode-UG ;
    skos:definition "Hierarchy of lithology from the major class of sedimentary rock (unconsolidated) and the group of glacial of type moraine" ;
    skos:inScheme glosis_cl:lithologyValueCode ;
    skos:notation "UG1" ;
    skos:prefLabel "moraine"@en .

glosis_cl:lithologyValueCode-UG2 a glosis_cl:LithologyValueCode,
        skos:Concept ;
    skos:broader glosis_cl:lithologyValueCode-UG ;
    skos:definition "Hierarchy of lithology from the major class of sedimentary rock (consolidated) and the group of glacial of type glacio-fluvial sand" ;
    skos:inScheme glosis_cl:lithologyValueCode ;
    skos:notation "UG2" ;
    skos:prefLabel "UG2 glacio-fluvial sand"@en .

glosis_cl:lithologyValueCode-UG3 a glosis_cl:LithologyValueCode,
        skos:Concept ;
    skos:broader glosis_cl:lithologyValueCode-UG ;
    skos:definition "Hierarchy of lithology from the major class of sedimentary rock (unconsolidated) and the group of kryogenic of type glacio-fluvial gravel" ;
    skos:inScheme glosis_cl:lithologyValueCode ;
    skos:notation "UG3" ;
    skos:prefLabel "UG3 glacio-fluvial gravel"@en .

glosis_cl:lithologyValueCode-UK a glosis_cl:LithologyValueCode,
        skos:Concept ;
    skos:broader glosis_cl:lithologyValueCode-U ;
    skos:definition "Hierarchy of lithology from the major class of sedimentary rock (consolidated) and the group of kryogenic" ;
    skos:inScheme glosis_cl:lithologyValueCode ;
    skos:narrower glosis_cl:lithologyValueCode-UK1,
        glosis_cl:lithologyValueCode-UK2 ;
    skos:notation "UK" ;
    skos:prefLabel "kryogenic"@en .

glosis_cl:lithologyValueCode-UK1 a glosis_cl:LithologyValueCode,
        skos:Concept ;
    skos:broader glosis_cl:lithologyValueCode-UK ;
    skos:definition "Hierarchy of lithology from the major class of sedimentary rock (unconsolidated) and the group of kryogenic of type periglacial rock debris" ;
    skos:inScheme glosis_cl:lithologyValueCode ;
    skos:notation "UK1" ;
    skos:prefLabel "periglacial rock debris"@en .

glosis_cl:lithologyValueCode-UK2 a glosis_cl:LithologyValueCode,
        skos:Concept ;
    skos:broader glosis_cl:lithologyValueCode-UK ;
    skos:definition "Hierarchy of lithology from the major class of sedimentary rock (unconsolidated) and the group of kryogenic of type periglacial solifluction layer" ;
    skos:inScheme glosis_cl:lithologyValueCode ;
    skos:notation "UK2" ;
    skos:prefLabel "periglacial solifluction layer"@en .

glosis_cl:lithologyValueCode-UL a glosis_cl:LithologyValueCode,
        skos:Concept ;
    skos:broader glosis_cl:lithologyValueCode-U ;
    skos:definition "Hierarchy of lithology from the major class of sedimentary rock (unconsolidated) and the group of lacustrine" ;
    skos:inScheme glosis_cl:lithologyValueCode ;
    skos:narrower glosis_cl:lithologyValueCode-UL1,
        glosis_cl:lithologyValueCode-UL2 ;
    skos:notation "UL" ;
    skos:prefLabel "lacustrine"@en .

glosis_cl:lithologyValueCode-UL1 a glosis_cl:LithologyValueCode,
        skos:Concept ;
    skos:broader glosis_cl:lithologyValueCode-UL ;
    skos:definition "Hierarchy of lithology from the major class of sedimentary rock (unconsolidated) and the group of lacustrine of type sand" ;
    skos:inScheme glosis_cl:lithologyValueCode ;
    skos:notation "UL1" ;
    skos:prefLabel "sand"@en .

glosis_cl:lithologyValueCode-UL2 a glosis_cl:LithologyValueCode,
        skos:Concept ;
    skos:broader glosis_cl:lithologyValueCode-UL ;
    skos:definition "Hierarchy of lithology from the major class of sedimentary rock (unconsolidated) and the group of lacustrine of type silt and clay" ;
    skos:inScheme glosis_cl:lithologyValueCode ;
    skos:notation "UL2" ;
    skos:prefLabel "silt and clay"@en .

glosis_cl:lithologyValueCode-UM a glosis_cl:LithologyValueCode,
        skos:Concept ;
    skos:broader glosis_cl:lithologyValueCode-U ;
    skos:definition "Hierarchy of lithology from the major class of sedimentary rock (consolidated) and the group of marine, estuarine" ;
    skos:inScheme glosis_cl:lithologyValueCode ;
    skos:narrower glosis_cl:lithologyValueCode-UM1,
        glosis_cl:lithologyValueCode-UM2 ;
    skos:notation "UM" ;
    skos:prefLabel "marine, estuarine"@en .

glosis_cl:lithologyValueCode-UM1 a glosis_cl:LithologyValueCode,
        skos:Concept ;
    skos:broader glosis_cl:lithologyValueCode-UM ;
    skos:definition "Hierarchy of lithology from the major class of sedimentary rock (unconsolidated) and the group of marine, estuarine of type sand" ;
    skos:inScheme glosis_cl:lithologyValueCode ;
    skos:notation "UM1" ;
    skos:prefLabel "sand"@en .

glosis_cl:lithologyValueCode-UM2 a glosis_cl:LithologyValueCode,
        skos:Concept ;
    skos:broader glosis_cl:lithologyValueCode-UM ;
    skos:definition "Hierarchy of lithology from the major class of sedimentary rock (consolidated) and the group of marine and estuarine of type clay and silt" ;
    skos:inScheme glosis_cl:lithologyValueCode ;
    skos:notation "UM2" ;
    skos:prefLabel "clay and silt"@en .

glosis_cl:lithologyValueCode-UO a glosis_cl:LithologyValueCode,
        skos:Concept ;
    skos:broader glosis_cl:lithologyValueCode-U ;
    skos:definition "Hierarchy of lithology from the group of organic" ;
    skos:inScheme glosis_cl:lithologyValueCode ;
    skos:narrower glosis_cl:lithologyValueCode-UO1,
        glosis_cl:lithologyValueCode-UO2 ;
    skos:notation "UO" ;
    skos:prefLabel "organic"@en .

glosis_cl:lithologyValueCode-UO1 a glosis_cl:LithologyValueCode,
        skos:Concept ;
    skos:broader glosis_cl:lithologyValueCode-UO ;
    skos:definition "Hierarchy of lithology from the group of organic of type rainwater-fed moor peat" ;
    skos:inScheme glosis_cl:lithologyValueCode ;
    skos:notation "UO1" ;
    skos:prefLabel "rainwater-fed moor peat"@en .

glosis_cl:lithologyValueCode-UO2 a glosis_cl:LithologyValueCode,
        skos:Concept ;
    skos:broader glosis_cl:lithologyValueCode-UO ;
    skos:definition "Hierarchy of lithology from the group of organic of type groundwater-fed bog peat" ;
    skos:inScheme glosis_cl:lithologyValueCode ;
    skos:notation "UO2" ;
    skos:prefLabel "groundwater-fed bog peat"@en .

glosis_cl:lithologyValueCode-UR a glosis_cl:LithologyValueCode,
        skos:Concept ;
    skos:broader glosis_cl:lithologyValueCode-U ;
    skos:definition "Hierarchy of lithology from the major class of sedimentary rock (unconsolidated) and the group of weathered residuum" ;
    skos:inScheme glosis_cl:lithologyValueCode ;
    skos:narrower glosis_cl:lithologyValueCode-UR1 ;
    skos:notation "UR" ;
    skos:prefLabel "weathered residuum"@en .

glosis_cl:lithologyValueCode-UR1 a glosis_cl:LithologyValueCode,
        skos:Concept ;
    skos:broader glosis_cl:lithologyValueCode-UR ;
    skos:definition "Hierarchy of lithology from the major class of sedimentary rock (unconsolidated) and the group of weathered residuum of type bauxite, laterite" ;
    skos:inScheme glosis_cl:lithologyValueCode ;
    skos:notation "UR1" ;
    skos:prefLabel "bauxite, laterite"@en .

glosis_cl:lithologyValueCode-UU a glosis_cl:LithologyValueCode,
        skos:Concept ;
    skos:broader glosis_cl:lithologyValueCode-U ;
    skos:definition "Hierarchy of lithology from the group of unspecified deposits" ;
    skos:inScheme glosis_cl:lithologyValueCode ;
    skos:narrower glosis_cl:lithologyValueCode-UU1,
        glosis_cl:lithologyValueCode-UU2,
        glosis_cl:lithologyValueCode-UU3,
        glosis_cl:lithologyValueCode-UU4,
        glosis_cl:lithologyValueCode-UU5 ;
    skos:notation "UU" ;
    skos:prefLabel "unspecified deposits"@en .

glosis_cl:lithologyValueCode-UU1 a glosis_cl:LithologyValueCode,
        skos:Concept ;
    skos:broader glosis_cl:lithologyValueCode-UU ;
    skos:definition "Hierarchy of lithology from the group of unspecified deposits of type clay" ;
    skos:inScheme glosis_cl:lithologyValueCode ;
    skos:notation "UU1" ;
    skos:prefLabel "clay"@en .

glosis_cl:lithologyValueCode-UU2 a glosis_cl:LithologyValueCode,
        skos:Concept ;
    skos:broader glosis_cl:lithologyValueCode-UU ;
    skos:definition "Hierarchy of lithology from the group of unspecified deposits of type loam and silt" ;
    skos:inScheme glosis_cl:lithologyValueCode ;
    skos:notation "UU2" ;
    skos:prefLabel "loam and silt"@en .

glosis_cl:lithologyValueCode-UU3 a glosis_cl:LithologyValueCode,
        skos:Concept ;
    skos:broader glosis_cl:lithologyValueCode-UU ;
    skos:definition "Hierarchy of lithology from group of unspecified depositsof type sand" ;
    skos:inScheme glosis_cl:lithologyValueCode ;
    skos:notation "UU3" ;
    skos:prefLabel "sand"@en .

glosis_cl:lithologyValueCode-UU4 a glosis_cl:LithologyValueCode,
        skos:Concept ;
    skos:broader glosis_cl:lithologyValueCode-UU ;
    skos:definition "Hierarchy of lithology from the group of unspecified deposits of type gravelly sand" ;
    skos:inScheme glosis_cl:lithologyValueCode ;
    skos:notation "UU4" ;
    skos:prefLabel "gravelly sand"@en .

glosis_cl:lithologyValueCode-UU5 a glosis_cl:LithologyValueCode,
        skos:Concept ;
    skos:broader glosis_cl:lithologyValueCode-UU ;
    skos:definition "Hierarchy of lithology from the group of unspecified deposits of type gravel, broken rock" ;
    skos:inScheme glosis_cl:lithologyValueCode ;
    skos:notation "UU5" ;
    skos:prefLabel "gravel, broken rock"@en .

glosis_cl:majorLandFormValueCode-L a glosis_cl:MajorLandFormValueCode,
        skos:Concept ;
    skos:definition "first level of landform is level land (L)" ;
    skos:inScheme glosis_cl:majorLandFormValueCode ;
    skos:narrower glosis_cl:majorLandFormValueCode-LD,
        glosis_cl:majorLandFormValueCode-LL,
        glosis_cl:majorLandFormValueCode-LP,
        glosis_cl:majorLandFormValueCode-LV ;
    skos:notation "L" ;
    skos:prefLabel "level land"@en ;
    skos:topConceptOf glosis_cl:majorLandFormValueCode .

glosis_cl:majorLandFormValueCode-LD a glosis_cl:MajorLandFormValueCode,
        skos:Concept ;
    skos:broader glosis_cl:majorLandFormValueCode-L ;
    skos:definition "first level of landform is level land (L) and the second level is depression (LD)" ;
    skos:inScheme glosis_cl:majorLandFormValueCode ;
    skos:notation "LD" ;
    skos:prefLabel "depression"@en .

glosis_cl:majorLandFormValueCode-LL a glosis_cl:MajorLandFormValueCode,
        skos:Concept ;
    skos:broader glosis_cl:majorLandFormValueCode-L ;
    skos:definition "first level of landform is level land (L) and the second level is plateau (LL)" ;
    skos:inScheme glosis_cl:majorLandFormValueCode ;
    skos:notation "LL" ;
    skos:prefLabel "plateau"@en .

glosis_cl:majorLandFormValueCode-LP a glosis_cl:MajorLandFormValueCode,
        skos:Concept ;
    skos:broader glosis_cl:majorLandFormValueCode-L ;
    skos:definition "first level of landform is level land (L) and the second level is plain (LP)" ;
    skos:inScheme glosis_cl:majorLandFormValueCode ;
    skos:notation "LP" ;
    skos:prefLabel "plain"@en .

glosis_cl:majorLandFormValueCode-LV a glosis_cl:MajorLandFormValueCode,
        skos:Concept ;
    skos:broader glosis_cl:majorLandFormValueCode-L ;
    skos:definition "first level of landform is level land (L) and the second level is valley floor (LV)" ;
    skos:inScheme glosis_cl:majorLandFormValueCode ;
    skos:notation "LV" ;
    skos:prefLabel "valley floor"@en .

glosis_cl:majorLandFormValueCode-S a glosis_cl:MajorLandFormValueCode,
        skos:Concept ;
    skos:definition "first level of landform is sloping land (S)" ;
    skos:inScheme glosis_cl:majorLandFormValueCode ;
    skos:narrower glosis_cl:majorLandFormValueCode-SE,
        glosis_cl:majorLandFormValueCode-SH,
        glosis_cl:majorLandFormValueCode-SM,
        glosis_cl:majorLandFormValueCode-SP,
        glosis_cl:majorLandFormValueCode-SV ;
    skos:notation "S" ;
    skos:prefLabel "sloping land"@en ;
    skos:topConceptOf glosis_cl:majorLandFormValueCode .

glosis_cl:majorLandFormValueCode-SE a glosis_cl:MajorLandFormValueCode,
        skos:Concept ;
    skos:broader glosis_cl:majorLandFormValueCode-S ;
    skos:definition "first level of landform is sloping land (S) and the second level is medium-gradient escarpment zone (SE)" ;
    skos:inScheme glosis_cl:majorLandFormValueCode ;
    skos:notation "SE" ;
    skos:prefLabel "medium-gradient escarpment zone"@en .

glosis_cl:majorLandFormValueCode-SH a glosis_cl:MajorLandFormValueCode,
        skos:Concept ;
    skos:broader glosis_cl:majorLandFormValueCode-S ;
    skos:definition "first level of landform is sloping land (S) and the second level is medium gradient hill (SH)" ;
    skos:inScheme glosis_cl:majorLandFormValueCode ;
    skos:notation "SH" ;
    skos:prefLabel "medium-gradient hill"@en .

glosis_cl:majorLandFormValueCode-SM a glosis_cl:MajorLandFormValueCode,
        skos:Concept ;
    skos:broader glosis_cl:majorLandFormValueCode-S ;
    skos:definition "first level of landform is sloping land (S) and the second level is medium-gradient mountain (SM)" ;
    skos:inScheme glosis_cl:majorLandFormValueCode ;
    skos:notation "SM" ;
    skos:prefLabel "medium-gradient mountain"@en .

glosis_cl:majorLandFormValueCode-SP a glosis_cl:MajorLandFormValueCode,
        skos:Concept ;
    skos:broader glosis_cl:majorLandFormValueCode-S ;
    skos:definition "first level of landform is sloping land (S) and the second level is dissected plain (SP)" ;
    skos:inScheme glosis_cl:majorLandFormValueCode ;
    skos:notation "SP" ;
    skos:prefLabel "dissected plain"@en .

glosis_cl:majorLandFormValueCode-SV a glosis_cl:MajorLandFormValueCode,
        skos:Concept ;
    skos:broader glosis_cl:majorLandFormValueCode-S ;
    skos:definition "first level of landform is sloping land (S) and the second level is medium gradient valley (SV)" ;
    skos:inScheme glosis_cl:majorLandFormValueCode ;
    skos:notation "SV" ;
    skos:prefLabel "medium-gradient valley"@en .

glosis_cl:majorLandFormValueCode-T a glosis_cl:MajorLandFormValueCode,
        skos:Concept ;
    skos:definition "first level of landform is steep land (T)" ;
    skos:inScheme glosis_cl:majorLandFormValueCode ;
    skos:narrower glosis_cl:majorLandFormValueCode-TE,
        glosis_cl:majorLandFormValueCode-TH,
        glosis_cl:majorLandFormValueCode-TM,
        glosis_cl:majorLandFormValueCode-TV ;
    skos:notation "T" ;
    skos:prefLabel "steep land"@en ;
    skos:topConceptOf glosis_cl:majorLandFormValueCode .

glosis_cl:majorLandFormValueCode-TE a glosis_cl:MajorLandFormValueCode,
        skos:Concept ;
    skos:broader glosis_cl:majorLandFormValueCode-T ;
    skos:definition "first level of landform is steep land (T) and the second level is high-gradient escarpment zone (TE)" ;
    skos:inScheme glosis_cl:majorLandFormValueCode ;
    skos:notation "TE" ;
    skos:prefLabel "high-gradient escarpment zone"@en .

glosis_cl:majorLandFormValueCode-TH a glosis_cl:MajorLandFormValueCode,
        skos:Concept ;
    skos:broader glosis_cl:majorLandFormValueCode-T ;
    skos:definition "first level of landform is steep land (T) and the second level is high gradient hill (TH)" ;
    skos:inScheme glosis_cl:majorLandFormValueCode ;
    skos:notation "TH" ;
    skos:prefLabel "high-gradient hill"@en .

glosis_cl:majorLandFormValueCode-TM a glosis_cl:MajorLandFormValueCode,
        skos:Concept ;
    skos:broader glosis_cl:majorLandFormValueCode-T ;
    skos:definition "first level of landform is steep land (T) and the second level is high-gradient mountain (TM)" ;
    skos:inScheme glosis_cl:majorLandFormValueCode ;
    skos:notation "TM" ;
    skos:prefLabel "high-gradient mountain"@en .

glosis_cl:majorLandFormValueCode-TV a glosis_cl:MajorLandFormValueCode,
        skos:Concept ;
    skos:broader glosis_cl:majorLandFormValueCode-T ;
    skos:definition "first level of landform is steep land (T) and the second level is high gradient valley (TV)" ;
    skos:inScheme glosis_cl:majorLandFormValueCode ;
    skos:notation "TV" ;
    skos:prefLabel "high-gradient valley"@en .

glosis_cl:mineralConcColourValueCode-BB a glosis_cl:MineralConcColourValueCode,
        skos:Concept ;
    skos:definition "Mineral concentration of color code Bluish-black" ;
    skos:inScheme glosis_cl:mineralConcColourValueCode ;
    skos:notation "BB" ;
    skos:prefLabel "Bluish-black"@en ;
    skos:topConceptOf glosis_cl:mineralConcColourValueCode .

glosis_cl:mineralConcColourValueCode-BL a glosis_cl:MineralConcColourValueCode,
        skos:Concept ;
    skos:definition "Mineral concentration of color code Black" ;
    skos:inScheme glosis_cl:mineralConcColourValueCode ;
    skos:notation "BL" ;
    skos:prefLabel "Black"@en ;
    skos:topConceptOf glosis_cl:mineralConcColourValueCode .

glosis_cl:mineralConcColourValueCode-BR a glosis_cl:MineralConcColourValueCode,
        skos:Concept ;
    skos:definition "Mineral concentration of color code Brown" ;
    skos:inScheme glosis_cl:mineralConcColourValueCode ;
    skos:notation "BR" ;
    skos:prefLabel "Brown"@en ;
    skos:topConceptOf glosis_cl:mineralConcColourValueCode .

glosis_cl:mineralConcColourValueCode-BS a glosis_cl:MineralConcColourValueCode,
        skos:Concept ;
    skos:definition "Mineral concentration of color code Brownish" ;
    skos:inScheme glosis_cl:mineralConcColourValueCode ;
    skos:notation "BS" ;
    skos:prefLabel "Brownish"@en ;
    skos:topConceptOf glosis_cl:mineralConcColourValueCode .

glosis_cl:mineralConcColourValueCode-BU a glosis_cl:MineralConcColourValueCode,
        skos:Concept ;
    skos:definition "Mineral concentration of color code Blue" ;
    skos:inScheme glosis_cl:mineralConcColourValueCode ;
    skos:notation "BU" ;
    skos:prefLabel "Blue"@en ;
    skos:topConceptOf glosis_cl:mineralConcColourValueCode .

glosis_cl:mineralConcColourValueCode-GE a glosis_cl:MineralConcColourValueCode,
        skos:Concept ;
    skos:definition "Mineral concentration of color code Greenish" ;
    skos:inScheme glosis_cl:mineralConcColourValueCode ;
    skos:notation "GE" ;
    skos:prefLabel "Greenish"@en ;
    skos:topConceptOf glosis_cl:mineralConcColourValueCode .

glosis_cl:mineralConcColourValueCode-GR a glosis_cl:MineralConcColourValueCode,
        skos:Concept ;
    skos:definition "Mineral concentration of color code Grey" ;
    skos:inScheme glosis_cl:mineralConcColourValueCode ;
    skos:notation "GR" ;
    skos:prefLabel "Grey"@en ;
    skos:topConceptOf glosis_cl:mineralConcColourValueCode .

glosis_cl:mineralConcColourValueCode-GS a glosis_cl:MineralConcColourValueCode,
        skos:Concept ;
    skos:definition "Mineral concentration of color code Greyish" ;
    skos:inScheme glosis_cl:mineralConcColourValueCode ;
    skos:notation "GS" ;
    skos:prefLabel "Greyish"@en ;
    skos:topConceptOf glosis_cl:mineralConcColourValueCode .

glosis_cl:mineralConcColourValueCode-MC a glosis_cl:MineralConcColourValueCode,
        skos:Concept ;
    skos:definition "Mineral concentration of color code Multicoloured" ;
    skos:inScheme glosis_cl:mineralConcColourValueCode ;
    skos:notation "MC" ;
    skos:prefLabel "Multicoloured"@en ;
    skos:topConceptOf glosis_cl:mineralConcColourValueCode .

glosis_cl:mineralConcColourValueCode-RB a glosis_cl:MineralConcColourValueCode,
        skos:Concept ;
    skos:definition "Mineral concentration of color code Reddish brown" ;
    skos:inScheme glosis_cl:mineralConcColourValueCode ;
    skos:notation "RB" ;
    skos:prefLabel "Reddish brown"@en ;
    skos:topConceptOf glosis_cl:mineralConcColourValueCode .

glosis_cl:mineralConcColourValueCode-RE a glosis_cl:MineralConcColourValueCode,
        skos:Concept ;
    skos:definition "Mineral concentration of color code Red" ;
    skos:inScheme glosis_cl:mineralConcColourValueCode ;
    skos:notation "RE" ;
    skos:prefLabel "Red"@en ;
    skos:topConceptOf glosis_cl:mineralConcColourValueCode .

glosis_cl:mineralConcColourValueCode-RS a glosis_cl:MineralConcColourValueCode,
        skos:Concept ;
    skos:definition "Mineral concentration of color code Reddish" ;
    skos:inScheme glosis_cl:mineralConcColourValueCode ;
    skos:notation "RS" ;
    skos:prefLabel "Reddish"@en ;
    skos:topConceptOf glosis_cl:mineralConcColourValueCode .

glosis_cl:mineralConcColourValueCode-RY a glosis_cl:MineralConcColourValueCode,
        skos:Concept ;
    skos:definition "Mineral concentration of color code Reddish yellow" ;
    skos:inScheme glosis_cl:mineralConcColourValueCode ;
    skos:notation "RY" ;
    skos:prefLabel "Reddish yellow"@en ;
    skos:topConceptOf glosis_cl:mineralConcColourValueCode .

glosis_cl:mineralConcColourValueCode-WH a glosis_cl:MineralConcColourValueCode,
        skos:Concept ;
    skos:definition "Mineral concentration of color code White" ;
    skos:inScheme glosis_cl:mineralConcColourValueCode ;
    skos:notation "WH" ;
    skos:prefLabel "White"@en ;
    skos:topConceptOf glosis_cl:mineralConcColourValueCode .

glosis_cl:mineralConcColourValueCode-YB a glosis_cl:MineralConcColourValueCode,
        skos:Concept ;
    skos:definition "Mineral concentration of color code Yellowish brown" ;
    skos:inScheme glosis_cl:mineralConcColourValueCode ;
    skos:notation "YB" ;
    skos:prefLabel "Yellowish brown"@en ;
    skos:topConceptOf glosis_cl:mineralConcColourValueCode .

glosis_cl:mineralConcColourValueCode-YE a glosis_cl:MineralConcColourValueCode,
        skos:Concept ;
    skos:definition "Mineral concentration of color code Yellow" ;
    skos:inScheme glosis_cl:mineralConcColourValueCode ;
    skos:notation "YE" ;
    skos:prefLabel "Yellow"@en ;
    skos:topConceptOf glosis_cl:mineralConcColourValueCode .

glosis_cl:mineralConcColourValueCode-YR a glosis_cl:MineralConcColourValueCode,
        skos:Concept ;
    skos:definition "Mineral concentration of color code Yellowish red" ;
    skos:inScheme glosis_cl:mineralConcColourValueCode ;
    skos:notation "YR" ;
    skos:prefLabel "Yellowish red"@en ;
    skos:topConceptOf glosis_cl:mineralConcColourValueCode .

glosis_cl:mineralConcHardnessValueCode-B a glosis_cl:MineralConcHardnessValueCode,
        skos:Concept ;
    skos:definition "Both hard and soft." ;
    skos:inScheme glosis_cl:mineralConcHardnessValueCode ;
    skos:notation "B" ;
    skos:prefLabel "Both hard and soft."@en ;
    skos:topConceptOf glosis_cl:mineralConcHardnessValueCode .

glosis_cl:mineralConcHardnessValueCode-H a glosis_cl:MineralConcHardnessValueCode,
        skos:Concept ;
    skos:definition "Cannot be broken in the fingers." ;
    skos:inScheme glosis_cl:mineralConcHardnessValueCode ;
    skos:notation "H" ;
    skos:prefLabel "Hard"@en ;
    skos:topConceptOf glosis_cl:mineralConcHardnessValueCode .

glosis_cl:mineralConcHardnessValueCode-S a glosis_cl:MineralConcHardnessValueCode,
        skos:Concept ;
    skos:definition "Can be broken between forefinger and thumb nail" ;
    skos:inScheme glosis_cl:mineralConcHardnessValueCode ;
    skos:notation "S" ;
    skos:prefLabel "Soft"@en ;
    skos:topConceptOf glosis_cl:mineralConcHardnessValueCode .

glosis_cl:mineralConcKindValueCode-C a glosis_cl:MineralConcKindValueCode,
        skos:Concept ;
    skos:definition "A discrete body with a concentric internal structure, generally cemented." ;
    skos:inScheme glosis_cl:mineralConcKindValueCode ;
    skos:notation "C" ;
    skos:prefLabel "Concretion"@en ;
    skos:topConceptOf glosis_cl:mineralConcKindValueCode .

glosis_cl:mineralConcKindValueCode-IC a glosis_cl:MineralConcKindValueCode,
        skos:Concept ;
    skos:definition "Crack infillings refer to the materials that accumulate within cracks or fissures in the soil, typically formed due to drying or other physical stresses on the soil structure. These materials can include clays, silt, sand, or mineral deposits that enter cracks over time, often through the action of water or wind. Crack infillings can influence the soil's physical properties, such as its permeability and structure, as they may either facilitate or impede the movement of water and air through the soil. Additionally, crack infillings can impact soil fertility, as they may contain higher concentrations of certain nutrients or minerals that accumulate in these voids. Source: Soil Science Society of America." ;
    skos:inScheme glosis_cl:mineralConcKindValueCode ;
    skos:notation "IC" ;
    skos:prefLabel "Crack infillings"@en ;
    skos:topConceptOf glosis_cl:mineralConcKindValueCode .

glosis_cl:mineralConcKindValueCode-IP a glosis_cl:MineralConcKindValueCode,
        skos:Concept ;
    skos:definition "Including pseudomycelium of carbonates or opal." ;
    skos:inScheme glosis_cl:mineralConcKindValueCode ;
    skos:notation "IP" ;
    skos:prefLabel "Pore infillings"@en ;
    skos:topConceptOf glosis_cl:mineralConcKindValueCode .

glosis_cl:mineralConcKindValueCode-N a glosis_cl:MineralConcKindValueCode,
        skos:Concept ;
    skos:definition "Discrete body without an internal organization." ;
    skos:inScheme glosis_cl:mineralConcKindValueCode ;
    skos:notation "N" ;
    skos:prefLabel "Nodule"@en ;
    skos:topConceptOf glosis_cl:mineralConcKindValueCode .

glosis_cl:mineralConcKindValueCode-O a glosis_cl:MineralConcKindValueCode,
        skos:Concept ;
    skos:definition "The term Other in the context of soil mineral concentrations generally refers to any minerals or materials found in the soil that do not fall under commonly categorized types such as clay, silt, or sand. This could include uncommon minerals, organic matter, or anthropogenic substances that are present in the soil but don't fit into the standard classifications of soil texture or composition. These other substances may have a significant effect on soil properties, influencing aspects like nutrient availability, soil pH, and the ability to retain water. In many cases, Other minerals are identified through advanced soil testing and chemical analysis. Source: Soil Science Society of America." ;
    skos:inScheme glosis_cl:mineralConcKindValueCode ;
    skos:notation "O" ;
    skos:prefLabel "Other"@en ;
    skos:topConceptOf glosis_cl:mineralConcKindValueCode .

glosis_cl:mineralConcKindValueCode-R a glosis_cl:MineralConcKindValueCode,
        skos:Concept ;
    skos:definition "Discrete impregnated body still showing rock structure." ;
    skos:inScheme glosis_cl:mineralConcKindValueCode ;
    skos:notation "R" ;
    skos:prefLabel "Residual rock fragment"@en ;
    skos:topConceptOf glosis_cl:mineralConcKindValueCode .

glosis_cl:mineralConcKindValueCode-S a glosis_cl:MineralConcKindValueCode,
        skos:Concept ;
    skos:definition "Differs from the surrounding soil mass in colour and composition but is not easily separated as a discrete body." ;
    skos:inScheme glosis_cl:mineralConcKindValueCode ;
    skos:notation "S" ;
    skos:prefLabel "Soft segregation (or soft accumulation)"@en ;
    skos:topConceptOf glosis_cl:mineralConcKindValueCode .

glosis_cl:mineralConcKindValueCode-SC a glosis_cl:MineralConcKindValueCode,
        skos:Concept ;
    skos:definition "Soft concretion" ;
    skos:inScheme glosis_cl:mineralConcKindValueCode ;
    skos:notation "SC" ;
    skos:prefLabel "Soft concretion"@en ;
    skos:topConceptOf glosis_cl:mineralConcKindValueCode .

glosis_cl:mineralConcKindValueCode-T a glosis_cl:MineralConcKindValueCode,
        skos:Concept ;
    skos:definition "Crystals in soil refer to solid, naturally occurring minerals that have a regular and repeating internal structure, which can often be seen under a microscope or with the naked eye. These crystal formations typically occur when minerals precipitate from water or melt and re-crystallize under certain environmental conditions, such as changes in temperature or pressure. Common crystal minerals in soil include quartz, gypsum, calcite, and halite. The presence of crystals in soil can significantly affect its properties, including drainage, fertility, and nutrient availability. For example, gypsum crystals can improve soil structure, while the presence of salt crystals can lead to soil salinity problems. Source: Brady & Weil (2017), The Nature and Properties of Soils." ;
    skos:inScheme glosis_cl:mineralConcKindValueCode ;
    skos:notation "T" ;
    skos:prefLabel "Crystal"@en ;
    skos:topConceptOf glosis_cl:mineralConcKindValueCode .

glosis_cl:mineralConcNatureValueCode-C a glosis_cl:MineralConcNatureValueCode,
        skos:Concept ;
    skos:definition "Nature of mineral concentration with Clay (argillaceous)" ;
    skos:inScheme glosis_cl:mineralConcNatureValueCode ;
    skos:notation "C" ;
    skos:prefLabel "Clay (argillaceous)"@en ;
    skos:topConceptOf glosis_cl:mineralConcNatureValueCode .

glosis_cl:mineralConcNatureValueCode-CS a glosis_cl:MineralConcNatureValueCode,
        skos:Concept ;
    skos:definition "Nature of mineral concentration with Clay–sesquioxides" ;
    skos:inScheme glosis_cl:mineralConcNatureValueCode ;
    skos:notation "CS" ;
    skos:prefLabel "Clay–sesquioxides"@en ;
    skos:topConceptOf glosis_cl:mineralConcNatureValueCode .

glosis_cl:mineralConcNatureValueCode-F a glosis_cl:MineralConcNatureValueCode,
        skos:Concept ;
    skos:definition "Nature of mineral concentration with Iron (ferruginous)" ;
    skos:inScheme glosis_cl:mineralConcNatureValueCode ;
    skos:notation "F" ;
    skos:prefLabel "Iron (ferruginous)"@en ;
    skos:topConceptOf glosis_cl:mineralConcNatureValueCode .

glosis_cl:mineralConcNatureValueCode-FM a glosis_cl:MineralConcNatureValueCode,
        skos:Concept ;
    skos:definition "Nature of mineral concentration with Iron–manganese (sesquioxides)" ;
    skos:inScheme glosis_cl:mineralConcNatureValueCode ;
    skos:notation "FM" ;
    skos:prefLabel "Iron–manganese (sesquioxides)"@en ;
    skos:topConceptOf glosis_cl:mineralConcNatureValueCode .

glosis_cl:mineralConcNatureValueCode-GB a glosis_cl:MineralConcNatureValueCode,
        skos:Concept ;
    skos:definition "Nature of mineral concentration with Gibbsite" ;
    skos:inScheme glosis_cl:mineralConcNatureValueCode ;
    skos:notation "GB" ;
    skos:prefLabel "Gibbsite"@en ;
    skos:topConceptOf glosis_cl:mineralConcNatureValueCode .

glosis_cl:mineralConcNatureValueCode-GY a glosis_cl:MineralConcNatureValueCode,
        skos:Concept ;
    skos:definition "Nature of mineral concentration with Gypsum (gypsiferous)" ;
    skos:inScheme glosis_cl:mineralConcNatureValueCode ;
    skos:notation "GY" ;
    skos:prefLabel "Gypsum (gypsiferous)"@en ;
    skos:topConceptOf glosis_cl:mineralConcNatureValueCode .

glosis_cl:mineralConcNatureValueCode-JA a glosis_cl:MineralConcNatureValueCode,
        skos:Concept ;
    skos:definition "Nature of mineral concentration with Jarosite" ;
    skos:inScheme glosis_cl:mineralConcNatureValueCode ;
    skos:notation "JA" ;
    skos:prefLabel "Jarosite"@en ;
    skos:topConceptOf glosis_cl:mineralConcNatureValueCode .

glosis_cl:mineralConcNatureValueCode-K a glosis_cl:MineralConcNatureValueCode,
        skos:Concept ;
    skos:definition "Nature of mineral concentration with Carbonates (calcareous)" ;
    skos:inScheme glosis_cl:mineralConcNatureValueCode ;
    skos:notation "K" ;
    skos:prefLabel "Carbonates (calcareous)"@en ;
    skos:topConceptOf glosis_cl:mineralConcNatureValueCode .

glosis_cl:mineralConcNatureValueCode-KQ a glosis_cl:MineralConcNatureValueCode,
        skos:Concept ;
    skos:definition "Nature of mineral concentration with Carbonates–silica" ;
    skos:inScheme glosis_cl:mineralConcNatureValueCode ;
    skos:notation "KQ" ;
    skos:prefLabel "Carbonates–silica"@en ;
    skos:topConceptOf glosis_cl:mineralConcNatureValueCode .

glosis_cl:mineralConcNatureValueCode-M a glosis_cl:MineralConcNatureValueCode,
        skos:Concept ;
    skos:definition "Nature of mineral concentration with Manganese (manganiferous)" ;
    skos:inScheme glosis_cl:mineralConcNatureValueCode ;
    skos:notation "M" ;
    skos:prefLabel "Manganese (manganiferous)"@en ;
    skos:topConceptOf glosis_cl:mineralConcNatureValueCode .

glosis_cl:mineralConcNatureValueCode-NK a glosis_cl:MineralConcNatureValueCode,
        skos:Concept ;
    skos:definition "Nature of mineral concentration with unknown substances" ;
    skos:inScheme glosis_cl:mineralConcNatureValueCode ;
    skos:notation "NK" ;
    skos:prefLabel "Not known"@en ;
    skos:topConceptOf glosis_cl:mineralConcNatureValueCode .

glosis_cl:mineralConcNatureValueCode-Q a glosis_cl:MineralConcNatureValueCode,
        skos:Concept ;
    skos:definition "Nature of mineral concentration with Silica (siliceous)" ;
    skos:inScheme glosis_cl:mineralConcNatureValueCode ;
    skos:notation "Q" ;
    skos:prefLabel "Silica (siliceous)"@en ;
    skos:topConceptOf glosis_cl:mineralConcNatureValueCode .

glosis_cl:mineralConcNatureValueCode-S a glosis_cl:MineralConcNatureValueCode,
        skos:Concept ;
    skos:definition "Nature of mineral concentration with Sulphur (sulphurous)" ;
    skos:inScheme glosis_cl:mineralConcNatureValueCode ;
    skos:notation "S" ;
    skos:prefLabel "Sulphur (sulphurous)"@en ;
    skos:topConceptOf glosis_cl:mineralConcNatureValueCode .

glosis_cl:mineralConcNatureValueCode-SA a glosis_cl:MineralConcNatureValueCode,
        skos:Concept ;
    skos:definition "Nature of mineral concentration with Salt (saline)" ;
    skos:inScheme glosis_cl:mineralConcNatureValueCode ;
    skos:notation "SA" ;
    skos:prefLabel "Salt (saline)"@en ;
    skos:topConceptOf glosis_cl:mineralConcNatureValueCode .

glosis_cl:mineralConcShapeValueCode-A a glosis_cl:MineralConcShapeValueCode,
        skos:Concept ;
    skos:definition "Angular shape of mineral concentrations" ;
    skos:inScheme glosis_cl:mineralConcShapeValueCode ;
    skos:notation "A" ;
    skos:prefLabel "Angular"@en ;
    skos:topConceptOf glosis_cl:mineralConcShapeValueCode .

glosis_cl:mineralConcShapeValueCode-E a glosis_cl:MineralConcShapeValueCode,
        skos:Concept ;
    skos:definition "Elongated shape of mineral concentrations" ;
    skos:inScheme glosis_cl:mineralConcShapeValueCode ;
    skos:notation "E" ;
    skos:prefLabel "Elongated"@en ;
    skos:topConceptOf glosis_cl:mineralConcShapeValueCode .

glosis_cl:mineralConcShapeValueCode-F a glosis_cl:MineralConcShapeValueCode,
        skos:Concept ;
    skos:definition "Flat shape of mineral concentrations" ;
    skos:inScheme glosis_cl:mineralConcShapeValueCode ;
    skos:notation "F" ;
    skos:prefLabel "Flat"@en ;
    skos:topConceptOf glosis_cl:mineralConcShapeValueCode .

glosis_cl:mineralConcShapeValueCode-I a glosis_cl:MineralConcShapeValueCode,
        skos:Concept ;
    skos:definition "Irregular shape of mineral concentrations" ;
    skos:inScheme glosis_cl:mineralConcShapeValueCode ;
    skos:notation "I" ;
    skos:prefLabel "Irregular"@en ;
    skos:topConceptOf glosis_cl:mineralConcShapeValueCode .

glosis_cl:mineralConcShapeValueCode-R a glosis_cl:MineralConcShapeValueCode,
        skos:Concept ;
    skos:definition "Rounded (spherical) shape of mineral concentrations" ;
    skos:inScheme glosis_cl:mineralConcShapeValueCode ;
    skos:notation "R" ;
    skos:prefLabel "Rounded (spherical)"@en ;
    skos:topConceptOf glosis_cl:mineralConcShapeValueCode .

glosis_cl:mineralConcSizeValueCode-C a glosis_cl:MineralConcSizeValueCode,
        skos:Concept ;
    skos:definition "Mineral concentration ranging fron size of  > 20mm" ;
    skos:inScheme glosis_cl:mineralConcSizeValueCode ;
    skos:notation "C" ;
    skos:prefLabel "Coarse"@en ;
    skos:topConceptOf glosis_cl:mineralConcSizeValueCode .

glosis_cl:mineralConcSizeValueCode-F a glosis_cl:MineralConcSizeValueCode,
        skos:Concept ;
    skos:definition "Mineral concentration ranging fron size of 2mm–6mm" ;
    skos:inScheme glosis_cl:mineralConcSizeValueCode ;
    skos:notation "F" ;
    skos:prefLabel "Fine"@en ;
    skos:topConceptOf glosis_cl:mineralConcSizeValueCode .

glosis_cl:mineralConcSizeValueCode-M a glosis_cl:MineralConcSizeValueCode,
        skos:Concept ;
    skos:definition "Mineral concentration ranging fron size of 6mm–20mm" ;
    skos:inScheme glosis_cl:mineralConcSizeValueCode ;
    skos:notation "M" ;
    skos:prefLabel "Medium"@en ;
    skos:topConceptOf glosis_cl:mineralConcSizeValueCode .

glosis_cl:mineralConcSizeValueCode-V a glosis_cl:MineralConcSizeValueCode,
        skos:Concept ;
    skos:definition "Mineral concentration ranging fron size of < 2mm" ;
    skos:inScheme glosis_cl:mineralConcSizeValueCode ;
    skos:notation "V" ;
    skos:prefLabel "Very fine"@en ;
    skos:topConceptOf glosis_cl:mineralConcSizeValueCode .

glosis_cl:mineralConcVolumeValueCode-A a glosis_cl:MineralConcVolumeValueCode,
        skos:Concept ;
    skos:definition "Having mineral concentarion volume of 40–80%" ;
    skos:inScheme glosis_cl:mineralConcVolumeValueCode ;
    skos:notation "A" ;
    skos:prefLabel "Abundant"@en ;
    skos:topConceptOf glosis_cl:mineralConcVolumeValueCode .

glosis_cl:mineralConcVolumeValueCode-C a glosis_cl:MineralConcVolumeValueCode,
        skos:Concept ;
    skos:definition "Having mineral concentarion volume of 5–15%" ;
    skos:inScheme glosis_cl:mineralConcVolumeValueCode ;
    skos:notation "C" ;
    skos:prefLabel "Common"@en ;
    skos:topConceptOf glosis_cl:mineralConcVolumeValueCode .

glosis_cl:mineralConcVolumeValueCode-D a glosis_cl:MineralConcVolumeValueCode,
        skos:Concept ;
    skos:definition "Having mineral concentarion volume of more than 80%" ;
    skos:inScheme glosis_cl:mineralConcVolumeValueCode ;
    skos:notation "D" ;
    skos:prefLabel "Dominant"@en ;
    skos:topConceptOf glosis_cl:mineralConcVolumeValueCode .

glosis_cl:mineralConcVolumeValueCode-F a glosis_cl:MineralConcVolumeValueCode,
        skos:Concept ;
    skos:definition "Having mineral concentarion volume of 2–5%" ;
    skos:inScheme glosis_cl:mineralConcVolumeValueCode ;
    skos:notation "F" ;
    skos:prefLabel "Few"@en ;
    skos:topConceptOf glosis_cl:mineralConcVolumeValueCode .

glosis_cl:mineralConcVolumeValueCode-M a glosis_cl:MineralConcVolumeValueCode,
        skos:Concept ;
    skos:definition "Having mineral concentarion volume of 15–40%" ;
    skos:inScheme glosis_cl:mineralConcVolumeValueCode ;
    skos:notation "M" ;
    skos:prefLabel "Many"@en ;
    skos:topConceptOf glosis_cl:mineralConcVolumeValueCode .

glosis_cl:mineralConcVolumeValueCode-N a glosis_cl:MineralConcVolumeValueCode,
        skos:Concept ;
    skos:definition "Having 0 mineral concentarion volume" ;
    skos:inScheme glosis_cl:mineralConcVolumeValueCode ;
    skos:notation "N" ;
    skos:prefLabel "None"@en ;
    skos:topConceptOf glosis_cl:mineralConcVolumeValueCode .

glosis_cl:mineralConcVolumeValueCode-V a glosis_cl:MineralConcVolumeValueCode,
        skos:Concept ;
    skos:definition "Having mineral concentarion volume of 0–2%" ;
    skos:inScheme glosis_cl:mineralConcVolumeValueCode ;
    skos:notation "V" ;
    skos:prefLabel "Very few"@en ;
    skos:topConceptOf glosis_cl:mineralConcVolumeValueCode .

glosis_cl:mineralFragmentsValueCode-FE a glosis_cl:MineralFragmentsValueCode,
        skos:Concept ;
    skos:definition "Rocks with primary mineral containing Feldspar" ;
    skos:inScheme glosis_cl:mineralFragmentsValueCode ;
    skos:notation "FE" ;
    skos:prefLabel "Feldspar"@en ;
    skos:topConceptOf glosis_cl:mineralFragmentsValueCode .

glosis_cl:mineralFragmentsValueCode-MI a glosis_cl:MineralFragmentsValueCode,
        skos:Concept ;
    skos:definition "Rocks with primary mineral containing Mica" ;
    skos:inScheme glosis_cl:mineralFragmentsValueCode ;
    skos:notation "MI" ;
    skos:prefLabel "Mica"@en ;
    skos:topConceptOf glosis_cl:mineralFragmentsValueCode .

glosis_cl:mineralFragmentsValueCode-QU a glosis_cl:MineralFragmentsValueCode,
        skos:Concept ;
    skos:definition "Rocks with primary mineral containing Quartz" ;
    skos:inScheme glosis_cl:mineralFragmentsValueCode ;
    skos:notation "QU" ;
    skos:prefLabel "Quartz"@en ;
    skos:topConceptOf glosis_cl:mineralFragmentsValueCode .

glosis_cl:mottlesAbundanceValueCode-A a glosis_cl:MottlesAbundanceValueCode,
        skos:Concept ;
    skos:definition "The muttle abundance is more than 40%" ;
    skos:inScheme glosis_cl:mottlesAbundanceValueCode ;
    skos:notation "A" ;
    skos:prefLabel "Abundant"@en ;
    skos:topConceptOf glosis_cl:mottlesAbundanceValueCode .

glosis_cl:mottlesAbundanceValueCode-C a glosis_cl:MottlesAbundanceValueCode,
        skos:Concept ;
    skos:definition "Commonly found muttle abundance of 5–15%" ;
    skos:inScheme glosis_cl:mottlesAbundanceValueCode ;
    skos:notation "C" ;
    skos:prefLabel "Common"@en ;
    skos:topConceptOf glosis_cl:mottlesAbundanceValueCode .

glosis_cl:mottlesAbundanceValueCode-F a glosis_cl:MottlesAbundanceValueCode,
        skos:Concept ;
    skos:definition "Fewer muttle abundace with 2–5 %" ;
    skos:inScheme glosis_cl:mottlesAbundanceValueCode ;
    skos:notation "F" ;
    skos:prefLabel "Few"@en ;
    skos:topConceptOf glosis_cl:mottlesAbundanceValueCode .

glosis_cl:mottlesAbundanceValueCode-M a glosis_cl:MottlesAbundanceValueCode,
        skos:Concept ;
    skos:definition "Muttle abundance of 15–40%" ;
    skos:inScheme glosis_cl:mottlesAbundanceValueCode ;
    skos:notation "M" ;
    skos:prefLabel "Many"@en ;
    skos:topConceptOf glosis_cl:mottlesAbundanceValueCode .

glosis_cl:mottlesAbundanceValueCode-N a glosis_cl:MottlesAbundanceValueCode,
        skos:Concept ;
    skos:definition "The muttle abundance is zero" ;
    skos:inScheme glosis_cl:mottlesAbundanceValueCode ;
    skos:notation "N" ;
    skos:prefLabel "None"@en ;
    skos:topConceptOf glosis_cl:mottlesAbundanceValueCode .

glosis_cl:mottlesAbundanceValueCode-V a glosis_cl:MottlesAbundanceValueCode,
        skos:Concept ;
    skos:definition "Very few muttle abundace of 0–2 %" ;
    skos:inScheme glosis_cl:mottlesAbundanceValueCode ;
    skos:notation "V" ;
    skos:prefLabel "Very few"@en ;
    skos:topConceptOf glosis_cl:mottlesAbundanceValueCode .

glosis_cl:mottlesSizeValueCode-A a glosis_cl:MottlesSizeValueCode,
        skos:Concept ;
    skos:definition "Coarse mottle of > 20" ;
    skos:inScheme glosis_cl:mottlesSizeValueCode ;
    skos:notation "A" ;
    skos:prefLabel "Coarse"@en ;
    skos:topConceptOf glosis_cl:mottlesSizeValueCode .

glosis_cl:mottlesSizeValueCode-F a glosis_cl:MottlesSizeValueCode,
        skos:Concept ;
    skos:definition "Fine mottle of size 2–6" ;
    skos:inScheme glosis_cl:mottlesSizeValueCode ;
    skos:notation "F" ;
    skos:prefLabel "F Fine"@en ;
    skos:topConceptOf glosis_cl:mottlesSizeValueCode .

glosis_cl:mottlesSizeValueCode-M a glosis_cl:MottlesSizeValueCode,
        skos:Concept ;
    skos:definition "Medium mottle of size 6–20" ;
    skos:inScheme glosis_cl:mottlesSizeValueCode ;
    skos:notation "M" ;
    skos:prefLabel "M Medium"@en ;
    skos:topConceptOf glosis_cl:mottlesSizeValueCode .

glosis_cl:mottlesSizeValueCode-V a glosis_cl:MottlesSizeValueCode,
        skos:Concept ;
    skos:definition "Very fine mottle size of less than  2" ;
    skos:inScheme glosis_cl:mottlesSizeValueCode ;
    skos:notation "V" ;
    skos:prefLabel "Very fine"@en ;
    skos:topConceptOf glosis_cl:mottlesSizeValueCode .

glosis_cl:peatDecompostionValueCode-D1 a glosis_cl:PeatDecompostionValueCode,
        skos:Concept ;
    skos:broader glosis_cl:peatDecompostionValueCode-Fibric ;
    skos:definition "Subtype Fibric and the degree of decomposition and humification of peat is very low" ;
    skos:inScheme glosis_cl:peatDecompostionValueCode ;
    skos:notation "D1" ;
    skos:prefLabel "very low"@en .

glosis_cl:peatDecompostionValueCode-D2 a glosis_cl:PeatDecompostionValueCode,
        skos:Concept ;
    skos:broader glosis_cl:peatDecompostionValueCode-Fibric ;
    skos:definition "Subtype Fibric and the degree of decomposition and humification of peat is low" ;
    skos:inScheme glosis_cl:peatDecompostionValueCode ;
    skos:notation "D2" ;
    skos:prefLabel "low"@en .

glosis_cl:peatDecompostionValueCode-D3 a glosis_cl:PeatDecompostionValueCode,
        skos:Concept ;
    skos:broader glosis_cl:peatDecompostionValueCode-Fibric ;
    skos:definition "Subtype Fibric and the degree of decomposition and humification of peat is moderate" ;
    skos:inScheme glosis_cl:peatDecompostionValueCode ;
    skos:notation "D3" ;
    skos:prefLabel "moderate"@en .

glosis_cl:peatDecompostionValueCode-D4 a glosis_cl:PeatDecompostionValueCode,
        skos:Concept ;
    skos:broader glosis_cl:peatDecompostionValueCode-Hemic ;
    skos:definition "Subtype Hemic and the degree of decomposition and humification of peat is strong" ;
    skos:inScheme glosis_cl:peatDecompostionValueCode ;
    skos:notation "D4" ;
    skos:prefLabel "strong"@en .

glosis_cl:peatDecompostionValueCode-D5.1 a glosis_cl:PeatDecompostionValueCode,
        skos:Concept ;
    skos:broader glosis_cl:peatDecompostionValueCode-Hemic ;
    skos:definition "Subtype Hemic and the degree of decomposition and humification of peat is moderately strong" ;
    skos:inScheme glosis_cl:peatDecompostionValueCode ;
    skos:notation "D5.1" ;
    skos:prefLabel "moderately strong"@en .

glosis_cl:peatDecompostionValueCode-D5.2 a glosis_cl:PeatDecompostionValueCode,
        skos:Concept ;
    skos:broader glosis_cl:peatDecompostionValueCode-Sapric ;
    skos:definition "Subtype Sapric and the degree of decomposition and humification of peat is very strong" ;
    skos:inScheme glosis_cl:peatDecompostionValueCode ;
    skos:notation "D5.2" ;
    skos:prefLabel "very strong"@en .

glosis_cl:peatDecompostionValueCode-Fibric a glosis_cl:PeatDecompostionValueCode,
        skos:Concept ;
    skos:definition "Degree of decomposition and humification of peat of subtype Fibric" ;
    skos:inScheme glosis_cl:peatDecompostionValueCode ;
    skos:narrower glosis_cl:peatDecompostionValueCode-D1,
        glosis_cl:peatDecompostionValueCode-D2,
        glosis_cl:peatDecompostionValueCode-D3 ;
    skos:notation "Fibric" ;
    skos:prefLabel "Fibric"@en ;
    skos:topConceptOf glosis_cl:peatDecompostionValueCode .

glosis_cl:peatDecompostionValueCode-Hemic a glosis_cl:PeatDecompostionValueCode,
        skos:Concept ;
    skos:definition "Degree of decomposition and humification of peat of subtype Hemic" ;
    skos:inScheme glosis_cl:peatDecompostionValueCode ;
    skos:narrower glosis_cl:peatDecompostionValueCode-D4,
        glosis_cl:peatDecompostionValueCode-D5.1 ;
    skos:notation "Hemic" ;
    skos:prefLabel "Hemic"@en ;
    skos:topConceptOf glosis_cl:peatDecompostionValueCode .

glosis_cl:peatDecompostionValueCode-Sapric a glosis_cl:PeatDecompostionValueCode,
        skos:Concept ;
    skos:definition "Degree of decomposition and humification of peat of subtype Sapric" ;
    skos:inScheme glosis_cl:peatDecompostionValueCode ;
    skos:narrower glosis_cl:peatDecompostionValueCode-D5.2 ;
    skos:notation "Sapric" ;
    skos:prefLabel "Sapric"@en ;
    skos:topConceptOf glosis_cl:peatDecompostionValueCode .

glosis_cl:peatDrainageValueCode-DC1 a glosis_cl:PeatDrainageValueCode,
        skos:Concept ;
    skos:definition "Undrained peat material" ;
    skos:inScheme glosis_cl:peatDrainageValueCode ;
    skos:notation "DC1" ;
    skos:prefLabel "Undrained"@en ;
    skos:topConceptOf glosis_cl:peatDrainageValueCode .

glosis_cl:peatDrainageValueCode-DC2 a glosis_cl:PeatDrainageValueCode,
        skos:Concept ;
    skos:definition "Weakly drained peat material" ;
    skos:inScheme glosis_cl:peatDrainageValueCode ;
    skos:notation "DC2" ;
    skos:prefLabel "Weakly drained"@en ;
    skos:topConceptOf glosis_cl:peatDrainageValueCode .

glosis_cl:peatDrainageValueCode-DC3 a glosis_cl:PeatDrainageValueCode,
        skos:Concept ;
    skos:definition "Moderately drained peat material" ;
    skos:inScheme glosis_cl:peatDrainageValueCode ;
    skos:notation "DC3" ;
    skos:prefLabel "Moderately drained"@en ;
    skos:topConceptOf glosis_cl:peatDrainageValueCode .

glosis_cl:peatDrainageValueCode-DC4 a glosis_cl:PeatDrainageValueCode,
        skos:Concept ;
    skos:definition "Well drained peat material" ;
    skos:inScheme glosis_cl:peatDrainageValueCode ;
    skos:notation "DC4" ;
    skos:prefLabel "Well drained"@en ;
    skos:topConceptOf glosis_cl:peatDrainageValueCode .

glosis_cl:peatVolumeValueCode-SV1 a glosis_cl:PeatVolumeValueCode,
        skos:Concept ;
    skos:definition "Solid Volume of percentage less than 3%: < 3%" ;
    skos:inScheme glosis_cl:peatVolumeValueCode ;
    skos:notation "SV1" ;
    skos:prefLabel "Less than 3%"@en ;
    skos:topConceptOf glosis_cl:peatVolumeValueCode .

glosis_cl:peatVolumeValueCode-SV2 a glosis_cl:PeatVolumeValueCode,
        skos:Concept ;
    skos:definition "Solid Volume of percentage of 3 - 5 %" ;
    skos:inScheme glosis_cl:peatVolumeValueCode ;
    skos:notation "SV2" ;
    skos:prefLabel "Between 3% and 5%"@en ;
    skos:topConceptOf glosis_cl:peatVolumeValueCode .

glosis_cl:peatVolumeValueCode-SV3 a glosis_cl:PeatVolumeValueCode,
        skos:Concept ;
    skos:definition "Solid Volume of percentage of 5 - 8%" ;
    skos:inScheme glosis_cl:peatVolumeValueCode ;
    skos:notation "SV3" ;
    skos:prefLabel "Between 5% and 8%"@en ;
    skos:topConceptOf glosis_cl:peatVolumeValueCode .

glosis_cl:peatVolumeValueCode-SV4 a glosis_cl:PeatVolumeValueCode,
        skos:Concept ;
    skos:definition "Solid Volume of percentage of 8 to 12%" ;
    skos:inScheme glosis_cl:peatVolumeValueCode ;
    skos:notation "SV4" ;
    skos:prefLabel "Between 8% and 12%"@en ;
    skos:topConceptOf glosis_cl:peatVolumeValueCode .

glosis_cl:peatVolumeValueCode-SV5 a glosis_cl:PeatVolumeValueCode,
        skos:Concept ;
    skos:definition "Solid Volume of percentage more than or equal to 12 %: ≥ 12%" ;
    skos:inScheme glosis_cl:peatVolumeValueCode ;
    skos:notation "SV5" ;
    skos:prefLabel "More than or equal to 12 %"@en ;
    skos:topConceptOf glosis_cl:peatVolumeValueCode .

glosis_cl:physioChemicalPropertyCode-Aciexc a glosis_cl:PhysioChemicalPropertyCode,
        skos:Concept ;
    skos:definition "Exchangeable acidity represents the amount of hydrogen (H⁺) and aluminum (Al³⁺) ions adsorbed onto soil particles that can be exchanged with the soil solution. It is a key factor in determining soil liming requirements and improving nutrient availability in acidic soils. Source: Brady & Weil (2017)." ;
    skos:inScheme glosis_cl:physioChemicalPropertyCode ;
    skos:notation "Aciexc" ;
    skos:prefLabel "Acidity - exchangeable"@en ;
    skos:topConceptOf glosis_cl:physioChemicalPropertyCode .

glosis_cl:physioChemicalPropertyCode-Aciext a glosis_cl:PhysioChemicalPropertyCode,
        skos:Concept ;
    skos:definition "Extractable acidity measures the active acidity in soil, including hydrogen ions in the soil solution and weakly bound to colloids. It is critical for assessing lime requirements and addressing soil pH imbalances to improve plant growth. Source: Soil Chemistry by Bohn et al." ;
    skos:inScheme glosis_cl:physioChemicalPropertyCode ;
    skos:notation "Aciext" ;
    skos:prefLabel "Acidity - extractable"@en ;
    skos:topConceptOf glosis_cl:physioChemicalPropertyCode .

glosis_cl:physioChemicalPropertyCode-Alu a dbo:ChemicalCompound,
        dbo:ChemicalSubstance,
        glosis_cl:PhysioChemicalPropertyCode,
        skos:Concept ;
    dbo:inchi "1S/Al" ;
    dbo:pubchem "5359268" ;
    dbprop:inchikey "XAGFODPZIPBFFR-UHFFFAOYSA-N" ;
    rdfs:seeAlso <https://pubchem.ncbi.nlm.nih.gov/compound/5359268> ;
    skos:definition "Sum of the oxalate-extractable aluminium concentration plus half the oxalate-extractable iron concentration" ;
    skos:inScheme glosis_cl:physioChemicalPropertyCode ;
    skos:notation "Alu" ;
    skos:prefLabel "Aluminium (Al) + 0.5 Fe oxalate"@en ;
    skos:topConceptOf glosis_cl:physioChemicalPropertyCode .

glosis_cl:physioChemicalPropertyCode-Aludit a dbo:ChemicalCompound,
        dbo:ChemicalSubstance,
        glosis_cl:PhysioChemicalPropertyCode,
        skos:Concept ;
    dbo:inchi "1S/Al" ;
    dbo:pubchem "5359268" ;
    dbprop:inchikey "XAGFODPZIPBFFR-UHFFFAOYSA-N" ;
    rdfs:seeAlso <https://pubchem.ncbi.nlm.nih.gov/compound/5359268> ;
    skos:definition "'Free' aluminium content extracted from amorphous compounds (weathering products) as well as crystaline, primary aluminium compounds (parent material) in the soil." ;
    skos:inScheme glosis_cl:physioChemicalPropertyCode ;
    skos:notation "Aludit" ;
    skos:prefLabel "Aluminium (Al) - dithionite extractable"@en ;
    skos:topConceptOf glosis_cl:physioChemicalPropertyCode .

glosis_cl:physioChemicalPropertyCode-Aluexc a dbo:ChemicalCompound,
        dbo:ChemicalSubstance,
        glosis_cl:PhysioChemicalPropertyCode,
        skos:Concept ;
    dbo:inchi "1S/Al" ;
    dbo:pubchem "5359268" ;
    dbprop:inchikey "XAGFODPZIPBFFR-UHFFFAOYSA-N" ;
    rdfs:seeAlso <https://pubchem.ncbi.nlm.nih.gov/compound/5359268> ;
    skos:definition "Aluminium ions bound to exchange surfaces in the soil such as clay minerals and organic matter that can be released to the soil solution upon exchange" ;
    skos:inScheme glosis_cl:physioChemicalPropertyCode ;
    skos:notation "Aluexc" ;
    skos:prefLabel "Aluminium (Al) exchangeable"@en ;
    skos:topConceptOf glosis_cl:physioChemicalPropertyCode .

glosis_cl:physioChemicalPropertyCode-Aluext a dbo:ChemicalCompound,
        dbo:ChemicalSubstance,
        glosis_cl:PhysioChemicalPropertyCode,
        skos:Concept ;
    dbo:inchi "1S/Al" ;
    dbo:pubchem "5359268" ;
    dbprop:inchikey "XAGFODPZIPBFFR-UHFFFAOYSA-N" ;
    rdfs:seeAlso <https://pubchem.ncbi.nlm.nih.gov/compound/5359268> ;
    skos:definition "Aluminium bound to the soil matrix but that can be released into the soil solution (i.e. become bio-available)" ;
    skos:inScheme glosis_cl:physioChemicalPropertyCode ;
    skos:notation "Aluext" ;
    skos:prefLabel "Aluminium (Al) extractable"@en ;
    skos:topConceptOf glosis_cl:physioChemicalPropertyCode .

glosis_cl:physioChemicalPropertyCode-Aluoxa a dbo:ChemicalCompound,
        dbo:ChemicalSubstance,
        glosis_cl:PhysioChemicalPropertyCode,
        skos:Concept ;
    dbo:inchi "1S/Al" ;
    dbo:pubchem "5359268" ;
    dbprop:inchikey "XAGFODPZIPBFFR-UHFFFAOYSA-N" ;
    rdfs:seeAlso <https://pubchem.ncbi.nlm.nih.gov/compound/5359268> ;
    skos:definition "'Active' aluminium content extracted from amorphous aluminium compounds that are the products of the weathering of primary soil particles" ;
    skos:inScheme glosis_cl:physioChemicalPropertyCode ;
    skos:notation "Aluoxa" ;
    skos:prefLabel "Aluminium (Al) - oxalate extractable"@en ;
    skos:topConceptOf glosis_cl:physioChemicalPropertyCode .

glosis_cl:physioChemicalPropertyCode-Alupyr a dbo:ChemicalCompound,
        dbo:ChemicalSubstance,
        glosis_cl:PhysioChemicalPropertyCode,
        skos:Concept ;
    dbo:inchi "1S/Al" ;
    dbo:pubchem "5359268" ;
    dbprop:inchikey "XAGFODPZIPBFFR-UHFFFAOYSA-N" ;
    rdfs:seeAlso <https://pubchem.ncbi.nlm.nih.gov/compound/5359268> ;
    skos:definition "Aluminium in soil that is organically bound in organo-metal complexes" ;
    skos:inScheme glosis_cl:physioChemicalPropertyCode ;
    skos:notation "Alupyr" ;
    skos:prefLabel "Aluminium (Al) - pyrophosphate extractable"@en ;
    skos:topConceptOf glosis_cl:physioChemicalPropertyCode .

glosis_cl:physioChemicalPropertyCode-Alusat a dbo:ChemicalCompound,
        dbo:ChemicalSubstance,
        glosis_cl:PhysioChemicalPropertyCode,
        skos:Concept ;
    dbo:inchi "1S/Al" ;
    dbo:pubchem "5359268" ;
    dbprop:inchikey "XAGFODPZIPBFFR-UHFFFAOYSA-N" ;
    rdfs:seeAlso <https://pubchem.ncbi.nlm.nih.gov/compound/5359268> ;
    skos:definition "Measure to describe the relative abundance of alumium in the soil. It is the percentage of the CEC occupied by aluminium" ;
    skos:inScheme glosis_cl:physioChemicalPropertyCode ;
    skos:notation "Alusat" ;
    skos:prefLabel "Aluminium (Al) saturation"@en ;
    skos:topConceptOf glosis_cl:physioChemicalPropertyCode .

glosis_cl:physioChemicalPropertyCode-Alutot a dbo:ChemicalCompound,
        dbo:ChemicalSubstance,
        glosis_cl:PhysioChemicalPropertyCode,
        skos:Concept ;
    dbo:inchi "1S/Al" ;
    dbo:pubchem "5359268" ;
    dbprop:inchikey "XAGFODPZIPBFFR-UHFFFAOYSA-N" ;
    rdfs:seeAlso <https://pubchem.ncbi.nlm.nih.gov/compound/5359268> ;
    skos:definition "Total concentration of aluminium in the soil, including both soluble and insoluble forms, typically measured after complete digestion of the soil sample." ;
    skos:inScheme glosis_cl:physioChemicalPropertyCode ;
    skos:notation "Alutot" ;
    skos:prefLabel "Aluminium (Al) total"@en ;
    skos:topConceptOf glosis_cl:physioChemicalPropertyCode .

glosis_cl:physioChemicalPropertyCode-Avavol a glosis_cl:PhysioChemicalPropertyCode,
        skos:Concept ;
    skos:definition "Available water capacity (AWC) measures the volume of water soil can retain between field capacity and the permanent wilting point. It represents the water accessible to plants for uptake. High AWC supports better plant growth, while low AWC may necessitate irrigation. Source: USDA NRCS." ;
    skos:inScheme glosis_cl:physioChemicalPropertyCode ;
    skos:notation "Avavol" ;
    skos:prefLabel "Available water capacity - volumetric (FC to WP)"@en ;
    skos:topConceptOf glosis_cl:physioChemicalPropertyCode .

glosis_cl:physioChemicalPropertyCode-Bascal a glosis_cl:PhysioChemicalPropertyCode,
        skos:Concept ;
    skos:definition "Base saturation represents the percentage of the soil's cation exchange capacity (CEC) occupied by basic cations such as calcium (Ca²⁺), magnesium (Mg²⁺), potassium (K⁺), and sodium (Na⁺). Higher base saturation typically correlates with higher fertility and a greater ability to supply essential nutrients to plants. This parameter also influences soil pH buffering capacity. Source: Brady & Weil (2017)." ;
    skos:inScheme glosis_cl:physioChemicalPropertyCode ;
    skos:notation "Bascal" ;
    skos:prefLabel "Base saturation - calculated"@en ;
    skos:topConceptOf glosis_cl:physioChemicalPropertyCode .

glosis_cl:physioChemicalPropertyCode-Basexc a glosis_cl:PhysioChemicalPropertyCode,
        skos:Concept ;
    skos:definition "Exchangeable bases refer to the cations (e.g., calcium, magnesium, potassium, and sodium) adsorbed onto soil colloids, which can readily exchange with soil solution ions. These cations are crucial for maintaining soil fertility, affecting nutrient availability and pH buffering capacity. High exchangeable base levels indicate fertile soil conducive to plant growth. Source: Soil Science Society of America." ;
    skos:inScheme glosis_cl:physioChemicalPropertyCode ;
    skos:notation "Basexc" ;
    skos:prefLabel "Bases - exchangeable"@en ;
    skos:topConceptOf glosis_cl:physioChemicalPropertyCode .

glosis_cl:physioChemicalPropertyCode-Bassum a glosis_cl:PhysioChemicalPropertyCode,
        skos:Concept ;
    skos:definition "Base saturation calculated as the sum of cations represents the proportion of the cation exchange capacity (CEC) occupied by essential base cations like calcium, magnesium, potassium, and sodium. It provides insight into the soil's fertility status and its ability to resist acidification. Source: Soil Science Society of America." ;
    skos:inScheme glosis_cl:physioChemicalPropertyCode ;
    skos:notation "Bassum" ;
    skos:prefLabel "Base saturation - sum of cations"@en ;
    skos:topConceptOf glosis_cl:physioChemicalPropertyCode .

glosis_cl:physioChemicalPropertyCode-Borext a dbo:ChemicalCompound,
        dbo:ChemicalSubstance,
        glosis_cl:PhysioChemicalPropertyCode,
        skos:Concept ;
    dbo:inchi "1S/B" ;
    dbo:pubchem "5462311" ;
    dbprop:inchikey "ZOXJGFHDIHLPTG-UHFFFAOYSA-N" ;
    rdfs:seeAlso <https://pubchem.ncbi.nlm.nih.gov/compound/5462311> ;
    skos:definition "Boron bound to the soil matrix but that can be released into the soil solution (i.e. become bio-available)" ;
    skos:inScheme glosis_cl:physioChemicalPropertyCode ;
    skos:notation "Borext" ;
    skos:prefLabel "Boron (B) - extractable"@en ;
    skos:topConceptOf glosis_cl:physioChemicalPropertyCode .

glosis_cl:physioChemicalPropertyCode-Bortot a dbo:ChemicalCompound,
        dbo:ChemicalSubstance,
        glosis_cl:PhysioChemicalPropertyCode,
        skos:Concept ;
    dbo:inchi "1S/B" ;
    dbo:pubchem "5462311" ;
    dbprop:inchikey "ZOXJGFHDIHLPTG-UHFFFAOYSA-N" ;
    rdfs:seeAlso <https://pubchem.ncbi.nlm.nih.gov/compound/5462311> ;
    skos:definition "Total boron includes all boron forms in soil, crucial for plant cell wall formation and reproductive processes. Deficiency can impair growth, while toxicity is a risk in arid soils or with excessive irrigation. Source: Havlin et al. (2014)." ;
    skos:inScheme glosis_cl:physioChemicalPropertyCode ;
    skos:notation "Bortot" ;
    skos:prefLabel "Boron (B) - total"@en ;
    skos:topConceptOf glosis_cl:physioChemicalPropertyCode .

glosis_cl:physioChemicalPropertyCode-Brod a dbo:ChemicalCompound,
        dbo:ChemicalSubstance,
        glosis_cl:PhysioChemicalPropertyCode,
        skos:Concept ;
    dbo:inchi "1S/BrH/h1H/p-1" ;
    dbo:pubchem "259" ;
    dbprop:inchikey "CPELXLSAUQHCOX-UHFFFAOYSA-M" ;
    rdfs:seeAlso <https://pubchem.ncbi.nlm.nih.gov/compound/259> ;
    skos:definition "Bromide bound to the soil matrix but that can be released into the soil solution (i.e. become bio-available)" ;
    skos:inScheme glosis_cl:physioChemicalPropertyCode ;
    skos:notation "Brod" ;
    skos:prefLabel "Bromide (Br-) - extractable"@en ;
    skos:topConceptOf glosis_cl:physioChemicalPropertyCode .

glosis_cl:physioChemicalPropertyCode-Brot a dbo:ChemicalCompound,
        dbo:ChemicalSubstance,
        glosis_cl:PhysioChemicalPropertyCode,
        skos:Concept ;
    dbo:inchi "1S/BrHO2/c2-1-3/h(H,2,3)/p-1" ;
    dbo:pubchem "5460628" ;
    dbprop:inchikey "DKSMCEUSSQTGBK-UHFFFAOYSA-M" ;
    rdfs:seeAlso <https://pubchem.ncbi.nlm.nih.gov/compound/5460628> ;
    skos:definition "Bromite (BrO₂⁻) is a rare intermediate oxidation state of bromine, generally not prevalent in natural soils. It may arise under specific chemical or environmental conditions and is of limited importance in typical soil science contexts. Source: Environmental Chemistry Textbooks." ;
    skos:inScheme glosis_cl:physioChemicalPropertyCode ;
    skos:notation "Brot" ;
    skos:prefLabel "Bromite (BrO2-)"@en ;
    skos:topConceptOf glosis_cl:physioChemicalPropertyCode .

glosis_cl:physioChemicalPropertyCode-BulDfine a glosis_cl:PhysioChemicalPropertyCode,
        skos:Concept ;
    skos:definition "This parameter measures the bulk density of the soil fraction smaller than 2 mm (excluding rocks and coarse fragments). It is used to assess the physical properties of soil related to root growth, water movement, and compaction. Source: Soil Science Society of America." ;
    skos:inScheme glosis_cl:physioChemicalPropertyCode ;
    skos:notation "BulDfine" ;
    skos:prefLabel "Bulk Density of the fine earth fraction"@en ;
    skos:topConceptOf glosis_cl:physioChemicalPropertyCode .

glosis_cl:physioChemicalPropertyCode-BulDwhole a glosis_cl:PhysioChemicalPropertyCode,
        skos:Concept ;
    skos:definition "Bulk density measures the mass of soil per unit volume, including both solids and pore spaces. It is a critical parameter for assessing soil compaction, porosity, and water infiltration capacity. High bulk density often indicates poor aeration and root penetration, while low values are associated with high organic matter content and good structure. Source: USDA NRCS." ;
    skos:inScheme glosis_cl:physioChemicalPropertyCode ;
    skos:notation "BulDwhole" ;
    skos:prefLabel "Bulk Density of the whole soil"@en ;
    skos:topConceptOf glosis_cl:physioChemicalPropertyCode .

glosis_cl:physioChemicalPropertyCode-CEC a glosis_cl:PhysioChemicalPropertyCode,
        skos:Concept ;
    skos:definition "CEC measures the soil’s ability to hold and exchange positively charged ions (cations). It is a critical indicator of soil fertility, as higher CEC values imply greater capacity to retain essential nutrients like calcium, magnesium, and potassium. Clayey and organic-rich soils typically exhibit higher CEC. Source: Soil Science Society of America." ;
    skos:inScheme glosis_cl:physioChemicalPropertyCode ;
    skos:notation "CEC" ;
    skos:prefLabel "Cation exchange capacity (CEC)"@en ;
    skos:topConceptOf glosis_cl:physioChemicalPropertyCode .

glosis_cl:physioChemicalPropertyCode-CaN a glosis_cl:PhysioChemicalPropertyCode,
        skos:Concept ;
    skos:definition "The C/N ratio represents the proportion of carbon to nitrogen in organic matter. It influences decomposition rates and nutrient availability. A lower C/N ratio promotes rapid organic matter breakdown and nitrogen release, while a high ratio may lead to nitrogen immobilization, affecting plant growth. Source: Brady & Weil (2017)." ;
    skos:inScheme glosis_cl:physioChemicalPropertyCode ;
    skos:notation "CaN" ;
    skos:prefLabel "Carbon/Nitrogen (C/N) ratio"@en ;
    skos:topConceptOf glosis_cl:physioChemicalPropertyCode .

glosis_cl:physioChemicalPropertyCode-Cad a dbo:ChemicalCompound,
        dbo:ChemicalSubstance,
        glosis_cl:PhysioChemicalPropertyCode,
        skos:Concept ;
    dbo:inchi "1S/Cd" ;
    dbo:pubchem "23973" ;
    dbprop:inchikey "BDOSMKKIYDKNTQ-UHFFFAOYSA-N" ;
    rdfs:seeAlso <https://pubchem.ncbi.nlm.nih.gov/compound/23973> ;
    skos:definition "Cadmium is a heavy metal present in trace amounts in soils, often introduced through industrial pollution or phosphate fertilizers. It is toxic to plants, animals, and humans even at low concentrations. Monitoring cadmium levels is crucial to ensure soil safety and reduce contamination risks in the food chain. Source: Sparks, D.L. (2003)." ;
    skos:inScheme glosis_cl:physioChemicalPropertyCode ;
    skos:notation "Cad" ;
    skos:prefLabel "Cadmium (Cd)"@en ;
    skos:topConceptOf glosis_cl:physioChemicalPropertyCode .

glosis_cl:physioChemicalPropertyCode-Calexc a dbo:ChemicalCompound,
        dbo:ChemicalSubstance,
        glosis_cl:PhysioChemicalPropertyCode,
        skos:Concept ;
    dbo:inchi "1S/Ca/q+2" ;
    dbo:pubchem "271" ;
    dbprop:inchikey "BHPQYMZQTOCNFJ-UHFFFAOYSA-N" ;
    rdfs:seeAlso <https://pubchem.ncbi.nlm.nih.gov/compound/271> ;
    skos:definition "Calcium bound to exchange surfaces in the soil such as clay minerals and organic matter that can be released to the soil solution upon exchange" ;
    skos:inScheme glosis_cl:physioChemicalPropertyCode ;
    skos:notation "Calexc" ;
    skos:prefLabel "Calcium (Ca++) - exchangeable"@en ;
    skos:topConceptOf glosis_cl:physioChemicalPropertyCode .

glosis_cl:physioChemicalPropertyCode-Calext a dbo:ChemicalCompound,
        dbo:ChemicalSubstance,
        glosis_cl:PhysioChemicalPropertyCode,
        skos:Concept ;
    dbo:inchi "1S/Ca/q+2" ;
    dbo:pubchem "271" ;
    dbprop:inchikey "BHPQYMZQTOCNFJ-UHFFFAOYSA-N" ;
    rdfs:seeAlso <https://pubchem.ncbi.nlm.nih.gov/compound/271> ;
    skos:definition "Calcium bound to the soil matrix but that can be released into the soil solution (i.e. become bio-available)" ;
    skos:inScheme glosis_cl:physioChemicalPropertyCode ;
    skos:notation "Calext" ;
    skos:prefLabel "Calcium (Ca++) - extractable"@en ;
    skos:topConceptOf glosis_cl:physioChemicalPropertyCode .

glosis_cl:physioChemicalPropertyCode-Calfra a dbo:ChemicalCompound,
        dbo:ChemicalSubstance,
        glosis_cl:PhysioChemicalPropertyCode,
        skos:Concept ;
    dbo:inchi "1S/CH2O3.Ca/c2-1(3)4;/h(H2,2,3,4);/q;+2/p-2" ;
    dbo:pubchem "10112" ;
    dbprop:inchikey "VTYYLEPIZMXCLO-UHFFFAOYSA-L" ;
    rdfs:seeAlso <https://pubchem.ncbi.nlm.nih.gov/compound/10112> ;
    skos:definition "This term quantifies the fraction of calcium carbonate (CaCO₃) in soil, indicating its lime content. Calcium carbonate acts as a pH buffer, neutralizing soil acidity and enhancing nutrient availability. High levels improve soil structure and aggregate stability, making it especially valuable for acidic soils. Source: FAO Soil Bulletin." ;
    skos:inScheme glosis_cl:physioChemicalPropertyCode ;
    skos:notation "Calfra" ;
    skos:prefLabel "Calcium carbonate equivalent - fraction"@en ;
    skos:topConceptOf glosis_cl:physioChemicalPropertyCode .

glosis_cl:physioChemicalPropertyCode-Calsol a dbo:ChemicalCompound,
        dbo:ChemicalSubstance,
        glosis_cl:PhysioChemicalPropertyCode,
        skos:Concept ;
    dbo:inchi "1S/Ca/q+2" ;
    dbo:pubchem "271" ;
    dbprop:inchikey "BHPQYMZQTOCNFJ-UHFFFAOYSA-N" ;
    rdfs:seeAlso <https://pubchem.ncbi.nlm.nih.gov/compound/271> ;
    skos:definition "Soluble Calcium cations accumulated in the soil. A contributor to soil salinisation." ;
    skos:inScheme glosis_cl:physioChemicalPropertyCode ;
    skos:notation "Calsol" ;
    skos:prefLabel "Calcium (Ca++) - soluble"@en ;
    skos:topConceptOf glosis_cl:physioChemicalPropertyCode .

glosis_cl:physioChemicalPropertyCode-Caltot a dbo:ChemicalCompound,
        dbo:ChemicalSubstance,
        glosis_cl:PhysioChemicalPropertyCode,
        skos:Concept ;
    dbo:inchi "1S/Ca/q+2" ;
    dbo:pubchem "271" ;
    dbprop:inchikey "BHPQYMZQTOCNFJ-UHFFFAOYSA-N" ;
    rdfs:seeAlso <https://pubchem.ncbi.nlm.nih.gov/compound/271> ;
    skos:definition "Total calcium in soil includes all forms, from exchangeable calcium to calcium in minerals. It is essential for plant cell wall structure, enzyme activation, and soil aggregation. Calcium levels influence soil pH and nutrient availability. Source: Havlin et al. (2014)." ;
    skos:inScheme glosis_cl:physioChemicalPropertyCode ;
    skos:notation "Caltot" ;
    skos:prefLabel "Calcium (Ca++) - total"@en ;
    skos:topConceptOf glosis_cl:physioChemicalPropertyCode .

glosis_cl:physioChemicalPropertyCode-Car a dbo:ChemicalCompound,
        dbo:ChemicalSubstance,
        glosis_cl:PhysioChemicalPropertyCode,
        skos:Concept ;
    dbo:inchi "1S/CH2O3/c2-1(3)4/h(H2,2,3,4)/p-2" ;
    dbo:pubchem "19660" ;
    dbprop:inchikey "BVKZGUZCCUSVTD-UHFFFAOYSA-L" ;
    rdfs:seeAlso <https://pubchem.ncbi.nlm.nih.gov/compound/19660> ;
    skos:definition "Soluble carbonates contribute to soil alkalinity and act as a pH buffer. They play a role in nutrient availability, particularly in arid and semi-arid regions, but excessive carbonates can immobilize certain nutrients like phosphorus and iron. Source: Soil Chemistry by Bohn et al." ;
    skos:inScheme glosis_cl:physioChemicalPropertyCode ;
    skos:notation "Car" ;
    skos:prefLabel "Carbonate (CO3--) - soluble"@en ;
    skos:topConceptOf glosis_cl:physioChemicalPropertyCode .

glosis_cl:physioChemicalPropertyCode-Carful a dbo:ChemicalCompound,
        dbo:ChemicalSubstance,
        glosis_cl:PhysioChemicalPropertyCode,
        skos:Concept ;
    dbo:inchi "1S/C" ;
    dbo:pubchem "5462310" ;
    dbprop:inchikey "OKTJSMMVPCPJKN-UHFFFAOYSA-N" ;
    rdfs:seeAlso <https://pubchem.ncbi.nlm.nih.gov/compound/5462310> ;
    skos:definition "Fulvic acid carbon is the most soluble and bioavailable fraction of soil organic matter. It plays a significant role in improving nutrient uptake, soil structure, and microbial activity, thereby enhancing soil productivity. Source: Stevenson, F.J. (1994)." ;
    skos:inScheme glosis_cl:physioChemicalPropertyCode ;
    skos:notation "Carful" ;
    skos:prefLabel "Carbon (C) - fulvic acid"@en ;
    skos:topConceptOf glosis_cl:physioChemicalPropertyCode .

glosis_cl:physioChemicalPropertyCode-Carhum a dbo:ChemicalCompound,
        dbo:ChemicalSubstance,
        glosis_cl:PhysioChemicalPropertyCode,
        skos:Concept ;
    dbo:inchi "1S/C" ;
    dbo:pubchem "5462310" ;
    dbprop:inchikey "OKTJSMMVPCPJKN-UHFFFAOYSA-N" ;
    rdfs:seeAlso <https://pubchem.ncbi.nlm.nih.gov/compound/5462310> ;
    skos:definition "Humic acid carbon is part of the soil organic matter, forming during the decomposition of plant and animal residues. It enhances nutrient retention, soil structure, and water-holding capacity, playing a vital role in maintaining soil fertility and resilience. Source: Stevenson, F.J. (1994). Humus Chemistry: Genesis, Composition, Reactions." ;
    skos:inScheme glosis_cl:physioChemicalPropertyCode ;
    skos:notation "Carhum" ;
    skos:prefLabel "Carbon (C) - humic acid"@en ;
    skos:topConceptOf glosis_cl:physioChemicalPropertyCode .

glosis_cl:physioChemicalPropertyCode-Carinorg a dbo:ChemicalCompound,
        dbo:ChemicalSubstance,
        glosis_cl:PhysioChemicalPropertyCode,
        skos:Concept ;
    dbo:inchi "1S/C" ;
    dbo:pubchem "5462310" ;
    dbprop:inchikey "OKTJSMMVPCPJKN-UHFFFAOYSA-N" ;
    rdfs:seeAlso <https://pubchem.ncbi.nlm.nih.gov/compound/5462310> ;
    skos:definition "Inorganic carbon in soil primarily consists of carbonates like calcium carbonate and magnesium carbonate. It contributes to soil pH buffering and is a significant feature of arid and calcareous soils. Excess inorganic carbon can immobilize certain nutrients, requiring careful management in agricultural systems. Source: Soil Science Society of America." ;
    skos:inScheme glosis_cl:physioChemicalPropertyCode ;
    skos:notation "Carinorg" ;
    skos:prefLabel "Carbon (C) - inorganic"@en ;
    skos:topConceptOf glosis_cl:physioChemicalPropertyCode .

glosis_cl:physioChemicalPropertyCode-Carorg a dbo:ChemicalCompound,
        dbo:ChemicalSubstance,
        glosis_cl:PhysioChemicalPropertyCode,
        skos:Concept ;
    dbo:inchi "1S/C" ;
    dbo:pubchem "5462310" ;
    dbprop:inchikey "OKTJSMMVPCPJKN-UHFFFAOYSA-N" ;
    rdfs:seeAlso <https://pubchem.ncbi.nlm.nih.gov/compound/5462310> ;
    skos:definition "Organic carbon refers to the carbon component of soil organic matter, derived from decomposed plant and microbial residues. It serves as a key energy source for soil microbes and influences nutrient cycling, soil structure, and water retention. Organic carbon is a primary indicator of soil fertility and health. Source: Brady & Weil (2017)." ;
    skos:inScheme glosis_cl:physioChemicalPropertyCode ;
    skos:notation "Carorg" ;
    skos:prefLabel "Carbon (C) - organic"@en ;
    skos:topConceptOf glosis_cl:physioChemicalPropertyCode .

glosis_cl:physioChemicalPropertyCode-Carpyr a dbo:ChemicalCompound,
        dbo:ChemicalSubstance,
        glosis_cl:PhysioChemicalPropertyCode,
        skos:Concept ;
    dbo:inchi "1S/C" ;
    dbo:pubchem "5462310" ;
    dbprop:inchikey "OKTJSMMVPCPJKN-UHFFFAOYSA-N" ;
    rdfs:seeAlso <https://pubchem.ncbi.nlm.nih.gov/compound/5462310> ;
    skos:definition "Carbon in soil that is organically bound in organo-metal complexes" ;
    skos:inScheme glosis_cl:physioChemicalPropertyCode ;
    skos:notation "Carpyr" ;
    skos:prefLabel "Carbon (C) - pyrophosphate extractable"@en ;
    skos:topConceptOf glosis_cl:physioChemicalPropertyCode .

glosis_cl:physioChemicalPropertyCode-Cartoh a dbo:ChemicalCompound,
        dbo:ChemicalSubstance,
        glosis_cl:PhysioChemicalPropertyCode,
        skos:Concept ;
    dbo:inchi "1S/C" ;
    dbo:pubchem "5462310" ;
    dbprop:inchikey "OKTJSMMVPCPJKN-UHFFFAOYSA-N" ;
    rdfs:seeAlso <https://pubchem.ncbi.nlm.nih.gov/compound/5462310> ;
    skos:definition "Total humic carbon represents the stable fraction of soil organic matter derived from humified materials. It improves soil structure, nutrient retention, and water-holding capacity, making it critical for long-term soil health and productivity. Source: Stevenson, F.J. (1994)." ;
    skos:inScheme glosis_cl:physioChemicalPropertyCode ;
    skos:notation "Cartoh" ;
    skos:prefLabel "Carbon (C) - total humic"@en ;
    skos:topConceptOf glosis_cl:physioChemicalPropertyCode .

glosis_cl:physioChemicalPropertyCode-Cartot a dbo:ChemicalCompound,
        dbo:ChemicalSubstance,
        glosis_cl:PhysioChemicalPropertyCode,
        skos:Concept ;
    dbo:inchi "1S/C" ;
    dbo:pubchem "5462310" ;
    dbprop:inchikey "OKTJSMMVPCPJKN-UHFFFAOYSA-N" ;
    rdfs:seeAlso <https://pubchem.ncbi.nlm.nih.gov/compound/5462310> ;
    skos:definition "Total carbon in soil includes both organic carbon (from plant and microbial residues) and inorganic carbon (primarily carbonates). It is a fundamental component of soil organic matter, influencing soil fertility, structure, and water retention. High carbon levels are associated with better soil health and productivity. Source: USDA NRCS." ;
    skos:inScheme glosis_cl:physioChemicalPropertyCode ;
    skos:notation "Cartot" ;
    skos:prefLabel "Carbon (C) - total"@en ;
    skos:topConceptOf glosis_cl:physioChemicalPropertyCode .

glosis_cl:physioChemicalPropertyCode-Ccetot a dbo:ChemicalCompound,
        dbo:ChemicalSubstance,
        glosis_cl:PhysioChemicalPropertyCode,
        skos:Concept ;
    dbo:inchi "1S/CH2O3.Ca/c2-1(3)4;/h(H2,2,3,4);/q;+2/p-2" ;
    dbo:pubchem "10112" ;
    dbprop:inchikey "VTYYLEPIZMXCLO-UHFFFAOYSA-L" ;
    rdfs:seeAlso <https://pubchem.ncbi.nlm.nih.gov/compound/10112> ;
    skos:definition "The total calcium carbonate equivalent measures the full capacity of soil to neutralize acidity, considering all forms of carbonate and bicarbonate minerals. It is essential for managing soil pH and nutrient availability in acidic soils. Source: FAO Soil Bulletin." ;
    skos:inScheme glosis_cl:physioChemicalPropertyCode ;
    skos:notation "Ccetot" ;
    skos:prefLabel "Calcium carbonate equivalent - total"@en ;
    skos:topConceptOf glosis_cl:physioChemicalPropertyCode .

glosis_cl:physioChemicalPropertyCode-Chl a dbo:ChemicalCompound,
        dbo:ChemicalSubstance,
        glosis_cl:PhysioChemicalPropertyCode,
        skos:Concept ;
    dbo:inchi "1S/ClH/h1H/p-1" ;
    dbo:pubchem "312" ;
    dbprop:inchikey "VEXZGXHMUGYJMC-UHFFFAOYSA-M" ;
    rdfs:seeAlso <https://pubchem.ncbi.nlm.nih.gov/compound/312> ;
    skos:definition "Soluble Chloride anions accumulated in the soil. A contributor to soil salinisation." ;
    skos:inScheme glosis_cl:physioChemicalPropertyCode ;
    skos:notation "Chl" ;
    skos:prefLabel "Chloride (Cl-) - soluble"@en ;
    skos:topConceptOf glosis_cl:physioChemicalPropertyCode .

glosis_cl:physioChemicalPropertyCode-Copext a dbo:ChemicalCompound,
        dbo:ChemicalSubstance,
        glosis_cl:PhysioChemicalPropertyCode,
        skos:Concept ;
    dbo:inchi "1S/Cu" ;
    dbo:pubchem "23978" ;
    dbprop:inchikey "RYGMFSIKBFXOCR-UHFFFAOYSA-N" ;
    rdfs:seeAlso <https://pubchem.ncbi.nlm.nih.gov/compound/23978> ;
    skos:definition "Copper bound to the soil matrix but that can be released into the soil solution (i.e. become bio-available)" ;
    skos:inScheme glosis_cl:physioChemicalPropertyCode ;
    skos:notation "Copext" ;
    skos:prefLabel "Copper (Cu) - extractable"@en ;
    skos:topConceptOf glosis_cl:physioChemicalPropertyCode .

glosis_cl:physioChemicalPropertyCode-Coptot a dbo:ChemicalCompound,
        dbo:ChemicalSubstance,
        glosis_cl:PhysioChemicalPropertyCode,
        skos:Concept ;
    dbo:inchi "1S/Cu" ;
    dbo:pubchem "23978" ;
    dbprop:inchikey "RYGMFSIKBFXOCR-UHFFFAOYSA-N" ;
    rdfs:seeAlso <https://pubchem.ncbi.nlm.nih.gov/compound/23978> ;
    skos:definition "Total copper comprises all soil copper, including bound and free forms. Copper is vital for plant enzyme activation and metabolic processes. Deficiencies can lead to reduced growth and yields, while excess copper may inhibit root development. Source: Soil Science Society of America." ;
    skos:inScheme glosis_cl:physioChemicalPropertyCode ;
    skos:notation "Coptot" ;
    skos:prefLabel "Copper (Cu) - total"@en ;
    skos:topConceptOf glosis_cl:physioChemicalPropertyCode .

glosis_cl:physioChemicalPropertyCode-ECEC a glosis_cl:PhysioChemicalPropertyCode,
        skos:Concept ;
    skos:definition "ECEC is the sum of exchangeable cations in soil at its natural pH. It provides a measure of the soil’s fertility under acidic conditions, as it considers both base cations and exchangeable aluminum. Source: Brady & Weil (2017)." ;
    skos:inScheme glosis_cl:physioChemicalPropertyCode ;
    skos:notation "ECEC" ;
    skos:prefLabel "Cation exchange capacity effective (ECEC)"@en ;
    skos:topConceptOf glosis_cl:physioChemicalPropertyCode .

glosis_cl:physioChemicalPropertyCode-Eleccond a glosis_cl:PhysioChemicalPropertyCode,
        skos:Concept ;
    skos:definition "Electrical conductivity (EC) measures the ability of soil to conduct an electrical current, which is directly related to the concentration of soluble salts. It is an essential indicator of soil salinity and is used to assess soil's suitability for crop growth. High EC levels can reduce plant water uptake and affect germination, while low levels indicate low salinity and better soil health. Source: USDA NRCS." ;
    skos:inScheme glosis_cl:physioChemicalPropertyCode ;
    skos:notation "Eleccond" ;
    skos:prefLabel "Electrical conductivity"@en ;
    skos:topConceptOf glosis_cl:physioChemicalPropertyCode .

glosis_cl:physioChemicalPropertyCode-Gyp a dbo:ChemicalCompound,
        dbo:ChemicalSubstance,
        glosis_cl:PhysioChemicalPropertyCode,
        skos:Concept ;
    dbo:pubchem "24497" ;
    rdfs:seeAlso <https://pubchem.ncbi.nlm.nih.gov/compound/24497> ;
    skos:definition "The gypsum content, expressed as weight, refers to the soil’s calcium sulfate levels. Gypsum improves soil structure, alleviates sodicity, and enhances water infiltration. It is commonly applied to saline-sodic soils for reclamation. Source: FAO Soil Bulletin." ;
    skos:inScheme glosis_cl:physioChemicalPropertyCode ;
    skos:notation "Gyp" ;
    skos:prefLabel "Gypsum content - weight"@en ;
    skos:topConceptOf glosis_cl:physioChemicalPropertyCode .

glosis_cl:physioChemicalPropertyCode-Hyd a dbo:ChemicalCompound,
        dbo:ChemicalSubstance,
        glosis_cl:PhysioChemicalPropertyCode,
        skos:Concept ;
    dbo:inchi "1S/CH2O3/c2-1(3)4/h(H2,2,3,4)/p-1" ;
    dbo:pubchem "769" ;
    dbprop:inchikey "BVKZGUZCCUSVTD-UHFFFAOYSA-M" ;
    rdfs:seeAlso <https://pubchem.ncbi.nlm.nih.gov/compound/769> ;
    skos:definition "Soluble Hydrocarbonate anions accumulated in the soil. A contributor to soil salinisation." ;
    skos:inScheme glosis_cl:physioChemicalPropertyCode ;
    skos:notation "Hyd" ;
    skos:prefLabel "Hydrocarbonate (HCO3-) - soluble"@en ;
    skos:topConceptOf glosis_cl:physioChemicalPropertyCode .

glosis_cl:physioChemicalPropertyCode-Hydcond a glosis_cl:PhysioChemicalPropertyCode,
        skos:Concept ;
    skos:definition "Hydraulic conductivity refers to the rate at which water moves through soil pores under a unit hydraulic gradient. It reflects the soil's ability to transmit water, influenced by texture, structure, and porosity. Soils with high hydraulic conductivity, like sandy soils, allow rapid water movement, while clayey soils exhibit slower water flow. This property is critical for understanding water infiltration, drainage, and irrigation management. Source: Brady, N.C., & Weil, R.R. (2017). The Nature and Properties of Soils." ;
    skos:inScheme glosis_cl:physioChemicalPropertyCode ;
    skos:notation "Hydcond" ;
    skos:prefLabel "Hydraulic conductivity"@en ;
    skos:topConceptOf glosis_cl:physioChemicalPropertyCode .

glosis_cl:physioChemicalPropertyCode-Hydexc a dbo:ChemicalCompound,
        dbo:ChemicalSubstance,
        glosis_cl:PhysioChemicalPropertyCode,
        skos:Concept ;
    dbo:inchi "1S/p+1" ;
    dbo:pubchem "1038" ;
    dbprop:inchikey "GPRLSGONYQIRFK-UHFFFAOYSA-N" ;
    rdfs:seeAlso <https://pubchem.ncbi.nlm.nih.gov/compound/1038> ;
    skos:definition "Hydrogen ions bound to exchange surfaces in the soil such as clay minerals and organic matter that can be released to the soil solution upon exchange" ;
    skos:inScheme glosis_cl:physioChemicalPropertyCode ;
    skos:notation "Hydexc" ;
    skos:prefLabel "Hydrogen (H+) - exchangeable"@en ;
    skos:topConceptOf glosis_cl:physioChemicalPropertyCode .

glosis_cl:physioChemicalPropertyCode-Irodit a dbo:ChemicalCompound,
        dbo:ChemicalSubstance,
        glosis_cl:PhysioChemicalPropertyCode,
        skos:Concept ;
    dbo:inchi "1S/Fe" ;
    dbo:pubchem "23925" ;
    dbprop:inchikey "XEEYBQQBJWHFJM-UHFFFAOYSA-N" ;
    rdfs:seeAlso <https://pubchem.ncbi.nlm.nih.gov/compound/23925> ;
    skos:definition "'Free' iron content extracted from amorphous compounds (weathering products) as well as crystaline, primary aluminium compounds (parent material) in the soil." ;
    skos:inScheme glosis_cl:physioChemicalPropertyCode ;
    skos:notation "Irodit" ;
    skos:prefLabel "Iron (Fe) - dithionite extractable"@en ;
    skos:topConceptOf glosis_cl:physioChemicalPropertyCode .

glosis_cl:physioChemicalPropertyCode-Iroext a dbo:ChemicalCompound,
        dbo:ChemicalSubstance,
        glosis_cl:PhysioChemicalPropertyCode,
        skos:Concept ;
    dbo:inchi "1S/Fe" ;
    dbo:pubchem "23925" ;
    dbprop:inchikey "XEEYBQQBJWHFJM-UHFFFAOYSA-N" ;
    rdfs:seeAlso <https://pubchem.ncbi.nlm.nih.gov/compound/23925> ;
    skos:definition "Iron bound to the soil matrix but that can be released into the soil solution (i.e. become bio-available)" ;
    skos:inScheme glosis_cl:physioChemicalPropertyCode ;
    skos:notation "Iroext" ;
    skos:prefLabel "Iron (Fe) - extractable"@en ;
    skos:topConceptOf glosis_cl:physioChemicalPropertyCode .

glosis_cl:physioChemicalPropertyCode-Irooxa a dbo:ChemicalCompound,
        dbo:ChemicalSubstance,
        glosis_cl:PhysioChemicalPropertyCode,
        skos:Concept ;
    dbo:inchi "1S/Fe" ;
    dbo:pubchem "23925" ;
    dbprop:inchikey "XEEYBQQBJWHFJM-UHFFFAOYSA-N" ;
    rdfs:seeAlso <https://pubchem.ncbi.nlm.nih.gov/compound/23925> ;
    skos:definition "'Active' iron content extracted from amorphous iron compounds that are the products of the weathering of primary soil particles" ;
    skos:inScheme glosis_cl:physioChemicalPropertyCode ;
    skos:notation "Irooxa" ;
    skos:prefLabel "Iron (Fe) - oxalate extractable"@en ;
    skos:topConceptOf glosis_cl:physioChemicalPropertyCode .

glosis_cl:physioChemicalPropertyCode-Iropyr a dbo:ChemicalCompound,
        dbo:ChemicalSubstance,
        glosis_cl:PhysioChemicalPropertyCode,
        skos:Concept ;
    dbo:inchi "1S/Fe" ;
    dbo:pubchem "23925" ;
    dbprop:inchikey "XEEYBQQBJWHFJM-UHFFFAOYSA-N" ;
    rdfs:seeAlso <https://pubchem.ncbi.nlm.nih.gov/compound/23925> ;
    skos:definition "Iron in soil that is organically bound in organo-metal complexes" ;
    skos:inScheme glosis_cl:physioChemicalPropertyCode ;
    skos:notation "Iropyr" ;
    skos:prefLabel "Iron (Fe) - pyrophosphate extractable"@en ;
    skos:topConceptOf glosis_cl:physioChemicalPropertyCode .

glosis_cl:physioChemicalPropertyCode-Irotot a dbo:ChemicalCompound,
        dbo:ChemicalSubstance,
        glosis_cl:PhysioChemicalPropertyCode,
        skos:Concept ;
    dbo:inchi "1S/Fe" ;
    dbo:pubchem "23925" ;
    dbprop:inchikey "XEEYBQQBJWHFJM-UHFFFAOYSA-N" ;
    rdfs:seeAlso <https://pubchem.ncbi.nlm.nih.gov/compound/23925> ;
    skos:definition "Total iron includes all iron forms in the soil, from soluble ferrous iron (Fe²⁺) to insoluble ferric iron (Fe³⁺). Iron is essential for plant chlorophyll synthesis and various enzymatic reactions. Deficiency, often seen in alkaline soils, results in chlorosis, while excessive iron can cause toxicity in acidic soils. Source: Soil Chemistry by Bohn et al." ;
    skos:inScheme glosis_cl:physioChemicalPropertyCode ;
    skos:notation "Irotot" ;
    skos:prefLabel "Iron (Fe) - total"@en ;
    skos:topConceptOf glosis_cl:physioChemicalPropertyCode .

glosis_cl:physioChemicalPropertyCode-Magexc a dbo:ChemicalCompound,
        dbo:ChemicalSubstance,
        glosis_cl:PhysioChemicalPropertyCode,
        skos:Concept ;
    dbo:inchi "1S/Mg/q+2" ;
    dbo:pubchem "888" ;
    dbprop:inchikey "JLVVSXFLKOJNIY-UHFFFAOYSA-N" ;
    rdfs:seeAlso <https://pubchem.ncbi.nlm.nih.gov/compound/888> ;
    skos:definition "Magnesium bound to exchange surfaces in the soil such as clay minerals and organic matter that can be released to the soil solution upon exchange" ;
    skos:inScheme glosis_cl:physioChemicalPropertyCode ;
    skos:notation "Magexc" ;
    skos:prefLabel "Magnesium (Mg++) - exchangeable"@en ;
    skos:topConceptOf glosis_cl:physioChemicalPropertyCode .

glosis_cl:physioChemicalPropertyCode-Magext a dbo:ChemicalCompound,
        dbo:ChemicalSubstance,
        glosis_cl:PhysioChemicalPropertyCode,
        skos:Concept ;
    dbo:inchi "1S/Mg" ;
    dbo:pubchem "5462224" ;
    dbprop:inchikey "FYYHWMGAXLPEAU-UHFFFAOYSA-N" ;
    rdfs:seeAlso <https://pubchem.ncbi.nlm.nih.gov/compound/5462224> ;
    skos:definition "Magnesium bound to the soil matrix but that can be released into the soil solution (i.e. become bio-available)" ;
    skos:inScheme glosis_cl:physioChemicalPropertyCode ;
    skos:notation "Magext" ;
    skos:prefLabel "Magnesium (Mg) - extractable"@en ;
    skos:topConceptOf glosis_cl:physioChemicalPropertyCode .

glosis_cl:physioChemicalPropertyCode-Magsol a dbo:ChemicalCompound,
        dbo:ChemicalSubstance,
        glosis_cl:PhysioChemicalPropertyCode,
        skos:Concept ;
    dbo:inchi "1S/Mg/q+2" ;
    dbo:pubchem "888" ;
    dbprop:inchikey "JLVVSXFLKOJNIY-UHFFFAOYSA-N" ;
    rdfs:seeAlso <https://pubchem.ncbi.nlm.nih.gov/compound/888> ;
    skos:definition "Soluble Magnesium cations accumulated in the soil. A contributor to soil salinisation." ;
    skos:inScheme glosis_cl:physioChemicalPropertyCode ;
    skos:notation "Magsol" ;
    skos:prefLabel "Magnesium (Mg++) - soluble"@en ;
    skos:topConceptOf glosis_cl:physioChemicalPropertyCode .

glosis_cl:physioChemicalPropertyCode-Magtot a dbo:ChemicalCompound,
        dbo:ChemicalSubstance,
        glosis_cl:PhysioChemicalPropertyCode,
        skos:Concept ;
    dbo:inchi "1S/Mg" ;
    dbo:pubchem "5462224" ;
    dbprop:inchikey "FYYHWMGAXLPEAU-UHFFFAOYSA-N" ;
    rdfs:seeAlso <https://pubchem.ncbi.nlm.nih.gov/compound/5462224> ;
    skos:definition "Total magnesium in soil includes exchangeable, soluble, and mineral-bound forms. Magnesium is essential for chlorophyll synthesis, enzyme activation, and nutrient transport in plants. Its availability is influenced by soil pH and texture. Source: Havlin et al. (2014)." ;
    skos:inScheme glosis_cl:physioChemicalPropertyCode ;
    skos:notation "Magtot" ;
    skos:prefLabel "Magnesium (Mg) - total"@en ;
    skos:topConceptOf glosis_cl:physioChemicalPropertyCode .

glosis_cl:physioChemicalPropertyCode-ManKCl a dbo:ChemicalCompound,
        dbo:ChemicalSubstance,
        glosis_cl:PhysioChemicalPropertyCode,
        skos:Concept ;
    dbo:inchi "1S/Mn" ;
    dbo:pubchem "23930" ;
    dbprop:inchikey "PWHULOQIROXLJO-UHFFFAOYSA-N" ;
    rdfs:seeAlso <https://pubchem.ncbi.nlm.nih.gov/compound/23930> ;
    skos:definition "KCl extractable manganese measures the readily available manganese fraction in soil. It provides a more accurate assessment of manganese availability to plants than total manganese. This method is commonly used for nutrient management. Source: Soil Science Society of America." ;
    skos:inScheme glosis_cl:physioChemicalPropertyCode ;
    skos:notation "ManKCl" ;
    skos:prefLabel "Manganese (Mn) - KCl extractable"@en ;
    skos:topConceptOf glosis_cl:physioChemicalPropertyCode .

glosis_cl:physioChemicalPropertyCode-Mandit a dbo:ChemicalCompound,
        dbo:ChemicalSubstance,
        glosis_cl:PhysioChemicalPropertyCode,
        skos:Concept ;
    dbo:inchi "1S/Mn" ;
    dbo:pubchem "23930" ;
    dbprop:inchikey "PWHULOQIROXLJO-UHFFFAOYSA-N" ;
    rdfs:seeAlso <https://pubchem.ncbi.nlm.nih.gov/compound/23930> ;
    skos:definition "'Free' manganese content extracted from amorphous compounds (weathering products) as well as crystaline, primary aluminium compounds (parent material) in the soil." ;
    skos:inScheme glosis_cl:physioChemicalPropertyCode ;
    skos:notation "Mandit" ;
    skos:prefLabel "Manganese (Mn) - dithionite extractable"@en ;
    skos:topConceptOf glosis_cl:physioChemicalPropertyCode .

glosis_cl:physioChemicalPropertyCode-Manext a dbo:ChemicalCompound,
        dbo:ChemicalSubstance,
        glosis_cl:PhysioChemicalPropertyCode,
        skos:Concept ;
    dbo:inchi "1S/Mn" ;
    dbo:pubchem "23930" ;
    dbprop:inchikey "PWHULOQIROXLJO-UHFFFAOYSA-N" ;
    rdfs:seeAlso <https://pubchem.ncbi.nlm.nih.gov/compound/23930> ;
    skos:definition "Manganese bound to the soil matrix but that can be released into the soil solution (i.e. become bio-available)" ;
    skos:inScheme glosis_cl:physioChemicalPropertyCode ;
    skos:notation "Manext" ;
    skos:prefLabel "Manganese (Mn) - extractable"@en ;
    skos:topConceptOf glosis_cl:physioChemicalPropertyCode .

glosis_cl:physioChemicalPropertyCode-Manoxa a dbo:ChemicalCompound,
        dbo:ChemicalSubstance,
        glosis_cl:PhysioChemicalPropertyCode,
        skos:Concept ;
    dbo:inchi "1S/Mn" ;
    dbo:pubchem "23930" ;
    dbprop:inchikey "PWHULOQIROXLJO-UHFFFAOYSA-N" ;
    rdfs:seeAlso <https://pubchem.ncbi.nlm.nih.gov/compound/23930> ;
    skos:definition "'Active' manganese content extracted from amorphous manganese compounds that are the products of the weathering of primary soil particles" ;
    skos:inScheme glosis_cl:physioChemicalPropertyCode ;
    skos:notation "Manoxa" ;
    skos:prefLabel "Manganese (Mn) - oxalate extractable"@en ;
    skos:topConceptOf glosis_cl:physioChemicalPropertyCode .

glosis_cl:physioChemicalPropertyCode-Manpyr a dbo:ChemicalCompound,
        dbo:ChemicalSubstance,
        glosis_cl:PhysioChemicalPropertyCode,
        skos:Concept ;
    dbo:inchi "1S/Mn" ;
    dbo:pubchem "23930" ;
    dbprop:inchikey "PWHULOQIROXLJO-UHFFFAOYSA-N" ;
    rdfs:seeAlso <https://pubchem.ncbi.nlm.nih.gov/compound/23930> ;
    skos:definition "Manganese in soil that is organically bound in organo-metal complexes" ;
    skos:inScheme glosis_cl:physioChemicalPropertyCode ;
    skos:notation "Manpyr" ;
    skos:prefLabel "Manganese (Mn) - pyrophosphate extractable"@en ;
    skos:topConceptOf glosis_cl:physioChemicalPropertyCode .

glosis_cl:physioChemicalPropertyCode-Mantot a dbo:ChemicalCompound,
        dbo:ChemicalSubstance,
        glosis_cl:PhysioChemicalPropertyCode,
        skos:Concept ;
    dbo:inchi "1S/Mn" ;
    dbo:pubchem "23930" ;
    dbprop:inchikey "PWHULOQIROXLJO-UHFFFAOYSA-N" ;
    rdfs:seeAlso <https://pubchem.ncbi.nlm.nih.gov/compound/23930> ;
    skos:definition "Total manganese refers to all forms of manganese in the soil, which is critical for photosynthesis, enzyme activation, and nitrogen metabolism in plants. Manganese deficiencies or toxicities are influenced by soil pH, with deficiencies occurring in high-pH soils and toxicities in low-pH, waterlogged soils.  Source: Brady & Weil (2017)." ;
    skos:inScheme glosis_cl:physioChemicalPropertyCode ;
    skos:notation "Mantot" ;
    skos:prefLabel "Manganese (Mn) - total"@en ;
    skos:topConceptOf glosis_cl:physioChemicalPropertyCode .

glosis_cl:physioChemicalPropertyCode-Mol a dbo:ChemicalCompound,
        dbo:ChemicalSubstance,
        glosis_cl:PhysioChemicalPropertyCode,
        skos:Concept ;
    dbo:pubchem "23932" ;
    rdfs:seeAlso <https://pubchem.ncbi.nlm.nih.gov/compound/23932> ;
    skos:definition "Molybdenum is a micronutrient essential for plant enzymes involved in nitrogen fixation and nitrate reduction. Deficiency, often observed in acidic soils, can lead to stunted growth and poor nitrogen utilization. Its availability increases with higher pH, making liming a common solution for molybdenum deficiencies. Source: Havlin et al. (2014)." ;
    skos:inScheme glosis_cl:physioChemicalPropertyCode ;
    skos:notation "Mol" ;
    skos:prefLabel "Molybdenum"@en ;
    skos:topConceptOf glosis_cl:physioChemicalPropertyCode .

glosis_cl:physioChemicalPropertyCode-Nit2 a dbo:ChemicalCompound,
        dbo:ChemicalSubstance,
        glosis_cl:PhysioChemicalPropertyCode,
        skos:Concept ;
    dbo:inchi "1S/HNO2/c2-1-3/h(H,2,3)/p-1" ;
    dbo:pubchem "946" ;
    dbprop:inchikey "IOVCWXUNBOPUCH-UHFFFAOYSA-M" ;
    rdfs:seeAlso <https://pubchem.ncbi.nlm.nih.gov/compound/946> ;
    skos:definition "Soluble Nitrite anions accumulated in the soil. A contributor to soil salinisation." ;
    skos:inScheme glosis_cl:physioChemicalPropertyCode ;
    skos:notation "Nit2" ;
    skos:prefLabel "Nitrite (NO2-) - soluble"@en ;
    skos:topConceptOf glosis_cl:physioChemicalPropertyCode .

glosis_cl:physioChemicalPropertyCode-Nit3 a dbo:ChemicalCompound,
        dbo:ChemicalSubstance,
        glosis_cl:PhysioChemicalPropertyCode,
        skos:Concept ;
    dbo:inchi "1S/NO3/c2-1(3)4/q-1" ;
    dbo:pubchem "943" ;
    dbprop:inchikey "NHNBFGGVMKEFGY-UHFFFAOYSA-N" ;
    rdfs:seeAlso <https://pubchem.ncbi.nlm.nih.gov/compound/943> ;
    skos:definition "Soluble Nitrate anions accumulated in the soil. A contributor to soil salinisation." ;
    skos:inScheme glosis_cl:physioChemicalPropertyCode ;
    skos:notation "Nit3" ;
    skos:prefLabel "Nitrate (NO3-) - soluble"@en ;
    skos:topConceptOf glosis_cl:physioChemicalPropertyCode .

glosis_cl:physioChemicalPropertyCode-Nittot a dbo:ChemicalCompound,
        dbo:ChemicalSubstance,
        glosis_cl:PhysioChemicalPropertyCode,
        skos:Concept ;
    dbo:inchi "1S/N2/c1-2" ;
    dbo:pubchem "947" ;
    dbprop:inchikey "IJGRMHOSHXDMSA-UHFFFAOYSA-N" ;
    rdfs:seeAlso <https://pubchem.ncbi.nlm.nih.gov/compound/947> ;
    skos:definition "Total nitrogen encompasses all nitrogen forms in soil, including organic nitrogen in humus and inorganic nitrogen such as ammonium (NH₄⁺) and nitrate (NO₃⁻). Nitrogen is essential for plant growth, being a vital component of amino acids, proteins, and chlorophyll. Total nitrogen is a key indicator of soil fertility and its capacity to sustain long-term crop productivity. Source: Brady & Weil (2017)." ;
    skos:inScheme glosis_cl:physioChemicalPropertyCode ;
    skos:notation "Nittot" ;
    skos:prefLabel "Nitrogen (N) - total"@en ;
    skos:topConceptOf glosis_cl:physioChemicalPropertyCode .

glosis_cl:physioChemicalPropertyCode-Orgmat a glosis_cl:PhysioChemicalPropertyCode,
        skos:Concept ;
    skos:definition "Soil organic matter is composed of decomposed plant and animal residues, living soil organisms, and humus. It improves soil structure, water retention, nutrient supply, and microbial activity, making it critical for sustainable agriculture and soil health. Source: Brady & Weil (2017)." ;
    skos:inScheme glosis_cl:physioChemicalPropertyCode ;
    skos:notation "Orgmat" ;
    skos:prefLabel "Organic matter"@en ;
    skos:topConceptOf glosis_cl:physioChemicalPropertyCode .

glosis_cl:physioChemicalPropertyCode-Pho a dbo:ChemicalCompound,
        dbo:ChemicalSubstance,
        glosis_cl:PhysioChemicalPropertyCode,
        skos:Concept ;
    dbo:inchi "1S/H3O4P/c1-5(2,3)4/h(H3,1,2,3,4)/p-3" ;
    dbo:pubchem "1061" ;
    dbprop:inchikey "NBIIXXVUZAFLBC-UHFFFAOYSA-K" ;
    rdfs:seeAlso <https://pubchem.ncbi.nlm.nih.gov/compound/1061> ;
    skos:definition "Soluble Phosphate anions accumulated in the soil. A contributor to soil salinisation." ;
    skos:inScheme glosis_cl:physioChemicalPropertyCode ;
    skos:notation "Pho" ;
    skos:prefLabel "Phosphate (PO4---) - soluble"@en ;
    skos:topConceptOf glosis_cl:physioChemicalPropertyCode .

glosis_cl:physioChemicalPropertyCode-Phoext a dbo:ChemicalCompound,
        dbo:ChemicalSubstance,
        glosis_cl:PhysioChemicalPropertyCode,
        skos:Concept ;
    dbo:inchi "1S/P" ;
    dbo:pubchem "5462309" ;
    dbprop:inchikey "OAICVXFJPJFONN-UHFFFAOYSA-N" ;
    rdfs:seeAlso <https://pubchem.ncbi.nlm.nih.gov/compound/5462309> ;
    skos:definition "Phosphorus bound to the soil matrix but that can be released into the soil solution (i.e. become bio-available)" ;
    skos:inScheme glosis_cl:physioChemicalPropertyCode ;
    skos:notation "Phoext" ;
    skos:prefLabel "Phosphorus (P) - extractable"@en ;
    skos:topConceptOf glosis_cl:physioChemicalPropertyCode .

glosis_cl:physioChemicalPropertyCode-Phooxa a dbo:ChemicalCompound,
        dbo:ChemicalSubstance,
        glosis_cl:PhysioChemicalPropertyCode,
        skos:Concept ;
    dbo:inchi "1S/P" ;
    dbo:pubchem "5462309" ;
    dbprop:inchikey "OAICVXFJPJFONN-UHFFFAOYSA-N" ;
    rdfs:seeAlso <https://pubchem.ncbi.nlm.nih.gov/compound/5462309> ;
    skos:definition "'Active' phosphorus content extracted from amorphous phosphorus compounds that are the products of the weathering of primary soil particles" ;
    skos:inScheme glosis_cl:physioChemicalPropertyCode ;
    skos:notation "Phooxa" ;
    skos:prefLabel "Phosphorus (P) - oxalate extractable"@en ;
    skos:topConceptOf glosis_cl:physioChemicalPropertyCode .

glosis_cl:physioChemicalPropertyCode-Phoret a dbo:ChemicalCompound,
        dbo:ChemicalSubstance,
        glosis_cl:PhysioChemicalPropertyCode,
        skos:Concept ;
    dbo:inchi "1S/P" ;
    dbo:pubchem "5462309" ;
    dbprop:inchikey "OAICVXFJPJFONN-UHFFFAOYSA-N" ;
    rdfs:seeAlso <https://pubchem.ncbi.nlm.nih.gov/compound/5462309> ;
    skos:definition "Phosphorus retention measures a soil's capacity to adsorb and hold phosphorus, influenced by soil texture, pH, and mineralogy. While high retention reduces leaching, it may also limit phosphorus availability to plants. Understanding phosphorus retention helps optimize fertilization and minimize environmental impacts. Source: Brady & Weil (2017)." ;
    skos:inScheme glosis_cl:physioChemicalPropertyCode ;
    skos:notation "Phoret" ;
    skos:prefLabel "Phosphorus (P) - retention"@en ;
    skos:topConceptOf glosis_cl:physioChemicalPropertyCode .

glosis_cl:physioChemicalPropertyCode-Photot a dbo:ChemicalCompound,
        dbo:ChemicalSubstance,
        glosis_cl:PhysioChemicalPropertyCode,
        skos:Concept ;
    dbo:inchi "1S/P" ;
    dbo:pubchem "5462309" ;
    dbprop:inchikey "OAICVXFJPJFONN-UHFFFAOYSA-N" ;
    rdfs:seeAlso <https://pubchem.ncbi.nlm.nih.gov/compound/5462309> ;
    skos:definition "Total phosphorus includes all forms of phosphorus in the soil, both organic and inorganic. While only a fraction is plant-available, total phosphorus serves as a long-term reserve for crop nutrition. Adequate phosphorus levels are crucial for energy transfer, photosynthesis, and root development in plants. Source: Soil Chemistry by Bohn et al." ;
    skos:inScheme glosis_cl:physioChemicalPropertyCode ;
    skos:notation "Photot" ;
    skos:prefLabel "Phosphorus (P) - total"@en ;
    skos:topConceptOf glosis_cl:physioChemicalPropertyCode .

glosis_cl:physioChemicalPropertyCode-Por a glosis_cl:PhysioChemicalPropertyCode,
        skos:Concept ;
    skos:definition "Porosity refers to the percentage of soil volume occupied by pores or voids, which hold air and water. It directly impacts water infiltration, drainage, and root growth. Soils with high porosity are better suited for crop cultivation, as they provide good aeration and water availability. Source: Brady & Weil (2017)." ;
    skos:inScheme glosis_cl:physioChemicalPropertyCode ;
    skos:notation "Por" ;
    skos:prefLabel "Porosity"@en ;
    skos:topConceptOf glosis_cl:physioChemicalPropertyCode .

glosis_cl:physioChemicalPropertyCode-Potexc a dbo:ChemicalCompound,
        dbo:ChemicalSubstance,
        glosis_cl:PhysioChemicalPropertyCode,
        skos:Concept ;
    dbo:inchi "1S/K/q+1" ;
    dbo:pubchem "813" ;
    dbprop:inchikey "NPYPAHLBTDXSSS-UHFFFAOYSA-N" ;
    rdfs:seeAlso <https://pubchem.ncbi.nlm.nih.gov/compound/813> ;
    skos:definition "Potassium bound to exchange surfaces in the soil such as clay minerals and organic matter that can be released to the soil solution upon exchange" ;
    skos:inScheme glosis_cl:physioChemicalPropertyCode ;
    skos:notation "Potexc" ;
    skos:prefLabel "Potassium (K+) - exchangeable"@en ;
    skos:topConceptOf glosis_cl:physioChemicalPropertyCode .

glosis_cl:physioChemicalPropertyCode-Potext a dbo:ChemicalCompound,
        dbo:ChemicalSubstance,
        glosis_cl:PhysioChemicalPropertyCode,
        skos:Concept ;
    dbo:inchi "1S/K" ;
    dbo:pubchem "5462222" ;
    dbprop:inchikey "ZLMJMSJWJFRBEC-UHFFFAOYSA-N" ;
    rdfs:seeAlso <https://pubchem.ncbi.nlm.nih.gov/compound/5462222> ;
    skos:definition "Potassium bound to the soil matrix but that can be released into the soil solution (i.e. become bio-available)" ;
    skos:inScheme glosis_cl:physioChemicalPropertyCode ;
    skos:notation "Potext" ;
    skos:prefLabel "Potassium (K) - extractable"@en ;
    skos:topConceptOf glosis_cl:physioChemicalPropertyCode .

glosis_cl:physioChemicalPropertyCode-Potsol a dbo:ChemicalCompound,
        dbo:ChemicalSubstance,
        glosis_cl:PhysioChemicalPropertyCode,
        skos:Concept ;
    dbo:inchi "1S/K/q+1" ;
    dbo:pubchem "813" ;
    dbprop:inchikey "NPYPAHLBTDXSSS-UHFFFAOYSA-N" ;
    rdfs:seeAlso <https://pubchem.ncbi.nlm.nih.gov/compound/813> ;
    skos:definition "Soluble Potassium cations accumulated in the soil. A contributor to soil salinisation." ;
    skos:inScheme glosis_cl:physioChemicalPropertyCode ;
    skos:notation "Potsol" ;
    skos:prefLabel "Potassium (K+) - soluble"@en ;
    skos:topConceptOf glosis_cl:physioChemicalPropertyCode .

glosis_cl:physioChemicalPropertyCode-Pottot a dbo:ChemicalCompound,
        dbo:ChemicalSubstance,
        glosis_cl:PhysioChemicalPropertyCode,
        skos:Concept ;
    dbo:inchi "1S/K" ;
    dbo:pubchem "5462222" ;
    dbprop:inchikey "ZLMJMSJWJFRBEC-UHFFFAOYSA-N" ;
    rdfs:seeAlso <https://pubchem.ncbi.nlm.nih.gov/compound/5462222> ;
    skos:definition "Total potassium includes all forms of potassium in soil, such as mineral-bound, exchangeable, and water-soluble potassium. It plays a vital role in plant growth by regulating water balance, enzyme activation, and photosynthesis. While only a fraction of total potassium is readily available to plants, it serves as a reserve to replenish exchangeable potassium over time. Adequate potassium levels improve crop yield, quality, and resistance to stress. Source: Soil Science Society of America." ;
    skos:inScheme glosis_cl:physioChemicalPropertyCode ;
    skos:notation "Pottot" ;
    skos:prefLabel "Potassium (K) - total"@en ;
    skos:topConceptOf glosis_cl:physioChemicalPropertyCode .

glosis_cl:physioChemicalPropertyCode-Selext a dbo:ChemicalCompound,
        dbo:ChemicalSubstance,
        glosis_cl:PhysioChemicalPropertyCode,
        skos:Concept ;
    dbo:inchi "1S/Se" ;
    dbo:pubchem "6326970" ;
    dbprop:inchikey "BUGBHKTXTAQXES-UHFFFAOYSA-N" ;
    rdfs:seeAlso <https://pubchem.ncbi.nlm.nih.gov/compound/6326970> ;
    skos:definition "Selenium bound to the soil matrix but that can be released into the soil solution (i.e. become bio-available)" ;
    skos:inScheme glosis_cl:physioChemicalPropertyCode ;
    skos:notation "Selext" ;
    skos:prefLabel "Selenium (Se) - extractable"@en ;
    skos:topConceptOf glosis_cl:physioChemicalPropertyCode .

glosis_cl:physioChemicalPropertyCode-Seltot a dbo:ChemicalCompound,
        dbo:ChemicalSubstance,
        glosis_cl:PhysioChemicalPropertyCode,
        skos:Concept ;
    dbo:inchi "1S/Se" ;
    dbo:pubchem "6326970" ;
    dbprop:inchikey "BUGBHKTXTAQXES-UHFFFAOYSA-N" ;
    rdfs:seeAlso <https://pubchem.ncbi.nlm.nih.gov/compound/6326970> ;
    skos:definition "Total selenium includes all selenium forms in soil, ranging from organic selenium in humus to inorganic selenium compounds. While trace amounts are essential for animal and human nutrition, excessive selenium can be toxic. Understanding selenium levels is critical for food safety and environmental management. Source: Sparks, D.L. (2003). Environmental Soil Chemistry." ;
    skos:inScheme glosis_cl:physioChemicalPropertyCode ;
    skos:notation "Seltot" ;
    skos:prefLabel "Selenium (Se) - total"@en ;
    skos:topConceptOf glosis_cl:physioChemicalPropertyCode .

glosis_cl:physioChemicalPropertyCode-Siloxa a dbo:ChemicalCompound,
        dbo:ChemicalSubstance,
        glosis_cl:PhysioChemicalPropertyCode,
        skos:Concept ;
    dbo:inchi "1S/Si" ;
    dbo:pubchem "5461123" ;
    dbprop:inchikey "XUIMIQQOPSSXEZ-UHFFFAOYSA-N" ;
    rdfs:seeAlso <https://pubchem.ncbi.nlm.nih.gov/compound/5461123> ;
    skos:definition "'Active' silicon content extracted from amorphous silicon compounds that are the products of the weathering of primary soil particles" ;
    skos:inScheme glosis_cl:physioChemicalPropertyCode ;
    skos:notation "Siloxa" ;
    skos:prefLabel "Silicon (Si) - oxalate extractable"@en ;
    skos:topConceptOf glosis_cl:physioChemicalPropertyCode .

glosis_cl:physioChemicalPropertyCode-Sodexc a dbo:ChemicalCompound,
        dbo:ChemicalSubstance,
        glosis_cl:PhysioChemicalPropertyCode,
        skos:Concept ;
    dbo:inchi "1S/Na/q+1" ;
    dbo:pubchem "923" ;
    dbprop:inchikey "FKNQFGJONOIPTF-UHFFFAOYSA-N" ;
    rdfs:seeAlso <https://pubchem.ncbi.nlm.nih.gov/compound/923> ;
    skos:definition "Exchangeable sodium percentage (ESP) measures the proportion of sodium ions in the cation exchange complex. High ESP levels (>15%) indicate sodic soils, which are prone to poor structure, reduced permeability, and nutrient imbalances. Management strategies include gypsum application and leaching. Source: USDA NRCS." ;
    skos:inScheme glosis_cl:physioChemicalPropertyCode ;
    skos:notation "Sodexc" ;
    skos:prefLabel "Sodium (Na+) - exchangeable %"@en ;
    skos:topConceptOf glosis_cl:physioChemicalPropertyCode .

glosis_cl:physioChemicalPropertyCode-Sodexp a dbo:ChemicalCompound,
        dbo:ChemicalSubstance,
        glosis_cl:PhysioChemicalPropertyCode,
        skos:Concept ;
    dbo:inchi "1S/Na/q+1" ;
    dbo:pubchem "923" ;
    dbprop:inchikey "FKNQFGJONOIPTF-UHFFFAOYSA-N" ;
    rdfs:seeAlso <https://pubchem.ncbi.nlm.nih.gov/compound/923> ;
    skos:definition "Sodium bound to exchange surfaces in the soil such as clay minerals and organic matter that can be released to the soil solution upon exchange" ;
    skos:inScheme glosis_cl:physioChemicalPropertyCode ;
    skos:notation "Sodexp" ;
    skos:prefLabel "Sodium (Na+) - exchangeable"@en ;
    skos:topConceptOf glosis_cl:physioChemicalPropertyCode .

glosis_cl:physioChemicalPropertyCode-Sodext a dbo:ChemicalCompound,
        dbo:ChemicalSubstance,
        glosis_cl:PhysioChemicalPropertyCode,
        skos:Concept ;
    dbo:inchi "1S/Na" ;
    dbo:pubchem "5360545" ;
    dbprop:inchikey "KEAYESYHFKHZAL-UHFFFAOYSA-N" ;
    rdfs:seeAlso <https://pubchem.ncbi.nlm.nih.gov/compound/5360545> ;
    skos:definition "Sodium bound to the soil matrix but that can be released into the soil solution (i.e. become bio-available)" ;
    skos:inScheme glosis_cl:physioChemicalPropertyCode ;
    skos:notation "Sodext" ;
    skos:prefLabel "Sodium (Na) - extractable"@en ;
    skos:topConceptOf glosis_cl:physioChemicalPropertyCode .

glosis_cl:physioChemicalPropertyCode-Sodsol a dbo:ChemicalCompound,
        dbo:ChemicalSubstance,
        glosis_cl:PhysioChemicalPropertyCode,
        skos:Concept ;
    dbo:inchi "1S/Na/q+1" ;
    dbo:pubchem "923" ;
    dbprop:inchikey "FKNQFGJONOIPTF-UHFFFAOYSA-N" ;
    rdfs:seeAlso <https://pubchem.ncbi.nlm.nih.gov/compound/923> ;
    skos:definition "Soluble Sodium cations accumulated in the soil. A contributor to soil salinisation." ;
    skos:inScheme glosis_cl:physioChemicalPropertyCode ;
    skos:notation "Sodsol" ;
    skos:prefLabel "Sodium (Na+) - soluble"@en ;
    skos:topConceptOf glosis_cl:physioChemicalPropertyCode .

glosis_cl:physioChemicalPropertyCode-Sodtot a dbo:ChemicalCompound,
        dbo:ChemicalSubstance,
        glosis_cl:PhysioChemicalPropertyCode,
        skos:Concept ;
    dbo:inchi "1S/Na" ;
    dbo:pubchem "5360545" ;
    dbprop:inchikey "KEAYESYHFKHZAL-UHFFFAOYSA-N" ;
    rdfs:seeAlso <https://pubchem.ncbi.nlm.nih.gov/compound/5360545> ;
    skos:definition "Total sodium includes all sodium present in soil, both soluble and bound. Excess sodium can lead to sodicity, which disrupts soil structure, reduces permeability, and impairs plant growth. Monitoring sodium levels is crucial for managing soil salinity in arid and irrigated regions. Source: Bohn, H.L., et al. (2001). Soil Chemistry." ;
    skos:inScheme glosis_cl:physioChemicalPropertyCode ;
    skos:notation "Sodtot" ;
    skos:prefLabel "Sodium (Na) - total"@en ;
    skos:topConceptOf glosis_cl:physioChemicalPropertyCode .

glosis_cl:physioChemicalPropertyCode-Solsal a glosis_cl:PhysioChemicalPropertyCode,
        skos:Concept ;
    skos:definition "Soluble salts refer to dissolved salts in the soil solution, primarily composed of sodium, calcium, magnesium, chloride, and sulfate ions. Excessive soluble salts cause salinity, which can impair plant water uptake and lead to osmotic stress. EC testing helps monitor salinity levels for effective management. Source: Soil Science Society of America." ;
    skos:inScheme glosis_cl:physioChemicalPropertyCode ;
    skos:notation "Solsal" ;
    skos:prefLabel "Soluble salts"@en ;
    skos:topConceptOf glosis_cl:physioChemicalPropertyCode .

glosis_cl:physioChemicalPropertyCode-Sul a dbo:ChemicalCompound,
        dbo:ChemicalSubstance,
        glosis_cl:PhysioChemicalPropertyCode,
        skos:Concept ;
    dbo:inchi "1S/H2O4S/c1-5(2,3)4/h(H2,1,2,3,4)/p-2" ;
    dbo:pubchem "1117" ;
    dbprop:inchikey "QAOWNCQODCNURD-UHFFFAOYSA-L" ;
    rdfs:seeAlso <https://pubchem.ncbi.nlm.nih.gov/compound/1117> ;
    skos:definition "Soluble Sulfate anions accumulated in the soil. A contributor to soil salinisation." ;
    skos:inScheme glosis_cl:physioChemicalPropertyCode ;
    skos:notation "Sul" ;
    skos:prefLabel "Sulfate (SO4--) - soluble"@en ;
    skos:topConceptOf glosis_cl:physioChemicalPropertyCode .

glosis_cl:physioChemicalPropertyCode-Sulext a dbo:ChemicalCompound,
        dbo:ChemicalSubstance,
        glosis_cl:PhysioChemicalPropertyCode,
        skos:Concept ;
    dbo:inchi "1S/S" ;
    dbo:pubchem "5362487" ;
    dbprop:inchikey "NINIDFKCEFEMDL-UHFFFAOYSA-N" ;
    rdfs:seeAlso <https://pubchem.ncbi.nlm.nih.gov/compound/5362487> ;
    skos:definition "Sulfur bound to the soil matrix but that can be released into the soil solution (i.e. become bio-available)" ;
    skos:inScheme glosis_cl:physioChemicalPropertyCode ;
    skos:notation "Sulext" ;
    skos:prefLabel "Sulfur (S) - extractable"@en ;
    skos:topConceptOf glosis_cl:physioChemicalPropertyCode .

glosis_cl:physioChemicalPropertyCode-Sultot a dbo:ChemicalCompound,
        dbo:ChemicalSubstance,
        glosis_cl:PhysioChemicalPropertyCode,
        skos:Concept ;
    dbo:inchi "1S/S" ;
    dbo:pubchem "5362487" ;
    dbprop:inchikey "NINIDFKCEFEMDL-UHFFFAOYSA-N" ;
    rdfs:seeAlso <https://pubchem.ncbi.nlm.nih.gov/compound/5362487> ;
    skos:definition "Total sulfur in soil includes both organic and inorganic forms, such as sulfates and sulfur in organic matter. Sulfur is essential for protein synthesis and enzyme functions in plants. Deficiency leads to stunted growth and yellowing of leaves. Total sulfur provides insight into the soil's potential to release plant-available sulfur over time, critical for sustaining crop health. Source: Havlin, J.L., et al. (2014). Soil Fertility and Fertilizers." ;
    skos:inScheme glosis_cl:physioChemicalPropertyCode ;
    skos:notation "Sultot" ;
    skos:prefLabel "Sulfur (S) - total"@en ;
    skos:topConceptOf glosis_cl:physioChemicalPropertyCode .

glosis_cl:physioChemicalPropertyCode-Zin a dbo:ChemicalCompound,
        dbo:ChemicalSubstance,
        glosis_cl:PhysioChemicalPropertyCode,
        skos:Concept ;
    dbo:inchi "1S/Zn" ;
    dbo:pubchem "23994" ;
    dbprop:inchikey "HCHKCACWOHOZIP-UHFFFAOYSA-N" ;
    rdfs:seeAlso <https://pubchem.ncbi.nlm.nih.gov/compound/23994> ;
    skos:definition "Zinc is a micronutrient essential for plant enzyme systems, protein synthesis, and growth regulation. Deficiency is common in calcareous soils and results in stunted growth and chlorosis. Zinc fertilizers or soil pH adjustments can address deficiencies. Source: Havlin et al. (2014)." ;
    skos:inScheme glosis_cl:physioChemicalPropertyCode ;
    skos:notation "Zin" ;
    skos:prefLabel "Zinc (Zn)"@en ;
    skos:topConceptOf glosis_cl:physioChemicalPropertyCode .

glosis_cl:physioChemicalPropertyCode-Zinext a dbo:ChemicalCompound,
        dbo:ChemicalSubstance,
        glosis_cl:PhysioChemicalPropertyCode,
        skos:Concept ;
    dbo:inchi "1S/Zn" ;
    dbo:pubchem "23994" ;
    dbprop:inchikey "HCHKCACWOHOZIP-UHFFFAOYSA-N" ;
    rdfs:seeAlso <https://pubchem.ncbi.nlm.nih.gov/compound/23994> ;
    skos:definition "Zinc bound to the soil matrix but that can be released into the soil solution (i.e. become bio-available)" ;
    skos:inScheme glosis_cl:physioChemicalPropertyCode ;
    skos:notation "Zinext" ;
    skos:prefLabel "Zinc (Zn) - extractable"@en ;
    skos:topConceptOf glosis_cl:physioChemicalPropertyCode .

glosis_cl:physioChemicalPropertyCode-pH a glosis_cl:PhysioChemicalPropertyCode,
        skos:Concept ;
    skos:definition "Soil pH measures the concentration of hydrogen ions (H⁺) in the soil solution, indicating its acidity or alkalinity on a scale from 1 to 14. Neutral soils have a pH of 7, while values below 7 are acidic and above are alkaline. Soil pH significantly affects nutrient availability, microbial activity, and plant growth. For instance, nutrients like phosphorus are most available in a pH range of 6 to 7. Lime or sulfur applications can adjust soil pH to optimize conditions for crops. Source: USDA Natural Resources Conservation Service (NRCS)." ;
    skos:inScheme glosis_cl:physioChemicalPropertyCode ;
    skos:notation "pH" ;
    skos:prefLabel "pH - Hydrogen potential"@en ;
    skos:topConceptOf glosis_cl:physioChemicalPropertyCode .

glosis_cl:physiographyValueCode-BOdl a glosis_cl:PhysiographyValueCode,
        skos:Concept ;
    skos:definition "Position in flat or almost flat terrain: Bottom (drainage line)" ;
    skos:inScheme glosis_cl:physiographyValueCode ;
    skos:notation "BOdl" ;
    skos:prefLabel "Bottom (drainage line)"@en ;
    skos:topConceptOf glosis_cl:physiographyValueCode .

glosis_cl:physiographyValueCode-BOf a glosis_cl:PhysiographyValueCode,
        skos:Concept ;
    skos:definition "Position in undulating to mountainous terrain: Bottom (flat)" ;
    skos:inScheme glosis_cl:physiographyValueCode ;
    skos:notation "BOf" ;
    skos:prefLabel "Bottom (flat)"@en ;
    skos:topConceptOf glosis_cl:physiographyValueCode .

glosis_cl:physiographyValueCode-CR a glosis_cl:PhysiographyValueCode,
        skos:Concept ;
    skos:definition "Position in undulating to mountainous terrain: Crest (summit)" ;
    skos:inScheme glosis_cl:physiographyValueCode ;
    skos:notation "CR" ;
    skos:prefLabel "Crest (summit)"@en ;
    skos:topConceptOf glosis_cl:physiographyValueCode .

glosis_cl:physiographyValueCode-HI a glosis_cl:PhysiographyValueCode,
        skos:Concept ;
    skos:definition "Position in flat or almost flat terrain: Higher part (rise)" ;
    skos:inScheme glosis_cl:physiographyValueCode ;
    skos:notation "HI" ;
    skos:prefLabel "Higher part (rise)"@en ;
    skos:topConceptOf glosis_cl:physiographyValueCode .

glosis_cl:physiographyValueCode-IN a glosis_cl:PhysiographyValueCode,
        skos:Concept ;
    skos:definition "Position in flat or almost flat terrain: Intermediate part (talf)" ;
    skos:inScheme glosis_cl:physiographyValueCode ;
    skos:notation "IN" ;
    skos:prefLabel "Intermediate part (talf)"@en ;
    skos:topConceptOf glosis_cl:physiographyValueCode .

glosis_cl:physiographyValueCode-LO a glosis_cl:PhysiographyValueCode,
        skos:Concept ;
    skos:definition "Position in flat or almost flat terrain: Lower part (and dip)" ;
    skos:inScheme glosis_cl:physiographyValueCode ;
    skos:notation "LO" ;
    skos:prefLabel "Lower part (and dip)"@en ;
    skos:topConceptOf glosis_cl:physiographyValueCode .

glosis_cl:physiographyValueCode-LS a glosis_cl:PhysiographyValueCode,
        skos:Concept ;
    skos:definition "Position in undulating to mountainous terrain: Lower slope (foot slope)" ;
    skos:inScheme glosis_cl:physiographyValueCode ;
    skos:notation "LS" ;
    skos:prefLabel "Lower slope (foot slope)"@en ;
    skos:topConceptOf glosis_cl:physiographyValueCode .

glosis_cl:physiographyValueCode-MS a glosis_cl:PhysiographyValueCode,
        skos:Concept ;
    skos:definition "Position in undulating to mountainous terrain: Middle slope (back slope)" ;
    skos:inScheme glosis_cl:physiographyValueCode ;
    skos:notation "MS" ;
    skos:prefLabel "Middle slope (back slope)"@en ;
    skos:topConceptOf glosis_cl:physiographyValueCode .

glosis_cl:physiographyValueCode-TS a glosis_cl:PhysiographyValueCode,
        skos:Concept ;
    skos:definition "Position in undulating to mountainous terrain: Toe slope" ;
    skos:inScheme glosis_cl:physiographyValueCode ;
    skos:notation "TS" ;
    skos:prefLabel "Toe slope"@en ;
    skos:topConceptOf glosis_cl:physiographyValueCode .

glosis_cl:physiographyValueCode-UP a glosis_cl:PhysiographyValueCode,
        skos:Concept ;
    skos:definition "Position in undulating to mountainous terrain: Upper slope (shoulder)" ;
    skos:inScheme glosis_cl:physiographyValueCode ;
    skos:notation "UP" ;
    skos:prefLabel "Upper slope (shoulder)"@en ;
    skos:topConceptOf glosis_cl:physiographyValueCode .

glosis_cl:plasticityValueCode-NPL a glosis_cl:PlasticityValueCode,
        skos:Concept ;
    skos:definition "No wire is formable." ;
    skos:inScheme glosis_cl:plasticityValueCode ;
    skos:notation "NPL" ;
    skos:prefLabel "Non-plastic"@en ;
    skos:topConceptOf glosis_cl:plasticityValueCode .

glosis_cl:plasticityValueCode-PL a glosis_cl:PlasticityValueCode,
        skos:Concept ;
    skos:definition "Wire formable but breaks if bent into a ring; slight to moderate force required for deformation of the soil mass." ;
    skos:inScheme glosis_cl:plasticityValueCode ;
    skos:notation "PL" ;
    skos:prefLabel "Plastic"@en ;
    skos:topConceptOf glosis_cl:plasticityValueCode .

glosis_cl:plasticityValueCode-PVP a glosis_cl:PlasticityValueCode,
        skos:Concept ;
    skos:definition "Additioanl plasticity code with combination of  PL and VPL" ;
    skos:inScheme glosis_cl:plasticityValueCode ;
    skos:notation "PVP" ;
    skos:prefLabel "plastic to very plastic"@en ;
    skos:topConceptOf glosis_cl:plasticityValueCode .

glosis_cl:plasticityValueCode-SPL a glosis_cl:PlasticityValueCode,
        skos:Concept ;
    skos:definition "Wire formable but breaks immediately if bent into a ring; soil mass deformed by very slight force." ;
    skos:inScheme glosis_cl:plasticityValueCode ;
    skos:notation "SPL" ;
    skos:prefLabel "Slightly plastic"@en ;
    skos:topConceptOf glosis_cl:plasticityValueCode .

glosis_cl:plasticityValueCode-SPP a glosis_cl:PlasticityValueCode,
        skos:Concept ;
    skos:definition "Additioanl plasticity code with combination of  SPL and PL" ;
    skos:inScheme glosis_cl:plasticityValueCode ;
    skos:notation "SPP" ;
    skos:prefLabel "slightly plastic to plastic"@en ;
    skos:topConceptOf glosis_cl:plasticityValueCode .

glosis_cl:plasticityValueCode-VPL a glosis_cl:PlasticityValueCode,
        skos:Concept ;
    skos:definition "Wire formable and can be bent into a ring; moderately strong to very strong force required for deformation of the soil mass." ;
    skos:inScheme glosis_cl:plasticityValueCode ;
    skos:notation "VPL" ;
    skos:prefLabel "Very plastic"@en ;
    skos:topConceptOf glosis_cl:plasticityValueCode .

glosis_cl:poresAbundanceValueCode-C a glosis_cl:PoresAbundanceValueCode,
        skos:Concept ;
    skos:definition "< 2 mm (number)50–200 ;> 2 mm (number)5–20" ;
    skos:inScheme glosis_cl:poresAbundanceValueCode ;
    skos:notation "C" ;
    skos:prefLabel "Common"@en ;
    skos:topConceptOf glosis_cl:poresAbundanceValueCode .

glosis_cl:poresAbundanceValueCode-F a glosis_cl:PoresAbundanceValueCode,
        skos:Concept ;
    skos:definition "< 2 mm (number)20–50;> 2 mm (number) 2–5" ;
    skos:inScheme glosis_cl:poresAbundanceValueCode ;
    skos:notation "F" ;
    skos:prefLabel "Few"@en ;
    skos:topConceptOf glosis_cl:poresAbundanceValueCode .

glosis_cl:poresAbundanceValueCode-M a glosis_cl:PoresAbundanceValueCode,
        skos:Concept ;
    skos:definition "< 2 mm (number)> 200 ;> 2 mm (number)> 20" ;
    skos:inScheme glosis_cl:poresAbundanceValueCode ;
    skos:notation "M" ;
    skos:prefLabel "Many"@en ;
    skos:topConceptOf glosis_cl:poresAbundanceValueCode .

glosis_cl:poresAbundanceValueCode-N a glosis_cl:PoresAbundanceValueCode,
        skos:Concept ;
    skos:definition "< 2 mm (number)0;> 2 mm (number)0" ;
    skos:inScheme glosis_cl:poresAbundanceValueCode ;
    skos:notation "N" ;
    skos:prefLabel "None"@en ;
    skos:topConceptOf glosis_cl:poresAbundanceValueCode .

glosis_cl:poresAbundanceValueCode-V a glosis_cl:PoresAbundanceValueCode,
        skos:Concept ;
    skos:definition "< 2 mm (number)1–20 ;> 2 mm (number)1–2" ;
    skos:inScheme glosis_cl:poresAbundanceValueCode ;
    skos:notation "V" ;
    skos:prefLabel "Very few"@en ;
    skos:topConceptOf glosis_cl:poresAbundanceValueCode .

glosis_cl:porosityClassValueCode-1 a glosis_cl:PorosityClassValueCode,
        skos:Concept ;
    skos:definition "Very low porosity of les than 2%" ;
    skos:inScheme glosis_cl:porosityClassValueCode ;
    skos:notation "1" ;
    skos:prefLabel "Very low"@en ;
    skos:topConceptOf glosis_cl:porosityClassValueCode .

glosis_cl:porosityClassValueCode-2 a glosis_cl:PorosityClassValueCode,
        skos:Concept ;
    skos:definition "Low porosity of 2–5%" ;
    skos:inScheme glosis_cl:porosityClassValueCode ;
    skos:notation "2" ;
    skos:prefLabel "Low"@en ;
    skos:topConceptOf glosis_cl:porosityClassValueCode .

glosis_cl:porosityClassValueCode-3 a glosis_cl:PorosityClassValueCode,
        skos:Concept ;
    skos:definition "Medium porosity of 5–15%" ;
    skos:inScheme glosis_cl:porosityClassValueCode ;
    skos:notation "3" ;
    skos:prefLabel "Medium"@en ;
    skos:topConceptOf glosis_cl:porosityClassValueCode .

glosis_cl:porosityClassValueCode-4 a glosis_cl:PorosityClassValueCode,
        skos:Concept ;
    skos:definition "High porosity of 15–40%" ;
    skos:inScheme glosis_cl:porosityClassValueCode ;
    skos:notation "4" ;
    skos:prefLabel "High"@en ;
    skos:topConceptOf glosis_cl:porosityClassValueCode .

glosis_cl:porosityClassValueCode-5 a glosis_cl:PorosityClassValueCode,
        skos:Concept ;
    skos:definition "Very high porosity of more than 40%" ;
    skos:inScheme glosis_cl:porosityClassValueCode ;
    skos:notation "5" ;
    skos:prefLabel "Very high"@en ;
    skos:topConceptOf glosis_cl:porosityClassValueCode .

glosis_cl:profileDescriptionStatusValueCode-1 a glosis_cl:ProfileDescriptionStatusValueCode,
        skos:Concept ;
    skos:definition "No essential elements or details are missing from the description, sampling or analysis. The accuracy and reliability of the description and analytical results permit the full characterization of all soil horizons to a depth of 125 cm, or more if required for classification, or down to a C or R horizon or layer, which may be shallower." ;
    skos:inScheme glosis_cl:profileDescriptionStatusValueCode ;
    skos:narrower glosis_cl:profileDescriptionStatusValueCode-1.1 ;
    skos:notation "1" ;
    skos:prefLabel "Reference profile description"@en ;
    skos:topConceptOf glosis_cl:profileDescriptionStatusValueCode .

glosis_cl:profileDescriptionStatusValueCode-1.1 a glosis_cl:ProfileDescriptionStatusValueCode,
        skos:Concept ;
    skos:broader glosis_cl:profileDescriptionStatusValueCode-1 ;
    skos:definition "If soil description is done without sampling." ;
    skos:inScheme glosis_cl:profileDescriptionStatusValueCode ;
    skos:notation "1.1" ;
    skos:prefLabel "Reference profile description - no sampling"@en .

glosis_cl:profileDescriptionStatusValueCode-2 a glosis_cl:ProfileDescriptionStatusValueCode,
        skos:Concept ;
    skos:definition "No essential elements are missing from the description, sampling or analysis. The number of samples collected is sufficient to characterize all major soil horizons, but may not allow precise definition of all subhorizons, especially in the deeper soil. The profile depth is 80 cm or more, or down to a C or R horizon or layer, which may be shallower. Additional augering and sampling may be required for lower level classification." ;
    skos:inScheme glosis_cl:profileDescriptionStatusValueCode ;
    skos:narrower glosis_cl:profileDescriptionStatusValueCode-2.1 ;
    skos:notation "2" ;
    skos:prefLabel "Routine profile description"@en ;
    skos:topConceptOf glosis_cl:profileDescriptionStatusValueCode .

glosis_cl:profileDescriptionStatusValueCode-2.1 a glosis_cl:ProfileDescriptionStatusValueCode,
        skos:Concept ;
    skos:broader glosis_cl:profileDescriptionStatusValueCode-2 ;
    skos:definition "If soil description is done without sampling." ;
    skos:inScheme glosis_cl:profileDescriptionStatusValueCode ;
    skos:notation "2.1" ;
    skos:prefLabel "Routine profile description - no sampling"@en .

glosis_cl:profileDescriptionStatusValueCode-3 a glosis_cl:ProfileDescriptionStatusValueCode,
        skos:Concept ;
    skos:definition "Certain relevant elements are missing from the description, an insufficient number of samples was collected, or the reliability of the analytical data does not permit a complete characterization of the soil. However, the description is useful for specific purposes and provides a satisfactory indication of the nature of the soil at high levels of soil taxonomic classification." ;
    skos:inScheme glosis_cl:profileDescriptionStatusValueCode ;
    skos:narrower glosis_cl:profileDescriptionStatusValueCode-3.1 ;
    skos:notation "3" ;
    skos:prefLabel "Incomplete description"@en ;
    skos:topConceptOf glosis_cl:profileDescriptionStatusValueCode .

glosis_cl:profileDescriptionStatusValueCode-3.1 a glosis_cl:ProfileDescriptionStatusValueCode,
        skos:Concept ;
    skos:broader glosis_cl:profileDescriptionStatusValueCode-3 ;
    skos:definition "If soil description is done without sampling." ;
    skos:inScheme glosis_cl:profileDescriptionStatusValueCode ;
    skos:notation "3.1" ;
    skos:prefLabel "Incomplete description - no sampling"@en .

glosis_cl:profileDescriptionStatusValueCode-4 a glosis_cl:ProfileDescriptionStatusValueCode,
        skos:Concept ;
    skos:definition "Soil augerings do no permit a comprehensive soil profile description. Augerings are made for routine soil observation and identification in soil mapping, and for that purpose normally provide a satisfactory indication of the soil characteristics. Soil samples may be collected from augerings." ;
    skos:inScheme glosis_cl:profileDescriptionStatusValueCode ;
    skos:narrower glosis_cl:profileDescriptionStatusValueCode-4.1 ;
    skos:notation "4" ;
    skos:prefLabel "Soil augering description"@en ;
    skos:topConceptOf glosis_cl:profileDescriptionStatusValueCode .

glosis_cl:profileDescriptionStatusValueCode-4.1 a glosis_cl:ProfileDescriptionStatusValueCode,
        skos:Concept ;
    skos:broader glosis_cl:profileDescriptionStatusValueCode-4 ;
    skos:definition "If soil description is done without sampling." ;
    skos:inScheme glosis_cl:profileDescriptionStatusValueCode ;
    skos:notation "4.1" ;
    skos:prefLabel "Soil augering description - no sampling"@en .

glosis_cl:profileDescriptionStatusValueCode-5 a glosis_cl:ProfileDescriptionStatusValueCode,
        skos:Concept ;
    skos:definition "Essential elements are missing from the description, preventing a satisfactory soil characterization and classification." ;
    skos:inScheme glosis_cl:profileDescriptionStatusValueCode ;
    skos:notation "5" ;
    skos:prefLabel "Other descriptions"@en ;
    skos:topConceptOf glosis_cl:profileDescriptionStatusValueCode .

glosis_cl:rockAbundanceValueCode-A a glosis_cl:RockAbundanceValueCode,
        skos:Concept ;
    skos:definition "40%–80% of rock fragments" ;
    skos:inScheme glosis_cl:rockAbundanceValueCode ;
    skos:notation "A" ;
    skos:prefLabel "Abundant"@en ;
    skos:topConceptOf glosis_cl:rockAbundanceValueCode .

glosis_cl:rockAbundanceValueCode-C a glosis_cl:RockAbundanceValueCode,
        skos:Concept ;
    skos:definition "5%–15% of rock fragments" ;
    skos:inScheme glosis_cl:rockAbundanceValueCode ;
    skos:notation "C" ;
    skos:prefLabel "Common"@en ;
    skos:topConceptOf glosis_cl:rockAbundanceValueCode .

glosis_cl:rockAbundanceValueCode-D a glosis_cl:RockAbundanceValueCode,
        skos:Concept ;
    skos:definition "> 80% of rock fragments" ;
    skos:inScheme glosis_cl:rockAbundanceValueCode ;
    skos:notation "D" ;
    skos:prefLabel "Dominant"@en ;
    skos:topConceptOf glosis_cl:rockAbundanceValueCode .

glosis_cl:rockAbundanceValueCode-F a glosis_cl:RockAbundanceValueCode,
        skos:Concept ;
    skos:definition "2%–5% of rock fragments" ;
    skos:inScheme glosis_cl:rockAbundanceValueCode ;
    skos:notation "F" ;
    skos:prefLabel "Few"@en ;
    skos:topConceptOf glosis_cl:rockAbundanceValueCode .

glosis_cl:rockAbundanceValueCode-M a glosis_cl:RockAbundanceValueCode,
        skos:Concept ;
    skos:definition "15%–40% of rock fragments" ;
    skos:inScheme glosis_cl:rockAbundanceValueCode ;
    skos:notation "M" ;
    skos:prefLabel "Many"@en ;
    skos:topConceptOf glosis_cl:rockAbundanceValueCode .

glosis_cl:rockAbundanceValueCode-N a glosis_cl:RockAbundanceValueCode,
        skos:Concept ;
    skos:definition "0% of rock fragments" ;
    skos:inScheme glosis_cl:rockAbundanceValueCode ;
    skos:notation "N" ;
    skos:prefLabel "None"@en ;
    skos:topConceptOf glosis_cl:rockAbundanceValueCode .

glosis_cl:rockAbundanceValueCode-S a glosis_cl:RockAbundanceValueCode,
        skos:Concept ;
    skos:definition "any content, but concentrated at a distinct depth of a horizon" ;
    skos:inScheme glosis_cl:rockAbundanceValueCode ;
    skos:notation "S" ;
    skos:prefLabel "Stone line"@en ;
    skos:topConceptOf glosis_cl:rockAbundanceValueCode .

glosis_cl:rockAbundanceValueCode-V a glosis_cl:RockAbundanceValueCode,
        skos:Concept ;
    skos:definition "0%–2% of rock fragments" ;
    skos:inScheme glosis_cl:rockAbundanceValueCode ;
    skos:notation "V" ;
    skos:prefLabel "Very few"@en ;
    skos:topConceptOf glosis_cl:rockAbundanceValueCode .

glosis_cl:rockOutcropsCoverValueCode-A a glosis_cl:RockOutcropsCoverValueCode,
        skos:Concept ;
    skos:definition "Rock outcorps of 40–80% with distance between rockcorps less than 2 m" ;
    skos:inScheme glosis_cl:rockOutcropsCoverValueCode ;
    skos:notation "M" ;
    skos:prefLabel "Abundant"@en ;
    skos:topConceptOf glosis_cl:rockOutcropsCoverValueCode .

glosis_cl:rockOutcropsCoverValueCode-C a glosis_cl:RockOutcropsCoverValueCode,
        skos:Concept ;
    skos:definition "Rock outcorps of 5–15% with distance between rockcorps 5–20 m" ;
    skos:inScheme glosis_cl:rockOutcropsCoverValueCode ;
    skos:notation "C" ;
    skos:prefLabel "Common"@en ;
    skos:topConceptOf glosis_cl:rockOutcropsCoverValueCode .

glosis_cl:rockOutcropsCoverValueCode-D a glosis_cl:RockOutcropsCoverValueCode,
        skos:Concept ;
    skos:definition "Rock outcorps of more than 80%" ;
    skos:inScheme glosis_cl:rockOutcropsCoverValueCode ;
    skos:notation "D" ;
    skos:prefLabel "Dominant"@en ;
    skos:topConceptOf glosis_cl:rockOutcropsCoverValueCode .

glosis_cl:rockOutcropsCoverValueCode-F a glosis_cl:RockOutcropsCoverValueCode,
        skos:Concept ;
    skos:definition "Rock outcorps of 2–5 % with distance between rockcorps 20–50 m" ;
    skos:inScheme glosis_cl:rockOutcropsCoverValueCode ;
    skos:notation "F" ;
    skos:prefLabel "Few"@en ;
    skos:topConceptOf glosis_cl:rockOutcropsCoverValueCode .

glosis_cl:rockOutcropsCoverValueCode-M a glosis_cl:RockOutcropsCoverValueCode,
        skos:Concept ;
    skos:definition "Rock outcorps of 15–40 % with distance between rockcorps 2–5 m" ;
    skos:inScheme glosis_cl:rockOutcropsCoverValueCode ;
    skos:notation "M" ;
    skos:prefLabel "Many"@en ;
    skos:topConceptOf glosis_cl:rockOutcropsCoverValueCode .

glosis_cl:rockOutcropsCoverValueCode-N a glosis_cl:RockOutcropsCoverValueCode,
        skos:Concept ;
    skos:definition "No rock outcorps on surface" ;
    skos:inScheme glosis_cl:rockOutcropsCoverValueCode ;
    skos:notation "N" ;
    skos:prefLabel "None"@en ;
    skos:topConceptOf glosis_cl:rockOutcropsCoverValueCode .

glosis_cl:rockOutcropsCoverValueCode-V a glosis_cl:RockOutcropsCoverValueCode,
        skos:Concept ;
    skos:definition "Rock outcorps of 0–2 % with distance between rockcorps greater than 50 m" ;
    skos:inScheme glosis_cl:rockOutcropsCoverValueCode ;
    skos:notation "V" ;
    skos:prefLabel "Very few"@en ;
    skos:topConceptOf glosis_cl:rockOutcropsCoverValueCode .

glosis_cl:rockOutcropsDistanceValueCode-1 a glosis_cl:RockOutcropsDistanceValueCode,
        skos:Concept ;
    skos:definition "Distance between rock outcrops is more than 50m: >50m" ;
    skos:inScheme glosis_cl:rockOutcropsDistanceValueCode ;
    skos:notation "1" ;
    skos:prefLabel "More than 50m"@en ;
    skos:topConceptOf glosis_cl:rockOutcropsDistanceValueCode .

glosis_cl:rockOutcropsDistanceValueCode-2 a glosis_cl:RockOutcropsDistanceValueCode,
        skos:Concept ;
    skos:definition "Distance between rock outcrops between 20 and 50 m" ;
    skos:inScheme glosis_cl:rockOutcropsDistanceValueCode ;
    skos:notation "2" ;
    skos:prefLabel "Between 20m and 50m"@en ;
    skos:topConceptOf glosis_cl:rockOutcropsDistanceValueCode .

glosis_cl:rockOutcropsDistanceValueCode-3 a glosis_cl:RockOutcropsDistanceValueCode,
        skos:Concept ;
    skos:definition "Distance between rock outcrops between 5 and 20 m" ;
    skos:inScheme glosis_cl:rockOutcropsDistanceValueCode ;
    skos:notation "3" ;
    skos:prefLabel "Between 5m and 20m"@en ;
    skos:topConceptOf glosis_cl:rockOutcropsDistanceValueCode .

glosis_cl:rockOutcropsDistanceValueCode-4 a glosis_cl:RockOutcropsDistanceValueCode,
        skos:Concept ;
    skos:definition "Distance between rock outcrops between 2 and 5 m" ;
    skos:inScheme glosis_cl:rockOutcropsDistanceValueCode ;
    skos:notation "4" ;
    skos:prefLabel "Between 2m and 5m"@en ;
    skos:topConceptOf glosis_cl:rockOutcropsDistanceValueCode .

glosis_cl:rockOutcropsDistanceValueCode-5 a glosis_cl:RockOutcropsDistanceValueCode,
        skos:Concept ;
    skos:definition "Distance between rock outcrops is less than 2m: < 2" ;
    skos:inScheme glosis_cl:rockOutcropsDistanceValueCode ;
    skos:notation "5" ;
    skos:prefLabel "Less than 2"@en ;
    skos:topConceptOf glosis_cl:rockOutcropsDistanceValueCode .

glosis_cl:rockShapeValueCode-A a glosis_cl:RockShapeValueCode,
        skos:Concept ;
    skos:definition "Angular rock shape" ;
    skos:inScheme glosis_cl:rockShapeValueCode ;
    skos:notation "A" ;
    skos:prefLabel "Angular"@en ;
    skos:topConceptOf glosis_cl:rockShapeValueCode .

glosis_cl:rockShapeValueCode-F a glosis_cl:RockShapeValueCode,
        skos:Concept ;
    skos:definition "Flat rock shape" ;
    skos:inScheme glosis_cl:rockShapeValueCode ;
    skos:notation "F" ;
    skos:prefLabel "Flat"@en ;
    skos:topConceptOf glosis_cl:rockShapeValueCode .

glosis_cl:rockShapeValueCode-R a glosis_cl:RockShapeValueCode,
        skos:Concept ;
    skos:definition "Rounded rock shape" ;
    skos:inScheme glosis_cl:rockShapeValueCode ;
    skos:notation "R" ;
    skos:prefLabel "Rounded"@en ;
    skos:topConceptOf glosis_cl:rockShapeValueCode .

glosis_cl:rockShapeValueCode-S a glosis_cl:RockShapeValueCode,
        skos:Concept ;
    skos:definition "Subrounded rock shape" ;
    skos:inScheme glosis_cl:rockShapeValueCode ;
    skos:notation "S" ;
    skos:prefLabel "Subrounded"@en ;
    skos:topConceptOf glosis_cl:rockShapeValueCode .

glosis_cl:rockSizeValueCode-A a glosis_cl:RockSizeValueCode,
        skos:Concept ;
    skos:definition "Aretfacts in soil measured in (mm)" ;
    skos:inScheme glosis_cl:rockSizeValueCode ;
    skos:narrower glosis_cl:rockSizeValueCode-AC,
        glosis_cl:rockSizeValueCode-AF,
        glosis_cl:rockSizeValueCode-AM,
        glosis_cl:rockSizeValueCode-AV ;
    skos:notation "A" ;
    skos:prefLabel "Artefacts"@en ;
    skos:topConceptOf glosis_cl:rockSizeValueCode .

glosis_cl:rockSizeValueCode-AC a glosis_cl:RockSizeValueCode,
        skos:Concept ;
    skos:broader glosis_cl:rockSizeValueCode-A ;
    skos:definition "Coarse artefacts in soil greater than 20mm" ;
    skos:inScheme glosis_cl:rockSizeValueCode ;
    skos:notation "AC" ;
    skos:prefLabel "Coarse artefacts"@en .

glosis_cl:rockSizeValueCode-AF a glosis_cl:RockSizeValueCode,
        skos:Concept ;
    skos:broader glosis_cl:rockSizeValueCode-A ;
    skos:definition "Fine artefacts in soild of size between 2mm–6mm" ;
    skos:inScheme glosis_cl:rockSizeValueCode ;
    skos:notation "AF" ;
    skos:prefLabel "Fine artefacts"@en .

glosis_cl:rockSizeValueCode-AM a glosis_cl:RockSizeValueCode,
        skos:Concept ;
    skos:broader glosis_cl:rockSizeValueCode-A ;
    skos:definition "6mm–20mm" ;
    skos:inScheme glosis_cl:rockSizeValueCode ;
    skos:notation "AM" ;
    skos:prefLabel "Medium artefacts"@en .

glosis_cl:rockSizeValueCode-AV a glosis_cl:RockSizeValueCode,
        skos:Concept ;
    skos:broader glosis_cl:rockSizeValueCode-A ;
    skos:definition "Very fine artefacsts in soil of size < 2mm" ;
    skos:inScheme glosis_cl:rockSizeValueCode ;
    skos:notation "AV" ;
    skos:prefLabel "Very fine artefacts"@en .

glosis_cl:rockSizeValueCode-BL a glosis_cl:RockSizeValueCode,
        skos:Concept ;
    skos:broader glosis_cl:rockSizeValueCode-C ;
    skos:definition "Combination of boulderds and large boulders" ;
    skos:inScheme glosis_cl:rockSizeValueCode ;
    skos:notation "BL" ;
    skos:prefLabel "Boulders and large boulders"@en .

glosis_cl:rockSizeValueCode-C a glosis_cl:RockSizeValueCode,
        skos:Concept ;
    skos:definition "Class combination of rock fragment and artefacts" ;
    skos:inScheme glosis_cl:rockSizeValueCode ;
    skos:narrower glosis_cl:rockSizeValueCode-BL,
        glosis_cl:rockSizeValueCode-CS,
        glosis_cl:rockSizeValueCode-FM,
        glosis_cl:rockSizeValueCode-MC,
        glosis_cl:rockSizeValueCode-SB ;
    skos:notation "C" ;
    skos:prefLabel "Combination of classes"@en ;
    skos:topConceptOf glosis_cl:rockSizeValueCode .

glosis_cl:rockSizeValueCode-CS a glosis_cl:RockSizeValueCode,
        skos:Concept ;
    skos:broader glosis_cl:rockSizeValueCode-C ;
    skos:definition "Combination rock fragments and artefacts of coarse gravel and stones" ;
    skos:inScheme glosis_cl:rockSizeValueCode ;
    skos:notation "CS" ;
    skos:prefLabel "Coarse gravel and stones"@en .

glosis_cl:rockSizeValueCode-FM a glosis_cl:RockSizeValueCode,
        skos:Concept ;
    skos:broader glosis_cl:rockSizeValueCode-C ;
    skos:definition "Combination of fine and medium gravel and artefacts" ;
    skos:inScheme glosis_cl:rockSizeValueCode ;
    skos:notation "FM" ;
    skos:prefLabel "Fine and medium gravel/artefacts"@en .

glosis_cl:rockSizeValueCode-MC a glosis_cl:RockSizeValueCode,
        skos:Concept ;
    skos:broader glosis_cl:rockSizeValueCode-C ;
    skos:definition "Combination of medium and course gravels and artefacts" ;
    skos:inScheme glosis_cl:rockSizeValueCode ;
    skos:notation "MC" ;
    skos:prefLabel "Medium and coarse gravel/artefacts"@en .

glosis_cl:rockSizeValueCode-R a glosis_cl:RockSizeValueCode,
        skos:Concept ;
    skos:definition "Rock fragments measured in mm" ;
    skos:inScheme glosis_cl:rockSizeValueCode ;
    skos:narrower glosis_cl:rockSizeValueCode-RB,
        glosis_cl:rockSizeValueCode-RC,
        glosis_cl:rockSizeValueCode-RF,
        glosis_cl:rockSizeValueCode-RL,
        glosis_cl:rockSizeValueCode-RM,
        glosis_cl:rockSizeValueCode-RS ;
    skos:notation "R" ;
    skos:prefLabel "Rock fragments"@en ;
    skos:topConceptOf glosis_cl:rockSizeValueCode .

glosis_cl:rockSizeValueCode-RB a glosis_cl:RockSizeValueCode,
        skos:Concept ;
    skos:broader glosis_cl:rockSizeValueCode-R ;
    skos:definition "60mm–200mm" ;
    skos:inScheme glosis_cl:rockSizeValueCode ;
    skos:notation "RB" ;
    skos:prefLabel "Boulders"@en .

glosis_cl:rockSizeValueCode-RC a glosis_cl:RockSizeValueCode,
        skos:Concept ;
    skos:broader glosis_cl:rockSizeValueCode-R ;
    skos:definition "Coarse gravel of size  20mm–60mm" ;
    skos:inScheme glosis_cl:rockSizeValueCode ;
    skos:notation "RC" ;
    skos:prefLabel "Coarse gravel"@en .

glosis_cl:rockSizeValueCode-RF a glosis_cl:RockSizeValueCode,
        skos:Concept ;
    skos:broader glosis_cl:rockSizeValueCode-R ;
    skos:definition "Rock fragments of mainly fine gravel of size from 2mm–6mm" ;
    skos:inScheme glosis_cl:rockSizeValueCode ;
    skos:notation "RF" ;
    skos:prefLabel "Fine gravel"@en .

glosis_cl:rockSizeValueCode-RL a glosis_cl:RockSizeValueCode,
        skos:Concept ;
    skos:broader glosis_cl:rockSizeValueCode-R ;
    skos:definition "Rock fragments mainly in the form of large boulders of size more than 600mm" ;
    skos:inScheme glosis_cl:rockSizeValueCode ;
    skos:notation "RL" ;
    skos:prefLabel "Large boulders"@en .

glosis_cl:rockSizeValueCode-RM a glosis_cl:RockSizeValueCode,
        skos:Concept ;
    skos:broader glosis_cl:rockSizeValueCode-R ;
    skos:definition "Combination of rocks and artefacts of medium gravel of size from 6mm–20mm" ;
    skos:inScheme glosis_cl:rockSizeValueCode ;
    skos:notation "RM" ;
    skos:prefLabel "Medium gravel"@en .

glosis_cl:rockSizeValueCode-RS a glosis_cl:RockSizeValueCode,
        skos:Concept ;
    skos:broader glosis_cl:rockSizeValueCode-R ;
    skos:definition "Rock fragments mainly stones of size from 60mm–200mm" ;
    skos:inScheme glosis_cl:rockSizeValueCode ;
    skos:notation "RS" ;
    skos:prefLabel "Stones"@en .

glosis_cl:rockSizeValueCode-SB a glosis_cl:RockSizeValueCode,
        skos:Concept ;
    skos:broader glosis_cl:rockSizeValueCode-C ;
    skos:definition "Combination of stone and boulders" ;
    skos:inScheme glosis_cl:rockSizeValueCode ;
    skos:notation "SB" ;
    skos:prefLabel "Stones and boulders"@en .

glosis_cl:rootsAbundanceValueCode-C a glosis_cl:RootsAbundanceValueCode,
        skos:Concept ;
    skos:definition "< 2 mm (number)50–200 ;> 2 mm (number)5–20" ;
    skos:inScheme glosis_cl:rootsAbundanceValueCode ;
    skos:notation "C" ;
    skos:prefLabel "Common"@en ;
    skos:topConceptOf glosis_cl:rootsAbundanceValueCode .

glosis_cl:rootsAbundanceValueCode-F a glosis_cl:RootsAbundanceValueCode,
        skos:Concept ;
    skos:definition "< 2 mm (number)20–50;> 2 mm (number) 2–5" ;
    skos:inScheme glosis_cl:rootsAbundanceValueCode ;
    skos:notation "F" ;
    skos:prefLabel "Few"@en ;
    skos:topConceptOf glosis_cl:rootsAbundanceValueCode .

glosis_cl:rootsAbundanceValueCode-M a glosis_cl:RootsAbundanceValueCode,
        skos:Concept ;
    skos:definition "< 2 mm (number)> 200 ;> 2 mm (number)> 20" ;
    skos:inScheme glosis_cl:rootsAbundanceValueCode ;
    skos:notation "M" ;
    skos:prefLabel "Many"@en ;
    skos:topConceptOf glosis_cl:rootsAbundanceValueCode .

glosis_cl:rootsAbundanceValueCode-N a glosis_cl:RootsAbundanceValueCode,
        skos:Concept ;
    skos:definition "< 2 mm (number)0;> 2 mm (number)0" ;
    skos:inScheme glosis_cl:rootsAbundanceValueCode ;
    skos:notation "N" ;
    skos:prefLabel "None"@en ;
    skos:topConceptOf glosis_cl:rootsAbundanceValueCode .

glosis_cl:rootsAbundanceValueCode-V a glosis_cl:RootsAbundanceValueCode,
        skos:Concept ;
    skos:definition "< 2 mm (number)1–20 ;> 2 mm (number)1–2" ;
    skos:inScheme glosis_cl:rootsAbundanceValueCode ;
    skos:notation "V" ;
    skos:prefLabel "Very few"@en ;
    skos:topConceptOf glosis_cl:rootsAbundanceValueCode .

glosis_cl:saltContentValueCode-EX a glosis_cl:SaltContentValueCode,
        skos:Concept ;
    skos:definition "Extremely salty soil with salt content > 15 dS m-1" ;
    skos:inScheme glosis_cl:saltContentValueCode ;
    skos:notation "EX" ;
    skos:prefLabel "Extremely salty"@en ;
    skos:topConceptOf glosis_cl:saltContentValueCode .

glosis_cl:saltContentValueCode-MO a glosis_cl:SaltContentValueCode,
        skos:Concept ;
    skos:definition "Extremely salty soil with salt content 2–4 dS m-1" ;
    skos:inScheme glosis_cl:saltContentValueCode ;
    skos:notation "MO" ;
    skos:prefLabel "Moderately salty"@en ;
    skos:topConceptOf glosis_cl:saltContentValueCode .

glosis_cl:saltContentValueCode-N a glosis_cl:SaltContentValueCode,
        skos:Concept ;
    skos:definition "Nearly not salty soild with salt content less than  0.75 dS m-1" ;
    skos:inScheme glosis_cl:saltContentValueCode ;
    skos:notation "N" ;
    skos:prefLabel "(nearly)Not salty"@en ;
    skos:topConceptOf glosis_cl:saltContentValueCode .

glosis_cl:saltContentValueCode-SL a glosis_cl:SaltContentValueCode,
        skos:Concept ;
    skos:definition "Slightly salty soil with salt content 0.75–2 dS m-1" ;
    skos:inScheme glosis_cl:saltContentValueCode ;
    skos:notation "SL" ;
    skos:prefLabel "Slightly salty"@en ;
    skos:topConceptOf glosis_cl:saltContentValueCode .

glosis_cl:saltContentValueCode-ST a glosis_cl:SaltContentValueCode,
        skos:Concept ;
    skos:definition "Strongly salty soil with salt content 4–8 dS m-1" ;
    skos:inScheme glosis_cl:saltContentValueCode ;
    skos:notation "ST" ;
    skos:prefLabel "Strongly salty"@en ;
    skos:topConceptOf glosis_cl:saltContentValueCode .

glosis_cl:saltContentValueCode-VST a glosis_cl:SaltContentValueCode,
        skos:Concept ;
    skos:definition "Very strongly salty soil with salt content 8–15 dS m-1" ;
    skos:inScheme glosis_cl:saltContentValueCode ;
    skos:notation "VST" ;
    skos:prefLabel "Very strongly salty"@en ;
    skos:topConceptOf glosis_cl:saltContentValueCode .

glosis_cl:saltCoverValueCode-0 a glosis_cl:SaltCoverValueCode,
        skos:Concept ;
    skos:definition "No salt content of 0%–2%" ;
    skos:inScheme glosis_cl:saltCoverValueCode ;
    skos:notation "0" ;
    skos:prefLabel "None"@en ;
    skos:topConceptOf glosis_cl:saltCoverValueCode .

glosis_cl:saltCoverValueCode-1 a glosis_cl:SaltCoverValueCode,
        skos:Concept ;
    skos:definition "Low salt content of 2%–15%" ;
    skos:inScheme glosis_cl:saltCoverValueCode ;
    skos:notation "1" ;
    skos:prefLabel "Low"@en ;
    skos:topConceptOf glosis_cl:saltCoverValueCode .

glosis_cl:saltCoverValueCode-2 a glosis_cl:SaltCoverValueCode,
        skos:Concept ;
    skos:definition "Moderate salt content of 15%–40%" ;
    skos:inScheme glosis_cl:saltCoverValueCode ;
    skos:notation "2" ;
    skos:prefLabel "Moderate"@en ;
    skos:topConceptOf glosis_cl:saltCoverValueCode .

glosis_cl:saltCoverValueCode-3 a glosis_cl:SaltCoverValueCode,
        skos:Concept ;
    skos:definition "High salt content of 40%–80%" ;
    skos:inScheme glosis_cl:saltCoverValueCode ;
    skos:notation "3" ;
    skos:prefLabel "High"@en ;
    skos:topConceptOf glosis_cl:saltCoverValueCode .

glosis_cl:saltCoverValueCode-4 a glosis_cl:SaltCoverValueCode,
        skos:Concept ;
    skos:definition "Dominant salt content of more than 80%" ;
    skos:inScheme glosis_cl:saltCoverValueCode ;
    skos:notation "4" ;
    skos:prefLabel "Dominant"@en ;
    skos:topConceptOf glosis_cl:saltCoverValueCode .

glosis_cl:saltThicknessValueCode-C a glosis_cl:SaltThicknessValueCode,
        skos:Concept ;
    skos:definition "Layer of salt occurance is  5mm–20mm" ;
    skos:inScheme glosis_cl:saltThicknessValueCode ;
    skos:notation "C" ;
    skos:prefLabel "Thick"@en ;
    skos:topConceptOf glosis_cl:saltThicknessValueCode .

glosis_cl:saltThicknessValueCode-F a glosis_cl:SaltThicknessValueCode,
        skos:Concept ;
    skos:definition "Layer of salt occurance is  < 2mm" ;
    skos:inScheme glosis_cl:saltThicknessValueCode ;
    skos:notation "F" ;
    skos:prefLabel "Thin"@en ;
    skos:topConceptOf glosis_cl:saltThicknessValueCode .

glosis_cl:saltThicknessValueCode-M a glosis_cl:SaltThicknessValueCode,
        skos:Concept ;
    skos:definition "Layer of salt occurance is 2mm–5mm" ;
    skos:inScheme glosis_cl:saltThicknessValueCode ;
    skos:notation "M" ;
    skos:prefLabel "Medium"@en ;
    skos:topConceptOf glosis_cl:saltThicknessValueCode .

glosis_cl:saltThicknessValueCode-N a glosis_cl:SaltThicknessValueCode,
        skos:Concept ;
    skos:definition "No salt occurance" ;
    skos:inScheme glosis_cl:saltThicknessValueCode ;
    skos:notation "N" ;
    skos:prefLabel "None"@en ;
    skos:topConceptOf glosis_cl:saltThicknessValueCode .

glosis_cl:saltThicknessValueCode-V a glosis_cl:SaltThicknessValueCode,
        skos:Concept ;
    skos:definition "Layer of salt occurance is > 20mm" ;
    skos:inScheme glosis_cl:saltThicknessValueCode ;
    skos:notation "V" ;
    skos:prefLabel "Very thick"@en ;
    skos:topConceptOf glosis_cl:saltThicknessValueCode .

glosis_cl:sandPropertyCode-SWD1 a glosis_cl:SandPropertyCode,
        skos:Concept ;
    skos:definition "Sand water dispersible at 0.1 indicates the sand fraction of soil that can be dispersed into water under a pressure of 0.1. This measure helps assess the ease with which sand particles can separate from aggregates and become suspended in water, impacting soil erosion potential and water retention characteristics. Source: Soil Science Society of America." ;
    skos:inScheme glosis_cl:sandPropertyCode ;
    skos:notation "SWD1" ;
    skos:prefLabel "Sand Water Dispersible 0.1"@en ;
    skos:topConceptOf glosis_cl:sandPropertyCode .

glosis_cl:sandPropertyCode-SWD2 a glosis_cl:SandPropertyCode,
        skos:Concept ;
    skos:definition "Sand water dispersible at 0.2 measures the sand fraction that can be dispersed at a 0.2 pressure. This parameter is crucial for evaluating the soil’s risk for erosion, particularly for sandy soils where the potential for particle dispersion can lead to structural degradation. Source: Soil Science Society of America." ;
    skos:inScheme glosis_cl:sandPropertyCode ;
    skos:notation "SWD2" ;
    skos:prefLabel "Sand Water Dispersible 0.2"@en ;
    skos:topConceptOf glosis_cl:sandPropertyCode .

glosis_cl:sandPropertyCode-SWD3 a glosis_cl:SandPropertyCode,
        skos:Concept ;
    skos:definition "Sand water dispersible at 0.3 refers to the portion of sand particles in the soil that can be dispersed into water under a specific condition, where the dispersion occurs at a 0.3 pressure. This measurement indicates how easily the sand fraction of the soil can break apart and be suspended in water. Dispersible sand is important in evaluating soil structure and its susceptibility to erosion and runoff. Source: Soil Science Society of America." ;
    skos:inScheme glosis_cl:sandPropertyCode ;
    skos:notation "SWD3" ;
    skos:prefLabel "Sand Water Dispersible 0.3"@en ;
    skos:topConceptOf glosis_cl:sandPropertyCode .

glosis_cl:sandPropertyCode-SWD4 a glosis_cl:SandPropertyCode,
        skos:Concept ;
    skos:definition "Sand water dispersible at 0.4 measures the fraction of sand particles that can be dispersed at a 0.4 pressure. This is useful for understanding how sand interacts with water under varying levels of stress, providing insight into soil stability, especially in sandy soils where dispersion might influence the soil structure and erosion potential. Source: Soil Science Society of America." ;
    skos:inScheme glosis_cl:sandPropertyCode ;
    skos:notation "SWD4" ;
    skos:prefLabel "Sand Water Dispersible 0.4"@en ;
    skos:topConceptOf glosis_cl:sandPropertyCode .

glosis_cl:sandPropertyCode-SWD5 a glosis_cl:SandPropertyCode,
        skos:Concept ;
    skos:definition "Sand water dispersible at 0.5 refers to the amount of sand particles that can be dispersed into water when subjected to a pressure of 0.5. This measure is used to assess the potential for soil degradation, particularly in sandy soils where dispersion may lead to erosion or changes in soil structure. Source: Soil Science Society of America." ;
    skos:inScheme glosis_cl:sandPropertyCode ;
    skos:notation "SWD5" ;
    skos:prefLabel "Sand Water Dispersible 0.5"@en ;
    skos:topConceptOf glosis_cl:sandPropertyCode .

glosis_cl:sandPropertyCode-SWDT a glosis_cl:SandPropertyCode,
        skos:Concept ;
    skos:definition "Sand water dispersible total refers to the sum of all sand particles that can be dispersed into water across a range of pressures, usually reflecting the total amount of dispersible sand in the soil. This value is important in understanding the overall erodibility of a soil, as high dispersibility is linked to increased susceptibility to erosion and degradation. Source: Soil Science Society of America." ;
    skos:inScheme glosis_cl:sandPropertyCode ;
    skos:notation "SWDT" ;
    skos:prefLabel "Sand Water Dispersible Total"@en ;
    skos:topConceptOf glosis_cl:sandPropertyCode .

glosis_cl:sandyTextureValueCode-CS a glosis_cl:SandyTextureValueCode,
        skos:Concept ;
    skos:definition "Coarse sand is a subdivision of the unspecified Sand (S) textural class" ;
    skos:inScheme glosis_cl:sandyTextureValueCode ;
    skos:notation "CS" ;
    skos:prefLabel "Coarse sand"@en ;
    skos:topConceptOf glosis_cl:sandyTextureValueCode .

glosis_cl:sandyTextureValueCode-CSL a glosis_cl:SandyTextureValueCode,
        skos:Concept ;
    skos:definition "Coarse sandy loam is a subdivision of the Sandy Loam (SL) textural class" ;
    skos:inScheme glosis_cl:sandyTextureValueCode ;
    skos:notation "CSL" ;
    skos:prefLabel "Coarse sandy loam"@en ;
    skos:topConceptOf glosis_cl:sandyTextureValueCode .

glosis_cl:sandyTextureValueCode-FS a glosis_cl:SandyTextureValueCode,
        skos:Concept ;
    skos:definition "Fine sand is a subdivision of the unspecified Sand (S) textural class" ;
    skos:inScheme glosis_cl:sandyTextureValueCode ;
    skos:notation "FS" ;
    skos:prefLabel "Fine sand"@en ;
    skos:topConceptOf glosis_cl:sandyTextureValueCode .

glosis_cl:sandyTextureValueCode-FSL a glosis_cl:SandyTextureValueCode,
        skos:Concept ;
    skos:definition "Fine sandy loam is a subdivision of the Sandy Loam (SL) textural class" ;
    skos:inScheme glosis_cl:sandyTextureValueCode ;
    skos:notation "FSL" ;
    skos:prefLabel "Fine sandy loam"@en ;
    skos:topConceptOf glosis_cl:sandyTextureValueCode .

glosis_cl:sandyTextureValueCode-LCS a glosis_cl:SandyTextureValueCode,
        skos:Concept ;
    skos:definition "Loamy coarse sand is a subdivision of the Loamy sand (LS) textural class" ;
    skos:inScheme glosis_cl:sandyTextureValueCode ;
    skos:notation "LCS" ;
    skos:prefLabel "Loamy coarse sand"@en ;
    skos:topConceptOf glosis_cl:sandyTextureValueCode .

glosis_cl:sandyTextureValueCode-LFS a glosis_cl:SandyTextureValueCode,
        skos:Concept ;
    skos:definition "Loamy fine sand is a subdivision of the Loamy sand (LS) textural class" ;
    skos:inScheme glosis_cl:sandyTextureValueCode ;
    skos:notation "LFS" ;
    skos:prefLabel "Loamy fine sand"@en ;
    skos:topConceptOf glosis_cl:sandyTextureValueCode .

glosis_cl:sandyTextureValueCode-LVFS a glosis_cl:SandyTextureValueCode,
        skos:Concept ;
    skos:definition "Loamy very fine sand is a subdivision of the Loamy sand (LS) textural class" ;
    skos:inScheme glosis_cl:sandyTextureValueCode ;
    skos:notation "LVFS" ;
    skos:prefLabel "Loamy very fine sand"@en ;
    skos:topConceptOf glosis_cl:sandyTextureValueCode .

glosis_cl:sandyTextureValueCode-MS a glosis_cl:SandyTextureValueCode,
        skos:Concept ;
    skos:definition "Medium sand is a subdivision of the unspecified Sand (S) textural class" ;
    skos:inScheme glosis_cl:sandyTextureValueCode ;
    skos:notation "MS" ;
    skos:prefLabel "Medium sand"@en ;
    skos:topConceptOf glosis_cl:sandyTextureValueCode .

glosis_cl:sandyTextureValueCode-US a glosis_cl:SandyTextureValueCode,
        skos:Concept ;
    skos:definition "Unsorted Sand is a subdivision of the unspecified Sand (S) textural class" ;
    skos:inScheme glosis_cl:sandyTextureValueCode ;
    skos:notation "US" ;
    skos:prefLabel "Sand, unsorted"@en ;
    skos:topConceptOf glosis_cl:sandyTextureValueCode .

glosis_cl:sandyTextureValueCode-VFS a glosis_cl:SandyTextureValueCode,
        skos:Concept ;
    skos:definition "Very fine sand is a subdivision of the unspecified Sand (S) textural class" ;
    skos:inScheme glosis_cl:sandyTextureValueCode ;
    skos:notation "VFS" ;
    skos:prefLabel "Very fine sand"@en ;
    skos:topConceptOf glosis_cl:sandyTextureValueCode .

glosis_cl:sealingConsistenceValueCode-E a glosis_cl:SealingConsistenceValueCode,
        skos:Concept ;
    skos:definition "Surface sealing with consistency Extremely hard" ;
    skos:inScheme glosis_cl:sealingConsistenceValueCode ;
    skos:notation "E" ;
    skos:prefLabel "Extremely hard"@en ;
    skos:topConceptOf glosis_cl:sealingConsistenceValueCode .

glosis_cl:sealingConsistenceValueCode-H a glosis_cl:SealingConsistenceValueCode,
        skos:Concept ;
    skos:definition "Surface sealing with consistency Hard" ;
    skos:inScheme glosis_cl:sealingConsistenceValueCode ;
    skos:notation "H" ;
    skos:prefLabel "Hard"@en ;
    skos:topConceptOf glosis_cl:sealingConsistenceValueCode .

glosis_cl:sealingConsistenceValueCode-S a glosis_cl:SealingConsistenceValueCode,
        skos:Concept ;
    skos:definition "Surface sealing with consistency Slightly hard" ;
    skos:inScheme glosis_cl:sealingConsistenceValueCode ;
    skos:notation "S" ;
    skos:prefLabel "Slightly hard"@en ;
    skos:topConceptOf glosis_cl:sealingConsistenceValueCode .

glosis_cl:sealingConsistenceValueCode-V a glosis_cl:SealingConsistenceValueCode,
        skos:Concept ;
    skos:definition "Surface sealing with consistency Very hard" ;
    skos:inScheme glosis_cl:sealingConsistenceValueCode ;
    skos:notation "V" ;
    skos:prefLabel "Very hard"@en ;
    skos:topConceptOf glosis_cl:sealingConsistenceValueCode .

glosis_cl:sealingThicknessValueCode-C a glosis_cl:SealingThicknessValueCode,
        skos:Concept ;
    skos:definition "Surface sealing with thickness  5mm–20mm" ;
    skos:inScheme glosis_cl:sealingThicknessValueCode ;
    skos:notation "C" ;
    skos:prefLabel "Thick"@en ;
    skos:topConceptOf glosis_cl:sealingThicknessValueCode .

glosis_cl:sealingThicknessValueCode-F a glosis_cl:SealingThicknessValueCode,
        skos:Concept ;
    skos:definition "Surface sealing with thickness < 2mm" ;
    skos:inScheme glosis_cl:sealingThicknessValueCode ;
    skos:notation "F" ;
    skos:prefLabel "Thin"@en ;
    skos:topConceptOf glosis_cl:sealingThicknessValueCode .

glosis_cl:sealingThicknessValueCode-M a glosis_cl:SealingThicknessValueCode,
        skos:Concept ;
    skos:definition "Surface sealing with thickness  2mm–5mm" ;
    skos:inScheme glosis_cl:sealingThicknessValueCode ;
    skos:notation "M" ;
    skos:prefLabel "Medium"@en ;
    skos:topConceptOf glosis_cl:sealingThicknessValueCode .

glosis_cl:sealingThicknessValueCode-N a glosis_cl:SealingThicknessValueCode,
        skos:Concept ;
    skos:definition "No surface sealing" ;
    skos:inScheme glosis_cl:sealingThicknessValueCode ;
    skos:notation "N" ;
    skos:prefLabel "None"@en ;
    skos:topConceptOf glosis_cl:sealingThicknessValueCode .

glosis_cl:sealingThicknessValueCode-V a glosis_cl:SealingThicknessValueCode,
        skos:Concept ;
    skos:definition "Surface sealing with thickness > 20mm" ;
    skos:inScheme glosis_cl:sealingThicknessValueCode ;
    skos:notation "V" ;
    skos:prefLabel "Very thick"@en ;
    skos:topConceptOf glosis_cl:sealingThicknessValueCode .

glosis_cl:siltPropertyCode-SWDF1 a glosis_cl:SiltPropertyCode,
        skos:Concept ;
    skos:definition "Silt water dispersible fraction at 0.1 refers to the portion of silt particles that can be dispersed into water when subjected to a 0.1 pressure. This measure helps determine the soil's erodibility, as silt tends to be more easily dispersed than sand, contributing to the formation of suspended particles in water, which can affect water quality and soil health. Source: Soil Science Society of America." ;
    skos:inScheme glosis_cl:siltPropertyCode ;
    skos:notation "SWDF1" ;
    skos:prefLabel "Silt Water Dispersible Fraction 0.1"@en ;
    skos:topConceptOf glosis_cl:siltPropertyCode .

glosis_cl:siltPropertyCode-SWDF2 a glosis_cl:SiltPropertyCode,
        skos:Concept ;
    skos:definition "Silt water dispersible fraction at 0.2 quantifies the amount of silt particles in the soil that can be dispersed at a 0.2 pressure. Dispersible silt can have a significant impact on soil stability and is particularly relevant for understanding how silt behaves under wet conditions, affecting erosion rates and water retention. Source: Soil Science Society of America." ;
    skos:inScheme glosis_cl:siltPropertyCode ;
    skos:notation "SWDF2" ;
    skos:prefLabel "Silt Water Dispersible Fraction 0.2"@en ;
    skos:topConceptOf glosis_cl:siltPropertyCode .

glosis_cl:siltPropertyCode-SWDFT a glosis_cl:SiltPropertyCode,
        skos:Concept ;
    skos:definition "Silt water dispersible fraction total refers to the total amount of silt particles that can be dispersed into water across different pressures. This total measure indicates the overall dispersibility of silt in a soil, which is important for assessing the soil’s vulnerability to erosion and degradation, especially in soils with a high silt content. Source: Soil Science Society of America." ;
    skos:inScheme glosis_cl:siltPropertyCode ;
    skos:notation "SWDFT" ;
    skos:prefLabel "Silt Water Dispersible Fraction Total"@en ;
    skos:topConceptOf glosis_cl:siltPropertyCode .

glosis_cl:slopeFormValueCode-C a glosis_cl:SlopeFormValueCode,
        skos:Concept ;
    skos:definition "concave slope form" ;
    skos:inScheme glosis_cl:slopeFormValueCode ;
    skos:notation "C" ;
    skos:prefLabel "concave"@en ;
    skos:topConceptOf glosis_cl:slopeFormValueCode .

glosis_cl:slopeFormValueCode-S a glosis_cl:SlopeFormValueCode,
        skos:Concept ;
    skos:definition "straight slope form" ;
    skos:inScheme glosis_cl:slopeFormValueCode ;
    skos:notation "S" ;
    skos:prefLabel "straight"@en ;
    skos:topConceptOf glosis_cl:slopeFormValueCode .

glosis_cl:slopeFormValueCode-T a glosis_cl:SlopeFormValueCode,
        skos:Concept ;
    skos:definition "terraced slope form" ;
    skos:inScheme glosis_cl:slopeFormValueCode ;
    skos:notation "T" ;
    skos:prefLabel "terraced"@en ;
    skos:topConceptOf glosis_cl:slopeFormValueCode .

glosis_cl:slopeFormValueCode-V a glosis_cl:SlopeFormValueCode,
        skos:Concept ;
    skos:definition "convex slope form" ;
    skos:inScheme glosis_cl:slopeFormValueCode ;
    skos:notation "V" ;
    skos:prefLabel "convex"@en ;
    skos:topConceptOf glosis_cl:slopeFormValueCode .

glosis_cl:slopeFormValueCode-X a glosis_cl:SlopeFormValueCode,
        skos:Concept ;
    skos:definition "complex (irregular) slope form" ;
    skos:inScheme glosis_cl:slopeFormValueCode ;
    skos:notation "X" ;
    skos:prefLabel "complex (irregular)"@en ;
    skos:topConceptOf glosis_cl:slopeFormValueCode .

glosis_cl:slopeGradientClassValueCode-1 a glosis_cl:SlopeGradientClassValueCode,
        skos:Concept ;
    skos:definition "0–0.2% of slope gradient" ;
    skos:inScheme glosis_cl:slopeGradientClassValueCode ;
    skos:notation "1" ;
    skos:prefLabel "Flat"@en ;
    skos:topConceptOf glosis_cl:slopeGradientClassValueCode .

glosis_cl:slopeGradientClassValueCode-10 a glosis_cl:SlopeGradientClassValueCode,
        skos:Concept ;
    skos:definition "> 60% of slope gradient" ;
    skos:inScheme glosis_cl:slopeGradientClassValueCode ;
    skos:notation "10" ;
    skos:prefLabel "Very steep"@en ;
    skos:topConceptOf glosis_cl:slopeGradientClassValueCode .

glosis_cl:slopeGradientClassValueCode-2 a glosis_cl:SlopeGradientClassValueCode,
        skos:Concept ;
    skos:definition "0.2–0.5 % of slope gradient" ;
    skos:inScheme glosis_cl:slopeGradientClassValueCode ;
    skos:notation "2" ;
    skos:prefLabel "Level"@en ;
    skos:topConceptOf glosis_cl:slopeGradientClassValueCode .

glosis_cl:slopeGradientClassValueCode-3 a glosis_cl:SlopeGradientClassValueCode,
        skos:Concept ;
    skos:definition "0.5–1.0 % of slope gradient" ;
    skos:inScheme glosis_cl:slopeGradientClassValueCode ;
    skos:notation "3" ;
    skos:prefLabel "Nearly level"@en ;
    skos:topConceptOf glosis_cl:slopeGradientClassValueCode .

glosis_cl:slopeGradientClassValueCode-4 a glosis_cl:SlopeGradientClassValueCode,
        skos:Concept ;
    skos:definition "1.0–2.0 % of slope gradient" ;
    skos:inScheme glosis_cl:slopeGradientClassValueCode ;
    skos:notation "4" ;
    skos:prefLabel "Very gently sloping"@en ;
    skos:topConceptOf glosis_cl:slopeGradientClassValueCode .

glosis_cl:slopeGradientClassValueCode-5 a glosis_cl:SlopeGradientClassValueCode,
        skos:Concept ;
    skos:definition "2–5% of slope gradient" ;
    skos:inScheme glosis_cl:slopeGradientClassValueCode ;
    skos:notation "5" ;
    skos:prefLabel "Gently sloping"@en ;
    skos:topConceptOf glosis_cl:slopeGradientClassValueCode .

glosis_cl:slopeGradientClassValueCode-6 a glosis_cl:SlopeGradientClassValueCode,
        skos:Concept ;
    skos:definition "5–10 % of slope gradient" ;
    skos:inScheme glosis_cl:slopeGradientClassValueCode ;
    skos:notation "6" ;
    skos:prefLabel "Sloping"@en ;
    skos:topConceptOf glosis_cl:slopeGradientClassValueCode .

glosis_cl:slopeGradientClassValueCode-7 a glosis_cl:SlopeGradientClassValueCode,
        skos:Concept ;
    skos:definition "10–15% of slope gradient" ;
    skos:inScheme glosis_cl:slopeGradientClassValueCode ;
    skos:notation "7" ;
    skos:prefLabel "Strongly sloping"@en ;
    skos:topConceptOf glosis_cl:slopeGradientClassValueCode .

glosis_cl:slopeGradientClassValueCode-8 a glosis_cl:SlopeGradientClassValueCode,
        skos:Concept ;
    skos:definition "15–30 % of slope gradient" ;
    skos:inScheme glosis_cl:slopeGradientClassValueCode ;
    skos:notation "8" ;
    skos:prefLabel "Moderately steep"@en ;
    skos:topConceptOf glosis_cl:slopeGradientClassValueCode .

glosis_cl:slopeGradientClassValueCode-9 a glosis_cl:SlopeGradientClassValueCode,
        skos:Concept ;
    skos:definition "30–60 % of slope gradient" ;
    skos:inScheme glosis_cl:slopeGradientClassValueCode ;
    skos:notation "9" ;
    skos:prefLabel "Steep"@en ;
    skos:topConceptOf glosis_cl:slopeGradientClassValueCode .

glosis_cl:slopePathwaysValueCode-CC a glosis_cl:SlopePathwaysValueCode,
        skos:Concept ;
    skos:definition "Concave slope" ;
    skos:inScheme glosis_cl:slopePathwaysValueCode ;
    skos:notation "CC" ;
    skos:prefLabel "CC"@en ;
    skos:topConceptOf glosis_cl:slopePathwaysValueCode .

glosis_cl:slopePathwaysValueCode-CS a glosis_cl:SlopePathwaysValueCode,
        skos:Concept ;
    skos:definition "concave stright slope" ;
    skos:inScheme glosis_cl:slopePathwaysValueCode ;
    skos:notation "CS" ;
    skos:prefLabel "CS"@en ;
    skos:topConceptOf glosis_cl:slopePathwaysValueCode .

glosis_cl:slopePathwaysValueCode-CV a glosis_cl:SlopePathwaysValueCode,
        skos:Concept ;
    skos:definition "concave vertical slope" ;
    skos:inScheme glosis_cl:slopePathwaysValueCode ;
    skos:notation "CV" ;
    skos:prefLabel "CV"@en ;
    skos:topConceptOf glosis_cl:slopePathwaysValueCode .

glosis_cl:slopePathwaysValueCode-SC a glosis_cl:SlopePathwaysValueCode,
        skos:Concept ;
    skos:definition "Straight concave slope" ;
    skos:inScheme glosis_cl:slopePathwaysValueCode ;
    skos:notation "SC" ;
    skos:prefLabel "SC"@en ;
    skos:topConceptOf glosis_cl:slopePathwaysValueCode .

glosis_cl:slopePathwaysValueCode-SS a glosis_cl:SlopePathwaysValueCode,
        skos:Concept ;
    skos:definition "straight slope" ;
    skos:inScheme glosis_cl:slopePathwaysValueCode ;
    skos:notation "SS" ;
    skos:prefLabel "SS"@en ;
    skos:topConceptOf glosis_cl:slopePathwaysValueCode .

glosis_cl:slopePathwaysValueCode-SV a glosis_cl:SlopePathwaysValueCode,
        skos:Concept ;
    skos:definition "straight convex slope" ;
    skos:inScheme glosis_cl:slopePathwaysValueCode ;
    skos:notation "SV" ;
    skos:prefLabel "SV"@en ;
    skos:topConceptOf glosis_cl:slopePathwaysValueCode .

glosis_cl:slopePathwaysValueCode-VC a glosis_cl:SlopePathwaysValueCode,
        skos:Concept ;
    skos:definition "Vertical concave slope" ;
    skos:inScheme glosis_cl:slopePathwaysValueCode ;
    skos:notation "VC" ;
    skos:prefLabel "VC"@en ;
    skos:topConceptOf glosis_cl:slopePathwaysValueCode .

glosis_cl:slopePathwaysValueCode-VS a glosis_cl:SlopePathwaysValueCode,
        skos:Concept ;
    skos:definition "Convex straight slope" ;
    skos:inScheme glosis_cl:slopePathwaysValueCode ;
    skos:notation "VS" ;
    skos:prefLabel "VS"@en ;
    skos:topConceptOf glosis_cl:slopePathwaysValueCode .

glosis_cl:slopePathwaysValueCode-VV a glosis_cl:SlopePathwaysValueCode,
        skos:Concept ;
    skos:definition "Convex vertical slope" ;
    skos:inScheme glosis_cl:slopePathwaysValueCode ;
    skos:notation "VV" ;
    skos:prefLabel "VV"@en ;
    skos:topConceptOf glosis_cl:slopePathwaysValueCode .

glosis_cl:stickinessValueCode-NST a glosis_cl:StickinessValueCode,
        skos:Concept ;
    skos:definition "After release of pressure, practically no soil material adheres to thumb and finger." ;
    skos:inScheme glosis_cl:stickinessValueCode ;
    skos:notation "NST" ;
    skos:prefLabel "Non-sticky"@en ;
    skos:topConceptOf glosis_cl:stickinessValueCode .

glosis_cl:stickinessValueCode-SSS a glosis_cl:StickinessValueCode,
        skos:Concept ;
    skos:definition "Additional code of combination of SST and ST" ;
    skos:inScheme glosis_cl:stickinessValueCode ;
    skos:notation "SSS" ;
    skos:prefLabel "slightly sticky to sticky"@en ;
    skos:topConceptOf glosis_cl:stickinessValueCode .

glosis_cl:stickinessValueCode-SST a glosis_cl:StickinessValueCode,
        skos:Concept ;
    skos:definition "After pressure, soil material adheres to both thumb and finger but comes off one or the other rather cleanly. It is not appreciably stretched when the digits are separated." ;
    skos:inScheme glosis_cl:stickinessValueCode ;
    skos:notation "SST" ;
    skos:prefLabel "Slightly sticky"@en ;
    skos:topConceptOf glosis_cl:stickinessValueCode .

glosis_cl:stickinessValueCode-ST a glosis_cl:StickinessValueCode,
        skos:Concept ;
    skos:definition "After pressure, soil material adheres to both thumb and finger and tends to stretch somewhat and pull apart rather than pulling free from either digit." ;
    skos:inScheme glosis_cl:stickinessValueCode ;
    skos:notation "ST" ;
    skos:prefLabel "Sticky"@en ;
    skos:topConceptOf glosis_cl:stickinessValueCode .

glosis_cl:stickinessValueCode-SVS a glosis_cl:StickinessValueCode,
        skos:Concept ;
    skos:definition "Additional code of combination of ST and VST" ;
    skos:inScheme glosis_cl:stickinessValueCode ;
    skos:notation "SVS" ;
    skos:prefLabel "sticky to very sticky"@en ;
    skos:topConceptOf glosis_cl:stickinessValueCode .

glosis_cl:stickinessValueCode-VST a glosis_cl:StickinessValueCode,
        skos:Concept ;
    skos:definition "After pressure, soil material adheres strongly to both thumb and finger and is decidedly stretched when they are separated." ;
    skos:inScheme glosis_cl:stickinessValueCode ;
    skos:notation "VST" ;
    skos:prefLabel "Very sticky"@en ;
    skos:topConceptOf glosis_cl:stickinessValueCode .

glosis_cl:structureGradeValueCode-MO a glosis_cl:StructureGradeValueCode,
        skos:Concept ;
    skos:definition "Aggregates are observable in place and there is a distinct arrangement of natural surfaces of weakness. When disturbed, the soil material breaks into a mixture of many entire aggregates, some broken aggregates, and little material without aggregates faces. Aggregates surfaces generally show distinct differences with the aggregates interiors." ;
    skos:inScheme glosis_cl:structureGradeValueCode ;
    skos:notation "MO" ;
    skos:prefLabel "Moderate"@en ;
    skos:topConceptOf glosis_cl:structureGradeValueCode .

glosis_cl:structureGradeValueCode-MS a glosis_cl:StructureGradeValueCode,
        skos:Concept ;
    skos:definition "Moderate to strong" ;
    skos:inScheme glosis_cl:structureGradeValueCode ;
    skos:notation "MS" ;
    skos:prefLabel "Moderate to strong"@en ;
    skos:topConceptOf glosis_cl:structureGradeValueCode .

glosis_cl:structureGradeValueCode-ST a glosis_cl:StructureGradeValueCode,
        skos:Concept ;
    skos:definition "Aggregates are clearly observable in place and there is a prominent arrangement of natural surfaces of weakness. When disturbed, the soil material separates mainly into entire aggregates. Aggregates surfaces generally differ markedly from aggregate interiors." ;
    skos:inScheme glosis_cl:structureGradeValueCode ;
    skos:notation "ST" ;
    skos:prefLabel "Strong"@en ;
    skos:topConceptOf glosis_cl:structureGradeValueCode .

glosis_cl:structureGradeValueCode-WE a glosis_cl:StructureGradeValueCode,
        skos:Concept ;
    skos:definition "Aggregates are barely observable in place and there is only a weak arrangement of natural surfaces of weakness. When gently disturbed, the soil material breaks into a mixture of few entire aggregates, many broken aggregates, and much material without aggregate faces. Aggregate surfaces differ in some way from the aggregate interior." ;
    skos:inScheme glosis_cl:structureGradeValueCode ;
    skos:notation "WE" ;
    skos:prefLabel "Weak"@en ;
    skos:topConceptOf glosis_cl:structureGradeValueCode .

glosis_cl:structureGradeValueCode-WM a glosis_cl:StructureGradeValueCode,
        skos:Concept ;
    skos:definition "Weak to moderate" ;
    skos:inScheme glosis_cl:structureGradeValueCode ;
    skos:notation "WM" ;
    skos:prefLabel "Weak to moderate"@en ;
    skos:topConceptOf glosis_cl:structureGradeValueCode .

glosis_cl:structureSizeValueCode-CO a glosis_cl:StructureSizeValueCode,
        skos:Concept ;
    skos:definition "5–10 50–100 20–50" ;
    skos:inScheme glosis_cl:structureSizeValueCode ;
    skos:notation "CO" ;
    skos:prefLabel "Coarse/thick"@en ;
    skos:topConceptOf glosis_cl:structureSizeValueCode .

glosis_cl:structureSizeValueCode-EC a glosis_cl:StructureSizeValueCode,
        skos:Concept ;
    skos:definition "– > 500 –" ;
    skos:inScheme glosis_cl:structureSizeValueCode ;
    skos:notation "EC" ;
    skos:prefLabel "Extremely coarse"@en ;
    skos:topConceptOf glosis_cl:structureSizeValueCode .

glosis_cl:structureSizeValueCode-FI a glosis_cl:StructureSizeValueCode,
        skos:Concept ;
    skos:definition "1–2 10–20 5–10" ;
    skos:inScheme glosis_cl:structureSizeValueCode ;
    skos:notation "FI" ;
    skos:prefLabel "Fine/thin"@en ;
    skos:topConceptOf glosis_cl:structureSizeValueCode .

glosis_cl:structureSizeValueCode-ME a glosis_cl:StructureSizeValueCode,
        skos:Concept ;
    skos:definition "2–5 20–50 10–20" ;
    skos:inScheme glosis_cl:structureSizeValueCode ;
    skos:notation "ME" ;
    skos:prefLabel "Medium"@en ;
    skos:topConceptOf glosis_cl:structureSizeValueCode .

glosis_cl:structureSizeValueCode-VC a glosis_cl:StructureSizeValueCode,
        skos:Concept ;
    skos:definition "> 10 1.1.000 > 50" ;
    skos:inScheme glosis_cl:structureSizeValueCode ;
    skos:notation "VC" ;
    skos:prefLabel "Very coarse/thick"@en ;
    skos:topConceptOf glosis_cl:structureSizeValueCode .

glosis_cl:structureSizeValueCode-VF a glosis_cl:StructureSizeValueCode,
        skos:Concept ;
    skos:definition "< 1 < 10 < 5" ;
    skos:inScheme glosis_cl:structureSizeValueCode ;
    skos:notation "VF" ;
    skos:prefLabel "Very fine/thin"@en ;
    skos:topConceptOf glosis_cl:structureSizeValueCode .

glosis_cl:surfaceAgeValueCode-Ha a glosis_cl:SurfaceAgeValueCode,
        skos:Concept ;
    skos:definition "Holocene (100–10 000 years) anthropogeomorphic: human-made relief modifications, such as terracing of forming hills or walls by early civilizations or during the Middle Ages or earlier, restriction of flooding by dykes, or surface raising." ;
    skos:inScheme glosis_cl:surfaceAgeValueCode ;
    skos:notation "Ha" ;
    skos:prefLabel "Holocene anthropogeomorphic"@en ;
    skos:topConceptOf glosis_cl:surfaceAgeValueCode .

glosis_cl:surfaceAgeValueCode-Hn a glosis_cl:SurfaceAgeValueCode,
        skos:Concept ;
    skos:definition "Holocene (100–10 000 years) natural: with loss by erosion or deposition of materials such as on tidal flats, of coastal dunes, in river valleys, landslides or desert areas." ;
    skos:inScheme glosis_cl:surfaceAgeValueCode ;
    skos:notation "Hn" ;
    skos:prefLabel "Holocene natural"@en ;
    skos:topConceptOf glosis_cl:surfaceAgeValueCode .

glosis_cl:surfaceAgeValueCode-O a glosis_cl:SurfaceAgeValueCode,
        skos:Concept ;
    skos:definition "Older, pre-Tertiary land surfaces, commonly high planes, terraces or peneplains, except incised valleys, frequent occurrence of palaeosoils." ;
    skos:inScheme glosis_cl:surfaceAgeValueCode ;
    skos:notation "O" ;
    skos:prefLabel "Older, pre-Tertiary land surfaces"@en ;
    skos:topConceptOf glosis_cl:surfaceAgeValueCode .

glosis_cl:surfaceAgeValueCode-T a glosis_cl:SurfaceAgeValueCode,
        skos:Concept ;
    skos:definition "Tertiary land surfaces, commonly high planes, terraces or peneplains, except incised valleys, frequent occurrence of palaeosoils." ;
    skos:inScheme glosis_cl:surfaceAgeValueCode ;
    skos:notation "T" ;
    skos:prefLabel "Tertiary land surfaces"@en ;
    skos:topConceptOf glosis_cl:surfaceAgeValueCode .

glosis_cl:surfaceAgeValueCode-Ya a glosis_cl:SurfaceAgeValueCode,
        skos:Concept ;
    skos:definition "Young (10–100 years) anthropogeomorphic: with complete disturbance of any natural surfaces (and soils) such as in urban, industrial and mining areas with early soil development from fresh natural, technogenic or a mixture of materials, or restriction of flooding by dykes." ;
    skos:inScheme glosis_cl:surfaceAgeValueCode ;
    skos:notation "Ya" ;
    skos:prefLabel "Young anthropogeomorphic"@en ;
    skos:topConceptOf glosis_cl:surfaceAgeValueCode .

glosis_cl:surfaceAgeValueCode-Yn a glosis_cl:SurfaceAgeValueCode,
        skos:Concept ;
    skos:definition "Young (10–100 years) natural: with loss by erosion or deposition of materials such as on tidal flats, of coastal dunes, river valleys, landslides or desert areas." ;
    skos:inScheme glosis_cl:surfaceAgeValueCode ;
    skos:notation "Yn" ;
    skos:prefLabel "Young natural"@en ;
    skos:topConceptOf glosis_cl:surfaceAgeValueCode .

glosis_cl:surfaceAgeValueCode-lPf a glosis_cl:SurfaceAgeValueCode,
        skos:Concept ;
    skos:definition "Late Pleistocene, without periglacial influence." ;
    skos:inScheme glosis_cl:surfaceAgeValueCode ;
    skos:notation "lPf" ;
    skos:prefLabel "Late Pleistocene, without periglacial influence."@en ;
    skos:topConceptOf glosis_cl:surfaceAgeValueCode .

glosis_cl:surfaceAgeValueCode-lPi a glosis_cl:SurfaceAgeValueCode,
        skos:Concept ;
    skos:definition "Late Pleistocene, ice covered, commonly recent soil formation on fresh materials." ;
    skos:inScheme glosis_cl:surfaceAgeValueCode ;
    skos:notation "lPi" ;
    skos:prefLabel "Late Pleistocene, ice covered"@en ;
    skos:topConceptOf glosis_cl:surfaceAgeValueCode .

glosis_cl:surfaceAgeValueCode-lPp a glosis_cl:SurfaceAgeValueCode,
        skos:Concept ;
    skos:definition "Late Pleistocene, periglacial, commonly recent soil formation on preweathered materials." ;
    skos:inScheme glosis_cl:surfaceAgeValueCode ;
    skos:notation "lPp" ;
    skos:prefLabel "Late Pleistocene, periglacial"@en ;
    skos:topConceptOf glosis_cl:surfaceAgeValueCode .

glosis_cl:surfaceAgeValueCode-oPf a glosis_cl:SurfaceAgeValueCode,
        skos:Concept ;
    skos:definition "Older Pleistocene, without periglacial influence." ;
    skos:inScheme glosis_cl:surfaceAgeValueCode ;
    skos:notation "oPf" ;
    skos:prefLabel "Older Pleistocene, without periglacial influence."@en ;
    skos:topConceptOf glosis_cl:surfaceAgeValueCode .

glosis_cl:surfaceAgeValueCode-oPi a glosis_cl:SurfaceAgeValueCode,
        skos:Concept ;
    skos:definition "Older Pleistocene, ice covered, commonly the recent soil formation on younger over older, preweathered materials." ;
    skos:inScheme glosis_cl:surfaceAgeValueCode ;
    skos:notation "oPi" ;
    skos:prefLabel "Older Pleistocene, ice covered"@en ;
    skos:topConceptOf glosis_cl:surfaceAgeValueCode .

glosis_cl:surfaceAgeValueCode-oPp a glosis_cl:SurfaceAgeValueCode,
        skos:Concept ;
    skos:definition "Older Pleistocene, with periglacial influence, commonly the recent soil formation on younger over older, preweathered materials." ;
    skos:inScheme glosis_cl:surfaceAgeValueCode ;
    skos:notation "oPp" ;
    skos:prefLabel "Older Pleistocene, with periglacial influence"@en ;
    skos:topConceptOf glosis_cl:surfaceAgeValueCode .

glosis_cl:surfaceAgeValueCode-vYa a glosis_cl:SurfaceAgeValueCode,
        skos:Concept ;
    skos:definition "Very young (1–10 years) anthropogeomorphic: with complete disturbance of natural surfaces (and soils) such as in urban, industrial and mining areas with very early soil development from fresh natural or technogenic or mixed materials." ;
    skos:inScheme glosis_cl:surfaceAgeValueCode ;
    skos:notation "vYa" ;
    skos:prefLabel "Very young anthropogeomorphic"@en ;
    skos:topConceptOf glosis_cl:surfaceAgeValueCode .

glosis_cl:surfaceAgeValueCode-vYn a glosis_cl:SurfaceAgeValueCode,
        skos:Concept ;
    skos:definition "Very young (1–10 years) natural: with loss by erosion or deposition of materials such as on tidal flats, of coastal dunes, in river valleys, landslides or desert areas." ;
    skos:inScheme glosis_cl:surfaceAgeValueCode ;
    skos:notation "vYn" ;
    skos:prefLabel "Very young natural"@en ;
    skos:topConceptOf glosis_cl:surfaceAgeValueCode .

glosis_cl:textClayPropertyCode-Cl a glosis_cl:TextClayPropertyCode,
        skos:Concept ;
    skos:definition "Very fine mineral particles smaller than 2 µm" ;
    skos:inScheme glosis_cl:textClayPropertyCode ;
    skos:notation "Cl" ;
    skos:prefLabel "Clay (< 0.002 mm)"@en ;
    skos:scopeNote <https://doi.org/10.1016/j.geoderma.2022.115783> ;
    skos:topConceptOf glosis_cl:textClayPropertyCode .

glosis_cl:textSandPropertyCode-Sa_ISO a glosis_cl:TextSandPropertyCode,
        skos:Concept ;
    skos:definition "Content of mineral particles with sizes between 0.063-2 mm in soil" ;
    skos:inScheme glosis_cl:textSandPropertyCode ;
    skos:narrower glosis_cl:textSandPropertyCode-cSa_ISO,
        glosis_cl:textSandPropertyCode-fSa_ISO,
        glosis_cl:textSandPropertyCode-mSa_ISO ;
    skos:notation "Sa_ISO" ;
    skos:prefLabel "Sand (0.063  - 2 mm)"@en ;
    skos:scopeNote <https://www.iso.org/standard/66345.html> ;
    skos:topConceptOf glosis_cl:textSandPropertyCode .

glosis_cl:textSandPropertyCode-Sa_ISSS a glosis_cl:TextSandPropertyCode,
        skos:Concept ;
    skos:definition "Content of mineral particles with sizes between 0.020-2 mm in soil" ;
    skos:inScheme glosis_cl:textSandPropertyCode ;
    skos:narrower glosis_cl:textSandPropertyCode-cSa_ISSS,
        glosis_cl:textSandPropertyCode-fSa_ISSS,
        glosis_cl:textSandPropertyCode-mSa_ISSS,
        glosis_cl:textSandPropertyCode-vcSa_ISSS,
        glosis_cl:textSandPropertyCode-vfSa_ISSS ;
    skos:notation "Sa_ISSS" ;
    skos:prefLabel "Sand (0.02 - 2 mm)"@en ;
    skos:scopeNote <https://doi.org/10.1016/j.geoderma.2022.115783> ;
    skos:topConceptOf glosis_cl:textSandPropertyCode .

glosis_cl:textSandPropertyCode-Sa_USDA a glosis_cl:TextSandPropertyCode,
        skos:Concept ;
    skos:definition "Content of mineral particles with sizes between 0.050-2 mm in soil" ;
    skos:inScheme glosis_cl:textSandPropertyCode ;
    skos:narrower glosis_cl:textSandPropertyCode-cSa_USDA,
        glosis_cl:textSandPropertyCode-fSa_USDA,
        glosis_cl:textSandPropertyCode-mSa_USDA,
        glosis_cl:textSandPropertyCode-vcSa_USDA,
        glosis_cl:textSandPropertyCode-vfSa_USDA ;
    skos:notation "Sa_USDA" ;
    skos:prefLabel "Sand (0.050  - 2 mm)"@en ;
    skos:scopeNote <https://doi.org/10.1111/j.1365-3091.2012.01335.x> ;
    skos:topConceptOf glosis_cl:textSandPropertyCode .

glosis_cl:textSandPropertyCode-cSa_ISO a glosis_cl:TextSandPropertyCode,
        skos:Concept ;
    skos:broader glosis_cl:textSandPropertyCode-Sa_ISO ;
    skos:definition "Content of mineral particles with sizes between 0.63-2 mm in soil" ;
    skos:inScheme glosis_cl:textSandPropertyCode ;
    skos:notation "cSa_ISO" ;
    skos:prefLabel "Coarse sand (0.63 - 2 mm)"@en ;
    skos:scopeNote <https://www.iso.org/standard/66345.html> .

glosis_cl:textSandPropertyCode-cSa_ISSS a glosis_cl:TextSandPropertyCode,
        skos:Concept ;
    skos:broader glosis_cl:textSandPropertyCode-Sa_ISSS ;
    skos:definition "Content of mineral particles with sizes between 0.2-2 mm in soil" ;
    skos:inScheme glosis_cl:textSandPropertyCode ;
    skos:notation "cSa_ISSS" ;
    skos:prefLabel "Coarse sand (0.2 - 2 mm)"@en ;
    skos:scopeNote <https://doi.org/10.1016/j.geoderma.2022.115783> .

glosis_cl:textSandPropertyCode-cSa_USDA a glosis_cl:TextSandPropertyCode,
        skos:Concept ;
    skos:broader glosis_cl:textSandPropertyCode-Sa_USDA ;
    skos:definition "Content of mineral particles with sizes between 0.5-1 mm in soil" ;
    skos:inScheme glosis_cl:textSandPropertyCode ;
    skos:notation "cSa_USDA" ;
    skos:prefLabel "Coarse sand (0.5 - 1 mm)"@en ;
    skos:scopeNote <https://doi.org/10.1111/j.1365-3091.2012.01335.x> .

glosis_cl:textSandPropertyCode-fSa_ISO a glosis_cl:TextSandPropertyCode,
        skos:Concept ;
    skos:broader glosis_cl:textSandPropertyCode-Sa_ISO ;
    skos:definition "Content of mineral particles with sizes between 0.063-0.2 mm in soil" ;
    skos:inScheme glosis_cl:textSandPropertyCode ;
    skos:notation "fSa_ISO" ;
    skos:prefLabel "Fine sand (0.063 - 0.2 mm)"@en ;
    skos:scopeNote <https://www.iso.org/standard/66345.html> .

glosis_cl:textSandPropertyCode-fSa_ISSS a glosis_cl:TextSandPropertyCode,
        skos:Concept ;
    skos:broader glosis_cl:textSandPropertyCode-Sa_ISSS ;
    skos:definition "Content of mineral particles with sizes between 0.02-0.2 mm in soil" ;
    skos:inScheme glosis_cl:textSandPropertyCode ;
    skos:notation "fSa_ISSS" ;
    skos:prefLabel "Fine sand (0.125 - 0.2 mm)"@en ;
    skos:scopeNote <https://doi.org/10.1016/j.geoderma.2022.115783> .

glosis_cl:textSandPropertyCode-fSa_USDA a glosis_cl:TextSandPropertyCode,
        skos:Concept ;
    skos:broader glosis_cl:textSandPropertyCode-Sa_USDA ;
    skos:definition "Content of mineral particles with sizes between 0.1-0.25 mm in soil" ;
    skos:inScheme glosis_cl:textSandPropertyCode ;
    skos:notation "fSa_USDA" ;
    skos:prefLabel "Fine sand (0.1 - 0.25 mm)"@en ;
    skos:scopeNote <https://doi.org/10.1111/j.1365-3091.2012.01335.x> .

glosis_cl:textSandPropertyCode-mSa_ISO a glosis_cl:TextSandPropertyCode,
        skos:Concept ;
    skos:broader glosis_cl:textSandPropertyCode-Sa_ISO ;
    skos:definition "Content of mineral particles with sizes between 0.02-0.63 mm in soil" ;
    skos:inScheme glosis_cl:textSandPropertyCode ;
    skos:notation "mSa_ISO" ;
    skos:prefLabel "Medium sand (0.2 - 0.63 mm)"@en ;
    skos:scopeNote <https://www.iso.org/standard/66345.html> .

glosis_cl:textSandPropertyCode-mSa_ISSS a glosis_cl:TextSandPropertyCode,
        skos:Concept ;
    skos:broader glosis_cl:textSandPropertyCode-Sa_ISSS ;
    skos:definition "Content of mineral particles with sizes between 0.2-0.63 mm in soil" ;
    skos:inScheme glosis_cl:textSandPropertyCode ;
    skos:notation "mSa_ISSS" ;
    skos:prefLabel "Medium sand (0.2 - 0.63 mm)"@en ;
    skos:scopeNote <https://doi.org/10.1016/j.geoderma.2022.115783> .

glosis_cl:textSandPropertyCode-mSa_USDA a glosis_cl:TextSandPropertyCode,
        skos:Concept ;
    skos:broader glosis_cl:textSandPropertyCode-Sa_USDA ;
    skos:definition "Content of mineral particles with sizes between 0.25-0.5 mm in soil" ;
    skos:inScheme glosis_cl:textSandPropertyCode ;
    skos:notation "mSa_USDA" ;
    skos:prefLabel "Medium sand (0.25 - 0.5 mm)"@en ;
    skos:scopeNote <https://doi.org/10.1111/j.1365-3091.2012.01335.x> .

glosis_cl:textSandPropertyCode-vcSa_ISSS a glosis_cl:TextSandPropertyCode,
        skos:Concept ;
    skos:broader glosis_cl:textSandPropertyCode-Sa_ISSS ;
    skos:definition "Content of mineral particles with sizes between 1.25-2 mm in soil" ;
    skos:inScheme glosis_cl:textSandPropertyCode ;
    skos:notation "vcSa_ISSS" ;
    skos:prefLabel "Very coarse sand (1.25 - 2 mm)"@en ;
    skos:scopeNote <https://doi.org/10.1016/j.geoderma.2022.115783> .

glosis_cl:textSandPropertyCode-vcSa_USDA a glosis_cl:TextSandPropertyCode,
        skos:Concept ;
    skos:broader glosis_cl:textSandPropertyCode-Sa_USDA ;
    skos:definition "Content of mineral particles with sizes between 1-2 mm in soil" ;
    skos:inScheme glosis_cl:textSandPropertyCode ;
    skos:notation "vcSa_USDA" ;
    skos:prefLabel "Very coarse sand (1 - 2 mm)"@en ;
    skos:scopeNote <https://doi.org/10.1111/j.1365-3091.2012.01335.x> .

glosis_cl:textSandPropertyCode-vfSa_ISSS a glosis_cl:TextSandPropertyCode,
        skos:Concept ;
    skos:broader glosis_cl:textSandPropertyCode-Sa_ISSS ;
    skos:definition "Content of mineral particles with sizes between 0.063-0.125 mm in soil" ;
    skos:inScheme glosis_cl:textSandPropertyCode ;
    skos:notation "vfSa_ISSS" ;
    skos:prefLabel "Very fine sand (0.063 - 0.125 mm)"@en ;
    skos:scopeNote <https://doi.org/10.1016/j.geoderma.2022.115783> .

glosis_cl:textSandPropertyCode-vfSa_USDA a glosis_cl:TextSandPropertyCode,
        skos:Concept ;
    skos:broader glosis_cl:textSandPropertyCode-Sa_USDA ;
    skos:definition "Content of mineral particles with sizes between 0.05-0.1 mm in soil" ;
    skos:inScheme glosis_cl:textSandPropertyCode ;
    skos:notation "vfSa_USDA" ;
    skos:prefLabel "Very fine sand (0.05 - 0.1 mm)"@en ;
    skos:scopeNote <https://doi.org/10.1111/j.1365-3091.2012.01335.x> .

glosis_cl:textSiltPropertyCode-Si_ISO a glosis_cl:TextSiltPropertyCode,
        skos:Concept ;
    skos:definition "Content of mineral particles with sizes between 2-63 µm in soil" ;
    skos:inScheme glosis_cl:textSiltPropertyCode ;
    skos:narrower glosis_cl:textSiltPropertyCode-cSi_ISO,
        glosis_cl:textSiltPropertyCode-fSi_ISO,
        glosis_cl:textSiltPropertyCode-mSi_ISO ;
    skos:notation "Si_ISO" ;
    skos:prefLabel "Silt (0.002 - 0.063 mm)"@en ;
    skos:scopeNote <https://www.iso.org/standard/66345.html> ;
    skos:topConceptOf glosis_cl:textSiltPropertyCode .

glosis_cl:textSiltPropertyCode-Si_ISSS a glosis_cl:TextSiltPropertyCode,
        skos:Concept ;
    skos:definition "Content of mineral particles with sizes between 2-20 µm in soil" ;
    skos:inScheme glosis_cl:textSiltPropertyCode ;
    skos:notation "Si_ISSS" ;
    skos:prefLabel "Silt (0.002 - 0.02 mm)"@en ;
    skos:scopeNote <https://doi.org/10.1016/j.geoderma.2022.115783> ;
    skos:topConceptOf glosis_cl:textSiltPropertyCode .

glosis_cl:textSiltPropertyCode-Si_USDA a glosis_cl:TextSiltPropertyCode,
        skos:Concept ;
    skos:definition "Content of mineral particles with sizes between 2-50 µm in soil" ;
    skos:inScheme glosis_cl:textSiltPropertyCode ;
    skos:narrower glosis_cl:textSiltPropertyCode-cSi_USDA,
        glosis_cl:textSiltPropertyCode-fSi_USDA ;
    skos:notation "Si_USDA" ;
    skos:prefLabel "Silt (0.002 - 0.05 mm)"@en ;
    skos:scopeNote <https://doi.org/10.1111/j.1365-3091.2012.01335.x> ;
    skos:topConceptOf glosis_cl:textSiltPropertyCode .

glosis_cl:textSiltPropertyCode-cSi_ISO a glosis_cl:TextSiltPropertyCode,
        skos:Concept ;
    skos:broader glosis_cl:textSiltPropertyCode-Si_ISO ;
    skos:definition "Content of mineral particles with sizes between 20-63 µm in soil" ;
    skos:inScheme glosis_cl:textSiltPropertyCode ;
    skos:notation "cSi_ISO" ;
    skos:prefLabel "Coarse silt (0.02 - 0.063 mm)"@en ;
    skos:scopeNote <https://www.iso.org/standard/66345.html> .

glosis_cl:textSiltPropertyCode-cSi_USDA a glosis_cl:TextSiltPropertyCode,
        skos:Concept ;
    skos:broader glosis_cl:textSiltPropertyCode-Si_USDA ;
    skos:definition "Content of mineral particles with sizes between 20-50 µm in soil" ;
    skos:inScheme glosis_cl:textSiltPropertyCode ;
    skos:notation "cSi_USDA" ;
    skos:prefLabel "Coarse silt (0.02 - 0.05 mm)"@en ;
    skos:scopeNote <https://doi.org/10.1111/j.1365-3091.2012.01335.x> .

glosis_cl:textSiltPropertyCode-fSi_ISO a glosis_cl:TextSiltPropertyCode,
        skos:Concept ;
    skos:broader glosis_cl:textSiltPropertyCode-Si_ISO ;
    skos:definition "Content of mineral particles with sizes between 2-6.3 µm in soil" ;
    skos:inScheme glosis_cl:textSiltPropertyCode ;
    skos:notation "fSi_ISO" ;
    skos:prefLabel "Fine silt (0.002 - 0.0063 mm)"@en ;
    skos:scopeNote <https://www.iso.org/standard/66345.html> .

glosis_cl:textSiltPropertyCode-fSi_USDA a glosis_cl:TextSiltPropertyCode,
        skos:Concept ;
    skos:broader glosis_cl:textSiltPropertyCode-Si_USDA ;
    skos:definition "Content of mineral particles with sizes between 2-20 µm in soil" ;
    skos:inScheme glosis_cl:textSiltPropertyCode ;
    skos:notation "fSi_USDA" ;
    skos:prefLabel "Fine silt (0.002 - 0.02 mm)"@en ;
    skos:scopeNote <https://doi.org/10.1111/j.1365-3091.2012.01335.x> .

glosis_cl:textSiltPropertyCode-mSi_ISO a glosis_cl:TextSiltPropertyCode,
        skos:Concept ;
    skos:broader glosis_cl:textSiltPropertyCode-Si_ISO ;
    skos:definition "Content of mineral particles with sizes between 6.3-20 µm in soil" ;
    skos:inScheme glosis_cl:textSiltPropertyCode ;
    skos:notation "mSi_ISO" ;
    skos:prefLabel "Medium silt (0.0063 - 0.02 mm)"@en ;
    skos:scopeNote <https://www.iso.org/standard/66345.html> .

glosis_cl:vegetationClassValueCode-B a glosis_cl:VegetationClassValueCode,
        skos:Concept ;
    skos:definition "Vegetation class of Groundwater-fed bog peat  (B)" ;
    skos:inScheme glosis_cl:vegetationClassValueCode ;
    skos:notation "B" ;
    skos:prefLabel "Groundwater-fed bog peat"@en ;
    skos:topConceptOf glosis_cl:vegetationClassValueCode .

glosis_cl:vegetationClassValueCode-D a glosis_cl:VegetationClassValueCode,
        skos:Concept ;
    skos:definition "Vegetation class of Dwarf shrub (D)" ;
    skos:inScheme glosis_cl:vegetationClassValueCode ;
    skos:narrower glosis_cl:vegetationClassValueCode-DD,
        glosis_cl:vegetationClassValueCode-DE,
        glosis_cl:vegetationClassValueCode-DS,
        glosis_cl:vegetationClassValueCode-DT,
        glosis_cl:vegetationClassValueCode-DX ;
    skos:notation "D" ;
    skos:prefLabel "Dwarf shrub"@en ;
    skos:topConceptOf glosis_cl:vegetationClassValueCode .

glosis_cl:vegetationClassValueCode-DD a glosis_cl:VegetationClassValueCode,
        skos:Concept ;
    skos:broader glosis_cl:vegetationClassValueCode-D ;
    skos:definition "Deciduous dwarf shrub from the vegtation class of Dwarf shrub (D)" ;
    skos:inScheme glosis_cl:vegetationClassValueCode ;
    skos:notation "DD" ;
    skos:prefLabel "Deciduous dwarf shrub"@en .

glosis_cl:vegetationClassValueCode-DE a glosis_cl:VegetationClassValueCode,
        skos:Concept ;
    skos:broader glosis_cl:vegetationClassValueCode-D ;
    skos:definition "Evergreen dwarf shrub from the vegtation class of Dwarf shrub (D)" ;
    skos:inScheme glosis_cl:vegetationClassValueCode ;
    skos:notation "DE" ;
    skos:prefLabel "Evergreen dwarf shrub"@en .

glosis_cl:vegetationClassValueCode-DS a glosis_cl:VegetationClassValueCode,
        skos:Concept ;
    skos:broader glosis_cl:vegetationClassValueCode-D ;
    skos:definition "Semi-deciduous dwarf shrub from the vegtation class of Dwarf shrub (D)" ;
    skos:inScheme glosis_cl:vegetationClassValueCode ;
    skos:notation "DS" ;
    skos:prefLabel "Semi-deciduous dwarf shrub"@en .

glosis_cl:vegetationClassValueCode-DT a glosis_cl:VegetationClassValueCode,
        skos:Concept ;
    skos:broader glosis_cl:vegetationClassValueCode-D ;
    skos:definition "Tundra from the vegtation class of Dwarf shrub (D)" ;
    skos:inScheme glosis_cl:vegetationClassValueCode ;
    skos:notation "DT" ;
    skos:prefLabel "Tundra"@en .

glosis_cl:vegetationClassValueCode-DX a glosis_cl:VegetationClassValueCode,
        skos:Concept ;
    skos:broader glosis_cl:vegetationClassValueCode-D ;
    skos:definition "Xermomorphic dwarf shrub from the vegtation class of Dwarf shrub (D)" ;
    skos:inScheme glosis_cl:vegetationClassValueCode ;
    skos:notation "DX" ;
    skos:prefLabel "Xermomorphic dwarf shrub"@en .

glosis_cl:vegetationClassValueCode-F a glosis_cl:VegetationClassValueCode,
        skos:Concept ;
    skos:definition "Vegetation class of Closed forest (F)" ;
    skos:inScheme glosis_cl:vegetationClassValueCode ;
    skos:narrower glosis_cl:vegetationClassValueCode-FC,
        glosis_cl:vegetationClassValueCode-FD,
        glosis_cl:vegetationClassValueCode-FE,
        glosis_cl:vegetationClassValueCode-FS,
        glosis_cl:vegetationClassValueCode-FX ;
    skos:notation "F" ;
    skos:prefLabel "Closed forest"@en ;
    skos:topConceptOf glosis_cl:vegetationClassValueCode .

glosis_cl:vegetationClassValueCode-FC a glosis_cl:VegetationClassValueCode,
        skos:Concept ;
    skos:broader glosis_cl:vegetationClassValueCode-F ;
    skos:definition "Coniferous forest from the vegtation class of Closed forest (F)" ;
    skos:inScheme glosis_cl:vegetationClassValueCode ;
    skos:notation "FC" ;
    skos:prefLabel "Coniferous forest"@en .

glosis_cl:vegetationClassValueCode-FD a glosis_cl:VegetationClassValueCode,
        skos:Concept ;
    skos:broader glosis_cl:vegetationClassValueCode-F ;
    skos:definition "Deciduous forest from the vegtation class of Closed forest (F)" ;
    skos:inScheme glosis_cl:vegetationClassValueCode ;
    skos:notation "FD" ;
    skos:prefLabel "Deciduous forest"@en .

glosis_cl:vegetationClassValueCode-FE a glosis_cl:VegetationClassValueCode,
        skos:Concept ;
    skos:broader glosis_cl:vegetationClassValueCode-F ;
    skos:definition "Evergreen broad-leaved forest from the vegtation class of Closed forest (F)" ;
    skos:inScheme glosis_cl:vegetationClassValueCode ;
    skos:notation "FE" ;
    skos:prefLabel "Evergreen broad-leaved forest"@en .

glosis_cl:vegetationClassValueCode-FS a glosis_cl:VegetationClassValueCode,
        skos:Concept ;
    skos:broader glosis_cl:vegetationClassValueCode-F ;
    skos:definition "Semi-deciduous forest from the vegtation class of Closed forest (F)" ;
    skos:inScheme glosis_cl:vegetationClassValueCode ;
    skos:notation "FS" ;
    skos:prefLabel "Semi-deciduous forest"@en .

glosis_cl:vegetationClassValueCode-FX a glosis_cl:VegetationClassValueCode,
        skos:Concept ;
    skos:broader glosis_cl:vegetationClassValueCode-F ;
    skos:definition "Xeromorphic forest from the vegtation class of Closed forest (F)" ;
    skos:inScheme glosis_cl:vegetationClassValueCode ;
    skos:notation "FX" ;
    skos:prefLabel "Xeromorphic forest"@en .

glosis_cl:vegetationClassValueCode-H a glosis_cl:VegetationClassValueCode,
        skos:Concept ;
    skos:definition "Vegetation class of Herbaceous (H)" ;
    skos:inScheme glosis_cl:vegetationClassValueCode ;
    skos:narrower glosis_cl:vegetationClassValueCode-HF,
        glosis_cl:vegetationClassValueCode-HM,
        glosis_cl:vegetationClassValueCode-HS,
        glosis_cl:vegetationClassValueCode-HT ;
    skos:notation "H" ;
    skos:prefLabel "Herbaceous"@en ;
    skos:topConceptOf glosis_cl:vegetationClassValueCode .

glosis_cl:vegetationClassValueCode-HF a glosis_cl:VegetationClassValueCode,
        skos:Concept ;
    skos:broader glosis_cl:vegetationClassValueCode-H ;
    skos:definition "Forb from the vegtation class of Herbaceous (H)" ;
    skos:inScheme glosis_cl:vegetationClassValueCode ;
    skos:notation "HF" ;
    skos:prefLabel "Forb"@en .

glosis_cl:vegetationClassValueCode-HM a glosis_cl:VegetationClassValueCode,
        skos:Concept ;
    skos:broader glosis_cl:vegetationClassValueCode-H ;
    skos:definition "Medium grassland from the vegtation class of Herbaceous (H)" ;
    skos:inScheme glosis_cl:vegetationClassValueCode ;
    skos:notation "HM" ;
    skos:prefLabel "Medium grassland"@en .

glosis_cl:vegetationClassValueCode-HS a glosis_cl:VegetationClassValueCode,
        skos:Concept ;
    skos:broader glosis_cl:vegetationClassValueCode-H ;
    skos:definition "Short grassland from the vegtation class of Herbaceous (H)" ;
    skos:inScheme glosis_cl:vegetationClassValueCode ;
    skos:notation "HS" ;
    skos:prefLabel "Short grassland"@en .

glosis_cl:vegetationClassValueCode-HT a glosis_cl:VegetationClassValueCode,
        skos:Concept ;
    skos:broader glosis_cl:vegetationClassValueCode-H ;
    skos:definition "Tall grassland from the vegtation class of Herbaceous (H)" ;
    skos:inScheme glosis_cl:vegetationClassValueCode ;
    skos:notation "HT" ;
    skos:prefLabel "Tall grassland"@en .

glosis_cl:vegetationClassValueCode-M a glosis_cl:VegetationClassValueCode,
        skos:Concept ;
    skos:definition "Vegetation class of Rainwater-fed moor peat (M)" ;
    skos:inScheme glosis_cl:vegetationClassValueCode ;
    skos:notation "M" ;
    skos:prefLabel "Rainwater-fed moor peat"@en ;
    skos:topConceptOf glosis_cl:vegetationClassValueCode .

glosis_cl:vegetationClassValueCode-S a glosis_cl:VegetationClassValueCode,
        skos:Concept ;
    skos:definition "Vegetation class of Shrub (S)" ;
    skos:inScheme glosis_cl:vegetationClassValueCode ;
    skos:narrower glosis_cl:vegetationClassValueCode-SD,
        glosis_cl:vegetationClassValueCode-SE,
        glosis_cl:vegetationClassValueCode-SS,
        glosis_cl:vegetationClassValueCode-SX ;
    skos:notation "S" ;
    skos:prefLabel "Shrub"@en ;
    skos:topConceptOf glosis_cl:vegetationClassValueCode .

glosis_cl:vegetationClassValueCode-SD a glosis_cl:VegetationClassValueCode,
        skos:Concept ;
    skos:broader glosis_cl:vegetationClassValueCode-S ;
    skos:definition "Deciduous shrub from the vegtation class of Shrub (S)" ;
    skos:inScheme glosis_cl:vegetationClassValueCode ;
    skos:notation "SD" ;
    skos:prefLabel "Deciduous shrub"@en .

glosis_cl:vegetationClassValueCode-SE a glosis_cl:VegetationClassValueCode,
        skos:Concept ;
    skos:broader glosis_cl:vegetationClassValueCode-S ;
    skos:definition "Evergreen shrub from the vegtation class of Shrub (S)" ;
    skos:inScheme glosis_cl:vegetationClassValueCode ;
    skos:notation "SE" ;
    skos:prefLabel "Evergreen shrub"@en .

glosis_cl:vegetationClassValueCode-SS a glosis_cl:VegetationClassValueCode,
        skos:Concept ;
    skos:broader glosis_cl:vegetationClassValueCode-S ;
    skos:definition "Semi-deciduous shrub from the vegtation class of Shrub (S)" ;
    skos:inScheme glosis_cl:vegetationClassValueCode ;
    skos:notation "SS" ;
    skos:prefLabel "Semi-deciduous shrub"@en .

glosis_cl:vegetationClassValueCode-SX a glosis_cl:VegetationClassValueCode,
        skos:Concept ;
    skos:broader glosis_cl:vegetationClassValueCode-S ;
    skos:definition "Xeromorphic shrub from the vegtation class of Shrub (S)" ;
    skos:inScheme glosis_cl:vegetationClassValueCode ;
    skos:notation "SX" ;
    skos:prefLabel "Xeromorphic shrub"@en .

glosis_cl:vegetationClassValueCode-W a glosis_cl:VegetationClassValueCode,
        skos:Concept ;
    skos:definition "Vegetation class of Woodland (W)" ;
    skos:inScheme glosis_cl:vegetationClassValueCode ;
    skos:notation "W" ;
    skos:prefLabel "Woodland"@en ;
    skos:topConceptOf glosis_cl:vegetationClassValueCode .

glosis_cl:vegetationClassValueCode-WD a glosis_cl:VegetationClassValueCode,
        skos:Concept ;
    skos:broader glosis_cl:vegetationClassValueCode-WE ;
    skos:definition "Deciduous woodland from the vegtation class of Woodland (W)" ;
    skos:inScheme glosis_cl:vegetationClassValueCode ;
    skos:notation "WD" ;
    skos:prefLabel "Deciduous woodland"@en .

glosis_cl:vegetationClassValueCode-WE a glosis_cl:VegetationClassValueCode,
        skos:Concept ;
    skos:broader glosis_cl:vegetationClassValueCode-WE ;
    skos:definition "Evergreen woodland from the vegtation class of Woodland (W)" ;
    skos:inScheme glosis_cl:vegetationClassValueCode ;
    skos:narrower glosis_cl:vegetationClassValueCode-WD,
        glosis_cl:vegetationClassValueCode-WE,
        glosis_cl:vegetationClassValueCode-WS,
        glosis_cl:vegetationClassValueCode-WX ;
    skos:notation "WE" ;
    skos:prefLabel "Evergreen woodland"@en .

glosis_cl:vegetationClassValueCode-WS a glosis_cl:VegetationClassValueCode,
        skos:Concept ;
    skos:broader glosis_cl:vegetationClassValueCode-WE ;
    skos:definition "Semi-deciduous woodland from the vegtation class of Woodland (W)" ;
    skos:inScheme glosis_cl:vegetationClassValueCode ;
    skos:notation "WS" ;
    skos:prefLabel "Semi-deciduous woodland"@en .

glosis_cl:vegetationClassValueCode-WX a glosis_cl:VegetationClassValueCode,
        skos:Concept ;
    skos:broader glosis_cl:vegetationClassValueCode-WE ;
    skos:definition "Xeromorphic woodland from the vegtation class of Woodland (W)" ;
    skos:inScheme glosis_cl:vegetationClassValueCode ;
    skos:notation "WX" ;
    skos:prefLabel "Xeromorphic woodland"@en .

glosis_cl:voidsClassificationValueCode-B a glosis_cl:VoidsClassificationValueCode,
        skos:Concept ;
    skos:definition "Discontinuous spherical or elliptical voids (chambers) of sedimentary origin or formed by compressed air, e.g. gas bubbles in slaking crusts after heavy rainfall. Relatively unimportant in connection with plant growth." ;
    skos:inScheme glosis_cl:voidsClassificationValueCode ;
    skos:notation "B" ;
    skos:prefLabel "Vesicular"@en ;
    skos:topConceptOf glosis_cl:voidsClassificationValueCode .

glosis_cl:voidsClassificationValueCode-C a glosis_cl:VoidsClassificationValueCode,
        skos:Concept ;
    skos:definition "Elongated voids of faunal or floral origin, mostly tubular in shape and continuous, varying strongly in diameter. When wider than a few centimetres (burrow holes), they are more adequately described under biological activity." ;
    skos:inScheme glosis_cl:voidsClassificationValueCode ;
    skos:notation "C" ;
    skos:prefLabel "Channels"@en ;
    skos:topConceptOf glosis_cl:voidsClassificationValueCode .

glosis_cl:voidsClassificationValueCode-I a glosis_cl:VoidsClassificationValueCode,
        skos:Concept ;
    skos:definition "Controlled by the fabric, or arrangement, of the soil particles, also known as textural voids. Subdivision possible into simple packing voids, which relate to the packing of sand particles, and compound packing voids, which result from the packing of non-accommodating peds. Predominantly irregular in shape and interconnected, and hard to quantify in the field." ;
    skos:inScheme glosis_cl:voidsClassificationValueCode ;
    skos:notation "I" ;
    skos:prefLabel "Interstitial"@en ;
    skos:topConceptOf glosis_cl:voidsClassificationValueCode .

glosis_cl:voidsClassificationValueCode-P a glosis_cl:VoidsClassificationValueCode,
        skos:Concept ;
    skos:definition "Most planes are extra-pedal voids, related to accommodating ped surfaces or cracking patterns. They are often not persistent and vary in size, shape and quantity depending on the moisture condition of the soil. Planar voids may be recorded, describing width and frequency." ;
    skos:inScheme glosis_cl:voidsClassificationValueCode ;
    skos:notation "P" ;
    skos:prefLabel "Planes"@en ;
    skos:topConceptOf glosis_cl:voidsClassificationValueCode .

glosis_cl:voidsClassificationValueCode-V a glosis_cl:VoidsClassificationValueCode,
        skos:Concept ;
    skos:definition "Mostly irregular, equidimensional voids of faunal origin or resulting from tillage or disturbance of other voids. Discontinuous or interconnected. May be quantified in specific cases." ;
    skos:inScheme glosis_cl:voidsClassificationValueCode ;
    skos:notation "V" ;
    skos:prefLabel "Vughs"@en ;
    skos:topConceptOf glosis_cl:voidsClassificationValueCode .

glosis_cl:voidsDiameterValueCode-C a glosis_cl:VoidsDiameterValueCode,
        skos:Concept ;
    skos:definition "Coarse void with diameter between 5–20 m" ;
    skos:inScheme glosis_cl:voidsDiameterValueCode ;
    skos:notation "C" ;
    skos:prefLabel "Coarse"@en ;
    skos:topConceptOf glosis_cl:voidsDiameterValueCode .

glosis_cl:voidsDiameterValueCode-F a glosis_cl:VoidsDiameterValueCode,
        skos:Concept ;
    skos:definition "Fine void with diameter between 0.5–2 m" ;
    skos:inScheme glosis_cl:voidsDiameterValueCode ;
    skos:notation "F" ;
    skos:prefLabel "Fine"@en ;
    skos:topConceptOf glosis_cl:voidsDiameterValueCode .

glosis_cl:voidsDiameterValueCode-FF a glosis_cl:VoidsDiameterValueCode,
        skos:Concept ;
    skos:definition "Fine and very fine void with combination of fine and very fine type" ;
    skos:inScheme glosis_cl:voidsDiameterValueCode ;
    skos:notation "FF" ;
    skos:prefLabel "fine and very fine"@en ;
    skos:topConceptOf glosis_cl:voidsDiameterValueCode .

glosis_cl:voidsDiameterValueCode-FM a glosis_cl:VoidsDiameterValueCode,
        skos:Concept ;
    skos:definition "Fine and medium void with combination of fine and medium type" ;
    skos:inScheme glosis_cl:voidsDiameterValueCode ;
    skos:notation "FM" ;
    skos:prefLabel "fine and medium"@en ;
    skos:topConceptOf glosis_cl:voidsDiameterValueCode .

glosis_cl:voidsDiameterValueCode-M a glosis_cl:VoidsDiameterValueCode,
        skos:Concept ;
    skos:definition "medium void with diameter 2–5" ;
    skos:inScheme glosis_cl:voidsDiameterValueCode ;
    skos:notation "M" ;
    skos:prefLabel "Medium"@en ;
    skos:topConceptOf glosis_cl:voidsDiameterValueCode .

glosis_cl:voidsDiameterValueCode-MC a glosis_cl:VoidsDiameterValueCode,
        skos:Concept ;
    skos:definition "Medium and coarse void with combination of medium and coarse type" ;
    skos:inScheme glosis_cl:voidsDiameterValueCode ;
    skos:notation "MC" ;
    skos:prefLabel "medium and coarse"@en ;
    skos:topConceptOf glosis_cl:voidsDiameterValueCode .

glosis_cl:voidsDiameterValueCode-V a glosis_cl:VoidsDiameterValueCode,
        skos:Concept ;
    skos:definition "Very fine void with diameter less than 0.5 m" ;
    skos:inScheme glosis_cl:voidsDiameterValueCode ;
    skos:notation "V" ;
    skos:prefLabel "Very fine"@en ;
    skos:topConceptOf glosis_cl:voidsDiameterValueCode .

glosis_cl:voidsDiameterValueCode-VC a glosis_cl:VoidsDiameterValueCode,
        skos:Concept ;
    skos:definition "very coarse void with diameter 20–50 m" ;
    skos:inScheme glosis_cl:voidsDiameterValueCode ;
    skos:notation "VC" ;
    skos:prefLabel "Very coarse"@en ;
    skos:topConceptOf glosis_cl:voidsDiameterValueCode .

glosis_cl:waterRetentionPropertyCode-WRG a glosis_cl:WaterRetentionPropertyCode,
        skos:Concept ;
    skos:definition "Gravimetric water retention refers to the amount of water held by the soil measured by weight, often expressed in terms of mass per unit mass of soil. It is a fundamental method for assessing soil moisture content and can be determined at various suction pressures like 33 kPa or 1500 kPa. Source: Soil Science Society of America." ;
    skos:inScheme glosis_cl:waterRetentionPropertyCode ;
    skos:notation "WRG" ;
    skos:prefLabel "Water Retention Gravimetric"@en ;
    skos:topConceptOf glosis_cl:waterRetentionPropertyCode .

glosis_cl:waterRetentionPropertyCode-WRG10 a glosis_cl:WaterRetentionPropertyCode,
        skos:Concept ;
    skos:definition "Gravimetric water retention at 10 kPa measures the water held in the soil at 10 kPa pressure, commonly representing the moisture content that is available to plants under normal growing conditions. This measurement is crucial for assessing the soil’s capacity to retain and supply water to plants. Source: Soil Science Society of America." ;
    skos:inScheme glosis_cl:waterRetentionPropertyCode ;
    skos:notation "WRG10" ;
    skos:prefLabel "Water Retention Gravimetric 10 kPa"@en ;
    skos:topConceptOf glosis_cl:waterRetentionPropertyCode .

glosis_cl:waterRetentionPropertyCode-WRG100 a glosis_cl:WaterRetentionPropertyCode,
        skos:Concept ;
    skos:definition "Gravimetric water retention at 100 kPa measures the water retained by the soil at this specific pressure, using the gravimetric method. It indicates the moisture available to plants between field capacity and the wilting point, providing a useful measurement for soil water management. Source: Soil Science Society of America." ;
    skos:inScheme glosis_cl:waterRetentionPropertyCode ;
    skos:notation "WRG100" ;
    skos:prefLabel "Water Retention Gravimetric 100 kPa"@en ;
    skos:topConceptOf glosis_cl:waterRetentionPropertyCode .

glosis_cl:waterRetentionPropertyCode-WRG1500 a glosis_cl:WaterRetentionPropertyCode,
        skos:Concept ;
    skos:definition "Gravimetric water retention at 1500 kPa refers to the mass of water retained by the soil at this pressure, as measured by the gravimetric method (weighing the soil before and after drying). This pressure represents the point at which water is tightly held by the soil and is no longer easily accessible to plants, closely corresponding to the permanent wilting point. Source: Soil Science Society of America." ;
    skos:inScheme glosis_cl:waterRetentionPropertyCode ;
    skos:notation "WRG1500" ;
    skos:prefLabel "Water Retention Gravimetric 1500 kPa"@en ;
    skos:topConceptOf glosis_cl:waterRetentionPropertyCode .

glosis_cl:waterRetentionPropertyCode-WRG200 a glosis_cl:WaterRetentionPropertyCode,
        skos:Concept ;
    skos:definition "Gravimetric water retention at 200 kPa is the mass of water retained by the soil at this specific suction pressure. It provides insight into the soil’s ability to retain water that is not easily lost by evaporation, offering a more accurate measurement of water held at pressures significant for plant growth. Source: Soil Science Society of America." ;
    skos:inScheme glosis_cl:waterRetentionPropertyCode ;
    skos:notation "WRG200" ;
    skos:prefLabel "Water Retention Gravimetric 200 kPa"@en ;
    skos:topConceptOf glosis_cl:waterRetentionPropertyCode .

glosis_cl:waterRetentionPropertyCode-WRG33 a glosis_cl:WaterRetentionPropertyCode,
        skos:Concept ;
    skos:definition "Gravimetric water retention at 33 kPa measures the amount of water retained by the soil at this specific pressure, determined by the mass of water held in the soil when subjected to the 33 kPa suction. It reflects the soil’s capacity to hold water available to plants under conditions of moderate water stress. Source: Soil Science Society of America." ;
    skos:inScheme glosis_cl:waterRetentionPropertyCode ;
    skos:notation "WRG33" ;
    skos:prefLabel "Water Retention Gravimetric 33 kPa"@en ;
    skos:topConceptOf glosis_cl:waterRetentionPropertyCode .

glosis_cl:waterRetentionPropertyCode-WRG500 a glosis_cl:WaterRetentionPropertyCode,
        skos:Concept ;
    skos:definition "Gravimetric water retention at 500 kPa indicates the amount of water retained in the soil at this pressure. This is closer to the permanent wilting point, with the gravimetric method determining the mass of water held in the soil at this specific tension. Source: Soil Science Society of America." ;
    skos:inScheme glosis_cl:waterRetentionPropertyCode ;
    skos:notation "WRG500" ;
    skos:prefLabel "Water Retention Gravimetric 500 kPa"@en ;
    skos:topConceptOf glosis_cl:waterRetentionPropertyCode .

glosis_cl:waterRetentionPropertyCode-WRG6 a glosis_cl:WaterRetentionPropertyCode,
        skos:Concept ;
    skos:definition "Gravimetric water retention at 6 kPa measures the soil's water content at a low suction pressure, typically indicative of the moisture available to plants under less favorable conditions. The gravimetric method involves weighing the soil before and after drying to assess the retained water. Source: Soil Science Society of America." ;
    skos:inScheme glosis_cl:waterRetentionPropertyCode ;
    skos:notation "WRG6" ;
    skos:prefLabel "Water Retention Gravimetric 6 kPa"@en ;
    skos:topConceptOf glosis_cl:waterRetentionPropertyCode .

glosis_cl:waterRetentionPropertyCode-WRV a glosis_cl:WaterRetentionPropertyCode,
        skos:Concept ;
    skos:definition "Volumetric water retention refers to the amount of water retained in the soil, expressed as a volume per unit volume of soil. This measure is crucial for understanding the soil's ability to retain and supply water to plants, and it is often assessed at different matric potentials, such as 33 kPa or 1500 kPa, depending on the context. Source: Soil Science Society of America." ;
    skos:inScheme glosis_cl:waterRetentionPropertyCode ;
    skos:notation "WRV" ;
    skos:prefLabel "Water Retention Volumetric"@en ;
    skos:topConceptOf glosis_cl:waterRetentionPropertyCode .

glosis_cl:waterRetentionPropertyCode-WRV10 a glosis_cl:WaterRetentionPropertyCode,
        skos:Concept ;
    skos:definition "Water retention at 10 kPa measures the volumetric water content of the soil at this pressure, which is typically considered within the zone of plant-available water. At 10 kPa, the soil retains water that can be easily accessed by plants for growth and physiological processes. Source: Soil Science Society of America." ;
    skos:inScheme glosis_cl:waterRetentionPropertyCode ;
    skos:notation "WRV10" ;
    skos:prefLabel "Water Retention Volumetric 10 kPa"@en ;
    skos:topConceptOf glosis_cl:waterRetentionPropertyCode .

glosis_cl:waterRetentionPropertyCode-WRV100 a glosis_cl:WaterRetentionPropertyCode,
        skos:Concept ;
    skos:definition "Water retention at 100 kPa measures the volumetric water content in the soil at this pressure. This value is often used to assess the availability of water for plant uptake under normal conditions, as it lies between field capacity and the wilting point for many soils. Source: Soil Science Society of America." ;
    skos:inScheme glosis_cl:waterRetentionPropertyCode ;
    skos:notation "WRV100" ;
    skos:prefLabel "Water Retention Volumetric 100 kPa"@en ;
    skos:topConceptOf glosis_cl:waterRetentionPropertyCode .

glosis_cl:waterRetentionPropertyCode-WRV1500 a glosis_cl:WaterRetentionPropertyCode,
        skos:Concept ;
    skos:definition "Water retention at 1500 kPa (or field capacity) measures the amount of water that a soil can hold at this specific suction pressure. This is a critical indicator of the soil's ability to retain water against gravity after it has drained. At 1500 kPa, the soil's moisture content represents the point at which most of the water available for plant use has been drained, and it is typically considered the permanent wilting point. Source: Soil Science Society of America." ;
    skos:inScheme glosis_cl:waterRetentionPropertyCode ;
    skos:notation "WRV1500" ;
    skos:prefLabel "Water Retention Volumetric 1500 kPa"@en ;
    skos:topConceptOf glosis_cl:waterRetentionPropertyCode .

glosis_cl:waterRetentionPropertyCode-WRV200 a glosis_cl:WaterRetentionPropertyCode,
        skos:Concept ;
    skos:definition "Water retention at 200 kPa refers to the volumetric water content retained by the soil at a 200 kPa pressure. This measurement typically lies between the field capacity and wilting point, giving an indication of the soil’s ability to hold water that plants can access under moderate stress conditions. Source: Soil Science Society of America." ;
    skos:inScheme glosis_cl:waterRetentionPropertyCode ;
    skos:notation "WRV200" ;
    skos:prefLabel "Water Retention Volumetric 200 kPa"@en ;
    skos:topConceptOf glosis_cl:waterRetentionPropertyCode .

glosis_cl:waterRetentionPropertyCode-WRV33 a glosis_cl:WaterRetentionPropertyCode,
        skos:Concept ;
    skos:definition "Water retention at 33 kPa represents the volumetric water content in soil at a pressure of 33 kPa, which is often associated with the field capacity of the soil. At this pressure, water is held in the soil that is available for most plant species, providing a balance between water retention and drainage. Source: Soil Science Society of America." ;
    skos:inScheme glosis_cl:waterRetentionPropertyCode ;
    skos:notation "WRV33" ;
    skos:prefLabel "Water Retention Volumetric 33 kPa"@en ;
    skos:topConceptOf glosis_cl:waterRetentionPropertyCode .

glosis_cl:waterRetentionPropertyCode-WRV500 a glosis_cl:WaterRetentionPropertyCode,
        skos:Concept ;
    skos:definition "Water retention at 500 kPa measures the volumetric water content of the soil at a pressure of 500 kPa, which lies between field capacity and permanent wilting point. This pressure is commonly used in assessing soil water retention characteristics for plants that are not able to access water at extremely low pressures. The volumetric water content at 500 kPa indicates the soil's capacity to hold water that is readily available for plant uptake. Source: Soil Science Society of America." ;
    skos:inScheme glosis_cl:waterRetentionPropertyCode ;
    skos:notation "WRV500" ;
    skos:prefLabel "Water Retention Volumetric 500 kPa"@en ;
    skos:topConceptOf glosis_cl:waterRetentionPropertyCode .

glosis_cl:waterRetentionPropertyCode-WRV6 a glosis_cl:WaterRetentionPropertyCode,
        skos:Concept ;
    skos:definition "Volumetric water retention at 6 kPa measures the soil’s ability to hold water at a low pressure, typically indicating the moisture content available to plants under conditions of mild water stress. It is important for understanding the soil's water-holding capacity and potential for plant growth. Source: Soil Science Society of America." ;
    skos:inScheme glosis_cl:waterRetentionPropertyCode ;
    skos:notation "WRV6" ;
    skos:prefLabel "Water Retention Volumetric 6 kPa"@en ;
    skos:topConceptOf glosis_cl:waterRetentionPropertyCode .

glosis_cl:weatherConditionsValueCode-OV a glosis_cl:WeatherConditionsValueCode,
        skos:Concept ;
    skos:definition "Present weather conditions (Schoeneberger et al., 2002)" ;
    skos:inScheme glosis_cl:weatherConditionsValueCode ;
    skos:notation "OV" ;
    skos:prefLabel "overcast"@en ;
    skos:topConceptOf glosis_cl:weatherConditionsValueCode .

glosis_cl:weatherConditionsValueCode-PC a glosis_cl:WeatherConditionsValueCode,
        skos:Concept ;
    skos:definition "Present weather conditions (Schoeneberger et al., 2002)" ;
    skos:inScheme glosis_cl:weatherConditionsValueCode ;
    skos:notation "PC" ;
    skos:prefLabel "partly cloudy"@en ;
    skos:topConceptOf glosis_cl:weatherConditionsValueCode .

glosis_cl:weatherConditionsValueCode-RA a glosis_cl:WeatherConditionsValueCode,
        skos:Concept ;
    skos:definition "Present weather conditions (Schoeneberger et al., 2002)" ;
    skos:inScheme glosis_cl:weatherConditionsValueCode ;
    skos:notation "RA" ;
    skos:prefLabel "rain"@en ;
    skos:topConceptOf glosis_cl:weatherConditionsValueCode .

glosis_cl:weatherConditionsValueCode-SL a glosis_cl:WeatherConditionsValueCode,
        skos:Concept ;
    skos:definition "Present weather conditions (Schoeneberger et al., 2002)" ;
    skos:inScheme glosis_cl:weatherConditionsValueCode ;
    skos:notation "SL" ;
    skos:prefLabel "sleet"@en ;
    skos:topConceptOf glosis_cl:weatherConditionsValueCode .

glosis_cl:weatherConditionsValueCode-SN a glosis_cl:WeatherConditionsValueCode,
        skos:Concept ;
    skos:definition "Present weather conditions (Schoeneberger et al., 2002)" ;
    skos:inScheme glosis_cl:weatherConditionsValueCode ;
    skos:notation "SN" ;
    skos:prefLabel "snow"@en ;
    skos:topConceptOf glosis_cl:weatherConditionsValueCode .

glosis_cl:weatherConditionsValueCode-SU a glosis_cl:WeatherConditionsValueCode,
        skos:Concept ;
    skos:definition "Present weather conditions (Schoeneberger et al., 2002)" ;
    skos:inScheme glosis_cl:weatherConditionsValueCode ;
    skos:notation "SU" ;
    skos:prefLabel "sunny/clear"@en ;
    skos:topConceptOf glosis_cl:weatherConditionsValueCode .

glosis_cl:weatherConditionsValueCode-WC1 a glosis_cl:WeatherConditionsValueCode,
        skos:Concept ;
    skos:definition "Former weather conditions (Ad-hoc-AG-Boden, 2005)" ;
    skos:inScheme glosis_cl:weatherConditionsValueCode ;
    skos:notation "WC1" ;
    skos:prefLabel "no rain in the last month"@en ;
    skos:topConceptOf glosis_cl:weatherConditionsValueCode .

glosis_cl:weatherConditionsValueCode-WC2 a glosis_cl:WeatherConditionsValueCode,
        skos:Concept ;
    skos:definition "Former weather conditions (Ad-hoc-AG-Boden, 2005)" ;
    skos:inScheme glosis_cl:weatherConditionsValueCode ;
    skos:notation "WC2" ;
    skos:prefLabel "no rain in the last week"@en ;
    skos:topConceptOf glosis_cl:weatherConditionsValueCode .

glosis_cl:weatherConditionsValueCode-WC3 a glosis_cl:WeatherConditionsValueCode,
        skos:Concept ;
    skos:definition "Former weather conditions (Ad-hoc-AG-Boden, 2005)" ;
    skos:inScheme glosis_cl:weatherConditionsValueCode ;
    skos:notation "WC3" ;
    skos:prefLabel "no rain in the last 24 hours"@en ;
    skos:topConceptOf glosis_cl:weatherConditionsValueCode .

glosis_cl:weatherConditionsValueCode-WC4 a glosis_cl:WeatherConditionsValueCode,
        skos:Concept ;
    skos:definition "Former weather conditions (Ad-hoc-AG-Boden, 2005)" ;
    skos:inScheme glosis_cl:weatherConditionsValueCode ;
    skos:notation "WC4" ;
    skos:prefLabel "rainy without heavy rain in the last 24 hours"@en ;
    skos:topConceptOf glosis_cl:weatherConditionsValueCode .

glosis_cl:weatherConditionsValueCode-WC5 a glosis_cl:WeatherConditionsValueCode,
        skos:Concept ;
    skos:definition "Former weather conditions (Ad-hoc-AG-Boden, 2005)" ;
    skos:inScheme glosis_cl:weatherConditionsValueCode ;
    skos:notation "WC5" ;
    skos:prefLabel "heavier rain for some days or rainstorm in the last 24 hours"@en ;
    skos:topConceptOf glosis_cl:weatherConditionsValueCode .

glosis_cl:weatherConditionsValueCode-WC6 a glosis_cl:WeatherConditionsValueCode,
        skos:Concept ;
    skos:definition "Former weather conditions (Ad-hoc-AG-Boden, 2005)" ;
    skos:inScheme glosis_cl:weatherConditionsValueCode ;
    skos:notation "WC6" ;
    skos:prefLabel "extremely rainy time or snow melting"@en ;
    skos:topConceptOf glosis_cl:weatherConditionsValueCode .

glosis_cl:weatheringValueCode-F a glosis_cl:WeatheringValueCode,
        skos:Concept ;
    skos:definition "Fragments show little or no signs of weathering." ;
    skos:inScheme glosis_cl:weatheringValueCode ;
    skos:notation "F" ;
    skos:prefLabel "Fresh or slightly weathered"@en ;
    skos:topConceptOf glosis_cl:weatheringValueCode .

glosis_cl:weatheringValueCode-S a glosis_cl:WeatheringValueCode,
        skos:Concept ;
    skos:definition "All but the most resistant minerals are weathered, strongly discoloured and altered throughout the fragments, which tend to disintegrate under only moderate pressure." ;
    skos:inScheme glosis_cl:weatheringValueCode ;
    skos:notation "S" ;
    skos:prefLabel "Strongly weathered"@en ;
    skos:topConceptOf glosis_cl:weatheringValueCode .

glosis_cl:weatheringValueCode-W a glosis_cl:WeatheringValueCode,
        skos:Concept ;
    skos:definition "Partial weathering is indicated by discoloration and loss of crystal form in the outer parts of the fragments while the centres remain relatively fresh and the fragments have lost little of their original strength." ;
    skos:inScheme glosis_cl:weatheringValueCode ;
    skos:notation "W" ;
    skos:prefLabel "Weathered"@en ;
    skos:topConceptOf glosis_cl:weatheringValueCode .

