@prefix dct: <http://purl.org/dc/terms/> .
@prefix foaf: <http://xmlns.com/foaf/0.1/> .
@prefix glosis_proc: <http://w3id.org/glosis/model/procedure/> .
@prefix owl: <http://www.w3.org/2002/07/owl#> .
@prefix rdf: <http://www.w3.org/1999/02/22-rdf-syntax-ns#> .
@prefix rdfs: <http://www.w3.org/2000/01/rdf-schema#> .
@prefix schema: <https://schema.org/> .
@prefix skos: <http://www.w3.org/2004/02/skos/core#> .
@prefix sosa: <http://www.w3.org/ns/sosa/> .

<http://w3id.org/glosis/model/procedure> a owl:Ontology ;
    dct:creator [ rdfs:seeAlso <http://orcid.org/0000-0003-4289-4922> ;
            foaf:name "Raul Palma" ;
            schema:affiliation [ foaf:name "PSNC" ] ],
        [ foaf:name "Bogusz Janiak" ;
            schema:affiliation [ foaf:name "PSNC" ] ],
        [ rdfs:seeAlso <http://orcid.org/0000-0002-5851-2071> ;
            foaf:name "Luís Moreira de Sousa" ;
            schema:affiliation [ foaf:name "Técnico ULisboa" ] ] ;
    dct:description "This ontology represents the laboratory analysis procedures in GLOSIS, an extension to the Global Soil Information System (GloSIS) v1.0, edited by Tomas Reznik and Katharina Schleidt"@en ;
    dct:rights "This ontology is distributed under Creative Commons Attribution 4.0 License - http://creativecommons.org/licenses/by/4.0"@en ;
    dct:source "Data model for the Global Soil Information System (GloSIS) v1.0, edited by Tomas Reznik and Katharina Schleidt and Africa Soil Profile Database"@en ;
    dct:title "GLOSIS Procedures"@en ;
    rdfs:comment "This module contains the code lists identifying laboratory processes employed to assess physio-chemical soil properties."@en ;
    owl:versionIRI glosis_proc:v1.5.1 ;
    owl:versionInfo "v1.5.1" .

glosis_proc:acidityExchangeableProcedure a skos:ConceptScheme ;
    rdfs:label "Code list for acidityExchangeable analysis procedures - codelist scheme"@en ;
    rdfs:seeAlso glosis_proc:AcidityExchangeableProcedure ;
    skos:definition "AfSP-derived interpretation (RwaSP)" ;
    skos:note "This code list provides analysis procedures for acidityExchangeable."@en ;
    skos:prefLabel "Code list for acidityExchangeable analysis procedures - codelist scheme"@en .

glosis_proc:availableWaterHoldingCapacityProcedure a skos:ConceptScheme ;
    rdfs:label "Code list for availableWaterHoldingCapacity analysis procedures - codelist scheme"@en ;
    rdfs:seeAlso glosis_proc:AvailableWaterHoldingCapacityProcedure ;
    skos:definition "AfSP-derived interpretation (RwaSP)" ;
    skos:note "This code list provides analysis procedures for availableWaterHoldingCapacity."@en ;
    skos:prefLabel "Code list for availableWaterHoldingCapacity analysis procedures - codelist scheme"@en .

glosis_proc:baseSaturationProcedure a skos:ConceptScheme ;
    rdfs:label "Code list for baseSaturation analysis procedures - codelist scheme"@en ;
    rdfs:seeAlso glosis_proc:BaseSaturationProcedure ;
    skos:definition "AfSP-derived interpretation (RwaSP)" ;
    skos:note "This code list provides analysis procedures for baseSaturation."@en ;
    skos:prefLabel "Code list for baseSaturation analysis procedures - codelist scheme"@en .

glosis_proc:bulkDensityFineEarthProcedure a skos:ConceptScheme ;
    rdfs:label "Code list for bulkDensityFineEarth analysis procedures - codelist scheme"@en ;
    rdfs:seeAlso glosis_proc:BulkDensityFineEarthProcedure ;
    skos:definition "AfSP-derived interpretation (RwaSP)" ;
    skos:note "This code list provides analysis procedures for bulkDensityFineEarth."@en ;
    skos:prefLabel "Code list for bulkDensityFineEarth analysis procedures - codelist scheme"@en .

glosis_proc:bulkDensityWholeSoilProcedure a skos:ConceptScheme ;
    rdfs:label "Code list for bulkDensityWholeSoil analysis procedures - codelist scheme"@en ;
    rdfs:seeAlso glosis_proc:BulkDensityWholeSoilProcedure ;
    skos:definition "AfSP-derived interpretation (RwaSP)" ;
    skos:note "This code list provides analysis procedures for bulkDensityWholeSoil."@en ;
    skos:prefLabel "Code list for bulkDensityWholeSoil analysis procedures - codelist scheme"@en .

glosis_proc:carbonInorganicProcedure a skos:ConceptScheme ;
    rdfs:label "Code list for carbonInorganic analysis procedures - codelist scheme"@en ;
    rdfs:seeAlso glosis_proc:CarbonInorganicProcedure ;
    skos:definition "AfSP-derived interpretation (RwaSP)" ;
    skos:note "This code list provides analysis procedures for carbonInorganic."@en ;
    skos:prefLabel "Code list for carbonInorganic analysis procedures - codelist scheme"@en .

glosis_proc:carbonOrganicProcedure a skos:ConceptScheme ;
    rdfs:label "Code list for carbonOrganic analysis procedures - codelist scheme"@en ;
    rdfs:seeAlso glosis_proc:CarbonOrganicProcedure ;
    skos:definition "AfSP-derived interpretation (RwaSP)" ;
    skos:note "This code list provides analysis procedures for carbonOrganic."@en ;
    skos:prefLabel "Code list for carbonOrganic analysis procedures - codelist scheme"@en .

glosis_proc:carbonTotalProcedure a skos:ConceptScheme ;
    rdfs:label "Code list for carbonTotal analysis procedures - codelist scheme"@en ;
    rdfs:seeAlso glosis_proc:CarbonTotalProcedure ;
    skos:definition "AfSP-derived interpretation (RwaSP)" ;
    skos:note "This code list provides analysis procedures for carbonTotal."@en ;
    skos:prefLabel "Code list for carbonTotal analysis procedures - codelist scheme"@en .

glosis_proc:cationExchangeCapacitySoilProcedure a skos:ConceptScheme ;
    rdfs:label "Code list for cationExchangeCapacitySoil analysis procedures - codelist scheme"@en ;
    rdfs:seeAlso glosis_proc:CationExchangeCapacitySoilProcedure ;
    skos:definition "AfSP-derived interpretation (RwaSP)" ;
    skos:note "This code list provides analysis procedures for cationExchangeCapacitySoil."@en ;
    skos:prefLabel "Code list for cationExchangeCapacitySoil analysis procedures - codelist scheme"@en .

glosis_proc:coarseFragmentsProcedure a skos:ConceptScheme ;
    rdfs:label "Code list for coarseFragments analysis procedures - codelist scheme"@en ;
    rdfs:seeAlso glosis_proc:CoarseFragmentsProcedure ;
    skos:definition "AfSP-derived interpretation (RwaSP)" ;
    skos:note "This code list provides analysis procedures for coarseFragments."@en ;
    skos:prefLabel "Code list for coarseFragments analysis procedures - codelist scheme"@en .

glosis_proc:effectiveCecProcedure a skos:ConceptScheme ;
    rdfs:label "Code list for effectiveCec analysis procedures - codelist scheme"@en ;
    rdfs:seeAlso glosis_proc:EffectiveCecProcedure ;
    skos:definition "AfSP-derived interpretation (RwaSP)" ;
    skos:note "This code list provides analysis procedures for effectiveCec."@en ;
    skos:prefLabel "Code list for effectiveCec analysis procedures - codelist scheme"@en .

glosis_proc:electricalConductivityProcedure a skos:ConceptScheme ;
    rdfs:label "Code list for electricalConductivity analysis procedures - codelist scheme"@en ;
    rdfs:seeAlso glosis_proc:ElectricalConductivityProcedure ;
    skos:definition "AfSP-derived interpretation (RwaSP)" ;
    skos:note "This code list provides analysis procedures for electricalConductivity."@en ;
    skos:prefLabel "Code list for electricalConductivity analysis procedures - codelist scheme"@en .

glosis_proc:exchangeableBasesProcedure a skos:ConceptScheme ;
    rdfs:label "Code list for exchangeableBases analysis procedures - codelist scheme"@en ;
    rdfs:seeAlso glosis_proc:ExchangeableBasesProcedure ;
    skos:definition "AfSP-derived interpretation (RwaSP)" ;
    skos:note "This code list provides analysis procedures for exchangeableBases."@en ;
    skos:prefLabel "Code list for exchangeableBases analysis procedures - codelist scheme"@en .

glosis_proc:extractableElementsProcedure a skos:ConceptScheme ;
    rdfs:label "Code list for extractableElements analysis procedures - codelist scheme"@en ;
    rdfs:seeAlso glosis_proc:ExtractableElementsProcedure ;
    skos:definition "AfSP-derived interpretation (RwaSP)" ;
    skos:note "This code list provides analysis procedures for extractableElements."@en ;
    skos:prefLabel "Code list for extractableElements analysis procedures - codelist scheme"@en .

glosis_proc:gypsumProcedure a skos:ConceptScheme ;
    rdfs:label "Code list for gypsum analysis procedures - codelist scheme"@en ;
    rdfs:seeAlso glosis_proc:GypsumProcedure ;
    skos:definition "AfSP-derived interpretation (RwaSP)" ;
    skos:note "This code list provides analysis procedures for gypsum."@en ;
    skos:prefLabel "Code list for gypsum analysis procedures - codelist scheme"@en .

glosis_proc:hydraulicConductivityProcedure a skos:ConceptScheme ;
    rdfs:label "Code list for hydraulicConductivity analysis procedures - codelist scheme"@en ;
    rdfs:seeAlso glosis_proc:HydraulicConductivityProcedure ;
    skos:definition "AfSP-derived interpretation (RwaSP)" ;
    skos:note "This code list provides analysis procedures for hydraulicConductivity."@en ;
    skos:prefLabel "Code list for hydraulicConductivity analysis procedures - codelist scheme"@en .

glosis_proc:moistureContentProcedure a skos:ConceptScheme ;
    rdfs:label "Code list for moistureContent analysis procedures - codelist scheme"@en ;
    rdfs:seeAlso glosis_proc:MoistureContentProcedure ;
    skos:definition "AfSP-derived interpretation (RwaSP)" ;
    skos:note "This code list provides analysis procedures for moistureContent."@en ;
    skos:prefLabel "Code list for moistureContent analysis procedures - codelist scheme"@en .

glosis_proc:nitrogenTotalProcedure a skos:ConceptScheme ;
    rdfs:label "Code list for nitrogenTotal analysis procedures - codelist scheme"@en ;
    rdfs:seeAlso glosis_proc:NitrogenTotalProcedure ;
    skos:definition "AfSP-derived interpretation (RwaSP)" ;
    skos:note "This code list provides analysis procedures for nitrogenTotal."@en ;
    skos:prefLabel "Code list for nitrogenTotal analysis procedures - codelist scheme"@en .

glosis_proc:organicMatterProcedure a skos:ConceptScheme ;
    rdfs:label "Code list for organicMatter analysis procedures - codelist scheme"@en ;
    rdfs:seeAlso glosis_proc:OrganicMatterProcedure ;
    skos:definition "AfSP-derived interpretation (RwaSP)" ;
    skos:note "This code list provides analysis procedures for organicMatter."@en ;
    skos:prefLabel "Code list for organicMatter analysis procedures - codelist scheme"@en .

glosis_proc:pHProcedure a skos:ConceptScheme ;
    rdfs:label "Code list for pH analysis procedures - codelist scheme"@en ;
    rdfs:seeAlso glosis_proc:PHProcedure ;
    skos:definition "AfSP-derived interpretation (RwaSP)" ;
    skos:note "This code list provides analysis procedures for pH."@en ;
    skos:prefLabel "Code list for pH analysis procedures - codelist scheme"@en .

glosis_proc:pSAProcedure a skos:ConceptScheme ;
    rdfs:label "Code list for pSA analysis procedures - codelist scheme"@en ;
    rdfs:seeAlso glosis_proc:PSAProcedure ;
    skos:definition "AfSP-derived interpretation (RwaSP)" ;
    skos:note "This code list provides analysis procedures for pSA."@en ;
    skos:prefLabel "Code list for pSA analysis procedures - codelist scheme"@en .

glosis_proc:phosphorusRetentionProcedure a skos:ConceptScheme ;
    rdfs:label "Code list for phosphorusRetention analysis procedures - codelist scheme"@en ;
    rdfs:seeAlso glosis_proc:PhosphorusRetentionProcedure ;
    skos:definition "AfSP-derived interpretation (RwaSP)" ;
    skos:note "This code list provides analysis procedures for phosphorusRetention."@en ;
    skos:prefLabel "Code list for phosphorusRetention analysis procedures - codelist scheme"@en .

glosis_proc:porosityProcedure a skos:ConceptScheme ;
    rdfs:label "Code list for porosity analysis procedures - codelist scheme"@en ;
    rdfs:seeAlso glosis_proc:PorosityProcedure ;
    skos:definition "AfSP-derived interpretation (RwaSP)" ;
    skos:note "This code list provides analysis procedures for porosity."@en ;
    skos:prefLabel "Code list for porosity analysis procedures - codelist scheme"@en .

glosis_proc:solubleSaltsProcedure a skos:ConceptScheme ;
    rdfs:label "Code list for solubleSalts analysis procedures - codelist scheme"@en ;
    rdfs:seeAlso glosis_proc:SolubleSaltsProcedure ;
    skos:definition "AfSP-derived interpretation (RwaSP)" ;
    skos:note "This code list provides analysis procedures for solubleSalts."@en ;
    skos:prefLabel "Code list for solubleSalts analysis procedures - codelist scheme"@en .

glosis_proc:textureSumProcedure a skos:ConceptScheme ;
    rdfs:label "Code list for textureSum analysis procedures - codelist scheme"@en ;
    rdfs:seeAlso glosis_proc:TextureSumProcedure ;
    skos:definition "AfSP-derived interpretation (RwaSP)" ;
    skos:note "This code list provides analysis procedures for textureSum."@en ;
    skos:prefLabel "Code list for textureSum analysis procedures - codelist scheme"@en .

glosis_proc:totalCarbonateEquivalentProcedure a skos:ConceptScheme ;
    rdfs:label "Code list for totalCarbonateEquivalent analysis procedures - codelist scheme"@en ;
    rdfs:seeAlso glosis_proc:TotalCarbonateEquivalentProcedure ;
    skos:definition "AfSP-derived interpretation (RwaSP)" ;
    skos:note "This code list provides analysis procedures for totalCarbonateEquivalent."@en ;
    skos:prefLabel "Code list for totalCarbonateEquivalent analysis procedures - codelist scheme"@en .

glosis_proc:totalElementsProcedure a skos:ConceptScheme ;
    rdfs:label "Code list for totalElements analysis procedures - codelist scheme"@en ;
    rdfs:seeAlso glosis_proc:TotalElementsProcedure ;
    skos:definition "AfSP-derived interpretation (RwaSP)" ;
    skos:note "This code list provides analysis procedures for totalElements."@en ;
    skos:prefLabel "Code list for totalElements analysis procedures - codelist scheme"@en .

glosis_proc:AcidityExchangeableProcedure a owl:Class ;
    rdfs:label "Procedures for AcidityExchangeable - codelist class"@en ;
    rdfs:comment "This code list provides analysis procedures for AcidityExchangeable."@en ;
    rdfs:seeAlso glosis_proc:acidityExchangeableProcedure ;
    rdfs:subClassOf skos:Concept,
        sosa:Procedure ;
    owl:oneOf ( glosis_proc:acidityExchangeableProcedure-ExchAcid_ph7-unkn glosis_proc:acidityExchangeableProcedure-ExchAcid_ph0-unkn glosis_proc:acidityExchangeableProcedure-ExchAcid_ph8-bacl2tea glosis_proc:acidityExchangeableProcedure-ExchAcid_ph0-kcl1m glosis_proc:acidityExchangeableProcedure-ExchAcid_ph0-nh4cl glosis_proc:acidityExchangeableProcedure-ExchAcid_ph7-caoac glosis_proc:acidityExchangeableProcedure-ExchAcid_ph8-unkn ) .

glosis_proc:AvailableWaterHoldingCapacityProcedure a owl:Class ;
    rdfs:label "Procedures for AvailableWaterHoldingCapacity - codelist class"@en ;
    rdfs:comment "This code list provides analysis procedures for AvailableWaterHoldingCapacity."@en ;
    rdfs:seeAlso glosis_proc:availableWaterHoldingCapacityProcedure ;
    rdfs:subClassOf skos:Concept,
        sosa:Procedure ;
    owl:oneOf ( glosis_proc:availableWaterHoldingCapacityProcedure-PAWHC_calcul-fc200wp glosis_proc:availableWaterHoldingCapacityProcedure-PAWHC_calcul-fc300wp glosis_proc:availableWaterHoldingCapacityProcedure-PAWHC_calcul-fc100wp ) .

glosis_proc:BaseSaturationProcedure a owl:Class ;
    rdfs:label "Procedures for BaseSaturation - codelist class"@en ;
    rdfs:comment "This code list provides analysis procedures for BaseSaturation."@en ;
    rdfs:seeAlso glosis_proc:baseSaturationProcedure ;
    rdfs:subClassOf skos:Concept,
        sosa:Procedure ;
    owl:oneOf ( glosis_proc:baseSaturationProcedure-BSat_calcul-ecec glosis_proc:baseSaturationProcedure-BSat_calcul-cec ) .

glosis_proc:BulkDensityFineEarthProcedure a owl:Class ;
    rdfs:label "Procedures for BulkDensityFineEarth - codelist class"@en ;
    rdfs:comment "This code list provides analysis procedures for BulkDensityFineEarth."@en ;
    rdfs:seeAlso glosis_proc:bulkDensityFineEarthProcedure ;
    rdfs:subClassOf skos:Concept,
        sosa:Procedure ;
    owl:oneOf ( glosis_proc:bulkDensityFineEarthProcedure-BlkDensF_fe-co-od glosis_proc:bulkDensityFineEarthProcedure-BlkDensF_fe-co-unkn glosis_proc:bulkDensityFineEarthProcedure-BlkDensF_fe-unkn-od glosis_proc:bulkDensityFineEarthProcedure-BlkDensF_fe-co-fc glosis_proc:bulkDensityFineEarthProcedure-BlkDensF_fe-rpl-unkn glosis_proc:bulkDensityFineEarthProcedure-BlkDensF_fe-cl-unkn glosis_proc:bulkDensityFineEarthProcedure-BlkDensF_fe-unkn-fc glosis_proc:bulkDensityFineEarthProcedure-BlkDensF_fe-cl-od glosis_proc:bulkDensityFineEarthProcedure-BlkDensF_fe-cl-fc glosis_proc:bulkDensityFineEarthProcedure-BlkDensF_fe-unkn ) .

glosis_proc:BulkDensityWholeSoilProcedure a owl:Class ;
    rdfs:label "Procedures for BulkDensityWholeSoil - codelist class"@en ;
    rdfs:comment "This code list provides analysis procedures for BulkDensityWholeSoil."@en ;
    rdfs:seeAlso glosis_proc:bulkDensityWholeSoilProcedure ;
    rdfs:subClassOf skos:Concept,
        sosa:Procedure ;
    owl:oneOf ( glosis_proc:bulkDensityWholeSoilProcedure-BlkDensW_we-unkn glosis_proc:bulkDensityWholeSoilProcedure-BlkDensW_we-cl-fc glosis_proc:bulkDensityWholeSoilProcedure-BlkDensW_we-cl-od glosis_proc:bulkDensityWholeSoilProcedure-BlkDensW_we-co-od glosis_proc:bulkDensityWholeSoilProcedure-BlkDensW_we-cl-unkn glosis_proc:bulkDensityWholeSoilProcedure-BlkDensW_we-co-fc glosis_proc:bulkDensityWholeSoilProcedure-BlkDensW_we-co-unkn glosis_proc:bulkDensityWholeSoilProcedure-BlkDensW_we-rpl-unkn ) .

glosis_proc:CarbonInorganicProcedure a owl:Class ;
    rdfs:label "Procedures for CarbonInorganic - codelist class"@en ;
    rdfs:comment "This code list provides analysis procedures for CarbonInorganic."@en ;
    rdfs:seeAlso glosis_proc:carbonInorganicProcedure ;
    rdfs:subClassOf skos:Concept,
        sosa:Procedure ;
    owl:oneOf ( glosis_proc:carbonInorganicProcedure-InOrgC_calcul-caco3 glosis_proc:carbonInorganicProcedure-InOrgC_calcul-tc-oc ) .

glosis_proc:CarbonOrganicProcedure a owl:Class ;
    rdfs:label "Procedures for CarbonOrganic - codelist class"@en ;
    rdfs:comment "This code list provides analysis procedures for CarbonOrganic."@en ;
    rdfs:seeAlso glosis_proc:carbonOrganicProcedure ;
    rdfs:subClassOf skos:Concept,
        sosa:Procedure ;
    owl:oneOf ( glosis_proc:carbonOrganicProcedure-OrgC_dc-lt-loi glosis_proc:carbonOrganicProcedure-OrgC_calcul-tc-ic glosis_proc:carbonOrganicProcedure-OrgC_wc-cro3-tiurin glosis_proc:carbonOrganicProcedure-OrgC_dc-lt glosis_proc:carbonOrganicProcedure-OrgC_acid-dc glosis_proc:carbonOrganicProcedure-OrgC_acid-dc-ht-analyser glosis_proc:carbonOrganicProcedure-OrgC_acid-dc-lt glosis_proc:carbonOrganicProcedure-OrgC_wc-cro3-nelson glosis_proc:carbonOrganicProcedure-OrgC_dc glosis_proc:carbonOrganicProcedure-OrgC_dc-ht glosis_proc:carbonOrganicProcedure-OrgC_acid-dc-lt-loi glosis_proc:carbonOrganicProcedure-OrgC_wc-cro3-walkleyblack glosis_proc:carbonOrganicProcedure-OrgC_acid-dc-ht glosis_proc:carbonOrganicProcedure-OrgC_dc-spec glosis_proc:carbonOrganicProcedure-OrgC_wc-cro3-knopp glosis_proc:carbonOrganicProcedure-OrgC_dc-ht-analyser glosis_proc:carbonOrganicProcedure-OrgC_wc-cro3-nrcs6a1c glosis_proc:carbonOrganicProcedure-OrgC_wc-cro3-kalembra glosis_proc:carbonOrganicProcedure-OrgC_acid-dc-mt glosis_proc:carbonOrganicProcedure-OrgC_wc glosis_proc:carbonOrganicProcedure-OrgC_wc-cro3-jackson glosis_proc:carbonOrganicProcedure-OrgC_acid-dc-spec glosis_proc:carbonOrganicProcedure-OrgC_wc-cro3-kurmies glosis_proc:carbonOrganicProcedure-OrgC_dc-mt ) .

glosis_proc:CarbonTotalProcedure a owl:Class ;
    rdfs:label "Procedures for CarbonTotal - codelist class"@en ;
    rdfs:comment "This code list provides analysis procedures for CarbonTotal."@en ;
    rdfs:seeAlso glosis_proc:carbonTotalProcedure ;
    rdfs:subClassOf skos:Concept,
        sosa:Procedure ;
    owl:oneOf ( glosis_proc:carbonTotalProcedure-TotC_dc-mt glosis_proc:carbonTotalProcedure-TotC_dc-ht-analyser glosis_proc:carbonTotalProcedure-TotC_dc-ht-spec glosis_proc:carbonTotalProcedure-TotC_calcul-ic-oc glosis_proc:carbonTotalProcedure-TotC_dc-ht ) .

glosis_proc:CationExchangeCapacitySoilProcedure a owl:Class ;
    rdfs:label "Procedures for CationExchangeCapacitySoil - codelist class"@en ;
    rdfs:comment "This code list provides analysis procedures for CationExchangeCapacitySoil."@en ;
    rdfs:seeAlso glosis_proc:cationExchangeCapacitySoilProcedure ;
    rdfs:subClassOf skos:Concept,
        sosa:Procedure ;
    owl:oneOf ( glosis_proc:cationExchangeCapacitySoilProcedure-CEC_ph0-cohex glosis_proc:cationExchangeCapacitySoilProcedure-CEC_ph8-baoac glosis_proc:cationExchangeCapacitySoilProcedure-CEC_ph8-nh4oac glosis_proc:cationExchangeCapacitySoilProcedure-CEC_ph0-nh4cl glosis_proc:cationExchangeCapacitySoilProcedure-CEC_ph8-unkn glosis_proc:cationExchangeCapacitySoilProcedure-CEC_ph-unkn-m3 glosis_proc:cationExchangeCapacitySoilProcedure-CEC_ph7-nh4oac glosis_proc:cationExchangeCapacitySoilProcedure-CEC_ph7-unkn glosis_proc:cationExchangeCapacitySoilProcedure-CEC_ph8-naoac glosis_proc:cationExchangeCapacitySoilProcedure-CEC_ph-unkn-cacl2 glosis_proc:cationExchangeCapacitySoilProcedure-CEC_ph0-kcl glosis_proc:cationExchangeCapacitySoilProcedure-CEC_ph7-edta glosis_proc:cationExchangeCapacitySoilProcedure-CEC_ph0-unkn glosis_proc:cationExchangeCapacitySoilProcedure-CEC_ph8-licl2tea glosis_proc:cationExchangeCapacitySoilProcedure-CEC_ph0-ag-thioura glosis_proc:cationExchangeCapacitySoilProcedure-CEC_ph0-bacl2 glosis_proc:cationExchangeCapacitySoilProcedure-CEC_ph8-bacl2tea glosis_proc:cationExchangeCapacitySoilProcedure-CEC_ph0-nh4oac glosis_proc:cationExchangeCapacitySoilProcedure-CEC_ph-unkn-lioac ) .

glosis_proc:CoarseFragmentsProcedure a owl:Class ;
    rdfs:label "Procedures for CoarseFragments - codelist class"@en ;
    rdfs:comment "This code list provides analysis procedures for CoarseFragments."@en ;
    rdfs:seeAlso glosis_proc:coarseFragmentsProcedure ;
    rdfs:subClassOf skos:Concept,
        sosa:Procedure ;
    owl:oneOf ( glosis_proc:coarseFragmentsProcedure-CrsFrg_fld glosis_proc:coarseFragmentsProcedure-CrsFrg_fldcls glosis_proc:coarseFragmentsProcedure-CrsFrg_lab ) .

glosis_proc:EffectiveCecProcedure a owl:Class ;
    rdfs:label "Procedures for EffectiveCec - codelist class"@en ;
    rdfs:comment "This code list provides analysis procedures for EffectiveCec."@en ;
    rdfs:seeAlso glosis_proc:effectiveCecProcedure ;
    rdfs:subClassOf skos:Concept,
        sosa:Procedure ;
    owl:oneOf ( glosis_proc:effectiveCecProcedure-EffCEC_calcul-b glosis_proc:effectiveCecProcedure-EffCEC_calcul-ba ) .

glosis_proc:ElectricalConductivityProcedure a owl:Class ;
    rdfs:label "Procedures for ElectricalConductivity - codelist class"@en ;
    rdfs:comment "This code list provides analysis procedures for ElectricalConductivity."@en ;
    rdfs:seeAlso glosis_proc:electricalConductivityProcedure ;
    rdfs:subClassOf skos:Concept,
        sosa:Procedure ;
    owl:oneOf ( glosis_proc:electricalConductivityProcedure-EC_ratio1-10 glosis_proc:electricalConductivityProcedure-EC_ratio1-2 glosis_proc:electricalConductivityProcedure-EC_ratio1-2.5 glosis_proc:electricalConductivityProcedure-EC_ratio1-5 glosis_proc:electricalConductivityProcedure-ECe_sat glosis_proc:electricalConductivityProcedure-EC_ratio1-1 ) .

glosis_proc:ExchangeableBasesProcedure a owl:Class ;
    rdfs:label "Procedures for ExchangeableBases - codelist class"@en ;
    rdfs:comment "This code list provides analysis procedures for ExchangeableBases."@en ;
    rdfs:seeAlso glosis_proc:exchangeableBasesProcedure ;
    rdfs:subClassOf skos:Concept,
        sosa:Procedure ;
    owl:oneOf ( glosis_proc:exchangeableBasesProcedure-ExchBases_ph7-nh4oac-fp glosis_proc:exchangeableBasesProcedure-ExchBases_ph8-bacl2tea glosis_proc:exchangeableBasesProcedure-ExchBases_ph-unkn-edta glosis_proc:exchangeableBasesProcedure-ExchBases_ph-unkn-m3 glosis_proc:exchangeableBasesProcedure-ExchBases_ph0-nh4cl glosis_proc:exchangeableBasesProcedure-ExchBases_ph8-unkn glosis_proc:exchangeableBasesProcedure-ExchBases_ph7-nh4oac glosis_proc:exchangeableBasesProcedure-ExchBases_ph0-cohex glosis_proc:exchangeableBasesProcedure-ExchBases_ph7-unkn glosis_proc:exchangeableBasesProcedure-ExchBases_ph-unkn-m3-spec glosis_proc:exchangeableBasesProcedure-ExchBases_ph7-nh4oac-aas ) .

glosis_proc:ExtractableElementsProcedure a owl:Class ;
    rdfs:label "Procedures for ExtractableElements - codelist class"@en ;
    rdfs:comment "This code list provides analysis procedures for ExtractableElements."@en ;
    rdfs:seeAlso glosis_proc:extractableElementsProcedure ;
    rdfs:subClassOf skos:Concept,
        sosa:Procedure ;
    owl:oneOf ( glosis_proc:extractableElementsProcedure-Extr_ap15 glosis_proc:extractableElementsProcedure-Extr_edta glosis_proc:extractableElementsProcedure-Extr_nahco3-olsen glosis_proc:extractableElementsProcedure-Extr_hcl-nh4f-bray1 glosis_proc:extractableElementsProcedure-Extr_ap20 glosis_proc:extractableElementsProcedure-Extr_hotwater glosis_proc:extractableElementsProcedure-Extr_m3 glosis_proc:extractableElementsProcedure-Extr_nahco3-olsen-dabin glosis_proc:extractableElementsProcedure-Extr_hcl-nh4f-kurtz-bray glosis_proc:extractableElementsProcedure-Extr_ap21 glosis_proc:extractableElementsProcedure-Extr_capo4 glosis_proc:extractableElementsProcedure-Extr_m1 glosis_proc:extractableElementsProcedure-Extr_dtpa glosis_proc:extractableElementsProcedure-Extr_hcl-h2so4-nelson glosis_proc:extractableElementsProcedure-Extr_nh4ch3ch-oh-cooh-leuven glosis_proc:extractableElementsProcedure-Extr_cacl2 glosis_proc:extractableElementsProcedure-Extr_c6h8o7-reeuwijk glosis_proc:extractableElementsProcedure-Extr_hno3 glosis_proc:extractableElementsProcedure-Extr_m2 glosis_proc:extractableElementsProcedure-Extr_m3-spec glosis_proc:extractableElementsProcedure-Extr_naoac-morgan glosis_proc:extractableElementsProcedure-Extr_h2so4-truog glosis_proc:extractableElementsProcedure-Extr_nh4-co3-2-ambic1 glosis_proc:extractableElementsProcedure-Extr_ap14 glosis_proc:extractableElementsProcedure-Extr_hcl-nh4f-bray2 ) .

glosis_proc:GypsumProcedure a owl:Class ;
    rdfs:label "Procedures for Gypsum - codelist class"@en ;
    rdfs:comment "This code list provides analysis procedures for Gypsum."@en ;
    rdfs:seeAlso glosis_proc:gypsumProcedure ;
    rdfs:subClassOf skos:Concept,
        sosa:Procedure ;
    owl:oneOf ( glosis_proc:gypsumProcedure-CaSO4_gy01 glosis_proc:gypsumProcedure-CaSO4_gy06 glosis_proc:gypsumProcedure-CaSO4_gy07 glosis_proc:gypsumProcedure-CaSO4_gy04 glosis_proc:gypsumProcedure-CaSO4_gy03 glosis_proc:gypsumProcedure-CaSO4_gy05 glosis_proc:gypsumProcedure-CaSO4_gy02 ) .

glosis_proc:HydraulicConductivityProcedure a owl:Class ;
    rdfs:label "Procedures for HydraulicConductivity - codelist class"@en ;
    rdfs:comment "This code list provides analysis procedures for HydraulicConductivity."@en ;
    rdfs:seeAlso glosis_proc:hydraulicConductivityProcedure ;
    rdfs:subClassOf skos:Concept,
        sosa:Procedure ;
    owl:oneOf ( glosis_proc:hydraulicConductivityProcedure-KSat_calcul-ptf-saxton glosis_proc:hydraulicConductivityProcedure-Ksat_invbhole glosis_proc:hydraulicConductivityProcedure-KSat_calcul-ptf glosis_proc:hydraulicConductivityProcedure-KSat_calcul-ptf-genuchten glosis_proc:hydraulicConductivityProcedure-Ksat_column glosis_proc:hydraulicConductivityProcedure-Ksat_dblring glosis_proc:hydraulicConductivityProcedure-Ksat_bhole ) .

glosis_proc:MoistureContentProcedure a owl:Class ;
    rdfs:label "Procedures for MoistureContent - codelist class"@en ;
    rdfs:comment "This code list provides analysis procedures for MoistureContent."@en ;
    rdfs:seeAlso glosis_proc:moistureContentProcedure ;
    rdfs:subClassOf skos:Concept,
        sosa:Procedure ;
    owl:oneOf ( glosis_proc:moistureContentProcedure-VMC_ud glosis_proc:moistureContentProcedure-VMC_d-cl-ww glosis_proc:moistureContentProcedure-VMC_calcul-ptf-brookscorey glosis_proc:moistureContentProcedure-VMC_d-ww glosis_proc:moistureContentProcedure-VMC_calcul-ptf glosis_proc:moistureContentProcedure-VMC_d-cl glosis_proc:moistureContentProcedure-VMC_d glosis_proc:moistureContentProcedure-VMC_ud-co glosis_proc:moistureContentProcedure-VMC_ud-cl ) .

glosis_proc:NitrogenTotalProcedure a owl:Class ;
    rdfs:label "Procedures for NitrogenTotal - codelist class"@en ;
    rdfs:comment "This code list provides analysis procedures for NitrogenTotal."@en ;
    rdfs:seeAlso glosis_proc:nitrogenTotalProcedure ;
    rdfs:subClassOf skos:Concept,
        sosa:Procedure ;
    owl:oneOf ( glosis_proc:nitrogenTotalProcedure-TotalN_h2so4 glosis_proc:nitrogenTotalProcedure-TotalN_calcul glosis_proc:nitrogenTotalProcedure-TotalN_kjeldahl glosis_proc:nitrogenTotalProcedure-TotalN_dc-spec glosis_proc:nitrogenTotalProcedure-TotalN_dc-ht-dumas glosis_proc:nitrogenTotalProcedure-TotalN_kjeldahl-nh4 glosis_proc:nitrogenTotalProcedure-TotalN_tn08 glosis_proc:nitrogenTotalProcedure-TotalN_tn04 glosis_proc:nitrogenTotalProcedure-TotalN_calcul-oc10 glosis_proc:nitrogenTotalProcedure-TotalN_nelson glosis_proc:nitrogenTotalProcedure-TotalN_dc glosis_proc:nitrogenTotalProcedure-TotalN_tn06 glosis_proc:nitrogenTotalProcedure-TotalN_bremner glosis_proc:nitrogenTotalProcedure-TotalN_dc-ht-leco ) .

glosis_proc:OrganicMatterProcedure a owl:Class ;
    rdfs:label "Procedures for OrganicMatter - codelist class"@en ;
    rdfs:comment "This code list provides analysis procedures for OrganicMatter."@en ;
    rdfs:seeAlso glosis_proc:organicMatterProcedure ;
    rdfs:subClassOf skos:Concept,
        sosa:Procedure ;
    owl:oneOf ( glosis_proc:organicMatterProcedure-HumAcidC_unkn glosis_proc:organicMatterProcedure-FulAcidC_unkn glosis_proc:organicMatterProcedure-TotHumC_unkn glosis_proc:organicMatterProcedure-OrgM_calcul-oc1.73 ) .

glosis_proc:PHProcedure a owl:Class ;
    rdfs:label "Procedures for PH - codelist class"@en ;
    rdfs:comment "This code list provides analysis procedures for PH."@en ;
    rdfs:seeAlso glosis_proc:pHProcedure ;
    rdfs:subClassOf skos:Concept,
        sosa:Procedure ;
    owl:oneOf ( glosis_proc:pHProcedure-pHNaF_ratio1-5 glosis_proc:pHProcedure-pHH2O glosis_proc:pHProcedure-pHNaF_ratio1-1 glosis_proc:pHProcedure-pHCaCl2_sat glosis_proc:pHProcedure-pHH2O_sat glosis_proc:pHProcedure-pHNaF_ratio1-2.5 glosis_proc:pHProcedure-pHCaCl2_ratio1-1 glosis_proc:pHProcedure-pHKCl_sat glosis_proc:pHProcedure-pHKCl_ratio1-2 glosis_proc:pHProcedure-pHH2O_unkn-spec glosis_proc:pHProcedure-pHKCl_ratio1-5 glosis_proc:pHProcedure-pHNaF_ratio1-2 glosis_proc:pHProcedure-pHKCl glosis_proc:pHProcedure-pHH2O_ratio1-2.5 glosis_proc:pHProcedure-pHCaCl2_ratio1-5 glosis_proc:pHProcedure-pHH2O_ratio1-1 glosis_proc:pHProcedure-pHCaCl2 glosis_proc:pHProcedure-pHH2O_ratio1-2 glosis_proc:pHProcedure-pHCaCl2_ratio1-10 glosis_proc:pHProcedure-pHH2O_ratio1-5 glosis_proc:pHProcedure-pHKCl_ratio1-1 glosis_proc:pHProcedure-pHCaCl2_ratio1-2 glosis_proc:pHProcedure-pHCaCl2_ratio1-2.5 glosis_proc:pHProcedure-pHNaF_sat glosis_proc:pHProcedure-pHNaF glosis_proc:pHProcedure-pHKCl_ratio1-2.5 glosis_proc:pHProcedure-pHNaF_ratio1-10 glosis_proc:pHProcedure-pHH2O_ratio1-10 glosis_proc:pHProcedure-pHKCl_ratio1-10 ) .

glosis_proc:PSAProcedure a owl:Class ;
    rdfs:label "Procedures for PSA - codelist class"@en ;
    rdfs:comment "This code list provides analysis procedures for PSA."@en ;
    rdfs:seeAlso glosis_proc:pSAProcedure ;
    rdfs:subClassOf skos:Concept,
        sosa:Procedure ;
    owl:oneOf ( glosis_proc:pSAProcedure-fldest glosis_proc:pSAProcedure-laser-disp glosis_proc:pSAProcedure-laser-nodisp glosis_proc:pSAProcedure-laser-unkdisp glosis_proc:pSAProcedure-beaker-disp glosis_proc:pSAProcedure-beaker-nodisp glosis_proc:pSAProcedure-beaker-unkdisp glosis_proc:pSAProcedure-pipette-disp glosis_proc:pSAProcedure-pipette-nodisp glosis_proc:pSAProcedure-pipette-unkdisp glosis_proc:pSAProcedure-hydrometer-disp glosis_proc:pSAProcedure-hydrometer-nodisp glosis_proc:pSAProcedure-hydrometer-unkdisp glosis_proc:pSAProcedure-laser-disp-spec glosis_proc:pSAProcedure-laser-nodisp-spec glosis_proc:pSAProcedure-laser-unkdisp-spec glosis_proc:pSAProcedure-beaker-disp-spec glosis_proc:pSAProcedure-beaker-nodisp-spec glosis_proc:pSAProcedure-beaker-unkdisp-spec glosis_proc:pSAProcedure-pipette-disp-spec glosis_proc:pSAProcedure-pipette-nodisp-spec glosis_proc:pSAProcedure-pipette-unkdisp-spec glosis_proc:pSAProcedure-hydrometer-disp-spec glosis_proc:pSAProcedure-hydrometer-nodisp-spec glosis_proc:pSAProcedure-hydrometer-unkdisp-spec ) .

glosis_proc:PhosphorusRetentionProcedure a owl:Class ;
    rdfs:label "Procedures for PhosphorusRetention - codelist class"@en ;
    rdfs:comment "This code list provides analysis procedures for PhosphorusRetention."@en ;
    rdfs:seeAlso glosis_proc:phosphorusRetentionProcedure ;
    rdfs:subClassOf skos:Concept,
        sosa:Procedure ;
    owl:oneOf ( glosis_proc:phosphorusRetentionProcedure-RetentP_unkn-spec glosis_proc:phosphorusRetentionProcedure-RetentP_blakemore ) .

glosis_proc:PorosityProcedure a owl:Class ;
    rdfs:label "Procedures for Porosity - codelist class"@en ;
    rdfs:comment "This code list provides analysis procedures for Porosity."@en ;
    rdfs:seeAlso glosis_proc:porosityProcedure ;
    rdfs:subClassOf skos:Concept,
        sosa:Procedure ;
    owl:oneOf ( glosis_proc:porosityProcedure-Poros_calcul-pf0 ) .

glosis_proc:SolubleSaltsProcedure a owl:Class ;
    rdfs:label "Procedures for SolubleSalts - codelist class"@en ;
    rdfs:comment "This code list provides analysis procedures for SolubleSalts."@en ;
    rdfs:seeAlso glosis_proc:solubleSaltsProcedure ;
    rdfs:subClassOf skos:Concept,
        sosa:Procedure ;
    owl:oneOf ( glosis_proc:solubleSaltsProcedure-SlbAn_calcul-unkn glosis_proc:solubleSaltsProcedure-SlbCat_calcul-unkn ) .

glosis_proc:TextureSumProcedure a owl:Class ;
    rdfs:label "Procedures for TextureSum - codelist class"@en ;
    rdfs:comment "This code list provides analysis procedures for TextureSum."@en ;
    rdfs:seeAlso glosis_proc:textureSumProcedure ;
    rdfs:subClassOf skos:Concept,
        sosa:Procedure ;
    owl:oneOf ( glosis_proc:textureSumProcedure-SumTxtr_calcul ) .

glosis_proc:TotalCarbonateEquivalentProcedure a owl:Class ;
    rdfs:label "Procedures for TotalCarbonateEquivalent - codelist class"@en ;
    rdfs:comment "This code list provides analysis procedures for TotalCarbonateEquivalent."@en ;
    rdfs:seeAlso glosis_proc:totalCarbonateEquivalentProcedure ;
    rdfs:subClassOf skos:Concept,
        sosa:Procedure ;
    owl:oneOf ( glosis_proc:totalCarbonateEquivalentProcedure-CaCO3_acid-h3po4-dc glosis_proc:totalCarbonateEquivalentProcedure-CaCO3_acid-h2so4-nodc glosis_proc:totalCarbonateEquivalentProcedure-CaCO3_acid-ch3cooh-unkn glosis_proc:totalCarbonateEquivalentProcedure-CaCO3_acid-dc glosis_proc:totalCarbonateEquivalentProcedure-CaCO3_acid-h2so4-dc glosis_proc:totalCarbonateEquivalentProcedure-CaCO3_ca11 glosis_proc:totalCarbonateEquivalentProcedure-CaCO3_acid-hcl-dc glosis_proc:totalCarbonateEquivalentProcedure-CaCO3_calcul-tc-oc glosis_proc:totalCarbonateEquivalentProcedure-CaCO3_ca01 glosis_proc:totalCarbonateEquivalentProcedure-CaCO3_ca10 glosis_proc:totalCarbonateEquivalentProcedure-CaCO3_ca04 glosis_proc:totalCarbonateEquivalentProcedure-CaCO3_acid-h2so4-unkn glosis_proc:totalCarbonateEquivalentProcedure-CaCO3_acid-hcl-unkn glosis_proc:totalCarbonateEquivalentProcedure-CaCO3_ca12 glosis_proc:totalCarbonateEquivalentProcedure-CaCO3_ca08 glosis_proc:totalCarbonateEquivalentProcedure-CaCO3_ca07 glosis_proc:totalCarbonateEquivalentProcedure-CaCO3_ca09 glosis_proc:totalCarbonateEquivalentProcedure-CaCO3_acid-ch3cooh-nodc glosis_proc:totalCarbonateEquivalentProcedure-CaCO3_acid-ch3cooh-dc glosis_proc:totalCarbonateEquivalentProcedure-CaCO3_ca06 glosis_proc:totalCarbonateEquivalentProcedure-CaCO3_acid-h3po4-unkn glosis_proc:totalCarbonateEquivalentProcedure-CaCO3_ca03 glosis_proc:totalCarbonateEquivalentProcedure-CaCO3_acid-h3po4-nodc glosis_proc:totalCarbonateEquivalentProcedure-CaCO3_ca05 glosis_proc:totalCarbonateEquivalentProcedure-CaCO3_acid-hcl-nodc glosis_proc:totalCarbonateEquivalentProcedure-CaCO3_acid-unkn glosis_proc:totalCarbonateEquivalentProcedure-CaCO3_ca02 glosis_proc:totalCarbonateEquivalentProcedure-CaCO3_acid-nodc ) .

glosis_proc:TotalElementsProcedure a owl:Class ;
    rdfs:label "Procedures for TotalElements - codelist class"@en ;
    rdfs:comment "This code list provides analysis procedures for TotalElements."@en ;
    rdfs:seeAlso glosis_proc:totalElementsProcedure ;
    rdfs:subClassOf skos:Concept,
        sosa:Procedure ;
    owl:oneOf ( glosis_proc:totalElementsProcedure-Total_nh4-6mo7o24 glosis_proc:totalElementsProcedure-Total_tp05 glosis_proc:totalElementsProcedure-Total_hcl-aquaregia glosis_proc:totalElementsProcedure-Total_xrf glosis_proc:totalElementsProcedure-Total_xrd glosis_proc:totalElementsProcedure-Total_xrf-p glosis_proc:totalElementsProcedure-Total_tp03 glosis_proc:totalElementsProcedure-Total_hcl glosis_proc:totalElementsProcedure-Total_hclo4 glosis_proc:totalElementsProcedure-Total_tp10 glosis_proc:totalElementsProcedure-Total_tp07 glosis_proc:totalElementsProcedure-Total_unkn glosis_proc:totalElementsProcedure-Total_tp04 glosis_proc:totalElementsProcedure-Total_tp09 glosis_proc:totalElementsProcedure-Total_tp08 glosis_proc:totalElementsProcedure-Total_h2so4 glosis_proc:totalElementsProcedure-Total_tp06 glosis_proc:totalElementsProcedure-Total_xtf-t glosis_proc:totalElementsProcedure-Total_hno3-aquafortis ) .

glosis_proc:acidityExchangeableProcedure-ExchAcid_ph0-kcl1m a glosis_proc:AcidityExchangeableProcedure,
        skos:Concept ;
    skos:definition "Exch acidity (H+Al) unbuffered, in 1 M KCl extract" ;
    skos:inScheme glosis_proc:acidityExchangeableProcedure ;
    skos:notation "ExchAcid_ph0-kcl1m" ;
    skos:prefLabel "ExchAcid_ph0-kcl1m"@en ;
    skos:scopeNote <https://www.isric.org/sites/default/files/isric_report_2014_01.pdf>,
        "Leenaars J.G.B., A.J.M. van Oostrum and M. Ruiperez Gonzalez, 2014. Africa Soil Profiles Database, Version 1.2. A compilation of georeferenced and standardised legacy soil profile data for Sub-Saharan Africa (with dataset). ISRIC Report 2014/01. Africa Soil Information Service (AfSIS) project and ISRIC - World Soil Information, Wageningen, the Netherlands. See Annex 4." ;
    skos:topConceptOf glosis_proc:acidityExchangeableProcedure .

glosis_proc:acidityExchangeableProcedure-ExchAcid_ph0-nh4cl a glosis_proc:AcidityExchangeableProcedure,
        skos:Concept ;
    skos:definition "Exch acidity (H+Al) unbuffered, in 0.05-0.1 M NH4Cl extract" ;
    skos:inScheme glosis_proc:acidityExchangeableProcedure ;
    skos:notation "ExchAcid_ph0-nh4cl" ;
    skos:prefLabel "ExchAcid_ph0-nh4cl"@en ;
    skos:scopeNote <https://www.isric.org/sites/default/files/isric_report_2014_01.pdf>,
        "Leenaars J.G.B., A.J.M. van Oostrum and M. Ruiperez Gonzalez, 2014. Africa Soil Profiles Database, Version 1.2. A compilation of georeferenced and standardised legacy soil profile data for Sub-Saharan Africa (with dataset). ISRIC Report 2014/01. Africa Soil Information Service (AfSIS) project and ISRIC - World Soil Information, Wageningen, the Netherlands. See Annex 4." ;
    skos:topConceptOf glosis_proc:acidityExchangeableProcedure .

glosis_proc:acidityExchangeableProcedure-ExchAcid_ph0-unkn a glosis_proc:AcidityExchangeableProcedure,
        skos:Concept ;
    skos:definition "Exch acidity (H+Al) unbuffered, in unknown extract" ;
    skos:inScheme glosis_proc:acidityExchangeableProcedure ;
    skos:notation "ExchAcid_ph0-unkn" ;
    skos:prefLabel "ExchAcid_ph0-unk"@en ;
    skos:scopeNote <https://www.isric.org/sites/default/files/isric_report_2014_01.pdf>,
        "Leenaars J.G.B., A.J.M. van Oostrum and M. Ruiperez Gonzalez, 2014. Africa Soil Profiles Database, Version 1.2. A compilation of georeferenced and standardised legacy soil profile data for Sub-Saharan Africa (with dataset). ISRIC Report 2014/01. Africa Soil Information Service (AfSIS) project and ISRIC - World Soil Information, Wageningen, the Netherlands. See Annex 4." ;
    skos:topConceptOf glosis_proc:acidityExchangeableProcedure .

glosis_proc:acidityExchangeableProcedure-ExchAcid_ph7-caoac a glosis_proc:AcidityExchangeableProcedure,
        skos:Concept ;
    skos:definition "Exch acidity (H+Al) buffered at pH 7, in 1M Ca-acetate extract" ;
    skos:inScheme glosis_proc:acidityExchangeableProcedure ;
    skos:notation "ExchAcid_ph7-caoac" ;
    skos:prefLabel "ExchAcid_ph7-caoac"@en ;
    skos:scopeNote <https://www.isric.org/sites/default/files/isric_report_2014_01.pdf>,
        "Leenaars J.G.B., A.J.M. van Oostrum and M. Ruiperez Gonzalez, 2014. Africa Soil Profiles Database, Version 1.2. A compilation of georeferenced and standardised legacy soil profile data for Sub-Saharan Africa (with dataset). ISRIC Report 2014/01. Africa Soil Information Service (AfSIS) project and ISRIC - World Soil Information, Wageningen, the Netherlands. See Annex 4." ;
    skos:topConceptOf glosis_proc:acidityExchangeableProcedure .

glosis_proc:acidityExchangeableProcedure-ExchAcid_ph7-unkn a glosis_proc:AcidityExchangeableProcedure,
        skos:Concept ;
    skos:definition "Exch acidity (H+Al) buffered at pH 7, in unknown extract" ;
    skos:inScheme glosis_proc:acidityExchangeableProcedure ;
    skos:notation "ExchAcid_ph7-unkn" ;
    skos:prefLabel "ExchAcid_ph7-unk"@en ;
    skos:scopeNote <https://www.isric.org/sites/default/files/isric_report_2014_01.pdf>,
        "Leenaars J.G.B., A.J.M. van Oostrum and M. Ruiperez Gonzalez, 2014. Africa Soil Profiles Database, Version 1.2. A compilation of georeferenced and standardised legacy soil profile data for Sub-Saharan Africa (with dataset). ISRIC Report 2014/01. Africa Soil Information Service (AfSIS) project and ISRIC - World Soil Information, Wageningen, the Netherlands. See Annex 4." ;
    skos:topConceptOf glosis_proc:acidityExchangeableProcedure .

glosis_proc:acidityExchangeableProcedure-ExchAcid_ph8-bacl2tea a glosis_proc:AcidityExchangeableProcedure,
        skos:Concept ;
    skos:definition "Exch (extractable / potential) acidity (Al) buffered at pH 8.0-8.5, in 1 M BaCl2 - TEA" ;
    skos:inScheme glosis_proc:acidityExchangeableProcedure ;
    skos:notation "ExchAcid_ph8-bacl2tea" ;
    skos:prefLabel "ExchAcid_ph8-bacl2tea"@en ;
    skos:scopeNote <https://www.isric.org/sites/default/files/isric_report_2014_01.pdf>,
        "Leenaars J.G.B., A.J.M. van Oostrum and M. Ruiperez Gonzalez, 2014. Africa Soil Profiles Database, Version 1.2. A compilation of georeferenced and standardised legacy soil profile data for Sub-Saharan Africa (with dataset). ISRIC Report 2014/01. Africa Soil Information Service (AfSIS) project and ISRIC - World Soil Information, Wageningen, the Netherlands. See Annex 4." ;
    skos:topConceptOf glosis_proc:acidityExchangeableProcedure .

glosis_proc:acidityExchangeableProcedure-ExchAcid_ph8-unkn a glosis_proc:AcidityExchangeableProcedure,
        skos:Concept ;
    skos:definition "Exch (extractable / potential) acidity (Al) buffered at pH 8.0-8.5, in unknown extract" ;
    skos:inScheme glosis_proc:acidityExchangeableProcedure ;
    skos:notation "ExchAcid_ph8-unkn" ;
    skos:prefLabel "ExchAcid_ph8-unk"@en ;
    skos:scopeNote <https://www.isric.org/sites/default/files/isric_report_2014_01.pdf>,
        "Leenaars J.G.B., A.J.M. van Oostrum and M. Ruiperez Gonzalez, 2014. Africa Soil Profiles Database, Version 1.2. A compilation of georeferenced and standardised legacy soil profile data for Sub-Saharan Africa (with dataset). ISRIC Report 2014/01. Africa Soil Information Service (AfSIS) project and ISRIC - World Soil Information, Wageningen, the Netherlands. See Annex 4." ;
    skos:topConceptOf glosis_proc:acidityExchangeableProcedure .

glosis_proc:availableWaterHoldingCapacityProcedure-PAWHC_calcul-fc100wp a glosis_proc:AvailableWaterHoldingCapacityProcedure,
        skos:Concept ;
    skos:definition "Plant available water holding capacity of the soil fine earth fraction, calculated with field capacity defined at 100 cm (pF 2.0)" ;
    skos:inScheme glosis_proc:availableWaterHoldingCapacityProcedure ;
    skos:notation "PAWHC_calcul-fc100wp" ;
    skos:prefLabel "PAWHC_calcul-fc100wp"@en ;
    skos:scopeNote <https://www.isric.org/sites/default/files/isric_report_2014_01.pdf>,
        "Leenaars J.G.B., A.J.M. van Oostrum and M. Ruiperez Gonzalez, 2014. Africa Soil Profiles Database, Version 1.2. A compilation of georeferenced and standardised legacy soil profile data for Sub-Saharan Africa (with dataset). ISRIC Report 2014/01. Africa Soil Information Service (AfSIS) project and ISRIC - World Soil Information, Wageningen, the Netherlands. See Annex 4." ;
    skos:topConceptOf glosis_proc:availableWaterHoldingCapacityProcedure .

glosis_proc:availableWaterHoldingCapacityProcedure-PAWHC_calcul-fc200wp a glosis_proc:AvailableWaterHoldingCapacityProcedure,
        skos:Concept ;
    skos:definition "Plant available water holding capacity of the soil fine earth fraction, calculated with field capacity defined at 200 cm (pF 2.3)" ;
    skos:inScheme glosis_proc:availableWaterHoldingCapacityProcedure ;
    skos:notation "PAWHC_calcul-fc200wp" ;
    skos:prefLabel "PAWHC_calcul-fc200wp"@en ;
    skos:scopeNote <https://www.isric.org/sites/default/files/isric_report_2014_01.pdf>,
        "Leenaars J.G.B., A.J.M. van Oostrum and M. Ruiperez Gonzalez, 2014. Africa Soil Profiles Database, Version 1.2. A compilation of georeferenced and standardised legacy soil profile data for Sub-Saharan Africa (with dataset). ISRIC Report 2014/01. Africa Soil Information Service (AfSIS) project and ISRIC - World Soil Information, Wageningen, the Netherlands. See Annex 4." ;
    skos:topConceptOf glosis_proc:availableWaterHoldingCapacityProcedure .

glosis_proc:availableWaterHoldingCapacityProcedure-PAWHC_calcul-fc300wp a glosis_proc:AvailableWaterHoldingCapacityProcedure,
        skos:Concept ;
    skos:definition "Plant available water holding capacity of the soil fine earth fraction, calculated with field capacity defined at 300 cm (pF 2.5)" ;
    skos:inScheme glosis_proc:availableWaterHoldingCapacityProcedure ;
    skos:notation "PAWHC_calcul-fc300wp" ;
    skos:prefLabel "PAWHC_calcul-fc300wp"@en ;
    skos:scopeNote <https://www.isric.org/sites/default/files/isric_report_2014_01.pdf>,
        "Leenaars J.G.B., A.J.M. van Oostrum and M. Ruiperez Gonzalez, 2014. Africa Soil Profiles Database, Version 1.2. A compilation of georeferenced and standardised legacy soil profile data for Sub-Saharan Africa (with dataset). ISRIC Report 2014/01. Africa Soil Information Service (AfSIS) project and ISRIC - World Soil Information, Wageningen, the Netherlands. See Annex 4." ;
    skos:topConceptOf glosis_proc:availableWaterHoldingCapacityProcedure .

glosis_proc:baseSaturationProcedure-BSat_calcul-cec a glosis_proc:BaseSaturationProcedure,
        skos:Concept ;
    skos:definition "Sum of exchangeable bases (Ca++, Mg++, K+, Na+) as percentage of CEC (method specified with CEC and ExchBases)" ;
    skos:inScheme glosis_proc:baseSaturationProcedure ;
    skos:notation "BSat_calcul-cec" ;
    skos:prefLabel "BSat_calcul-cec"@en ;
    skos:scopeNote <https://www.isric.org/sites/default/files/isric_report_2014_01.pdf>,
        "Leenaars J.G.B., A.J.M. van Oostrum and M. Ruiperez Gonzalez, 2014. Africa Soil Profiles Database, Version 1.2. A compilation of georeferenced and standardised legacy soil profile data for Sub-Saharan Africa (with dataset). ISRIC Report 2014/01. Africa Soil Information Service (AfSIS) project and ISRIC - World Soil Information, Wageningen, the Netherlands. See Annex 4." ;
    skos:topConceptOf glosis_proc:baseSaturationProcedure .

glosis_proc:baseSaturationProcedure-BSat_calcul-ecec a glosis_proc:BaseSaturationProcedure,
        skos:Concept ;
    skos:definition "Sum of exchangeable bases (Ca++, Mg++, K+, Na+) as percentage of EffCEC (method specified with EffCEC and ExchBases)" ;
    skos:inScheme glosis_proc:baseSaturationProcedure ;
    skos:notation "BSat_calcul-ecec" ;
    skos:prefLabel "BSat_calcul-ecec"@en ;
    skos:scopeNote <https://www.isric.org/sites/default/files/isric_report_2014_01.pdf>,
        "Leenaars J.G.B., A.J.M. van Oostrum and M. Ruiperez Gonzalez, 2014. Africa Soil Profiles Database, Version 1.2. A compilation of georeferenced and standardised legacy soil profile data for Sub-Saharan Africa (with dataset). ISRIC Report 2014/01. Africa Soil Information Service (AfSIS) project and ISRIC - World Soil Information, Wageningen, the Netherlands. See Annex 4." ;
    skos:topConceptOf glosis_proc:baseSaturationProcedure .

glosis_proc:bulkDensityFineEarthProcedure-BlkDensF_fe-cl-fc a glosis_proc:BulkDensityFineEarthProcedure,
        skos:Concept ;
    skos:definition "Fine earth. Clod samples (natural clods or reconstituted from < 2mm sample), at field capacity (0.33 bar, 33 kPa, 330 cm, pF 2.5), corrected for coarse fragments if any" ;
    skos:inScheme glosis_proc:bulkDensityFineEarthProcedure ;
    skos:notation "BlkDensF_fe-cl-fc" ;
    skos:prefLabel "BlkDensF_fe-cl-fc"@en ;
    skos:scopeNote <https://www.isric.org/sites/default/files/isric_report_2014_01.pdf>,
        "Leenaars J.G.B., A.J.M. van Oostrum and M. Ruiperez Gonzalez, 2014. Africa Soil Profiles Database, Version 1.2. A compilation of georeferenced and standardised legacy soil profile data for Sub-Saharan Africa (with dataset). ISRIC Report 2014/01. Africa Soil Information Service (AfSIS) project and ISRIC - World Soil Information, Wageningen, the Netherlands. See Annex 4." ;
    skos:topConceptOf glosis_proc:bulkDensityFineEarthProcedure .

glosis_proc:bulkDensityFineEarthProcedure-BlkDensF_fe-cl-od a glosis_proc:BulkDensityFineEarthProcedure,
        skos:Concept ;
    skos:definition "Fine earth. Clod samples (natural clods or reconstituted from < 2mm sample), at oven dry, corrected for coarse fragments if any" ;
    skos:inScheme glosis_proc:bulkDensityFineEarthProcedure ;
    skos:notation "BlkDensF_fe-cl-od" ;
    skos:prefLabel "BlkDensF_fe-cl-od"@en ;
    skos:scopeNote <https://www.isric.org/sites/default/files/isric_report_2014_01.pdf>,
        "Leenaars J.G.B., A.J.M. van Oostrum and M. Ruiperez Gonzalez, 2014. Africa Soil Profiles Database, Version 1.2. A compilation of georeferenced and standardised legacy soil profile data for Sub-Saharan Africa (with dataset). ISRIC Report 2014/01. Africa Soil Information Service (AfSIS) project and ISRIC - World Soil Information, Wageningen, the Netherlands. See Annex 4." ;
    skos:topConceptOf glosis_proc:bulkDensityFineEarthProcedure .

glosis_proc:bulkDensityFineEarthProcedure-BlkDensF_fe-cl-unkn a glosis_proc:BulkDensityFineEarthProcedure,
        skos:Concept ;
    skos:definition "Fine earth. Clod samples (natural clods or reconstituted from < 2mm sample), at unknown humidity, corrected for coarse fragments if any" ;
    skos:inScheme glosis_proc:bulkDensityFineEarthProcedure ;
    skos:notation "BlkDensF_fe-cl-unkn" ;
    skos:prefLabel "BlkDensF_fe-cl-unk"@en ;
    skos:scopeNote <https://www.isric.org/sites/default/files/isric_report_2014_01.pdf>,
        "Leenaars J.G.B., A.J.M. van Oostrum and M. Ruiperez Gonzalez, 2014. Africa Soil Profiles Database, Version 1.2. A compilation of georeferenced and standardised legacy soil profile data for Sub-Saharan Africa (with dataset). ISRIC Report 2014/01. Africa Soil Information Service (AfSIS) project and ISRIC - World Soil Information, Wageningen, the Netherlands. See Annex 4." ;
    skos:topConceptOf glosis_proc:bulkDensityFineEarthProcedure .

glosis_proc:bulkDensityFineEarthProcedure-BlkDensF_fe-co-fc a glosis_proc:BulkDensityFineEarthProcedure,
        skos:Concept ;
    skos:definition "Fine earth. Core sampling (pF rings), at field capacity (0.33 bar, 33 kPa, 336 cm, pF 2.5), corrected for coarse fragments if any" ;
    skos:inScheme glosis_proc:bulkDensityFineEarthProcedure ;
    skos:notation "BlkDensF_fe-co-fc" ;
    skos:prefLabel "BlkDensF_fe-co-fc"@en ;
    skos:scopeNote <https://www.isric.org/sites/default/files/isric_report_2014_01.pdf>,
        "Leenaars J.G.B., A.J.M. van Oostrum and M. Ruiperez Gonzalez, 2014. Africa Soil Profiles Database, Version 1.2. A compilation of georeferenced and standardised legacy soil profile data for Sub-Saharan Africa (with dataset). ISRIC Report 2014/01. Africa Soil Information Service (AfSIS) project and ISRIC - World Soil Information, Wageningen, the Netherlands. See Annex 4." ;
    skos:topConceptOf glosis_proc:bulkDensityFineEarthProcedure .

glosis_proc:bulkDensityFineEarthProcedure-BlkDensF_fe-co-od a glosis_proc:BulkDensityFineEarthProcedure,
        skos:Concept ;
    skos:definition "Fine earth. Core sampling (pF rings), at oven dry, corrected for coarse fragments if any" ;
    skos:inScheme glosis_proc:bulkDensityFineEarthProcedure ;
    skos:notation "BlkDensF_fe-co-od" ;
    skos:prefLabel "BlkDensF_fe-co-od"@en ;
    skos:scopeNote <https://www.isric.org/sites/default/files/isric_report_2014_01.pdf>,
        "Leenaars J.G.B., A.J.M. van Oostrum and M. Ruiperez Gonzalez, 2014. Africa Soil Profiles Database, Version 1.2. A compilation of georeferenced and standardised legacy soil profile data for Sub-Saharan Africa (with dataset). ISRIC Report 2014/01. Africa Soil Information Service (AfSIS) project and ISRIC - World Soil Information, Wageningen, the Netherlands. See Annex 4." ;
    skos:topConceptOf glosis_proc:bulkDensityFineEarthProcedure .

glosis_proc:bulkDensityFineEarthProcedure-BlkDensF_fe-co-unkn a glosis_proc:BulkDensityFineEarthProcedure,
        skos:Concept ;
    skos:definition "Fine earth. Core sampling (pF rings), at unknown humidity, corrected for coarse fragments if any" ;
    skos:inScheme glosis_proc:bulkDensityFineEarthProcedure ;
    skos:notation "BlkDensF_fe-co-unkn" ;
    skos:prefLabel "BlkDensF_fe-co-unk"@en ;
    skos:scopeNote <https://www.isric.org/sites/default/files/isric_report_2014_01.pdf>,
        "Leenaars J.G.B., A.J.M. van Oostrum and M. Ruiperez Gonzalez, 2014. Africa Soil Profiles Database, Version 1.2. A compilation of georeferenced and standardised legacy soil profile data for Sub-Saharan Africa (with dataset). ISRIC Report 2014/01. Africa Soil Information Service (AfSIS) project and ISRIC - World Soil Information, Wageningen, the Netherlands. See Annex 4." ;
    skos:topConceptOf glosis_proc:bulkDensityFineEarthProcedure .

glosis_proc:bulkDensityFineEarthProcedure-BlkDensF_fe-rpl-unkn a glosis_proc:BulkDensityFineEarthProcedure,
        skos:Concept ;
    skos:definition "Fine earth. Excavation and replacement (i.e. soils too fragile to remove a stable sample) e.g. by auger, at unknown humidity, corrected for coarse fragments if any" ;
    skos:inScheme glosis_proc:bulkDensityFineEarthProcedure ;
    skos:notation "BlkDensF_fe-rpl-unkn" ;
    skos:prefLabel "BlkDensF_fe-rpl-unk"@en ;
    skos:scopeNote <https://www.isric.org/sites/default/files/isric_report_2014_01.pdf>,
        "Leenaars J.G.B., A.J.M. van Oostrum and M. Ruiperez Gonzalez, 2014. Africa Soil Profiles Database, Version 1.2. A compilation of georeferenced and standardised legacy soil profile data for Sub-Saharan Africa (with dataset). ISRIC Report 2014/01. Africa Soil Information Service (AfSIS) project and ISRIC - World Soil Information, Wageningen, the Netherlands. See Annex 4." ;
    skos:topConceptOf glosis_proc:bulkDensityFineEarthProcedure .

glosis_proc:bulkDensityFineEarthProcedure-BlkDensF_fe-unkn a glosis_proc:BulkDensityFineEarthProcedure,
        skos:Concept ;
    skos:definition "Fine earth. Type of sample unknown, at unknown humidity, corrected for coarse fragments if any" ;
    skos:inScheme glosis_proc:bulkDensityFineEarthProcedure ;
    skos:notation "BlkDensF_fe-unkn" ;
    skos:prefLabel "BlkDensF_fe-unk"@en ;
    skos:scopeNote <https://www.isric.org/sites/default/files/isric_report_2014_01.pdf>,
        "Leenaars J.G.B., A.J.M. van Oostrum and M. Ruiperez Gonzalez, 2014. Africa Soil Profiles Database, Version 1.2. A compilation of georeferenced and standardised legacy soil profile data for Sub-Saharan Africa (with dataset). ISRIC Report 2014/01. Africa Soil Information Service (AfSIS) project and ISRIC - World Soil Information, Wageningen, the Netherlands. See Annex 4." ;
    skos:topConceptOf glosis_proc:bulkDensityFineEarthProcedure .

glosis_proc:bulkDensityFineEarthProcedure-BlkDensF_fe-unkn-fc a glosis_proc:BulkDensityFineEarthProcedure,
        skos:Concept ;
    skos:definition "Fine earth. Type of sample unknown, at field capacity (0.33 bar, 33 kPa, 330 cm, pF 2.5), corrected for coarse fragments if any" ;
    skos:inScheme glosis_proc:bulkDensityFineEarthProcedure ;
    skos:notation "BlkDensF_fe-unkn-fc" ;
    skos:prefLabel "BlkDensF_fe-unkn-fc"@en ;
    skos:scopeNote <https://www.isric.org/sites/default/files/isric_report_2014_01.pdf>,
        "Leenaars J.G.B., A.J.M. van Oostrum and M. Ruiperez Gonzalez, 2014. Africa Soil Profiles Database, Version 1.2. A compilation of georeferenced and standardised legacy soil profile data for Sub-Saharan Africa (with dataset). ISRIC Report 2014/01. Africa Soil Information Service (AfSIS) project and ISRIC - World Soil Information, Wageningen, the Netherlands. See Annex 4." ;
    skos:topConceptOf glosis_proc:bulkDensityFineEarthProcedure .

glosis_proc:bulkDensityFineEarthProcedure-BlkDensF_fe-unkn-od a glosis_proc:BulkDensityFineEarthProcedure,
        skos:Concept ;
    skos:definition "Fine earth. Type of sample unknown, at oven dry, corrected for coarse fragments if any" ;
    skos:inScheme glosis_proc:bulkDensityFineEarthProcedure ;
    skos:notation "BlkDensF_fe-unkn-od" ;
    skos:prefLabel "BlkDensF_fe-unkn-od"@en ;
    skos:scopeNote <https://www.isric.org/sites/default/files/isric_report_2014_01.pdf>,
        "Leenaars J.G.B., A.J.M. van Oostrum and M. Ruiperez Gonzalez, 2014. Africa Soil Profiles Database, Version 1.2. A compilation of georeferenced and standardised legacy soil profile data for Sub-Saharan Africa (with dataset). ISRIC Report 2014/01. Africa Soil Information Service (AfSIS) project and ISRIC - World Soil Information, Wageningen, the Netherlands. See Annex 4." ;
    skos:topConceptOf glosis_proc:bulkDensityFineEarthProcedure .

glosis_proc:bulkDensityWholeSoilProcedure-BlkDensW_we-cl-fc a glosis_proc:BulkDensityWholeSoilProcedure,
        skos:Concept ;
    skos:definition "Whole earth. Clod samples (natural clods), at field capacity (0.33 bar, 33 kPa, 330 cm, pF 2.5), not corrected for coarse fragments if any" ;
    skos:inScheme glosis_proc:bulkDensityWholeSoilProcedure ;
    skos:notation "BlkDensW_we-cl-fc" ;
    skos:prefLabel "BlkDensW_we-cl-fc"@en ;
    skos:scopeNote <https://www.isric.org/sites/default/files/isric_report_2014_01.pdf>,
        "Leenaars J.G.B., A.J.M. van Oostrum and M. Ruiperez Gonzalez, 2014. Africa Soil Profiles Database, Version 1.2. A compilation of georeferenced and standardised legacy soil profile data for Sub-Saharan Africa (with dataset). ISRIC Report 2014/01. Africa Soil Information Service (AfSIS) project and ISRIC - World Soil Information, Wageningen, the Netherlands. See Annex 4." ;
    skos:topConceptOf glosis_proc:bulkDensityWholeSoilProcedure .

glosis_proc:bulkDensityWholeSoilProcedure-BlkDensW_we-cl-od a glosis_proc:BulkDensityWholeSoilProcedure,
        skos:Concept ;
    skos:definition "Whole earth. Clod samples (natural clods), at oven dry, not corrected for coarse fragments if any" ;
    skos:inScheme glosis_proc:bulkDensityWholeSoilProcedure ;
    skos:notation "BlkDensW_we-cl-od" ;
    skos:prefLabel "BlkDensW_we-cl-od"@en ;
    skos:scopeNote <https://www.isric.org/sites/default/files/isric_report_2014_01.pdf>,
        "Leenaars J.G.B., A.J.M. van Oostrum and M. Ruiperez Gonzalez, 2014. Africa Soil Profiles Database, Version 1.2. A compilation of georeferenced and standardised legacy soil profile data for Sub-Saharan Africa (with dataset). ISRIC Report 2014/01. Africa Soil Information Service (AfSIS) project and ISRIC - World Soil Information, Wageningen, the Netherlands. See Annex 4." ;
    skos:topConceptOf glosis_proc:bulkDensityWholeSoilProcedure .

glosis_proc:bulkDensityWholeSoilProcedure-BlkDensW_we-cl-unkn a glosis_proc:BulkDensityWholeSoilProcedure,
        skos:Concept ;
    skos:definition "Whole earth. Clod samples (natural clods), at unknown humidity, not corrected for coarse fragments if any" ;
    skos:inScheme glosis_proc:bulkDensityWholeSoilProcedure ;
    skos:notation "BlkDensW_we-cl-unkn" ;
    skos:prefLabel "BlkDensW_we-cl-unk"@en ;
    skos:scopeNote <https://www.isric.org/sites/default/files/isric_report_2014_01.pdf>,
        "Leenaars J.G.B., A.J.M. van Oostrum and M. Ruiperez Gonzalez, 2014. Africa Soil Profiles Database, Version 1.2. A compilation of georeferenced and standardised legacy soil profile data for Sub-Saharan Africa (with dataset). ISRIC Report 2014/01. Africa Soil Information Service (AfSIS) project and ISRIC - World Soil Information, Wageningen, the Netherlands. See Annex 4." ;
    skos:topConceptOf glosis_proc:bulkDensityWholeSoilProcedure .

glosis_proc:bulkDensityWholeSoilProcedure-BlkDensW_we-co-fc a glosis_proc:BulkDensityWholeSoilProcedure,
        skos:Concept ;
    skos:definition "Whole earth. Core sampling (pF rings), at field capacity (0.33 bar, 33 kPa, 336 cm, pF 2.5), not corrected for coarse fragments if any" ;
    skos:inScheme glosis_proc:bulkDensityWholeSoilProcedure ;
    skos:notation "BlkDensW_we-co-fc" ;
    skos:prefLabel "BlkDensW_we-co-fc"@en ;
    skos:scopeNote <https://www.isric.org/sites/default/files/isric_report_2014_01.pdf>,
        "Leenaars J.G.B., A.J.M. van Oostrum and M. Ruiperez Gonzalez, 2014. Africa Soil Profiles Database, Version 1.2. A compilation of georeferenced and standardised legacy soil profile data for Sub-Saharan Africa (with dataset). ISRIC Report 2014/01. Africa Soil Information Service (AfSIS) project and ISRIC - World Soil Information, Wageningen, the Netherlands. See Annex 4." ;
    skos:topConceptOf glosis_proc:bulkDensityWholeSoilProcedure .

glosis_proc:bulkDensityWholeSoilProcedure-BlkDensW_we-co-od a glosis_proc:BulkDensityWholeSoilProcedure,
        skos:Concept ;
    skos:definition "Whole earth. Core sampling (pF rings), at oven dry, not corrected for coarse fragments if any" ;
    skos:inScheme glosis_proc:bulkDensityWholeSoilProcedure ;
    skos:notation "BlkDensW_we-co-od" ;
    skos:prefLabel "BlkDensW_we-co-od"@en ;
    skos:scopeNote <https://www.isric.org/sites/default/files/isric_report_2014_01.pdf>,
        "Leenaars J.G.B., A.J.M. van Oostrum and M. Ruiperez Gonzalez, 2014. Africa Soil Profiles Database, Version 1.2. A compilation of georeferenced and standardised legacy soil profile data for Sub-Saharan Africa (with dataset). ISRIC Report 2014/01. Africa Soil Information Service (AfSIS) project and ISRIC - World Soil Information, Wageningen, the Netherlands. See Annex 4." ;
    skos:topConceptOf glosis_proc:bulkDensityWholeSoilProcedure .

glosis_proc:bulkDensityWholeSoilProcedure-BlkDensW_we-co-unkn a glosis_proc:BulkDensityWholeSoilProcedure,
        skos:Concept ;
    skos:definition "Whole earth. Core sampling (pF rings), at unknown humidity, not corrected for coarse fragments if any" ;
    skos:inScheme glosis_proc:bulkDensityWholeSoilProcedure ;
    skos:notation "BlkDensW_we-co-unkn" ;
    skos:prefLabel "BlkDensW_we-co-unk"@en ;
    skos:scopeNote <https://www.isric.org/sites/default/files/isric_report_2014_01.pdf>,
        "Leenaars J.G.B., A.J.M. van Oostrum and M. Ruiperez Gonzalez, 2014. Africa Soil Profiles Database, Version 1.2. A compilation of georeferenced and standardised legacy soil profile data for Sub-Saharan Africa (with dataset). ISRIC Report 2014/01. Africa Soil Information Service (AfSIS) project and ISRIC - World Soil Information, Wageningen, the Netherlands. See Annex 4." ;
    skos:topConceptOf glosis_proc:bulkDensityWholeSoilProcedure .

glosis_proc:bulkDensityWholeSoilProcedure-BlkDensW_we-rpl-unkn a glosis_proc:BulkDensityWholeSoilProcedure,
        skos:Concept ;
    skos:definition "Whole earth. Excavation and replacement (i.e. soils too fragile to remove a stable sample) e.g. by auger, at unknown humidity, not corrected for coarse fragments if any" ;
    skos:inScheme glosis_proc:bulkDensityWholeSoilProcedure ;
    skos:notation "BlkDensW_we-rpl-unkn" ;
    skos:prefLabel "BlkDensW_we-rpl-unk"@en ;
    skos:scopeNote <https://www.isric.org/sites/default/files/isric_report_2014_01.pdf>,
        "Leenaars J.G.B., A.J.M. van Oostrum and M. Ruiperez Gonzalez, 2014. Africa Soil Profiles Database, Version 1.2. A compilation of georeferenced and standardised legacy soil profile data for Sub-Saharan Africa (with dataset). ISRIC Report 2014/01. Africa Soil Information Service (AfSIS) project and ISRIC - World Soil Information, Wageningen, the Netherlands. See Annex 4." ;
    skos:topConceptOf glosis_proc:bulkDensityWholeSoilProcedure .

glosis_proc:bulkDensityWholeSoilProcedure-BlkDensW_we-unkn a glosis_proc:BulkDensityWholeSoilProcedure,
        skos:Concept ;
    skos:definition "Whole earth. Type of sample unknown, at unknown humidity, not corrected for coarse fragments if any" ;
    skos:inScheme glosis_proc:bulkDensityWholeSoilProcedure ;
    skos:notation "BlkDensW_we-unkn" ;
    skos:prefLabel "BlkDensW_we-unk"@en ;
    skos:scopeNote <https://www.isric.org/sites/default/files/isric_report_2014_01.pdf>,
        "Leenaars J.G.B., A.J.M. van Oostrum and M. Ruiperez Gonzalez, 2014. Africa Soil Profiles Database, Version 1.2. A compilation of georeferenced and standardised legacy soil profile data for Sub-Saharan Africa (with dataset). ISRIC Report 2014/01. Africa Soil Information Service (AfSIS) project and ISRIC - World Soil Information, Wageningen, the Netherlands. See Annex 4." ;
    skos:topConceptOf glosis_proc:bulkDensityWholeSoilProcedure .

glosis_proc:carbonInorganicProcedure-InOrgC_calcul-caco3 a glosis_proc:CarbonInorganicProcedure,
        skos:Concept ;
    skos:definition "Indirect estimate from total carbonate equivalent, with a factor of 0.12 (molar weights: CaCO3 100g/mol, C 12g/mol)" ;
    skos:inScheme glosis_proc:carbonInorganicProcedure ;
    skos:notation "InOrgC_calcul-caco3" ;
    skos:prefLabel "InOrgC_calcul-caco3"@en ;
    skos:scopeNote <https://www.isric.org/sites/default/files/isric_report_2014_01.pdf>,
        "Leenaars J.G.B., A.J.M. van Oostrum and M. Ruiperez Gonzalez, 2014. Africa Soil Profiles Database, Version 1.2. A compilation of georeferenced and standardised legacy soil profile data for Sub-Saharan Africa (with dataset). ISRIC Report 2014/01. Africa Soil Information Service (AfSIS) project and ISRIC - World Soil Information, Wageningen, the Netherlands. See Annex 4." ;
    skos:topConceptOf glosis_proc:carbonInorganicProcedure .

glosis_proc:carbonInorganicProcedure-InOrgC_calcul-tc-oc a glosis_proc:CarbonInorganicProcedure,
        skos:Concept ;
    skos:definition "Indirect estimate (total carbon minus organic carbon = inorganic carbon)" ;
    skos:inScheme glosis_proc:carbonInorganicProcedure ;
    skos:notation "InOrgC_calcul-tc-oc" ;
    skos:prefLabel "InOrgC_calcul-tc-oc"@en ;
    skos:scopeNote <https://www.isric.org/sites/default/files/isric_report_2014_01.pdf>,
        "Leenaars J.G.B., A.J.M. van Oostrum and M. Ruiperez Gonzalez, 2014. Africa Soil Profiles Database, Version 1.2. A compilation of georeferenced and standardised legacy soil profile data for Sub-Saharan Africa (with dataset). ISRIC Report 2014/01. Africa Soil Information Service (AfSIS) project and ISRIC - World Soil Information, Wageningen, the Netherlands. See Annex 4." ;
    skos:topConceptOf glosis_proc:carbonInorganicProcedure .

glosis_proc:carbonOrganicProcedure-OrgC_acid-dc a glosis_proc:CarbonOrganicProcedure,
        skos:Concept ;
    skos:definition "Acidified dry combustion or dry oxidation methods (after removal of carbonates)" ;
    skos:inScheme glosis_proc:carbonOrganicProcedure ;
    skos:notation "OrgC_acid-dc" ;
    skos:prefLabel "OrgC_acid-dc"@en ;
    skos:scopeNote <https://www.isric.org/sites/default/files/isric_report_2014_01.pdf>,
        "Leenaars J.G.B., A.J.M. van Oostrum and M. Ruiperez Gonzalez, 2014. Africa Soil Profiles Database, Version 1.2. A compilation of georeferenced and standardised legacy soil profile data for Sub-Saharan Africa (with dataset). ISRIC Report 2014/01. Africa Soil Information Service (AfSIS) project and ISRIC - World Soil Information, Wageningen, the Netherlands. See Annex 4." ;
    skos:topConceptOf glosis_proc:carbonOrganicProcedure .

glosis_proc:carbonOrganicProcedure-OrgC_acid-dc-ht a glosis_proc:CarbonOrganicProcedure,
        skos:Concept ;
    skos:definition "Acidified. Dry combustion at 1200 C and colometric CO2 measurement (Schlichting et al. 1995)" ;
    skos:inScheme glosis_proc:carbonOrganicProcedure ;
    skos:notation "OrgC_acid-dc-ht" ;
    skos:prefLabel "OrgC_acid-dc-ht"@en ;
    skos:scopeNote "Schlichting E, Blume HP, Stahr K (1995) Soils Practical (in German). Blackwell, Berlin" ;
    skos:topConceptOf glosis_proc:carbonOrganicProcedure .

glosis_proc:carbonOrganicProcedure-OrgC_acid-dc-ht-analyser a glosis_proc:CarbonOrganicProcedure,
        skos:Concept ;
    skos:definition "Acidified. Furnace combustion (e.g., LECO combustion analyzer, Dumas method)" ;
    skos:inScheme glosis_proc:carbonOrganicProcedure ;
    skos:notation "OrgC_acid-dc-ht-analyser" ;
    skos:prefLabel "OrgC_acid-dc-ht-analyser"@en ;
    skos:scopeNote <https://www.isric.org/sites/default/files/isric_report_2014_01.pdf>,
        "Leenaars J.G.B., A.J.M. van Oostrum and M. Ruiperez Gonzalez, 2014. Africa Soil Profiles Database, Version 1.2. A compilation of georeferenced and standardised legacy soil profile data for Sub-Saharan Africa (with dataset). ISRIC Report 2014/01. Africa Soil Information Service (AfSIS) project and ISRIC - World Soil Information, Wageningen, the Netherlands. See Annex 4." ;
    skos:topConceptOf glosis_proc:carbonOrganicProcedure .

glosis_proc:carbonOrganicProcedure-OrgC_acid-dc-lt a glosis_proc:CarbonOrganicProcedure,
        skos:Concept ;
    skos:definition "Acidified. Dry combustion at 500 C" ;
    skos:inScheme glosis_proc:carbonOrganicProcedure ;
    skos:notation "OrgC_acid-dc-lt" ;
    skos:prefLabel "OrgC_acid-dc-lt"@en ;
    skos:scopeNote <https://www.isric.org/sites/default/files/isric_report_2014_01.pdf>,
        "Leenaars J.G.B., A.J.M. van Oostrum and M. Ruiperez Gonzalez, 2014. Africa Soil Profiles Database, Version 1.2. A compilation of georeferenced and standardised legacy soil profile data for Sub-Saharan Africa (with dataset). ISRIC Report 2014/01. Africa Soil Information Service (AfSIS) project and ISRIC - World Soil Information, Wageningen, the Netherlands. See Annex 4." ;
    skos:topConceptOf glosis_proc:carbonOrganicProcedure .

glosis_proc:carbonOrganicProcedure-OrgC_acid-dc-lt-loi a glosis_proc:CarbonOrganicProcedure,
        skos:Concept ;
    skos:definition "Acidified. Loss on ignition (NL)" ;
    skos:inScheme glosis_proc:carbonOrganicProcedure ;
    skos:notation "OrgC_acid-dc-lt-loi" ;
    skos:prefLabel "OrgC_acid-dc-lt-loi"@en ;
    skos:scopeNote <https://www.isric.org/sites/default/files/isric_report_2014_01.pdf>,
        "Leenaars J.G.B., A.J.M. van Oostrum and M. Ruiperez Gonzalez, 2014. Africa Soil Profiles Database, Version 1.2. A compilation of georeferenced and standardised legacy soil profile data for Sub-Saharan Africa (with dataset). ISRIC Report 2014/01. Africa Soil Information Service (AfSIS) project and ISRIC - World Soil Information, Wageningen, the Netherlands. See Annex 4." ;
    skos:topConceptOf glosis_proc:carbonOrganicProcedure .

glosis_proc:carbonOrganicProcedure-OrgC_acid-dc-mt a glosis_proc:CarbonOrganicProcedure,
        skos:Concept ;
    skos:definition "Acidified. Dry combustion at 840 C" ;
    skos:inScheme glosis_proc:carbonOrganicProcedure ;
    skos:notation "OrgC_acid-dc-mt" ;
    skos:prefLabel "OrgC_acid-dc-mt"@en ;
    skos:scopeNote <https://www.isric.org/sites/default/files/isric_report_2014_01.pdf>,
        "Leenaars J.G.B., A.J.M. van Oostrum and M. Ruiperez Gonzalez, 2014. Africa Soil Profiles Database, Version 1.2. A compilation of georeferenced and standardised legacy soil profile data for Sub-Saharan Africa (with dataset). ISRIC Report 2014/01. Africa Soil Information Service (AfSIS) project and ISRIC - World Soil Information, Wageningen, the Netherlands. See Annex 4." ;
    skos:topConceptOf glosis_proc:carbonOrganicProcedure .

glosis_proc:carbonOrganicProcedure-OrgC_acid-dc-spec a glosis_proc:CarbonOrganicProcedure,
        skos:Concept ;
    skos:definition "Spectrally measured and converted to Acidified dry combustion or dry oxidation methods (after removal of carbonates)" ;
    skos:inScheme glosis_proc:carbonOrganicProcedure ;
    skos:notation "OrgC_acid-dc-spec" ;
    skos:prefLabel "OrgC_acid-dc-spec"@en ;
    skos:scopeNote <https://www.isric.org/sites/default/files/isric_report_2014_01.pdf>,
        "Leenaars J.G.B., A.J.M. van Oostrum and M. Ruiperez Gonzalez, 2014. Africa Soil Profiles Database, Version 1.2. A compilation of georeferenced and standardised legacy soil profile data for Sub-Saharan Africa (with dataset). ISRIC Report 2014/01. Africa Soil Information Service (AfSIS) project and ISRIC - World Soil Information, Wageningen, the Netherlands. See Annex 4." ;
    skos:topConceptOf glosis_proc:carbonOrganicProcedure .

glosis_proc:carbonOrganicProcedure-OrgC_calcul-tc-ic a glosis_proc:CarbonOrganicProcedure,
        skos:Concept ;
    skos:definition "Calculated as total carbon minus inorganic carbon" ;
    skos:inScheme glosis_proc:carbonOrganicProcedure ;
    skos:notation "OrgC_calcul-tc-ic" ;
    skos:prefLabel "OrgC_calcul-tc-ic"@en ;
    skos:scopeNote <https://www.isric.org/sites/default/files/isric_report_2014_01.pdf>,
        "Leenaars J.G.B., A.J.M. van Oostrum and M. Ruiperez Gonzalez, 2014. Africa Soil Profiles Database, Version 1.2. A compilation of georeferenced and standardised legacy soil profile data for Sub-Saharan Africa (with dataset). ISRIC Report 2014/01. Africa Soil Information Service (AfSIS) project and ISRIC - World Soil Information, Wageningen, the Netherlands. See Annex 4." ;
    skos:topConceptOf glosis_proc:carbonOrganicProcedure .

glosis_proc:carbonOrganicProcedure-OrgC_dc a glosis_proc:CarbonOrganicProcedure,
        skos:Concept ;
    skos:definition "Unacidified. Dry combustion or dry oxidation methods (without prior removal of carbonates)" ;
    skos:inScheme glosis_proc:carbonOrganicProcedure ;
    skos:notation "OrgC_dc" ;
    skos:prefLabel "OrgC_dc"@en ;
    skos:scopeNote <https://www.isric.org/sites/default/files/isric_report_2014_01.pdf>,
        "Leenaars J.G.B., A.J.M. van Oostrum and M. Ruiperez Gonzalez, 2014. Africa Soil Profiles Database, Version 1.2. A compilation of georeferenced and standardised legacy soil profile data for Sub-Saharan Africa (with dataset). ISRIC Report 2014/01. Africa Soil Information Service (AfSIS) project and ISRIC - World Soil Information, Wageningen, the Netherlands. See Annex 4." ;
    skos:topConceptOf glosis_proc:carbonOrganicProcedure .

glosis_proc:carbonOrganicProcedure-OrgC_dc-ht a glosis_proc:CarbonOrganicProcedure,
        skos:Concept ;
    skos:definition "Unacidified. Dry combustion at high temperature (e.g. 1200 C and colometric CO2 measurement (Schlichting et al. 1995)" ;
    skos:inScheme glosis_proc:carbonOrganicProcedure ;
    skos:notation "OrgC_dc-ht" ;
    skos:prefLabel "OrgC_dc-ht"@en ;
    skos:scopeNote "Schlichting E, Blume HP, Stahr K (1995) Soils Practical (in German). Blackwell, Berlin" ;
    skos:topConceptOf glosis_proc:carbonOrganicProcedure .

glosis_proc:carbonOrganicProcedure-OrgC_dc-ht-analyser a glosis_proc:CarbonOrganicProcedure,
        skos:Concept ;
    skos:definition "Unacidified. Dry combustion by furnace (e.g., LECO combustion analyzer, Dumas method). Is total Carbon?" ;
    skos:inScheme glosis_proc:carbonOrganicProcedure ;
    skos:notation "OrgC_dc-ht-analyser" ;
    skos:prefLabel "OrgC_dc-ht-analyser"@en ;
    skos:scopeNote <https://www.isric.org/sites/default/files/isric_report_2014_01.pdf>,
        "Leenaars J.G.B., A.J.M. van Oostrum and M. Ruiperez Gonzalez, 2014. Africa Soil Profiles Database, Version 1.2. A compilation of georeferenced and standardised legacy soil profile data for Sub-Saharan Africa (with dataset). ISRIC Report 2014/01. Africa Soil Information Service (AfSIS) project and ISRIC - World Soil Information, Wageningen, the Netherlands. See Annex 4." ;
    skos:topConceptOf glosis_proc:carbonOrganicProcedure .

glosis_proc:carbonOrganicProcedure-OrgC_dc-lt a glosis_proc:CarbonOrganicProcedure,
        skos:Concept ;
    skos:definition "Unacidified. Dry combustion at low temperature e.g. 500 C" ;
    skos:inScheme glosis_proc:carbonOrganicProcedure ;
    skos:notation "OrgC_dc-lt" ;
    skos:prefLabel "OrgC_dc-lt"@en ;
    skos:scopeNote <https://www.isric.org/sites/default/files/isric_report_2014_01.pdf>,
        "Leenaars J.G.B., A.J.M. van Oostrum and M. Ruiperez Gonzalez, 2014. Africa Soil Profiles Database, Version 1.2. A compilation of georeferenced and standardised legacy soil profile data for Sub-Saharan Africa (with dataset). ISRIC Report 2014/01. Africa Soil Information Service (AfSIS) project and ISRIC - World Soil Information, Wageningen, the Netherlands. See Annex 4." ;
    skos:topConceptOf glosis_proc:carbonOrganicProcedure .

glosis_proc:carbonOrganicProcedure-OrgC_dc-lt-loi a glosis_proc:CarbonOrganicProcedure,
        skos:Concept ;
    skos:definition "Unacidified. Loss on ignition (NL) is total Organic Carbon" ;
    skos:inScheme glosis_proc:carbonOrganicProcedure ;
    skos:notation "OrgC_dc-lt-loi" ;
    skos:prefLabel "OrgC_dc-lt-loi"@en ;
    skos:scopeNote <https://www.isric.org/sites/default/files/isric_report_2014_01.pdf>,
        "Leenaars J.G.B., A.J.M. van Oostrum and M. Ruiperez Gonzalez, 2014. Africa Soil Profiles Database, Version 1.2. A compilation of georeferenced and standardised legacy soil profile data for Sub-Saharan Africa (with dataset). ISRIC Report 2014/01. Africa Soil Information Service (AfSIS) project and ISRIC - World Soil Information, Wageningen, the Netherlands. See Annex 4." ;
    skos:topConceptOf glosis_proc:carbonOrganicProcedure .

glosis_proc:carbonOrganicProcedure-OrgC_dc-mt a glosis_proc:CarbonOrganicProcedure,
        skos:Concept ;
    skos:definition "Unacidified. Dry combustion at medium temperature e.g. 840 C" ;
    skos:inScheme glosis_proc:carbonOrganicProcedure ;
    skos:notation "OrgC_dc-mt" ;
    skos:prefLabel "OrgC_dc-mt"@en ;
    skos:scopeNote <https://www.isric.org/sites/default/files/isric_report_2014_01.pdf>,
        "Leenaars J.G.B., A.J.M. van Oostrum and M. Ruiperez Gonzalez, 2014. Africa Soil Profiles Database, Version 1.2. A compilation of georeferenced and standardised legacy soil profile data for Sub-Saharan Africa (with dataset). ISRIC Report 2014/01. Africa Soil Information Service (AfSIS) project and ISRIC - World Soil Information, Wageningen, the Netherlands. See Annex 4." ;
    skos:topConceptOf glosis_proc:carbonOrganicProcedure .

glosis_proc:carbonOrganicProcedure-OrgC_dc-spec a glosis_proc:CarbonOrganicProcedure,
        skos:Concept ;
    skos:definition "Spectrally measured and converted to Unacidified Dry combustion or dry oxidation methods" ;
    skos:inScheme glosis_proc:carbonOrganicProcedure ;
    skos:notation "OrgC_dc-spec" ;
    skos:prefLabel "OrgC_dc-spec"@en ;
    skos:scopeNote <https://www.isric.org/sites/default/files/isric_report_2014_01.pdf>,
        "Leenaars J.G.B., A.J.M. van Oostrum and M. Ruiperez Gonzalez, 2014. Africa Soil Profiles Database, Version 1.2. A compilation of georeferenced and standardised legacy soil profile data for Sub-Saharan Africa (with dataset). ISRIC Report 2014/01. Africa Soil Information Service (AfSIS) project and ISRIC - World Soil Information, Wageningen, the Netherlands. See Annex 4." ;
    skos:topConceptOf glosis_proc:carbonOrganicProcedure .

glosis_proc:carbonOrganicProcedure-OrgC_wc a glosis_proc:CarbonOrganicProcedure,
        skos:Concept ;
    skos:definition "Wet oxidation or wet combustion methods" ;
    skos:inScheme glosis_proc:carbonOrganicProcedure ;
    skos:notation "OrgC_wc" ;
    skos:prefLabel "OrgC_wc"@en ;
    skos:topConceptOf glosis_proc:carbonOrganicProcedure .

glosis_proc:carbonOrganicProcedure-OrgC_wc-cro3-jackson a glosis_proc:CarbonOrganicProcedure,
        skos:Concept ;
    skos:definition "Wet oxidation according to Jackson (1958) with chromic acid digestion" ;
    skos:inScheme glosis_proc:carbonOrganicProcedure ;
    skos:notation "OrgC_wc-cro3-jackson" ;
    skos:prefLabel "OrgC_wc-cro3-jackso"@en ;
    skos:scopeNote "Jackson, M. L. (1958) Soil Chemical Analysis. Prentice-Hall, Englewood Cliffs, New Jersey." ;
    skos:topConceptOf glosis_proc:carbonOrganicProcedure .

glosis_proc:carbonOrganicProcedure-OrgC_wc-cro3-kalembra a glosis_proc:CarbonOrganicProcedure,
        skos:Concept ;
    skos:definition "Wet oxidation according to Kalembra and Jenkinson (1973) with acid dichromate" ;
    skos:inScheme glosis_proc:carbonOrganicProcedure ;
    skos:notation "OrgC_wc-cro3-kalembra" ;
    skos:prefLabel "OrgC_wc-cro3-kalembra"@en ;
    skos:scopeNote <https://doi.org/10.1002/jsfa.2740240910> ;
    skos:topConceptOf glosis_proc:carbonOrganicProcedure .

glosis_proc:carbonOrganicProcedure-OrgC_wc-cro3-knopp a glosis_proc:CarbonOrganicProcedure,
        skos:Concept ;
    skos:definition "Wet oxidation according to Knopp with chromic acid and gravimetric determination of CO2" ;
    skos:inScheme glosis_proc:carbonOrganicProcedure ;
    skos:notation "OrgC_wc-cro3-knopp" ;
    skos:prefLabel "OrgC_wc-cro3-knopp"@en ;
    skos:scopeNote <https://www.isric.org/sites/default/files/isric_report_2014_01.pdf>,
        "Leenaars J.G.B., A.J.M. van Oostrum and M. Ruiperez Gonzalez, 2014. Africa Soil Profiles Database, Version 1.2. A compilation of georeferenced and standardised legacy soil profile data for Sub-Saharan Africa (with dataset). ISRIC Report 2014/01. Africa Soil Information Service (AfSIS) project and ISRIC - World Soil Information, Wageningen, the Netherlands. See Annex 4." ;
    skos:topConceptOf glosis_proc:carbonOrganicProcedure .

glosis_proc:carbonOrganicProcedure-OrgC_wc-cro3-kurmies a glosis_proc:CarbonOrganicProcedure,
        skos:Concept ;
    skos:definition "Wet oxidation according to Kurmies with K2Cr2O7+H2SO4" ;
    skos:inScheme glosis_proc:carbonOrganicProcedure ;
    skos:notation "OrgC_wc-cro3-kurmies" ;
    skos:prefLabel "OrgC_wc-cro3-kurmies"@en ;
    skos:scopeNote "B. KURMIES, Z. Pflanzenernühr. Dung. u Bodenk., 44 (1949) 121" ;
    skos:topConceptOf glosis_proc:carbonOrganicProcedure .

glosis_proc:carbonOrganicProcedure-OrgC_wc-cro3-nelson a glosis_proc:CarbonOrganicProcedure,
        skos:Concept ;
    skos:definition "Wet oxidation according to Nelson and Sommers (1996)" ;
    skos:inScheme glosis_proc:carbonOrganicProcedure ;
    skos:notation "OrgC_wc-cro3-nelson" ;
    skos:prefLabel "OrgC_wc-cro3-nelso"@en ;
    skos:scopeNote "Nelson and Sommers (1996) in: Sparks DL (ed.). Soil Sci. Soc. Am. book series 5, part 3, pp 961-1010." ;
    skos:topConceptOf glosis_proc:carbonOrganicProcedure .

glosis_proc:carbonOrganicProcedure-OrgC_wc-cro3-nrcs6a1c a glosis_proc:CarbonOrganicProcedure,
        skos:Concept ;
    skos:definition "Wet oxidation according to USDA-NRCS method 6A1c with acid dichromate digestion, FeSO4 titration, automatic titrator" ;
    skos:inScheme glosis_proc:carbonOrganicProcedure ;
    skos:notation "OrgC_wc-cro3-nrcs6a1c" ;
    skos:prefLabel "OrgC_wc-cro3-nrcs6a1c"@en ;
    skos:scopeNote <https://www.nrcs.usda.gov/Internet/FSE_DOCUMENTS/stelprdb1253872.pdf> ;
    skos:topConceptOf glosis_proc:carbonOrganicProcedure .

glosis_proc:carbonOrganicProcedure-OrgC_wc-cro3-tiurin a glosis_proc:CarbonOrganicProcedure,
        skos:Concept ;
    skos:definition "Wet oxidation according to Tiurin with K-dichromate" ;
    skos:inScheme glosis_proc:carbonOrganicProcedure ;
    skos:notation "OrgC_wc-cro3-tiurin" ;
    skos:prefLabel "OrgC_wc-cro3-tiuri"@en ;
    skos:scopeNote "I. V. TIURIN, Pochvovodenie (Pedology), (1931) 36." ;
    skos:topConceptOf glosis_proc:carbonOrganicProcedure .

glosis_proc:carbonOrganicProcedure-OrgC_wc-cro3-walkleyblack a glosis_proc:CarbonOrganicProcedure,
        skos:Concept ;
    skos:definition "Walkley-Black method (chromic acid digestion)" ;
    skos:inScheme glosis_proc:carbonOrganicProcedure ;
    skos:notation "OrgC_wc-cro3-walkleyblack" ;
    skos:prefLabel "OrgC_wc-cro3-walkleyblack"@en ;
    skos:scopeNote "Walkley, A. and I. A. Black. 1934. An Examination of Degtjareff Method for Determining Soil Organic Matter and a Proposed Modification of the Chromic Acid Titration Method. Soil Sci. 37:29–37." ;
    skos:topConceptOf glosis_proc:carbonOrganicProcedure .

glosis_proc:carbonTotalProcedure-TotC_calcul-ic-oc a glosis_proc:CarbonTotalProcedure,
        skos:Concept ;
    skos:definition "Calculated as sum of inorganic carbon and organic carbon" ;
    skos:inScheme glosis_proc:carbonTotalProcedure ;
    skos:notation "TotC_calcul-ic-oc" ;
    skos:prefLabel "TotC_calcul-ic-oc"@en ;
    skos:scopeNote <https://www.isric.org/sites/default/files/isric_report_2014_01.pdf>,
        "Leenaars J.G.B., A.J.M. van Oostrum and M. Ruiperez Gonzalez, 2014. Africa Soil Profiles Database, Version 1.2. A compilation of georeferenced and standardised legacy soil profile data for Sub-Saharan Africa (with dataset). ISRIC Report 2014/01. Africa Soil Information Service (AfSIS) project and ISRIC - World Soil Information, Wageningen, the Netherlands. See Annex 4." ;
    skos:topConceptOf glosis_proc:carbonTotalProcedure .

glosis_proc:carbonTotalProcedure-TotC_dc-ht a glosis_proc:CarbonTotalProcedure,
        skos:Concept ;
    skos:definition "Unacidified dry combustion at high temperature (950-1400 C). Total Carbon" ;
    skos:inScheme glosis_proc:carbonTotalProcedure ;
    skos:notation "TotC_dc-ht" ;
    skos:prefLabel "TotC_dc-ht"@en ;
    skos:scopeNote <https://www.isric.org/sites/default/files/isric_report_2014_01.pdf>,
        "Leenaars J.G.B., A.J.M. van Oostrum and M. Ruiperez Gonzalez, 2014. Africa Soil Profiles Database, Version 1.2. A compilation of georeferenced and standardised legacy soil profile data for Sub-Saharan Africa (with dataset). ISRIC Report 2014/01. Africa Soil Information Service (AfSIS) project and ISRIC - World Soil Information, Wageningen, the Netherlands. See Annex 4." ;
    skos:topConceptOf glosis_proc:carbonTotalProcedure .

glosis_proc:carbonTotalProcedure-TotC_dc-ht-analyser a glosis_proc:CarbonTotalProcedure,
        skos:Concept ;
    skos:definition "Unacidified dry combustion at high temperature (950-1400 C). Total Carbon (USDA-NRCS method 6A), LECO analyzer at 1140 C" ;
    skos:inScheme glosis_proc:carbonTotalProcedure ;
    skos:notation "TotC_dc-ht-analyser" ;
    skos:prefLabel "TotC_dc-ht-analyser"@en ;
    skos:scopeNote <https://www.nrcs.usda.gov/Internet/FSE_DOCUMENTS/stelprdb1253872.pdf> ;
    skos:topConceptOf glosis_proc:carbonTotalProcedure .

glosis_proc:carbonTotalProcedure-TotC_dc-ht-spec a glosis_proc:CarbonTotalProcedure,
        skos:Concept ;
    skos:definition "Spectrally measured and converted to Unacidified dry combustion at high temperature (950-1400 C)." ;
    skos:inScheme glosis_proc:carbonTotalProcedure ;
    skos:notation "TotC_dc-ht-spec" ;
    skos:prefLabel "TotC_dc-ht-spec"@en ;
    skos:scopeNote <https://www.isric.org/sites/default/files/isric_report_2014_01.pdf>,
        "Leenaars J.G.B., A.J.M. van Oostrum and M. Ruiperez Gonzalez, 2014. Africa Soil Profiles Database, Version 1.2. A compilation of georeferenced and standardised legacy soil profile data for Sub-Saharan Africa (with dataset). ISRIC Report 2014/01. Africa Soil Information Service (AfSIS) project and ISRIC - World Soil Information, Wageningen, the Netherlands. See Annex 4." ;
    skos:topConceptOf glosis_proc:carbonTotalProcedure .

glosis_proc:carbonTotalProcedure-TotC_dc-mt a glosis_proc:CarbonTotalProcedure,
        skos:Concept ;
    skos:definition "Unacidified dry combustion at medium temperature (550-950 C)." ;
    skos:inScheme glosis_proc:carbonTotalProcedure ;
    skos:notation "TotC_dc-mt" ;
    skos:prefLabel "TotC_dc-mt"@en ;
    skos:scopeNote <https://www.isric.org/sites/default/files/isric_report_2014_01.pdf>,
        "Leenaars J.G.B., A.J.M. van Oostrum and M. Ruiperez Gonzalez, 2014. Africa Soil Profiles Database, Version 1.2. A compilation of georeferenced and standardised legacy soil profile data for Sub-Saharan Africa (with dataset). ISRIC Report 2014/01. Africa Soil Information Service (AfSIS) project and ISRIC - World Soil Information, Wageningen, the Netherlands. See Annex 4." ;
    skos:topConceptOf glosis_proc:carbonTotalProcedure .

glosis_proc:cationExchangeCapacitySoilProcedure-CEC_ph-unkn-cacl2 a glosis_proc:CationExchangeCapacitySoilProcedure,
        skos:Concept ;
    skos:definition "CEC at unknown buffer, in 0.1 M CaCl2 exchange solution" ;
    skos:inScheme glosis_proc:cationExchangeCapacitySoilProcedure ;
    skos:notation "CEC_ph-unkn-cacl2" ;
    skos:prefLabel "CEC_ph-unkn-cacl2"@en ;
    skos:scopeNote <https://www.isric.org/sites/default/files/isric_report_2014_01.pdf>,
        "Leenaars J.G.B., A.J.M. van Oostrum and M. Ruiperez Gonzalez, 2014. Africa Soil Profiles Database, Version 1.2. A compilation of georeferenced and standardised legacy soil profile data for Sub-Saharan Africa (with dataset). ISRIC Report 2014/01. Africa Soil Information Service (AfSIS) project and ISRIC - World Soil Information, Wageningen, the Netherlands. See Annex 4." ;
    skos:topConceptOf glosis_proc:cationExchangeCapacitySoilProcedure .

glosis_proc:cationExchangeCapacitySoilProcedure-CEC_ph-unkn-lioac a glosis_proc:CationExchangeCapacitySoilProcedure,
        skos:Concept ;
    skos:definition "CEC at unknown buffer, in 0.5 M Li-acetate exchange solution" ;
    skos:inScheme glosis_proc:cationExchangeCapacitySoilProcedure ;
    skos:notation "CEC_ph-unkn-lioac" ;
    skos:prefLabel "CEC_ph-unkn-lioac"@en ;
    skos:scopeNote <https://www.isric.org/sites/default/files/isric_report_2014_01.pdf>,
        "Leenaars J.G.B., A.J.M. van Oostrum and M. Ruiperez Gonzalez, 2014. Africa Soil Profiles Database, Version 1.2. A compilation of georeferenced and standardised legacy soil profile data for Sub-Saharan Africa (with dataset). ISRIC Report 2014/01. Africa Soil Information Service (AfSIS) project and ISRIC - World Soil Information, Wageningen, the Netherlands. See Annex 4." ;
    skos:topConceptOf glosis_proc:cationExchangeCapacitySoilProcedure .

glosis_proc:cationExchangeCapacitySoilProcedure-CEC_ph-unkn-m3 a glosis_proc:CationExchangeCapacitySoilProcedure,
        skos:Concept ;
    skos:definition "CEC at unknown buffer, in Mehlich III exchange solution" ;
    skos:inScheme glosis_proc:cationExchangeCapacitySoilProcedure ;
    skos:notation "CEC_ph-unkn-m3" ;
    skos:prefLabel "CEC_ph-unkn-m3"@en ;
    skos:scopeNote <https://www.isric.org/sites/default/files/isric_report_2014_01.pdf>,
        "Leenaars J.G.B., A.J.M. van Oostrum and M. Ruiperez Gonzalez, 2014. Africa Soil Profiles Database, Version 1.2. A compilation of georeferenced and standardised legacy soil profile data for Sub-Saharan Africa (with dataset). ISRIC Report 2014/01. Africa Soil Information Service (AfSIS) project and ISRIC - World Soil Information, Wageningen, the Netherlands. See Annex 4." ;
    skos:topConceptOf glosis_proc:cationExchangeCapacitySoilProcedure .

glosis_proc:cationExchangeCapacitySoilProcedure-CEC_ph0-ag-thioura a glosis_proc:CationExchangeCapacitySoilProcedure,
        skos:Concept ;
    skos:definition "CEC unbuffered at pH of the soil, in 0.01 M Ag-thioura exchange solution" ;
    skos:inScheme glosis_proc:cationExchangeCapacitySoilProcedure ;
    skos:notation "CEC_ph0-ag-thioura" ;
    skos:prefLabel "CEC_ph0-ag-thioura"@en ;
    skos:scopeNote <https://www.isric.org/sites/default/files/isric_report_2014_01.pdf>,
        "Leenaars J.G.B., A.J.M. van Oostrum and M. Ruiperez Gonzalez, 2014. Africa Soil Profiles Database, Version 1.2. A compilation of georeferenced and standardised legacy soil profile data for Sub-Saharan Africa (with dataset). ISRIC Report 2014/01. Africa Soil Information Service (AfSIS) project and ISRIC - World Soil Information, Wageningen, the Netherlands. See Annex 4." ;
    skos:topConceptOf glosis_proc:cationExchangeCapacitySoilProcedure .

glosis_proc:cationExchangeCapacitySoilProcedure-CEC_ph0-bacl2 a glosis_proc:CationExchangeCapacitySoilProcedure,
        skos:Concept ;
    skos:definition "CEC unbuffered at pH o the soil, in 0.5 M BaCl2 exchange solution (0.1.1.0 M)" ;
    skos:inScheme glosis_proc:cationExchangeCapacitySoilProcedure ;
    skos:notation "CEC_ph0-bacl2" ;
    skos:prefLabel "CEC_ph0-bacl2"@en ;
    skos:scopeNote <https://www.isric.org/sites/default/files/isric_report_2014_01.pdf>,
        "Leenaars J.G.B., A.J.M. van Oostrum and M. Ruiperez Gonzalez, 2014. Africa Soil Profiles Database, Version 1.2. A compilation of georeferenced and standardised legacy soil profile data for Sub-Saharan Africa (with dataset). ISRIC Report 2014/01. Africa Soil Information Service (AfSIS) project and ISRIC - World Soil Information, Wageningen, the Netherlands. See Annex 4." ;
    skos:topConceptOf glosis_proc:cationExchangeCapacitySoilProcedure .

glosis_proc:cationExchangeCapacitySoilProcedure-CEC_ph0-cohex a glosis_proc:CationExchangeCapacitySoilProcedure,
        skos:Concept ;
    skos:definition "CEC unbuffered at pH of the soil, in Cobalt(III) hexamine chloride solution 0,0166M (Cohex) [Co[NH3]6]Cl3 ), ISO 23470 (2007)  exchange solution" ;
    skos:inScheme glosis_proc:cationExchangeCapacitySoilProcedure ;
    skos:notation "CEC_ph0-cohex" ;
    skos:prefLabel "CEC_ph0-cohex"@en ;
    skos:scopeNote <https://www.iso.org/standard/36879.html> ;
    skos:topConceptOf glosis_proc:cationExchangeCapacitySoilProcedure .

glosis_proc:cationExchangeCapacitySoilProcedure-CEC_ph0-kcl a glosis_proc:CationExchangeCapacitySoilProcedure,
        skos:Concept ;
    skos:definition "CEC unbuffered at pH of the soil, in 1 M KCl exchange solution" ;
    skos:inScheme glosis_proc:cationExchangeCapacitySoilProcedure ;
    skos:notation "CEC_ph0-kcl" ;
    skos:prefLabel "CEC_ph0-kcl"@en ;
    skos:scopeNote <https://www.isric.org/sites/default/files/isric_report_2014_01.pdf>,
        "Leenaars J.G.B., A.J.M. van Oostrum and M. Ruiperez Gonzalez, 2014. Africa Soil Profiles Database, Version 1.2. A compilation of georeferenced and standardised legacy soil profile data for Sub-Saharan Africa (with dataset). ISRIC Report 2014/01. Africa Soil Information Service (AfSIS) project and ISRIC - World Soil Information, Wageningen, the Netherlands. See Annex 4." ;
    skos:topConceptOf glosis_proc:cationExchangeCapacitySoilProcedure .

glosis_proc:cationExchangeCapacitySoilProcedure-CEC_ph0-nh4cl a glosis_proc:CationExchangeCapacitySoilProcedure,
        skos:Concept ;
    skos:definition "CEC unbuffered at pH of the soil, in 1 M NH4-chloride exchange solution (0.2-1.0 M)" ;
    skos:inScheme glosis_proc:cationExchangeCapacitySoilProcedure ;
    skos:notation "CEC_ph0-nh4cl" ;
    skos:prefLabel "CEC_ph0-nh4cl"@en ;
    skos:scopeNote <https://www.isric.org/sites/default/files/isric_report_2014_01.pdf>,
        "Leenaars J.G.B., A.J.M. van Oostrum and M. Ruiperez Gonzalez, 2014. Africa Soil Profiles Database, Version 1.2. A compilation of georeferenced and standardised legacy soil profile data for Sub-Saharan Africa (with dataset). ISRIC Report 2014/01. Africa Soil Information Service (AfSIS) project and ISRIC - World Soil Information, Wageningen, the Netherlands. See Annex 4." ;
    skos:topConceptOf glosis_proc:cationExchangeCapacitySoilProcedure .

glosis_proc:cationExchangeCapacitySoilProcedure-CEC_ph0-nh4oac a glosis_proc:CationExchangeCapacitySoilProcedure,
        skos:Concept ;
    skos:definition "CEC unbuffered at pH of the soil, in 1 M NH4-acetate (NH4OAc) exchange solution (0.25-1.0 M)" ;
    skos:inScheme glosis_proc:cationExchangeCapacitySoilProcedure ;
    skos:notation "CEC_ph0-nh4oac" ;
    skos:prefLabel "CEC_ph0-nh4oac"@en ;
    skos:scopeNote <https://www.isric.org/sites/default/files/isric_report_2014_01.pdf>,
        "Leenaars J.G.B., A.J.M. van Oostrum and M. Ruiperez Gonzalez, 2014. Africa Soil Profiles Database, Version 1.2. A compilation of georeferenced and standardised legacy soil profile data for Sub-Saharan Africa (with dataset). ISRIC Report 2014/01. Africa Soil Information Service (AfSIS) project and ISRIC - World Soil Information, Wageningen, the Netherlands. See Annex 4." ;
    skos:topConceptOf glosis_proc:cationExchangeCapacitySoilProcedure .

glosis_proc:cationExchangeCapacitySoilProcedure-CEC_ph0-unkn a glosis_proc:CationExchangeCapacitySoilProcedure,
        skos:Concept ;
    skos:definition "CEC unbuffered at pH of the soil, in unknown exchange solution" ;
    skos:inScheme glosis_proc:cationExchangeCapacitySoilProcedure ;
    skos:notation "CEC_ph0-unkn" ;
    skos:prefLabel "CEC_ph0-unk"@en ;
    skos:scopeNote <https://www.isric.org/sites/default/files/isric_report_2014_01.pdf>,
        "Leenaars J.G.B., A.J.M. van Oostrum and M. Ruiperez Gonzalez, 2014. Africa Soil Profiles Database, Version 1.2. A compilation of georeferenced and standardised legacy soil profile data for Sub-Saharan Africa (with dataset). ISRIC Report 2014/01. Africa Soil Information Service (AfSIS) project and ISRIC - World Soil Information, Wageningen, the Netherlands. See Annex 4." ;
    skos:topConceptOf glosis_proc:cationExchangeCapacitySoilProcedure .

glosis_proc:cationExchangeCapacitySoilProcedure-CEC_ph7-edta a glosis_proc:CationExchangeCapacitySoilProcedure,
        skos:Concept ;
    skos:definition "CEC buffered at pH 7, in 0.1 M Li-EDTA exchange solution" ;
    skos:inScheme glosis_proc:cationExchangeCapacitySoilProcedure ;
    skos:notation "CEC_ph7-edta" ;
    skos:prefLabel "CEC_ph7-edta"@en ;
    skos:scopeNote <https://www.isric.org/sites/default/files/isric_report_2014_01.pdf>,
        "Leenaars J.G.B., A.J.M. van Oostrum and M. Ruiperez Gonzalez, 2014. Africa Soil Profiles Database, Version 1.2. A compilation of georeferenced and standardised legacy soil profile data for Sub-Saharan Africa (with dataset). ISRIC Report 2014/01. Africa Soil Information Service (AfSIS) project and ISRIC - World Soil Information, Wageningen, the Netherlands. See Annex 4." ;
    skos:topConceptOf glosis_proc:cationExchangeCapacitySoilProcedure .

glosis_proc:cationExchangeCapacitySoilProcedure-CEC_ph7-nh4oac a glosis_proc:CationExchangeCapacitySoilProcedure,
        skos:Concept ;
    skos:definition "CEC buffered at pH 7, in 1 M NH4-acetate (NH4OAc) exchange solution (0.25-1.0 M)" ;
    skos:inScheme glosis_proc:cationExchangeCapacitySoilProcedure ;
    skos:notation "CEC_ph7-nh4oac" ;
    skos:prefLabel "CEC_ph7-nh4oac"@en ;
    skos:scopeNote <https://www.isric.org/sites/default/files/isric_report_2014_01.pdf>,
        "Leenaars J.G.B., A.J.M. van Oostrum and M. Ruiperez Gonzalez, 2014. Africa Soil Profiles Database, Version 1.2. A compilation of georeferenced and standardised legacy soil profile data for Sub-Saharan Africa (with dataset). ISRIC Report 2014/01. Africa Soil Information Service (AfSIS) project and ISRIC - World Soil Information, Wageningen, the Netherlands. See Annex 4." ;
    skos:topConceptOf glosis_proc:cationExchangeCapacitySoilProcedure .

glosis_proc:cationExchangeCapacitySoilProcedure-CEC_ph7-unkn a glosis_proc:CationExchangeCapacitySoilProcedure,
        skos:Concept ;
    skos:definition "CEC buffered at pH 7, in unknown exchange solution" ;
    skos:inScheme glosis_proc:cationExchangeCapacitySoilProcedure ;
    skos:notation "CEC_ph7-unkn" ;
    skos:prefLabel "CEC_ph7-unk"@en ;
    skos:scopeNote <https://www.isric.org/sites/default/files/isric_report_2014_01.pdf>,
        "Leenaars J.G.B., A.J.M. van Oostrum and M. Ruiperez Gonzalez, 2014. Africa Soil Profiles Database, Version 1.2. A compilation of georeferenced and standardised legacy soil profile data for Sub-Saharan Africa (with dataset). ISRIC Report 2014/01. Africa Soil Information Service (AfSIS) project and ISRIC - World Soil Information, Wageningen, the Netherlands. See Annex 4." ;
    skos:topConceptOf glosis_proc:cationExchangeCapacitySoilProcedure .

glosis_proc:cationExchangeCapacitySoilProcedure-CEC_ph8-bacl2tea a glosis_proc:CationExchangeCapacitySoilProcedure,
        skos:Concept ;
    skos:definition "CEC buffered at pH 8.0-8.5, in 0.5 M BaCl2-TEA exchange solution (0.1.1.0 M)" ;
    skos:inScheme glosis_proc:cationExchangeCapacitySoilProcedure ;
    skos:notation "CEC_ph8-bacl2tea" ;
    skos:prefLabel "CEC_ph8-bacl2tea"@en ;
    skos:scopeNote <https://www.isric.org/sites/default/files/isric_report_2014_01.pdf>,
        "Leenaars J.G.B., A.J.M. van Oostrum and M. Ruiperez Gonzalez, 2014. Africa Soil Profiles Database, Version 1.2. A compilation of georeferenced and standardised legacy soil profile data for Sub-Saharan Africa (with dataset). ISRIC Report 2014/01. Africa Soil Information Service (AfSIS) project and ISRIC - World Soil Information, Wageningen, the Netherlands. See Annex 4." ;
    skos:topConceptOf glosis_proc:cationExchangeCapacitySoilProcedure .

glosis_proc:cationExchangeCapacitySoilProcedure-CEC_ph8-baoac a glosis_proc:CationExchangeCapacitySoilProcedure,
        skos:Concept ;
    skos:definition "CEC buffered at pH 8.0-8.5, in 0.5 M Ba-acetate exchange solution" ;
    skos:inScheme glosis_proc:cationExchangeCapacitySoilProcedure ;
    skos:notation "CEC_ph8-baoac" ;
    skos:prefLabel "CEC_ph8-baoac"@en ;
    skos:scopeNote <https://www.isric.org/sites/default/files/isric_report_2014_01.pdf>,
        "Leenaars J.G.B., A.J.M. van Oostrum and M. Ruiperez Gonzalez, 2014. Africa Soil Profiles Database, Version 1.2. A compilation of georeferenced and standardised legacy soil profile data for Sub-Saharan Africa (with dataset). ISRIC Report 2014/01. Africa Soil Information Service (AfSIS) project and ISRIC - World Soil Information, Wageningen, the Netherlands. See Annex 4." ;
    skos:topConceptOf glosis_proc:cationExchangeCapacitySoilProcedure .

glosis_proc:cationExchangeCapacitySoilProcedure-CEC_ph8-licl2tea a glosis_proc:CationExchangeCapacitySoilProcedure,
        skos:Concept ;
    skos:definition "CEC buffered at pH 8.0-8.5, in 0.5 M Li-chloride - TEA exchange solution" ;
    skos:inScheme glosis_proc:cationExchangeCapacitySoilProcedure ;
    skos:notation "CEC_ph8-licl2tea" ;
    skos:prefLabel "CEC_ph8-licl2tea"@en ;
    skos:scopeNote <https://www.isric.org/sites/default/files/isric_report_2014_01.pdf>,
        "Leenaars J.G.B., A.J.M. van Oostrum and M. Ruiperez Gonzalez, 2014. Africa Soil Profiles Database, Version 1.2. A compilation of georeferenced and standardised legacy soil profile data for Sub-Saharan Africa (with dataset). ISRIC Report 2014/01. Africa Soil Information Service (AfSIS) project and ISRIC - World Soil Information, Wageningen, the Netherlands. See Annex 4." ;
    skos:topConceptOf glosis_proc:cationExchangeCapacitySoilProcedure .

glosis_proc:cationExchangeCapacitySoilProcedure-CEC_ph8-naoac a glosis_proc:CationExchangeCapacitySoilProcedure,
        skos:Concept ;
    skos:definition "CEC buffered at pH 8.0-8.5, in 1 M Na-acetate exchange solution" ;
    skos:inScheme glosis_proc:cationExchangeCapacitySoilProcedure ;
    skos:notation "CEC_ph8-naoac" ;
    skos:prefLabel "CEC_ph8-naoac"@en ;
    skos:scopeNote <https://www.isric.org/sites/default/files/isric_report_2014_01.pdf>,
        "Leenaars J.G.B., A.J.M. van Oostrum and M. Ruiperez Gonzalez, 2014. Africa Soil Profiles Database, Version 1.2. A compilation of georeferenced and standardised legacy soil profile data for Sub-Saharan Africa (with dataset). ISRIC Report 2014/01. Africa Soil Information Service (AfSIS) project and ISRIC - World Soil Information, Wageningen, the Netherlands. See Annex 4." ;
    skos:topConceptOf glosis_proc:cationExchangeCapacitySoilProcedure .

glosis_proc:cationExchangeCapacitySoilProcedure-CEC_ph8-nh4oac a glosis_proc:CationExchangeCapacitySoilProcedure,
        skos:Concept ;
    skos:definition "CEC buffered at pH 8.0-8.5, in 1 M NH4-acetate exchange solution (0.25-1.0 M)" ;
    skos:inScheme glosis_proc:cationExchangeCapacitySoilProcedure ;
    skos:notation "CEC_ph8-nh4oac" ;
    skos:prefLabel "CEC_ph8-nh4oac"@en ;
    skos:scopeNote <https://www.isric.org/sites/default/files/isric_report_2014_01.pdf>,
        "Leenaars J.G.B., A.J.M. van Oostrum and M. Ruiperez Gonzalez, 2014. Africa Soil Profiles Database, Version 1.2. A compilation of georeferenced and standardised legacy soil profile data for Sub-Saharan Africa (with dataset). ISRIC Report 2014/01. Africa Soil Information Service (AfSIS) project and ISRIC - World Soil Information, Wageningen, the Netherlands. See Annex 4." ;
    skos:topConceptOf glosis_proc:cationExchangeCapacitySoilProcedure .

glosis_proc:cationExchangeCapacitySoilProcedure-CEC_ph8-unkn a glosis_proc:CationExchangeCapacitySoilProcedure,
        skos:Concept ;
    skos:definition "CEC buffered at pH 8.0-8.5, in unknown exchange solution" ;
    skos:inScheme glosis_proc:cationExchangeCapacitySoilProcedure ;
    skos:notation "CEC_ph8-unkn" ;
    skos:prefLabel "CEC_ph8-unk"@en ;
    skos:scopeNote <https://www.isric.org/sites/default/files/isric_report_2014_01.pdf>,
        "Leenaars J.G.B., A.J.M. van Oostrum and M. Ruiperez Gonzalez, 2014. Africa Soil Profiles Database, Version 1.2. A compilation of georeferenced and standardised legacy soil profile data for Sub-Saharan Africa (with dataset). ISRIC Report 2014/01. Africa Soil Information Service (AfSIS) project and ISRIC - World Soil Information, Wageningen, the Netherlands. See Annex 4." ;
    skos:topConceptOf glosis_proc:cationExchangeCapacitySoilProcedure .

glosis_proc:coarseFragmentsProcedure-CrsFrg_fld a glosis_proc:CoarseFragmentsProcedure,
        skos:Concept ;
    skos:definition "Particles > 2 mm observed in the field. May include concretions and very hard aggregates" ;
    skos:inScheme glosis_proc:coarseFragmentsProcedure ;
    skos:notation "CrsFrg_fld" ;
    skos:prefLabel "CrsFrg_fld"@en ;
    skos:scopeNote <https://www.isric.org/sites/default/files/isric_report_2014_01.pdf>,
        "Leenaars J.G.B., A.J.M. van Oostrum and M. Ruiperez Gonzalez, 2014. Africa Soil Profiles Database, Version 1.2. A compilation of georeferenced and standardised legacy soil profile data for Sub-Saharan Africa (with dataset). ISRIC Report 2014/01. Africa Soil Information Service (AfSIS) project and ISRIC - World Soil Information, Wageningen, the Netherlands. See Annex 4." ;
    skos:topConceptOf glosis_proc:coarseFragmentsProcedure .

glosis_proc:coarseFragmentsProcedure-CrsFrg_fldcls a glosis_proc:CoarseFragmentsProcedure,
        skos:Concept ;
    skos:definition "Particles > 2 mm observed in the field and calculated from class values. May include concretions and very hard aggregates" ;
    skos:inScheme glosis_proc:coarseFragmentsProcedure ;
    skos:notation "CrsFrg_fldcls" ;
    skos:prefLabel "CrsFrg_fldcls"@en ;
    skos:scopeNote <https://www.isric.org/sites/default/files/isric_report_2014_01.pdf>,
        "Leenaars J.G.B., A.J.M. van Oostrum and M. Ruiperez Gonzalez, 2014. Africa Soil Profiles Database, Version 1.2. A compilation of georeferenced and standardised legacy soil profile data for Sub-Saharan Africa (with dataset). ISRIC Report 2014/01. Africa Soil Information Service (AfSIS) project and ISRIC - World Soil Information, Wageningen, the Netherlands. See Annex 4." ;
    skos:topConceptOf glosis_proc:coarseFragmentsProcedure .

glosis_proc:coarseFragmentsProcedure-CrsFrg_lab a glosis_proc:CoarseFragmentsProcedure,
        skos:Concept ;
    skos:definition "Particles > 2 mm measured in laboratory (sieved after light pounding). May include concretions and very hard aggregates" ;
    skos:inScheme glosis_proc:coarseFragmentsProcedure ;
    skos:notation "CrsFrg_lab" ;
    skos:prefLabel "CrsFrg_lab"@en ;
    skos:scopeNote <https://www.isric.org/sites/default/files/isric_report_2014_01.pdf>,
        "Leenaars J.G.B., A.J.M. van Oostrum and M. Ruiperez Gonzalez, 2014. Africa Soil Profiles Database, Version 1.2. A compilation of georeferenced and standardised legacy soil profile data for Sub-Saharan Africa (with dataset). ISRIC Report 2014/01. Africa Soil Information Service (AfSIS) project and ISRIC - World Soil Information, Wageningen, the Netherlands. See Annex 4." ;
    skos:topConceptOf glosis_proc:coarseFragmentsProcedure .

glosis_proc:effectiveCecProcedure-EffCEC_calcul-b a glosis_proc:EffectiveCecProcedure,
        skos:Concept ;
    skos:definition "Sum of exchangeable bases (Ca, Mg, K, Na) without exchangeable acidity (H+Al), see ExchBases and ExchAcids for methods" ;
    skos:inScheme glosis_proc:effectiveCecProcedure ;
    skos:notation "EffCEC_calcul-b" ;
    skos:prefLabel "EffCEC_calcul-b"@en ;
    skos:scopeNote <https://www.isric.org/sites/default/files/isric_report_2014_01.pdf>,
        "Leenaars J.G.B., A.J.M. van Oostrum and M. Ruiperez Gonzalez, 2014. Africa Soil Profiles Database, Version 1.2. A compilation of georeferenced and standardised legacy soil profile data for Sub-Saharan Africa (with dataset). ISRIC Report 2014/01. Africa Soil Information Service (AfSIS) project and ISRIC - World Soil Information, Wageningen, the Netherlands. See Annex 4." ;
    skos:topConceptOf glosis_proc:effectiveCecProcedure .

glosis_proc:effectiveCecProcedure-EffCEC_calcul-ba a glosis_proc:EffectiveCecProcedure,
        skos:Concept ;
    skos:definition "Sum of exchangeable bases (Ca, Mg, K, Na) plus exchangeable acidity (H+Al), see ExchBases and ExchAcids for methods" ;
    skos:inScheme glosis_proc:effectiveCecProcedure ;
    skos:notation "EffCEC_calcul-ba" ;
    skos:prefLabel "EffCEC_calcul-ba"@en ;
    skos:scopeNote <https://www.isric.org/sites/default/files/isric_report_2014_01.pdf>,
        "Leenaars J.G.B., A.J.M. van Oostrum and M. Ruiperez Gonzalez, 2014. Africa Soil Profiles Database, Version 1.2. A compilation of georeferenced and standardised legacy soil profile data for Sub-Saharan Africa (with dataset). ISRIC Report 2014/01. Africa Soil Information Service (AfSIS) project and ISRIC - World Soil Information, Wageningen, the Netherlands. See Annex 4." ;
    skos:topConceptOf glosis_proc:effectiveCecProcedure .

glosis_proc:electricalConductivityProcedure-EC_ratio1-1 a glosis_proc:ElectricalConductivityProcedure,
        skos:Concept ;
    skos:definition "Elec. conductivity at 1:1 soil/water ratio" ;
    skos:inScheme glosis_proc:electricalConductivityProcedure ;
    skos:notation "EC_ratio1-1" ;
    skos:prefLabel "EC_ratio1-1"@en ;
    skos:scopeNote <https://www.isric.org/sites/default/files/isric_report_2014_01.pdf>,
        "Leenaars J.G.B., A.J.M. van Oostrum and M. Ruiperez Gonzalez, 2014. Africa Soil Profiles Database, Version 1.2. A compilation of georeferenced and standardised legacy soil profile data for Sub-Saharan Africa (with dataset). ISRIC Report 2014/01. Africa Soil Information Service (AfSIS) project and ISRIC - World Soil Information, Wageningen, the Netherlands. See Annex 4." ;
    skos:topConceptOf glosis_proc:electricalConductivityProcedure .

glosis_proc:electricalConductivityProcedure-EC_ratio1-10 a glosis_proc:ElectricalConductivityProcedure,
        skos:Concept ;
    skos:definition "Elec. conductivity at 1:10 soil/water ratio" ;
    skos:inScheme glosis_proc:electricalConductivityProcedure ;
    skos:notation "EC_ratio1-10" ;
    skos:prefLabel "EC_ratio1-10"@en ;
    skos:scopeNote <https://www.isric.org/sites/default/files/isric_report_2014_01.pdf>,
        "Leenaars J.G.B., A.J.M. van Oostrum and M. Ruiperez Gonzalez, 2014. Africa Soil Profiles Database, Version 1.2. A compilation of georeferenced and standardised legacy soil profile data for Sub-Saharan Africa (with dataset). ISRIC Report 2014/01. Africa Soil Information Service (AfSIS) project and ISRIC - World Soil Information, Wageningen, the Netherlands. See Annex 4." ;
    skos:topConceptOf glosis_proc:electricalConductivityProcedure .

glosis_proc:electricalConductivityProcedure-EC_ratio1-2 a glosis_proc:ElectricalConductivityProcedure,
        skos:Concept ;
    skos:definition "Elec. conductivity at 1:2 soil/water ratio" ;
    skos:inScheme glosis_proc:electricalConductivityProcedure ;
    skos:notation "EC_ratio1-2" ;
    skos:prefLabel "EC_ratio1-2"@en ;
    skos:scopeNote <https://www.isric.org/sites/default/files/isric_report_2014_01.pdf>,
        "Leenaars J.G.B., A.J.M. van Oostrum and M. Ruiperez Gonzalez, 2014. Africa Soil Profiles Database, Version 1.2. A compilation of georeferenced and standardised legacy soil profile data for Sub-Saharan Africa (with dataset). ISRIC Report 2014/01. Africa Soil Information Service (AfSIS) project and ISRIC - World Soil Information, Wageningen, the Netherlands. See Annex 4." ;
    skos:topConceptOf glosis_proc:electricalConductivityProcedure .

glosis_proc:electricalConductivityProcedure-EC_ratio1-2.5 a glosis_proc:ElectricalConductivityProcedure,
        skos:Concept ;
    skos:definition "Elec. conductivity at 1:2.5 soil/water ratio" ;
    skos:inScheme glosis_proc:electricalConductivityProcedure ;
    skos:notation "EC_ratio1-2.5" ;
    skos:prefLabel "EC_ratio1-2.5"@en ;
    skos:scopeNote <https://www.isric.org/sites/default/files/isric_report_2014_01.pdf>,
        "Leenaars J.G.B., A.J.M. van Oostrum and M. Ruiperez Gonzalez, 2014. Africa Soil Profiles Database, Version 1.2. A compilation of georeferenced and standardised legacy soil profile data for Sub-Saharan Africa (with dataset). ISRIC Report 2014/01. Africa Soil Information Service (AfSIS) project and ISRIC - World Soil Information, Wageningen, the Netherlands. See Annex 4." ;
    skos:topConceptOf glosis_proc:electricalConductivityProcedure .

glosis_proc:electricalConductivityProcedure-EC_ratio1-5 a glosis_proc:ElectricalConductivityProcedure,
        skos:Concept ;
    skos:definition "Elec. conductivity at 1:5 soil/water ratio" ;
    skos:inScheme glosis_proc:electricalConductivityProcedure ;
    skos:notation "EC_ratio1-5" ;
    skos:prefLabel "EC_ratio1-5"@en ;
    skos:scopeNote <https://www.isric.org/sites/default/files/isric_report_2014_01.pdf>,
        "Leenaars J.G.B., A.J.M. van Oostrum and M. Ruiperez Gonzalez, 2014. Africa Soil Profiles Database, Version 1.2. A compilation of georeferenced and standardised legacy soil profile data for Sub-Saharan Africa (with dataset). ISRIC Report 2014/01. Africa Soil Information Service (AfSIS) project and ISRIC - World Soil Information, Wageningen, the Netherlands. See Annex 4." ;
    skos:topConceptOf glosis_proc:electricalConductivityProcedure .

glosis_proc:electricalConductivityProcedure-ECe_sat a glosis_proc:ElectricalConductivityProcedure,
        skos:Concept ;
    skos:definition "Elec. conductivity in saturated paste (ECe)" ;
    skos:inScheme glosis_proc:electricalConductivityProcedure ;
    skos:notation "ECe_sat" ;
    skos:prefLabel "ECe_sat"@en ;
    skos:scopeNote <https://www.isric.org/sites/default/files/isric_report_2014_01.pdf>,
        "Leenaars J.G.B., A.J.M. van Oostrum and M. Ruiperez Gonzalez, 2014. Africa Soil Profiles Database, Version 1.2. A compilation of georeferenced and standardised legacy soil profile data for Sub-Saharan Africa (with dataset). ISRIC Report 2014/01. Africa Soil Information Service (AfSIS) project and ISRIC - World Soil Information, Wageningen, the Netherlands. See Annex 4." ;
    skos:topConceptOf glosis_proc:electricalConductivityProcedure .

glosis_proc:exchangeableBasesProcedure-ExchBases_ph-unkn-edta a glosis_proc:ExchangeableBasesProcedure,
        skos:Concept ;
    skos:definition "Exch bases (Ca, Mg, K, Na) unknown buffer, in EDTA solution" ;
    skos:inScheme glosis_proc:exchangeableBasesProcedure ;
    skos:notation "ExchBases_ph-unkn-edta" ;
    skos:prefLabel "ExchBases_ph-unkn-edta"@en ;
    skos:scopeNote <https://www.isric.org/sites/default/files/isric_report_2014_01.pdf>,
        "Leenaars J.G.B., A.J.M. van Oostrum and M. Ruiperez Gonzalez, 2014. Africa Soil Profiles Database, Version 1.2. A compilation of georeferenced and standardised legacy soil profile data for Sub-Saharan Africa (with dataset). ISRIC Report 2014/01. Africa Soil Information Service (AfSIS) project and ISRIC - World Soil Information, Wageningen, the Netherlands. See Annex 4." ;
    skos:topConceptOf glosis_proc:exchangeableBasesProcedure .

glosis_proc:exchangeableBasesProcedure-ExchBases_ph-unkn-m3 a glosis_proc:ExchangeableBasesProcedure,
        skos:Concept ;
    skos:definition "Exch bases (Ca, Mg, K, Na) unknown buffer, in Mehlich3 solution with extractable ppm assumed exchangeable cmolc/kg" ;
    skos:inScheme glosis_proc:exchangeableBasesProcedure ;
    skos:notation "ExchBases_ph-unkn-m3" ;
    skos:prefLabel "ExchBases_ph-unkn-m3"@en ;
    skos:scopeNote <https://doi.org/10.1080/00103628409367568> ;
    skos:topConceptOf glosis_proc:exchangeableBasesProcedure .

glosis_proc:exchangeableBasesProcedure-ExchBases_ph-unkn-m3-spec a glosis_proc:ExchangeableBasesProcedure,
        skos:Concept ;
    skos:definition "Exch bases (Ca, Mg, K, Na) spectrally measured and converted to, unknown buffer, in Mehlich3 solution with extractable ppm assumed exchangeable cmolc/kg" ;
    skos:inScheme glosis_proc:exchangeableBasesProcedure ;
    skos:notation "ExchBases_ph-unkn-m3-spec" ;
    skos:prefLabel "ExchBases_ph-unkn-m3-spec"@en ;
    skos:scopeNote <https://doi.org/10.1080/00103628409367568> ;
    skos:topConceptOf glosis_proc:exchangeableBasesProcedure .

glosis_proc:exchangeableBasesProcedure-ExchBases_ph0-cohex a glosis_proc:ExchangeableBasesProcedure,
        skos:Concept ;
    skos:definition "Exch bases (Ca, Mg, K, Na) unbuffered, in Cobalt(III) hexamine chloride solution 0,0166M (Cohex) [Co[NH3]6]Cl3 ), ISO 23470 (2007)" ;
    skos:inScheme glosis_proc:exchangeableBasesProcedure ;
    skos:notation "ExchBases_ph0-cohex" ;
    skos:prefLabel "ExchBases_ph0-cohex"@en ;
    skos:scopeNote <https://www.iso.org/standard/36879.html> ;
    skos:topConceptOf glosis_proc:exchangeableBasesProcedure .

glosis_proc:exchangeableBasesProcedure-ExchBases_ph0-nh4cl a glosis_proc:ExchangeableBasesProcedure,
        skos:Concept ;
    skos:definition "Exch bases (Ca, Mg, K, Na) unbuffered, in 1 M NH4Cl (0.05-1.0 m?)" ;
    skos:inScheme glosis_proc:exchangeableBasesProcedure ;
    skos:notation "ExchBases_ph0-nh4cl" ;
    skos:prefLabel "ExchBases_ph0-nh4cl"@en ;
    skos:scopeNote <https://www.isric.org/sites/default/files/isric_report_2014_01.pdf>,
        "Leenaars J.G.B., A.J.M. van Oostrum and M. Ruiperez Gonzalez, 2014. Africa Soil Profiles Database, Version 1.2. A compilation of georeferenced and standardised legacy soil profile data for Sub-Saharan Africa (with dataset). ISRIC Report 2014/01. Africa Soil Information Service (AfSIS) project and ISRIC - World Soil Information, Wageningen, the Netherlands. See Annex 4." ;
    skos:topConceptOf glosis_proc:exchangeableBasesProcedure .

glosis_proc:exchangeableBasesProcedure-ExchBases_ph7-nh4oac a glosis_proc:ExchangeableBasesProcedure,
        skos:Concept ;
    skos:definition "Exch bases (Ca, Mg, K, Na) buffered at pH 7, in 1M NH4OAc" ;
    skos:inScheme glosis_proc:exchangeableBasesProcedure ;
    skos:notation "ExchBases_ph7-nh4oac" ;
    skos:prefLabel "ExchBases_ph7-nh4oac"@en ;
    skos:scopeNote <https://www.isric.org/sites/default/files/isric_report_2014_01.pdf>,
        "Leenaars J.G.B., A.J.M. van Oostrum and M. Ruiperez Gonzalez, 2014. Africa Soil Profiles Database, Version 1.2. A compilation of georeferenced and standardised legacy soil profile data for Sub-Saharan Africa (with dataset). ISRIC Report 2014/01. Africa Soil Information Service (AfSIS) project and ISRIC - World Soil Information, Wageningen, the Netherlands. See Annex 4." ;
    skos:topConceptOf glosis_proc:exchangeableBasesProcedure .

glosis_proc:exchangeableBasesProcedure-ExchBases_ph7-nh4oac-aas a glosis_proc:ExchangeableBasesProcedure,
        skos:Concept ;
    skos:definition "Exch bases (Ca, Mg, K, Na) buffered at pH 7, in 1M NH4OAc, Ca and Mg with AAS (Atomic Absorption Spectrometry)" ;
    skos:inScheme glosis_proc:exchangeableBasesProcedure ;
    skos:notation "ExchBases_ph7-nh4oac-aas" ;
    skos:prefLabel "ExchBases_ph7-nh4oac-aas"@en ;
    skos:scopeNote <https://www.isric.org/sites/default/files/isric_report_2014_01.pdf>,
        "Leenaars J.G.B., A.J.M. van Oostrum and M. Ruiperez Gonzalez, 2014. Africa Soil Profiles Database, Version 1.2. A compilation of georeferenced and standardised legacy soil profile data for Sub-Saharan Africa (with dataset). ISRIC Report 2014/01. Africa Soil Information Service (AfSIS) project and ISRIC - World Soil Information, Wageningen, the Netherlands. See Annex 4." ;
    skos:topConceptOf glosis_proc:exchangeableBasesProcedure .

glosis_proc:exchangeableBasesProcedure-ExchBases_ph7-nh4oac-fp a glosis_proc:ExchangeableBasesProcedure,
        skos:Concept ;
    skos:definition "Exch bases (Ca, Mg, K, Na) buffered at pH 7, in 1M NH4OAc, K and Na with FP (Flame Photometry)" ;
    skos:inScheme glosis_proc:exchangeableBasesProcedure ;
    skos:notation "ExchBases_ph7-nh4oac-fp" ;
    skos:prefLabel "ExchBases_ph7-nh4oac-fp"@en ;
    skos:scopeNote <https://www.isric.org/sites/default/files/isric_report_2014_01.pdf>,
        "Leenaars J.G.B., A.J.M. van Oostrum and M. Ruiperez Gonzalez, 2014. Africa Soil Profiles Database, Version 1.2. A compilation of georeferenced and standardised legacy soil profile data for Sub-Saharan Africa (with dataset). ISRIC Report 2014/01. Africa Soil Information Service (AfSIS) project and ISRIC - World Soil Information, Wageningen, the Netherlands. See Annex 4." ;
    skos:topConceptOf glosis_proc:exchangeableBasesProcedure .

glosis_proc:exchangeableBasesProcedure-ExchBases_ph7-unkn a glosis_proc:ExchangeableBasesProcedure,
        skos:Concept ;
    skos:definition "Exch bases (Ca, Mg, K, Na) buffered at pH 7, in unknown solution" ;
    skos:inScheme glosis_proc:exchangeableBasesProcedure ;
    skos:notation "ExchBases_ph7-unkn" ;
    skos:prefLabel "ExchBases_ph7-unk"@en ;
    skos:scopeNote <https://www.isric.org/sites/default/files/WOSISprocedureManual_2020nov17web.pdf#page=70> ;
    skos:topConceptOf glosis_proc:exchangeableBasesProcedure .

glosis_proc:exchangeableBasesProcedure-ExchBases_ph8-bacl2tea a glosis_proc:ExchangeableBasesProcedure,
        skos:Concept ;
    skos:definition "Exch bases (Ca, Mg, K, Na) buffered at pH 8.0-8.5, in 0.5 M BaCl2 - TEA solution" ;
    skos:inScheme glosis_proc:exchangeableBasesProcedure ;
    skos:notation "ExchBases_ph8-bacl2tea" ;
    skos:prefLabel "ExchBases_ph8-bacl2tea"@en ;
    skos:scopeNote <https://www.isric.org/sites/default/files/isric_report_2014_01.pdf>,
        "Leenaars J.G.B., A.J.M. van Oostrum and M. Ruiperez Gonzalez, 2014. Africa Soil Profiles Database, Version 1.2. A compilation of georeferenced and standardised legacy soil profile data for Sub-Saharan Africa (with dataset). ISRIC Report 2014/01. Africa Soil Information Service (AfSIS) project and ISRIC - World Soil Information, Wageningen, the Netherlands. See Annex 4." ;
    skos:topConceptOf glosis_proc:exchangeableBasesProcedure .

glosis_proc:exchangeableBasesProcedure-ExchBases_ph8-unkn a glosis_proc:ExchangeableBasesProcedure,
        skos:Concept ;
    skos:definition "Exch bases (Ca, Mg, K, Na) buffered at pH 8.0-8.5, in unknown solution" ;
    skos:inScheme glosis_proc:exchangeableBasesProcedure ;
    skos:notation "ExchBases_ph8-unkn" ;
    skos:prefLabel "ExchBases_ph8-unk"@en ;
    skos:scopeNote <https://www.isric.org/sites/default/files/isric_report_2014_01.pdf>,
        "Leenaars J.G.B., A.J.M. van Oostrum and M. Ruiperez Gonzalez, 2014. Africa Soil Profiles Database, Version 1.2. A compilation of georeferenced and standardised legacy soil profile data for Sub-Saharan Africa (with dataset). ISRIC Report 2014/01. Africa Soil Information Service (AfSIS) project and ISRIC - World Soil Information, Wageningen, the Netherlands. See Annex 4." ;
    skos:topConceptOf glosis_proc:exchangeableBasesProcedure .

glosis_proc:extractableElementsProcedure-Extr_ap14 a glosis_proc:ExtractableElementsProcedure,
        skos:Concept ;
    skos:definition "Method of Saunders and Metelerkamp (anion-exch. resin). Particularly used for available P." ;
    skos:inScheme glosis_proc:extractableElementsProcedure ;
    skos:notation "Extr_ap14" ;
    skos:prefLabel "Extr_ap14"@en ;
    skos:scopeNote "Saunders and Metelerkamp" ;
    skos:topConceptOf glosis_proc:extractableElementsProcedure .

glosis_proc:extractableElementsProcedure-Extr_ap15 a glosis_proc:ExtractableElementsProcedure,
        skos:Concept ;
    skos:definition "Method of Hunter (1975) modified after ISFEI method. Particularly used for available P." ;
    skos:inScheme glosis_proc:extractableElementsProcedure ;
    skos:notation "Extr_ap15" ;
    skos:prefLabel "Extr_ap15"@en ;
    skos:scopeNote "Hunter, A. 1975. New techniques and equipment for routine soil/plant analytical procedures. In: Soil Management in Tropical America. (eds E. Borremiza & A. Alvarado). N.C. State University, Raleigh, NC." ;
    skos:topConceptOf glosis_proc:extractableElementsProcedure .

glosis_proc:extractableElementsProcedure-Extr_ap20 a glosis_proc:ExtractableElementsProcedure,
        skos:Concept ;
    skos:definition "Olsen (not acid soils) resp. Bray I (acid soils). Particularly used for available P." ;
    skos:inScheme glosis_proc:extractableElementsProcedure ;
    skos:notation "Extr_ap20" ;
    skos:prefLabel "Extr_ap20"@en ;
    skos:scopeNote <https://www.isric.org/sites/default/files/isric_report_2014_01.pdf>,
        "Leenaars J.G.B., A.J.M. van Oostrum and M. Ruiperez Gonzalez, 2014. Africa Soil Profiles Database, Version 1.2. A compilation of georeferenced and standardised legacy soil profile data for Sub-Saharan Africa (with dataset). ISRIC Report 2014/01. Africa Soil Information Service (AfSIS) project and ISRIC - World Soil Information, Wageningen, the Netherlands. See Annex 4." ;
    skos:topConceptOf glosis_proc:extractableElementsProcedure .

glosis_proc:extractableElementsProcedure-Extr_ap21 a glosis_proc:ExtractableElementsProcedure,
        skos:Concept ;
    skos:definition "Olsen (if pH > 7) resp. Mehlich (if pH < 7). Particularly used for available P." ;
    skos:inScheme glosis_proc:extractableElementsProcedure ;
    skos:notation "Extr_ap21" ;
    skos:prefLabel "Extr_ap21"@en ;
    skos:scopeNote <https://www.isric.org/sites/default/files/isric_report_2014_01.pdf>,
        "Leenaars J.G.B., A.J.M. van Oostrum and M. Ruiperez Gonzalez, 2014. Africa Soil Profiles Database, Version 1.2. A compilation of georeferenced and standardised legacy soil profile data for Sub-Saharan Africa (with dataset). ISRIC Report 2014/01. Africa Soil Information Service (AfSIS) project and ISRIC - World Soil Information, Wageningen, the Netherlands. See Annex 4." ;
    skos:topConceptOf glosis_proc:extractableElementsProcedure .

glosis_proc:extractableElementsProcedure-Extr_c6h8o7-reeuwijk a glosis_proc:ExtractableElementsProcedure,
        skos:Concept ;
    skos:definition "Complexation with citric acid (van Reeuwijk). Particularly used for available P." ;
    skos:inScheme glosis_proc:extractableElementsProcedure ;
    skos:notation "Extr_c6h8o7-reeuwijk" ;
    skos:prefLabel "Extr_c6h8o7-reeuwijk"@en ;
    skos:scopeNote <https://www.isric.org/documents/document-type/technical-paper-09-procedures-soil-analysis-6th-edition> ;
    skos:topConceptOf glosis_proc:extractableElementsProcedure .

glosis_proc:extractableElementsProcedure-Extr_cacl2 a glosis_proc:ExtractableElementsProcedure,
        skos:Concept ;
    skos:definition "CaCl2. Particularly used for soluble P." ;
    skos:inScheme glosis_proc:extractableElementsProcedure ;
    skos:notation "Extr_cacl2" ;
    skos:prefLabel "Extr_cacl2"@en ;
    skos:scopeNote <https://www.isric.org/sites/default/files/isric_report_2014_01.pdf>,
        "Leenaars J.G.B., A.J.M. van Oostrum and M. Ruiperez Gonzalez, 2014. Africa Soil Profiles Database, Version 1.2. A compilation of georeferenced and standardised legacy soil profile data for Sub-Saharan Africa (with dataset). ISRIC Report 2014/01. Africa Soil Information Service (AfSIS) project and ISRIC - World Soil Information, Wageningen, the Netherlands. See Annex 4." ;
    skos:topConceptOf glosis_proc:extractableElementsProcedure .

glosis_proc:extractableElementsProcedure-Extr_capo4 a glosis_proc:ExtractableElementsProcedure,
        skos:Concept ;
    skos:definition "Ca phosphate. Particularly used for available S." ;
    skos:inScheme glosis_proc:extractableElementsProcedure ;
    skos:notation "Extr_capo4" ;
    skos:prefLabel "Extr_capo4"@en ;
    skos:scopeNote <https://www.isric.org/sites/default/files/isric_report_2014_01.pdf>,
        "Leenaars J.G.B., A.J.M. van Oostrum and M. Ruiperez Gonzalez, 2014. Africa Soil Profiles Database, Version 1.2. A compilation of georeferenced and standardised legacy soil profile data for Sub-Saharan Africa (with dataset). ISRIC Report 2014/01. Africa Soil Information Service (AfSIS) project and ISRIC - World Soil Information, Wageningen, the Netherlands. See Annex 4." ;
    skos:topConceptOf glosis_proc:extractableElementsProcedure .

glosis_proc:extractableElementsProcedure-Extr_dtpa a glosis_proc:ExtractableElementsProcedure,
        skos:Concept ;
    skos:definition "DiethyneleTriaminePentaAcetic acid (DTPA) method" ;
    skos:inScheme glosis_proc:extractableElementsProcedure ;
    skos:notation "Extr_dtpa" ;
    skos:prefLabel "Extr_dtpa"@en ;
    skos:scopeNote <https://doi.org/10.2136/sssaj1978.03615995004200030009x> ;
    skos:topConceptOf glosis_proc:extractableElementsProcedure .

glosis_proc:extractableElementsProcedure-Extr_edta a glosis_proc:ExtractableElementsProcedure,
        skos:Concept ;
    skos:definition "EthyleneDiamineTetraAcetic acid (EDTA) method" ;
    skos:inScheme glosis_proc:extractableElementsProcedure ;
    skos:notation "Extr_edta" ;
    skos:prefLabel "Extr_edta"@en ;
    skos:scopeNote <https://journals.lww.com/soilsci/Citation/1954/10000/SOIL_AND_PLANT_STUDIES_WITH_CHELATES_OF.8.aspx> ;
    skos:topConceptOf glosis_proc:extractableElementsProcedure .

glosis_proc:extractableElementsProcedure-Extr_h2so4-truog a glosis_proc:ExtractableElementsProcedure,
        skos:Concept ;
    skos:definition "Method of Truog (dilute H2SO4). Particularly used for available P." ;
    skos:inScheme glosis_proc:extractableElementsProcedure ;
    skos:notation "Extr_h2so4-truog" ;
    skos:prefLabel "Extr_h2so4-truog"@en ;
    skos:scopeNote <https://doi.org/10.2134/agronj1930.00021962002200100008x> ;
    skos:topConceptOf glosis_proc:extractableElementsProcedure .

glosis_proc:extractableElementsProcedure-Extr_hcl-h2so4-nelson a glosis_proc:ExtractableElementsProcedure,
        skos:Concept ;
    skos:definition "Method of Nelson (dilute HCl/H2SO4). Particularly used for available P." ;
    skos:inScheme glosis_proc:extractableElementsProcedure ;
    skos:notation "Extr_hcl-h2so4-nelson" ;
    skos:prefLabel "Extr_hcl-h2so4-nelso"@en ;
    skos:scopeNote <https://www.isric.org/sites/default/files/isric_report_2014_01.pdf>,
        "Leenaars J.G.B., A.J.M. van Oostrum and M. Ruiperez Gonzalez, 2014. Africa Soil Profiles Database, Version 1.2. A compilation of georeferenced and standardised legacy soil profile data for Sub-Saharan Africa (with dataset). ISRIC Report 2014/01. Africa Soil Information Service (AfSIS) project and ISRIC - World Soil Information, Wageningen, the Netherlands. See Annex 4." ;
    skos:topConceptOf glosis_proc:extractableElementsProcedure .

glosis_proc:extractableElementsProcedure-Extr_hcl-nh4f-bray1 a glosis_proc:ExtractableElementsProcedure,
        skos:Concept ;
    skos:definition "Method of Bray I  (dilute HCl/NH4F). Particularly used for available P." ;
    skos:inScheme glosis_proc:extractableElementsProcedure ;
    skos:notation "Extr_hcl-nh4f-bray1" ;
    skos:prefLabel "Extr_hcl-nh4f-bray1"@en ;
    skos:scopeNote <https://doi.org/10.1097/00010694-194501000-00006> ;
    skos:topConceptOf glosis_proc:extractableElementsProcedure .

glosis_proc:extractableElementsProcedure-Extr_hcl-nh4f-bray2 a glosis_proc:ExtractableElementsProcedure,
        skos:Concept ;
    skos:definition "Method of Bray II (dilute HCl/NH4F). Particularly used for available P." ;
    skos:inScheme glosis_proc:extractableElementsProcedure ;
    skos:notation "Extr_hcl-nh4f-bray2" ;
    skos:prefLabel "Extr_hcl-nh4f-bray2"@en ;
    skos:scopeNote <https://doi.org/10.1097/00010694-194501000-00006> ;
    skos:topConceptOf glosis_proc:extractableElementsProcedure .

glosis_proc:extractableElementsProcedure-Extr_hcl-nh4f-kurtz-bray a glosis_proc:ExtractableElementsProcedure,
        skos:Concept ;
    skos:definition "Method of Kurtz-Bray I (0.025 M HCl + 0.03 M NH4F). Particularly used for available P." ;
    skos:inScheme glosis_proc:extractableElementsProcedure ;
    skos:notation "Extr_hcl-nh4f-kurtz-bray" ;
    skos:prefLabel "Extr_hcl-nh4f-kurtz-bray"@en ;
    skos:scopeNote <https://doi.org/10.1097/00010694-194501000-00006> ;
    skos:topConceptOf glosis_proc:extractableElementsProcedure .

glosis_proc:extractableElementsProcedure-Extr_hno3 a glosis_proc:ExtractableElementsProcedure,
        skos:Concept ;
    skos:definition "Nitric acid (HNO3) method" ;
    skos:inScheme glosis_proc:extractableElementsProcedure ;
    skos:notation "Extr_hno3" ;
    skos:prefLabel "Extr_hno3"@en ;
    skos:scopeNote <https://www.iso.org/standard/60060.html>,
        "ISO. ISO/DIS 17586 Soil Quality - Extraction of Trace Elements Using Dilute Nitric Acid, 2016; p 14" ;
    skos:topConceptOf glosis_proc:extractableElementsProcedure .

glosis_proc:extractableElementsProcedure-Extr_hotwater a glosis_proc:ExtractableElementsProcedure,
        skos:Concept ;
    skos:definition "Hot water. Particularly used for available B" ;
    skos:inScheme glosis_proc:extractableElementsProcedure ;
    skos:notation "Extr_hotwater" ;
    skos:prefLabel "Extr_hotwater"@en ;
    skos:scopeNote <https://www.isric.org/sites/default/files/isric_report_2014_01.pdf>,
        "Leenaars J.G.B., A.J.M. van Oostrum and M. Ruiperez Gonzalez, 2014. Africa Soil Profiles Database, Version 1.2. A compilation of georeferenced and standardised legacy soil profile data for Sub-Saharan Africa (with dataset). ISRIC Report 2014/01. Africa Soil Information Service (AfSIS) project and ISRIC - World Soil Information, Wageningen, the Netherlands. See Annex 4." ;
    skos:topConceptOf glosis_proc:extractableElementsProcedure .

glosis_proc:extractableElementsProcedure-Extr_m1 a glosis_proc:ExtractableElementsProcedure,
        skos:Concept ;
    skos:definition "Mehlich1 method" ;
    skos:inScheme glosis_proc:extractableElementsProcedure ;
    skos:notation "Extr_m1" ;
    skos:prefLabel "Extr_m1"@en ;
    skos:scopeNote <https://www.ncagr.gov/AGRONOMI/pdffiles/mehlich53.pdf> ;
    skos:topConceptOf glosis_proc:extractableElementsProcedure .

glosis_proc:extractableElementsProcedure-Extr_m2 a glosis_proc:ExtractableElementsProcedure,
        skos:Concept ;
    skos:definition "Mehlich2 method" ;
    skos:inScheme glosis_proc:extractableElementsProcedure ;
    skos:notation "Extr_m2" ;
    skos:prefLabel "Extr_m2"@en ;
    skos:scopeNote <https://doi.org/10.1080/00103627609366673> ;
    skos:topConceptOf glosis_proc:extractableElementsProcedure .

glosis_proc:extractableElementsProcedure-Extr_m3 a glosis_proc:ExtractableElementsProcedure,
        skos:Concept ;
    skos:definition "Mehlich3 method (extractant 0.2 N CH3COOH + 0.25 N NH4NO3 + 0.015 N NH4F + 0.013 N HNO3 + 0.001 M EDTA)" ;
    skos:inScheme glosis_proc:extractableElementsProcedure ;
    skos:notation "Extr_m3" ;
    skos:prefLabel "Extr_m3"@en ;
    skos:scopeNote <https://doi.org/10.1080/00103628409367568> ;
    skos:topConceptOf glosis_proc:extractableElementsProcedure .

glosis_proc:extractableElementsProcedure-Extr_m3-spec a glosis_proc:ExtractableElementsProcedure,
        skos:Concept ;
    skos:definition "Spectrally measured and converted to Mehlich3 method (extractant 0.2 N CH3COOH + 0.25 N NH4NO3 + 0.015 N NH4F + 0.013 N HNO3 + 0.001 M EDTA)" ;
    skos:inScheme glosis_proc:extractableElementsProcedure ;
    skos:notation "Extr_m3-spec" ;
    skos:prefLabel "Extr_m3-spec"@en ;
    skos:scopeNote <https://doi.org/10.1080/00103628409367568> ;
    skos:topConceptOf glosis_proc:extractableElementsProcedure .

glosis_proc:extractableElementsProcedure-Extr_nahco3-olsen a glosis_proc:ExtractableElementsProcedure,
        skos:Concept ;
    skos:definition "Method of Olsen (0.5 M Sodium Bicarbonate (NaHCO3) extraction at pH8.5). Particularly used for available P." ;
    skos:inScheme glosis_proc:extractableElementsProcedure ;
    skos:notation "Extr_nahco3-olsen" ;
    skos:prefLabel "Extr_nahco3-ols"@en ;
    skos:scopeNote <https://acsess.onlinelibrary.wiley.com/doi/book/10.2134/agronmonogr9.2> ;
    skos:topConceptOf glosis_proc:extractableElementsProcedure .

glosis_proc:extractableElementsProcedure-Extr_nahco3-olsen-dabin a glosis_proc:ExtractableElementsProcedure,
        skos:Concept ;
    skos:definition "Method of Olsen, modified by Dabin (ORSTOM). Particularly used for available P." ;
    skos:inScheme glosis_proc:extractableElementsProcedure ;
    skos:notation "Extr_nahco3-olsen-dabin" ;
    skos:prefLabel "Extr_nahco3-olsen-dabi"@en ;
    skos:scopeNote <https://docplayer.fr/81912854-Application-des-dosages-automatiques-a-l-analyse-des-sols-2e-partie-par.html> ;
    skos:topConceptOf glosis_proc:extractableElementsProcedure .

glosis_proc:extractableElementsProcedure-Extr_naoac-morgan a glosis_proc:ExtractableElementsProcedure,
        skos:Concept ;
    skos:definition "Method of Morgan (Na-acetate/acetic acid). Particularly used for available P." ;
    skos:inScheme glosis_proc:extractableElementsProcedure ;
    skos:notation "Extr_naoac-morgan" ;
    skos:prefLabel "Extr_naoac-morga"@en ;
    skos:scopeNote <https://portal.ct.gov/-/media/CAES/DOCUMENTS/Publications/Bulletins/B450pdf.pdf?la=en> ;
    skos:topConceptOf glosis_proc:extractableElementsProcedure .

glosis_proc:extractableElementsProcedure-Extr_nh4-co3-2-ambic1 a glosis_proc:ExtractableElementsProcedure,
        skos:Concept ;
    skos:definition "Ambic1 method (ammonium bicarbonate) (South Africa). Particularly used for available P." ;
    skos:inScheme glosis_proc:extractableElementsProcedure ;
    skos:notation "Extr_nh4-co3-2-ambic1" ;
    skos:prefLabel "Extr_nh4-co3-2-ambic1"@en ;
    skos:scopeNote <https://www.isric.org/sites/default/files/isric_report_2014_01.pdf>,
        "Leenaars J.G.B., A.J.M. van Oostrum and M. Ruiperez Gonzalez, 2014. Africa Soil Profiles Database, Version 1.2. A compilation of georeferenced and standardised legacy soil profile data for Sub-Saharan Africa (with dataset). ISRIC Report 2014/01. Africa Soil Information Service (AfSIS) project and ISRIC - World Soil Information, Wageningen, the Netherlands. See Annex 4." ;
    skos:topConceptOf glosis_proc:extractableElementsProcedure .

glosis_proc:extractableElementsProcedure-Extr_nh4ch3ch-oh-cooh-leuven a glosis_proc:ExtractableElementsProcedure,
        skos:Concept ;
    skos:definition "NH4-lactate extraction method (KU-Leuven). Particularly used for available P." ;
    skos:inScheme glosis_proc:extractableElementsProcedure ;
    skos:notation "Extr_nh4ch3ch-oh-cooh-leuven" ;
    skos:prefLabel "Extr_nh4ch3ch-oh-cooh-leuv"@en ;
    skos:scopeNote <https://www.isric.org/sites/default/files/isric_report_2014_01.pdf>,
        "Leenaars J.G.B., A.J.M. van Oostrum and M. Ruiperez Gonzalez, 2014. Africa Soil Profiles Database, Version 1.2. A compilation of georeferenced and standardised legacy soil profile data for Sub-Saharan Africa (with dataset). ISRIC Report 2014/01. Africa Soil Information Service (AfSIS) project and ISRIC - World Soil Information, Wageningen, the Netherlands. See Annex 4." ;
    skos:topConceptOf glosis_proc:extractableElementsProcedure .

glosis_proc:gypsumProcedure-CaSO4_gy01 a glosis_proc:GypsumProcedure,
        skos:Concept ;
    skos:definition "Dissolved in water and precipitated by acetone" ;
    skos:inScheme glosis_proc:gypsumProcedure ;
    skos:notation "CaSO4_gy01" ;
    skos:prefLabel "CaSO4_gy01"@en ;
    skos:scopeNote <https://www.isric.org/sites/default/files/isric_report_2014_01.pdf>,
        "Leenaars J.G.B., A.J.M. van Oostrum and M. Ruiperez Gonzalez, 2014. Africa Soil Profiles Database, Version 1.2. A compilation of georeferenced and standardised legacy soil profile data for Sub-Saharan Africa (with dataset). ISRIC Report 2014/01. Africa Soil Information Service (AfSIS) project and ISRIC - World Soil Information, Wageningen, the Netherlands. See Annex 4." ;
    skos:topConceptOf glosis_proc:gypsumProcedure .

glosis_proc:gypsumProcedure-CaSO4_gy02 a glosis_proc:GypsumProcedure,
        skos:Concept ;
    skos:definition "Differ. between Ca-conc. in sat. extr. and Ca-conc. in 1/50 s/w solution" ;
    skos:inScheme glosis_proc:gypsumProcedure ;
    skos:notation "CaSO4_gy02" ;
    skos:prefLabel "CaSO4_gy02"@en ;
    skos:scopeNote <https://www.isric.org/sites/default/files/isric_report_2014_01.pdf>,
        "Leenaars J.G.B., A.J.M. van Oostrum and M. Ruiperez Gonzalez, 2014. Africa Soil Profiles Database, Version 1.2. A compilation of georeferenced and standardised legacy soil profile data for Sub-Saharan Africa (with dataset). ISRIC Report 2014/01. Africa Soil Information Service (AfSIS) project and ISRIC - World Soil Information, Wageningen, the Netherlands. See Annex 4." ;
    skos:topConceptOf glosis_proc:gypsumProcedure .

glosis_proc:gypsumProcedure-CaSO4_gy03 a glosis_proc:GypsumProcedure,
        skos:Concept ;
    skos:definition "Calculated from conductivity of successive dilutions" ;
    skos:inScheme glosis_proc:gypsumProcedure ;
    skos:notation "CaSO4_gy03" ;
    skos:prefLabel "CaSO4_gy03"@en ;
    skos:scopeNote <https://www.isric.org/sites/default/files/isric_report_2014_01.pdf>,
        "Leenaars J.G.B., A.J.M. van Oostrum and M. Ruiperez Gonzalez, 2014. Africa Soil Profiles Database, Version 1.2. A compilation of georeferenced and standardised legacy soil profile data for Sub-Saharan Africa (with dataset). ISRIC Report 2014/01. Africa Soil Information Service (AfSIS) project and ISRIC - World Soil Information, Wageningen, the Netherlands. See Annex 4." ;
    skos:topConceptOf glosis_proc:gypsumProcedure .

glosis_proc:gypsumProcedure-CaSO4_gy04 a glosis_proc:GypsumProcedure,
        skos:Concept ;
    skos:definition "In 0.1 M Na3-EDTA-/- turbidimetric (Begheijn, 1993)" ;
    skos:inScheme glosis_proc:gypsumProcedure ;
    skos:notation "CaSO4_gy04" ;
    skos:prefLabel "CaSO4_gy04"@en ;
    skos:scopeNote <https://www.isric.org/sites/default/files/isric_report_2014_01.pdf>,
        "Leenaars J.G.B., A.J.M. van Oostrum and M. Ruiperez Gonzalez, 2014. Africa Soil Profiles Database, Version 1.2. A compilation of georeferenced and standardised legacy soil profile data for Sub-Saharan Africa (with dataset). ISRIC Report 2014/01. Africa Soil Information Service (AfSIS) project and ISRIC - World Soil Information, Wageningen, the Netherlands. See Annex 4." ;
    skos:topConceptOf glosis_proc:gypsumProcedure .

glosis_proc:gypsumProcedure-CaSO4_gy05 a glosis_proc:GypsumProcedure,
        skos:Concept ;
    skos:definition "Gravimetric after dissolution in 0.2 N HCl (USSR-method)" ;
    skos:inScheme glosis_proc:gypsumProcedure ;
    skos:notation "CaSO4_gy05" ;
    skos:prefLabel "CaSO4_gy05"@en ;
    skos:scopeNote <https://www.isric.org/sites/default/files/isric_report_2014_01.pdf>,
        "Leenaars J.G.B., A.J.M. van Oostrum and M. Ruiperez Gonzalez, 2014. Africa Soil Profiles Database, Version 1.2. A compilation of georeferenced and standardised legacy soil profile data for Sub-Saharan Africa (with dataset). ISRIC Report 2014/01. Africa Soil Information Service (AfSIS) project and ISRIC - World Soil Information, Wageningen, the Netherlands. See Annex 4." ;
    skos:topConceptOf glosis_proc:gypsumProcedure .

glosis_proc:gypsumProcedure-CaSO4_gy06 a glosis_proc:GypsumProcedure,
        skos:Concept ;
    skos:definition "Total-S, using LECO furnace, minus easily soluble MgSO4 and Na2SO4" ;
    skos:inScheme glosis_proc:gypsumProcedure ;
    skos:notation "CaSO4_gy06" ;
    skos:prefLabel "CaSO4_gy06"@en ;
    skos:scopeNote <https://www.isric.org/sites/default/files/isric_report_2014_01.pdf>,
        "Leenaars J.G.B., A.J.M. van Oostrum and M. Ruiperez Gonzalez, 2014. Africa Soil Profiles Database, Version 1.2. A compilation of georeferenced and standardised legacy soil profile data for Sub-Saharan Africa (with dataset). ISRIC Report 2014/01. Africa Soil Information Service (AfSIS) project and ISRIC - World Soil Information, Wageningen, the Netherlands. See Annex 4." ;
    skos:topConceptOf glosis_proc:gypsumProcedure .

glosis_proc:gypsumProcedure-CaSO4_gy07 a glosis_proc:GypsumProcedure,
        skos:Concept ;
    skos:definition "Schleiff method, electrometric" ;
    skos:inScheme glosis_proc:gypsumProcedure ;
    skos:notation "CaSO4_gy07" ;
    skos:prefLabel "CaSO4_gy07"@en ;
    skos:scopeNote <https://www.isric.org/sites/default/files/isric_report_2014_01.pdf>,
        "Leenaars J.G.B., A.J.M. van Oostrum and M. Ruiperez Gonzalez, 2014. Africa Soil Profiles Database, Version 1.2. A compilation of georeferenced and standardised legacy soil profile data for Sub-Saharan Africa (with dataset). ISRIC Report 2014/01. Africa Soil Information Service (AfSIS) project and ISRIC - World Soil Information, Wageningen, the Netherlands. See Annex 4." ;
    skos:topConceptOf glosis_proc:gypsumProcedure .

glosis_proc:hydraulicConductivityProcedure-KSat_calcul-ptf a glosis_proc:HydraulicConductivityProcedure,
        skos:Concept ;
    skos:definition "Saturated hydraulic conductivity." ;
    skos:inScheme glosis_proc:hydraulicConductivityProcedure ;
    skos:notation "KSat_calcul-ptf" ;
    skos:prefLabel "KSat_calcul-ptf"@en ;
    skos:scopeNote <https://www.isric.org/sites/default/files/isric_report_2014_01.pdf>,
        "Leenaars J.G.B., A.J.M. van Oostrum and M. Ruiperez Gonzalez, 2014. Africa Soil Profiles Database, Version 1.2. A compilation of georeferenced and standardised legacy soil profile data for Sub-Saharan Africa (with dataset). ISRIC Report 2014/01. Africa Soil Information Service (AfSIS) project and ISRIC - World Soil Information, Wageningen, the Netherlands. See Annex 4." ;
    skos:topConceptOf glosis_proc:hydraulicConductivityProcedure .

glosis_proc:hydraulicConductivityProcedure-KSat_calcul-ptf-genuchten a glosis_proc:HydraulicConductivityProcedure,
        skos:Concept ;
    skos:definition "Saturated and not saturated hydraulic conductivity." ;
    skos:inScheme glosis_proc:hydraulicConductivityProcedure ;
    skos:notation "KSat_calcul-ptf-genuchten" ;
    skos:prefLabel "KSat_calcul-ptf-genucht"@en ;
    skos:scopeNote <https://www.isric.org/sites/default/files/isric_report_2014_01.pdf>,
        "Leenaars J.G.B., A.J.M. van Oostrum and M. Ruiperez Gonzalez, 2014. Africa Soil Profiles Database, Version 1.2. A compilation of georeferenced and standardised legacy soil profile data for Sub-Saharan Africa (with dataset). ISRIC Report 2014/01. Africa Soil Information Service (AfSIS) project and ISRIC - World Soil Information, Wageningen, the Netherlands. See Annex 4." ;
    skos:topConceptOf glosis_proc:hydraulicConductivityProcedure .

glosis_proc:hydraulicConductivityProcedure-KSat_calcul-ptf-saxton a glosis_proc:HydraulicConductivityProcedure,
        skos:Concept ;
    skos:definition "Saturated hydraulic conductivity." ;
    skos:inScheme glosis_proc:hydraulicConductivityProcedure ;
    skos:notation "KSat_calcul-ptf-saxton" ;
    skos:prefLabel "KSat_calcul-ptf-saxto"@en ;
    skos:scopeNote <https://www.isric.org/sites/default/files/isric_report_2014_01.pdf>,
        "Leenaars J.G.B., A.J.M. van Oostrum and M. Ruiperez Gonzalez, 2014. Africa Soil Profiles Database, Version 1.2. A compilation of georeferenced and standardised legacy soil profile data for Sub-Saharan Africa (with dataset). ISRIC Report 2014/01. Africa Soil Information Service (AfSIS) project and ISRIC - World Soil Information, Wageningen, the Netherlands. See Annex 4." ;
    skos:topConceptOf glosis_proc:hydraulicConductivityProcedure .

glosis_proc:hydraulicConductivityProcedure-Ksat_bhole a glosis_proc:HydraulicConductivityProcedure,
        skos:Concept ;
    skos:definition "Saturated hydraulic conductivity. Bore hole method" ;
    skos:inScheme glosis_proc:hydraulicConductivityProcedure ;
    skos:notation "Ksat_bhole" ;
    skos:prefLabel "Ksat_bhol"@en ;
    skos:scopeNote <https://www.isric.org/sites/default/files/isric_report_2014_01.pdf>,
        "Leenaars J.G.B., A.J.M. van Oostrum and M. Ruiperez Gonzalez, 2014. Africa Soil Profiles Database, Version 1.2. A compilation of georeferenced and standardised legacy soil profile data for Sub-Saharan Africa (with dataset). ISRIC Report 2014/01. Africa Soil Information Service (AfSIS) project and ISRIC - World Soil Information, Wageningen, the Netherlands. See Annex 4." ;
    skos:topConceptOf glosis_proc:hydraulicConductivityProcedure .

glosis_proc:hydraulicConductivityProcedure-Ksat_column a glosis_proc:HydraulicConductivityProcedure,
        skos:Concept ;
    skos:definition "Saturated hydraulic conductivity. Permeability in cm/hr determined in column filled with fine earth fraction" ;
    skos:inScheme glosis_proc:hydraulicConductivityProcedure ;
    skos:notation "Ksat_column" ;
    skos:prefLabel "Ksat_colum"@en ;
    skos:scopeNote <https://www.isric.org/sites/default/files/isric_report_2014_01.pdf>,
        "Leenaars J.G.B., A.J.M. van Oostrum and M. Ruiperez Gonzalez, 2014. Africa Soil Profiles Database, Version 1.2. A compilation of georeferenced and standardised legacy soil profile data for Sub-Saharan Africa (with dataset). ISRIC Report 2014/01. Africa Soil Information Service (AfSIS) project and ISRIC - World Soil Information, Wageningen, the Netherlands. See Annex 4." ;
    skos:topConceptOf glosis_proc:hydraulicConductivityProcedure .

glosis_proc:hydraulicConductivityProcedure-Ksat_dblring a glosis_proc:HydraulicConductivityProcedure,
        skos:Concept ;
    skos:definition "Saturated hydraulic conductivity. Double ring method" ;
    skos:inScheme glosis_proc:hydraulicConductivityProcedure ;
    skos:notation "Ksat_dblring" ;
    skos:prefLabel "Ksat_dblring"@en ;
    skos:scopeNote <https://www.isric.org/sites/default/files/isric_report_2014_01.pdf>,
        "Leenaars J.G.B., A.J.M. van Oostrum and M. Ruiperez Gonzalez, 2014. Africa Soil Profiles Database, Version 1.2. A compilation of georeferenced and standardised legacy soil profile data for Sub-Saharan Africa (with dataset). ISRIC Report 2014/01. Africa Soil Information Service (AfSIS) project and ISRIC - World Soil Information, Wageningen, the Netherlands. See Annex 4." ;
    skos:topConceptOf glosis_proc:hydraulicConductivityProcedure .

glosis_proc:hydraulicConductivityProcedure-Ksat_invbhole a glosis_proc:HydraulicConductivityProcedure,
        skos:Concept ;
    skos:definition "Saturated hydraulic conductivity. Inverse bore hole method" ;
    skos:inScheme glosis_proc:hydraulicConductivityProcedure ;
    skos:notation "Ksat_invbhole" ;
    skos:prefLabel "Ksat_invbhol"@en ;
    skos:scopeNote <https://www.isric.org/sites/default/files/isric_report_2014_01.pdf>,
        "Leenaars J.G.B., A.J.M. van Oostrum and M. Ruiperez Gonzalez, 2014. Africa Soil Profiles Database, Version 1.2. A compilation of georeferenced and standardised legacy soil profile data for Sub-Saharan Africa (with dataset). ISRIC Report 2014/01. Africa Soil Information Service (AfSIS) project and ISRIC - World Soil Information, Wageningen, the Netherlands. See Annex 4." ;
    skos:topConceptOf glosis_proc:hydraulicConductivityProcedure .

glosis_proc:moistureContentProcedure-VMC_calcul-ptf a glosis_proc:MoistureContentProcedure,
        skos:Concept ;
    skos:definition "Calculated by PTF" ;
    skos:inScheme glosis_proc:moistureContentProcedure ;
    skos:notation "VMC_calcul-ptf" ;
    skos:prefLabel "VMC_calcul-ptf"@en ;
    skos:scopeNote <https://www.isric.org/sites/default/files/isric_report_2014_01.pdf>,
        "Leenaars J.G.B., A.J.M. van Oostrum and M. Ruiperez Gonzalez, 2014. Africa Soil Profiles Database, Version 1.2. A compilation of georeferenced and standardised legacy soil profile data for Sub-Saharan Africa (with dataset). ISRIC Report 2014/01. Africa Soil Information Service (AfSIS) project and ISRIC - World Soil Information, Wageningen, the Netherlands. See Annex 4." ;
    skos:topConceptOf glosis_proc:moistureContentProcedure .

glosis_proc:moistureContentProcedure-VMC_calcul-ptf-brookscorey a glosis_proc:MoistureContentProcedure,
        skos:Concept ;
    skos:definition "Calculated by PTF of brooks - corey" ;
    skos:inScheme glosis_proc:moistureContentProcedure ;
    skos:notation "VMC_calcul-ptf-brookscorey" ;
    skos:prefLabel "VMC_calcul-ptf-brookscorey"@en ;
    skos:scopeNote <https://www.isric.org/sites/default/files/isric_report_2014_01.pdf>,
        "Leenaars J.G.B., A.J.M. van Oostrum and M. Ruiperez Gonzalez, 2014. Africa Soil Profiles Database, Version 1.2. A compilation of georeferenced and standardised legacy soil profile data for Sub-Saharan Africa (with dataset). ISRIC Report 2014/01. Africa Soil Information Service (AfSIS) project and ISRIC - World Soil Information, Wageningen, the Netherlands. See Annex 4." ;
    skos:topConceptOf glosis_proc:moistureContentProcedure .

glosis_proc:moistureContentProcedure-VMC_d a glosis_proc:MoistureContentProcedure,
        skos:Concept ;
    skos:definition "Volumetric moisture content in disturbed samples" ;
    skos:inScheme glosis_proc:moistureContentProcedure ;
    skos:notation "VMC_d" ;
    skos:prefLabel "VMC_d"@en ;
    skos:scopeNote <https://www.isric.org/sites/default/files/isric_report_2014_01.pdf>,
        "Leenaars J.G.B., A.J.M. van Oostrum and M. Ruiperez Gonzalez, 2014. Africa Soil Profiles Database, Version 1.2. A compilation of georeferenced and standardised legacy soil profile data for Sub-Saharan Africa (with dataset). ISRIC Report 2014/01. Africa Soil Information Service (AfSIS) project and ISRIC - World Soil Information, Wageningen, the Netherlands. See Annex 4." ;
    skos:topConceptOf glosis_proc:moistureContentProcedure .

glosis_proc:moistureContentProcedure-VMC_d-cl a glosis_proc:MoistureContentProcedure,
        skos:Concept ;
    skos:definition "Pressure-plate extraction, disturbed -clod- samples (wt%) * density" ;
    skos:inScheme glosis_proc:moistureContentProcedure ;
    skos:notation "VMC_d-cl" ;
    skos:prefLabel "VMC_d-cl"@en ;
    skos:scopeNote <https://www.isric.org/sites/default/files/isric_report_2014_01.pdf>,
        "Leenaars J.G.B., A.J.M. van Oostrum and M. Ruiperez Gonzalez, 2014. Africa Soil Profiles Database, Version 1.2. A compilation of georeferenced and standardised legacy soil profile data for Sub-Saharan Africa (with dataset). ISRIC Report 2014/01. Africa Soil Information Service (AfSIS) project and ISRIC - World Soil Information, Wageningen, the Netherlands. See Annex 4." ;
    skos:topConceptOf glosis_proc:moistureContentProcedure .

glosis_proc:moistureContentProcedure-VMC_d-cl-ww a glosis_proc:MoistureContentProcedure,
        skos:Concept ;
    skos:definition "Pressure-plate extraction, disturbed -clod- samples (wt%) * density on weight/weight basis; to be converted to v/v (with BD at appropriate humidity)" ;
    skos:inScheme glosis_proc:moistureContentProcedure ;
    skos:notation "VMC_d-cl-ww" ;
    skos:prefLabel "VMC_d-cl-ww"@en ;
    skos:scopeNote <https://www.isric.org/sites/default/files/isric_report_2014_01.pdf>,
        "Leenaars J.G.B., A.J.M. van Oostrum and M. Ruiperez Gonzalez, 2014. Africa Soil Profiles Database, Version 1.2. A compilation of georeferenced and standardised legacy soil profile data for Sub-Saharan Africa (with dataset). ISRIC Report 2014/01. Africa Soil Information Service (AfSIS) project and ISRIC - World Soil Information, Wageningen, the Netherlands. See Annex 4." ;
    skos:topConceptOf glosis_proc:moistureContentProcedure .

glosis_proc:moistureContentProcedure-VMC_d-ww a glosis_proc:MoistureContentProcedure,
        skos:Concept ;
    skos:definition "Volumetric moisture content in disturbed samples on weight/weight basis to be converted to v/v (with BD at appropriate humidity)" ;
    skos:inScheme glosis_proc:moistureContentProcedure ;
    skos:notation "VMC_d-ww" ;
    skos:prefLabel "VMC_d-ww"@en ;
    skos:scopeNote <https://www.isric.org/sites/default/files/isric_report_2014_01.pdf>,
        "Leenaars J.G.B., A.J.M. van Oostrum and M. Ruiperez Gonzalez, 2014. Africa Soil Profiles Database, Version 1.2. A compilation of georeferenced and standardised legacy soil profile data for Sub-Saharan Africa (with dataset). ISRIC Report 2014/01. Africa Soil Information Service (AfSIS) project and ISRIC - World Soil Information, Wageningen, the Netherlands. See Annex 4." ;
    skos:topConceptOf glosis_proc:moistureContentProcedure .

glosis_proc:moistureContentProcedure-VMC_ud a glosis_proc:MoistureContentProcedure,
        skos:Concept ;
    skos:definition "Undisturbed samples" ;
    skos:inScheme glosis_proc:moistureContentProcedure ;
    skos:notation "VMC_ud" ;
    skos:prefLabel "VMC_ud"@en ;
    skos:scopeNote <https://www.isric.org/sites/default/files/isric_report_2014_01.pdf>,
        "Leenaars J.G.B., A.J.M. van Oostrum and M. Ruiperez Gonzalez, 2014. Africa Soil Profiles Database, Version 1.2. A compilation of georeferenced and standardised legacy soil profile data for Sub-Saharan Africa (with dataset). ISRIC Report 2014/01. Africa Soil Information Service (AfSIS) project and ISRIC - World Soil Information, Wageningen, the Netherlands. See Annex 4." ;
    skos:topConceptOf glosis_proc:moistureContentProcedure .

glosis_proc:moistureContentProcedure-VMC_ud-cl a glosis_proc:MoistureContentProcedure,
        skos:Concept ;
    skos:definition "Natural clod" ;
    skos:inScheme glosis_proc:moistureContentProcedure ;
    skos:notation "VMC_ud-cl" ;
    skos:prefLabel "VMC_ud-cl"@en ;
    skos:scopeNote <https://www.isric.org/sites/default/files/isric_report_2014_01.pdf>,
        "Leenaars J.G.B., A.J.M. van Oostrum and M. Ruiperez Gonzalez, 2014. Africa Soil Profiles Database, Version 1.2. A compilation of georeferenced and standardised legacy soil profile data for Sub-Saharan Africa (with dataset). ISRIC Report 2014/01. Africa Soil Information Service (AfSIS) project and ISRIC - World Soil Information, Wageningen, the Netherlands. See Annex 4." ;
    skos:topConceptOf glosis_proc:moistureContentProcedure .

glosis_proc:moistureContentProcedure-VMC_ud-co a glosis_proc:MoistureContentProcedure,
        skos:Concept ;
    skos:definition "Volumetric moisture content in undisturbed samples (pF rings cores)" ;
    skos:inScheme glosis_proc:moistureContentProcedure ;
    skos:notation "VMC_ud-co" ;
    skos:prefLabel "VMC_ud-co"@en ;
    skos:scopeNote <https://www.isric.org/sites/default/files/isric_report_2014_01.pdf>,
        "Leenaars J.G.B., A.J.M. van Oostrum and M. Ruiperez Gonzalez, 2014. Africa Soil Profiles Database, Version 1.2. A compilation of georeferenced and standardised legacy soil profile data for Sub-Saharan Africa (with dataset). ISRIC Report 2014/01. Africa Soil Information Service (AfSIS) project and ISRIC - World Soil Information, Wageningen, the Netherlands. See Annex 4." ;
    skos:topConceptOf glosis_proc:moistureContentProcedure .

glosis_proc:nitrogenTotalProcedure-TotalN_bremner a glosis_proc:NitrogenTotalProcedure,
        skos:Concept ;
    skos:definition "Total N (Bremner, 1965, p. 1162-1164)" ;
    skos:inScheme glosis_proc:nitrogenTotalProcedure ;
    skos:notation "TotalN_bremner" ;
    skos:prefLabel "TotalN_bremner"@en ;
    skos:scopeNote <https://doi.org/10.2134/agronmonogr9.2.c32>,
        "Bremner, J. M. 1965. Total Nitrogen. In: C. A. Black (ed.) Methods of soil analysis. Part 2: Chemical and microbial properties. Number 9 in series Agronomy. American Society of Agronomy, Inc. Publisher, Madison, USA. Pp. 1049-1178" ;
    skos:topConceptOf glosis_proc:nitrogenTotalProcedure .

glosis_proc:nitrogenTotalProcedure-TotalN_calcul a glosis_proc:NitrogenTotalProcedure,
        skos:Concept ;
    skos:definition "OC * 1.72 / 20 (gives C/N=11.6009)" ;
    skos:inScheme glosis_proc:nitrogenTotalProcedure ;
    skos:notation "TotalN_calcul" ;
    skos:prefLabel "TotalN_calcul"@en ;
    skos:scopeNote <https://www.isric.org/sites/default/files/isric_report_2014_01.pdf>,
        "Leenaars J.G.B., A.J.M. van Oostrum and M. Ruiperez Gonzalez, 2014. Africa Soil Profiles Database, Version 1.2. A compilation of georeferenced and standardised legacy soil profile data for Sub-Saharan Africa (with dataset). ISRIC Report 2014/01. Africa Soil Information Service (AfSIS) project and ISRIC - World Soil Information, Wageningen, the Netherlands. See Annex 4." ;
    skos:topConceptOf glosis_proc:nitrogenTotalProcedure .

glosis_proc:nitrogenTotalProcedure-TotalN_calcul-oc10 a glosis_proc:NitrogenTotalProcedure,
        skos:Concept ;
    skos:definition "Calculated from OrgC and C/N ratio of 10" ;
    skos:inScheme glosis_proc:nitrogenTotalProcedure ;
    skos:notation "TotalN_calcul-oc10" ;
    skos:prefLabel "TotalN_calcul-oc10"@en ;
    skos:scopeNote <https://www.isric.org/sites/default/files/isric_report_2014_01.pdf>,
        "Leenaars J.G.B., A.J.M. van Oostrum and M. Ruiperez Gonzalez, 2014. Africa Soil Profiles Database, Version 1.2. A compilation of georeferenced and standardised legacy soil profile data for Sub-Saharan Africa (with dataset). ISRIC Report 2014/01. Africa Soil Information Service (AfSIS) project and ISRIC - World Soil Information, Wageningen, the Netherlands. See Annex 4." ;
    skos:topConceptOf glosis_proc:nitrogenTotalProcedure .

glosis_proc:nitrogenTotalProcedure-TotalN_dc a glosis_proc:NitrogenTotalProcedure,
        skos:Concept ;
    skos:definition "Dry combustion" ;
    skos:inScheme glosis_proc:nitrogenTotalProcedure ;
    skos:narrower glosis_proc:nitrogenTotalProcedure-TotalN_dc-ht-dumas,
        glosis_proc:nitrogenTotalProcedure-TotalN_dc-ht-leco,
        glosis_proc:nitrogenTotalProcedure-TotalN_dc-spec ;
    skos:notation "TotalN_dc" ;
    skos:prefLabel "TotalN_dc"@en ;
    skos:scopeNote <https://www.isric.org/sites/default/files/isric_report_2014_01.pdf>,
        "Leenaars J.G.B., A.J.M. van Oostrum and M. Ruiperez Gonzalez, 2014. Africa Soil Profiles Database, Version 1.2. A compilation of georeferenced and standardised legacy soil profile data for Sub-Saharan Africa (with dataset). ISRIC Report 2014/01. Africa Soil Information Service (AfSIS) project and ISRIC - World Soil Information, Wageningen, the Netherlands. See Annex 4." ;
    skos:topConceptOf glosis_proc:nitrogenTotalProcedure .

glosis_proc:nitrogenTotalProcedure-TotalN_dc-ht-dumas a glosis_proc:NitrogenTotalProcedure,
        skos:Concept ;
    skos:broader glosis_proc:nitrogenTotalProcedure-TotalN_dc ;
    skos:definition "Dry combustion at 800-1000 C celcius (Dumas method)" ;
    skos:inScheme glosis_proc:nitrogenTotalProcedure ;
    skos:notation "TotalN_dc-ht-dumas" ;
    skos:prefLabel "TotalN_dc-ht-dumas"@en ;
    skos:scopeNote <https://www.isric.org/sites/default/files/isric_report_2014_01.pdf>,
        "Leenaars J.G.B., A.J.M. van Oostrum and M. Ruiperez Gonzalez, 2014. Africa Soil Profiles Database, Version 1.2. A compilation of georeferenced and standardised legacy soil profile data for Sub-Saharan Africa (with dataset). ISRIC Report 2014/01. Africa Soil Information Service (AfSIS) project and ISRIC - World Soil Information, Wageningen, the Netherlands. See Annex 4." .

glosis_proc:nitrogenTotalProcedure-TotalN_dc-ht-leco a glosis_proc:NitrogenTotalProcedure,
        skos:Concept ;
    skos:broader glosis_proc:nitrogenTotalProcedure-TotalN_dc ;
    skos:definition "Element analyzer (LECO analyzer), Dry Combustion" ;
    skos:inScheme glosis_proc:nitrogenTotalProcedure ;
    skos:notation "TotalN_dc-ht-leco" ;
    skos:prefLabel "TotalN_dc-ht-leco"@en ;
    skos:scopeNote <https://www.isric.org/sites/default/files/isric_report_2014_01.pdf>,
        "Leenaars J.G.B., A.J.M. van Oostrum and M. Ruiperez Gonzalez, 2014. Africa Soil Profiles Database, Version 1.2. A compilation of georeferenced and standardised legacy soil profile data for Sub-Saharan Africa (with dataset). ISRIC Report 2014/01. Africa Soil Information Service (AfSIS) project and ISRIC - World Soil Information, Wageningen, the Netherlands. See Annex 4." .

glosis_proc:nitrogenTotalProcedure-TotalN_dc-spec a glosis_proc:NitrogenTotalProcedure,
        skos:Concept ;
    skos:broader glosis_proc:nitrogenTotalProcedure-TotalN_dc ;
    skos:definition "Spectrally measured and converted to N by dry combustion" ;
    skos:inScheme glosis_proc:nitrogenTotalProcedure ;
    skos:notation "TotalN_dc-spec" ;
    skos:prefLabel "TotalN_dc-spec"@en ;
    skos:scopeNote <https://www.isric.org/sites/default/files/isric_report_2014_01.pdf>,
        "Leenaars J.G.B., A.J.M. van Oostrum and M. Ruiperez Gonzalez, 2014. Africa Soil Profiles Database, Version 1.2. A compilation of georeferenced and standardised legacy soil profile data for Sub-Saharan Africa (with dataset). ISRIC Report 2014/01. Africa Soil Information Service (AfSIS) project and ISRIC - World Soil Information, Wageningen, the Netherlands. See Annex 4." .

glosis_proc:nitrogenTotalProcedure-TotalN_h2so4 a glosis_proc:NitrogenTotalProcedure,
        skos:Concept ;
    skos:definition "H2SO4" ;
    skos:inScheme glosis_proc:nitrogenTotalProcedure ;
    skos:notation "TotalN_h2so4" ;
    skos:prefLabel "TotalN_h2so4"@en ;
    skos:topConceptOf glosis_proc:nitrogenTotalProcedure .

glosis_proc:nitrogenTotalProcedure-TotalN_kjeldahl a glosis_proc:NitrogenTotalProcedure,
        skos:Concept ;
    skos:definition "Method of Kjeldahl (digestion)" ;
    skos:inScheme glosis_proc:nitrogenTotalProcedure ;
    skos:notation "TotalN_kjeldahl" ;
    skos:prefLabel "TotalN_kjeldahl"@en ;
    skos:scopeNote <https://en.wikipedia.org/wiki/Kjeldahl_method>,
        "Kjeldahl, J. (1883) ‘Neue Methode zur Bestimmung des Stickstoffs in organischen Körpern’ (New method for the determination of nitrogen in organic substances), Zeitschrift für analytische Chemie, 22 (1) : 366-383." ;
    skos:topConceptOf glosis_proc:nitrogenTotalProcedure .

glosis_proc:nitrogenTotalProcedure-TotalN_kjeldahl-nh4 a glosis_proc:NitrogenTotalProcedure,
        skos:Concept ;
    skos:definition "Kjeldahl, and ammonia distillation" ;
    skos:inScheme glosis_proc:nitrogenTotalProcedure ;
    skos:notation "TotalN_kjeldahl-nh4" ;
    skos:prefLabel "TotalN_kjeldahl-nh4"@en ;
    skos:scopeNote <https://www.isric.org/sites/default/files/isric_report_2014_01.pdf>,
        "Leenaars J.G.B., A.J.M. van Oostrum and M. Ruiperez Gonzalez, 2014. Africa Soil Profiles Database, Version 1.2. A compilation of georeferenced and standardised legacy soil profile data for Sub-Saharan Africa (with dataset). ISRIC Report 2014/01. Africa Soil Information Service (AfSIS) project and ISRIC - World Soil Information, Wageningen, the Netherlands. See Annex 4." ;
    skos:topConceptOf glosis_proc:nitrogenTotalProcedure .

glosis_proc:nitrogenTotalProcedure-TotalN_nelson a glosis_proc:NitrogenTotalProcedure,
        skos:Concept ;
    skos:definition "Nelson and Sommers, 1980" ;
    skos:inScheme glosis_proc:nitrogenTotalProcedure ;
    skos:notation "TotalN_nelson" ;
    skos:prefLabel "TotalN_nelso"@en ;
    skos:scopeNote <https://doi.org/10.1093/jaoac/63.4.770>,
        "Darrell W Nelson, Lee E Sommers, Total Nitrogen Analysis of Soil and Plant Tissues, Journal of Association of Official Analytical Chemists, Volume 63, Issue 4, 1 July 1980, Pages 770–778," ;
    skos:topConceptOf glosis_proc:nitrogenTotalProcedure .

glosis_proc:nitrogenTotalProcedure-TotalN_tn04 a glosis_proc:NitrogenTotalProcedure,
        skos:Concept ;
    skos:definition "Dry combustion using a CN-corder and cobalt oxide or copper oxide as an oxidation accelerator (Tanabe and Araragi, 1970)" ;
    skos:inScheme glosis_proc:nitrogenTotalProcedure ;
    skos:notation "TotalN_tn04" ;
    skos:prefLabel "TotalN_tn04"@en ;
    skos:scopeNote <https://www.isric.org/sites/default/files/isric_report_2014_01.pdf>,
        "Leenaars J.G.B., A.J.M. van Oostrum and M. Ruiperez Gonzalez, 2014. Africa Soil Profiles Database, Version 1.2. A compilation of georeferenced and standardised legacy soil profile data for Sub-Saharan Africa (with dataset). ISRIC Report 2014/01. Africa Soil Information Service (AfSIS) project and ISRIC - World Soil Information, Wageningen, the Netherlands. See Annex 4." ;
    skos:topConceptOf glosis_proc:nitrogenTotalProcedure .

glosis_proc:nitrogenTotalProcedure-TotalN_tn06 a glosis_proc:NitrogenTotalProcedure,
        skos:Concept ;
    skos:definition "Continuous flow analyser after digestion with H2SO4/salicyclic acid/H2O2/Se" ;
    skos:inScheme glosis_proc:nitrogenTotalProcedure ;
    skos:notation "TotalN_tn06" ;
    skos:prefLabel "TotalN_tn06"@en ;
    skos:scopeNote <https://www.isric.org/sites/default/files/isric_report_2014_01.pdf>,
        "Leenaars J.G.B., A.J.M. van Oostrum and M. Ruiperez Gonzalez, 2014. Africa Soil Profiles Database, Version 1.2. A compilation of georeferenced and standardised legacy soil profile data for Sub-Saharan Africa (with dataset). ISRIC Report 2014/01. Africa Soil Information Service (AfSIS) project and ISRIC - World Soil Information, Wageningen, the Netherlands. See Annex 4." ;
    skos:topConceptOf glosis_proc:nitrogenTotalProcedure .

glosis_proc:nitrogenTotalProcedure-TotalN_tn08 a glosis_proc:NitrogenTotalProcedure,
        skos:Concept ;
    skos:definition "Sample digested by sulphuric acid, distillation of released ammonia, back titration against sulpuric acid" ;
    skos:inScheme glosis_proc:nitrogenTotalProcedure ;
    skos:notation "TotalN_tn08" ;
    skos:prefLabel "TotalN_tn08"@en ;
    skos:scopeNote <https://www.isric.org/sites/default/files/isric_report_2014_01.pdf>,
        "Leenaars J.G.B., A.J.M. van Oostrum and M. Ruiperez Gonzalez, 2014. Africa Soil Profiles Database, Version 1.2. A compilation of georeferenced and standardised legacy soil profile data for Sub-Saharan Africa (with dataset). ISRIC Report 2014/01. Africa Soil Information Service (AfSIS) project and ISRIC - World Soil Information, Wageningen, the Netherlands. See Annex 4." ;
    skos:topConceptOf glosis_proc:nitrogenTotalProcedure .

glosis_proc:organicMatterProcedure-FulAcidC_unkn a glosis_proc:OrganicMatterProcedure,
        skos:Concept ;
    skos:definition "Fulvic acid carbon_unknown method" ;
    skos:inScheme glosis_proc:organicMatterProcedure ;
    skos:notation "FulAcidC_unkn" ;
    skos:prefLabel "FulAcidC_unk"@en ;
    skos:scopeNote <https://www.isric.org/sites/default/files/isric_report_2014_01.pdf>,
        "Leenaars J.G.B., A.J.M. van Oostrum and M. Ruiperez Gonzalez, 2014. Africa Soil Profiles Database, Version 1.2. A compilation of georeferenced and standardised legacy soil profile data for Sub-Saharan Africa (with dataset). ISRIC Report 2014/01. Africa Soil Information Service (AfSIS) project and ISRIC - World Soil Information, Wageningen, the Netherlands. See Annex 4." ;
    skos:topConceptOf glosis_proc:organicMatterProcedure .

glosis_proc:organicMatterProcedure-HumAcidC_unkn a glosis_proc:OrganicMatterProcedure,
        skos:Concept ;
    skos:definition "Humic acid carbon_unknown method" ;
    skos:inScheme glosis_proc:organicMatterProcedure ;
    skos:notation "HumAcidC_unkn" ;
    skos:prefLabel "HumAcidC_unk"@en ;
    skos:scopeNote <https://www.isric.org/sites/default/files/isric_report_2014_01.pdf>,
        "Leenaars J.G.B., A.J.M. van Oostrum and M. Ruiperez Gonzalez, 2014. Africa Soil Profiles Database, Version 1.2. A compilation of georeferenced and standardised legacy soil profile data for Sub-Saharan Africa (with dataset). ISRIC Report 2014/01. Africa Soil Information Service (AfSIS) project and ISRIC - World Soil Information, Wageningen, the Netherlands. See Annex 4." ;
    skos:topConceptOf glosis_proc:organicMatterProcedure .

glosis_proc:organicMatterProcedure-OrgM_calcul-oc1.73 a glosis_proc:OrganicMatterProcedure,
        skos:Concept ;
    skos:definition "Organic carbon * 1,73" ;
    skos:inScheme glosis_proc:organicMatterProcedure ;
    skos:notation "OrgM_calcul-oc1.73" ;
    skos:prefLabel "OrgM_calcul-oc1.73"@en ;
    skos:scopeNote <https://www.isric.org/sites/default/files/isric_report_2014_01.pdf>,
        "Leenaars J.G.B., A.J.M. van Oostrum and M. Ruiperez Gonzalez, 2014. Africa Soil Profiles Database, Version 1.2. A compilation of georeferenced and standardised legacy soil profile data for Sub-Saharan Africa (with dataset). ISRIC Report 2014/01. Africa Soil Information Service (AfSIS) project and ISRIC - World Soil Information, Wageningen, the Netherlands. See Annex 4." ;
    skos:topConceptOf glosis_proc:organicMatterProcedure .

glosis_proc:organicMatterProcedure-TotHumC_unkn a glosis_proc:OrganicMatterProcedure,
        skos:Concept ;
    skos:definition "Total humic carbon_unknown method" ;
    skos:inScheme glosis_proc:organicMatterProcedure ;
    skos:notation "TotHumC_unkn" ;
    skos:prefLabel "TotHumC_unk"@en ;
    skos:scopeNote <https://www.isric.org/sites/default/files/isric_report_2014_01.pdf>,
        "Leenaars J.G.B., A.J.M. van Oostrum and M. Ruiperez Gonzalez, 2014. Africa Soil Profiles Database, Version 1.2. A compilation of georeferenced and standardised legacy soil profile data for Sub-Saharan Africa (with dataset). ISRIC Report 2014/01. Africa Soil Information Service (AfSIS) project and ISRIC - World Soil Information, Wageningen, the Netherlands. See Annex 4." ;
    skos:topConceptOf glosis_proc:organicMatterProcedure .

glosis_proc:pHProcedure-pHCaCl2 a glosis_proc:PHProcedure,
        skos:Concept ;
    skos:definition "pHCaCl2 (soil reaction) in a soil/CaCl2 solution (0.01-1 M)" ;
    skos:inScheme glosis_proc:pHProcedure ;
    skos:narrower glosis_proc:pHProcedure-pHCaCl2_ratio1-1,
        glosis_proc:pHProcedure-pHCaCl2_ratio1-10,
        glosis_proc:pHProcedure-pHCaCl2_ratio1-2,
        glosis_proc:pHProcedure-pHCaCl2_ratio1-2.5,
        glosis_proc:pHProcedure-pHCaCl2_ratio1-5,
        glosis_proc:pHProcedure-pHCaCl2_sat ;
    skos:notation "pHCaCl2" ;
    skos:prefLabel "pHCaCl2"@en ;
    skos:scopeNote <https://www.isric.org/sites/default/files/isric_report_2014_01.pdf>,
        "Leenaars J.G.B., A.J.M. van Oostrum and M. Ruiperez Gonzalez, 2014. Africa Soil Profiles Database, Version 1.2. A compilation of georeferenced and standardised legacy soil profile data for Sub-Saharan Africa (with dataset). ISRIC Report 2014/01. Africa Soil Information Service (AfSIS) project and ISRIC - World Soil Information, Wageningen, the Netherlands. See Annex 4." ;
    skos:topConceptOf glosis_proc:pHProcedure .

glosis_proc:pHProcedure-pHCaCl2_ratio1-1 a glosis_proc:PHProcedure,
        skos:Concept ;
    skos:broader glosis_proc:pHProcedure-pHCaCl2 ;
    skos:definition "pHCaCl2 (soil reaction) in 1:1 soil/1 M CaCl2 solution (1 M)" ;
    skos:inScheme glosis_proc:pHProcedure ;
    skos:notation "pHCaCl2_ratio1-1" ;
    skos:prefLabel "pHCaCl2_ratio1-1"@en ;
    skos:scopeNote <https://www.isric.org/sites/default/files/isric_report_2014_01.pdf>,
        "Leenaars J.G.B., A.J.M. van Oostrum and M. Ruiperez Gonzalez, 2014. Africa Soil Profiles Database, Version 1.2. A compilation of georeferenced and standardised legacy soil profile data for Sub-Saharan Africa (with dataset). ISRIC Report 2014/01. Africa Soil Information Service (AfSIS) project and ISRIC - World Soil Information, Wageningen, the Netherlands. See Annex 4." .

glosis_proc:pHProcedure-pHCaCl2_ratio1-10 a glosis_proc:PHProcedure,
        skos:Concept ;
    skos:broader glosis_proc:pHProcedure-pHCaCl2 ;
    skos:definition "pHCaCl2 (soil reaction) in 1:10 soil/CaCl2 solution (0.01-1 M)" ;
    skos:inScheme glosis_proc:pHProcedure ;
    skos:notation "pHCaCl2_ratio1-10" ;
    skos:prefLabel "pHCaCl2_ratio1-10"@en ;
    skos:scopeNote <https://www.isric.org/sites/default/files/isric_report_2014_01.pdf>,
        "Leenaars J.G.B., A.J.M. van Oostrum and M. Ruiperez Gonzalez, 2014. Africa Soil Profiles Database, Version 1.2. A compilation of georeferenced and standardised legacy soil profile data for Sub-Saharan Africa (with dataset). ISRIC Report 2014/01. Africa Soil Information Service (AfSIS) project and ISRIC - World Soil Information, Wageningen, the Netherlands. See Annex 4." .

glosis_proc:pHProcedure-pHCaCl2_ratio1-2 a glosis_proc:PHProcedure,
        skos:Concept ;
    skos:broader glosis_proc:pHProcedure-pHCaCl2 ;
    skos:definition "pHCaCl2 (soil reaction) in 1:2 soil/CaCl2 solution (0.01-1 M)" ;
    skos:inScheme glosis_proc:pHProcedure ;
    skos:notation "pHCaCl2_ratio1-2" ;
    skos:prefLabel "pHCaCl2_ratio1-2"@en ;
    skos:scopeNote <https://www.isric.org/sites/default/files/isric_report_2014_01.pdf>,
        "Leenaars J.G.B., A.J.M. van Oostrum and M. Ruiperez Gonzalez, 2014. Africa Soil Profiles Database, Version 1.2. A compilation of georeferenced and standardised legacy soil profile data for Sub-Saharan Africa (with dataset). ISRIC Report 2014/01. Africa Soil Information Service (AfSIS) project and ISRIC - World Soil Information, Wageningen, the Netherlands. See Annex 4." .

glosis_proc:pHProcedure-pHCaCl2_ratio1-2.5 a glosis_proc:PHProcedure,
        skos:Concept ;
    skos:broader glosis_proc:pHProcedure-pHCaCl2 ;
    skos:definition "pHCaCl2 (soil reaction) in 1:2.5 soil/CaCl2 solution (0.01-1 M)" ;
    skos:inScheme glosis_proc:pHProcedure ;
    skos:notation "pHCaCl2_ratio1-2.5" ;
    skos:prefLabel "pHCaCl2_ratio1-2.5"@en ;
    skos:scopeNote <https://www.isric.org/sites/default/files/isric_report_2014_01.pdf>,
        "Leenaars J.G.B., A.J.M. van Oostrum and M. Ruiperez Gonzalez, 2014. Africa Soil Profiles Database, Version 1.2. A compilation of georeferenced and standardised legacy soil profile data for Sub-Saharan Africa (with dataset). ISRIC Report 2014/01. Africa Soil Information Service (AfSIS) project and ISRIC - World Soil Information, Wageningen, the Netherlands. See Annex 4." .

glosis_proc:pHProcedure-pHCaCl2_ratio1-5 a glosis_proc:PHProcedure,
        skos:Concept ;
    skos:broader glosis_proc:pHProcedure-pHCaCl2 ;
    skos:definition "pHCaCl2 (soil reaction) in 1:5 soil/CaCl2 solution (0.01-1 M)" ;
    skos:inScheme glosis_proc:pHProcedure ;
    skos:notation "pHCaCl2_ratio1-5" ;
    skos:prefLabel "pHCaCl2_ratio1-5"@en ;
    skos:scopeNote <https://www.isric.org/sites/default/files/isric_report_2014_01.pdf>,
        "Leenaars J.G.B., A.J.M. van Oostrum and M. Ruiperez Gonzalez, 2014. Africa Soil Profiles Database, Version 1.2. A compilation of georeferenced and standardised legacy soil profile data for Sub-Saharan Africa (with dataset). ISRIC Report 2014/01. Africa Soil Information Service (AfSIS) project and ISRIC - World Soil Information, Wageningen, the Netherlands. See Annex 4." .

glosis_proc:pHProcedure-pHCaCl2_sat a glosis_proc:PHProcedure,
        skos:Concept ;
    skos:broader glosis_proc:pHProcedure-pHCaCl2 ;
    skos:definition "pHCaCl2 (soil reaction) in saturated paste" ;
    skos:inScheme glosis_proc:pHProcedure ;
    skos:notation "pHCaCl2_sat" ;
    skos:prefLabel "pHCaCl2_sat"@en ;
    skos:scopeNote <https://www.isric.org/sites/default/files/isric_report_2014_01.pdf>,
        "Leenaars J.G.B., A.J.M. van Oostrum and M. Ruiperez Gonzalez, 2014. Africa Soil Profiles Database, Version 1.2. A compilation of georeferenced and standardised legacy soil profile data for Sub-Saharan Africa (with dataset). ISRIC Report 2014/01. Africa Soil Information Service (AfSIS) project and ISRIC - World Soil Information, Wageningen, the Netherlands. See Annex 4." .

glosis_proc:pHProcedure-pHH2O a glosis_proc:PHProcedure,
        skos:Concept ;
    skos:definition "pHH2O (soil reaction) in a soil/water solution" ;
    skos:inScheme glosis_proc:pHProcedure ;
    skos:narrower glosis_proc:pHProcedure-pHH2O_ratio1-1,
        glosis_proc:pHProcedure-pHH2O_ratio1-10,
        glosis_proc:pHProcedure-pHH2O_ratio1-2,
        glosis_proc:pHProcedure-pHH2O_ratio1-2.5,
        glosis_proc:pHProcedure-pHH2O_ratio1-5,
        glosis_proc:pHProcedure-pHH2O_sat,
        glosis_proc:pHProcedure-pHH2O_unkn-spec ;
    skos:notation "pHH2O" ;
    skos:prefLabel "pHH2O"@en ;
    skos:scopeNote <https://www.isric.org/sites/default/files/isric_report_2014_01.pdf>,
        "Leenaars J.G.B., A.J.M. van Oostrum and M. Ruiperez Gonzalez, 2014. Africa Soil Profiles Database, Version 1.2. A compilation of georeferenced and standardised legacy soil profile data for Sub-Saharan Africa (with dataset). ISRIC Report 2014/01. Africa Soil Information Service (AfSIS) project and ISRIC - World Soil Information, Wageningen, the Netherlands. See Annex 4." ;
    skos:topConceptOf glosis_proc:pHProcedure .

glosis_proc:pHProcedure-pHH2O_ratio1-1 a glosis_proc:PHProcedure,
        skos:Concept ;
    skos:broader glosis_proc:pHProcedure-pHH2O ;
    skos:definition "pHH2O (soil reaction) in 1:1 soil/water solution" ;
    skos:inScheme glosis_proc:pHProcedure ;
    skos:notation "pHH2O_ratio1-1" ;
    skos:prefLabel "pHH2O_ratio1-1"@en ;
    skos:scopeNote <https://www.isric.org/sites/default/files/isric_report_2014_01.pdf>,
        "Leenaars J.G.B., A.J.M. van Oostrum and M. Ruiperez Gonzalez, 2014. Africa Soil Profiles Database, Version 1.2. A compilation of georeferenced and standardised legacy soil profile data for Sub-Saharan Africa (with dataset). ISRIC Report 2014/01. Africa Soil Information Service (AfSIS) project and ISRIC - World Soil Information, Wageningen, the Netherlands. See Annex 4." .

glosis_proc:pHProcedure-pHH2O_ratio1-10 a glosis_proc:PHProcedure,
        skos:Concept ;
    skos:broader glosis_proc:pHProcedure-pHH2O ;
    skos:definition "pHH2O (soil reaction) in 1:10 soil/water solution" ;
    skos:inScheme glosis_proc:pHProcedure ;
    skos:notation "pHH2O_ratio1-10" ;
    skos:prefLabel "pHH2O_ratio1-10"@en ;
    skos:scopeNote <https://www.isric.org/sites/default/files/isric_report_2014_01.pdf>,
        "Leenaars J.G.B., A.J.M. van Oostrum and M. Ruiperez Gonzalez, 2014. Africa Soil Profiles Database, Version 1.2. A compilation of georeferenced and standardised legacy soil profile data for Sub-Saharan Africa (with dataset). ISRIC Report 2014/01. Africa Soil Information Service (AfSIS) project and ISRIC - World Soil Information, Wageningen, the Netherlands. See Annex 4." .

glosis_proc:pHProcedure-pHH2O_ratio1-2 a glosis_proc:PHProcedure,
        skos:Concept ;
    skos:broader glosis_proc:pHProcedure-pHH2O ;
    skos:definition "pHH2O (soil reaction) in 1:2 soil/water solution" ;
    skos:inScheme glosis_proc:pHProcedure ;
    skos:notation "pHH2O_ratio1-2" ;
    skos:prefLabel "pHH2O_ratio1-2"@en ;
    skos:scopeNote <https://www.isric.org/sites/default/files/isric_report_2014_01.pdf>,
        "Leenaars J.G.B., A.J.M. van Oostrum and M. Ruiperez Gonzalez, 2014. Africa Soil Profiles Database, Version 1.2. A compilation of georeferenced and standardised legacy soil profile data for Sub-Saharan Africa (with dataset). ISRIC Report 2014/01. Africa Soil Information Service (AfSIS) project and ISRIC - World Soil Information, Wageningen, the Netherlands. See Annex 4." .

glosis_proc:pHProcedure-pHH2O_ratio1-2.5 a glosis_proc:PHProcedure,
        skos:Concept ;
    skos:broader glosis_proc:pHProcedure-pHH2O ;
    skos:definition "pHH2O (soil reaction) in 1:2.5 soil/water solution" ;
    skos:inScheme glosis_proc:pHProcedure ;
    skos:notation "pHH2O_ratio1-2.5" ;
    skos:prefLabel "pHH2O_ratio1-2.5"@en ;
    skos:scopeNote <https://www.isric.org/sites/default/files/isric_report_2014_01.pdf>,
        "Leenaars J.G.B., A.J.M. van Oostrum and M. Ruiperez Gonzalez, 2014. Africa Soil Profiles Database, Version 1.2. A compilation of georeferenced and standardised legacy soil profile data for Sub-Saharan Africa (with dataset). ISRIC Report 2014/01. Africa Soil Information Service (AfSIS) project and ISRIC - World Soil Information, Wageningen, the Netherlands. See Annex 4." .

glosis_proc:pHProcedure-pHH2O_ratio1-5 a glosis_proc:PHProcedure,
        skos:Concept ;
    skos:broader glosis_proc:pHProcedure-pHH2O ;
    skos:definition "pHH2O (soil reaction) in 1:5 soil/water solution" ;
    skos:inScheme glosis_proc:pHProcedure ;
    skos:notation "pHH2O_ratio1-5" ;
    skos:prefLabel "pHH2O_ratio1-5"@en ;
    skos:scopeNote <https://www.isric.org/sites/default/files/isric_report_2014_01.pdf>,
        "Leenaars J.G.B., A.J.M. van Oostrum and M. Ruiperez Gonzalez, 2014. Africa Soil Profiles Database, Version 1.2. A compilation of georeferenced and standardised legacy soil profile data for Sub-Saharan Africa (with dataset). ISRIC Report 2014/01. Africa Soil Information Service (AfSIS) project and ISRIC - World Soil Information, Wageningen, the Netherlands. See Annex 4." .

glosis_proc:pHProcedure-pHH2O_sat a glosis_proc:PHProcedure,
        skos:Concept ;
    skos:broader glosis_proc:pHProcedure-pHH2O ;
    skos:definition "pHH2O (soil reaction) in water saturated paste" ;
    skos:inScheme glosis_proc:pHProcedure ;
    skos:notation "pHH2O_sat" ;
    skos:prefLabel "pHH2O_sat"@en ;
    skos:scopeNote <https://www.isric.org/sites/default/files/isric_report_2014_01.pdf>,
        "Leenaars J.G.B., A.J.M. van Oostrum and M. Ruiperez Gonzalez, 2014. Africa Soil Profiles Database, Version 1.2. A compilation of georeferenced and standardised legacy soil profile data for Sub-Saharan Africa (with dataset). ISRIC Report 2014/01. Africa Soil Information Service (AfSIS) project and ISRIC - World Soil Information, Wageningen, the Netherlands. See Annex 4." .

glosis_proc:pHProcedure-pHH2O_unkn-spec a glosis_proc:PHProcedure,
        skos:Concept ;
    skos:broader glosis_proc:pHProcedure-pHH2O ;
    skos:definition "Spectrally measured and converted to pHH2O (soil reaction) in unknown soil/water solution" ;
    skos:inScheme glosis_proc:pHProcedure ;
    skos:notation "pHH2O_unkn-spec" ;
    skos:prefLabel "pHH2O_unkn-spec"@en ;
    skos:scopeNote <https://www.isric.org/sites/default/files/isric_report_2014_01.pdf>,
        "Leenaars J.G.B., A.J.M. van Oostrum and M. Ruiperez Gonzalez, 2014. Africa Soil Profiles Database, Version 1.2. A compilation of georeferenced and standardised legacy soil profile data for Sub-Saharan Africa (with dataset). ISRIC Report 2014/01. Africa Soil Information Service (AfSIS) project and ISRIC - World Soil Information, Wageningen, the Netherlands. See Annex 4." .

glosis_proc:pHProcedure-pHKCl a glosis_proc:PHProcedure,
        skos:Concept ;
    skos:definition "pHKCl (soil reaction) in a soil/KCl solution (0.01-1 M)" ;
    skos:inScheme glosis_proc:pHProcedure ;
    skos:narrower glosis_proc:pHProcedure-pHKCl_ratio1-1,
        glosis_proc:pHProcedure-pHKCl_ratio1-10,
        glosis_proc:pHProcedure-pHKCl_ratio1-2,
        glosis_proc:pHProcedure-pHKCl_ratio1-2.5,
        glosis_proc:pHProcedure-pHKCl_ratio1-5 ;
    skos:notation "pHKCl" ;
    skos:prefLabel "pHKCl"@en ;
    skos:scopeNote <https://www.isric.org/sites/default/files/isric_report_2014_01.pdf>,
        "Leenaars J.G.B., A.J.M. van Oostrum and M. Ruiperez Gonzalez, 2014. Africa Soil Profiles Database, Version 1.2. A compilation of georeferenced and standardised legacy soil profile data for Sub-Saharan Africa (with dataset). ISRIC Report 2014/01. Africa Soil Information Service (AfSIS) project and ISRIC - World Soil Information, Wageningen, the Netherlands. See Annex 4." ;
    skos:topConceptOf glosis_proc:pHProcedure .

glosis_proc:pHProcedure-pHKCl_ratio1-1 a glosis_proc:PHProcedure,
        skos:Concept ;
    skos:broader glosis_proc:pHProcedure-pHKCl ;
    skos:definition "pHKCl (soil reaction) in 1:1 soil/KCl solution (1 M)" ;
    skos:inScheme glosis_proc:pHProcedure ;
    skos:notation "pHKCl_ratio1-1" ;
    skos:prefLabel "pHKCl_ratio1-1"@en ;
    skos:scopeNote <https://www.isric.org/sites/default/files/isric_report_2014_01.pdf>,
        "Leenaars J.G.B., A.J.M. van Oostrum and M. Ruiperez Gonzalez, 2014. Africa Soil Profiles Database, Version 1.2. A compilation of georeferenced and standardised legacy soil profile data for Sub-Saharan Africa (with dataset). ISRIC Report 2014/01. Africa Soil Information Service (AfSIS) project and ISRIC - World Soil Information, Wageningen, the Netherlands. See Annex 4." .

glosis_proc:pHProcedure-pHKCl_ratio1-10 a glosis_proc:PHProcedure,
        skos:Concept ;
    skos:broader glosis_proc:pHProcedure-pHKCl ;
    skos:definition "pHKCl (soil reaction) in 1:10 soil/KCl solution (0.01-1 M)" ;
    skos:inScheme glosis_proc:pHProcedure ;
    skos:notation "pHKCl_ratio1-10" ;
    skos:prefLabel "pHKCl_ratio1-10"@en ;
    skos:scopeNote <https://www.isric.org/sites/default/files/isric_report_2014_01.pdf>,
        "Leenaars J.G.B., A.J.M. van Oostrum and M. Ruiperez Gonzalez, 2014. Africa Soil Profiles Database, Version 1.2. A compilation of georeferenced and standardised legacy soil profile data for Sub-Saharan Africa (with dataset). ISRIC Report 2014/01. Africa Soil Information Service (AfSIS) project and ISRIC - World Soil Information, Wageningen, the Netherlands. See Annex 4." .

glosis_proc:pHProcedure-pHKCl_ratio1-2 a glosis_proc:PHProcedure,
        skos:Concept ;
    skos:broader glosis_proc:pHProcedure-pHKCl ;
    skos:definition "pHKCl (soil reaction) in 1:2 soil/KCl solution (0.01-1 M)" ;
    skos:inScheme glosis_proc:pHProcedure ;
    skos:notation "pHKCl_ratio1-2" ;
    skos:prefLabel "pHKCl_ratio1-2"@en ;
    skos:scopeNote <https://www.isric.org/sites/default/files/isric_report_2014_01.pdf>,
        "Leenaars J.G.B., A.J.M. van Oostrum and M. Ruiperez Gonzalez, 2014. Africa Soil Profiles Database, Version 1.2. A compilation of georeferenced and standardised legacy soil profile data for Sub-Saharan Africa (with dataset). ISRIC Report 2014/01. Africa Soil Information Service (AfSIS) project and ISRIC - World Soil Information, Wageningen, the Netherlands. See Annex 4." .

glosis_proc:pHProcedure-pHKCl_ratio1-2.5 a glosis_proc:PHProcedure,
        skos:Concept ;
    skos:broader glosis_proc:pHProcedure-pHKCl ;
    skos:definition "pHKCl (soil reaction) in 1:2.5 soil/KCl solution (0.01-1 M)" ;
    skos:inScheme glosis_proc:pHProcedure ;
    skos:notation "pHKCl_ratio1-2.5" ;
    skos:prefLabel "pHKCl_ratio1-2.5"@en ;
    skos:scopeNote <https://www.isric.org/sites/default/files/isric_report_2014_01.pdf>,
        "Leenaars J.G.B., A.J.M. van Oostrum and M. Ruiperez Gonzalez, 2014. Africa Soil Profiles Database, Version 1.2. A compilation of georeferenced and standardised legacy soil profile data for Sub-Saharan Africa (with dataset). ISRIC Report 2014/01. Africa Soil Information Service (AfSIS) project and ISRIC - World Soil Information, Wageningen, the Netherlands. See Annex 4." .

glosis_proc:pHProcedure-pHKCl_ratio1-5 a glosis_proc:PHProcedure,
        skos:Concept ;
    skos:broader glosis_proc:pHProcedure-pHKCl ;
    skos:definition "pHKCl (soil reaction) in 1:5 soil/KCl solution (0.01-1 M)" ;
    skos:inScheme glosis_proc:pHProcedure ;
    skos:notation "pHKCl_ratio1-5" ;
    skos:prefLabel "pHKCl_ratio1-5"@en ;
    skos:scopeNote <https://www.isric.org/sites/default/files/isric_report_2014_01.pdf>,
        "Leenaars J.G.B., A.J.M. van Oostrum and M. Ruiperez Gonzalez, 2014. Africa Soil Profiles Database, Version 1.2. A compilation of georeferenced and standardised legacy soil profile data for Sub-Saharan Africa (with dataset). ISRIC Report 2014/01. Africa Soil Information Service (AfSIS) project and ISRIC - World Soil Information, Wageningen, the Netherlands. See Annex 4." .

glosis_proc:pHProcedure-pHKCl_sat a glosis_proc:PHProcedure,
        skos:Concept ;
    skos:definition "pHKCl (soil reaction) in saturated paste" ;
    skos:inScheme glosis_proc:pHProcedure ;
    skos:notation "pHKCl_sat" ;
    skos:prefLabel "pHKCl_sat"@en ;
    skos:scopeNote <https://www.isric.org/sites/default/files/isric_report_2014_01.pdf>,
        "Leenaars J.G.B., A.J.M. van Oostrum and M. Ruiperez Gonzalez, 2014. Africa Soil Profiles Database, Version 1.2. A compilation of georeferenced and standardised legacy soil profile data for Sub-Saharan Africa (with dataset). ISRIC Report 2014/01. Africa Soil Information Service (AfSIS) project and ISRIC - World Soil Information, Wageningen, the Netherlands. See Annex 4." ;
    skos:topConceptOf glosis_proc:pHProcedure .

glosis_proc:pHProcedure-pHNaF a glosis_proc:PHProcedure,
        skos:Concept ;
    skos:definition "pHNaF (soil reaction) in a soil/NaF solution (0.01-1 M)" ;
    skos:inScheme glosis_proc:pHProcedure ;
    skos:narrower glosis_proc:pHProcedure-pHNaF_ratio1-1,
        glosis_proc:pHProcedure-pHNaF_ratio1-10,
        glosis_proc:pHProcedure-pHNaF_ratio1-2,
        glosis_proc:pHProcedure-pHNaF_ratio1-2.5,
        glosis_proc:pHProcedure-pHNaF_ratio1-5,
        glosis_proc:pHProcedure-pHNaF_sat ;
    skos:notation "pHNaF" ;
    skos:prefLabel "pHNaF"@en ;
    skos:scopeNote <https://www.isric.org/sites/default/files/isric_report_2014_01.pdf>,
        "Leenaars J.G.B., A.J.M. van Oostrum and M. Ruiperez Gonzalez, 2014. Africa Soil Profiles Database, Version 1.2. A compilation of georeferenced and standardised legacy soil profile data for Sub-Saharan Africa (with dataset). ISRIC Report 2014/01. Africa Soil Information Service (AfSIS) project and ISRIC - World Soil Information, Wageningen, the Netherlands. See Annex 4." ;
    skos:topConceptOf glosis_proc:pHProcedure .

glosis_proc:pHProcedure-pHNaF_ratio1-1 a glosis_proc:PHProcedure,
        skos:Concept ;
    skos:broader glosis_proc:pHProcedure-pHNaF ;
    skos:definition "pHNaF (soil reaction) in 1:1 soil/NaF solution (1 M)" ;
    skos:inScheme glosis_proc:pHProcedure ;
    skos:notation "pHNaF_ratio1-1" ;
    skos:prefLabel "pHNaF_ratio1-1"@en ;
    skos:scopeNote <https://www.isric.org/sites/default/files/isric_report_2014_01.pdf>,
        "Leenaars J.G.B., A.J.M. van Oostrum and M. Ruiperez Gonzalez, 2014. Africa Soil Profiles Database, Version 1.2. A compilation of georeferenced and standardised legacy soil profile data for Sub-Saharan Africa (with dataset). ISRIC Report 2014/01. Africa Soil Information Service (AfSIS) project and ISRIC - World Soil Information, Wageningen, the Netherlands. See Annex 4." .

glosis_proc:pHProcedure-pHNaF_ratio1-10 a glosis_proc:PHProcedure,
        skos:Concept ;
    skos:broader glosis_proc:pHProcedure-pHNaF ;
    skos:definition "pHNaF (soil reaction) in 1:10 soil/NaF solution (0.01-1 M)" ;
    skos:inScheme glosis_proc:pHProcedure ;
    skos:notation "pHNaF_ratio1-10" ;
    skos:prefLabel "pHNaF_ratio1-10"@en ;
    skos:scopeNote <https://www.isric.org/sites/default/files/isric_report_2014_01.pdf>,
        "Leenaars J.G.B., A.J.M. van Oostrum and M. Ruiperez Gonzalez, 2014. Africa Soil Profiles Database, Version 1.2. A compilation of georeferenced and standardised legacy soil profile data for Sub-Saharan Africa (with dataset). ISRIC Report 2014/01. Africa Soil Information Service (AfSIS) project and ISRIC - World Soil Information, Wageningen, the Netherlands. See Annex 4." .

glosis_proc:pHProcedure-pHNaF_ratio1-2 a glosis_proc:PHProcedure,
        skos:Concept ;
    skos:broader glosis_proc:pHProcedure-pHNaF ;
    skos:definition "pHNaF (soil reaction) in 1:2 soil/NaF solution (0.01-1 M)" ;
    skos:inScheme glosis_proc:pHProcedure ;
    skos:notation "pHNaF_ratio1-2" ;
    skos:prefLabel "pHNaF_ratio1-2"@en ;
    skos:scopeNote <https://www.isric.org/sites/default/files/isric_report_2014_01.pdf>,
        "Leenaars J.G.B., A.J.M. van Oostrum and M. Ruiperez Gonzalez, 2014. Africa Soil Profiles Database, Version 1.2. A compilation of georeferenced and standardised legacy soil profile data for Sub-Saharan Africa (with dataset). ISRIC Report 2014/01. Africa Soil Information Service (AfSIS) project and ISRIC - World Soil Information, Wageningen, the Netherlands. See Annex 4." .

glosis_proc:pHProcedure-pHNaF_ratio1-2.5 a glosis_proc:PHProcedure,
        skos:Concept ;
    skos:broader glosis_proc:pHProcedure-pHNaF ;
    skos:definition "pHNaF (soil reaction) in 1:2.5 soil/NaF solution (0.01-1 M)" ;
    skos:inScheme glosis_proc:pHProcedure ;
    skos:notation "pHNaF_ratio1-2.5" ;
    skos:prefLabel "pHNaF_ratio1-2.5"@en ;
    skos:scopeNote <https://www.isric.org/sites/default/files/isric_report_2014_01.pdf>,
        "Leenaars J.G.B., A.J.M. van Oostrum and M. Ruiperez Gonzalez, 2014. Africa Soil Profiles Database, Version 1.2. A compilation of georeferenced and standardised legacy soil profile data for Sub-Saharan Africa (with dataset). ISRIC Report 2014/01. Africa Soil Information Service (AfSIS) project and ISRIC - World Soil Information, Wageningen, the Netherlands. See Annex 4." .

glosis_proc:pHProcedure-pHNaF_ratio1-5 a glosis_proc:PHProcedure,
        skos:Concept ;
    skos:broader glosis_proc:pHProcedure-pHNaF ;
    skos:definition "pHNaF (soil reaction) in 1:5 soil/NaF solution (0.01-1 M)" ;
    skos:inScheme glosis_proc:pHProcedure ;
    skos:notation "pHNaF_ratio1-5" ;
    skos:prefLabel "pHNaF_ratio1-5"@en ;
    skos:scopeNote <https://www.isric.org/sites/default/files/isric_report_2014_01.pdf>,
        "Leenaars J.G.B., A.J.M. van Oostrum and M. Ruiperez Gonzalez, 2014. Africa Soil Profiles Database, Version 1.2. A compilation of georeferenced and standardised legacy soil profile data for Sub-Saharan Africa (with dataset). ISRIC Report 2014/01. Africa Soil Information Service (AfSIS) project and ISRIC - World Soil Information, Wageningen, the Netherlands. See Annex 4." .

glosis_proc:pHProcedure-pHNaF_sat a glosis_proc:PHProcedure,
        skos:Concept ;
    skos:broader glosis_proc:pHProcedure-pHNaF ;
    skos:definition "pHNaF (soil reaction) in saturated paste" ;
    skos:inScheme glosis_proc:pHProcedure ;
    skos:notation "pHNaF_sat" ;
    skos:prefLabel "pHNaF_sat"@en ;
    skos:scopeNote <https://www.isric.org/sites/default/files/isric_report_2014_01.pdf>,
        "Leenaars J.G.B., A.J.M. van Oostrum and M. Ruiperez Gonzalez, 2014. Africa Soil Profiles Database, Version 1.2. A compilation of georeferenced and standardised legacy soil profile data for Sub-Saharan Africa (with dataset). ISRIC Report 2014/01. Africa Soil Information Service (AfSIS) project and ISRIC - World Soil Information, Wageningen, the Netherlands. See Annex 4." .

glosis_proc:pSAProcedure-beaker-disp a glosis_proc:PSAProcedure,
        skos:Concept ;
    skos:definition "Particle size analysis with beaker method with appropriate dispersion of the primary particles and pretreatment to remove cementing particles (organic matter, carbonates)" ;
    skos:inScheme glosis_proc:pSAProcedure ;
    skos:notation "beaker-disp" ;
    skos:prefLabel "beaker-dispersion"@en ;
    skos:scopeNote <https://www.isric.org/sites/default/files/isric_report_2014_01.pdf>,
        "Leenaars J.G.B., A.J.M. van Oostrum and M. Ruiperez Gonzalez, 2014. Africa Soil Profiles Database, Version 1.2. A compilation of georeferenced and standardised legacy soil profile data for Sub-Saharan Africa (with dataset). ISRIC Report 2014/01. Africa Soil Information Service (AfSIS) project and ISRIC - World Soil Information, Wageningen, the Netherlands. See Annex 4." ;
    skos:topConceptOf glosis_proc:pSAProcedure .

glosis_proc:pSAProcedure-beaker-disp-spec a glosis_proc:PSAProcedure,
        skos:Concept ;
    skos:definition "Spectrally predicted based on measurments with the beaker method with appropriate dispersion of the primary particles and pretreatment to remove cementing particles (organic matter, carbonates)" ;
    skos:inScheme glosis_proc:pSAProcedure ;
    skos:notation "beaker-disp-spec" ;
    skos:prefLabel "beaker-dispersion-spectral"@en ;
    skos:scopeNote <https://www.isric.org/sites/default/files/isric_report_2014_01.pdf>,
        "Leenaars J.G.B., A.J.M. van Oostrum and M. Ruiperez Gonzalez, 2014. Africa Soil Profiles Database, Version 1.2. A compilation of georeferenced and standardised legacy soil profile data for Sub-Saharan Africa (with dataset). ISRIC Report 2014/01. Africa Soil Information Service (AfSIS) project and ISRIC - World Soil Information, Wageningen, the Netherlands. See Annex 4." ;
    skos:topConceptOf glosis_proc:pSAProcedure .

glosis_proc:pSAProcedure-beaker-nodisp a glosis_proc:PSAProcedure,
        skos:Concept ;
    skos:definition "Particle size analysis with beaker method with no dispersion of the primary particlesand pretreatment to remove cementing particles (organic matter, carbonates)" ;
    skos:inScheme glosis_proc:pSAProcedure ;
    skos:notation "beaker-nodisp" ;
    skos:prefLabel "beaker-no_dispersion"@en ;
    skos:scopeNote <https://www.isric.org/sites/default/files/isric_report_2014_01.pdf>,
        "Leenaars J.G.B., A.J.M. van Oostrum and M. Ruiperez Gonzalez, 2014. Africa Soil Profiles Database, Version 1.2. A compilation of georeferenced and standardised legacy soil profile data for Sub-Saharan Africa (with dataset). ISRIC Report 2014/01. Africa Soil Information Service (AfSIS) project and ISRIC - World Soil Information, Wageningen, the Netherlands. See Annex 4." ;
    skos:topConceptOf glosis_proc:pSAProcedure .

glosis_proc:pSAProcedure-beaker-nodisp-spec a glosis_proc:PSAProcedure,
        skos:Concept ;
    skos:definition "Spectrally predicted based on measurments with the beaker method with no dispersion of the primary particles and pretreatment to remove cementing particles (organic matter, carbonates)" ;
    skos:inScheme glosis_proc:pSAProcedure ;
    skos:notation "beaker-nodisp-spec" ;
    skos:prefLabel "beaker-no_dispersion-spectral"@en ;
    skos:scopeNote <https://www.isric.org/sites/default/files/isric_report_2014_01.pdf>,
        "Leenaars J.G.B., A.J.M. van Oostrum and M. Ruiperez Gonzalez, 2014. Africa Soil Profiles Database, Version 1.2. A compilation of georeferenced and standardised legacy soil profile data for Sub-Saharan Africa (with dataset). ISRIC Report 2014/01. Africa Soil Information Service (AfSIS) project and ISRIC - World Soil Information, Wageningen, the Netherlands. See Annex 4." ;
    skos:topConceptOf glosis_proc:pSAProcedure .

glosis_proc:pSAProcedure-beaker-unkdisp a glosis_proc:PSAProcedure,
        skos:Concept ;
    skos:definition "Particle size analysis with beaker method unknown dispersion of the primary particles and pretreatment to remove cementing particles (organic matter, carbonates)" ;
    skos:inScheme glosis_proc:pSAProcedure ;
    skos:notation "beaker-unkdisp" ;
    skos:prefLabel "beaker-unknown_dispersion"@en ;
    skos:scopeNote <https://www.isric.org/sites/default/files/isric_report_2014_01.pdf>,
        "Leenaars J.G.B., A.J.M. van Oostrum and M. Ruiperez Gonzalez, 2014. Africa Soil Profiles Database, Version 1.2. A compilation of georeferenced and standardised legacy soil profile data for Sub-Saharan Africa (with dataset). ISRIC Report 2014/01. Africa Soil Information Service (AfSIS) project and ISRIC - World Soil Information, Wageningen, the Netherlands. See Annex 4." ;
    skos:topConceptOf glosis_proc:pSAProcedure .

glosis_proc:pSAProcedure-beaker-unkdisp-spec a glosis_proc:PSAProcedure,
        skos:Concept ;
    skos:definition "Spectrally predicted based on measurments with the beaker method unknown dispersion of the primary particles and pretreatment to remove cementing particles (organic matter, carbonates)" ;
    skos:inScheme glosis_proc:pSAProcedure ;
    skos:notation "beaker-unkdisp-spec" ;
    skos:prefLabel "beaker-unknown_dispersion-spectral"@en ;
    skos:scopeNote <https://www.isric.org/sites/default/files/isric_report_2014_01.pdf>,
        "Leenaars J.G.B., A.J.M. van Oostrum and M. Ruiperez Gonzalez, 2014. Africa Soil Profiles Database, Version 1.2. A compilation of georeferenced and standardised legacy soil profile data for Sub-Saharan Africa (with dataset). ISRIC Report 2014/01. Africa Soil Information Service (AfSIS) project and ISRIC - World Soil Information, Wageningen, the Netherlands. See Annex 4." ;
    skos:topConceptOf glosis_proc:pSAProcedure .

glosis_proc:pSAProcedure-fldest a glosis_proc:PSAProcedure,
        skos:Concept ;
    skos:definition "Field estimate of the particle size distribution, typically done by hand" ;
    skos:inScheme glosis_proc:pSAProcedure ;
    skos:notation "fldest" ;
    skos:prefLabel "field estimate"@en ;
    skos:scopeNote <https://www.isric.org/sites/default/files/isric_report_2014_01.pdf>,
        "Leenaars J.G.B., A.J.M. van Oostrum and M. Ruiperez Gonzalez, 2014. Africa Soil Profiles Database, Version 1.2. A compilation of georeferenced and standardised legacy soil profile data for Sub-Saharan Africa (with dataset). ISRIC Report 2014/01. Africa Soil Information Service (AfSIS) project and ISRIC - World Soil Information, Wageningen, the Netherlands. See Annex 4." ;
    skos:topConceptOf glosis_proc:pSAProcedure .

glosis_proc:pSAProcedure-hydrometer-disp a glosis_proc:PSAProcedure,
        skos:Concept ;
    skos:definition "Particle size analysis with hydrometer (bouyoucos) method with appropriate dispersion of the primary particles and pretreatment to remove cementing particles (organic matter, carbonates)" ;
    skos:inScheme glosis_proc:pSAProcedure ;
    skos:notation "hydrometer-disp" ;
    skos:prefLabel "hydrometer (bouyoucos)-dispersion"@en ;
    skos:scopeNote <https://www.isric.org/sites/default/files/isric_report_2014_01.pdf>,
        "Leenaars J.G.B., A.J.M. van Oostrum and M. Ruiperez Gonzalez, 2014. Africa Soil Profiles Database, Version 1.2. A compilation of georeferenced and standardised legacy soil profile data for Sub-Saharan Africa (with dataset). ISRIC Report 2014/01. Africa Soil Information Service (AfSIS) project and ISRIC - World Soil Information, Wageningen, the Netherlands. See Annex 4." ;
    skos:topConceptOf glosis_proc:pSAProcedure .

glosis_proc:pSAProcedure-hydrometer-disp-spec a glosis_proc:PSAProcedure,
        skos:Concept ;
    skos:definition "Spectrally predicted based on measurments with the hydrometer (bouyoucos) method with appropriate dispersion of the primary particles and pretreatment to remove cementing particles (organic matter, carbonates)" ;
    skos:inScheme glosis_proc:pSAProcedure ;
    skos:notation "hydrometer-disp-spec" ;
    skos:prefLabel "hydrometer (bouyoucos)-dispersion-spectral"@en ;
    skos:scopeNote <https://www.isric.org/sites/default/files/isric_report_2014_01.pdf>,
        "Leenaars J.G.B., A.J.M. van Oostrum and M. Ruiperez Gonzalez, 2014. Africa Soil Profiles Database, Version 1.2. A compilation of georeferenced and standardised legacy soil profile data for Sub-Saharan Africa (with dataset). ISRIC Report 2014/01. Africa Soil Information Service (AfSIS) project and ISRIC - World Soil Information, Wageningen, the Netherlands. See Annex 4." ;
    skos:topConceptOf glosis_proc:pSAProcedure .

glosis_proc:pSAProcedure-hydrometer-nodisp a glosis_proc:PSAProcedure,
        skos:Concept ;
    skos:definition "Particle size analysis with hydrometer (bouyoucos) method with no dispersion of the primary particles and removal of cementing particles (organic matter, carbonates)" ;
    skos:inScheme glosis_proc:pSAProcedure ;
    skos:notation "hydrometer-nodisp" ;
    skos:prefLabel "hydrometer (bouyoucos)-no_dispersion"@en ;
    skos:scopeNote <https://www.isric.org/sites/default/files/isric_report_2014_01.pdf>,
        "Leenaars J.G.B., A.J.M. van Oostrum and M. Ruiperez Gonzalez, 2014. Africa Soil Profiles Database, Version 1.2. A compilation of georeferenced and standardised legacy soil profile data for Sub-Saharan Africa (with dataset). ISRIC Report 2014/01. Africa Soil Information Service (AfSIS) project and ISRIC - World Soil Information, Wageningen, the Netherlands. See Annex 4." ;
    skos:topConceptOf glosis_proc:pSAProcedure .

glosis_proc:pSAProcedure-hydrometer-nodisp-spec a glosis_proc:PSAProcedure,
        skos:Concept ;
    skos:definition "Spectrally predicted based on measurments with the hydrometer (bouyoucos) method with no dispersion of the primary particles and pretreatment to remove cementing particles (organic matter, carbonates)" ;
    skos:inScheme glosis_proc:pSAProcedure ;
    skos:notation "hydrometer-nodisp-spec" ;
    skos:prefLabel "hydrometer (bouyoucos)-no_dispersion-spectral"@en ;
    skos:scopeNote <https://www.isric.org/sites/default/files/isric_report_2014_01.pdf>,
        "Leenaars J.G.B., A.J.M. van Oostrum and M. Ruiperez Gonzalez, 2014. Africa Soil Profiles Database, Version 1.2. A compilation of georeferenced and standardised legacy soil profile data for Sub-Saharan Africa (with dataset). ISRIC Report 2014/01. Africa Soil Information Service (AfSIS) project and ISRIC - World Soil Information, Wageningen, the Netherlands. See Annex 4." ;
    skos:topConceptOf glosis_proc:pSAProcedure .

glosis_proc:pSAProcedure-hydrometer-unkdisp a glosis_proc:PSAProcedure,
        skos:Concept ;
    skos:definition "Particle size analysis with hydrometer (bouyoucos) method unknown dispersion of the primary particles and pretreatment to remove cementing particles (organic matter, carbonates)" ;
    skos:inScheme glosis_proc:pSAProcedure ;
    skos:notation "hydrometer-unkdisp" ;
    skos:prefLabel "hydrometer (bouyoucos)-unknown_dispersion"@en ;
    skos:scopeNote <https://www.isric.org/sites/default/files/isric_report_2014_01.pdf>,
        "Leenaars J.G.B., A.J.M. van Oostrum and M. Ruiperez Gonzalez, 2014. Africa Soil Profiles Database, Version 1.2. A compilation of georeferenced and standardised legacy soil profile data for Sub-Saharan Africa (with dataset). ISRIC Report 2014/01. Africa Soil Information Service (AfSIS) project and ISRIC - World Soil Information, Wageningen, the Netherlands. See Annex 4." ;
    skos:topConceptOf glosis_proc:pSAProcedure .

glosis_proc:pSAProcedure-hydrometer-unkdisp-spec a glosis_proc:PSAProcedure,
        skos:Concept ;
    skos:definition "Spectrally predicted based on measurments with the hydrometer (bouyoucos) method unknown dispersion of the primary particles and pretreatment to remove cementing particles (organic matter, carbonates)" ;
    skos:inScheme glosis_proc:pSAProcedure ;
    skos:notation "hydrometer-unkdisp-spec" ;
    skos:prefLabel "hydrometer (bouyoucos)-unknown_dispersion-spectral"@en ;
    skos:scopeNote <https://www.isric.org/sites/default/files/isric_report_2014_01.pdf>,
        "Leenaars J.G.B., A.J.M. van Oostrum and M. Ruiperez Gonzalez, 2014. Africa Soil Profiles Database, Version 1.2. A compilation of georeferenced and standardised legacy soil profile data for Sub-Saharan Africa (with dataset). ISRIC Report 2014/01. Africa Soil Information Service (AfSIS) project and ISRIC - World Soil Information, Wageningen, the Netherlands. See Annex 4." ;
    skos:topConceptOf glosis_proc:pSAProcedure .

glosis_proc:pSAProcedure-laser-disp a glosis_proc:PSAProcedure,
        skos:Concept ;
    skos:definition "Particle size analysis with laser diffraction with appropriate disperson of the primary particles and pretreatment to remove cementing particles (organic matter, carbonates)" ;
    skos:inScheme glosis_proc:pSAProcedure ;
    skos:notation "laser-disp" ;
    skos:prefLabel "laser diffraction-dispersion"@en ;
    skos:scopeNote <https://www.isric.org/sites/default/files/isric_report_2014_01.pdf>,
        "Leenaars J.G.B., A.J.M. van Oostrum and M. Ruiperez Gonzalez, 2014. Africa Soil Profiles Database, Version 1.2. A compilation of georeferenced and standardised legacy soil profile data for Sub-Saharan Africa (with dataset). ISRIC Report 2014/01. Africa Soil Information Service (AfSIS) project and ISRIC - World Soil Information, Wageningen, the Netherlands. See Annex 4." ;
    skos:topConceptOf glosis_proc:pSAProcedure .

glosis_proc:pSAProcedure-laser-disp-spec a glosis_proc:PSAProcedure,
        skos:Concept ;
    skos:definition "Spectrally predicted based on measurments with laser diffraction analysis with appropriate disperson of the primary particles and pretreatment to remove cementing particles (organic matter, carbonates)" ;
    skos:inScheme glosis_proc:pSAProcedure ;
    skos:notation "laser-disp-spec" ;
    skos:prefLabel "laser diffraction-dispersion-spectral"@en ;
    skos:scopeNote <https://www.isric.org/sites/default/files/isric_report_2014_01.pdf>,
        "Leenaars J.G.B., A.J.M. van Oostrum and M. Ruiperez Gonzalez, 2014. Africa Soil Profiles Database, Version 1.2. A compilation of georeferenced and standardised legacy soil profile data for Sub-Saharan Africa (with dataset). ISRIC Report 2014/01. Africa Soil Information Service (AfSIS) project and ISRIC - World Soil Information, Wageningen, the Netherlands. See Annex 4." ;
    skos:topConceptOf glosis_proc:pSAProcedure .

glosis_proc:pSAProcedure-laser-nodisp a glosis_proc:PSAProcedure,
        skos:Concept ;
    skos:definition "Particle size analysis with laser diffraction with no dispersion of the primary particles and pretreatment to remove cementing particles (organic matter, carbonates)" ;
    skos:inScheme glosis_proc:pSAProcedure ;
    skos:notation "laser-nodisp" ;
    skos:prefLabel "laser diffraction-no_dispersion"@en ;
    skos:scopeNote <https://www.isric.org/sites/default/files/isric_report_2014_01.pdf>,
        "Leenaars J.G.B., A.J.M. van Oostrum and M. Ruiperez Gonzalez, 2014. Africa Soil Profiles Database, Version 1.2. A compilation of georeferenced and standardised legacy soil profile data for Sub-Saharan Africa (with dataset). ISRIC Report 2014/01. Africa Soil Information Service (AfSIS) project and ISRIC - World Soil Information, Wageningen, the Netherlands. See Annex 4." ;
    skos:topConceptOf glosis_proc:pSAProcedure .

glosis_proc:pSAProcedure-laser-nodisp-spec a glosis_proc:PSAProcedure,
        skos:Concept ;
    skos:definition "Spectrally predicted based on measurments with laser diffraction analysis with no dispersion of the primary particles and pretreatment to remove cementing particles (organic matter, carbonates)" ;
    skos:inScheme glosis_proc:pSAProcedure ;
    skos:notation "laser-nodisp-spec" ;
    skos:prefLabel "laser diffraction-no_dispersion-spectral"@en ;
    skos:scopeNote <https://www.isric.org/sites/default/files/isric_report_2014_01.pdf>,
        "Leenaars J.G.B., A.J.M. van Oostrum and M. Ruiperez Gonzalez, 2014. Africa Soil Profiles Database, Version 1.2. A compilation of georeferenced and standardised legacy soil profile data for Sub-Saharan Africa (with dataset). ISRIC Report 2014/01. Africa Soil Information Service (AfSIS) project and ISRIC - World Soil Information, Wageningen, the Netherlands. See Annex 4." ;
    skos:topConceptOf glosis_proc:pSAProcedure .

glosis_proc:pSAProcedure-laser-unkdisp a glosis_proc:PSAProcedure,
        skos:Concept ;
    skos:definition "Particle size analysis with laser diffraction with unknown dispersion of the primary particles and pretreatment to remove cementing particles (organic matter, carbonates)" ;
    skos:inScheme glosis_proc:pSAProcedure ;
    skos:notation "laser-unkdisp" ;
    skos:prefLabel "laser diffraction-unknown_dispersion"@en ;
    skos:scopeNote <https://www.isric.org/sites/default/files/isric_report_2014_01.pdf>,
        "Leenaars J.G.B., A.J.M. van Oostrum and M. Ruiperez Gonzalez, 2014. Africa Soil Profiles Database, Version 1.2. A compilation of georeferenced and standardised legacy soil profile data for Sub-Saharan Africa (with dataset). ISRIC Report 2014/01. Africa Soil Information Service (AfSIS) project and ISRIC - World Soil Information, Wageningen, the Netherlands. See Annex 4." ;
    skos:topConceptOf glosis_proc:pSAProcedure .

glosis_proc:pSAProcedure-laser-unkdisp-spec a glosis_proc:PSAProcedure,
        skos:Concept ;
    skos:definition "Spectrally predicted based on measurments with laser diffraction analysis with unknown dispersion of the primary particles and pretreatment to remove cementing particles (organic matter, carbonates)" ;
    skos:inScheme glosis_proc:pSAProcedure ;
    skos:notation "laser-unkdisp-spec" ;
    skos:prefLabel "laser diffraction-unknown_dispersion-spectral"@en ;
    skos:scopeNote <https://www.isric.org/sites/default/files/isric_report_2014_01.pdf>,
        "Leenaars J.G.B., A.J.M. van Oostrum and M. Ruiperez Gonzalez, 2014. Africa Soil Profiles Database, Version 1.2. A compilation of georeferenced and standardised legacy soil profile data for Sub-Saharan Africa (with dataset). ISRIC Report 2014/01. Africa Soil Information Service (AfSIS) project and ISRIC - World Soil Information, Wageningen, the Netherlands. See Annex 4." ;
    skos:topConceptOf glosis_proc:pSAProcedure .

glosis_proc:pSAProcedure-pipette-disp a glosis_proc:PSAProcedure,
        skos:Concept ;
    skos:definition "Particle size analysis with pipette method with appropriate dispersion of the primary particles and pretreatment to remove cementing particles (organic matter, carbonates)" ;
    skos:inScheme glosis_proc:pSAProcedure ;
    skos:notation "pipette-disp" ;
    skos:prefLabel "pipette-dispersion"@en ;
    skos:scopeNote <https://www.isric.org/sites/default/files/isric_report_2014_01.pdf>,
        "Leenaars J.G.B., A.J.M. van Oostrum and M. Ruiperez Gonzalez, 2014. Africa Soil Profiles Database, Version 1.2. A compilation of georeferenced and standardised legacy soil profile data for Sub-Saharan Africa (with dataset). ISRIC Report 2014/01. Africa Soil Information Service (AfSIS) project and ISRIC - World Soil Information, Wageningen, the Netherlands. See Annex 4." ;
    skos:topConceptOf glosis_proc:pSAProcedure .

glosis_proc:pSAProcedure-pipette-disp-spec a glosis_proc:PSAProcedure,
        skos:Concept ;
    skos:definition "Spectrally predicted based on measurments with the pipette method with appropriate dispersion of the primary particles and pretreatment to remove cementing particles (organic matter, carbonates)" ;
    skos:inScheme glosis_proc:pSAProcedure ;
    skos:notation "pipette-disp-spec" ;
    skos:prefLabel "pipette-dispersion-spectral"@en ;
    skos:scopeNote <https://www.isric.org/sites/default/files/isric_report_2014_01.pdf>,
        "Leenaars J.G.B., A.J.M. van Oostrum and M. Ruiperez Gonzalez, 2014. Africa Soil Profiles Database, Version 1.2. A compilation of georeferenced and standardised legacy soil profile data for Sub-Saharan Africa (with dataset). ISRIC Report 2014/01. Africa Soil Information Service (AfSIS) project and ISRIC - World Soil Information, Wageningen, the Netherlands. See Annex 4." ;
    skos:topConceptOf glosis_proc:pSAProcedure .

glosis_proc:pSAProcedure-pipette-nodisp a glosis_proc:PSAProcedure,
        skos:Concept ;
    skos:definition "Particle size analysis with pipette method with no dispersion of the primary particles and pretreatment to remove cementing particles (organic matter, carbonates)" ;
    skos:inScheme glosis_proc:pSAProcedure ;
    skos:notation "pipette-nodisp" ;
    skos:prefLabel "pipette-no_dispersion"@en ;
    skos:scopeNote <https://www.isric.org/sites/default/files/isric_report_2014_01.pdf>,
        "Leenaars J.G.B., A.J.M. van Oostrum and M. Ruiperez Gonzalez, 2014. Africa Soil Profiles Database, Version 1.2. A compilation of georeferenced and standardised legacy soil profile data for Sub-Saharan Africa (with dataset). ISRIC Report 2014/01. Africa Soil Information Service (AfSIS) project and ISRIC - World Soil Information, Wageningen, the Netherlands. See Annex 4." ;
    skos:topConceptOf glosis_proc:pSAProcedure .

glosis_proc:pSAProcedure-pipette-nodisp-spec a glosis_proc:PSAProcedure,
        skos:Concept ;
    skos:definition "Spectrally predicted based on measurments with the pipette method with no dispersion of the primary particles and pretreatment to remove cementing particles (organic matter, carbonates)" ;
    skos:inScheme glosis_proc:pSAProcedure ;
    skos:notation "pipette-nodisp-spec" ;
    skos:prefLabel "pipette-no_dispersion-spectral"@en ;
    skos:scopeNote <https://www.isric.org/sites/default/files/isric_report_2014_01.pdf>,
        "Leenaars J.G.B., A.J.M. van Oostrum and M. Ruiperez Gonzalez, 2014. Africa Soil Profiles Database, Version 1.2. A compilation of georeferenced and standardised legacy soil profile data for Sub-Saharan Africa (with dataset). ISRIC Report 2014/01. Africa Soil Information Service (AfSIS) project and ISRIC - World Soil Information, Wageningen, the Netherlands. See Annex 4." ;
    skos:topConceptOf glosis_proc:pSAProcedure .

glosis_proc:pSAProcedure-pipette-unkdisp a glosis_proc:PSAProcedure,
        skos:Concept ;
    skos:definition "Particle size analysis with pipette method unknown dispersion of the primary particles and pretreatment to remove cementing particles (organic matter, carbonates)" ;
    skos:inScheme glosis_proc:pSAProcedure ;
    skos:notation "pipette-unkdisp" ;
    skos:prefLabel "pipette-unknown_dispersion"@en ;
    skos:scopeNote <https://www.isric.org/sites/default/files/isric_report_2014_01.pdf>,
        "Leenaars J.G.B., A.J.M. van Oostrum and M. Ruiperez Gonzalez, 2014. Africa Soil Profiles Database, Version 1.2. A compilation of georeferenced and standardised legacy soil profile data for Sub-Saharan Africa (with dataset). ISRIC Report 2014/01. Africa Soil Information Service (AfSIS) project and ISRIC - World Soil Information, Wageningen, the Netherlands. See Annex 4." ;
    skos:topConceptOf glosis_proc:pSAProcedure .

glosis_proc:pSAProcedure-pipette-unkdisp-spec a glosis_proc:PSAProcedure,
        skos:Concept ;
    skos:definition "Spectrally predicted based on measurments with the pipette method unknown dispersion of the primary particles and pretreatment to remove cementing particles (organic matter, carbonates)" ;
    skos:inScheme glosis_proc:pSAProcedure ;
    skos:notation "pipette-unkdisp-spec" ;
    skos:prefLabel "pipette-unknown_dispersion-spectral"@en ;
    skos:scopeNote <https://www.isric.org/sites/default/files/isric_report_2014_01.pdf>,
        "Leenaars J.G.B., A.J.M. van Oostrum and M. Ruiperez Gonzalez, 2014. Africa Soil Profiles Database, Version 1.2. A compilation of georeferenced and standardised legacy soil profile data for Sub-Saharan Africa (with dataset). ISRIC Report 2014/01. Africa Soil Information Service (AfSIS) project and ISRIC - World Soil Information, Wageningen, the Netherlands. See Annex 4." ;
    skos:topConceptOf glosis_proc:pSAProcedure .

glosis_proc:phosphorusRetentionProcedure-RetentP_blakemore a glosis_proc:PhosphorusRetentionProcedure,
        skos:Concept ;
    skos:definition "P retention at ~pH4.6  (acc. Blakemore 1987)" ;
    skos:inScheme glosis_proc:phosphorusRetentionProcedure ;
    skos:notation "RetentP_blakemore" ;
    skos:prefLabel "RetentP_blakemor"@en ;
    skos:scopeNote "Blakemore L.C. Searle P.L. and Daly, B.K. (1987) Methods for chemical analysis of soils. NZ Soil Bureau, Lower Hutt, New Zealand." ;
    skos:topConceptOf glosis_proc:phosphorusRetentionProcedure .

glosis_proc:phosphorusRetentionProcedure-RetentP_unkn-spec a glosis_proc:PhosphorusRetentionProcedure,
        skos:Concept ;
    skos:definition "Spectrally measured and converted to P retention (P buffer index)" ;
    skos:inScheme glosis_proc:phosphorusRetentionProcedure ;
    skos:notation "RetentP_unkn-spec" ;
    skos:prefLabel "RetentP_unkn-spec"@en ;
    skos:scopeNote <https://www.isric.org/sites/default/files/isric_report_2014_01.pdf>,
        "Leenaars J.G.B., A.J.M. van Oostrum and M. Ruiperez Gonzalez, 2014. Africa Soil Profiles Database, Version 1.2. A compilation of georeferenced and standardised legacy soil profile data for Sub-Saharan Africa (with dataset). ISRIC Report 2014/01. Africa Soil Information Service (AfSIS) project and ISRIC - World Soil Information, Wageningen, the Netherlands. See Annex 4." ;
    skos:topConceptOf glosis_proc:phosphorusRetentionProcedure .

glosis_proc:porosityProcedure-Poros_calcul-pf0 a glosis_proc:PorosityProcedure,
        skos:Concept ;
    skos:definition "Porosity calculated from volumetric moisture content at pF 0 (1 cm)" ;
    skos:inScheme glosis_proc:porosityProcedure ;
    skos:notation "Poros_calcul-pf0" ;
    skos:prefLabel "Poros_calcul-pf0"@en ;
    skos:scopeNote <https://www.isric.org/sites/default/files/isric_report_2014_01.pdf>,
        "Leenaars J.G.B., A.J.M. van Oostrum and M. Ruiperez Gonzalez, 2014. Africa Soil Profiles Database, Version 1.2. A compilation of georeferenced and standardised legacy soil profile data for Sub-Saharan Africa (with dataset). ISRIC Report 2014/01. Africa Soil Information Service (AfSIS) project and ISRIC - World Soil Information, Wageningen, the Netherlands. See Annex 4." ;
    skos:topConceptOf glosis_proc:porosityProcedure .

glosis_proc:solubleSaltsProcedure-SlbAn_calcul-unkn a glosis_proc:SolubleSaltsProcedure,
        skos:Concept ;
    skos:definition "Sum of soluble anions (Cl, SO4, HCO2, CO3, NO3, F)" ;
    skos:inScheme glosis_proc:solubleSaltsProcedure ;
    skos:notation "SlbAn_calcul-unkn" ;
    skos:prefLabel "SlbAn_calcul-unk"@en ;
    skos:scopeNote <https://www.isric.org/sites/default/files/isric_report_2014_01.pdf>,
        "Leenaars J.G.B., A.J.M. van Oostrum and M. Ruiperez Gonzalez, 2014. Africa Soil Profiles Database, Version 1.2. A compilation of georeferenced and standardised legacy soil profile data for Sub-Saharan Africa (with dataset). ISRIC Report 2014/01. Africa Soil Information Service (AfSIS) project and ISRIC - World Soil Information, Wageningen, the Netherlands. See Annex 4." ;
    skos:topConceptOf glosis_proc:solubleSaltsProcedure .

glosis_proc:solubleSaltsProcedure-SlbCat_calcul-unkn a glosis_proc:SolubleSaltsProcedure,
        skos:Concept ;
    skos:definition "Sum of soluble cations (Ca, Mg, K, Na)" ;
    skos:inScheme glosis_proc:solubleSaltsProcedure ;
    skos:notation "SlbCat_calcul-unkn" ;
    skos:prefLabel "SlbCat_calcul-unk"@en ;
    skos:scopeNote <https://www.isric.org/sites/default/files/isric_report_2014_01.pdf>,
        "Leenaars J.G.B., A.J.M. van Oostrum and M. Ruiperez Gonzalez, 2014. Africa Soil Profiles Database, Version 1.2. A compilation of georeferenced and standardised legacy soil profile data for Sub-Saharan Africa (with dataset). ISRIC Report 2014/01. Africa Soil Information Service (AfSIS) project and ISRIC - World Soil Information, Wageningen, the Netherlands. See Annex 4." ;
    skos:topConceptOf glosis_proc:solubleSaltsProcedure .

glosis_proc:textureSumProcedure-SumTxtr_calcul a glosis_proc:TextureSumProcedure,
        skos:Concept ;
    skos:definition "Calculated sum of sand, silt and clay fractions" ;
    skos:inScheme glosis_proc:textureSumProcedure ;
    skos:notation "SumTxtr_calcul" ;
    skos:prefLabel "SumTxtr_calcul"@en ;
    skos:scopeNote <https://www.isric.org/sites/default/files/isric_report_2014_01.pdf>,
        "Leenaars J.G.B., A.J.M. van Oostrum and M. Ruiperez Gonzalez, 2014. Africa Soil Profiles Database, Version 1.2. A compilation of georeferenced and standardised legacy soil profile data for Sub-Saharan Africa (with dataset). ISRIC Report 2014/01. Africa Soil Information Service (AfSIS) project and ISRIC - World Soil Information, Wageningen, the Netherlands. See Annex 4." ;
    skos:topConceptOf glosis_proc:textureSumProcedure .

glosis_proc:totalCarbonateEquivalentProcedure-CaCO3_acid-ch3cooh-dc a glosis_proc:TotalCarbonateEquivalentProcedure,
        skos:Concept ;
    skos:definition "Dissolution of carbonates by Acetic acid [CH3COOH], external heat (dry combustion)" ;
    skos:inScheme glosis_proc:totalCarbonateEquivalentProcedure ;
    skos:notation "CaCO3_acid-ch3cooh-dc" ;
    skos:prefLabel "CaCO3_acid-ch3cooh-dc"@en ;
    skos:scopeNote <https://www.isric.org/sites/default/files/isric_report_2014_01.pdf>,
        "Leenaars J.G.B., A.J.M. van Oostrum and M. Ruiperez Gonzalez, 2014. Africa Soil Profiles Database, Version 1.2. A compilation of georeferenced and standardised legacy soil profile data for Sub-Saharan Africa (with dataset). ISRIC Report 2014/01. Africa Soil Information Service (AfSIS) project and ISRIC - World Soil Information, Wageningen, the Netherlands. See Annex 4." ;
    skos:topConceptOf glosis_proc:totalCarbonateEquivalentProcedure .

glosis_proc:totalCarbonateEquivalentProcedure-CaCO3_acid-ch3cooh-nodc a glosis_proc:TotalCarbonateEquivalentProcedure,
        skos:Concept ;
    skos:definition "Dissolution of carbonates by Acetic acid [CH3COOH], no external (no dry combustion)" ;
    skos:inScheme glosis_proc:totalCarbonateEquivalentProcedure ;
    skos:notation "CaCO3_acid-ch3cooh-nodc" ;
    skos:prefLabel "CaCO3_acid-ch3cooh-nodc"@en ;
    skos:scopeNote <https://www.isric.org/sites/default/files/isric_report_2014_01.pdf>,
        "Leenaars J.G.B., A.J.M. van Oostrum and M. Ruiperez Gonzalez, 2014. Africa Soil Profiles Database, Version 1.2. A compilation of georeferenced and standardised legacy soil profile data for Sub-Saharan Africa (with dataset). ISRIC Report 2014/01. Africa Soil Information Service (AfSIS) project and ISRIC - World Soil Information, Wageningen, the Netherlands. See Annex 4." ;
    skos:topConceptOf glosis_proc:totalCarbonateEquivalentProcedure .

glosis_proc:totalCarbonateEquivalentProcedure-CaCO3_acid-ch3cooh-unkn a glosis_proc:TotalCarbonateEquivalentProcedure,
        skos:Concept ;
    skos:definition "Dissolution of carbonates by Acetic acid [CH3COOH], external heat unknown" ;
    skos:inScheme glosis_proc:totalCarbonateEquivalentProcedure ;
    skos:notation "CaCO3_acid-ch3cooh-unkn" ;
    skos:prefLabel "CaCO3_acid-ch3cooh-unk"@en ;
    skos:scopeNote <https://www.isric.org/sites/default/files/isric_report_2014_01.pdf>,
        "Leenaars J.G.B., A.J.M. van Oostrum and M. Ruiperez Gonzalez, 2014. Africa Soil Profiles Database, Version 1.2. A compilation of georeferenced and standardised legacy soil profile data for Sub-Saharan Africa (with dataset). ISRIC Report 2014/01. Africa Soil Information Service (AfSIS) project and ISRIC - World Soil Information, Wageningen, the Netherlands. See Annex 4." ;
    skos:topConceptOf glosis_proc:totalCarbonateEquivalentProcedure .

glosis_proc:totalCarbonateEquivalentProcedure-CaCO3_acid-dc a glosis_proc:TotalCarbonateEquivalentProcedure,
        skos:Concept ;
    skos:definition "Dissolution of carbonates by acid, external heat (dry combustion)" ;
    skos:inScheme glosis_proc:totalCarbonateEquivalentProcedure ;
    skos:notation "CaCO3_acid-dc" ;
    skos:prefLabel "CaCO3_acid-dc"@en ;
    skos:scopeNote <https://www.isric.org/sites/default/files/isric_report_2014_01.pdf>,
        "Leenaars J.G.B., A.J.M. van Oostrum and M. Ruiperez Gonzalez, 2014. Africa Soil Profiles Database, Version 1.2. A compilation of georeferenced and standardised legacy soil profile data for Sub-Saharan Africa (with dataset). ISRIC Report 2014/01. Africa Soil Information Service (AfSIS) project and ISRIC - World Soil Information, Wageningen, the Netherlands. See Annex 4." ;
    skos:topConceptOf glosis_proc:totalCarbonateEquivalentProcedure .

glosis_proc:totalCarbonateEquivalentProcedure-CaCO3_acid-h2so4-dc a glosis_proc:TotalCarbonateEquivalentProcedure,
        skos:Concept ;
    skos:definition "Dissolution of carbonates by Sulfuric acid [H2SO4], external heat (dry combustion)" ;
    skos:inScheme glosis_proc:totalCarbonateEquivalentProcedure ;
    skos:notation "CaCO3_acid-h2so4-dc" ;
    skos:prefLabel "CaCO3_acid-h2so4-dc"@en ;
    skos:scopeNote <https://www.isric.org/sites/default/files/isric_report_2014_01.pdf>,
        "Leenaars J.G.B., A.J.M. van Oostrum and M. Ruiperez Gonzalez, 2014. Africa Soil Profiles Database, Version 1.2. A compilation of georeferenced and standardised legacy soil profile data for Sub-Saharan Africa (with dataset). ISRIC Report 2014/01. Africa Soil Information Service (AfSIS) project and ISRIC - World Soil Information, Wageningen, the Netherlands. See Annex 4." ;
    skos:topConceptOf glosis_proc:totalCarbonateEquivalentProcedure .

glosis_proc:totalCarbonateEquivalentProcedure-CaCO3_acid-h2so4-nodc a glosis_proc:TotalCarbonateEquivalentProcedure,
        skos:Concept ;
    skos:definition "Dissolution of carbonates by Sulfuric acid [H2SO4], no external (no dry combustion)" ;
    skos:inScheme glosis_proc:totalCarbonateEquivalentProcedure ;
    skos:notation "CaCO3_acid-h2so4-nodc" ;
    skos:prefLabel "CaCO3_acid-h2so4-nodc"@en ;
    skos:scopeNote <https://www.isric.org/sites/default/files/isric_report_2014_01.pdf>,
        "Leenaars J.G.B., A.J.M. van Oostrum and M. Ruiperez Gonzalez, 2014. Africa Soil Profiles Database, Version 1.2. A compilation of georeferenced and standardised legacy soil profile data for Sub-Saharan Africa (with dataset). ISRIC Report 2014/01. Africa Soil Information Service (AfSIS) project and ISRIC - World Soil Information, Wageningen, the Netherlands. See Annex 4." ;
    skos:topConceptOf glosis_proc:totalCarbonateEquivalentProcedure .

glosis_proc:totalCarbonateEquivalentProcedure-CaCO3_acid-h2so4-unkn a glosis_proc:TotalCarbonateEquivalentProcedure,
        skos:Concept ;
    skos:definition "Dissolution of carbonates by Sulfuric acid [H2SO4], external heat unknown" ;
    skos:inScheme glosis_proc:totalCarbonateEquivalentProcedure ;
    skos:notation "CaCO3_acid-h2so4-unkn" ;
    skos:prefLabel "CaCO3_acid-h2so4-unk"@en ;
    skos:scopeNote <https://www.isric.org/sites/default/files/isric_report_2014_01.pdf>,
        "Leenaars J.G.B., A.J.M. van Oostrum and M. Ruiperez Gonzalez, 2014. Africa Soil Profiles Database, Version 1.2. A compilation of georeferenced and standardised legacy soil profile data for Sub-Saharan Africa (with dataset). ISRIC Report 2014/01. Africa Soil Information Service (AfSIS) project and ISRIC - World Soil Information, Wageningen, the Netherlands. See Annex 4." ;
    skos:topConceptOf glosis_proc:totalCarbonateEquivalentProcedure .

glosis_proc:totalCarbonateEquivalentProcedure-CaCO3_acid-h3po4-dc a glosis_proc:TotalCarbonateEquivalentProcedure,
        skos:Concept ;
    skos:definition "Dissolution of carbonates by Phosphoric acid [H3PO4], external heat (dry combustion)" ;
    skos:inScheme glosis_proc:totalCarbonateEquivalentProcedure ;
    skos:notation "CaCO3_acid-h3po4-dc" ;
    skos:prefLabel "CaCO3_acid-h3po4-dc"@en ;
    skos:scopeNote <https://www.isric.org/sites/default/files/isric_report_2014_01.pdf>,
        "Leenaars J.G.B., A.J.M. van Oostrum and M. Ruiperez Gonzalez, 2014. Africa Soil Profiles Database, Version 1.2. A compilation of georeferenced and standardised legacy soil profile data for Sub-Saharan Africa (with dataset). ISRIC Report 2014/01. Africa Soil Information Service (AfSIS) project and ISRIC - World Soil Information, Wageningen, the Netherlands. See Annex 4." ;
    skos:topConceptOf glosis_proc:totalCarbonateEquivalentProcedure .

glosis_proc:totalCarbonateEquivalentProcedure-CaCO3_acid-h3po4-nodc a glosis_proc:TotalCarbonateEquivalentProcedure,
        skos:Concept ;
    skos:definition "Dissolution of carbonates by Phosphoric acid [H3PO4], no external (no dry combustion)" ;
    skos:inScheme glosis_proc:totalCarbonateEquivalentProcedure ;
    skos:notation "CaCO3_acid-h3po4-nodc" ;
    skos:prefLabel "CaCO3_acid-h3po4-nodc"@en ;
    skos:scopeNote <https://www.isric.org/sites/default/files/isric_report_2014_01.pdf>,
        "Leenaars J.G.B., A.J.M. van Oostrum and M. Ruiperez Gonzalez, 2014. Africa Soil Profiles Database, Version 1.2. A compilation of georeferenced and standardised legacy soil profile data for Sub-Saharan Africa (with dataset). ISRIC Report 2014/01. Africa Soil Information Service (AfSIS) project and ISRIC - World Soil Information, Wageningen, the Netherlands. See Annex 4." ;
    skos:topConceptOf glosis_proc:totalCarbonateEquivalentProcedure .

glosis_proc:totalCarbonateEquivalentProcedure-CaCO3_acid-h3po4-unkn a glosis_proc:TotalCarbonateEquivalentProcedure,
        skos:Concept ;
    skos:definition "Dissolution of carbonates by Phosphoric acid [H3PO4], external heat unknown" ;
    skos:inScheme glosis_proc:totalCarbonateEquivalentProcedure ;
    skos:notation "CaCO3_acid-h3po4-unkn" ;
    skos:prefLabel "CaCO3_acid-h3po4-unk"@en ;
    skos:scopeNote <https://www.isric.org/sites/default/files/isric_report_2014_01.pdf>,
        "Leenaars J.G.B., A.J.M. van Oostrum and M. Ruiperez Gonzalez, 2014. Africa Soil Profiles Database, Version 1.2. A compilation of georeferenced and standardised legacy soil profile data for Sub-Saharan Africa (with dataset). ISRIC Report 2014/01. Africa Soil Information Service (AfSIS) project and ISRIC - World Soil Information, Wageningen, the Netherlands. See Annex 4." ;
    skos:topConceptOf glosis_proc:totalCarbonateEquivalentProcedure .

glosis_proc:totalCarbonateEquivalentProcedure-CaCO3_acid-hcl-dc a glosis_proc:TotalCarbonateEquivalentProcedure,
        skos:Concept ;
    skos:definition "Dissolution of carbonates by Hydrochloric acid [HCl], or Perchloric acid [HClO4], external heat (dry combustion)" ;
    skos:inScheme glosis_proc:totalCarbonateEquivalentProcedure ;
    skos:notation "CaCO3_acid-hcl-dc" ;
    skos:prefLabel "CaCO3_acid-hcl-dc"@en ;
    skos:scopeNote <https://www.isric.org/sites/default/files/isric_report_2014_01.pdf>,
        "Leenaars J.G.B., A.J.M. van Oostrum and M. Ruiperez Gonzalez, 2014. Africa Soil Profiles Database, Version 1.2. A compilation of georeferenced and standardised legacy soil profile data for Sub-Saharan Africa (with dataset). ISRIC Report 2014/01. Africa Soil Information Service (AfSIS) project and ISRIC - World Soil Information, Wageningen, the Netherlands. See Annex 4." ;
    skos:topConceptOf glosis_proc:totalCarbonateEquivalentProcedure .

glosis_proc:totalCarbonateEquivalentProcedure-CaCO3_acid-hcl-nodc a glosis_proc:TotalCarbonateEquivalentProcedure,
        skos:Concept ;
    skos:definition "Dissolution of carbonates by Hydrochloric acid [HCl], or Perchloric acid [HClO4], no external (no dry combustion)" ;
    skos:inScheme glosis_proc:totalCarbonateEquivalentProcedure ;
    skos:notation "CaCO3_acid-hcl-nodc" ;
    skos:prefLabel "CaCO3_acid-hcl-nodc"@en ;
    skos:scopeNote <https://www.isric.org/sites/default/files/isric_report_2014_01.pdf>,
        "Leenaars J.G.B., A.J.M. van Oostrum and M. Ruiperez Gonzalez, 2014. Africa Soil Profiles Database, Version 1.2. A compilation of georeferenced and standardised legacy soil profile data for Sub-Saharan Africa (with dataset). ISRIC Report 2014/01. Africa Soil Information Service (AfSIS) project and ISRIC - World Soil Information, Wageningen, the Netherlands. See Annex 4." ;
    skos:topConceptOf glosis_proc:totalCarbonateEquivalentProcedure .

glosis_proc:totalCarbonateEquivalentProcedure-CaCO3_acid-hcl-unkn a glosis_proc:TotalCarbonateEquivalentProcedure,
        skos:Concept ;
    skos:definition "Dissolution of carbonates by Hydrochloric acid [HCl], or Perchloric acid [HClO4], external heat unknown" ;
    skos:inScheme glosis_proc:totalCarbonateEquivalentProcedure ;
    skos:notation "CaCO3_acid-hcl-unkn" ;
    skos:prefLabel "CaCO3_acid-hcl-unk"@en ;
    skos:scopeNote <https://www.isric.org/sites/default/files/isric_report_2014_01.pdf>,
        "Leenaars J.G.B., A.J.M. van Oostrum and M. Ruiperez Gonzalez, 2014. Africa Soil Profiles Database, Version 1.2. A compilation of georeferenced and standardised legacy soil profile data for Sub-Saharan Africa (with dataset). ISRIC Report 2014/01. Africa Soil Information Service (AfSIS) project and ISRIC - World Soil Information, Wageningen, the Netherlands. See Annex 4." ;
    skos:topConceptOf glosis_proc:totalCarbonateEquivalentProcedure .

glosis_proc:totalCarbonateEquivalentProcedure-CaCO3_acid-nodc a glosis_proc:TotalCarbonateEquivalentProcedure,
        skos:Concept ;
    skos:definition "Dissolution of carbonates by acid, no external (no dry combustion)" ;
    skos:inScheme glosis_proc:totalCarbonateEquivalentProcedure ;
    skos:notation "CaCO3_acid-nodc" ;
    skos:prefLabel "CaCO3_acid-nodc"@en ;
    skos:scopeNote <https://www.isric.org/sites/default/files/isric_report_2014_01.pdf>,
        "Leenaars J.G.B., A.J.M. van Oostrum and M. Ruiperez Gonzalez, 2014. Africa Soil Profiles Database, Version 1.2. A compilation of georeferenced and standardised legacy soil profile data for Sub-Saharan Africa (with dataset). ISRIC Report 2014/01. Africa Soil Information Service (AfSIS) project and ISRIC - World Soil Information, Wageningen, the Netherlands. See Annex 4." ;
    skos:topConceptOf glosis_proc:totalCarbonateEquivalentProcedure .

glosis_proc:totalCarbonateEquivalentProcedure-CaCO3_acid-unkn a glosis_proc:TotalCarbonateEquivalentProcedure,
        skos:Concept ;
    skos:definition "Dissolution of carbonates by acid, external heat unknown" ;
    skos:inScheme glosis_proc:totalCarbonateEquivalentProcedure ;
    skos:notation "CaCO3_acid-unkn" ;
    skos:prefLabel "CaCO3_acid-unk"@en ;
    skos:scopeNote <https://www.isric.org/sites/default/files/isric_report_2014_01.pdf>,
        "Leenaars J.G.B., A.J.M. van Oostrum and M. Ruiperez Gonzalez, 2014. Africa Soil Profiles Database, Version 1.2. A compilation of georeferenced and standardised legacy soil profile data for Sub-Saharan Africa (with dataset). ISRIC Report 2014/01. Africa Soil Information Service (AfSIS) project and ISRIC - World Soil Information, Wageningen, the Netherlands. See Annex 4." ;
    skos:topConceptOf glosis_proc:totalCarbonateEquivalentProcedure .

glosis_proc:totalCarbonateEquivalentProcedure-CaCO3_ca01 a glosis_proc:TotalCarbonateEquivalentProcedure,
        skos:Concept ;
    skos:definition "Method of Scheibler (volumetric)" ;
    skos:inScheme glosis_proc:totalCarbonateEquivalentProcedure ;
    skos:notation "CaCO3_ca01" ;
    skos:prefLabel "CaCO3_ca01"@en ;
    skos:scopeNote "ON L 1084-99 (1999) Chemical analyses of soils—determination of carbonate. In: Austrian Standards Institute (ed) O‹ NORM L 1084. Austrian Standards Institute, Vienna" ;
    skos:topConceptOf glosis_proc:totalCarbonateEquivalentProcedure .

glosis_proc:totalCarbonateEquivalentProcedure-CaCO3_ca02 a glosis_proc:TotalCarbonateEquivalentProcedure,
        skos:Concept ;
    skos:definition "Method of Wesemael" ;
    skos:inScheme glosis_proc:totalCarbonateEquivalentProcedure ;
    skos:notation "CaCO3_ca02" ;
    skos:prefLabel "CaCO3_ca02"@en ;
    skos:scopeNote "Wesemael, J.C., 1955. De bepaling van van calciumcarbonaatgehalte van gronden. Chemisch Weekblad 51, 35-36." ;
    skos:topConceptOf glosis_proc:totalCarbonateEquivalentProcedure .

glosis_proc:totalCarbonateEquivalentProcedure-CaCO3_ca03 a glosis_proc:TotalCarbonateEquivalentProcedure,
        skos:Concept ;
    skos:definition "Method of Piper (HCl)" ;
    skos:inScheme glosis_proc:totalCarbonateEquivalentProcedure ;
    skos:notation "CaCO3_ca03" ;
    skos:prefLabel "CaCO3_ca03"@en ;
    skos:scopeNote <https://www.isric.org/sites/default/files/isric_report_2014_01.pdf>,
        "Leenaars J.G.B., A.J.M. van Oostrum and M. Ruiperez Gonzalez, 2014. Africa Soil Profiles Database, Version 1.2. A compilation of georeferenced and standardised legacy soil profile data for Sub-Saharan Africa (with dataset). ISRIC Report 2014/01. Africa Soil Information Service (AfSIS) project and ISRIC - World Soil Information, Wageningen, the Netherlands. See Annex 4." ;
    skos:topConceptOf glosis_proc:totalCarbonateEquivalentProcedure .

glosis_proc:totalCarbonateEquivalentProcedure-CaCO3_ca04 a glosis_proc:TotalCarbonateEquivalentProcedure,
        skos:Concept ;
    skos:definition "Calcimeter method (volumetric after adition of dilute acid)" ;
    skos:inScheme glosis_proc:totalCarbonateEquivalentProcedure ;
    skos:notation "CaCO3_ca04" ;
    skos:prefLabel "CaCO3_ca04"@en ;
    skos:scopeNote <https://www.isric.org/sites/default/files/isric_report_2014_01.pdf>,
        "Leenaars J.G.B., A.J.M. van Oostrum and M. Ruiperez Gonzalez, 2014. Africa Soil Profiles Database, Version 1.2. A compilation of georeferenced and standardised legacy soil profile data for Sub-Saharan Africa (with dataset). ISRIC Report 2014/01. Africa Soil Information Service (AfSIS) project and ISRIC - World Soil Information, Wageningen, the Netherlands. See Annex 4." ;
    skos:topConceptOf glosis_proc:totalCarbonateEquivalentProcedure .

glosis_proc:totalCarbonateEquivalentProcedure-CaCO3_ca05 a glosis_proc:TotalCarbonateEquivalentProcedure,
        skos:Concept ;
    skos:definition "Gravimetric (USDA Agr. Hdbk 60-/- method Richards et al., 1954)" ;
    skos:inScheme glosis_proc:totalCarbonateEquivalentProcedure ;
    skos:notation "CaCO3_ca05" ;
    skos:prefLabel "CaCO3_ca05"@en ;
    skos:scopeNote <https://www.isric.org/sites/default/files/isric_report_2014_01.pdf>,
        "Leenaars J.G.B., A.J.M. van Oostrum and M. Ruiperez Gonzalez, 2014. Africa Soil Profiles Database, Version 1.2. A compilation of georeferenced and standardised legacy soil profile data for Sub-Saharan Africa (with dataset). ISRIC Report 2014/01. Africa Soil Information Service (AfSIS) project and ISRIC - World Soil Information, Wageningen, the Netherlands. See Annex 4." ;
    skos:topConceptOf glosis_proc:totalCarbonateEquivalentProcedure .

glosis_proc:totalCarbonateEquivalentProcedure-CaCO3_ca06 a glosis_proc:TotalCarbonateEquivalentProcedure,
        skos:Concept ;
    skos:definition "H3PO4 acid at 80C, conductometric in NaOH (Schlichting & Blume, 1966)" ;
    skos:inScheme glosis_proc:totalCarbonateEquivalentProcedure ;
    skos:notation "CaCO3_ca06" ;
    skos:prefLabel "CaCO3_ca06"@en ;
    skos:scopeNote <https://www.isric.org/sites/default/files/isric_report_2014_01.pdf>,
        "Leenaars J.G.B., A.J.M. van Oostrum and M. Ruiperez Gonzalez, 2014. Africa Soil Profiles Database, Version 1.2. A compilation of georeferenced and standardised legacy soil profile data for Sub-Saharan Africa (with dataset). ISRIC Report 2014/01. Africa Soil Information Service (AfSIS) project and ISRIC - World Soil Information, Wageningen, the Netherlands. See Annex 4." ;
    skos:topConceptOf glosis_proc:totalCarbonateEquivalentProcedure .

glosis_proc:totalCarbonateEquivalentProcedure-CaCO3_ca07 a glosis_proc:TotalCarbonateEquivalentProcedure,
        skos:Concept ;
    skos:definition "Pressure calcimeter (Nelson, 1982)" ;
    skos:inScheme glosis_proc:totalCarbonateEquivalentProcedure ;
    skos:notation "CaCO3_ca07" ;
    skos:prefLabel "CaCO3_ca07"@en ;
    skos:scopeNote <https://acsess.onlinelibrary.wiley.com/doi/book/10.2134/agronmonogr9.2.2ed>,
        "Nelson, D.W., and L.E. Sommers. 1982. Total carbon, organic carbon and organic matter. p. 539-579. In A.L. Page (ed.), 1983. Methods of soil analysis. Part 2. 2nd ed. Agron. Monogr. 9. ASA and SSSA, Madison, WI." ;
    skos:topConceptOf glosis_proc:totalCarbonateEquivalentProcedure .

glosis_proc:totalCarbonateEquivalentProcedure-CaCO3_ca08 a glosis_proc:TotalCarbonateEquivalentProcedure,
        skos:Concept ;
    skos:definition "Bernard calcimeter (Total CaCO3)" ;
    skos:inScheme glosis_proc:totalCarbonateEquivalentProcedure ;
    skos:notation "CaCO3_ca08" ;
    skos:prefLabel "CaCO3_ca08"@en ;
    skos:scopeNote <https://www.isric.org/sites/default/files/isric_report_2014_01.pdf>,
        "Leenaars J.G.B., A.J.M. van Oostrum and M. Ruiperez Gonzalez, 2014. Africa Soil Profiles Database, Version 1.2. A compilation of georeferenced and standardised legacy soil profile data for Sub-Saharan Africa (with dataset). ISRIC Report 2014/01. Africa Soil Information Service (AfSIS) project and ISRIC - World Soil Information, Wageningen, the Netherlands. See Annex 4." ;
    skos:topConceptOf glosis_proc:totalCarbonateEquivalentProcedure .

glosis_proc:totalCarbonateEquivalentProcedure-CaCO3_ca09 a glosis_proc:TotalCarbonateEquivalentProcedure,
        skos:Concept ;
    skos:definition "Carbonates: H3PO4 treatment at 80 deg. C and CO2 measurement like TOC (OC13), transformation into CaCO3 (Schlichting et al. 1995)" ;
    skos:inScheme glosis_proc:totalCarbonateEquivalentProcedure ;
    skos:notation "CaCO3_ca09" ;
    skos:prefLabel "CaCO3_ca09"@en ;
    skos:scopeNote <https://www.isric.org/sites/default/files/isric_report_2014_01.pdf>,
        "Leenaars J.G.B., A.J.M. van Oostrum and M. Ruiperez Gonzalez, 2014. Africa Soil Profiles Database, Version 1.2. A compilation of georeferenced and standardised legacy soil profile data for Sub-Saharan Africa (with dataset). ISRIC Report 2014/01. Africa Soil Information Service (AfSIS) project and ISRIC - World Soil Information, Wageningen, the Netherlands. See Annex 4." ;
    skos:topConceptOf glosis_proc:totalCarbonateEquivalentProcedure .

glosis_proc:totalCarbonateEquivalentProcedure-CaCO3_ca10 a glosis_proc:TotalCarbonateEquivalentProcedure,
        skos:Concept ;
    skos:definition "CaCO3 Equivalent, CO2 evolution after HCl treatment. Gravimetric" ;
    skos:inScheme glosis_proc:totalCarbonateEquivalentProcedure ;
    skos:notation "CaCO3_ca10" ;
    skos:prefLabel "CaCO3_ca10"@en ;
    skos:scopeNote <https://www.isric.org/sites/default/files/isric_report_2014_01.pdf>,
        "Leenaars J.G.B., A.J.M. van Oostrum and M. Ruiperez Gonzalez, 2014. Africa Soil Profiles Database, Version 1.2. A compilation of georeferenced and standardised legacy soil profile data for Sub-Saharan Africa (with dataset). ISRIC Report 2014/01. Africa Soil Information Service (AfSIS) project and ISRIC - World Soil Information, Wageningen, the Netherlands. See Annex 4." ;
    skos:topConceptOf glosis_proc:totalCarbonateEquivalentProcedure .

glosis_proc:totalCarbonateEquivalentProcedure-CaCO3_ca11 a glosis_proc:TotalCarbonateEquivalentProcedure,
        skos:Concept ;
    skos:definition "Black, 1965-HCl" ;
    skos:inScheme glosis_proc:totalCarbonateEquivalentProcedure ;
    skos:notation "CaCO3_ca11" ;
    skos:prefLabel "CaCO3_ca11"@en ;
    skos:scopeNote <https://www.isric.org/sites/default/files/isric_report_2014_01.pdf>,
        "Leenaars J.G.B., A.J.M. van Oostrum and M. Ruiperez Gonzalez, 2014. Africa Soil Profiles Database, Version 1.2. A compilation of georeferenced and standardised legacy soil profile data for Sub-Saharan Africa (with dataset). ISRIC Report 2014/01. Africa Soil Information Service (AfSIS) project and ISRIC - World Soil Information, Wageningen, the Netherlands. See Annex 4." ;
    skos:topConceptOf glosis_proc:totalCarbonateEquivalentProcedure .

glosis_proc:totalCarbonateEquivalentProcedure-CaCO3_ca12 a glosis_proc:TotalCarbonateEquivalentProcedure,
        skos:Concept ;
    skos:definition "Treatment with H2SO4 N/2 acid followed by titration with NaOH N/2 in presence of an indicator" ;
    skos:inScheme glosis_proc:totalCarbonateEquivalentProcedure ;
    skos:notation "CaCO3_ca12" ;
    skos:prefLabel "CaCO3_ca12"@en ;
    skos:scopeNote <https://www.isric.org/sites/default/files/isric_report_2014_01.pdf>,
        "Leenaars J.G.B., A.J.M. van Oostrum and M. Ruiperez Gonzalez, 2014. Africa Soil Profiles Database, Version 1.2. A compilation of georeferenced and standardised legacy soil profile data for Sub-Saharan Africa (with dataset). ISRIC Report 2014/01. Africa Soil Information Service (AfSIS) project and ISRIC - World Soil Information, Wageningen, the Netherlands. See Annex 4." ;
    skos:topConceptOf glosis_proc:totalCarbonateEquivalentProcedure .

glosis_proc:totalCarbonateEquivalentProcedure-CaCO3_calcul-tc-oc a glosis_proc:TotalCarbonateEquivalentProcedure,
        skos:Concept ;
    skos:definition "Indirect estimate: inorganic carbon divided by 0.12 (computed as total carbon minus organic carbon)" ;
    skos:inScheme glosis_proc:totalCarbonateEquivalentProcedure ;
    skos:notation "CaCO3_calcul-tc-oc" ;
    skos:prefLabel "CaCO3_calcul-tc-oc"@en ;
    skos:scopeNote <https://www.isric.org/sites/default/files/isric_report_2014_01.pdf>,
        "Leenaars J.G.B., A.J.M. van Oostrum and M. Ruiperez Gonzalez, 2014. Africa Soil Profiles Database, Version 1.2. A compilation of georeferenced and standardised legacy soil profile data for Sub-Saharan Africa (with dataset). ISRIC Report 2014/01. Africa Soil Information Service (AfSIS) project and ISRIC - World Soil Information, Wageningen, the Netherlands. See Annex 4." ;
    skos:topConceptOf glosis_proc:totalCarbonateEquivalentProcedure .

glosis_proc:totalElementsProcedure-Total_h2so4 a glosis_proc:TotalElementsProcedure,
        skos:Concept ;
    skos:definition "Total P-/- colorimetric in H2SO4-Se-Salicylic acid digest( sulfuric acid) Particularly used for Total P." ;
    skos:inScheme glosis_proc:totalElementsProcedure ;
    skos:notation "Total_h2so4" ;
    skos:prefLabel "Total_h2so4"@en ;
    skos:scopeNote <https://www.isric.org/sites/default/files/isric_report_2014_01.pdf>,
        "Leenaars J.G.B., A.J.M. van Oostrum and M. Ruiperez Gonzalez, 2014. Africa Soil Profiles Database, Version 1.2. A compilation of georeferenced and standardised legacy soil profile data for Sub-Saharan Africa (with dataset). ISRIC Report 2014/01. Africa Soil Information Service (AfSIS) project and ISRIC - World Soil Information, Wageningen, the Netherlands. See Annex 4." ;
    skos:topConceptOf glosis_proc:totalElementsProcedure .

glosis_proc:totalElementsProcedure-Total_hcl a glosis_proc:TotalElementsProcedure,
        skos:Concept ;
    skos:definition "HCl extraction. Particularly used for Total P." ;
    skos:inScheme glosis_proc:totalElementsProcedure ;
    skos:notation "Total_hcl" ;
    skos:prefLabel "Total_hcl"@en ;
    skos:scopeNote <https://www.isric.org/sites/default/files/isric_report_2014_01.pdf>,
        "Leenaars J.G.B., A.J.M. van Oostrum and M. Ruiperez Gonzalez, 2014. Africa Soil Profiles Database, Version 1.2. A compilation of georeferenced and standardised legacy soil profile data for Sub-Saharan Africa (with dataset). ISRIC Report 2014/01. Africa Soil Information Service (AfSIS) project and ISRIC - World Soil Information, Wageningen, the Netherlands. See Annex 4." ;
    skos:topConceptOf glosis_proc:totalElementsProcedure .

glosis_proc:totalElementsProcedure-Total_hcl-aquaregia a glosis_proc:TotalElementsProcedure,
        skos:Concept ;
    skos:definition "Hydrocloric (HCl) extraction in nitric/perchloric acid mixture (totals) aqua regia" ;
    skos:inScheme glosis_proc:totalElementsProcedure ;
    skos:notation "Total_hcl-aquaregia" ;
    skos:prefLabel "Total_hcl-aquaregia"@en ;
    skos:scopeNote <https://www.isric.org/sites/default/files/isric_report_2014_01.pdf>,
        "Leenaars J.G.B., A.J.M. van Oostrum and M. Ruiperez Gonzalez, 2014. Africa Soil Profiles Database, Version 1.2. A compilation of georeferenced and standardised legacy soil profile data for Sub-Saharan Africa (with dataset). ISRIC Report 2014/01. Africa Soil Information Service (AfSIS) project and ISRIC - World Soil Information, Wageningen, the Netherlands. See Annex 4." ;
    skos:topConceptOf glosis_proc:totalElementsProcedure .

glosis_proc:totalElementsProcedure-Total_hclo4 a glosis_proc:TotalElementsProcedure,
        skos:Concept ;
    skos:definition "Perchloric acid percolation. Particularly used for Total P." ;
    skos:inScheme glosis_proc:totalElementsProcedure ;
    skos:notation "Total_hclo4" ;
    skos:prefLabel "Total_hclo4"@en ;
    skos:scopeNote <https://www.isric.org/sites/default/files/isric_report_2014_01.pdf>,
        "Leenaars J.G.B., A.J.M. van Oostrum and M. Ruiperez Gonzalez, 2014. Africa Soil Profiles Database, Version 1.2. A compilation of georeferenced and standardised legacy soil profile data for Sub-Saharan Africa (with dataset). ISRIC Report 2014/01. Africa Soil Information Service (AfSIS) project and ISRIC - World Soil Information, Wageningen, the Netherlands. See Annex 4." ;
    skos:topConceptOf glosis_proc:totalElementsProcedure .

glosis_proc:totalElementsProcedure-Total_hno3-aquafortis a glosis_proc:TotalElementsProcedure,
        skos:Concept ;
    skos:definition "Nitric acid attack. Particularly used for Total P." ;
    skos:inScheme glosis_proc:totalElementsProcedure ;
    skos:notation "Total_hno3-aquafortis" ;
    skos:prefLabel "Total_hno3-aquafortis"@en ;
    skos:scopeNote <https://www.isric.org/sites/default/files/isric_report_2014_01.pdf>,
        "Leenaars J.G.B., A.J.M. van Oostrum and M. Ruiperez Gonzalez, 2014. Africa Soil Profiles Database, Version 1.2. A compilation of georeferenced and standardised legacy soil profile data for Sub-Saharan Africa (with dataset). ISRIC Report 2014/01. Africa Soil Information Service (AfSIS) project and ISRIC - World Soil Information, Wageningen, the Netherlands. See Annex 4." ;
    skos:topConceptOf glosis_proc:totalElementsProcedure .

glosis_proc:totalElementsProcedure-Total_nh4-6mo7o24 a glosis_proc:TotalElementsProcedure,
        skos:Concept ;
    skos:definition "COLORIMETRIC VANADATE MOLYBDATE. Particularly used for Total P." ;
    skos:inScheme glosis_proc:totalElementsProcedure ;
    skos:notation "Total_nh4-6mo7o24" ;
    skos:prefLabel "Total_nh4-6mo7o24"@en ;
    skos:scopeNote <https://www.isric.org/sites/default/files/isric_report_2014_01.pdf>,
        "Leenaars J.G.B., A.J.M. van Oostrum and M. Ruiperez Gonzalez, 2014. Africa Soil Profiles Database, Version 1.2. A compilation of georeferenced and standardised legacy soil profile data for Sub-Saharan Africa (with dataset). ISRIC Report 2014/01. Africa Soil Information Service (AfSIS) project and ISRIC - World Soil Information, Wageningen, the Netherlands. See Annex 4." ;
    skos:topConceptOf glosis_proc:totalElementsProcedure .

glosis_proc:totalElementsProcedure-Total_tp03 a glosis_proc:TotalElementsProcedure,
        skos:Concept ;
    skos:definition "reagent of Baeyens. Precipitation in form of Phosphomolybdate. Particularly used for Total P." ;
    skos:inScheme glosis_proc:totalElementsProcedure ;
    skos:notation "Total_tp03" ;
    skos:prefLabel "Total_tp03"@en ;
    skos:scopeNote <https://www.isric.org/sites/default/files/isric_report_2014_01.pdf>,
        "Leenaars J.G.B., A.J.M. van Oostrum and M. Ruiperez Gonzalez, 2014. Africa Soil Profiles Database, Version 1.2. A compilation of georeferenced and standardised legacy soil profile data for Sub-Saharan Africa (with dataset). ISRIC Report 2014/01. Africa Soil Information Service (AfSIS) project and ISRIC - World Soil Information, Wageningen, the Netherlands. See Annex 4." ;
    skos:topConceptOf glosis_proc:totalElementsProcedure .

glosis_proc:totalElementsProcedure-Total_tp04 a glosis_proc:TotalElementsProcedure,
        skos:Concept ;
    skos:definition "acid fleischman. Particularly used for Total P." ;
    skos:inScheme glosis_proc:totalElementsProcedure ;
    skos:notation "Total_tp04" ;
    skos:prefLabel "Total_tp04"@en ;
    skos:scopeNote <https://www.isric.org/sites/default/files/isric_report_2014_01.pdf>,
        "Leenaars J.G.B., A.J.M. van Oostrum and M. Ruiperez Gonzalez, 2014. Africa Soil Profiles Database, Version 1.2. A compilation of georeferenced and standardised legacy soil profile data for Sub-Saharan Africa (with dataset). ISRIC Report 2014/01. Africa Soil Information Service (AfSIS) project and ISRIC - World Soil Information, Wageningen, the Netherlands. See Annex 4." ;
    skos:topConceptOf glosis_proc:totalElementsProcedure .

glosis_proc:totalElementsProcedure-Total_tp05 a glosis_proc:TotalElementsProcedure,
        skos:Concept ;
    skos:definition "8 M HCl extraction. Particularly used for Total P." ;
    skos:inScheme glosis_proc:totalElementsProcedure ;
    skos:notation "Total_tp05" ;
    skos:prefLabel "Total_tp05"@en ;
    skos:scopeNote <https://www.isric.org/sites/default/files/isric_report_2014_01.pdf>,
        "Leenaars J.G.B., A.J.M. van Oostrum and M. Ruiperez Gonzalez, 2014. Africa Soil Profiles Database, Version 1.2. A compilation of georeferenced and standardised legacy soil profile data for Sub-Saharan Africa (with dataset). ISRIC Report 2014/01. Africa Soil Information Service (AfSIS) project and ISRIC - World Soil Information, Wageningen, the Netherlands. See Annex 4." ;
    skos:topConceptOf glosis_proc:totalElementsProcedure .

glosis_proc:totalElementsProcedure-Total_tp06 a glosis_proc:TotalElementsProcedure,
        skos:Concept ;
    skos:definition "Molybdenum blue method, using ascorbic acid as reductant after heating of soil to 550 C and extraction with 6M sulphuric acid. Particularly used for Total P." ;
    skos:inScheme glosis_proc:totalElementsProcedure ;
    skos:notation "Total_tp06" ;
    skos:prefLabel "Total_tp06"@en ;
    skos:scopeNote <https://www.isric.org/sites/default/files/isric_report_2014_01.pdf>,
        "Leenaars J.G.B., A.J.M. van Oostrum and M. Ruiperez Gonzalez, 2014. Africa Soil Profiles Database, Version 1.2. A compilation of georeferenced and standardised legacy soil profile data for Sub-Saharan Africa (with dataset). ISRIC Report 2014/01. Africa Soil Information Service (AfSIS) project and ISRIC - World Soil Information, Wageningen, the Netherlands. See Annex 4." ;
    skos:topConceptOf glosis_proc:totalElementsProcedure .

glosis_proc:totalElementsProcedure-Total_tp07 a glosis_proc:TotalElementsProcedure,
        skos:Concept ;
    skos:definition "1:1 H2SO4 : HNO3. Particularly used for Total P." ;
    skos:inScheme glosis_proc:totalElementsProcedure ;
    skos:notation "Total_tp07" ;
    skos:prefLabel "Total_tp07"@en ;
    skos:scopeNote <https://www.isric.org/sites/default/files/isric_report_2014_01.pdf>,
        "Leenaars J.G.B., A.J.M. van Oostrum and M. Ruiperez Gonzalez, 2014. Africa Soil Profiles Database, Version 1.2. A compilation of georeferenced and standardised legacy soil profile data for Sub-Saharan Africa (with dataset). ISRIC Report 2014/01. Africa Soil Information Service (AfSIS) project and ISRIC - World Soil Information, Wageningen, the Netherlands. See Annex 4." ;
    skos:topConceptOf glosis_proc:totalElementsProcedure .

glosis_proc:totalElementsProcedure-Total_tp08 a glosis_proc:TotalElementsProcedure,
        skos:Concept ;
    skos:definition "After Nitric acid attack (boiling with HNO3), colometric determination (method of Duval).. Particularly used for Total P." ;
    skos:inScheme glosis_proc:totalElementsProcedure ;
    skos:notation "Total_tp08" ;
    skos:prefLabel "Total_tp08"@en ;
    skos:scopeNote <https://www.isric.org/sites/default/files/isric_report_2014_01.pdf>,
        "Leenaars J.G.B., A.J.M. van Oostrum and M. Ruiperez Gonzalez, 2014. Africa Soil Profiles Database, Version 1.2. A compilation of georeferenced and standardised legacy soil profile data for Sub-Saharan Africa (with dataset). ISRIC Report 2014/01. Africa Soil Information Service (AfSIS) project and ISRIC - World Soil Information, Wageningen, the Netherlands. See Annex 4." ;
    skos:topConceptOf glosis_proc:totalElementsProcedure .

glosis_proc:totalElementsProcedure-Total_tp09 a glosis_proc:TotalElementsProcedure,
        skos:Concept ;
    skos:definition "Walker and Adams, 1958. Particularly used for Total P." ;
    skos:inScheme glosis_proc:totalElementsProcedure ;
    skos:notation "Total_tp09" ;
    skos:prefLabel "Total_tp09"@en ;
    skos:scopeNote "WALKER, T. W., AND A. F. R. ADAMS. 1958. Studies on soil organic matter. I. Soil Sci. 85: 307-318. " ;
    skos:topConceptOf glosis_proc:totalElementsProcedure .

glosis_proc:totalElementsProcedure-Total_tp10 a glosis_proc:TotalElementsProcedure,
        skos:Concept ;
    skos:definition "Colorimetric, unspecified extract" ;
    skos:inScheme glosis_proc:totalElementsProcedure ;
    skos:notation "Total_tp10" ;
    skos:prefLabel "Total_tp10"@en ;
    skos:scopeNote <https://www.isric.org/sites/default/files/isric_report_2014_01.pdf>,
        "Leenaars J.G.B., A.J.M. van Oostrum and M. Ruiperez Gonzalez, 2014. Africa Soil Profiles Database, Version 1.2. A compilation of georeferenced and standardised legacy soil profile data for Sub-Saharan Africa (with dataset). ISRIC Report 2014/01. Africa Soil Information Service (AfSIS) project and ISRIC - World Soil Information, Wageningen, the Netherlands. See Annex 4." ;
    skos:topConceptOf glosis_proc:totalElementsProcedure .

glosis_proc:totalElementsProcedure-Total_unkn a glosis_proc:TotalElementsProcedure,
        skos:Concept ;
    skos:definition "Unspecified method" ;
    skos:inScheme glosis_proc:totalElementsProcedure ;
    skos:notation "Total_unkn" ;
    skos:prefLabel "Total_unk"@en ;
    skos:scopeNote <https://www.isric.org/sites/default/files/isric_report_2014_01.pdf>,
        "Leenaars J.G.B., A.J.M. van Oostrum and M. Ruiperez Gonzalez, 2014. Africa Soil Profiles Database, Version 1.2. A compilation of georeferenced and standardised legacy soil profile data for Sub-Saharan Africa (with dataset). ISRIC Report 2014/01. Africa Soil Information Service (AfSIS) project and ISRIC - World Soil Information, Wageningen, the Netherlands. See Annex 4." ;
    skos:topConceptOf glosis_proc:totalElementsProcedure .

glosis_proc:totalElementsProcedure-Total_xrd a glosis_proc:TotalElementsProcedure,
        skos:Concept ;
    skos:definition "XRD" ;
    skos:inScheme glosis_proc:totalElementsProcedure ;
    skos:notation "Total_xrd" ;
    skos:prefLabel "Total_xrd"@en ;
    skos:scopeNote <https://www.isric.org/sites/default/files/isric_report_2014_01.pdf>,
        "Leenaars J.G.B., A.J.M. van Oostrum and M. Ruiperez Gonzalez, 2014. Africa Soil Profiles Database, Version 1.2. A compilation of georeferenced and standardised legacy soil profile data for Sub-Saharan Africa (with dataset). ISRIC Report 2014/01. Africa Soil Information Service (AfSIS) project and ISRIC - World Soil Information, Wageningen, the Netherlands. See Annex 4." ;
    skos:topConceptOf glosis_proc:totalElementsProcedure .

glosis_proc:totalElementsProcedure-Total_xrf a glosis_proc:TotalElementsProcedure,
        skos:Concept ;
    skos:definition "XRF" ;
    skos:inScheme glosis_proc:totalElementsProcedure ;
    skos:notation "Total_xrf" ;
    skos:prefLabel "Total_xrf"@en ;
    skos:scopeNote <https://www.isric.org/sites/default/files/isric_report_2014_01.pdf>,
        "Leenaars J.G.B., A.J.M. van Oostrum and M. Ruiperez Gonzalez, 2014. Africa Soil Profiles Database, Version 1.2. A compilation of georeferenced and standardised legacy soil profile data for Sub-Saharan Africa (with dataset). ISRIC Report 2014/01. Africa Soil Information Service (AfSIS) project and ISRIC - World Soil Information, Wageningen, the Netherlands. See Annex 4." ;
    skos:topConceptOf glosis_proc:totalElementsProcedure .

glosis_proc:totalElementsProcedure-Total_xrf-p a glosis_proc:TotalElementsProcedure,
        skos:Concept ;
    skos:definition "PXRF" ;
    skos:inScheme glosis_proc:totalElementsProcedure ;
    skos:notation "Total_xrf-p" ;
    skos:prefLabel "Total_xrf-p"@en ;
    skos:scopeNote <https://www.isric.org/sites/default/files/isric_report_2014_01.pdf>,
        "Leenaars J.G.B., A.J.M. van Oostrum and M. Ruiperez Gonzalez, 2014. Africa Soil Profiles Database, Version 1.2. A compilation of georeferenced and standardised legacy soil profile data for Sub-Saharan Africa (with dataset). ISRIC Report 2014/01. Africa Soil Information Service (AfSIS) project and ISRIC - World Soil Information, Wageningen, the Netherlands. See Annex 4." ;
    skos:topConceptOf glosis_proc:totalElementsProcedure .

glosis_proc:totalElementsProcedure-Total_xtf-t a glosis_proc:TotalElementsProcedure,
        skos:Concept ;
    skos:definition "TXRF" ;
    skos:inScheme glosis_proc:totalElementsProcedure ;
    skos:notation "Total_xtf-t" ;
    skos:prefLabel "Total_xtf-t"@en ;
    skos:scopeNote <https://www.isric.org/sites/default/files/isric_report_2014_01.pdf>,
        "Leenaars J.G.B., A.J.M. van Oostrum and M. Ruiperez Gonzalez, 2014. Africa Soil Profiles Database, Version 1.2. A compilation of georeferenced and standardised legacy soil profile data for Sub-Saharan Africa (with dataset). ISRIC Report 2014/01. Africa Soil Information Service (AfSIS) project and ISRIC - World Soil Information, Wageningen, the Netherlands. See Annex 4." ;
    skos:topConceptOf glosis_proc:totalElementsProcedure .

