<?xml version="1.0"?>
<rdf:RDF xmlns="http://w3id.org/glosis/model/procedure#"
     xml:base="http://w3id.org/glosis/model/procedure"
     xmlns:owl="http://www.w3.org/2002/07/owl#"
     xmlns:rdf="http://www.w3.org/1999/02/22-rdf-syntax-ns#"
     xmlns:xml="http://www.w3.org/XML/1998/namespace"
     xmlns:xsd="http://www.w3.org/2001/XMLSchema#"
     xmlns:foaf="http://xmlns.com/foaf/0.1/"
     xmlns:rdfs="http://www.w3.org/2000/01/rdf-schema#"
     xmlns:skos="http://www.w3.org/2004/02/skos/core#"
     xmlns:terms="http://purl.org/dc/terms/"
     xmlns:schema="https://schema.org/">
    <owl:Ontology rdf:about="http://w3id.org/glosis/model/procedure">
        <owl:versionIRI rdf:resource="http://w3id.org/glosis/model/procedure/v1.5.1"/>
        <terms:creator rdf:resource="_:genid-nodeid-node1ilmc51d6x3"/>
        <terms:creator rdf:resource="_:genid-nodeid-node1ilmc51d6x5"/>
        <terms:creator rdf:nodeID="genid1"/>
        <terms:creator rdf:nodeID="genid3"/>
        <terms:creator rdf:nodeID="genid5"/>
        <terms:description xml:lang="en">This ontology represents the laboratory analysis procedures in GLOSIS, an extension to the Global Soil Information System (GloSIS) v1.0, edited by Tomas Reznik and Katharina Schleidt</terms:description>
        <terms:rights xml:lang="en">This ontology is distributed under Creative Commons Attribution 4.0 License - http://creativecommons.org/licenses/by/4.0</terms:rights>
        <terms:source xml:lang="en">Data model for the Global Soil Information System (GloSIS) v1.0, edited by Tomas Reznik and Katharina Schleidt and Africa Soil Profile Database</terms:source>
        <terms:title xml:lang="en">GLOSIS Procedures</terms:title>
        <rdfs:comment xml:lang="en">This module contains the code lists identifying laboratory processes employed to assess physio-chemical soil properties.</rdfs:comment>
        <owl:versionInfo>v1.5.1</owl:versionInfo>
    </owl:Ontology>
    <rdf:Description rdf:nodeID="genid1">
        <foaf:name>Bogusz Janiak</foaf:name>
        <schema:affiliation>
            <rdf:Description>
                <foaf:name>PSNC</foaf:name>
            </rdf:Description>
        </schema:affiliation>
    </rdf:Description>
    <rdf:Description rdf:nodeID="genid3">
        <rdfs:seeAlso rdf:resource="http://orcid.org/0000-0003-4289-4922"/>
        <foaf:name>Raul Palma</foaf:name>
        <schema:affiliation>
            <rdf:Description>
                <foaf:name>PSNC</foaf:name>
            </rdf:Description>
        </schema:affiliation>
    </rdf:Description>
    <rdf:Description rdf:nodeID="genid5">
        <rdfs:seeAlso rdf:resource="http://orcid.org/0000-0002-5851-2071"/>
        <foaf:name>Luís Moreira de Sousa</foaf:name>
        <schema:affiliation>
            <rdf:Description>
                <foaf:name>Técnico ULisboa</foaf:name>
            </rdf:Description>
        </schema:affiliation>
    </rdf:Description>
    


    <!-- 
    ///////////////////////////////////////////////////////////////////////////////////////
    //
    // Annotation properties
    //
    ///////////////////////////////////////////////////////////////////////////////////////
     -->


    


    <!-- http://purl.org/dc/terms/creator -->


    <owl:AnnotationProperty rdf:about="http://purl.org/dc/terms/creator"/>
    


    <!-- http://purl.org/dc/terms/description -->


    <owl:AnnotationProperty rdf:about="http://purl.org/dc/terms/description"/>
    


    <!-- http://purl.org/dc/terms/rights -->


    <owl:AnnotationProperty rdf:about="http://purl.org/dc/terms/rights"/>
    


    <!-- http://purl.org/dc/terms/source -->


    <owl:AnnotationProperty rdf:about="http://purl.org/dc/terms/source"/>
    


    <!-- http://purl.org/dc/terms/title -->


    <owl:AnnotationProperty rdf:about="http://purl.org/dc/terms/title"/>
    


    <!-- http://www.w3.org/2004/02/skos/core#broader -->


    <owl:AnnotationProperty rdf:about="http://www.w3.org/2004/02/skos/core#broader"/>
    


    <!-- http://www.w3.org/2004/02/skos/core#definition -->


    <owl:AnnotationProperty rdf:about="http://www.w3.org/2004/02/skos/core#definition"/>
    


    <!-- http://www.w3.org/2004/02/skos/core#inScheme -->


    <owl:AnnotationProperty rdf:about="http://www.w3.org/2004/02/skos/core#inScheme"/>
    


    <!-- http://www.w3.org/2004/02/skos/core#narrower -->


    <owl:AnnotationProperty rdf:about="http://www.w3.org/2004/02/skos/core#narrower"/>
    


    <!-- http://www.w3.org/2004/02/skos/core#notation -->


    <owl:AnnotationProperty rdf:about="http://www.w3.org/2004/02/skos/core#notation"/>
    


    <!-- http://www.w3.org/2004/02/skos/core#note -->


    <owl:AnnotationProperty rdf:about="http://www.w3.org/2004/02/skos/core#note"/>
    


    <!-- http://www.w3.org/2004/02/skos/core#prefLabel -->


    <owl:AnnotationProperty rdf:about="http://www.w3.org/2004/02/skos/core#prefLabel"/>
    


    <!-- http://www.w3.org/2004/02/skos/core#scopeNote -->


    <owl:AnnotationProperty rdf:about="http://www.w3.org/2004/02/skos/core#scopeNote"/>
    


    <!-- http://www.w3.org/2004/02/skos/core#topConceptOf -->


    <owl:AnnotationProperty rdf:about="http://www.w3.org/2004/02/skos/core#topConceptOf"/>
    


    <!-- http://xmlns.com/foaf/0.1/name -->


    <owl:AnnotationProperty rdf:about="http://xmlns.com/foaf/0.1/name"/>
    


    <!-- https://schema.org/affiliation -->


    <owl:AnnotationProperty rdf:about="https://schema.org/affiliation"/>
    


    <!-- 
    ///////////////////////////////////////////////////////////////////////////////////////
    //
    // Classes
    //
    ///////////////////////////////////////////////////////////////////////////////////////
     -->


    


    <!-- http://w3id.org/glosis/model/procedure/AcidityExchangeableProcedure -->


    <owl:Class rdf:about="http://w3id.org/glosis/model/procedure/AcidityExchangeableProcedure">
        <owl:equivalentClass>
            <owl:Class>
                <owl:oneOf rdf:parseType="Collection">
                    <rdf:Description rdf:about="http://w3id.org/glosis/model/procedure/acidityExchangeableProcedure-ExchAcid_ph0-kcl1m"/>
                    <rdf:Description rdf:about="http://w3id.org/glosis/model/procedure/acidityExchangeableProcedure-ExchAcid_ph0-nh4cl"/>
                    <rdf:Description rdf:about="http://w3id.org/glosis/model/procedure/acidityExchangeableProcedure-ExchAcid_ph0-unkn"/>
                    <rdf:Description rdf:about="http://w3id.org/glosis/model/procedure/acidityExchangeableProcedure-ExchAcid_ph7-caoac"/>
                    <rdf:Description rdf:about="http://w3id.org/glosis/model/procedure/acidityExchangeableProcedure-ExchAcid_ph7-unkn"/>
                    <rdf:Description rdf:about="http://w3id.org/glosis/model/procedure/acidityExchangeableProcedure-ExchAcid_ph8-bacl2tea"/>
                    <rdf:Description rdf:about="http://w3id.org/glosis/model/procedure/acidityExchangeableProcedure-ExchAcid_ph8-unkn"/>
                </owl:oneOf>
            </owl:Class>
        </owl:equivalentClass>
        <rdfs:subClassOf rdf:resource="http://www.w3.org/2004/02/skos/core#Concept"/>
        <rdfs:subClassOf rdf:resource="http://www.w3.org/ns/sosa/Procedure"/>
        <rdfs:comment xml:lang="en">This code list provides analysis procedures for AcidityExchangeable.</rdfs:comment>
        <rdfs:label xml:lang="en">Procedures for AcidityExchangeable - codelist class</rdfs:label>
        <rdfs:seeAlso rdf:resource="http://w3id.org/glosis/model/procedure/acidityExchangeableProcedure"/>
    </owl:Class>
    


    <!-- http://w3id.org/glosis/model/procedure/AvailableWaterHoldingCapacityProcedure -->


    <owl:Class rdf:about="http://w3id.org/glosis/model/procedure/AvailableWaterHoldingCapacityProcedure">
        <owl:equivalentClass>
            <owl:Class>
                <owl:oneOf rdf:parseType="Collection">
                    <rdf:Description rdf:about="http://w3id.org/glosis/model/procedure/availableWaterHoldingCapacityProcedure-PAWHC_calcul-fc100wp"/>
                    <rdf:Description rdf:about="http://w3id.org/glosis/model/procedure/availableWaterHoldingCapacityProcedure-PAWHC_calcul-fc200wp"/>
                    <rdf:Description rdf:about="http://w3id.org/glosis/model/procedure/availableWaterHoldingCapacityProcedure-PAWHC_calcul-fc300wp"/>
                </owl:oneOf>
            </owl:Class>
        </owl:equivalentClass>
        <rdfs:subClassOf rdf:resource="http://www.w3.org/2004/02/skos/core#Concept"/>
        <rdfs:subClassOf rdf:resource="http://www.w3.org/ns/sosa/Procedure"/>
        <rdfs:comment xml:lang="en">This code list provides analysis procedures for AvailableWaterHoldingCapacity.</rdfs:comment>
        <rdfs:label xml:lang="en">Procedures for AvailableWaterHoldingCapacity - codelist class</rdfs:label>
        <rdfs:seeAlso rdf:resource="http://w3id.org/glosis/model/procedure/availableWaterHoldingCapacityProcedure"/>
    </owl:Class>
    


    <!-- http://w3id.org/glosis/model/procedure/BaseSaturationProcedure -->


    <owl:Class rdf:about="http://w3id.org/glosis/model/procedure/BaseSaturationProcedure">
        <owl:equivalentClass>
            <owl:Class>
                <owl:oneOf rdf:parseType="Collection">
                    <rdf:Description rdf:about="http://w3id.org/glosis/model/procedure/baseSaturationProcedure-BSat_calcul-cec"/>
                    <rdf:Description rdf:about="http://w3id.org/glosis/model/procedure/baseSaturationProcedure-BSat_calcul-ecec"/>
                </owl:oneOf>
            </owl:Class>
        </owl:equivalentClass>
        <rdfs:subClassOf rdf:resource="http://www.w3.org/2004/02/skos/core#Concept"/>
        <rdfs:subClassOf rdf:resource="http://www.w3.org/ns/sosa/Procedure"/>
        <rdfs:comment xml:lang="en">This code list provides analysis procedures for BaseSaturation.</rdfs:comment>
        <rdfs:label xml:lang="en">Procedures for BaseSaturation - codelist class</rdfs:label>
        <rdfs:seeAlso rdf:resource="http://w3id.org/glosis/model/procedure/baseSaturationProcedure"/>
    </owl:Class>
    


    <!-- http://w3id.org/glosis/model/procedure/BulkDensityFineEarthProcedure -->


    <owl:Class rdf:about="http://w3id.org/glosis/model/procedure/BulkDensityFineEarthProcedure">
        <owl:equivalentClass>
            <owl:Class>
                <owl:oneOf rdf:parseType="Collection">
                    <rdf:Description rdf:about="http://w3id.org/glosis/model/procedure/bulkDensityFineEarthProcedure-BlkDensF_fe-cl-fc"/>
                    <rdf:Description rdf:about="http://w3id.org/glosis/model/procedure/bulkDensityFineEarthProcedure-BlkDensF_fe-cl-od"/>
                    <rdf:Description rdf:about="http://w3id.org/glosis/model/procedure/bulkDensityFineEarthProcedure-BlkDensF_fe-cl-unkn"/>
                    <rdf:Description rdf:about="http://w3id.org/glosis/model/procedure/bulkDensityFineEarthProcedure-BlkDensF_fe-co-fc"/>
                    <rdf:Description rdf:about="http://w3id.org/glosis/model/procedure/bulkDensityFineEarthProcedure-BlkDensF_fe-co-od"/>
                    <rdf:Description rdf:about="http://w3id.org/glosis/model/procedure/bulkDensityFineEarthProcedure-BlkDensF_fe-co-unkn"/>
                    <rdf:Description rdf:about="http://w3id.org/glosis/model/procedure/bulkDensityFineEarthProcedure-BlkDensF_fe-rpl-unkn"/>
                    <rdf:Description rdf:about="http://w3id.org/glosis/model/procedure/bulkDensityFineEarthProcedure-BlkDensF_fe-unkn"/>
                    <rdf:Description rdf:about="http://w3id.org/glosis/model/procedure/bulkDensityFineEarthProcedure-BlkDensF_fe-unkn-fc"/>
                    <rdf:Description rdf:about="http://w3id.org/glosis/model/procedure/bulkDensityFineEarthProcedure-BlkDensF_fe-unkn-od"/>
                </owl:oneOf>
            </owl:Class>
        </owl:equivalentClass>
        <rdfs:subClassOf rdf:resource="http://www.w3.org/2004/02/skos/core#Concept"/>
        <rdfs:subClassOf rdf:resource="http://www.w3.org/ns/sosa/Procedure"/>
        <rdfs:comment xml:lang="en">This code list provides analysis procedures for BulkDensityFineEarth.</rdfs:comment>
        <rdfs:label xml:lang="en">Procedures for BulkDensityFineEarth - codelist class</rdfs:label>
        <rdfs:seeAlso rdf:resource="http://w3id.org/glosis/model/procedure/bulkDensityFineEarthProcedure"/>
    </owl:Class>
    


    <!-- http://w3id.org/glosis/model/procedure/BulkDensityWholeSoilProcedure -->


    <owl:Class rdf:about="http://w3id.org/glosis/model/procedure/BulkDensityWholeSoilProcedure">
        <owl:equivalentClass>
            <owl:Class>
                <owl:oneOf rdf:parseType="Collection">
                    <rdf:Description rdf:about="http://w3id.org/glosis/model/procedure/bulkDensityWholeSoilProcedure-BlkDensW_we-cl-fc"/>
                    <rdf:Description rdf:about="http://w3id.org/glosis/model/procedure/bulkDensityWholeSoilProcedure-BlkDensW_we-cl-od"/>
                    <rdf:Description rdf:about="http://w3id.org/glosis/model/procedure/bulkDensityWholeSoilProcedure-BlkDensW_we-cl-unkn"/>
                    <rdf:Description rdf:about="http://w3id.org/glosis/model/procedure/bulkDensityWholeSoilProcedure-BlkDensW_we-co-fc"/>
                    <rdf:Description rdf:about="http://w3id.org/glosis/model/procedure/bulkDensityWholeSoilProcedure-BlkDensW_we-co-od"/>
                    <rdf:Description rdf:about="http://w3id.org/glosis/model/procedure/bulkDensityWholeSoilProcedure-BlkDensW_we-co-unkn"/>
                    <rdf:Description rdf:about="http://w3id.org/glosis/model/procedure/bulkDensityWholeSoilProcedure-BlkDensW_we-rpl-unkn"/>
                    <rdf:Description rdf:about="http://w3id.org/glosis/model/procedure/bulkDensityWholeSoilProcedure-BlkDensW_we-unkn"/>
                </owl:oneOf>
            </owl:Class>
        </owl:equivalentClass>
        <rdfs:subClassOf rdf:resource="http://www.w3.org/2004/02/skos/core#Concept"/>
        <rdfs:subClassOf rdf:resource="http://www.w3.org/ns/sosa/Procedure"/>
        <rdfs:comment xml:lang="en">This code list provides analysis procedures for BulkDensityWholeSoil.</rdfs:comment>
        <rdfs:label xml:lang="en">Procedures for BulkDensityWholeSoil - codelist class</rdfs:label>
        <rdfs:seeAlso rdf:resource="http://w3id.org/glosis/model/procedure/bulkDensityWholeSoilProcedure"/>
    </owl:Class>
    


    <!-- http://w3id.org/glosis/model/procedure/CarbonInorganicProcedure -->


    <owl:Class rdf:about="http://w3id.org/glosis/model/procedure/CarbonInorganicProcedure">
        <owl:equivalentClass>
            <owl:Class>
                <owl:oneOf rdf:parseType="Collection">
                    <rdf:Description rdf:about="http://w3id.org/glosis/model/procedure/carbonInorganicProcedure-InOrgC_calcul-caco3"/>
                    <rdf:Description rdf:about="http://w3id.org/glosis/model/procedure/carbonInorganicProcedure-InOrgC_calcul-tc-oc"/>
                </owl:oneOf>
            </owl:Class>
        </owl:equivalentClass>
        <rdfs:subClassOf rdf:resource="http://www.w3.org/2004/02/skos/core#Concept"/>
        <rdfs:subClassOf rdf:resource="http://www.w3.org/ns/sosa/Procedure"/>
        <rdfs:comment xml:lang="en">This code list provides analysis procedures for CarbonInorganic.</rdfs:comment>
        <rdfs:label xml:lang="en">Procedures for CarbonInorganic - codelist class</rdfs:label>
        <rdfs:seeAlso rdf:resource="http://w3id.org/glosis/model/procedure/carbonInorganicProcedure"/>
    </owl:Class>
    


    <!-- http://w3id.org/glosis/model/procedure/CarbonOrganicProcedure -->


    <owl:Class rdf:about="http://w3id.org/glosis/model/procedure/CarbonOrganicProcedure">
        <owl:equivalentClass>
            <owl:Class>
                <owl:oneOf rdf:parseType="Collection">
                    <rdf:Description rdf:about="http://w3id.org/glosis/model/procedure/carbonOrganicProcedure-OrgC_acid-dc"/>
                    <rdf:Description rdf:about="http://w3id.org/glosis/model/procedure/carbonOrganicProcedure-OrgC_acid-dc-ht"/>
                    <rdf:Description rdf:about="http://w3id.org/glosis/model/procedure/carbonOrganicProcedure-OrgC_acid-dc-ht-analyser"/>
                    <rdf:Description rdf:about="http://w3id.org/glosis/model/procedure/carbonOrganicProcedure-OrgC_acid-dc-lt"/>
                    <rdf:Description rdf:about="http://w3id.org/glosis/model/procedure/carbonOrganicProcedure-OrgC_acid-dc-lt-loi"/>
                    <rdf:Description rdf:about="http://w3id.org/glosis/model/procedure/carbonOrganicProcedure-OrgC_acid-dc-mt"/>
                    <rdf:Description rdf:about="http://w3id.org/glosis/model/procedure/carbonOrganicProcedure-OrgC_acid-dc-spec"/>
                    <rdf:Description rdf:about="http://w3id.org/glosis/model/procedure/carbonOrganicProcedure-OrgC_calcul-tc-ic"/>
                    <rdf:Description rdf:about="http://w3id.org/glosis/model/procedure/carbonOrganicProcedure-OrgC_dc"/>
                    <rdf:Description rdf:about="http://w3id.org/glosis/model/procedure/carbonOrganicProcedure-OrgC_dc-ht"/>
                    <rdf:Description rdf:about="http://w3id.org/glosis/model/procedure/carbonOrganicProcedure-OrgC_dc-ht-analyser"/>
                    <rdf:Description rdf:about="http://w3id.org/glosis/model/procedure/carbonOrganicProcedure-OrgC_dc-lt"/>
                    <rdf:Description rdf:about="http://w3id.org/glosis/model/procedure/carbonOrganicProcedure-OrgC_dc-lt-loi"/>
                    <rdf:Description rdf:about="http://w3id.org/glosis/model/procedure/carbonOrganicProcedure-OrgC_dc-mt"/>
                    <rdf:Description rdf:about="http://w3id.org/glosis/model/procedure/carbonOrganicProcedure-OrgC_dc-spec"/>
                    <rdf:Description rdf:about="http://w3id.org/glosis/model/procedure/carbonOrganicProcedure-OrgC_wc"/>
                    <rdf:Description rdf:about="http://w3id.org/glosis/model/procedure/carbonOrganicProcedure-OrgC_wc-cro3-jackson"/>
                    <rdf:Description rdf:about="http://w3id.org/glosis/model/procedure/carbonOrganicProcedure-OrgC_wc-cro3-kalembra"/>
                    <rdf:Description rdf:about="http://w3id.org/glosis/model/procedure/carbonOrganicProcedure-OrgC_wc-cro3-knopp"/>
                    <rdf:Description rdf:about="http://w3id.org/glosis/model/procedure/carbonOrganicProcedure-OrgC_wc-cro3-kurmies"/>
                    <rdf:Description rdf:about="http://w3id.org/glosis/model/procedure/carbonOrganicProcedure-OrgC_wc-cro3-nelson"/>
                    <rdf:Description rdf:about="http://w3id.org/glosis/model/procedure/carbonOrganicProcedure-OrgC_wc-cro3-nrcs6a1c"/>
                    <rdf:Description rdf:about="http://w3id.org/glosis/model/procedure/carbonOrganicProcedure-OrgC_wc-cro3-tiurin"/>
                    <rdf:Description rdf:about="http://w3id.org/glosis/model/procedure/carbonOrganicProcedure-OrgC_wc-cro3-walkleyblack"/>
                </owl:oneOf>
            </owl:Class>
        </owl:equivalentClass>
        <rdfs:subClassOf rdf:resource="http://www.w3.org/2004/02/skos/core#Concept"/>
        <rdfs:subClassOf rdf:resource="http://www.w3.org/ns/sosa/Procedure"/>
        <rdfs:comment xml:lang="en">This code list provides analysis procedures for CarbonOrganic.</rdfs:comment>
        <rdfs:label xml:lang="en">Procedures for CarbonOrganic - codelist class</rdfs:label>
        <rdfs:seeAlso rdf:resource="http://w3id.org/glosis/model/procedure/carbonOrganicProcedure"/>
    </owl:Class>
    


    <!-- http://w3id.org/glosis/model/procedure/CarbonTotalProcedure -->


    <owl:Class rdf:about="http://w3id.org/glosis/model/procedure/CarbonTotalProcedure">
        <owl:equivalentClass>
            <owl:Class>
                <owl:oneOf rdf:parseType="Collection">
                    <rdf:Description rdf:about="http://w3id.org/glosis/model/procedure/carbonTotalProcedure-TotC_calcul-ic-oc"/>
                    <rdf:Description rdf:about="http://w3id.org/glosis/model/procedure/carbonTotalProcedure-TotC_dc-ht"/>
                    <rdf:Description rdf:about="http://w3id.org/glosis/model/procedure/carbonTotalProcedure-TotC_dc-ht-analyser"/>
                    <rdf:Description rdf:about="http://w3id.org/glosis/model/procedure/carbonTotalProcedure-TotC_dc-ht-spec"/>
                    <rdf:Description rdf:about="http://w3id.org/glosis/model/procedure/carbonTotalProcedure-TotC_dc-mt"/>
                </owl:oneOf>
            </owl:Class>
        </owl:equivalentClass>
        <rdfs:subClassOf rdf:resource="http://www.w3.org/2004/02/skos/core#Concept"/>
        <rdfs:subClassOf rdf:resource="http://www.w3.org/ns/sosa/Procedure"/>
        <rdfs:comment xml:lang="en">This code list provides analysis procedures for CarbonTotal.</rdfs:comment>
        <rdfs:label xml:lang="en">Procedures for CarbonTotal - codelist class</rdfs:label>
        <rdfs:seeAlso rdf:resource="http://w3id.org/glosis/model/procedure/carbonTotalProcedure"/>
    </owl:Class>
    


    <!-- http://w3id.org/glosis/model/procedure/CationExchangeCapacitySoilProcedure -->


    <owl:Class rdf:about="http://w3id.org/glosis/model/procedure/CationExchangeCapacitySoilProcedure">
        <owl:equivalentClass>
            <owl:Class>
                <owl:oneOf rdf:parseType="Collection">
                    <rdf:Description rdf:about="http://w3id.org/glosis/model/procedure/cationExchangeCapacitySoilProcedure-CEC_ph-unkn-cacl2"/>
                    <rdf:Description rdf:about="http://w3id.org/glosis/model/procedure/cationExchangeCapacitySoilProcedure-CEC_ph-unkn-lioac"/>
                    <rdf:Description rdf:about="http://w3id.org/glosis/model/procedure/cationExchangeCapacitySoilProcedure-CEC_ph-unkn-m3"/>
                    <rdf:Description rdf:about="http://w3id.org/glosis/model/procedure/cationExchangeCapacitySoilProcedure-CEC_ph0-ag-thioura"/>
                    <rdf:Description rdf:about="http://w3id.org/glosis/model/procedure/cationExchangeCapacitySoilProcedure-CEC_ph0-bacl2"/>
                    <rdf:Description rdf:about="http://w3id.org/glosis/model/procedure/cationExchangeCapacitySoilProcedure-CEC_ph0-cohex"/>
                    <rdf:Description rdf:about="http://w3id.org/glosis/model/procedure/cationExchangeCapacitySoilProcedure-CEC_ph0-kcl"/>
                    <rdf:Description rdf:about="http://w3id.org/glosis/model/procedure/cationExchangeCapacitySoilProcedure-CEC_ph0-nh4cl"/>
                    <rdf:Description rdf:about="http://w3id.org/glosis/model/procedure/cationExchangeCapacitySoilProcedure-CEC_ph0-nh4oac"/>
                    <rdf:Description rdf:about="http://w3id.org/glosis/model/procedure/cationExchangeCapacitySoilProcedure-CEC_ph0-unkn"/>
                    <rdf:Description rdf:about="http://w3id.org/glosis/model/procedure/cationExchangeCapacitySoilProcedure-CEC_ph7-edta"/>
                    <rdf:Description rdf:about="http://w3id.org/glosis/model/procedure/cationExchangeCapacitySoilProcedure-CEC_ph7-nh4oac"/>
                    <rdf:Description rdf:about="http://w3id.org/glosis/model/procedure/cationExchangeCapacitySoilProcedure-CEC_ph7-unkn"/>
                    <rdf:Description rdf:about="http://w3id.org/glosis/model/procedure/cationExchangeCapacitySoilProcedure-CEC_ph8-bacl2tea"/>
                    <rdf:Description rdf:about="http://w3id.org/glosis/model/procedure/cationExchangeCapacitySoilProcedure-CEC_ph8-baoac"/>
                    <rdf:Description rdf:about="http://w3id.org/glosis/model/procedure/cationExchangeCapacitySoilProcedure-CEC_ph8-licl2tea"/>
                    <rdf:Description rdf:about="http://w3id.org/glosis/model/procedure/cationExchangeCapacitySoilProcedure-CEC_ph8-naoac"/>
                    <rdf:Description rdf:about="http://w3id.org/glosis/model/procedure/cationExchangeCapacitySoilProcedure-CEC_ph8-nh4oac"/>
                    <rdf:Description rdf:about="http://w3id.org/glosis/model/procedure/cationExchangeCapacitySoilProcedure-CEC_ph8-unkn"/>
                </owl:oneOf>
            </owl:Class>
        </owl:equivalentClass>
        <rdfs:subClassOf rdf:resource="http://www.w3.org/2004/02/skos/core#Concept"/>
        <rdfs:subClassOf rdf:resource="http://www.w3.org/ns/sosa/Procedure"/>
        <rdfs:comment xml:lang="en">This code list provides analysis procedures for CationExchangeCapacitySoil.</rdfs:comment>
        <rdfs:label xml:lang="en">Procedures for CationExchangeCapacitySoil - codelist class</rdfs:label>
        <rdfs:seeAlso rdf:resource="http://w3id.org/glosis/model/procedure/cationExchangeCapacitySoilProcedure"/>
    </owl:Class>
    


    <!-- http://w3id.org/glosis/model/procedure/CoarseFragmentsProcedure -->


    <owl:Class rdf:about="http://w3id.org/glosis/model/procedure/CoarseFragmentsProcedure">
        <owl:equivalentClass>
            <owl:Class>
                <owl:oneOf rdf:parseType="Collection">
                    <rdf:Description rdf:about="http://w3id.org/glosis/model/procedure/coarseFragmentsProcedure-CrsFrg_fld"/>
                    <rdf:Description rdf:about="http://w3id.org/glosis/model/procedure/coarseFragmentsProcedure-CrsFrg_fldcls"/>
                    <rdf:Description rdf:about="http://w3id.org/glosis/model/procedure/coarseFragmentsProcedure-CrsFrg_lab"/>
                </owl:oneOf>
            </owl:Class>
        </owl:equivalentClass>
        <rdfs:subClassOf rdf:resource="http://www.w3.org/2004/02/skos/core#Concept"/>
        <rdfs:subClassOf rdf:resource="http://www.w3.org/ns/sosa/Procedure"/>
        <rdfs:comment xml:lang="en">This code list provides analysis procedures for CoarseFragments.</rdfs:comment>
        <rdfs:label xml:lang="en">Procedures for CoarseFragments - codelist class</rdfs:label>
        <rdfs:seeAlso rdf:resource="http://w3id.org/glosis/model/procedure/coarseFragmentsProcedure"/>
    </owl:Class>
    


    <!-- http://w3id.org/glosis/model/procedure/EffectiveCecProcedure -->


    <owl:Class rdf:about="http://w3id.org/glosis/model/procedure/EffectiveCecProcedure">
        <owl:equivalentClass>
            <owl:Class>
                <owl:oneOf rdf:parseType="Collection">
                    <rdf:Description rdf:about="http://w3id.org/glosis/model/procedure/effectiveCecProcedure-EffCEC_calcul-b"/>
                    <rdf:Description rdf:about="http://w3id.org/glosis/model/procedure/effectiveCecProcedure-EffCEC_calcul-ba"/>
                </owl:oneOf>
            </owl:Class>
        </owl:equivalentClass>
        <rdfs:subClassOf rdf:resource="http://www.w3.org/2004/02/skos/core#Concept"/>
        <rdfs:subClassOf rdf:resource="http://www.w3.org/ns/sosa/Procedure"/>
        <rdfs:comment xml:lang="en">This code list provides analysis procedures for EffectiveCec.</rdfs:comment>
        <rdfs:label xml:lang="en">Procedures for EffectiveCec - codelist class</rdfs:label>
        <rdfs:seeAlso rdf:resource="http://w3id.org/glosis/model/procedure/effectiveCecProcedure"/>
    </owl:Class>
    


    <!-- http://w3id.org/glosis/model/procedure/ElectricalConductivityProcedure -->


    <owl:Class rdf:about="http://w3id.org/glosis/model/procedure/ElectricalConductivityProcedure">
        <owl:equivalentClass>
            <owl:Class>
                <owl:oneOf rdf:parseType="Collection">
                    <rdf:Description rdf:about="http://w3id.org/glosis/model/procedure/electricalConductivityProcedure-EC_ratio1-1"/>
                    <rdf:Description rdf:about="http://w3id.org/glosis/model/procedure/electricalConductivityProcedure-EC_ratio1-10"/>
                    <rdf:Description rdf:about="http://w3id.org/glosis/model/procedure/electricalConductivityProcedure-EC_ratio1-2"/>
                    <rdf:Description rdf:about="http://w3id.org/glosis/model/procedure/electricalConductivityProcedure-EC_ratio1-2.5"/>
                    <rdf:Description rdf:about="http://w3id.org/glosis/model/procedure/electricalConductivityProcedure-EC_ratio1-5"/>
                    <rdf:Description rdf:about="http://w3id.org/glosis/model/procedure/electricalConductivityProcedure-ECe_sat"/>
                </owl:oneOf>
            </owl:Class>
        </owl:equivalentClass>
        <rdfs:subClassOf rdf:resource="http://www.w3.org/2004/02/skos/core#Concept"/>
        <rdfs:subClassOf rdf:resource="http://www.w3.org/ns/sosa/Procedure"/>
        <rdfs:comment xml:lang="en">This code list provides analysis procedures for ElectricalConductivity.</rdfs:comment>
        <rdfs:label xml:lang="en">Procedures for ElectricalConductivity - codelist class</rdfs:label>
        <rdfs:seeAlso rdf:resource="http://w3id.org/glosis/model/procedure/electricalConductivityProcedure"/>
    </owl:Class>
    


    <!-- http://w3id.org/glosis/model/procedure/ExchangeableBasesProcedure -->


    <owl:Class rdf:about="http://w3id.org/glosis/model/procedure/ExchangeableBasesProcedure">
        <owl:equivalentClass>
            <owl:Class>
                <owl:oneOf rdf:parseType="Collection">
                    <rdf:Description rdf:about="http://w3id.org/glosis/model/procedure/exchangeableBasesProcedure-ExchBases_ph-unkn-edta"/>
                    <rdf:Description rdf:about="http://w3id.org/glosis/model/procedure/exchangeableBasesProcedure-ExchBases_ph-unkn-m3"/>
                    <rdf:Description rdf:about="http://w3id.org/glosis/model/procedure/exchangeableBasesProcedure-ExchBases_ph-unkn-m3-spec"/>
                    <rdf:Description rdf:about="http://w3id.org/glosis/model/procedure/exchangeableBasesProcedure-ExchBases_ph0-cohex"/>
                    <rdf:Description rdf:about="http://w3id.org/glosis/model/procedure/exchangeableBasesProcedure-ExchBases_ph0-nh4cl"/>
                    <rdf:Description rdf:about="http://w3id.org/glosis/model/procedure/exchangeableBasesProcedure-ExchBases_ph7-nh4oac"/>
                    <rdf:Description rdf:about="http://w3id.org/glosis/model/procedure/exchangeableBasesProcedure-ExchBases_ph7-nh4oac-aas"/>
                    <rdf:Description rdf:about="http://w3id.org/glosis/model/procedure/exchangeableBasesProcedure-ExchBases_ph7-nh4oac-fp"/>
                    <rdf:Description rdf:about="http://w3id.org/glosis/model/procedure/exchangeableBasesProcedure-ExchBases_ph7-unkn"/>
                    <rdf:Description rdf:about="http://w3id.org/glosis/model/procedure/exchangeableBasesProcedure-ExchBases_ph8-bacl2tea"/>
                    <rdf:Description rdf:about="http://w3id.org/glosis/model/procedure/exchangeableBasesProcedure-ExchBases_ph8-unkn"/>
                </owl:oneOf>
            </owl:Class>
        </owl:equivalentClass>
        <rdfs:subClassOf rdf:resource="http://www.w3.org/2004/02/skos/core#Concept"/>
        <rdfs:subClassOf rdf:resource="http://www.w3.org/ns/sosa/Procedure"/>
        <rdfs:comment xml:lang="en">This code list provides analysis procedures for ExchangeableBases.</rdfs:comment>
        <rdfs:label xml:lang="en">Procedures for ExchangeableBases - codelist class</rdfs:label>
        <rdfs:seeAlso rdf:resource="http://w3id.org/glosis/model/procedure/exchangeableBasesProcedure"/>
    </owl:Class>
    


    <!-- http://w3id.org/glosis/model/procedure/ExtractableElementsProcedure -->


    <owl:Class rdf:about="http://w3id.org/glosis/model/procedure/ExtractableElementsProcedure">
        <owl:equivalentClass>
            <owl:Class>
                <owl:oneOf rdf:parseType="Collection">
                    <rdf:Description rdf:about="http://w3id.org/glosis/model/procedure/extractableElementsProcedure-Extr_ap14"/>
                    <rdf:Description rdf:about="http://w3id.org/glosis/model/procedure/extractableElementsProcedure-Extr_ap15"/>
                    <rdf:Description rdf:about="http://w3id.org/glosis/model/procedure/extractableElementsProcedure-Extr_ap20"/>
                    <rdf:Description rdf:about="http://w3id.org/glosis/model/procedure/extractableElementsProcedure-Extr_ap21"/>
                    <rdf:Description rdf:about="http://w3id.org/glosis/model/procedure/extractableElementsProcedure-Extr_c6h8o7-reeuwijk"/>
                    <rdf:Description rdf:about="http://w3id.org/glosis/model/procedure/extractableElementsProcedure-Extr_cacl2"/>
                    <rdf:Description rdf:about="http://w3id.org/glosis/model/procedure/extractableElementsProcedure-Extr_capo4"/>
                    <rdf:Description rdf:about="http://w3id.org/glosis/model/procedure/extractableElementsProcedure-Extr_dtpa"/>
                    <rdf:Description rdf:about="http://w3id.org/glosis/model/procedure/extractableElementsProcedure-Extr_edta"/>
                    <rdf:Description rdf:about="http://w3id.org/glosis/model/procedure/extractableElementsProcedure-Extr_h2so4-truog"/>
                    <rdf:Description rdf:about="http://w3id.org/glosis/model/procedure/extractableElementsProcedure-Extr_hcl-h2so4-nelson"/>
                    <rdf:Description rdf:about="http://w3id.org/glosis/model/procedure/extractableElementsProcedure-Extr_hcl-nh4f-bray1"/>
                    <rdf:Description rdf:about="http://w3id.org/glosis/model/procedure/extractableElementsProcedure-Extr_hcl-nh4f-bray2"/>
                    <rdf:Description rdf:about="http://w3id.org/glosis/model/procedure/extractableElementsProcedure-Extr_hcl-nh4f-kurtz-bray"/>
                    <rdf:Description rdf:about="http://w3id.org/glosis/model/procedure/extractableElementsProcedure-Extr_hno3"/>
                    <rdf:Description rdf:about="http://w3id.org/glosis/model/procedure/extractableElementsProcedure-Extr_hotwater"/>
                    <rdf:Description rdf:about="http://w3id.org/glosis/model/procedure/extractableElementsProcedure-Extr_m1"/>
                    <rdf:Description rdf:about="http://w3id.org/glosis/model/procedure/extractableElementsProcedure-Extr_m2"/>
                    <rdf:Description rdf:about="http://w3id.org/glosis/model/procedure/extractableElementsProcedure-Extr_m3"/>
                    <rdf:Description rdf:about="http://w3id.org/glosis/model/procedure/extractableElementsProcedure-Extr_m3-spec"/>
                    <rdf:Description rdf:about="http://w3id.org/glosis/model/procedure/extractableElementsProcedure-Extr_nahco3-olsen"/>
                    <rdf:Description rdf:about="http://w3id.org/glosis/model/procedure/extractableElementsProcedure-Extr_nahco3-olsen-dabin"/>
                    <rdf:Description rdf:about="http://w3id.org/glosis/model/procedure/extractableElementsProcedure-Extr_naoac-morgan"/>
                    <rdf:Description rdf:about="http://w3id.org/glosis/model/procedure/extractableElementsProcedure-Extr_nh4-co3-2-ambic1"/>
                    <rdf:Description rdf:about="http://w3id.org/glosis/model/procedure/extractableElementsProcedure-Extr_nh4ch3ch-oh-cooh-leuven"/>
                </owl:oneOf>
            </owl:Class>
        </owl:equivalentClass>
        <rdfs:subClassOf rdf:resource="http://www.w3.org/2004/02/skos/core#Concept"/>
        <rdfs:subClassOf rdf:resource="http://www.w3.org/ns/sosa/Procedure"/>
        <rdfs:comment xml:lang="en">This code list provides analysis procedures for ExtractableElements.</rdfs:comment>
        <rdfs:label xml:lang="en">Procedures for ExtractableElements - codelist class</rdfs:label>
        <rdfs:seeAlso rdf:resource="http://w3id.org/glosis/model/procedure/extractableElementsProcedure"/>
    </owl:Class>
    


    <!-- http://w3id.org/glosis/model/procedure/GypsumProcedure -->


    <owl:Class rdf:about="http://w3id.org/glosis/model/procedure/GypsumProcedure">
        <owl:equivalentClass>
            <owl:Class>
                <owl:oneOf rdf:parseType="Collection">
                    <rdf:Description rdf:about="http://w3id.org/glosis/model/procedure/gypsumProcedure-CaSO4_gy01"/>
                    <rdf:Description rdf:about="http://w3id.org/glosis/model/procedure/gypsumProcedure-CaSO4_gy02"/>
                    <rdf:Description rdf:about="http://w3id.org/glosis/model/procedure/gypsumProcedure-CaSO4_gy03"/>
                    <rdf:Description rdf:about="http://w3id.org/glosis/model/procedure/gypsumProcedure-CaSO4_gy04"/>
                    <rdf:Description rdf:about="http://w3id.org/glosis/model/procedure/gypsumProcedure-CaSO4_gy05"/>
                    <rdf:Description rdf:about="http://w3id.org/glosis/model/procedure/gypsumProcedure-CaSO4_gy06"/>
                    <rdf:Description rdf:about="http://w3id.org/glosis/model/procedure/gypsumProcedure-CaSO4_gy07"/>
                </owl:oneOf>
            </owl:Class>
        </owl:equivalentClass>
        <rdfs:subClassOf rdf:resource="http://www.w3.org/2004/02/skos/core#Concept"/>
        <rdfs:subClassOf rdf:resource="http://www.w3.org/ns/sosa/Procedure"/>
        <rdfs:comment xml:lang="en">This code list provides analysis procedures for Gypsum.</rdfs:comment>
        <rdfs:label xml:lang="en">Procedures for Gypsum - codelist class</rdfs:label>
        <rdfs:seeAlso rdf:resource="http://w3id.org/glosis/model/procedure/gypsumProcedure"/>
    </owl:Class>
    


    <!-- http://w3id.org/glosis/model/procedure/HydraulicConductivityProcedure -->


    <owl:Class rdf:about="http://w3id.org/glosis/model/procedure/HydraulicConductivityProcedure">
        <owl:equivalentClass>
            <owl:Class>
                <owl:oneOf rdf:parseType="Collection">
                    <rdf:Description rdf:about="http://w3id.org/glosis/model/procedure/hydraulicConductivityProcedure-KSat_calcul-ptf"/>
                    <rdf:Description rdf:about="http://w3id.org/glosis/model/procedure/hydraulicConductivityProcedure-KSat_calcul-ptf-genuchten"/>
                    <rdf:Description rdf:about="http://w3id.org/glosis/model/procedure/hydraulicConductivityProcedure-KSat_calcul-ptf-saxton"/>
                    <rdf:Description rdf:about="http://w3id.org/glosis/model/procedure/hydraulicConductivityProcedure-Ksat_bhole"/>
                    <rdf:Description rdf:about="http://w3id.org/glosis/model/procedure/hydraulicConductivityProcedure-Ksat_column"/>
                    <rdf:Description rdf:about="http://w3id.org/glosis/model/procedure/hydraulicConductivityProcedure-Ksat_dblring"/>
                    <rdf:Description rdf:about="http://w3id.org/glosis/model/procedure/hydraulicConductivityProcedure-Ksat_invbhole"/>
                </owl:oneOf>
            </owl:Class>
        </owl:equivalentClass>
        <rdfs:subClassOf rdf:resource="http://www.w3.org/2004/02/skos/core#Concept"/>
        <rdfs:subClassOf rdf:resource="http://www.w3.org/ns/sosa/Procedure"/>
        <rdfs:comment xml:lang="en">This code list provides analysis procedures for HydraulicConductivity.</rdfs:comment>
        <rdfs:label xml:lang="en">Procedures for HydraulicConductivity - codelist class</rdfs:label>
        <rdfs:seeAlso rdf:resource="http://w3id.org/glosis/model/procedure/hydraulicConductivityProcedure"/>
    </owl:Class>
    


    <!-- http://w3id.org/glosis/model/procedure/MoistureContentProcedure -->


    <owl:Class rdf:about="http://w3id.org/glosis/model/procedure/MoistureContentProcedure">
        <owl:equivalentClass>
            <owl:Class>
                <owl:oneOf rdf:parseType="Collection">
                    <rdf:Description rdf:about="http://w3id.org/glosis/model/procedure/moistureContentProcedure-VMC_calcul-ptf"/>
                    <rdf:Description rdf:about="http://w3id.org/glosis/model/procedure/moistureContentProcedure-VMC_calcul-ptf-brookscorey"/>
                    <rdf:Description rdf:about="http://w3id.org/glosis/model/procedure/moistureContentProcedure-VMC_d"/>
                    <rdf:Description rdf:about="http://w3id.org/glosis/model/procedure/moistureContentProcedure-VMC_d-cl"/>
                    <rdf:Description rdf:about="http://w3id.org/glosis/model/procedure/moistureContentProcedure-VMC_d-cl-ww"/>
                    <rdf:Description rdf:about="http://w3id.org/glosis/model/procedure/moistureContentProcedure-VMC_d-ww"/>
                    <rdf:Description rdf:about="http://w3id.org/glosis/model/procedure/moistureContentProcedure-VMC_ud"/>
                    <rdf:Description rdf:about="http://w3id.org/glosis/model/procedure/moistureContentProcedure-VMC_ud-cl"/>
                    <rdf:Description rdf:about="http://w3id.org/glosis/model/procedure/moistureContentProcedure-VMC_ud-co"/>
                </owl:oneOf>
            </owl:Class>
        </owl:equivalentClass>
        <rdfs:subClassOf rdf:resource="http://www.w3.org/2004/02/skos/core#Concept"/>
        <rdfs:subClassOf rdf:resource="http://www.w3.org/ns/sosa/Procedure"/>
        <rdfs:comment xml:lang="en">This code list provides analysis procedures for MoistureContent.</rdfs:comment>
        <rdfs:label xml:lang="en">Procedures for MoistureContent - codelist class</rdfs:label>
        <rdfs:seeAlso rdf:resource="http://w3id.org/glosis/model/procedure/moistureContentProcedure"/>
    </owl:Class>
    


    <!-- http://w3id.org/glosis/model/procedure/NitrogenTotalProcedure -->


    <owl:Class rdf:about="http://w3id.org/glosis/model/procedure/NitrogenTotalProcedure">
        <owl:equivalentClass>
            <owl:Class>
                <owl:oneOf rdf:parseType="Collection">
                    <rdf:Description rdf:about="http://w3id.org/glosis/model/procedure/nitrogenTotalProcedure-TotalN_bremner"/>
                    <rdf:Description rdf:about="http://w3id.org/glosis/model/procedure/nitrogenTotalProcedure-TotalN_calcul"/>
                    <rdf:Description rdf:about="http://w3id.org/glosis/model/procedure/nitrogenTotalProcedure-TotalN_calcul-oc10"/>
                    <rdf:Description rdf:about="http://w3id.org/glosis/model/procedure/nitrogenTotalProcedure-TotalN_dc"/>
                    <rdf:Description rdf:about="http://w3id.org/glosis/model/procedure/nitrogenTotalProcedure-TotalN_dc-ht-dumas"/>
                    <rdf:Description rdf:about="http://w3id.org/glosis/model/procedure/nitrogenTotalProcedure-TotalN_dc-ht-leco"/>
                    <rdf:Description rdf:about="http://w3id.org/glosis/model/procedure/nitrogenTotalProcedure-TotalN_dc-spec"/>
                    <rdf:Description rdf:about="http://w3id.org/glosis/model/procedure/nitrogenTotalProcedure-TotalN_h2so4"/>
                    <rdf:Description rdf:about="http://w3id.org/glosis/model/procedure/nitrogenTotalProcedure-TotalN_kjeldahl"/>
                    <rdf:Description rdf:about="http://w3id.org/glosis/model/procedure/nitrogenTotalProcedure-TotalN_kjeldahl-nh4"/>
                    <rdf:Description rdf:about="http://w3id.org/glosis/model/procedure/nitrogenTotalProcedure-TotalN_nelson"/>
                    <rdf:Description rdf:about="http://w3id.org/glosis/model/procedure/nitrogenTotalProcedure-TotalN_tn04"/>
                    <rdf:Description rdf:about="http://w3id.org/glosis/model/procedure/nitrogenTotalProcedure-TotalN_tn06"/>
                    <rdf:Description rdf:about="http://w3id.org/glosis/model/procedure/nitrogenTotalProcedure-TotalN_tn08"/>
                </owl:oneOf>
            </owl:Class>
        </owl:equivalentClass>
        <rdfs:subClassOf rdf:resource="http://www.w3.org/2004/02/skos/core#Concept"/>
        <rdfs:subClassOf rdf:resource="http://www.w3.org/ns/sosa/Procedure"/>
        <rdfs:comment xml:lang="en">This code list provides analysis procedures for NitrogenTotal.</rdfs:comment>
        <rdfs:label xml:lang="en">Procedures for NitrogenTotal - codelist class</rdfs:label>
        <rdfs:seeAlso rdf:resource="http://w3id.org/glosis/model/procedure/nitrogenTotalProcedure"/>
    </owl:Class>
    


    <!-- http://w3id.org/glosis/model/procedure/OrganicMatterProcedure -->


    <owl:Class rdf:about="http://w3id.org/glosis/model/procedure/OrganicMatterProcedure">
        <owl:equivalentClass>
            <owl:Class>
                <owl:oneOf rdf:parseType="Collection">
                    <rdf:Description rdf:about="http://w3id.org/glosis/model/procedure/organicMatterProcedure-FulAcidC_unkn"/>
                    <rdf:Description rdf:about="http://w3id.org/glosis/model/procedure/organicMatterProcedure-HumAcidC_unkn"/>
                    <rdf:Description rdf:about="http://w3id.org/glosis/model/procedure/organicMatterProcedure-OrgM_calcul-oc1.73"/>
                    <rdf:Description rdf:about="http://w3id.org/glosis/model/procedure/organicMatterProcedure-TotHumC_unkn"/>
                </owl:oneOf>
            </owl:Class>
        </owl:equivalentClass>
        <rdfs:subClassOf rdf:resource="http://www.w3.org/2004/02/skos/core#Concept"/>
        <rdfs:subClassOf rdf:resource="http://www.w3.org/ns/sosa/Procedure"/>
        <rdfs:comment xml:lang="en">This code list provides analysis procedures for OrganicMatter.</rdfs:comment>
        <rdfs:label xml:lang="en">Procedures for OrganicMatter - codelist class</rdfs:label>
        <rdfs:seeAlso rdf:resource="http://w3id.org/glosis/model/procedure/organicMatterProcedure"/>
    </owl:Class>
    


    <!-- http://w3id.org/glosis/model/procedure/PHProcedure -->


    <owl:Class rdf:about="http://w3id.org/glosis/model/procedure/PHProcedure">
        <owl:equivalentClass>
            <owl:Class>
                <owl:oneOf rdf:parseType="Collection">
                    <rdf:Description rdf:about="http://w3id.org/glosis/model/procedure/pHProcedure-pHCaCl2"/>
                    <rdf:Description rdf:about="http://w3id.org/glosis/model/procedure/pHProcedure-pHCaCl2_ratio1-1"/>
                    <rdf:Description rdf:about="http://w3id.org/glosis/model/procedure/pHProcedure-pHCaCl2_ratio1-10"/>
                    <rdf:Description rdf:about="http://w3id.org/glosis/model/procedure/pHProcedure-pHCaCl2_ratio1-2"/>
                    <rdf:Description rdf:about="http://w3id.org/glosis/model/procedure/pHProcedure-pHCaCl2_ratio1-2.5"/>
                    <rdf:Description rdf:about="http://w3id.org/glosis/model/procedure/pHProcedure-pHCaCl2_ratio1-5"/>
                    <rdf:Description rdf:about="http://w3id.org/glosis/model/procedure/pHProcedure-pHCaCl2_sat"/>
                    <rdf:Description rdf:about="http://w3id.org/glosis/model/procedure/pHProcedure-pHH2O"/>
                    <rdf:Description rdf:about="http://w3id.org/glosis/model/procedure/pHProcedure-pHH2O_ratio1-1"/>
                    <rdf:Description rdf:about="http://w3id.org/glosis/model/procedure/pHProcedure-pHH2O_ratio1-10"/>
                    <rdf:Description rdf:about="http://w3id.org/glosis/model/procedure/pHProcedure-pHH2O_ratio1-2"/>
                    <rdf:Description rdf:about="http://w3id.org/glosis/model/procedure/pHProcedure-pHH2O_ratio1-2.5"/>
                    <rdf:Description rdf:about="http://w3id.org/glosis/model/procedure/pHProcedure-pHH2O_ratio1-5"/>
                    <rdf:Description rdf:about="http://w3id.org/glosis/model/procedure/pHProcedure-pHH2O_sat"/>
                    <rdf:Description rdf:about="http://w3id.org/glosis/model/procedure/pHProcedure-pHH2O_unkn-spec"/>
                    <rdf:Description rdf:about="http://w3id.org/glosis/model/procedure/pHProcedure-pHKCl"/>
                    <rdf:Description rdf:about="http://w3id.org/glosis/model/procedure/pHProcedure-pHKCl_ratio1-1"/>
                    <rdf:Description rdf:about="http://w3id.org/glosis/model/procedure/pHProcedure-pHKCl_ratio1-10"/>
                    <rdf:Description rdf:about="http://w3id.org/glosis/model/procedure/pHProcedure-pHKCl_ratio1-2"/>
                    <rdf:Description rdf:about="http://w3id.org/glosis/model/procedure/pHProcedure-pHKCl_ratio1-2.5"/>
                    <rdf:Description rdf:about="http://w3id.org/glosis/model/procedure/pHProcedure-pHKCl_ratio1-5"/>
                    <rdf:Description rdf:about="http://w3id.org/glosis/model/procedure/pHProcedure-pHKCl_sat"/>
                    <rdf:Description rdf:about="http://w3id.org/glosis/model/procedure/pHProcedure-pHNaF"/>
                    <rdf:Description rdf:about="http://w3id.org/glosis/model/procedure/pHProcedure-pHNaF_ratio1-1"/>
                    <rdf:Description rdf:about="http://w3id.org/glosis/model/procedure/pHProcedure-pHNaF_ratio1-10"/>
                    <rdf:Description rdf:about="http://w3id.org/glosis/model/procedure/pHProcedure-pHNaF_ratio1-2"/>
                    <rdf:Description rdf:about="http://w3id.org/glosis/model/procedure/pHProcedure-pHNaF_ratio1-2.5"/>
                    <rdf:Description rdf:about="http://w3id.org/glosis/model/procedure/pHProcedure-pHNaF_ratio1-5"/>
                    <rdf:Description rdf:about="http://w3id.org/glosis/model/procedure/pHProcedure-pHNaF_sat"/>
                </owl:oneOf>
            </owl:Class>
        </owl:equivalentClass>
        <rdfs:subClassOf rdf:resource="http://www.w3.org/2004/02/skos/core#Concept"/>
        <rdfs:subClassOf rdf:resource="http://www.w3.org/ns/sosa/Procedure"/>
        <rdfs:comment xml:lang="en">This code list provides analysis procedures for PH.</rdfs:comment>
        <rdfs:label xml:lang="en">Procedures for PH - codelist class</rdfs:label>
        <rdfs:seeAlso rdf:resource="http://w3id.org/glosis/model/procedure/pHProcedure"/>
    </owl:Class>
    


    <!-- http://w3id.org/glosis/model/procedure/PSAProcedure -->


    <owl:Class rdf:about="http://w3id.org/glosis/model/procedure/PSAProcedure">
        <owl:equivalentClass>
            <owl:Class>
                <owl:oneOf rdf:parseType="Collection">
                    <rdf:Description rdf:about="http://w3id.org/glosis/model/procedure/pSAProcedure-beaker-disp"/>
                    <rdf:Description rdf:about="http://w3id.org/glosis/model/procedure/pSAProcedure-beaker-disp-spec"/>
                    <rdf:Description rdf:about="http://w3id.org/glosis/model/procedure/pSAProcedure-beaker-nodisp"/>
                    <rdf:Description rdf:about="http://w3id.org/glosis/model/procedure/pSAProcedure-beaker-nodisp-spec"/>
                    <rdf:Description rdf:about="http://w3id.org/glosis/model/procedure/pSAProcedure-beaker-unkdisp"/>
                    <rdf:Description rdf:about="http://w3id.org/glosis/model/procedure/pSAProcedure-beaker-unkdisp-spec"/>
                    <rdf:Description rdf:about="http://w3id.org/glosis/model/procedure/pSAProcedure-fldest"/>
                    <rdf:Description rdf:about="http://w3id.org/glosis/model/procedure/pSAProcedure-hydrometer-disp"/>
                    <rdf:Description rdf:about="http://w3id.org/glosis/model/procedure/pSAProcedure-hydrometer-disp-spec"/>
                    <rdf:Description rdf:about="http://w3id.org/glosis/model/procedure/pSAProcedure-hydrometer-nodisp"/>
                    <rdf:Description rdf:about="http://w3id.org/glosis/model/procedure/pSAProcedure-hydrometer-nodisp-spec"/>
                    <rdf:Description rdf:about="http://w3id.org/glosis/model/procedure/pSAProcedure-hydrometer-unkdisp"/>
                    <rdf:Description rdf:about="http://w3id.org/glosis/model/procedure/pSAProcedure-hydrometer-unkdisp-spec"/>
                    <rdf:Description rdf:about="http://w3id.org/glosis/model/procedure/pSAProcedure-laser-disp"/>
                    <rdf:Description rdf:about="http://w3id.org/glosis/model/procedure/pSAProcedure-laser-disp-spec"/>
                    <rdf:Description rdf:about="http://w3id.org/glosis/model/procedure/pSAProcedure-laser-nodisp"/>
                    <rdf:Description rdf:about="http://w3id.org/glosis/model/procedure/pSAProcedure-laser-nodisp-spec"/>
                    <rdf:Description rdf:about="http://w3id.org/glosis/model/procedure/pSAProcedure-laser-unkdisp"/>
                    <rdf:Description rdf:about="http://w3id.org/glosis/model/procedure/pSAProcedure-laser-unkdisp-spec"/>
                    <rdf:Description rdf:about="http://w3id.org/glosis/model/procedure/pSAProcedure-pipette-disp"/>
                    <rdf:Description rdf:about="http://w3id.org/glosis/model/procedure/pSAProcedure-pipette-disp-spec"/>
                    <rdf:Description rdf:about="http://w3id.org/glosis/model/procedure/pSAProcedure-pipette-nodisp"/>
                    <rdf:Description rdf:about="http://w3id.org/glosis/model/procedure/pSAProcedure-pipette-nodisp-spec"/>
                    <rdf:Description rdf:about="http://w3id.org/glosis/model/procedure/pSAProcedure-pipette-unkdisp"/>
                    <rdf:Description rdf:about="http://w3id.org/glosis/model/procedure/pSAProcedure-pipette-unkdisp-spec"/>
                </owl:oneOf>
            </owl:Class>
        </owl:equivalentClass>
        <rdfs:subClassOf rdf:resource="http://www.w3.org/2004/02/skos/core#Concept"/>
        <rdfs:subClassOf rdf:resource="http://www.w3.org/ns/sosa/Procedure"/>
        <rdfs:comment xml:lang="en">This code list provides analysis procedures for PSA.</rdfs:comment>
        <rdfs:label xml:lang="en">Procedures for PSA - codelist class</rdfs:label>
        <rdfs:seeAlso rdf:resource="http://w3id.org/glosis/model/procedure/pSAProcedure"/>
    </owl:Class>
    


    <!-- http://w3id.org/glosis/model/procedure/PhosphorusRetentionProcedure -->


    <owl:Class rdf:about="http://w3id.org/glosis/model/procedure/PhosphorusRetentionProcedure">
        <owl:equivalentClass>
            <owl:Class>
                <owl:oneOf rdf:parseType="Collection">
                    <rdf:Description rdf:about="http://w3id.org/glosis/model/procedure/phosphorusRetentionProcedure-RetentP_blakemore"/>
                    <rdf:Description rdf:about="http://w3id.org/glosis/model/procedure/phosphorusRetentionProcedure-RetentP_unkn-spec"/>
                </owl:oneOf>
            </owl:Class>
        </owl:equivalentClass>
        <rdfs:subClassOf rdf:resource="http://www.w3.org/2004/02/skos/core#Concept"/>
        <rdfs:subClassOf rdf:resource="http://www.w3.org/ns/sosa/Procedure"/>
        <rdfs:comment xml:lang="en">This code list provides analysis procedures for PhosphorusRetention.</rdfs:comment>
        <rdfs:label xml:lang="en">Procedures for PhosphorusRetention - codelist class</rdfs:label>
        <rdfs:seeAlso rdf:resource="http://w3id.org/glosis/model/procedure/phosphorusRetentionProcedure"/>
    </owl:Class>
    


    <!-- http://w3id.org/glosis/model/procedure/PorosityProcedure -->


    <owl:Class rdf:about="http://w3id.org/glosis/model/procedure/PorosityProcedure">
        <owl:equivalentClass>
            <owl:Class>
                <owl:oneOf rdf:parseType="Collection">
                    <rdf:Description rdf:about="http://w3id.org/glosis/model/procedure/porosityProcedure-Poros_calcul-pf0"/>
                </owl:oneOf>
            </owl:Class>
        </owl:equivalentClass>
        <rdfs:subClassOf rdf:resource="http://www.w3.org/2004/02/skos/core#Concept"/>
        <rdfs:subClassOf rdf:resource="http://www.w3.org/ns/sosa/Procedure"/>
        <rdfs:comment xml:lang="en">This code list provides analysis procedures for Porosity.</rdfs:comment>
        <rdfs:label xml:lang="en">Procedures for Porosity - codelist class</rdfs:label>
        <rdfs:seeAlso rdf:resource="http://w3id.org/glosis/model/procedure/porosityProcedure"/>
    </owl:Class>
    


    <!-- http://w3id.org/glosis/model/procedure/SolubleSaltsProcedure -->


    <owl:Class rdf:about="http://w3id.org/glosis/model/procedure/SolubleSaltsProcedure">
        <owl:equivalentClass>
            <owl:Class>
                <owl:oneOf rdf:parseType="Collection">
                    <rdf:Description rdf:about="http://w3id.org/glosis/model/procedure/solubleSaltsProcedure-SlbAn_calcul-unkn"/>
                    <rdf:Description rdf:about="http://w3id.org/glosis/model/procedure/solubleSaltsProcedure-SlbCat_calcul-unkn"/>
                </owl:oneOf>
            </owl:Class>
        </owl:equivalentClass>
        <rdfs:subClassOf rdf:resource="http://www.w3.org/2004/02/skos/core#Concept"/>
        <rdfs:subClassOf rdf:resource="http://www.w3.org/ns/sosa/Procedure"/>
        <rdfs:comment xml:lang="en">This code list provides analysis procedures for SolubleSalts.</rdfs:comment>
        <rdfs:label xml:lang="en">Procedures for SolubleSalts - codelist class</rdfs:label>
        <rdfs:seeAlso rdf:resource="http://w3id.org/glosis/model/procedure/solubleSaltsProcedure"/>
    </owl:Class>
    


    <!-- http://w3id.org/glosis/model/procedure/TextureSumProcedure -->


    <owl:Class rdf:about="http://w3id.org/glosis/model/procedure/TextureSumProcedure">
        <owl:equivalentClass>
            <owl:Class>
                <owl:oneOf rdf:parseType="Collection">
                    <rdf:Description rdf:about="http://w3id.org/glosis/model/procedure/textureSumProcedure-SumTxtr_calcul"/>
                </owl:oneOf>
            </owl:Class>
        </owl:equivalentClass>
        <rdfs:subClassOf rdf:resource="http://www.w3.org/2004/02/skos/core#Concept"/>
        <rdfs:subClassOf rdf:resource="http://www.w3.org/ns/sosa/Procedure"/>
        <rdfs:comment xml:lang="en">This code list provides analysis procedures for TextureSum.</rdfs:comment>
        <rdfs:label xml:lang="en">Procedures for TextureSum - codelist class</rdfs:label>
        <rdfs:seeAlso rdf:resource="http://w3id.org/glosis/model/procedure/textureSumProcedure"/>
    </owl:Class>
    


    <!-- http://w3id.org/glosis/model/procedure/TotalCarbonateEquivalentProcedure -->


    <owl:Class rdf:about="http://w3id.org/glosis/model/procedure/TotalCarbonateEquivalentProcedure">
        <owl:equivalentClass>
            <owl:Class>
                <owl:oneOf rdf:parseType="Collection">
                    <rdf:Description rdf:about="http://w3id.org/glosis/model/procedure/totalCarbonateEquivalentProcedure-CaCO3_acid-ch3cooh-dc"/>
                    <rdf:Description rdf:about="http://w3id.org/glosis/model/procedure/totalCarbonateEquivalentProcedure-CaCO3_acid-ch3cooh-nodc"/>
                    <rdf:Description rdf:about="http://w3id.org/glosis/model/procedure/totalCarbonateEquivalentProcedure-CaCO3_acid-ch3cooh-unkn"/>
                    <rdf:Description rdf:about="http://w3id.org/glosis/model/procedure/totalCarbonateEquivalentProcedure-CaCO3_acid-dc"/>
                    <rdf:Description rdf:about="http://w3id.org/glosis/model/procedure/totalCarbonateEquivalentProcedure-CaCO3_acid-h2so4-dc"/>
                    <rdf:Description rdf:about="http://w3id.org/glosis/model/procedure/totalCarbonateEquivalentProcedure-CaCO3_acid-h2so4-nodc"/>
                    <rdf:Description rdf:about="http://w3id.org/glosis/model/procedure/totalCarbonateEquivalentProcedure-CaCO3_acid-h2so4-unkn"/>
                    <rdf:Description rdf:about="http://w3id.org/glosis/model/procedure/totalCarbonateEquivalentProcedure-CaCO3_acid-h3po4-dc"/>
                    <rdf:Description rdf:about="http://w3id.org/glosis/model/procedure/totalCarbonateEquivalentProcedure-CaCO3_acid-h3po4-nodc"/>
                    <rdf:Description rdf:about="http://w3id.org/glosis/model/procedure/totalCarbonateEquivalentProcedure-CaCO3_acid-h3po4-unkn"/>
                    <rdf:Description rdf:about="http://w3id.org/glosis/model/procedure/totalCarbonateEquivalentProcedure-CaCO3_acid-hcl-dc"/>
                    <rdf:Description rdf:about="http://w3id.org/glosis/model/procedure/totalCarbonateEquivalentProcedure-CaCO3_acid-hcl-nodc"/>
                    <rdf:Description rdf:about="http://w3id.org/glosis/model/procedure/totalCarbonateEquivalentProcedure-CaCO3_acid-hcl-unkn"/>
                    <rdf:Description rdf:about="http://w3id.org/glosis/model/procedure/totalCarbonateEquivalentProcedure-CaCO3_acid-nodc"/>
                    <rdf:Description rdf:about="http://w3id.org/glosis/model/procedure/totalCarbonateEquivalentProcedure-CaCO3_acid-unkn"/>
                    <rdf:Description rdf:about="http://w3id.org/glosis/model/procedure/totalCarbonateEquivalentProcedure-CaCO3_ca01"/>
                    <rdf:Description rdf:about="http://w3id.org/glosis/model/procedure/totalCarbonateEquivalentProcedure-CaCO3_ca02"/>
                    <rdf:Description rdf:about="http://w3id.org/glosis/model/procedure/totalCarbonateEquivalentProcedure-CaCO3_ca03"/>
                    <rdf:Description rdf:about="http://w3id.org/glosis/model/procedure/totalCarbonateEquivalentProcedure-CaCO3_ca04"/>
                    <rdf:Description rdf:about="http://w3id.org/glosis/model/procedure/totalCarbonateEquivalentProcedure-CaCO3_ca05"/>
                    <rdf:Description rdf:about="http://w3id.org/glosis/model/procedure/totalCarbonateEquivalentProcedure-CaCO3_ca06"/>
                    <rdf:Description rdf:about="http://w3id.org/glosis/model/procedure/totalCarbonateEquivalentProcedure-CaCO3_ca07"/>
                    <rdf:Description rdf:about="http://w3id.org/glosis/model/procedure/totalCarbonateEquivalentProcedure-CaCO3_ca08"/>
                    <rdf:Description rdf:about="http://w3id.org/glosis/model/procedure/totalCarbonateEquivalentProcedure-CaCO3_ca09"/>
                    <rdf:Description rdf:about="http://w3id.org/glosis/model/procedure/totalCarbonateEquivalentProcedure-CaCO3_ca10"/>
                    <rdf:Description rdf:about="http://w3id.org/glosis/model/procedure/totalCarbonateEquivalentProcedure-CaCO3_ca11"/>
                    <rdf:Description rdf:about="http://w3id.org/glosis/model/procedure/totalCarbonateEquivalentProcedure-CaCO3_ca12"/>
                    <rdf:Description rdf:about="http://w3id.org/glosis/model/procedure/totalCarbonateEquivalentProcedure-CaCO3_calcul-tc-oc"/>
                </owl:oneOf>
            </owl:Class>
        </owl:equivalentClass>
        <rdfs:subClassOf rdf:resource="http://www.w3.org/2004/02/skos/core#Concept"/>
        <rdfs:subClassOf rdf:resource="http://www.w3.org/ns/sosa/Procedure"/>
        <rdfs:comment xml:lang="en">This code list provides analysis procedures for TotalCarbonateEquivalent.</rdfs:comment>
        <rdfs:label xml:lang="en">Procedures for TotalCarbonateEquivalent - codelist class</rdfs:label>
        <rdfs:seeAlso rdf:resource="http://w3id.org/glosis/model/procedure/totalCarbonateEquivalentProcedure"/>
    </owl:Class>
    


    <!-- http://w3id.org/glosis/model/procedure/TotalElementsProcedure -->


    <owl:Class rdf:about="http://w3id.org/glosis/model/procedure/TotalElementsProcedure">
        <owl:equivalentClass>
            <owl:Class>
                <owl:oneOf rdf:parseType="Collection">
                    <rdf:Description rdf:about="http://w3id.org/glosis/model/procedure/totalElementsProcedure-Total_h2so4"/>
                    <rdf:Description rdf:about="http://w3id.org/glosis/model/procedure/totalElementsProcedure-Total_hcl"/>
                    <rdf:Description rdf:about="http://w3id.org/glosis/model/procedure/totalElementsProcedure-Total_hcl-aquaregia"/>
                    <rdf:Description rdf:about="http://w3id.org/glosis/model/procedure/totalElementsProcedure-Total_hclo4"/>
                    <rdf:Description rdf:about="http://w3id.org/glosis/model/procedure/totalElementsProcedure-Total_hno3-aquafortis"/>
                    <rdf:Description rdf:about="http://w3id.org/glosis/model/procedure/totalElementsProcedure-Total_nh4-6mo7o24"/>
                    <rdf:Description rdf:about="http://w3id.org/glosis/model/procedure/totalElementsProcedure-Total_tp03"/>
                    <rdf:Description rdf:about="http://w3id.org/glosis/model/procedure/totalElementsProcedure-Total_tp04"/>
                    <rdf:Description rdf:about="http://w3id.org/glosis/model/procedure/totalElementsProcedure-Total_tp05"/>
                    <rdf:Description rdf:about="http://w3id.org/glosis/model/procedure/totalElementsProcedure-Total_tp06"/>
                    <rdf:Description rdf:about="http://w3id.org/glosis/model/procedure/totalElementsProcedure-Total_tp07"/>
                    <rdf:Description rdf:about="http://w3id.org/glosis/model/procedure/totalElementsProcedure-Total_tp08"/>
                    <rdf:Description rdf:about="http://w3id.org/glosis/model/procedure/totalElementsProcedure-Total_tp09"/>
                    <rdf:Description rdf:about="http://w3id.org/glosis/model/procedure/totalElementsProcedure-Total_tp10"/>
                    <rdf:Description rdf:about="http://w3id.org/glosis/model/procedure/totalElementsProcedure-Total_unkn"/>
                    <rdf:Description rdf:about="http://w3id.org/glosis/model/procedure/totalElementsProcedure-Total_xrd"/>
                    <rdf:Description rdf:about="http://w3id.org/glosis/model/procedure/totalElementsProcedure-Total_xrf"/>
                    <rdf:Description rdf:about="http://w3id.org/glosis/model/procedure/totalElementsProcedure-Total_xrf-p"/>
                    <rdf:Description rdf:about="http://w3id.org/glosis/model/procedure/totalElementsProcedure-Total_xtf-t"/>
                </owl:oneOf>
            </owl:Class>
        </owl:equivalentClass>
        <rdfs:subClassOf rdf:resource="http://www.w3.org/2004/02/skos/core#Concept"/>
        <rdfs:subClassOf rdf:resource="http://www.w3.org/ns/sosa/Procedure"/>
        <rdfs:comment xml:lang="en">This code list provides analysis procedures for TotalElements.</rdfs:comment>
        <rdfs:label xml:lang="en">Procedures for TotalElements - codelist class</rdfs:label>
        <rdfs:seeAlso rdf:resource="http://w3id.org/glosis/model/procedure/totalElementsProcedure"/>
    </owl:Class>
    


    <!-- http://www.w3.org/2004/02/skos/core#Concept -->


    <owl:Class rdf:about="http://www.w3.org/2004/02/skos/core#Concept"/>
    


    <!-- http://www.w3.org/2004/02/skos/core#ConceptScheme -->


    <owl:Class rdf:about="http://www.w3.org/2004/02/skos/core#ConceptScheme"/>
    


    <!-- http://www.w3.org/ns/sosa/Procedure -->


    <owl:Class rdf:about="http://www.w3.org/ns/sosa/Procedure"/>
    


    <!-- 
    ///////////////////////////////////////////////////////////////////////////////////////
    //
    // Individuals
    //
    ///////////////////////////////////////////////////////////////////////////////////////
     -->


    


    <!-- http://w3id.org/glosis/model/procedure/acidityExchangeableProcedure -->


    <owl:NamedIndividual rdf:about="http://w3id.org/glosis/model/procedure/acidityExchangeableProcedure">
        <rdf:type rdf:resource="http://www.w3.org/2004/02/skos/core#ConceptScheme"/>
        <rdfs:label xml:lang="en">Code list for acidityExchangeable analysis procedures - codelist scheme</rdfs:label>
        <rdfs:seeAlso rdf:resource="http://w3id.org/glosis/model/procedure/AcidityExchangeableProcedure"/>
        <skos:definition>AfSP-derived interpretation (RwaSP)</skos:definition>
        <skos:note xml:lang="en">This code list provides analysis procedures for acidityExchangeable.</skos:note>
        <skos:prefLabel xml:lang="en">Code list for acidityExchangeable analysis procedures - codelist scheme</skos:prefLabel>
    </owl:NamedIndividual>
    


    <!-- http://w3id.org/glosis/model/procedure/acidityExchangeableProcedure-ExchAcid_ph0-kcl1m -->


    <owl:NamedIndividual rdf:about="http://w3id.org/glosis/model/procedure/acidityExchangeableProcedure-ExchAcid_ph0-kcl1m">
        <rdf:type rdf:resource="http://w3id.org/glosis/model/procedure/AcidityExchangeableProcedure"/>
        <rdf:type rdf:resource="http://www.w3.org/2004/02/skos/core#Concept"/>
        <skos:definition>Exch acidity (H+Al) unbuffered, in 1 M KCl extract</skos:definition>
        <skos:inScheme rdf:resource="http://w3id.org/glosis/model/procedure/acidityExchangeableProcedure"/>
        <skos:notation>ExchAcid_ph0-kcl1m</skos:notation>
        <skos:prefLabel xml:lang="en">ExchAcid_ph0-kcl1m</skos:prefLabel>
        <skos:scopeNote rdf:resource="https://www.isric.org/sites/default/files/isric_report_2014_01.pdf"/>
        <skos:scopeNote>Leenaars J.G.B., A.J.M. van Oostrum and M. Ruiperez Gonzalez, 2014. Africa Soil Profiles Database, Version 1.2. A compilation of georeferenced and standardised legacy soil profile data for Sub-Saharan Africa (with dataset). ISRIC Report 2014/01. Africa Soil Information Service (AfSIS) project and ISRIC - World Soil Information, Wageningen, the Netherlands. See Annex 4.</skos:scopeNote>
        <skos:topConceptOf rdf:resource="http://w3id.org/glosis/model/procedure/acidityExchangeableProcedure"/>
    </owl:NamedIndividual>
    


    <!-- http://w3id.org/glosis/model/procedure/acidityExchangeableProcedure-ExchAcid_ph0-nh4cl -->


    <owl:NamedIndividual rdf:about="http://w3id.org/glosis/model/procedure/acidityExchangeableProcedure-ExchAcid_ph0-nh4cl">
        <rdf:type rdf:resource="http://w3id.org/glosis/model/procedure/AcidityExchangeableProcedure"/>
        <rdf:type rdf:resource="http://www.w3.org/2004/02/skos/core#Concept"/>
        <skos:definition>Exch acidity (H+Al) unbuffered, in 0.05-0.1 M NH4Cl extract</skos:definition>
        <skos:inScheme rdf:resource="http://w3id.org/glosis/model/procedure/acidityExchangeableProcedure"/>
        <skos:notation>ExchAcid_ph0-nh4cl</skos:notation>
        <skos:prefLabel xml:lang="en">ExchAcid_ph0-nh4cl</skos:prefLabel>
        <skos:scopeNote rdf:resource="https://www.isric.org/sites/default/files/isric_report_2014_01.pdf"/>
        <skos:scopeNote>Leenaars J.G.B., A.J.M. van Oostrum and M. Ruiperez Gonzalez, 2014. Africa Soil Profiles Database, Version 1.2. A compilation of georeferenced and standardised legacy soil profile data for Sub-Saharan Africa (with dataset). ISRIC Report 2014/01. Africa Soil Information Service (AfSIS) project and ISRIC - World Soil Information, Wageningen, the Netherlands. See Annex 4.</skos:scopeNote>
        <skos:topConceptOf rdf:resource="http://w3id.org/glosis/model/procedure/acidityExchangeableProcedure"/>
    </owl:NamedIndividual>
    


    <!-- http://w3id.org/glosis/model/procedure/acidityExchangeableProcedure-ExchAcid_ph0-unkn -->


    <owl:NamedIndividual rdf:about="http://w3id.org/glosis/model/procedure/acidityExchangeableProcedure-ExchAcid_ph0-unkn">
        <rdf:type rdf:resource="http://w3id.org/glosis/model/procedure/AcidityExchangeableProcedure"/>
        <rdf:type rdf:resource="http://www.w3.org/2004/02/skos/core#Concept"/>
        <skos:definition>Exch acidity (H+Al) unbuffered, in unknown extract</skos:definition>
        <skos:inScheme rdf:resource="http://w3id.org/glosis/model/procedure/acidityExchangeableProcedure"/>
        <skos:notation>ExchAcid_ph0-unkn</skos:notation>
        <skos:prefLabel xml:lang="en">ExchAcid_ph0-unk</skos:prefLabel>
        <skos:scopeNote rdf:resource="https://www.isric.org/sites/default/files/isric_report_2014_01.pdf"/>
        <skos:scopeNote>Leenaars J.G.B., A.J.M. van Oostrum and M. Ruiperez Gonzalez, 2014. Africa Soil Profiles Database, Version 1.2. A compilation of georeferenced and standardised legacy soil profile data for Sub-Saharan Africa (with dataset). ISRIC Report 2014/01. Africa Soil Information Service (AfSIS) project and ISRIC - World Soil Information, Wageningen, the Netherlands. See Annex 4.</skos:scopeNote>
        <skos:topConceptOf rdf:resource="http://w3id.org/glosis/model/procedure/acidityExchangeableProcedure"/>
    </owl:NamedIndividual>
    


    <!-- http://w3id.org/glosis/model/procedure/acidityExchangeableProcedure-ExchAcid_ph7-caoac -->


    <owl:NamedIndividual rdf:about="http://w3id.org/glosis/model/procedure/acidityExchangeableProcedure-ExchAcid_ph7-caoac">
        <rdf:type rdf:resource="http://w3id.org/glosis/model/procedure/AcidityExchangeableProcedure"/>
        <rdf:type rdf:resource="http://www.w3.org/2004/02/skos/core#Concept"/>
        <skos:definition>Exch acidity (H+Al) buffered at pH 7, in 1M Ca-acetate extract</skos:definition>
        <skos:inScheme rdf:resource="http://w3id.org/glosis/model/procedure/acidityExchangeableProcedure"/>
        <skos:notation>ExchAcid_ph7-caoac</skos:notation>
        <skos:prefLabel xml:lang="en">ExchAcid_ph7-caoac</skos:prefLabel>
        <skos:scopeNote rdf:resource="https://www.isric.org/sites/default/files/isric_report_2014_01.pdf"/>
        <skos:scopeNote>Leenaars J.G.B., A.J.M. van Oostrum and M. Ruiperez Gonzalez, 2014. Africa Soil Profiles Database, Version 1.2. A compilation of georeferenced and standardised legacy soil profile data for Sub-Saharan Africa (with dataset). ISRIC Report 2014/01. Africa Soil Information Service (AfSIS) project and ISRIC - World Soil Information, Wageningen, the Netherlands. See Annex 4.</skos:scopeNote>
        <skos:topConceptOf rdf:resource="http://w3id.org/glosis/model/procedure/acidityExchangeableProcedure"/>
    </owl:NamedIndividual>
    


    <!-- http://w3id.org/glosis/model/procedure/acidityExchangeableProcedure-ExchAcid_ph7-unkn -->


    <owl:NamedIndividual rdf:about="http://w3id.org/glosis/model/procedure/acidityExchangeableProcedure-ExchAcid_ph7-unkn">
        <rdf:type rdf:resource="http://w3id.org/glosis/model/procedure/AcidityExchangeableProcedure"/>
        <rdf:type rdf:resource="http://www.w3.org/2004/02/skos/core#Concept"/>
        <skos:definition>Exch acidity (H+Al) buffered at pH 7, in unknown extract</skos:definition>
        <skos:inScheme rdf:resource="http://w3id.org/glosis/model/procedure/acidityExchangeableProcedure"/>
        <skos:notation>ExchAcid_ph7-unkn</skos:notation>
        <skos:prefLabel xml:lang="en">ExchAcid_ph7-unk</skos:prefLabel>
        <skos:scopeNote rdf:resource="https://www.isric.org/sites/default/files/isric_report_2014_01.pdf"/>
        <skos:scopeNote>Leenaars J.G.B., A.J.M. van Oostrum and M. Ruiperez Gonzalez, 2014. Africa Soil Profiles Database, Version 1.2. A compilation of georeferenced and standardised legacy soil profile data for Sub-Saharan Africa (with dataset). ISRIC Report 2014/01. Africa Soil Information Service (AfSIS) project and ISRIC - World Soil Information, Wageningen, the Netherlands. See Annex 4.</skos:scopeNote>
        <skos:topConceptOf rdf:resource="http://w3id.org/glosis/model/procedure/acidityExchangeableProcedure"/>
    </owl:NamedIndividual>
    


    <!-- http://w3id.org/glosis/model/procedure/acidityExchangeableProcedure-ExchAcid_ph8-bacl2tea -->


    <owl:NamedIndividual rdf:about="http://w3id.org/glosis/model/procedure/acidityExchangeableProcedure-ExchAcid_ph8-bacl2tea">
        <rdf:type rdf:resource="http://w3id.org/glosis/model/procedure/AcidityExchangeableProcedure"/>
        <rdf:type rdf:resource="http://www.w3.org/2004/02/skos/core#Concept"/>
        <skos:definition>Exch (extractable / potential) acidity (Al) buffered at pH 8.0-8.5, in 1 M BaCl2 - TEA</skos:definition>
        <skos:inScheme rdf:resource="http://w3id.org/glosis/model/procedure/acidityExchangeableProcedure"/>
        <skos:notation>ExchAcid_ph8-bacl2tea</skos:notation>
        <skos:prefLabel xml:lang="en">ExchAcid_ph8-bacl2tea</skos:prefLabel>
        <skos:scopeNote rdf:resource="https://www.isric.org/sites/default/files/isric_report_2014_01.pdf"/>
        <skos:scopeNote>Leenaars J.G.B., A.J.M. van Oostrum and M. Ruiperez Gonzalez, 2014. Africa Soil Profiles Database, Version 1.2. A compilation of georeferenced and standardised legacy soil profile data for Sub-Saharan Africa (with dataset). ISRIC Report 2014/01. Africa Soil Information Service (AfSIS) project and ISRIC - World Soil Information, Wageningen, the Netherlands. See Annex 4.</skos:scopeNote>
        <skos:topConceptOf rdf:resource="http://w3id.org/glosis/model/procedure/acidityExchangeableProcedure"/>
    </owl:NamedIndividual>
    


    <!-- http://w3id.org/glosis/model/procedure/acidityExchangeableProcedure-ExchAcid_ph8-unkn -->


    <owl:NamedIndividual rdf:about="http://w3id.org/glosis/model/procedure/acidityExchangeableProcedure-ExchAcid_ph8-unkn">
        <rdf:type rdf:resource="http://w3id.org/glosis/model/procedure/AcidityExchangeableProcedure"/>
        <rdf:type rdf:resource="http://www.w3.org/2004/02/skos/core#Concept"/>
        <skos:definition>Exch (extractable / potential) acidity (Al) buffered at pH 8.0-8.5, in unknown extract</skos:definition>
        <skos:inScheme rdf:resource="http://w3id.org/glosis/model/procedure/acidityExchangeableProcedure"/>
        <skos:notation>ExchAcid_ph8-unkn</skos:notation>
        <skos:prefLabel xml:lang="en">ExchAcid_ph8-unk</skos:prefLabel>
        <skos:scopeNote rdf:resource="https://www.isric.org/sites/default/files/isric_report_2014_01.pdf"/>
        <skos:scopeNote>Leenaars J.G.B., A.J.M. van Oostrum and M. Ruiperez Gonzalez, 2014. Africa Soil Profiles Database, Version 1.2. A compilation of georeferenced and standardised legacy soil profile data for Sub-Saharan Africa (with dataset). ISRIC Report 2014/01. Africa Soil Information Service (AfSIS) project and ISRIC - World Soil Information, Wageningen, the Netherlands. See Annex 4.</skos:scopeNote>
        <skos:topConceptOf rdf:resource="http://w3id.org/glosis/model/procedure/acidityExchangeableProcedure"/>
    </owl:NamedIndividual>
    


    <!-- http://w3id.org/glosis/model/procedure/availableWaterHoldingCapacityProcedure -->


    <owl:NamedIndividual rdf:about="http://w3id.org/glosis/model/procedure/availableWaterHoldingCapacityProcedure">
        <rdf:type rdf:resource="http://www.w3.org/2004/02/skos/core#ConceptScheme"/>
        <rdfs:label xml:lang="en">Code list for availableWaterHoldingCapacity analysis procedures - codelist scheme</rdfs:label>
        <rdfs:seeAlso rdf:resource="http://w3id.org/glosis/model/procedure/AvailableWaterHoldingCapacityProcedure"/>
        <skos:definition>AfSP-derived interpretation (RwaSP)</skos:definition>
        <skos:note xml:lang="en">This code list provides analysis procedures for availableWaterHoldingCapacity.</skos:note>
        <skos:prefLabel xml:lang="en">Code list for availableWaterHoldingCapacity analysis procedures - codelist scheme</skos:prefLabel>
    </owl:NamedIndividual>
    


    <!-- http://w3id.org/glosis/model/procedure/availableWaterHoldingCapacityProcedure-PAWHC_calcul-fc100wp -->


    <owl:NamedIndividual rdf:about="http://w3id.org/glosis/model/procedure/availableWaterHoldingCapacityProcedure-PAWHC_calcul-fc100wp">
        <rdf:type rdf:resource="http://w3id.org/glosis/model/procedure/AvailableWaterHoldingCapacityProcedure"/>
        <rdf:type rdf:resource="http://www.w3.org/2004/02/skos/core#Concept"/>
        <skos:definition>Plant available water holding capacity of the soil fine earth fraction, calculated with field capacity defined at 100 cm (pF 2.0)</skos:definition>
        <skos:inScheme rdf:resource="http://w3id.org/glosis/model/procedure/availableWaterHoldingCapacityProcedure"/>
        <skos:notation>PAWHC_calcul-fc100wp</skos:notation>
        <skos:prefLabel xml:lang="en">PAWHC_calcul-fc100wp</skos:prefLabel>
        <skos:scopeNote rdf:resource="https://www.isric.org/sites/default/files/isric_report_2014_01.pdf"/>
        <skos:scopeNote>Leenaars J.G.B., A.J.M. van Oostrum and M. Ruiperez Gonzalez, 2014. Africa Soil Profiles Database, Version 1.2. A compilation of georeferenced and standardised legacy soil profile data for Sub-Saharan Africa (with dataset). ISRIC Report 2014/01. Africa Soil Information Service (AfSIS) project and ISRIC - World Soil Information, Wageningen, the Netherlands. See Annex 4.</skos:scopeNote>
        <skos:topConceptOf rdf:resource="http://w3id.org/glosis/model/procedure/availableWaterHoldingCapacityProcedure"/>
    </owl:NamedIndividual>
    


    <!-- http://w3id.org/glosis/model/procedure/availableWaterHoldingCapacityProcedure-PAWHC_calcul-fc200wp -->


    <owl:NamedIndividual rdf:about="http://w3id.org/glosis/model/procedure/availableWaterHoldingCapacityProcedure-PAWHC_calcul-fc200wp">
        <rdf:type rdf:resource="http://w3id.org/glosis/model/procedure/AvailableWaterHoldingCapacityProcedure"/>
        <rdf:type rdf:resource="http://www.w3.org/2004/02/skos/core#Concept"/>
        <skos:definition>Plant available water holding capacity of the soil fine earth fraction, calculated with field capacity defined at 200 cm (pF 2.3)</skos:definition>
        <skos:inScheme rdf:resource="http://w3id.org/glosis/model/procedure/availableWaterHoldingCapacityProcedure"/>
        <skos:notation>PAWHC_calcul-fc200wp</skos:notation>
        <skos:prefLabel xml:lang="en">PAWHC_calcul-fc200wp</skos:prefLabel>
        <skos:scopeNote rdf:resource="https://www.isric.org/sites/default/files/isric_report_2014_01.pdf"/>
        <skos:scopeNote>Leenaars J.G.B., A.J.M. van Oostrum and M. Ruiperez Gonzalez, 2014. Africa Soil Profiles Database, Version 1.2. A compilation of georeferenced and standardised legacy soil profile data for Sub-Saharan Africa (with dataset). ISRIC Report 2014/01. Africa Soil Information Service (AfSIS) project and ISRIC - World Soil Information, Wageningen, the Netherlands. See Annex 4.</skos:scopeNote>
        <skos:topConceptOf rdf:resource="http://w3id.org/glosis/model/procedure/availableWaterHoldingCapacityProcedure"/>
    </owl:NamedIndividual>
    


    <!-- http://w3id.org/glosis/model/procedure/availableWaterHoldingCapacityProcedure-PAWHC_calcul-fc300wp -->


    <owl:NamedIndividual rdf:about="http://w3id.org/glosis/model/procedure/availableWaterHoldingCapacityProcedure-PAWHC_calcul-fc300wp">
        <rdf:type rdf:resource="http://w3id.org/glosis/model/procedure/AvailableWaterHoldingCapacityProcedure"/>
        <rdf:type rdf:resource="http://www.w3.org/2004/02/skos/core#Concept"/>
        <skos:definition>Plant available water holding capacity of the soil fine earth fraction, calculated with field capacity defined at 300 cm (pF 2.5)</skos:definition>
        <skos:inScheme rdf:resource="http://w3id.org/glosis/model/procedure/availableWaterHoldingCapacityProcedure"/>
        <skos:notation>PAWHC_calcul-fc300wp</skos:notation>
        <skos:prefLabel xml:lang="en">PAWHC_calcul-fc300wp</skos:prefLabel>
        <skos:scopeNote rdf:resource="https://www.isric.org/sites/default/files/isric_report_2014_01.pdf"/>
        <skos:scopeNote>Leenaars J.G.B., A.J.M. van Oostrum and M. Ruiperez Gonzalez, 2014. Africa Soil Profiles Database, Version 1.2. A compilation of georeferenced and standardised legacy soil profile data for Sub-Saharan Africa (with dataset). ISRIC Report 2014/01. Africa Soil Information Service (AfSIS) project and ISRIC - World Soil Information, Wageningen, the Netherlands. See Annex 4.</skos:scopeNote>
        <skos:topConceptOf rdf:resource="http://w3id.org/glosis/model/procedure/availableWaterHoldingCapacityProcedure"/>
    </owl:NamedIndividual>
    


    <!-- http://w3id.org/glosis/model/procedure/baseSaturationProcedure -->


    <owl:NamedIndividual rdf:about="http://w3id.org/glosis/model/procedure/baseSaturationProcedure">
        <rdf:type rdf:resource="http://www.w3.org/2004/02/skos/core#ConceptScheme"/>
        <rdfs:label xml:lang="en">Code list for baseSaturation analysis procedures - codelist scheme</rdfs:label>
        <rdfs:seeAlso rdf:resource="http://w3id.org/glosis/model/procedure/BaseSaturationProcedure"/>
        <skos:definition>AfSP-derived interpretation (RwaSP)</skos:definition>
        <skos:note xml:lang="en">This code list provides analysis procedures for baseSaturation.</skos:note>
        <skos:prefLabel xml:lang="en">Code list for baseSaturation analysis procedures - codelist scheme</skos:prefLabel>
    </owl:NamedIndividual>
    


    <!-- http://w3id.org/glosis/model/procedure/baseSaturationProcedure-BSat_calcul-cec -->


    <owl:NamedIndividual rdf:about="http://w3id.org/glosis/model/procedure/baseSaturationProcedure-BSat_calcul-cec">
        <rdf:type rdf:resource="http://w3id.org/glosis/model/procedure/BaseSaturationProcedure"/>
        <rdf:type rdf:resource="http://www.w3.org/2004/02/skos/core#Concept"/>
        <skos:definition>Sum of exchangeable bases (Ca++, Mg++, K+, Na+) as percentage of CEC (method specified with CEC and ExchBases)</skos:definition>
        <skos:inScheme rdf:resource="http://w3id.org/glosis/model/procedure/baseSaturationProcedure"/>
        <skos:notation>BSat_calcul-cec</skos:notation>
        <skos:prefLabel xml:lang="en">BSat_calcul-cec</skos:prefLabel>
        <skos:scopeNote rdf:resource="https://www.isric.org/sites/default/files/isric_report_2014_01.pdf"/>
        <skos:scopeNote>Leenaars J.G.B., A.J.M. van Oostrum and M. Ruiperez Gonzalez, 2014. Africa Soil Profiles Database, Version 1.2. A compilation of georeferenced and standardised legacy soil profile data for Sub-Saharan Africa (with dataset). ISRIC Report 2014/01. Africa Soil Information Service (AfSIS) project and ISRIC - World Soil Information, Wageningen, the Netherlands. See Annex 4.</skos:scopeNote>
        <skos:topConceptOf rdf:resource="http://w3id.org/glosis/model/procedure/baseSaturationProcedure"/>
    </owl:NamedIndividual>
    


    <!-- http://w3id.org/glosis/model/procedure/baseSaturationProcedure-BSat_calcul-ecec -->


    <owl:NamedIndividual rdf:about="http://w3id.org/glosis/model/procedure/baseSaturationProcedure-BSat_calcul-ecec">
        <rdf:type rdf:resource="http://w3id.org/glosis/model/procedure/BaseSaturationProcedure"/>
        <rdf:type rdf:resource="http://www.w3.org/2004/02/skos/core#Concept"/>
        <skos:definition>Sum of exchangeable bases (Ca++, Mg++, K+, Na+) as percentage of EffCEC (method specified with EffCEC and ExchBases)</skos:definition>
        <skos:inScheme rdf:resource="http://w3id.org/glosis/model/procedure/baseSaturationProcedure"/>
        <skos:notation>BSat_calcul-ecec</skos:notation>
        <skos:prefLabel xml:lang="en">BSat_calcul-ecec</skos:prefLabel>
        <skos:scopeNote rdf:resource="https://www.isric.org/sites/default/files/isric_report_2014_01.pdf"/>
        <skos:scopeNote>Leenaars J.G.B., A.J.M. van Oostrum and M. Ruiperez Gonzalez, 2014. Africa Soil Profiles Database, Version 1.2. A compilation of georeferenced and standardised legacy soil profile data for Sub-Saharan Africa (with dataset). ISRIC Report 2014/01. Africa Soil Information Service (AfSIS) project and ISRIC - World Soil Information, Wageningen, the Netherlands. See Annex 4.</skos:scopeNote>
        <skos:topConceptOf rdf:resource="http://w3id.org/glosis/model/procedure/baseSaturationProcedure"/>
    </owl:NamedIndividual>
    


    <!-- http://w3id.org/glosis/model/procedure/bulkDensityFineEarthProcedure -->


    <owl:NamedIndividual rdf:about="http://w3id.org/glosis/model/procedure/bulkDensityFineEarthProcedure">
        <rdf:type rdf:resource="http://www.w3.org/2004/02/skos/core#ConceptScheme"/>
        <rdfs:label xml:lang="en">Code list for bulkDensityFineEarth analysis procedures - codelist scheme</rdfs:label>
        <rdfs:seeAlso rdf:resource="http://w3id.org/glosis/model/procedure/BulkDensityFineEarthProcedure"/>
        <skos:definition>AfSP-derived interpretation (RwaSP)</skos:definition>
        <skos:note xml:lang="en">This code list provides analysis procedures for bulkDensityFineEarth.</skos:note>
        <skos:prefLabel xml:lang="en">Code list for bulkDensityFineEarth analysis procedures - codelist scheme</skos:prefLabel>
    </owl:NamedIndividual>
    


    <!-- http://w3id.org/glosis/model/procedure/bulkDensityFineEarthProcedure-BlkDensF_fe-cl-fc -->


    <owl:NamedIndividual rdf:about="http://w3id.org/glosis/model/procedure/bulkDensityFineEarthProcedure-BlkDensF_fe-cl-fc">
        <rdf:type rdf:resource="http://w3id.org/glosis/model/procedure/BulkDensityFineEarthProcedure"/>
        <rdf:type rdf:resource="http://www.w3.org/2004/02/skos/core#Concept"/>
        <skos:definition>Fine earth. Clod samples (natural clods or reconstituted from &lt; 2mm sample), at field capacity (0.33 bar, 33 kPa, 330 cm, pF 2.5), corrected for coarse fragments if any</skos:definition>
        <skos:inScheme rdf:resource="http://w3id.org/glosis/model/procedure/bulkDensityFineEarthProcedure"/>
        <skos:notation>BlkDensF_fe-cl-fc</skos:notation>
        <skos:prefLabel xml:lang="en">BlkDensF_fe-cl-fc</skos:prefLabel>
        <skos:scopeNote rdf:resource="https://www.isric.org/sites/default/files/isric_report_2014_01.pdf"/>
        <skos:scopeNote>Leenaars J.G.B., A.J.M. van Oostrum and M. Ruiperez Gonzalez, 2014. Africa Soil Profiles Database, Version 1.2. A compilation of georeferenced and standardised legacy soil profile data for Sub-Saharan Africa (with dataset). ISRIC Report 2014/01. Africa Soil Information Service (AfSIS) project and ISRIC - World Soil Information, Wageningen, the Netherlands. See Annex 4.</skos:scopeNote>
        <skos:topConceptOf rdf:resource="http://w3id.org/glosis/model/procedure/bulkDensityFineEarthProcedure"/>
    </owl:NamedIndividual>
    


    <!-- http://w3id.org/glosis/model/procedure/bulkDensityFineEarthProcedure-BlkDensF_fe-cl-od -->


    <owl:NamedIndividual rdf:about="http://w3id.org/glosis/model/procedure/bulkDensityFineEarthProcedure-BlkDensF_fe-cl-od">
        <rdf:type rdf:resource="http://w3id.org/glosis/model/procedure/BulkDensityFineEarthProcedure"/>
        <rdf:type rdf:resource="http://www.w3.org/2004/02/skos/core#Concept"/>
        <skos:definition>Fine earth. Clod samples (natural clods or reconstituted from &lt; 2mm sample), at oven dry, corrected for coarse fragments if any</skos:definition>
        <skos:inScheme rdf:resource="http://w3id.org/glosis/model/procedure/bulkDensityFineEarthProcedure"/>
        <skos:notation>BlkDensF_fe-cl-od</skos:notation>
        <skos:prefLabel xml:lang="en">BlkDensF_fe-cl-od</skos:prefLabel>
        <skos:scopeNote rdf:resource="https://www.isric.org/sites/default/files/isric_report_2014_01.pdf"/>
        <skos:scopeNote>Leenaars J.G.B., A.J.M. van Oostrum and M. Ruiperez Gonzalez, 2014. Africa Soil Profiles Database, Version 1.2. A compilation of georeferenced and standardised legacy soil profile data for Sub-Saharan Africa (with dataset). ISRIC Report 2014/01. Africa Soil Information Service (AfSIS) project and ISRIC - World Soil Information, Wageningen, the Netherlands. See Annex 4.</skos:scopeNote>
        <skos:topConceptOf rdf:resource="http://w3id.org/glosis/model/procedure/bulkDensityFineEarthProcedure"/>
    </owl:NamedIndividual>
    


    <!-- http://w3id.org/glosis/model/procedure/bulkDensityFineEarthProcedure-BlkDensF_fe-cl-unkn -->


    <owl:NamedIndividual rdf:about="http://w3id.org/glosis/model/procedure/bulkDensityFineEarthProcedure-BlkDensF_fe-cl-unkn">
        <rdf:type rdf:resource="http://w3id.org/glosis/model/procedure/BulkDensityFineEarthProcedure"/>
        <rdf:type rdf:resource="http://www.w3.org/2004/02/skos/core#Concept"/>
        <skos:definition>Fine earth. Clod samples (natural clods or reconstituted from &lt; 2mm sample), at unknown humidity, corrected for coarse fragments if any</skos:definition>
        <skos:inScheme rdf:resource="http://w3id.org/glosis/model/procedure/bulkDensityFineEarthProcedure"/>
        <skos:notation>BlkDensF_fe-cl-unkn</skos:notation>
        <skos:prefLabel xml:lang="en">BlkDensF_fe-cl-unk</skos:prefLabel>
        <skos:scopeNote rdf:resource="https://www.isric.org/sites/default/files/isric_report_2014_01.pdf"/>
        <skos:scopeNote>Leenaars J.G.B., A.J.M. van Oostrum and M. Ruiperez Gonzalez, 2014. Africa Soil Profiles Database, Version 1.2. A compilation of georeferenced and standardised legacy soil profile data for Sub-Saharan Africa (with dataset). ISRIC Report 2014/01. Africa Soil Information Service (AfSIS) project and ISRIC - World Soil Information, Wageningen, the Netherlands. See Annex 4.</skos:scopeNote>
        <skos:topConceptOf rdf:resource="http://w3id.org/glosis/model/procedure/bulkDensityFineEarthProcedure"/>
    </owl:NamedIndividual>
    


    <!-- http://w3id.org/glosis/model/procedure/bulkDensityFineEarthProcedure-BlkDensF_fe-co-fc -->


    <owl:NamedIndividual rdf:about="http://w3id.org/glosis/model/procedure/bulkDensityFineEarthProcedure-BlkDensF_fe-co-fc">
        <rdf:type rdf:resource="http://w3id.org/glosis/model/procedure/BulkDensityFineEarthProcedure"/>
        <rdf:type rdf:resource="http://www.w3.org/2004/02/skos/core#Concept"/>
        <skos:definition>Fine earth. Core sampling (pF rings), at field capacity (0.33 bar, 33 kPa, 336 cm, pF 2.5), corrected for coarse fragments if any</skos:definition>
        <skos:inScheme rdf:resource="http://w3id.org/glosis/model/procedure/bulkDensityFineEarthProcedure"/>
        <skos:notation>BlkDensF_fe-co-fc</skos:notation>
        <skos:prefLabel xml:lang="en">BlkDensF_fe-co-fc</skos:prefLabel>
        <skos:scopeNote rdf:resource="https://www.isric.org/sites/default/files/isric_report_2014_01.pdf"/>
        <skos:scopeNote>Leenaars J.G.B., A.J.M. van Oostrum and M. Ruiperez Gonzalez, 2014. Africa Soil Profiles Database, Version 1.2. A compilation of georeferenced and standardised legacy soil profile data for Sub-Saharan Africa (with dataset). ISRIC Report 2014/01. Africa Soil Information Service (AfSIS) project and ISRIC - World Soil Information, Wageningen, the Netherlands. See Annex 4.</skos:scopeNote>
        <skos:topConceptOf rdf:resource="http://w3id.org/glosis/model/procedure/bulkDensityFineEarthProcedure"/>
    </owl:NamedIndividual>
    


    <!-- http://w3id.org/glosis/model/procedure/bulkDensityFineEarthProcedure-BlkDensF_fe-co-od -->


    <owl:NamedIndividual rdf:about="http://w3id.org/glosis/model/procedure/bulkDensityFineEarthProcedure-BlkDensF_fe-co-od">
        <rdf:type rdf:resource="http://w3id.org/glosis/model/procedure/BulkDensityFineEarthProcedure"/>
        <rdf:type rdf:resource="http://www.w3.org/2004/02/skos/core#Concept"/>
        <skos:definition>Fine earth. Core sampling (pF rings), at oven dry, corrected for coarse fragments if any</skos:definition>
        <skos:inScheme rdf:resource="http://w3id.org/glosis/model/procedure/bulkDensityFineEarthProcedure"/>
        <skos:notation>BlkDensF_fe-co-od</skos:notation>
        <skos:prefLabel xml:lang="en">BlkDensF_fe-co-od</skos:prefLabel>
        <skos:scopeNote rdf:resource="https://www.isric.org/sites/default/files/isric_report_2014_01.pdf"/>
        <skos:scopeNote>Leenaars J.G.B., A.J.M. van Oostrum and M. Ruiperez Gonzalez, 2014. Africa Soil Profiles Database, Version 1.2. A compilation of georeferenced and standardised legacy soil profile data for Sub-Saharan Africa (with dataset). ISRIC Report 2014/01. Africa Soil Information Service (AfSIS) project and ISRIC - World Soil Information, Wageningen, the Netherlands. See Annex 4.</skos:scopeNote>
        <skos:topConceptOf rdf:resource="http://w3id.org/glosis/model/procedure/bulkDensityFineEarthProcedure"/>
    </owl:NamedIndividual>
    


    <!-- http://w3id.org/glosis/model/procedure/bulkDensityFineEarthProcedure-BlkDensF_fe-co-unkn -->


    <owl:NamedIndividual rdf:about="http://w3id.org/glosis/model/procedure/bulkDensityFineEarthProcedure-BlkDensF_fe-co-unkn">
        <rdf:type rdf:resource="http://w3id.org/glosis/model/procedure/BulkDensityFineEarthProcedure"/>
        <rdf:type rdf:resource="http://www.w3.org/2004/02/skos/core#Concept"/>
        <skos:definition>Fine earth. Core sampling (pF rings), at unknown humidity, corrected for coarse fragments if any</skos:definition>
        <skos:inScheme rdf:resource="http://w3id.org/glosis/model/procedure/bulkDensityFineEarthProcedure"/>
        <skos:notation>BlkDensF_fe-co-unkn</skos:notation>
        <skos:prefLabel xml:lang="en">BlkDensF_fe-co-unk</skos:prefLabel>
        <skos:scopeNote rdf:resource="https://www.isric.org/sites/default/files/isric_report_2014_01.pdf"/>
        <skos:scopeNote>Leenaars J.G.B., A.J.M. van Oostrum and M. Ruiperez Gonzalez, 2014. Africa Soil Profiles Database, Version 1.2. A compilation of georeferenced and standardised legacy soil profile data for Sub-Saharan Africa (with dataset). ISRIC Report 2014/01. Africa Soil Information Service (AfSIS) project and ISRIC - World Soil Information, Wageningen, the Netherlands. See Annex 4.</skos:scopeNote>
        <skos:topConceptOf rdf:resource="http://w3id.org/glosis/model/procedure/bulkDensityFineEarthProcedure"/>
    </owl:NamedIndividual>
    


    <!-- http://w3id.org/glosis/model/procedure/bulkDensityFineEarthProcedure-BlkDensF_fe-rpl-unkn -->


    <owl:NamedIndividual rdf:about="http://w3id.org/glosis/model/procedure/bulkDensityFineEarthProcedure-BlkDensF_fe-rpl-unkn">
        <rdf:type rdf:resource="http://w3id.org/glosis/model/procedure/BulkDensityFineEarthProcedure"/>
        <rdf:type rdf:resource="http://www.w3.org/2004/02/skos/core#Concept"/>
        <skos:definition>Fine earth. Excavation and replacement (i.e. soils too fragile to remove a stable sample) e.g. by auger, at unknown humidity, corrected for coarse fragments if any</skos:definition>
        <skos:inScheme rdf:resource="http://w3id.org/glosis/model/procedure/bulkDensityFineEarthProcedure"/>
        <skos:notation>BlkDensF_fe-rpl-unkn</skos:notation>
        <skos:prefLabel xml:lang="en">BlkDensF_fe-rpl-unk</skos:prefLabel>
        <skos:scopeNote rdf:resource="https://www.isric.org/sites/default/files/isric_report_2014_01.pdf"/>
        <skos:scopeNote>Leenaars J.G.B., A.J.M. van Oostrum and M. Ruiperez Gonzalez, 2014. Africa Soil Profiles Database, Version 1.2. A compilation of georeferenced and standardised legacy soil profile data for Sub-Saharan Africa (with dataset). ISRIC Report 2014/01. Africa Soil Information Service (AfSIS) project and ISRIC - World Soil Information, Wageningen, the Netherlands. See Annex 4.</skos:scopeNote>
        <skos:topConceptOf rdf:resource="http://w3id.org/glosis/model/procedure/bulkDensityFineEarthProcedure"/>
    </owl:NamedIndividual>
    


    <!-- http://w3id.org/glosis/model/procedure/bulkDensityFineEarthProcedure-BlkDensF_fe-unkn -->


    <owl:NamedIndividual rdf:about="http://w3id.org/glosis/model/procedure/bulkDensityFineEarthProcedure-BlkDensF_fe-unkn">
        <rdf:type rdf:resource="http://w3id.org/glosis/model/procedure/BulkDensityFineEarthProcedure"/>
        <rdf:type rdf:resource="http://www.w3.org/2004/02/skos/core#Concept"/>
        <skos:definition>Fine earth. Type of sample unknown, at unknown humidity, corrected for coarse fragments if any</skos:definition>
        <skos:inScheme rdf:resource="http://w3id.org/glosis/model/procedure/bulkDensityFineEarthProcedure"/>
        <skos:notation>BlkDensF_fe-unkn</skos:notation>
        <skos:prefLabel xml:lang="en">BlkDensF_fe-unk</skos:prefLabel>
        <skos:scopeNote rdf:resource="https://www.isric.org/sites/default/files/isric_report_2014_01.pdf"/>
        <skos:scopeNote>Leenaars J.G.B., A.J.M. van Oostrum and M. Ruiperez Gonzalez, 2014. Africa Soil Profiles Database, Version 1.2. A compilation of georeferenced and standardised legacy soil profile data for Sub-Saharan Africa (with dataset). ISRIC Report 2014/01. Africa Soil Information Service (AfSIS) project and ISRIC - World Soil Information, Wageningen, the Netherlands. See Annex 4.</skos:scopeNote>
        <skos:topConceptOf rdf:resource="http://w3id.org/glosis/model/procedure/bulkDensityFineEarthProcedure"/>
    </owl:NamedIndividual>
    


    <!-- http://w3id.org/glosis/model/procedure/bulkDensityFineEarthProcedure-BlkDensF_fe-unkn-fc -->


    <owl:NamedIndividual rdf:about="http://w3id.org/glosis/model/procedure/bulkDensityFineEarthProcedure-BlkDensF_fe-unkn-fc">
        <rdf:type rdf:resource="http://w3id.org/glosis/model/procedure/BulkDensityFineEarthProcedure"/>
        <rdf:type rdf:resource="http://www.w3.org/2004/02/skos/core#Concept"/>
        <skos:definition>Fine earth. Type of sample unknown, at field capacity (0.33 bar, 33 kPa, 330 cm, pF 2.5), corrected for coarse fragments if any</skos:definition>
        <skos:inScheme rdf:resource="http://w3id.org/glosis/model/procedure/bulkDensityFineEarthProcedure"/>
        <skos:notation>BlkDensF_fe-unkn-fc</skos:notation>
        <skos:prefLabel xml:lang="en">BlkDensF_fe-unkn-fc</skos:prefLabel>
        <skos:scopeNote rdf:resource="https://www.isric.org/sites/default/files/isric_report_2014_01.pdf"/>
        <skos:scopeNote>Leenaars J.G.B., A.J.M. van Oostrum and M. Ruiperez Gonzalez, 2014. Africa Soil Profiles Database, Version 1.2. A compilation of georeferenced and standardised legacy soil profile data for Sub-Saharan Africa (with dataset). ISRIC Report 2014/01. Africa Soil Information Service (AfSIS) project and ISRIC - World Soil Information, Wageningen, the Netherlands. See Annex 4.</skos:scopeNote>
        <skos:topConceptOf rdf:resource="http://w3id.org/glosis/model/procedure/bulkDensityFineEarthProcedure"/>
    </owl:NamedIndividual>
    


    <!-- http://w3id.org/glosis/model/procedure/bulkDensityFineEarthProcedure-BlkDensF_fe-unkn-od -->


    <owl:NamedIndividual rdf:about="http://w3id.org/glosis/model/procedure/bulkDensityFineEarthProcedure-BlkDensF_fe-unkn-od">
        <rdf:type rdf:resource="http://w3id.org/glosis/model/procedure/BulkDensityFineEarthProcedure"/>
        <rdf:type rdf:resource="http://www.w3.org/2004/02/skos/core#Concept"/>
        <skos:definition>Fine earth. Type of sample unknown, at oven dry, corrected for coarse fragments if any</skos:definition>
        <skos:inScheme rdf:resource="http://w3id.org/glosis/model/procedure/bulkDensityFineEarthProcedure"/>
        <skos:notation>BlkDensF_fe-unkn-od</skos:notation>
        <skos:prefLabel xml:lang="en">BlkDensF_fe-unkn-od</skos:prefLabel>
        <skos:scopeNote rdf:resource="https://www.isric.org/sites/default/files/isric_report_2014_01.pdf"/>
        <skos:scopeNote>Leenaars J.G.B., A.J.M. van Oostrum and M. Ruiperez Gonzalez, 2014. Africa Soil Profiles Database, Version 1.2. A compilation of georeferenced and standardised legacy soil profile data for Sub-Saharan Africa (with dataset). ISRIC Report 2014/01. Africa Soil Information Service (AfSIS) project and ISRIC - World Soil Information, Wageningen, the Netherlands. See Annex 4.</skos:scopeNote>
        <skos:topConceptOf rdf:resource="http://w3id.org/glosis/model/procedure/bulkDensityFineEarthProcedure"/>
    </owl:NamedIndividual>
    


    <!-- http://w3id.org/glosis/model/procedure/bulkDensityWholeSoilProcedure -->


    <owl:NamedIndividual rdf:about="http://w3id.org/glosis/model/procedure/bulkDensityWholeSoilProcedure">
        <rdf:type rdf:resource="http://www.w3.org/2004/02/skos/core#ConceptScheme"/>
        <rdfs:label xml:lang="en">Code list for bulkDensityWholeSoil analysis procedures - codelist scheme</rdfs:label>
        <rdfs:seeAlso rdf:resource="http://w3id.org/glosis/model/procedure/BulkDensityWholeSoilProcedure"/>
        <skos:definition>AfSP-derived interpretation (RwaSP)</skos:definition>
        <skos:note xml:lang="en">This code list provides analysis procedures for bulkDensityWholeSoil.</skos:note>
        <skos:prefLabel xml:lang="en">Code list for bulkDensityWholeSoil analysis procedures - codelist scheme</skos:prefLabel>
    </owl:NamedIndividual>
    


    <!-- http://w3id.org/glosis/model/procedure/bulkDensityWholeSoilProcedure-BlkDensW_we-cl-fc -->


    <owl:NamedIndividual rdf:about="http://w3id.org/glosis/model/procedure/bulkDensityWholeSoilProcedure-BlkDensW_we-cl-fc">
        <rdf:type rdf:resource="http://w3id.org/glosis/model/procedure/BulkDensityWholeSoilProcedure"/>
        <rdf:type rdf:resource="http://www.w3.org/2004/02/skos/core#Concept"/>
        <skos:definition>Whole earth. Clod samples (natural clods), at field capacity (0.33 bar, 33 kPa, 330 cm, pF 2.5), not corrected for coarse fragments if any</skos:definition>
        <skos:inScheme rdf:resource="http://w3id.org/glosis/model/procedure/bulkDensityWholeSoilProcedure"/>
        <skos:notation>BlkDensW_we-cl-fc</skos:notation>
        <skos:prefLabel xml:lang="en">BlkDensW_we-cl-fc</skos:prefLabel>
        <skos:scopeNote rdf:resource="https://www.isric.org/sites/default/files/isric_report_2014_01.pdf"/>
        <skos:scopeNote>Leenaars J.G.B., A.J.M. van Oostrum and M. Ruiperez Gonzalez, 2014. Africa Soil Profiles Database, Version 1.2. A compilation of georeferenced and standardised legacy soil profile data for Sub-Saharan Africa (with dataset). ISRIC Report 2014/01. Africa Soil Information Service (AfSIS) project and ISRIC - World Soil Information, Wageningen, the Netherlands. See Annex 4.</skos:scopeNote>
        <skos:topConceptOf rdf:resource="http://w3id.org/glosis/model/procedure/bulkDensityWholeSoilProcedure"/>
    </owl:NamedIndividual>
    


    <!-- http://w3id.org/glosis/model/procedure/bulkDensityWholeSoilProcedure-BlkDensW_we-cl-od -->


    <owl:NamedIndividual rdf:about="http://w3id.org/glosis/model/procedure/bulkDensityWholeSoilProcedure-BlkDensW_we-cl-od">
        <rdf:type rdf:resource="http://w3id.org/glosis/model/procedure/BulkDensityWholeSoilProcedure"/>
        <rdf:type rdf:resource="http://www.w3.org/2004/02/skos/core#Concept"/>
        <skos:definition>Whole earth. Clod samples (natural clods), at oven dry, not corrected for coarse fragments if any</skos:definition>
        <skos:inScheme rdf:resource="http://w3id.org/glosis/model/procedure/bulkDensityWholeSoilProcedure"/>
        <skos:notation>BlkDensW_we-cl-od</skos:notation>
        <skos:prefLabel xml:lang="en">BlkDensW_we-cl-od</skos:prefLabel>
        <skos:scopeNote rdf:resource="https://www.isric.org/sites/default/files/isric_report_2014_01.pdf"/>
        <skos:scopeNote>Leenaars J.G.B., A.J.M. van Oostrum and M. Ruiperez Gonzalez, 2014. Africa Soil Profiles Database, Version 1.2. A compilation of georeferenced and standardised legacy soil profile data for Sub-Saharan Africa (with dataset). ISRIC Report 2014/01. Africa Soil Information Service (AfSIS) project and ISRIC - World Soil Information, Wageningen, the Netherlands. See Annex 4.</skos:scopeNote>
        <skos:topConceptOf rdf:resource="http://w3id.org/glosis/model/procedure/bulkDensityWholeSoilProcedure"/>
    </owl:NamedIndividual>
    


    <!-- http://w3id.org/glosis/model/procedure/bulkDensityWholeSoilProcedure-BlkDensW_we-cl-unkn -->


    <owl:NamedIndividual rdf:about="http://w3id.org/glosis/model/procedure/bulkDensityWholeSoilProcedure-BlkDensW_we-cl-unkn">
        <rdf:type rdf:resource="http://w3id.org/glosis/model/procedure/BulkDensityWholeSoilProcedure"/>
        <rdf:type rdf:resource="http://www.w3.org/2004/02/skos/core#Concept"/>
        <skos:definition>Whole earth. Clod samples (natural clods), at unknown humidity, not corrected for coarse fragments if any</skos:definition>
        <skos:inScheme rdf:resource="http://w3id.org/glosis/model/procedure/bulkDensityWholeSoilProcedure"/>
        <skos:notation>BlkDensW_we-cl-unkn</skos:notation>
        <skos:prefLabel xml:lang="en">BlkDensW_we-cl-unk</skos:prefLabel>
        <skos:scopeNote rdf:resource="https://www.isric.org/sites/default/files/isric_report_2014_01.pdf"/>
        <skos:scopeNote>Leenaars J.G.B., A.J.M. van Oostrum and M. Ruiperez Gonzalez, 2014. Africa Soil Profiles Database, Version 1.2. A compilation of georeferenced and standardised legacy soil profile data for Sub-Saharan Africa (with dataset). ISRIC Report 2014/01. Africa Soil Information Service (AfSIS) project and ISRIC - World Soil Information, Wageningen, the Netherlands. See Annex 4.</skos:scopeNote>
        <skos:topConceptOf rdf:resource="http://w3id.org/glosis/model/procedure/bulkDensityWholeSoilProcedure"/>
    </owl:NamedIndividual>
    


    <!-- http://w3id.org/glosis/model/procedure/bulkDensityWholeSoilProcedure-BlkDensW_we-co-fc -->


    <owl:NamedIndividual rdf:about="http://w3id.org/glosis/model/procedure/bulkDensityWholeSoilProcedure-BlkDensW_we-co-fc">
        <rdf:type rdf:resource="http://w3id.org/glosis/model/procedure/BulkDensityWholeSoilProcedure"/>
        <rdf:type rdf:resource="http://www.w3.org/2004/02/skos/core#Concept"/>
        <skos:definition>Whole earth. Core sampling (pF rings), at field capacity (0.33 bar, 33 kPa, 336 cm, pF 2.5), not corrected for coarse fragments if any</skos:definition>
        <skos:inScheme rdf:resource="http://w3id.org/glosis/model/procedure/bulkDensityWholeSoilProcedure"/>
        <skos:notation>BlkDensW_we-co-fc</skos:notation>
        <skos:prefLabel xml:lang="en">BlkDensW_we-co-fc</skos:prefLabel>
        <skos:scopeNote rdf:resource="https://www.isric.org/sites/default/files/isric_report_2014_01.pdf"/>
        <skos:scopeNote>Leenaars J.G.B., A.J.M. van Oostrum and M. Ruiperez Gonzalez, 2014. Africa Soil Profiles Database, Version 1.2. A compilation of georeferenced and standardised legacy soil profile data for Sub-Saharan Africa (with dataset). ISRIC Report 2014/01. Africa Soil Information Service (AfSIS) project and ISRIC - World Soil Information, Wageningen, the Netherlands. See Annex 4.</skos:scopeNote>
        <skos:topConceptOf rdf:resource="http://w3id.org/glosis/model/procedure/bulkDensityWholeSoilProcedure"/>
    </owl:NamedIndividual>
    


    <!-- http://w3id.org/glosis/model/procedure/bulkDensityWholeSoilProcedure-BlkDensW_we-co-od -->


    <owl:NamedIndividual rdf:about="http://w3id.org/glosis/model/procedure/bulkDensityWholeSoilProcedure-BlkDensW_we-co-od">
        <rdf:type rdf:resource="http://w3id.org/glosis/model/procedure/BulkDensityWholeSoilProcedure"/>
        <rdf:type rdf:resource="http://www.w3.org/2004/02/skos/core#Concept"/>
        <skos:definition>Whole earth. Core sampling (pF rings), at oven dry, not corrected for coarse fragments if any</skos:definition>
        <skos:inScheme rdf:resource="http://w3id.org/glosis/model/procedure/bulkDensityWholeSoilProcedure"/>
        <skos:notation>BlkDensW_we-co-od</skos:notation>
        <skos:prefLabel xml:lang="en">BlkDensW_we-co-od</skos:prefLabel>
        <skos:scopeNote rdf:resource="https://www.isric.org/sites/default/files/isric_report_2014_01.pdf"/>
        <skos:scopeNote>Leenaars J.G.B., A.J.M. van Oostrum and M. Ruiperez Gonzalez, 2014. Africa Soil Profiles Database, Version 1.2. A compilation of georeferenced and standardised legacy soil profile data for Sub-Saharan Africa (with dataset). ISRIC Report 2014/01. Africa Soil Information Service (AfSIS) project and ISRIC - World Soil Information, Wageningen, the Netherlands. See Annex 4.</skos:scopeNote>
        <skos:topConceptOf rdf:resource="http://w3id.org/glosis/model/procedure/bulkDensityWholeSoilProcedure"/>
    </owl:NamedIndividual>
    


    <!-- http://w3id.org/glosis/model/procedure/bulkDensityWholeSoilProcedure-BlkDensW_we-co-unkn -->


    <owl:NamedIndividual rdf:about="http://w3id.org/glosis/model/procedure/bulkDensityWholeSoilProcedure-BlkDensW_we-co-unkn">
        <rdf:type rdf:resource="http://w3id.org/glosis/model/procedure/BulkDensityWholeSoilProcedure"/>
        <rdf:type rdf:resource="http://www.w3.org/2004/02/skos/core#Concept"/>
        <skos:definition>Whole earth. Core sampling (pF rings), at unknown humidity, not corrected for coarse fragments if any</skos:definition>
        <skos:inScheme rdf:resource="http://w3id.org/glosis/model/procedure/bulkDensityWholeSoilProcedure"/>
        <skos:notation>BlkDensW_we-co-unkn</skos:notation>
        <skos:prefLabel xml:lang="en">BlkDensW_we-co-unk</skos:prefLabel>
        <skos:scopeNote rdf:resource="https://www.isric.org/sites/default/files/isric_report_2014_01.pdf"/>
        <skos:scopeNote>Leenaars J.G.B., A.J.M. van Oostrum and M. Ruiperez Gonzalez, 2014. Africa Soil Profiles Database, Version 1.2. A compilation of georeferenced and standardised legacy soil profile data for Sub-Saharan Africa (with dataset). ISRIC Report 2014/01. Africa Soil Information Service (AfSIS) project and ISRIC - World Soil Information, Wageningen, the Netherlands. See Annex 4.</skos:scopeNote>
        <skos:topConceptOf rdf:resource="http://w3id.org/glosis/model/procedure/bulkDensityWholeSoilProcedure"/>
    </owl:NamedIndividual>
    


    <!-- http://w3id.org/glosis/model/procedure/bulkDensityWholeSoilProcedure-BlkDensW_we-rpl-unkn -->


    <owl:NamedIndividual rdf:about="http://w3id.org/glosis/model/procedure/bulkDensityWholeSoilProcedure-BlkDensW_we-rpl-unkn">
        <rdf:type rdf:resource="http://w3id.org/glosis/model/procedure/BulkDensityWholeSoilProcedure"/>
        <rdf:type rdf:resource="http://www.w3.org/2004/02/skos/core#Concept"/>
        <skos:definition>Whole earth. Excavation and replacement (i.e. soils too fragile to remove a stable sample) e.g. by auger, at unknown humidity, not corrected for coarse fragments if any</skos:definition>
        <skos:inScheme rdf:resource="http://w3id.org/glosis/model/procedure/bulkDensityWholeSoilProcedure"/>
        <skos:notation>BlkDensW_we-rpl-unkn</skos:notation>
        <skos:prefLabel xml:lang="en">BlkDensW_we-rpl-unk</skos:prefLabel>
        <skos:scopeNote rdf:resource="https://www.isric.org/sites/default/files/isric_report_2014_01.pdf"/>
        <skos:scopeNote>Leenaars J.G.B., A.J.M. van Oostrum and M. Ruiperez Gonzalez, 2014. Africa Soil Profiles Database, Version 1.2. A compilation of georeferenced and standardised legacy soil profile data for Sub-Saharan Africa (with dataset). ISRIC Report 2014/01. Africa Soil Information Service (AfSIS) project and ISRIC - World Soil Information, Wageningen, the Netherlands. See Annex 4.</skos:scopeNote>
        <skos:topConceptOf rdf:resource="http://w3id.org/glosis/model/procedure/bulkDensityWholeSoilProcedure"/>
    </owl:NamedIndividual>
    


    <!-- http://w3id.org/glosis/model/procedure/bulkDensityWholeSoilProcedure-BlkDensW_we-unkn -->


    <owl:NamedIndividual rdf:about="http://w3id.org/glosis/model/procedure/bulkDensityWholeSoilProcedure-BlkDensW_we-unkn">
        <rdf:type rdf:resource="http://w3id.org/glosis/model/procedure/BulkDensityWholeSoilProcedure"/>
        <rdf:type rdf:resource="http://www.w3.org/2004/02/skos/core#Concept"/>
        <skos:definition>Whole earth. Type of sample unknown, at unknown humidity, not corrected for coarse fragments if any</skos:definition>
        <skos:inScheme rdf:resource="http://w3id.org/glosis/model/procedure/bulkDensityWholeSoilProcedure"/>
        <skos:notation>BlkDensW_we-unkn</skos:notation>
        <skos:prefLabel xml:lang="en">BlkDensW_we-unk</skos:prefLabel>
        <skos:scopeNote rdf:resource="https://www.isric.org/sites/default/files/isric_report_2014_01.pdf"/>
        <skos:scopeNote>Leenaars J.G.B., A.J.M. van Oostrum and M. Ruiperez Gonzalez, 2014. Africa Soil Profiles Database, Version 1.2. A compilation of georeferenced and standardised legacy soil profile data for Sub-Saharan Africa (with dataset). ISRIC Report 2014/01. Africa Soil Information Service (AfSIS) project and ISRIC - World Soil Information, Wageningen, the Netherlands. See Annex 4.</skos:scopeNote>
        <skos:topConceptOf rdf:resource="http://w3id.org/glosis/model/procedure/bulkDensityWholeSoilProcedure"/>
    </owl:NamedIndividual>
    


    <!-- http://w3id.org/glosis/model/procedure/carbonInorganicProcedure -->


    <owl:NamedIndividual rdf:about="http://w3id.org/glosis/model/procedure/carbonInorganicProcedure">
        <rdf:type rdf:resource="http://www.w3.org/2004/02/skos/core#ConceptScheme"/>
        <rdfs:label xml:lang="en">Code list for carbonInorganic analysis procedures - codelist scheme</rdfs:label>
        <rdfs:seeAlso rdf:resource="http://w3id.org/glosis/model/procedure/CarbonInorganicProcedure"/>
        <skos:definition>AfSP-derived interpretation (RwaSP)</skos:definition>
        <skos:note xml:lang="en">This code list provides analysis procedures for carbonInorganic.</skos:note>
        <skos:prefLabel xml:lang="en">Code list for carbonInorganic analysis procedures - codelist scheme</skos:prefLabel>
    </owl:NamedIndividual>
    


    <!-- http://w3id.org/glosis/model/procedure/carbonInorganicProcedure-InOrgC_calcul-caco3 -->


    <owl:NamedIndividual rdf:about="http://w3id.org/glosis/model/procedure/carbonInorganicProcedure-InOrgC_calcul-caco3">
        <rdf:type rdf:resource="http://w3id.org/glosis/model/procedure/CarbonInorganicProcedure"/>
        <rdf:type rdf:resource="http://www.w3.org/2004/02/skos/core#Concept"/>
        <skos:definition>Indirect estimate from total carbonate equivalent, with a factor of 0.12 (molar weights: CaCO3 100g/mol, C 12g/mol)</skos:definition>
        <skos:inScheme rdf:resource="http://w3id.org/glosis/model/procedure/carbonInorganicProcedure"/>
        <skos:notation>InOrgC_calcul-caco3</skos:notation>
        <skos:prefLabel xml:lang="en">InOrgC_calcul-caco3</skos:prefLabel>
        <skos:scopeNote rdf:resource="https://www.isric.org/sites/default/files/isric_report_2014_01.pdf"/>
        <skos:scopeNote>Leenaars J.G.B., A.J.M. van Oostrum and M. Ruiperez Gonzalez, 2014. Africa Soil Profiles Database, Version 1.2. A compilation of georeferenced and standardised legacy soil profile data for Sub-Saharan Africa (with dataset). ISRIC Report 2014/01. Africa Soil Information Service (AfSIS) project and ISRIC - World Soil Information, Wageningen, the Netherlands. See Annex 4.</skos:scopeNote>
        <skos:topConceptOf rdf:resource="http://w3id.org/glosis/model/procedure/carbonInorganicProcedure"/>
    </owl:NamedIndividual>
    


    <!-- http://w3id.org/glosis/model/procedure/carbonInorganicProcedure-InOrgC_calcul-tc-oc -->


    <owl:NamedIndividual rdf:about="http://w3id.org/glosis/model/procedure/carbonInorganicProcedure-InOrgC_calcul-tc-oc">
        <rdf:type rdf:resource="http://w3id.org/glosis/model/procedure/CarbonInorganicProcedure"/>
        <rdf:type rdf:resource="http://www.w3.org/2004/02/skos/core#Concept"/>
        <skos:definition>Indirect estimate (total carbon minus organic carbon = inorganic carbon)</skos:definition>
        <skos:inScheme rdf:resource="http://w3id.org/glosis/model/procedure/carbonInorganicProcedure"/>
        <skos:notation>InOrgC_calcul-tc-oc</skos:notation>
        <skos:prefLabel xml:lang="en">InOrgC_calcul-tc-oc</skos:prefLabel>
        <skos:scopeNote rdf:resource="https://www.isric.org/sites/default/files/isric_report_2014_01.pdf"/>
        <skos:scopeNote>Leenaars J.G.B., A.J.M. van Oostrum and M. Ruiperez Gonzalez, 2014. Africa Soil Profiles Database, Version 1.2. A compilation of georeferenced and standardised legacy soil profile data for Sub-Saharan Africa (with dataset). ISRIC Report 2014/01. Africa Soil Information Service (AfSIS) project and ISRIC - World Soil Information, Wageningen, the Netherlands. See Annex 4.</skos:scopeNote>
        <skos:topConceptOf rdf:resource="http://w3id.org/glosis/model/procedure/carbonInorganicProcedure"/>
    </owl:NamedIndividual>
    


    <!-- http://w3id.org/glosis/model/procedure/carbonOrganicProcedure -->


    <owl:NamedIndividual rdf:about="http://w3id.org/glosis/model/procedure/carbonOrganicProcedure">
        <rdf:type rdf:resource="http://www.w3.org/2004/02/skos/core#ConceptScheme"/>
        <rdfs:label xml:lang="en">Code list for carbonOrganic analysis procedures - codelist scheme</rdfs:label>
        <rdfs:seeAlso rdf:resource="http://w3id.org/glosis/model/procedure/CarbonOrganicProcedure"/>
        <skos:definition>AfSP-derived interpretation (RwaSP)</skos:definition>
        <skos:note xml:lang="en">This code list provides analysis procedures for carbonOrganic.</skos:note>
        <skos:prefLabel xml:lang="en">Code list for carbonOrganic analysis procedures - codelist scheme</skos:prefLabel>
    </owl:NamedIndividual>
    


    <!-- http://w3id.org/glosis/model/procedure/carbonOrganicProcedure-OrgC_acid-dc -->


    <owl:NamedIndividual rdf:about="http://w3id.org/glosis/model/procedure/carbonOrganicProcedure-OrgC_acid-dc">
        <rdf:type rdf:resource="http://w3id.org/glosis/model/procedure/CarbonOrganicProcedure"/>
        <rdf:type rdf:resource="http://www.w3.org/2004/02/skos/core#Concept"/>
        <skos:definition>Acidified dry combustion or dry oxidation methods (after removal of carbonates)</skos:definition>
        <skos:inScheme rdf:resource="http://w3id.org/glosis/model/procedure/carbonOrganicProcedure"/>
        <skos:notation>OrgC_acid-dc</skos:notation>
        <skos:prefLabel xml:lang="en">OrgC_acid-dc</skos:prefLabel>
        <skos:scopeNote rdf:resource="https://www.isric.org/sites/default/files/isric_report_2014_01.pdf"/>
        <skos:scopeNote>Leenaars J.G.B., A.J.M. van Oostrum and M. Ruiperez Gonzalez, 2014. Africa Soil Profiles Database, Version 1.2. A compilation of georeferenced and standardised legacy soil profile data for Sub-Saharan Africa (with dataset). ISRIC Report 2014/01. Africa Soil Information Service (AfSIS) project and ISRIC - World Soil Information, Wageningen, the Netherlands. See Annex 4.</skos:scopeNote>
        <skos:topConceptOf rdf:resource="http://w3id.org/glosis/model/procedure/carbonOrganicProcedure"/>
    </owl:NamedIndividual>
    


    <!-- http://w3id.org/glosis/model/procedure/carbonOrganicProcedure-OrgC_acid-dc-ht -->


    <owl:NamedIndividual rdf:about="http://w3id.org/glosis/model/procedure/carbonOrganicProcedure-OrgC_acid-dc-ht">
        <rdf:type rdf:resource="http://w3id.org/glosis/model/procedure/CarbonOrganicProcedure"/>
        <rdf:type rdf:resource="http://www.w3.org/2004/02/skos/core#Concept"/>
        <skos:definition>Acidified. Dry combustion at 1200 C and colometric CO2 measurement (Schlichting et al. 1995)</skos:definition>
        <skos:inScheme rdf:resource="http://w3id.org/glosis/model/procedure/carbonOrganicProcedure"/>
        <skos:notation>OrgC_acid-dc-ht</skos:notation>
        <skos:prefLabel xml:lang="en">OrgC_acid-dc-ht</skos:prefLabel>
        <skos:scopeNote>Schlichting E, Blume HP, Stahr K (1995) Soils Practical (in German). Blackwell, Berlin</skos:scopeNote>
        <skos:topConceptOf rdf:resource="http://w3id.org/glosis/model/procedure/carbonOrganicProcedure"/>
    </owl:NamedIndividual>
    


    <!-- http://w3id.org/glosis/model/procedure/carbonOrganicProcedure-OrgC_acid-dc-ht-analyser -->


    <owl:NamedIndividual rdf:about="http://w3id.org/glosis/model/procedure/carbonOrganicProcedure-OrgC_acid-dc-ht-analyser">
        <rdf:type rdf:resource="http://w3id.org/glosis/model/procedure/CarbonOrganicProcedure"/>
        <rdf:type rdf:resource="http://www.w3.org/2004/02/skos/core#Concept"/>
        <skos:definition>Acidified. Furnace combustion (e.g., LECO combustion analyzer, Dumas method)</skos:definition>
        <skos:inScheme rdf:resource="http://w3id.org/glosis/model/procedure/carbonOrganicProcedure"/>
        <skos:notation>OrgC_acid-dc-ht-analyser</skos:notation>
        <skos:prefLabel xml:lang="en">OrgC_acid-dc-ht-analyser</skos:prefLabel>
        <skos:scopeNote rdf:resource="https://www.isric.org/sites/default/files/isric_report_2014_01.pdf"/>
        <skos:scopeNote>Leenaars J.G.B., A.J.M. van Oostrum and M. Ruiperez Gonzalez, 2014. Africa Soil Profiles Database, Version 1.2. A compilation of georeferenced and standardised legacy soil profile data for Sub-Saharan Africa (with dataset). ISRIC Report 2014/01. Africa Soil Information Service (AfSIS) project and ISRIC - World Soil Information, Wageningen, the Netherlands. See Annex 4.</skos:scopeNote>
        <skos:topConceptOf rdf:resource="http://w3id.org/glosis/model/procedure/carbonOrganicProcedure"/>
    </owl:NamedIndividual>
    


    <!-- http://w3id.org/glosis/model/procedure/carbonOrganicProcedure-OrgC_acid-dc-lt -->


    <owl:NamedIndividual rdf:about="http://w3id.org/glosis/model/procedure/carbonOrganicProcedure-OrgC_acid-dc-lt">
        <rdf:type rdf:resource="http://w3id.org/glosis/model/procedure/CarbonOrganicProcedure"/>
        <rdf:type rdf:resource="http://www.w3.org/2004/02/skos/core#Concept"/>
        <skos:definition>Acidified. Dry combustion at 500 C</skos:definition>
        <skos:inScheme rdf:resource="http://w3id.org/glosis/model/procedure/carbonOrganicProcedure"/>
        <skos:notation>OrgC_acid-dc-lt</skos:notation>
        <skos:prefLabel xml:lang="en">OrgC_acid-dc-lt</skos:prefLabel>
        <skos:scopeNote rdf:resource="https://www.isric.org/sites/default/files/isric_report_2014_01.pdf"/>
        <skos:scopeNote>Leenaars J.G.B., A.J.M. van Oostrum and M. Ruiperez Gonzalez, 2014. Africa Soil Profiles Database, Version 1.2. A compilation of georeferenced and standardised legacy soil profile data for Sub-Saharan Africa (with dataset). ISRIC Report 2014/01. Africa Soil Information Service (AfSIS) project and ISRIC - World Soil Information, Wageningen, the Netherlands. See Annex 4.</skos:scopeNote>
        <skos:topConceptOf rdf:resource="http://w3id.org/glosis/model/procedure/carbonOrganicProcedure"/>
    </owl:NamedIndividual>
    


    <!-- http://w3id.org/glosis/model/procedure/carbonOrganicProcedure-OrgC_acid-dc-lt-loi -->


    <owl:NamedIndividual rdf:about="http://w3id.org/glosis/model/procedure/carbonOrganicProcedure-OrgC_acid-dc-lt-loi">
        <rdf:type rdf:resource="http://w3id.org/glosis/model/procedure/CarbonOrganicProcedure"/>
        <rdf:type rdf:resource="http://www.w3.org/2004/02/skos/core#Concept"/>
        <skos:definition>Acidified. Loss on ignition (NL)</skos:definition>
        <skos:inScheme rdf:resource="http://w3id.org/glosis/model/procedure/carbonOrganicProcedure"/>
        <skos:notation>OrgC_acid-dc-lt-loi</skos:notation>
        <skos:prefLabel xml:lang="en">OrgC_acid-dc-lt-loi</skos:prefLabel>
        <skos:scopeNote rdf:resource="https://www.isric.org/sites/default/files/isric_report_2014_01.pdf"/>
        <skos:scopeNote>Leenaars J.G.B., A.J.M. van Oostrum and M. Ruiperez Gonzalez, 2014. Africa Soil Profiles Database, Version 1.2. A compilation of georeferenced and standardised legacy soil profile data for Sub-Saharan Africa (with dataset). ISRIC Report 2014/01. Africa Soil Information Service (AfSIS) project and ISRIC - World Soil Information, Wageningen, the Netherlands. See Annex 4.</skos:scopeNote>
        <skos:topConceptOf rdf:resource="http://w3id.org/glosis/model/procedure/carbonOrganicProcedure"/>
    </owl:NamedIndividual>
    


    <!-- http://w3id.org/glosis/model/procedure/carbonOrganicProcedure-OrgC_acid-dc-mt -->


    <owl:NamedIndividual rdf:about="http://w3id.org/glosis/model/procedure/carbonOrganicProcedure-OrgC_acid-dc-mt">
        <rdf:type rdf:resource="http://w3id.org/glosis/model/procedure/CarbonOrganicProcedure"/>
        <rdf:type rdf:resource="http://www.w3.org/2004/02/skos/core#Concept"/>
        <skos:definition>Acidified. Dry combustion at 840 C</skos:definition>
        <skos:inScheme rdf:resource="http://w3id.org/glosis/model/procedure/carbonOrganicProcedure"/>
        <skos:notation>OrgC_acid-dc-mt</skos:notation>
        <skos:prefLabel xml:lang="en">OrgC_acid-dc-mt</skos:prefLabel>
        <skos:scopeNote rdf:resource="https://www.isric.org/sites/default/files/isric_report_2014_01.pdf"/>
        <skos:scopeNote>Leenaars J.G.B., A.J.M. van Oostrum and M. Ruiperez Gonzalez, 2014. Africa Soil Profiles Database, Version 1.2. A compilation of georeferenced and standardised legacy soil profile data for Sub-Saharan Africa (with dataset). ISRIC Report 2014/01. Africa Soil Information Service (AfSIS) project and ISRIC - World Soil Information, Wageningen, the Netherlands. See Annex 4.</skos:scopeNote>
        <skos:topConceptOf rdf:resource="http://w3id.org/glosis/model/procedure/carbonOrganicProcedure"/>
    </owl:NamedIndividual>
    


    <!-- http://w3id.org/glosis/model/procedure/carbonOrganicProcedure-OrgC_acid-dc-spec -->


    <owl:NamedIndividual rdf:about="http://w3id.org/glosis/model/procedure/carbonOrganicProcedure-OrgC_acid-dc-spec">
        <rdf:type rdf:resource="http://w3id.org/glosis/model/procedure/CarbonOrganicProcedure"/>
        <rdf:type rdf:resource="http://www.w3.org/2004/02/skos/core#Concept"/>
        <skos:definition>Spectrally measured and converted to Acidified dry combustion or dry oxidation methods (after removal of carbonates)</skos:definition>
        <skos:inScheme rdf:resource="http://w3id.org/glosis/model/procedure/carbonOrganicProcedure"/>
        <skos:notation>OrgC_acid-dc-spec</skos:notation>
        <skos:prefLabel xml:lang="en">OrgC_acid-dc-spec</skos:prefLabel>
        <skos:scopeNote rdf:resource="https://www.isric.org/sites/default/files/isric_report_2014_01.pdf"/>
        <skos:scopeNote>Leenaars J.G.B., A.J.M. van Oostrum and M. Ruiperez Gonzalez, 2014. Africa Soil Profiles Database, Version 1.2. A compilation of georeferenced and standardised legacy soil profile data for Sub-Saharan Africa (with dataset). ISRIC Report 2014/01. Africa Soil Information Service (AfSIS) project and ISRIC - World Soil Information, Wageningen, the Netherlands. See Annex 4.</skos:scopeNote>
        <skos:topConceptOf rdf:resource="http://w3id.org/glosis/model/procedure/carbonOrganicProcedure"/>
    </owl:NamedIndividual>
    


    <!-- http://w3id.org/glosis/model/procedure/carbonOrganicProcedure-OrgC_calcul-tc-ic -->


    <owl:NamedIndividual rdf:about="http://w3id.org/glosis/model/procedure/carbonOrganicProcedure-OrgC_calcul-tc-ic">
        <rdf:type rdf:resource="http://w3id.org/glosis/model/procedure/CarbonOrganicProcedure"/>
        <rdf:type rdf:resource="http://www.w3.org/2004/02/skos/core#Concept"/>
        <skos:definition>Calculated as total carbon minus inorganic carbon</skos:definition>
        <skos:inScheme rdf:resource="http://w3id.org/glosis/model/procedure/carbonOrganicProcedure"/>
        <skos:notation>OrgC_calcul-tc-ic</skos:notation>
        <skos:prefLabel xml:lang="en">OrgC_calcul-tc-ic</skos:prefLabel>
        <skos:scopeNote rdf:resource="https://www.isric.org/sites/default/files/isric_report_2014_01.pdf"/>
        <skos:scopeNote>Leenaars J.G.B., A.J.M. van Oostrum and M. Ruiperez Gonzalez, 2014. Africa Soil Profiles Database, Version 1.2. A compilation of georeferenced and standardised legacy soil profile data for Sub-Saharan Africa (with dataset). ISRIC Report 2014/01. Africa Soil Information Service (AfSIS) project and ISRIC - World Soil Information, Wageningen, the Netherlands. See Annex 4.</skos:scopeNote>
        <skos:topConceptOf rdf:resource="http://w3id.org/glosis/model/procedure/carbonOrganicProcedure"/>
    </owl:NamedIndividual>
    


    <!-- http://w3id.org/glosis/model/procedure/carbonOrganicProcedure-OrgC_dc -->


    <owl:NamedIndividual rdf:about="http://w3id.org/glosis/model/procedure/carbonOrganicProcedure-OrgC_dc">
        <rdf:type rdf:resource="http://w3id.org/glosis/model/procedure/CarbonOrganicProcedure"/>
        <rdf:type rdf:resource="http://www.w3.org/2004/02/skos/core#Concept"/>
        <skos:definition>Unacidified. Dry combustion or dry oxidation methods (without prior removal of carbonates)</skos:definition>
        <skos:inScheme rdf:resource="http://w3id.org/glosis/model/procedure/carbonOrganicProcedure"/>
        <skos:notation>OrgC_dc</skos:notation>
        <skos:prefLabel xml:lang="en">OrgC_dc</skos:prefLabel>
        <skos:scopeNote rdf:resource="https://www.isric.org/sites/default/files/isric_report_2014_01.pdf"/>
        <skos:scopeNote>Leenaars J.G.B., A.J.M. van Oostrum and M. Ruiperez Gonzalez, 2014. Africa Soil Profiles Database, Version 1.2. A compilation of georeferenced and standardised legacy soil profile data for Sub-Saharan Africa (with dataset). ISRIC Report 2014/01. Africa Soil Information Service (AfSIS) project and ISRIC - World Soil Information, Wageningen, the Netherlands. See Annex 4.</skos:scopeNote>
        <skos:topConceptOf rdf:resource="http://w3id.org/glosis/model/procedure/carbonOrganicProcedure"/>
    </owl:NamedIndividual>
    


    <!-- http://w3id.org/glosis/model/procedure/carbonOrganicProcedure-OrgC_dc-ht -->


    <owl:NamedIndividual rdf:about="http://w3id.org/glosis/model/procedure/carbonOrganicProcedure-OrgC_dc-ht">
        <rdf:type rdf:resource="http://w3id.org/glosis/model/procedure/CarbonOrganicProcedure"/>
        <rdf:type rdf:resource="http://www.w3.org/2004/02/skos/core#Concept"/>
        <skos:definition>Unacidified. Dry combustion at high temperature (e.g. 1200 C and colometric CO2 measurement (Schlichting et al. 1995)</skos:definition>
        <skos:inScheme rdf:resource="http://w3id.org/glosis/model/procedure/carbonOrganicProcedure"/>
        <skos:notation>OrgC_dc-ht</skos:notation>
        <skos:prefLabel xml:lang="en">OrgC_dc-ht</skos:prefLabel>
        <skos:scopeNote>Schlichting E, Blume HP, Stahr K (1995) Soils Practical (in German). Blackwell, Berlin</skos:scopeNote>
        <skos:topConceptOf rdf:resource="http://w3id.org/glosis/model/procedure/carbonOrganicProcedure"/>
    </owl:NamedIndividual>
    


    <!-- http://w3id.org/glosis/model/procedure/carbonOrganicProcedure-OrgC_dc-ht-analyser -->


    <owl:NamedIndividual rdf:about="http://w3id.org/glosis/model/procedure/carbonOrganicProcedure-OrgC_dc-ht-analyser">
        <rdf:type rdf:resource="http://w3id.org/glosis/model/procedure/CarbonOrganicProcedure"/>
        <rdf:type rdf:resource="http://www.w3.org/2004/02/skos/core#Concept"/>
        <skos:definition>Unacidified. Dry combustion by furnace (e.g., LECO combustion analyzer, Dumas method). Is total Carbon?</skos:definition>
        <skos:inScheme rdf:resource="http://w3id.org/glosis/model/procedure/carbonOrganicProcedure"/>
        <skos:notation>OrgC_dc-ht-analyser</skos:notation>
        <skos:prefLabel xml:lang="en">OrgC_dc-ht-analyser</skos:prefLabel>
        <skos:scopeNote rdf:resource="https://www.isric.org/sites/default/files/isric_report_2014_01.pdf"/>
        <skos:scopeNote>Leenaars J.G.B., A.J.M. van Oostrum and M. Ruiperez Gonzalez, 2014. Africa Soil Profiles Database, Version 1.2. A compilation of georeferenced and standardised legacy soil profile data for Sub-Saharan Africa (with dataset). ISRIC Report 2014/01. Africa Soil Information Service (AfSIS) project and ISRIC - World Soil Information, Wageningen, the Netherlands. See Annex 4.</skos:scopeNote>
        <skos:topConceptOf rdf:resource="http://w3id.org/glosis/model/procedure/carbonOrganicProcedure"/>
    </owl:NamedIndividual>
    


    <!-- http://w3id.org/glosis/model/procedure/carbonOrganicProcedure-OrgC_dc-lt -->


    <owl:NamedIndividual rdf:about="http://w3id.org/glosis/model/procedure/carbonOrganicProcedure-OrgC_dc-lt">
        <rdf:type rdf:resource="http://w3id.org/glosis/model/procedure/CarbonOrganicProcedure"/>
        <rdf:type rdf:resource="http://www.w3.org/2004/02/skos/core#Concept"/>
        <skos:definition>Unacidified. Dry combustion at low temperature e.g. 500 C</skos:definition>
        <skos:inScheme rdf:resource="http://w3id.org/glosis/model/procedure/carbonOrganicProcedure"/>
        <skos:notation>OrgC_dc-lt</skos:notation>
        <skos:prefLabel xml:lang="en">OrgC_dc-lt</skos:prefLabel>
        <skos:scopeNote rdf:resource="https://www.isric.org/sites/default/files/isric_report_2014_01.pdf"/>
        <skos:scopeNote>Leenaars J.G.B., A.J.M. van Oostrum and M. Ruiperez Gonzalez, 2014. Africa Soil Profiles Database, Version 1.2. A compilation of georeferenced and standardised legacy soil profile data for Sub-Saharan Africa (with dataset). ISRIC Report 2014/01. Africa Soil Information Service (AfSIS) project and ISRIC - World Soil Information, Wageningen, the Netherlands. See Annex 4.</skos:scopeNote>
        <skos:topConceptOf rdf:resource="http://w3id.org/glosis/model/procedure/carbonOrganicProcedure"/>
    </owl:NamedIndividual>
    


    <!-- http://w3id.org/glosis/model/procedure/carbonOrganicProcedure-OrgC_dc-lt-loi -->


    <owl:NamedIndividual rdf:about="http://w3id.org/glosis/model/procedure/carbonOrganicProcedure-OrgC_dc-lt-loi">
        <rdf:type rdf:resource="http://w3id.org/glosis/model/procedure/CarbonOrganicProcedure"/>
        <rdf:type rdf:resource="http://www.w3.org/2004/02/skos/core#Concept"/>
        <skos:definition>Unacidified. Loss on ignition (NL) is total Organic Carbon</skos:definition>
        <skos:inScheme rdf:resource="http://w3id.org/glosis/model/procedure/carbonOrganicProcedure"/>
        <skos:notation>OrgC_dc-lt-loi</skos:notation>
        <skos:prefLabel xml:lang="en">OrgC_dc-lt-loi</skos:prefLabel>
        <skos:scopeNote rdf:resource="https://www.isric.org/sites/default/files/isric_report_2014_01.pdf"/>
        <skos:scopeNote>Leenaars J.G.B., A.J.M. van Oostrum and M. Ruiperez Gonzalez, 2014. Africa Soil Profiles Database, Version 1.2. A compilation of georeferenced and standardised legacy soil profile data for Sub-Saharan Africa (with dataset). ISRIC Report 2014/01. Africa Soil Information Service (AfSIS) project and ISRIC - World Soil Information, Wageningen, the Netherlands. See Annex 4.</skos:scopeNote>
        <skos:topConceptOf rdf:resource="http://w3id.org/glosis/model/procedure/carbonOrganicProcedure"/>
    </owl:NamedIndividual>
    


    <!-- http://w3id.org/glosis/model/procedure/carbonOrganicProcedure-OrgC_dc-mt -->


    <owl:NamedIndividual rdf:about="http://w3id.org/glosis/model/procedure/carbonOrganicProcedure-OrgC_dc-mt">
        <rdf:type rdf:resource="http://w3id.org/glosis/model/procedure/CarbonOrganicProcedure"/>
        <rdf:type rdf:resource="http://www.w3.org/2004/02/skos/core#Concept"/>
        <skos:definition>Unacidified. Dry combustion at medium temperature e.g. 840 C</skos:definition>
        <skos:inScheme rdf:resource="http://w3id.org/glosis/model/procedure/carbonOrganicProcedure"/>
        <skos:notation>OrgC_dc-mt</skos:notation>
        <skos:prefLabel xml:lang="en">OrgC_dc-mt</skos:prefLabel>
        <skos:scopeNote rdf:resource="https://www.isric.org/sites/default/files/isric_report_2014_01.pdf"/>
        <skos:scopeNote>Leenaars J.G.B., A.J.M. van Oostrum and M. Ruiperez Gonzalez, 2014. Africa Soil Profiles Database, Version 1.2. A compilation of georeferenced and standardised legacy soil profile data for Sub-Saharan Africa (with dataset). ISRIC Report 2014/01. Africa Soil Information Service (AfSIS) project and ISRIC - World Soil Information, Wageningen, the Netherlands. See Annex 4.</skos:scopeNote>
        <skos:topConceptOf rdf:resource="http://w3id.org/glosis/model/procedure/carbonOrganicProcedure"/>
    </owl:NamedIndividual>
    


    <!-- http://w3id.org/glosis/model/procedure/carbonOrganicProcedure-OrgC_dc-spec -->


    <owl:NamedIndividual rdf:about="http://w3id.org/glosis/model/procedure/carbonOrganicProcedure-OrgC_dc-spec">
        <rdf:type rdf:resource="http://w3id.org/glosis/model/procedure/CarbonOrganicProcedure"/>
        <rdf:type rdf:resource="http://www.w3.org/2004/02/skos/core#Concept"/>
        <skos:definition>Spectrally measured and converted to Unacidified Dry combustion or dry oxidation methods</skos:definition>
        <skos:inScheme rdf:resource="http://w3id.org/glosis/model/procedure/carbonOrganicProcedure"/>
        <skos:notation>OrgC_dc-spec</skos:notation>
        <skos:prefLabel xml:lang="en">OrgC_dc-spec</skos:prefLabel>
        <skos:scopeNote rdf:resource="https://www.isric.org/sites/default/files/isric_report_2014_01.pdf"/>
        <skos:scopeNote>Leenaars J.G.B., A.J.M. van Oostrum and M. Ruiperez Gonzalez, 2014. Africa Soil Profiles Database, Version 1.2. A compilation of georeferenced and standardised legacy soil profile data for Sub-Saharan Africa (with dataset). ISRIC Report 2014/01. Africa Soil Information Service (AfSIS) project and ISRIC - World Soil Information, Wageningen, the Netherlands. See Annex 4.</skos:scopeNote>
        <skos:topConceptOf rdf:resource="http://w3id.org/glosis/model/procedure/carbonOrganicProcedure"/>
    </owl:NamedIndividual>
    


    <!-- http://w3id.org/glosis/model/procedure/carbonOrganicProcedure-OrgC_wc -->


    <owl:NamedIndividual rdf:about="http://w3id.org/glosis/model/procedure/carbonOrganicProcedure-OrgC_wc">
        <rdf:type rdf:resource="http://w3id.org/glosis/model/procedure/CarbonOrganicProcedure"/>
        <rdf:type rdf:resource="http://www.w3.org/2004/02/skos/core#Concept"/>
        <skos:definition>Wet oxidation or wet combustion methods</skos:definition>
        <skos:inScheme rdf:resource="http://w3id.org/glosis/model/procedure/carbonOrganicProcedure"/>
        <skos:notation>OrgC_wc</skos:notation>
        <skos:prefLabel xml:lang="en">OrgC_wc</skos:prefLabel>
        <skos:topConceptOf rdf:resource="http://w3id.org/glosis/model/procedure/carbonOrganicProcedure"/>
    </owl:NamedIndividual>
    


    <!-- http://w3id.org/glosis/model/procedure/carbonOrganicProcedure-OrgC_wc-cro3-jackson -->


    <owl:NamedIndividual rdf:about="http://w3id.org/glosis/model/procedure/carbonOrganicProcedure-OrgC_wc-cro3-jackson">
        <rdf:type rdf:resource="http://w3id.org/glosis/model/procedure/CarbonOrganicProcedure"/>
        <rdf:type rdf:resource="http://www.w3.org/2004/02/skos/core#Concept"/>
        <skos:definition>Wet oxidation according to Jackson (1958) with chromic acid digestion</skos:definition>
        <skos:inScheme rdf:resource="http://w3id.org/glosis/model/procedure/carbonOrganicProcedure"/>
        <skos:notation>OrgC_wc-cro3-jackson</skos:notation>
        <skos:prefLabel xml:lang="en">OrgC_wc-cro3-jackso</skos:prefLabel>
        <skos:scopeNote>Jackson, M. L. (1958) Soil Chemical Analysis. Prentice-Hall, Englewood Cliffs, New Jersey.</skos:scopeNote>
        <skos:topConceptOf rdf:resource="http://w3id.org/glosis/model/procedure/carbonOrganicProcedure"/>
    </owl:NamedIndividual>
    


    <!-- http://w3id.org/glosis/model/procedure/carbonOrganicProcedure-OrgC_wc-cro3-kalembra -->


    <owl:NamedIndividual rdf:about="http://w3id.org/glosis/model/procedure/carbonOrganicProcedure-OrgC_wc-cro3-kalembra">
        <rdf:type rdf:resource="http://w3id.org/glosis/model/procedure/CarbonOrganicProcedure"/>
        <rdf:type rdf:resource="http://www.w3.org/2004/02/skos/core#Concept"/>
        <skos:definition>Wet oxidation according to Kalembra and Jenkinson (1973) with acid dichromate</skos:definition>
        <skos:inScheme rdf:resource="http://w3id.org/glosis/model/procedure/carbonOrganicProcedure"/>
        <skos:notation>OrgC_wc-cro3-kalembra</skos:notation>
        <skos:prefLabel xml:lang="en">OrgC_wc-cro3-kalembra</skos:prefLabel>
        <skos:scopeNote rdf:resource="https://doi.org/10.1002/jsfa.2740240910"/>
        <skos:topConceptOf rdf:resource="http://w3id.org/glosis/model/procedure/carbonOrganicProcedure"/>
    </owl:NamedIndividual>
    


    <!-- http://w3id.org/glosis/model/procedure/carbonOrganicProcedure-OrgC_wc-cro3-knopp -->


    <owl:NamedIndividual rdf:about="http://w3id.org/glosis/model/procedure/carbonOrganicProcedure-OrgC_wc-cro3-knopp">
        <rdf:type rdf:resource="http://w3id.org/glosis/model/procedure/CarbonOrganicProcedure"/>
        <rdf:type rdf:resource="http://www.w3.org/2004/02/skos/core#Concept"/>
        <skos:definition>Wet oxidation according to Knopp with chromic acid and gravimetric determination of CO2</skos:definition>
        <skos:inScheme rdf:resource="http://w3id.org/glosis/model/procedure/carbonOrganicProcedure"/>
        <skos:notation>OrgC_wc-cro3-knopp</skos:notation>
        <skos:prefLabel xml:lang="en">OrgC_wc-cro3-knopp</skos:prefLabel>
        <skos:scopeNote rdf:resource="https://www.isric.org/sites/default/files/isric_report_2014_01.pdf"/>
        <skos:scopeNote>Leenaars J.G.B., A.J.M. van Oostrum and M. Ruiperez Gonzalez, 2014. Africa Soil Profiles Database, Version 1.2. A compilation of georeferenced and standardised legacy soil profile data for Sub-Saharan Africa (with dataset). ISRIC Report 2014/01. Africa Soil Information Service (AfSIS) project and ISRIC - World Soil Information, Wageningen, the Netherlands. See Annex 4.</skos:scopeNote>
        <skos:topConceptOf rdf:resource="http://w3id.org/glosis/model/procedure/carbonOrganicProcedure"/>
    </owl:NamedIndividual>
    


    <!-- http://w3id.org/glosis/model/procedure/carbonOrganicProcedure-OrgC_wc-cro3-kurmies -->


    <owl:NamedIndividual rdf:about="http://w3id.org/glosis/model/procedure/carbonOrganicProcedure-OrgC_wc-cro3-kurmies">
        <rdf:type rdf:resource="http://w3id.org/glosis/model/procedure/CarbonOrganicProcedure"/>
        <rdf:type rdf:resource="http://www.w3.org/2004/02/skos/core#Concept"/>
        <skos:definition>Wet oxidation according to Kurmies with K2Cr2O7+H2SO4</skos:definition>
        <skos:inScheme rdf:resource="http://w3id.org/glosis/model/procedure/carbonOrganicProcedure"/>
        <skos:notation>OrgC_wc-cro3-kurmies</skos:notation>
        <skos:prefLabel xml:lang="en">OrgC_wc-cro3-kurmies</skos:prefLabel>
        <skos:scopeNote>B. KURMIES, Z. Pflanzenernühr. Dung. u Bodenk., 44 (1949) 121</skos:scopeNote>
        <skos:topConceptOf rdf:resource="http://w3id.org/glosis/model/procedure/carbonOrganicProcedure"/>
    </owl:NamedIndividual>
    


    <!-- http://w3id.org/glosis/model/procedure/carbonOrganicProcedure-OrgC_wc-cro3-nelson -->


    <owl:NamedIndividual rdf:about="http://w3id.org/glosis/model/procedure/carbonOrganicProcedure-OrgC_wc-cro3-nelson">
        <rdf:type rdf:resource="http://w3id.org/glosis/model/procedure/CarbonOrganicProcedure"/>
        <rdf:type rdf:resource="http://www.w3.org/2004/02/skos/core#Concept"/>
        <skos:definition>Wet oxidation according to Nelson and Sommers (1996)</skos:definition>
        <skos:inScheme rdf:resource="http://w3id.org/glosis/model/procedure/carbonOrganicProcedure"/>
        <skos:notation>OrgC_wc-cro3-nelson</skos:notation>
        <skos:prefLabel xml:lang="en">OrgC_wc-cro3-nelso</skos:prefLabel>
        <skos:scopeNote>Nelson and Sommers (1996) in: Sparks DL (ed.). Soil Sci. Soc. Am. book series 5, part 3, pp 961-1010.</skos:scopeNote>
        <skos:topConceptOf rdf:resource="http://w3id.org/glosis/model/procedure/carbonOrganicProcedure"/>
    </owl:NamedIndividual>
    


    <!-- http://w3id.org/glosis/model/procedure/carbonOrganicProcedure-OrgC_wc-cro3-nrcs6a1c -->


    <owl:NamedIndividual rdf:about="http://w3id.org/glosis/model/procedure/carbonOrganicProcedure-OrgC_wc-cro3-nrcs6a1c">
        <rdf:type rdf:resource="http://w3id.org/glosis/model/procedure/CarbonOrganicProcedure"/>
        <rdf:type rdf:resource="http://www.w3.org/2004/02/skos/core#Concept"/>
        <skos:definition>Wet oxidation according to USDA-NRCS method 6A1c with acid dichromate digestion, FeSO4 titration, automatic titrator</skos:definition>
        <skos:inScheme rdf:resource="http://w3id.org/glosis/model/procedure/carbonOrganicProcedure"/>
        <skos:notation>OrgC_wc-cro3-nrcs6a1c</skos:notation>
        <skos:prefLabel xml:lang="en">OrgC_wc-cro3-nrcs6a1c</skos:prefLabel>
        <skos:scopeNote rdf:resource="https://www.nrcs.usda.gov/Internet/FSE_DOCUMENTS/stelprdb1253872.pdf"/>
        <skos:topConceptOf rdf:resource="http://w3id.org/glosis/model/procedure/carbonOrganicProcedure"/>
    </owl:NamedIndividual>
    


    <!-- http://w3id.org/glosis/model/procedure/carbonOrganicProcedure-OrgC_wc-cro3-tiurin -->


    <owl:NamedIndividual rdf:about="http://w3id.org/glosis/model/procedure/carbonOrganicProcedure-OrgC_wc-cro3-tiurin">
        <rdf:type rdf:resource="http://w3id.org/glosis/model/procedure/CarbonOrganicProcedure"/>
        <rdf:type rdf:resource="http://www.w3.org/2004/02/skos/core#Concept"/>
        <skos:definition>Wet oxidation according to Tiurin with K-dichromate</skos:definition>
        <skos:inScheme rdf:resource="http://w3id.org/glosis/model/procedure/carbonOrganicProcedure"/>
        <skos:notation>OrgC_wc-cro3-tiurin</skos:notation>
        <skos:prefLabel xml:lang="en">OrgC_wc-cro3-tiuri</skos:prefLabel>
        <skos:scopeNote>I. V. TIURIN, Pochvovodenie (Pedology), (1931) 36.</skos:scopeNote>
        <skos:topConceptOf rdf:resource="http://w3id.org/glosis/model/procedure/carbonOrganicProcedure"/>
    </owl:NamedIndividual>
    


    <!-- http://w3id.org/glosis/model/procedure/carbonOrganicProcedure-OrgC_wc-cro3-walkleyblack -->


    <owl:NamedIndividual rdf:about="http://w3id.org/glosis/model/procedure/carbonOrganicProcedure-OrgC_wc-cro3-walkleyblack">
        <rdf:type rdf:resource="http://w3id.org/glosis/model/procedure/CarbonOrganicProcedure"/>
        <rdf:type rdf:resource="http://www.w3.org/2004/02/skos/core#Concept"/>
        <skos:definition>Walkley-Black method (chromic acid digestion)</skos:definition>
        <skos:inScheme rdf:resource="http://w3id.org/glosis/model/procedure/carbonOrganicProcedure"/>
        <skos:notation>OrgC_wc-cro3-walkleyblack</skos:notation>
        <skos:prefLabel xml:lang="en">OrgC_wc-cro3-walkleyblack</skos:prefLabel>
        <skos:scopeNote>Walkley, A. and I. A. Black. 1934. An Examination of Degtjareff Method for Determining Soil Organic Matter and a Proposed Modification of the Chromic Acid Titration Method. Soil Sci. 37:29–37.</skos:scopeNote>
        <skos:topConceptOf rdf:resource="http://w3id.org/glosis/model/procedure/carbonOrganicProcedure"/>
    </owl:NamedIndividual>
    


    <!-- http://w3id.org/glosis/model/procedure/carbonTotalProcedure -->


    <owl:NamedIndividual rdf:about="http://w3id.org/glosis/model/procedure/carbonTotalProcedure">
        <rdf:type rdf:resource="http://www.w3.org/2004/02/skos/core#ConceptScheme"/>
        <rdfs:label xml:lang="en">Code list for carbonTotal analysis procedures - codelist scheme</rdfs:label>
        <rdfs:seeAlso rdf:resource="http://w3id.org/glosis/model/procedure/CarbonTotalProcedure"/>
        <skos:definition>AfSP-derived interpretation (RwaSP)</skos:definition>
        <skos:note xml:lang="en">This code list provides analysis procedures for carbonTotal.</skos:note>
        <skos:prefLabel xml:lang="en">Code list for carbonTotal analysis procedures - codelist scheme</skos:prefLabel>
    </owl:NamedIndividual>
    


    <!-- http://w3id.org/glosis/model/procedure/carbonTotalProcedure-TotC_calcul-ic-oc -->


    <owl:NamedIndividual rdf:about="http://w3id.org/glosis/model/procedure/carbonTotalProcedure-TotC_calcul-ic-oc">
        <rdf:type rdf:resource="http://w3id.org/glosis/model/procedure/CarbonTotalProcedure"/>
        <rdf:type rdf:resource="http://www.w3.org/2004/02/skos/core#Concept"/>
        <skos:definition>Calculated as sum of inorganic carbon and organic carbon</skos:definition>
        <skos:inScheme rdf:resource="http://w3id.org/glosis/model/procedure/carbonTotalProcedure"/>
        <skos:notation>TotC_calcul-ic-oc</skos:notation>
        <skos:prefLabel xml:lang="en">TotC_calcul-ic-oc</skos:prefLabel>
        <skos:scopeNote rdf:resource="https://www.isric.org/sites/default/files/isric_report_2014_01.pdf"/>
        <skos:scopeNote>Leenaars J.G.B., A.J.M. van Oostrum and M. Ruiperez Gonzalez, 2014. Africa Soil Profiles Database, Version 1.2. A compilation of georeferenced and standardised legacy soil profile data for Sub-Saharan Africa (with dataset). ISRIC Report 2014/01. Africa Soil Information Service (AfSIS) project and ISRIC - World Soil Information, Wageningen, the Netherlands. See Annex 4.</skos:scopeNote>
        <skos:topConceptOf rdf:resource="http://w3id.org/glosis/model/procedure/carbonTotalProcedure"/>
    </owl:NamedIndividual>
    


    <!-- http://w3id.org/glosis/model/procedure/carbonTotalProcedure-TotC_dc-ht -->


    <owl:NamedIndividual rdf:about="http://w3id.org/glosis/model/procedure/carbonTotalProcedure-TotC_dc-ht">
        <rdf:type rdf:resource="http://w3id.org/glosis/model/procedure/CarbonTotalProcedure"/>
        <rdf:type rdf:resource="http://www.w3.org/2004/02/skos/core#Concept"/>
        <skos:definition>Unacidified dry combustion at high temperature (950-1400 C). Total Carbon</skos:definition>
        <skos:inScheme rdf:resource="http://w3id.org/glosis/model/procedure/carbonTotalProcedure"/>
        <skos:notation>TotC_dc-ht</skos:notation>
        <skos:prefLabel xml:lang="en">TotC_dc-ht</skos:prefLabel>
        <skos:scopeNote rdf:resource="https://www.isric.org/sites/default/files/isric_report_2014_01.pdf"/>
        <skos:scopeNote>Leenaars J.G.B., A.J.M. van Oostrum and M. Ruiperez Gonzalez, 2014. Africa Soil Profiles Database, Version 1.2. A compilation of georeferenced and standardised legacy soil profile data for Sub-Saharan Africa (with dataset). ISRIC Report 2014/01. Africa Soil Information Service (AfSIS) project and ISRIC - World Soil Information, Wageningen, the Netherlands. See Annex 4.</skos:scopeNote>
        <skos:topConceptOf rdf:resource="http://w3id.org/glosis/model/procedure/carbonTotalProcedure"/>
    </owl:NamedIndividual>
    


    <!-- http://w3id.org/glosis/model/procedure/carbonTotalProcedure-TotC_dc-ht-analyser -->


    <owl:NamedIndividual rdf:about="http://w3id.org/glosis/model/procedure/carbonTotalProcedure-TotC_dc-ht-analyser">
        <rdf:type rdf:resource="http://w3id.org/glosis/model/procedure/CarbonTotalProcedure"/>
        <rdf:type rdf:resource="http://www.w3.org/2004/02/skos/core#Concept"/>
        <skos:definition>Unacidified dry combustion at high temperature (950-1400 C). Total Carbon (USDA-NRCS method 6A), LECO analyzer at 1140 C</skos:definition>
        <skos:inScheme rdf:resource="http://w3id.org/glosis/model/procedure/carbonTotalProcedure"/>
        <skos:notation>TotC_dc-ht-analyser</skos:notation>
        <skos:prefLabel xml:lang="en">TotC_dc-ht-analyser</skos:prefLabel>
        <skos:scopeNote rdf:resource="https://www.nrcs.usda.gov/Internet/FSE_DOCUMENTS/stelprdb1253872.pdf"/>
        <skos:topConceptOf rdf:resource="http://w3id.org/glosis/model/procedure/carbonTotalProcedure"/>
    </owl:NamedIndividual>
    


    <!-- http://w3id.org/glosis/model/procedure/carbonTotalProcedure-TotC_dc-ht-spec -->


    <owl:NamedIndividual rdf:about="http://w3id.org/glosis/model/procedure/carbonTotalProcedure-TotC_dc-ht-spec">
        <rdf:type rdf:resource="http://w3id.org/glosis/model/procedure/CarbonTotalProcedure"/>
        <rdf:type rdf:resource="http://www.w3.org/2004/02/skos/core#Concept"/>
        <skos:definition>Spectrally measured and converted to Unacidified dry combustion at high temperature (950-1400 C).</skos:definition>
        <skos:inScheme rdf:resource="http://w3id.org/glosis/model/procedure/carbonTotalProcedure"/>
        <skos:notation>TotC_dc-ht-spec</skos:notation>
        <skos:prefLabel xml:lang="en">TotC_dc-ht-spec</skos:prefLabel>
        <skos:scopeNote rdf:resource="https://www.isric.org/sites/default/files/isric_report_2014_01.pdf"/>
        <skos:scopeNote>Leenaars J.G.B., A.J.M. van Oostrum and M. Ruiperez Gonzalez, 2014. Africa Soil Profiles Database, Version 1.2. A compilation of georeferenced and standardised legacy soil profile data for Sub-Saharan Africa (with dataset). ISRIC Report 2014/01. Africa Soil Information Service (AfSIS) project and ISRIC - World Soil Information, Wageningen, the Netherlands. See Annex 4.</skos:scopeNote>
        <skos:topConceptOf rdf:resource="http://w3id.org/glosis/model/procedure/carbonTotalProcedure"/>
    </owl:NamedIndividual>
    


    <!-- http://w3id.org/glosis/model/procedure/carbonTotalProcedure-TotC_dc-mt -->


    <owl:NamedIndividual rdf:about="http://w3id.org/glosis/model/procedure/carbonTotalProcedure-TotC_dc-mt">
        <rdf:type rdf:resource="http://w3id.org/glosis/model/procedure/CarbonTotalProcedure"/>
        <rdf:type rdf:resource="http://www.w3.org/2004/02/skos/core#Concept"/>
        <skos:definition>Unacidified dry combustion at medium temperature (550-950 C).</skos:definition>
        <skos:inScheme rdf:resource="http://w3id.org/glosis/model/procedure/carbonTotalProcedure"/>
        <skos:notation>TotC_dc-mt</skos:notation>
        <skos:prefLabel xml:lang="en">TotC_dc-mt</skos:prefLabel>
        <skos:scopeNote rdf:resource="https://www.isric.org/sites/default/files/isric_report_2014_01.pdf"/>
        <skos:scopeNote>Leenaars J.G.B., A.J.M. van Oostrum and M. Ruiperez Gonzalez, 2014. Africa Soil Profiles Database, Version 1.2. A compilation of georeferenced and standardised legacy soil profile data for Sub-Saharan Africa (with dataset). ISRIC Report 2014/01. Africa Soil Information Service (AfSIS) project and ISRIC - World Soil Information, Wageningen, the Netherlands. See Annex 4.</skos:scopeNote>
        <skos:topConceptOf rdf:resource="http://w3id.org/glosis/model/procedure/carbonTotalProcedure"/>
    </owl:NamedIndividual>
    


    <!-- http://w3id.org/glosis/model/procedure/cationExchangeCapacitySoilProcedure -->


    <owl:NamedIndividual rdf:about="http://w3id.org/glosis/model/procedure/cationExchangeCapacitySoilProcedure">
        <rdf:type rdf:resource="http://www.w3.org/2004/02/skos/core#ConceptScheme"/>
        <rdfs:label xml:lang="en">Code list for cationExchangeCapacitySoil analysis procedures - codelist scheme</rdfs:label>
        <rdfs:seeAlso rdf:resource="http://w3id.org/glosis/model/procedure/CationExchangeCapacitySoilProcedure"/>
        <skos:definition>AfSP-derived interpretation (RwaSP)</skos:definition>
        <skos:note xml:lang="en">This code list provides analysis procedures for cationExchangeCapacitySoil.</skos:note>
        <skos:prefLabel xml:lang="en">Code list for cationExchangeCapacitySoil analysis procedures - codelist scheme</skos:prefLabel>
    </owl:NamedIndividual>
    


    <!-- http://w3id.org/glosis/model/procedure/cationExchangeCapacitySoilProcedure-CEC_ph-unkn-cacl2 -->


    <owl:NamedIndividual rdf:about="http://w3id.org/glosis/model/procedure/cationExchangeCapacitySoilProcedure-CEC_ph-unkn-cacl2">
        <rdf:type rdf:resource="http://w3id.org/glosis/model/procedure/CationExchangeCapacitySoilProcedure"/>
        <rdf:type rdf:resource="http://www.w3.org/2004/02/skos/core#Concept"/>
        <skos:definition>CEC at unknown buffer, in 0.1 M CaCl2 exchange solution</skos:definition>
        <skos:inScheme rdf:resource="http://w3id.org/glosis/model/procedure/cationExchangeCapacitySoilProcedure"/>
        <skos:notation>CEC_ph-unkn-cacl2</skos:notation>
        <skos:prefLabel xml:lang="en">CEC_ph-unkn-cacl2</skos:prefLabel>
        <skos:scopeNote rdf:resource="https://www.isric.org/sites/default/files/isric_report_2014_01.pdf"/>
        <skos:scopeNote>Leenaars J.G.B., A.J.M. van Oostrum and M. Ruiperez Gonzalez, 2014. Africa Soil Profiles Database, Version 1.2. A compilation of georeferenced and standardised legacy soil profile data for Sub-Saharan Africa (with dataset). ISRIC Report 2014/01. Africa Soil Information Service (AfSIS) project and ISRIC - World Soil Information, Wageningen, the Netherlands. See Annex 4.</skos:scopeNote>
        <skos:topConceptOf rdf:resource="http://w3id.org/glosis/model/procedure/cationExchangeCapacitySoilProcedure"/>
    </owl:NamedIndividual>
    


    <!-- http://w3id.org/glosis/model/procedure/cationExchangeCapacitySoilProcedure-CEC_ph-unkn-lioac -->


    <owl:NamedIndividual rdf:about="http://w3id.org/glosis/model/procedure/cationExchangeCapacitySoilProcedure-CEC_ph-unkn-lioac">
        <rdf:type rdf:resource="http://w3id.org/glosis/model/procedure/CationExchangeCapacitySoilProcedure"/>
        <rdf:type rdf:resource="http://www.w3.org/2004/02/skos/core#Concept"/>
        <skos:definition>CEC at unknown buffer, in 0.5 M Li-acetate exchange solution</skos:definition>
        <skos:inScheme rdf:resource="http://w3id.org/glosis/model/procedure/cationExchangeCapacitySoilProcedure"/>
        <skos:notation>CEC_ph-unkn-lioac</skos:notation>
        <skos:prefLabel xml:lang="en">CEC_ph-unkn-lioac</skos:prefLabel>
        <skos:scopeNote rdf:resource="https://www.isric.org/sites/default/files/isric_report_2014_01.pdf"/>
        <skos:scopeNote>Leenaars J.G.B., A.J.M. van Oostrum and M. Ruiperez Gonzalez, 2014. Africa Soil Profiles Database, Version 1.2. A compilation of georeferenced and standardised legacy soil profile data for Sub-Saharan Africa (with dataset). ISRIC Report 2014/01. Africa Soil Information Service (AfSIS) project and ISRIC - World Soil Information, Wageningen, the Netherlands. See Annex 4.</skos:scopeNote>
        <skos:topConceptOf rdf:resource="http://w3id.org/glosis/model/procedure/cationExchangeCapacitySoilProcedure"/>
    </owl:NamedIndividual>
    


    <!-- http://w3id.org/glosis/model/procedure/cationExchangeCapacitySoilProcedure-CEC_ph-unkn-m3 -->


    <owl:NamedIndividual rdf:about="http://w3id.org/glosis/model/procedure/cationExchangeCapacitySoilProcedure-CEC_ph-unkn-m3">
        <rdf:type rdf:resource="http://w3id.org/glosis/model/procedure/CationExchangeCapacitySoilProcedure"/>
        <rdf:type rdf:resource="http://www.w3.org/2004/02/skos/core#Concept"/>
        <skos:definition>CEC at unknown buffer, in Mehlich III exchange solution</skos:definition>
        <skos:inScheme rdf:resource="http://w3id.org/glosis/model/procedure/cationExchangeCapacitySoilProcedure"/>
        <skos:notation>CEC_ph-unkn-m3</skos:notation>
        <skos:prefLabel xml:lang="en">CEC_ph-unkn-m3</skos:prefLabel>
        <skos:scopeNote rdf:resource="https://www.isric.org/sites/default/files/isric_report_2014_01.pdf"/>
        <skos:scopeNote>Leenaars J.G.B., A.J.M. van Oostrum and M. Ruiperez Gonzalez, 2014. Africa Soil Profiles Database, Version 1.2. A compilation of georeferenced and standardised legacy soil profile data for Sub-Saharan Africa (with dataset). ISRIC Report 2014/01. Africa Soil Information Service (AfSIS) project and ISRIC - World Soil Information, Wageningen, the Netherlands. See Annex 4.</skos:scopeNote>
        <skos:topConceptOf rdf:resource="http://w3id.org/glosis/model/procedure/cationExchangeCapacitySoilProcedure"/>
    </owl:NamedIndividual>
    


    <!-- http://w3id.org/glosis/model/procedure/cationExchangeCapacitySoilProcedure-CEC_ph0-ag-thioura -->


    <owl:NamedIndividual rdf:about="http://w3id.org/glosis/model/procedure/cationExchangeCapacitySoilProcedure-CEC_ph0-ag-thioura">
        <rdf:type rdf:resource="http://w3id.org/glosis/model/procedure/CationExchangeCapacitySoilProcedure"/>
        <rdf:type rdf:resource="http://www.w3.org/2004/02/skos/core#Concept"/>
        <skos:definition>CEC unbuffered at pH of the soil, in 0.01 M Ag-thioura exchange solution</skos:definition>
        <skos:inScheme rdf:resource="http://w3id.org/glosis/model/procedure/cationExchangeCapacitySoilProcedure"/>
        <skos:notation>CEC_ph0-ag-thioura</skos:notation>
        <skos:prefLabel xml:lang="en">CEC_ph0-ag-thioura</skos:prefLabel>
        <skos:scopeNote rdf:resource="https://www.isric.org/sites/default/files/isric_report_2014_01.pdf"/>
        <skos:scopeNote>Leenaars J.G.B., A.J.M. van Oostrum and M. Ruiperez Gonzalez, 2014. Africa Soil Profiles Database, Version 1.2. A compilation of georeferenced and standardised legacy soil profile data for Sub-Saharan Africa (with dataset). ISRIC Report 2014/01. Africa Soil Information Service (AfSIS) project and ISRIC - World Soil Information, Wageningen, the Netherlands. See Annex 4.</skos:scopeNote>
        <skos:topConceptOf rdf:resource="http://w3id.org/glosis/model/procedure/cationExchangeCapacitySoilProcedure"/>
    </owl:NamedIndividual>
    


    <!-- http://w3id.org/glosis/model/procedure/cationExchangeCapacitySoilProcedure-CEC_ph0-bacl2 -->


    <owl:NamedIndividual rdf:about="http://w3id.org/glosis/model/procedure/cationExchangeCapacitySoilProcedure-CEC_ph0-bacl2">
        <rdf:type rdf:resource="http://w3id.org/glosis/model/procedure/CationExchangeCapacitySoilProcedure"/>
        <rdf:type rdf:resource="http://www.w3.org/2004/02/skos/core#Concept"/>
        <skos:definition>CEC unbuffered at pH o the soil, in 0.5 M BaCl2 exchange solution (0.1.1.0 M)</skos:definition>
        <skos:inScheme rdf:resource="http://w3id.org/glosis/model/procedure/cationExchangeCapacitySoilProcedure"/>
        <skos:notation>CEC_ph0-bacl2</skos:notation>
        <skos:prefLabel xml:lang="en">CEC_ph0-bacl2</skos:prefLabel>
        <skos:scopeNote rdf:resource="https://www.isric.org/sites/default/files/isric_report_2014_01.pdf"/>
        <skos:scopeNote>Leenaars J.G.B., A.J.M. van Oostrum and M. Ruiperez Gonzalez, 2014. Africa Soil Profiles Database, Version 1.2. A compilation of georeferenced and standardised legacy soil profile data for Sub-Saharan Africa (with dataset). ISRIC Report 2014/01. Africa Soil Information Service (AfSIS) project and ISRIC - World Soil Information, Wageningen, the Netherlands. See Annex 4.</skos:scopeNote>
        <skos:topConceptOf rdf:resource="http://w3id.org/glosis/model/procedure/cationExchangeCapacitySoilProcedure"/>
    </owl:NamedIndividual>
    


    <!-- http://w3id.org/glosis/model/procedure/cationExchangeCapacitySoilProcedure-CEC_ph0-cohex -->


    <owl:NamedIndividual rdf:about="http://w3id.org/glosis/model/procedure/cationExchangeCapacitySoilProcedure-CEC_ph0-cohex">
        <rdf:type rdf:resource="http://w3id.org/glosis/model/procedure/CationExchangeCapacitySoilProcedure"/>
        <rdf:type rdf:resource="http://www.w3.org/2004/02/skos/core#Concept"/>
        <skos:definition>CEC unbuffered at pH of the soil, in Cobalt(III) hexamine chloride solution 0,0166M (Cohex) [Co[NH3]6]Cl3 ), ISO 23470 (2007)  exchange solution</skos:definition>
        <skos:inScheme rdf:resource="http://w3id.org/glosis/model/procedure/cationExchangeCapacitySoilProcedure"/>
        <skos:notation>CEC_ph0-cohex</skos:notation>
        <skos:prefLabel xml:lang="en">CEC_ph0-cohex</skos:prefLabel>
        <skos:scopeNote rdf:resource="https://www.iso.org/standard/36879.html"/>
        <skos:topConceptOf rdf:resource="http://w3id.org/glosis/model/procedure/cationExchangeCapacitySoilProcedure"/>
    </owl:NamedIndividual>
    


    <!-- http://w3id.org/glosis/model/procedure/cationExchangeCapacitySoilProcedure-CEC_ph0-kcl -->


    <owl:NamedIndividual rdf:about="http://w3id.org/glosis/model/procedure/cationExchangeCapacitySoilProcedure-CEC_ph0-kcl">
        <rdf:type rdf:resource="http://w3id.org/glosis/model/procedure/CationExchangeCapacitySoilProcedure"/>
        <rdf:type rdf:resource="http://www.w3.org/2004/02/skos/core#Concept"/>
        <skos:definition>CEC unbuffered at pH of the soil, in 1 M KCl exchange solution</skos:definition>
        <skos:inScheme rdf:resource="http://w3id.org/glosis/model/procedure/cationExchangeCapacitySoilProcedure"/>
        <skos:notation>CEC_ph0-kcl</skos:notation>
        <skos:prefLabel xml:lang="en">CEC_ph0-kcl</skos:prefLabel>
        <skos:scopeNote rdf:resource="https://www.isric.org/sites/default/files/isric_report_2014_01.pdf"/>
        <skos:scopeNote>Leenaars J.G.B., A.J.M. van Oostrum and M. Ruiperez Gonzalez, 2014. Africa Soil Profiles Database, Version 1.2. A compilation of georeferenced and standardised legacy soil profile data for Sub-Saharan Africa (with dataset). ISRIC Report 2014/01. Africa Soil Information Service (AfSIS) project and ISRIC - World Soil Information, Wageningen, the Netherlands. See Annex 4.</skos:scopeNote>
        <skos:topConceptOf rdf:resource="http://w3id.org/glosis/model/procedure/cationExchangeCapacitySoilProcedure"/>
    </owl:NamedIndividual>
    


    <!-- http://w3id.org/glosis/model/procedure/cationExchangeCapacitySoilProcedure-CEC_ph0-nh4cl -->


    <owl:NamedIndividual rdf:about="http://w3id.org/glosis/model/procedure/cationExchangeCapacitySoilProcedure-CEC_ph0-nh4cl">
        <rdf:type rdf:resource="http://w3id.org/glosis/model/procedure/CationExchangeCapacitySoilProcedure"/>
        <rdf:type rdf:resource="http://www.w3.org/2004/02/skos/core#Concept"/>
        <skos:definition>CEC unbuffered at pH of the soil, in 1 M NH4-chloride exchange solution (0.2-1.0 M)</skos:definition>
        <skos:inScheme rdf:resource="http://w3id.org/glosis/model/procedure/cationExchangeCapacitySoilProcedure"/>
        <skos:notation>CEC_ph0-nh4cl</skos:notation>
        <skos:prefLabel xml:lang="en">CEC_ph0-nh4cl</skos:prefLabel>
        <skos:scopeNote rdf:resource="https://www.isric.org/sites/default/files/isric_report_2014_01.pdf"/>
        <skos:scopeNote>Leenaars J.G.B., A.J.M. van Oostrum and M. Ruiperez Gonzalez, 2014. Africa Soil Profiles Database, Version 1.2. A compilation of georeferenced and standardised legacy soil profile data for Sub-Saharan Africa (with dataset). ISRIC Report 2014/01. Africa Soil Information Service (AfSIS) project and ISRIC - World Soil Information, Wageningen, the Netherlands. See Annex 4.</skos:scopeNote>
        <skos:topConceptOf rdf:resource="http://w3id.org/glosis/model/procedure/cationExchangeCapacitySoilProcedure"/>
    </owl:NamedIndividual>
    


    <!-- http://w3id.org/glosis/model/procedure/cationExchangeCapacitySoilProcedure-CEC_ph0-nh4oac -->


    <owl:NamedIndividual rdf:about="http://w3id.org/glosis/model/procedure/cationExchangeCapacitySoilProcedure-CEC_ph0-nh4oac">
        <rdf:type rdf:resource="http://w3id.org/glosis/model/procedure/CationExchangeCapacitySoilProcedure"/>
        <rdf:type rdf:resource="http://www.w3.org/2004/02/skos/core#Concept"/>
        <skos:definition>CEC unbuffered at pH of the soil, in 1 M NH4-acetate (NH4OAc) exchange solution (0.25-1.0 M)</skos:definition>
        <skos:inScheme rdf:resource="http://w3id.org/glosis/model/procedure/cationExchangeCapacitySoilProcedure"/>
        <skos:notation>CEC_ph0-nh4oac</skos:notation>
        <skos:prefLabel xml:lang="en">CEC_ph0-nh4oac</skos:prefLabel>
        <skos:scopeNote rdf:resource="https://www.isric.org/sites/default/files/isric_report_2014_01.pdf"/>
        <skos:scopeNote>Leenaars J.G.B., A.J.M. van Oostrum and M. Ruiperez Gonzalez, 2014. Africa Soil Profiles Database, Version 1.2. A compilation of georeferenced and standardised legacy soil profile data for Sub-Saharan Africa (with dataset). ISRIC Report 2014/01. Africa Soil Information Service (AfSIS) project and ISRIC - World Soil Information, Wageningen, the Netherlands. See Annex 4.</skos:scopeNote>
        <skos:topConceptOf rdf:resource="http://w3id.org/glosis/model/procedure/cationExchangeCapacitySoilProcedure"/>
    </owl:NamedIndividual>
    


    <!-- http://w3id.org/glosis/model/procedure/cationExchangeCapacitySoilProcedure-CEC_ph0-unkn -->


    <owl:NamedIndividual rdf:about="http://w3id.org/glosis/model/procedure/cationExchangeCapacitySoilProcedure-CEC_ph0-unkn">
        <rdf:type rdf:resource="http://w3id.org/glosis/model/procedure/CationExchangeCapacitySoilProcedure"/>
        <rdf:type rdf:resource="http://www.w3.org/2004/02/skos/core#Concept"/>
        <skos:definition>CEC unbuffered at pH of the soil, in unknown exchange solution</skos:definition>
        <skos:inScheme rdf:resource="http://w3id.org/glosis/model/procedure/cationExchangeCapacitySoilProcedure"/>
        <skos:notation>CEC_ph0-unkn</skos:notation>
        <skos:prefLabel xml:lang="en">CEC_ph0-unk</skos:prefLabel>
        <skos:scopeNote rdf:resource="https://www.isric.org/sites/default/files/isric_report_2014_01.pdf"/>
        <skos:scopeNote>Leenaars J.G.B., A.J.M. van Oostrum and M. Ruiperez Gonzalez, 2014. Africa Soil Profiles Database, Version 1.2. A compilation of georeferenced and standardised legacy soil profile data for Sub-Saharan Africa (with dataset). ISRIC Report 2014/01. Africa Soil Information Service (AfSIS) project and ISRIC - World Soil Information, Wageningen, the Netherlands. See Annex 4.</skos:scopeNote>
        <skos:topConceptOf rdf:resource="http://w3id.org/glosis/model/procedure/cationExchangeCapacitySoilProcedure"/>
    </owl:NamedIndividual>
    


    <!-- http://w3id.org/glosis/model/procedure/cationExchangeCapacitySoilProcedure-CEC_ph7-edta -->


    <owl:NamedIndividual rdf:about="http://w3id.org/glosis/model/procedure/cationExchangeCapacitySoilProcedure-CEC_ph7-edta">
        <rdf:type rdf:resource="http://w3id.org/glosis/model/procedure/CationExchangeCapacitySoilProcedure"/>
        <rdf:type rdf:resource="http://www.w3.org/2004/02/skos/core#Concept"/>
        <skos:definition>CEC buffered at pH 7, in 0.1 M Li-EDTA exchange solution</skos:definition>
        <skos:inScheme rdf:resource="http://w3id.org/glosis/model/procedure/cationExchangeCapacitySoilProcedure"/>
        <skos:notation>CEC_ph7-edta</skos:notation>
        <skos:prefLabel xml:lang="en">CEC_ph7-edta</skos:prefLabel>
        <skos:scopeNote rdf:resource="https://www.isric.org/sites/default/files/isric_report_2014_01.pdf"/>
        <skos:scopeNote>Leenaars J.G.B., A.J.M. van Oostrum and M. Ruiperez Gonzalez, 2014. Africa Soil Profiles Database, Version 1.2. A compilation of georeferenced and standardised legacy soil profile data for Sub-Saharan Africa (with dataset). ISRIC Report 2014/01. Africa Soil Information Service (AfSIS) project and ISRIC - World Soil Information, Wageningen, the Netherlands. See Annex 4.</skos:scopeNote>
        <skos:topConceptOf rdf:resource="http://w3id.org/glosis/model/procedure/cationExchangeCapacitySoilProcedure"/>
    </owl:NamedIndividual>
    


    <!-- http://w3id.org/glosis/model/procedure/cationExchangeCapacitySoilProcedure-CEC_ph7-nh4oac -->


    <owl:NamedIndividual rdf:about="http://w3id.org/glosis/model/procedure/cationExchangeCapacitySoilProcedure-CEC_ph7-nh4oac">
        <rdf:type rdf:resource="http://w3id.org/glosis/model/procedure/CationExchangeCapacitySoilProcedure"/>
        <rdf:type rdf:resource="http://www.w3.org/2004/02/skos/core#Concept"/>
        <skos:definition>CEC buffered at pH 7, in 1 M NH4-acetate (NH4OAc) exchange solution (0.25-1.0 M)</skos:definition>
        <skos:inScheme rdf:resource="http://w3id.org/glosis/model/procedure/cationExchangeCapacitySoilProcedure"/>
        <skos:notation>CEC_ph7-nh4oac</skos:notation>
        <skos:prefLabel xml:lang="en">CEC_ph7-nh4oac</skos:prefLabel>
        <skos:scopeNote rdf:resource="https://www.isric.org/sites/default/files/isric_report_2014_01.pdf"/>
        <skos:scopeNote>Leenaars J.G.B., A.J.M. van Oostrum and M. Ruiperez Gonzalez, 2014. Africa Soil Profiles Database, Version 1.2. A compilation of georeferenced and standardised legacy soil profile data for Sub-Saharan Africa (with dataset). ISRIC Report 2014/01. Africa Soil Information Service (AfSIS) project and ISRIC - World Soil Information, Wageningen, the Netherlands. See Annex 4.</skos:scopeNote>
        <skos:topConceptOf rdf:resource="http://w3id.org/glosis/model/procedure/cationExchangeCapacitySoilProcedure"/>
    </owl:NamedIndividual>
    


    <!-- http://w3id.org/glosis/model/procedure/cationExchangeCapacitySoilProcedure-CEC_ph7-unkn -->


    <owl:NamedIndividual rdf:about="http://w3id.org/glosis/model/procedure/cationExchangeCapacitySoilProcedure-CEC_ph7-unkn">
        <rdf:type rdf:resource="http://w3id.org/glosis/model/procedure/CationExchangeCapacitySoilProcedure"/>
        <rdf:type rdf:resource="http://www.w3.org/2004/02/skos/core#Concept"/>
        <skos:definition>CEC buffered at pH 7, in unknown exchange solution</skos:definition>
        <skos:inScheme rdf:resource="http://w3id.org/glosis/model/procedure/cationExchangeCapacitySoilProcedure"/>
        <skos:notation>CEC_ph7-unkn</skos:notation>
        <skos:prefLabel xml:lang="en">CEC_ph7-unk</skos:prefLabel>
        <skos:scopeNote rdf:resource="https://www.isric.org/sites/default/files/isric_report_2014_01.pdf"/>
        <skos:scopeNote>Leenaars J.G.B., A.J.M. van Oostrum and M. Ruiperez Gonzalez, 2014. Africa Soil Profiles Database, Version 1.2. A compilation of georeferenced and standardised legacy soil profile data for Sub-Saharan Africa (with dataset). ISRIC Report 2014/01. Africa Soil Information Service (AfSIS) project and ISRIC - World Soil Information, Wageningen, the Netherlands. See Annex 4.</skos:scopeNote>
        <skos:topConceptOf rdf:resource="http://w3id.org/glosis/model/procedure/cationExchangeCapacitySoilProcedure"/>
    </owl:NamedIndividual>
    


    <!-- http://w3id.org/glosis/model/procedure/cationExchangeCapacitySoilProcedure-CEC_ph8-bacl2tea -->


    <owl:NamedIndividual rdf:about="http://w3id.org/glosis/model/procedure/cationExchangeCapacitySoilProcedure-CEC_ph8-bacl2tea">
        <rdf:type rdf:resource="http://w3id.org/glosis/model/procedure/CationExchangeCapacitySoilProcedure"/>
        <rdf:type rdf:resource="http://www.w3.org/2004/02/skos/core#Concept"/>
        <skos:definition>CEC buffered at pH 8.0-8.5, in 0.5 M BaCl2-TEA exchange solution (0.1.1.0 M)</skos:definition>
        <skos:inScheme rdf:resource="http://w3id.org/glosis/model/procedure/cationExchangeCapacitySoilProcedure"/>
        <skos:notation>CEC_ph8-bacl2tea</skos:notation>
        <skos:prefLabel xml:lang="en">CEC_ph8-bacl2tea</skos:prefLabel>
        <skos:scopeNote rdf:resource="https://www.isric.org/sites/default/files/isric_report_2014_01.pdf"/>
        <skos:scopeNote>Leenaars J.G.B., A.J.M. van Oostrum and M. Ruiperez Gonzalez, 2014. Africa Soil Profiles Database, Version 1.2. A compilation of georeferenced and standardised legacy soil profile data for Sub-Saharan Africa (with dataset). ISRIC Report 2014/01. Africa Soil Information Service (AfSIS) project and ISRIC - World Soil Information, Wageningen, the Netherlands. See Annex 4.</skos:scopeNote>
        <skos:topConceptOf rdf:resource="http://w3id.org/glosis/model/procedure/cationExchangeCapacitySoilProcedure"/>
    </owl:NamedIndividual>
    


    <!-- http://w3id.org/glosis/model/procedure/cationExchangeCapacitySoilProcedure-CEC_ph8-baoac -->


    <owl:NamedIndividual rdf:about="http://w3id.org/glosis/model/procedure/cationExchangeCapacitySoilProcedure-CEC_ph8-baoac">
        <rdf:type rdf:resource="http://w3id.org/glosis/model/procedure/CationExchangeCapacitySoilProcedure"/>
        <rdf:type rdf:resource="http://www.w3.org/2004/02/skos/core#Concept"/>
        <skos:definition>CEC buffered at pH 8.0-8.5, in 0.5 M Ba-acetate exchange solution</skos:definition>
        <skos:inScheme rdf:resource="http://w3id.org/glosis/model/procedure/cationExchangeCapacitySoilProcedure"/>
        <skos:notation>CEC_ph8-baoac</skos:notation>
        <skos:prefLabel xml:lang="en">CEC_ph8-baoac</skos:prefLabel>
        <skos:scopeNote rdf:resource="https://www.isric.org/sites/default/files/isric_report_2014_01.pdf"/>
        <skos:scopeNote>Leenaars J.G.B., A.J.M. van Oostrum and M. Ruiperez Gonzalez, 2014. Africa Soil Profiles Database, Version 1.2. A compilation of georeferenced and standardised legacy soil profile data for Sub-Saharan Africa (with dataset). ISRIC Report 2014/01. Africa Soil Information Service (AfSIS) project and ISRIC - World Soil Information, Wageningen, the Netherlands. See Annex 4.</skos:scopeNote>
        <skos:topConceptOf rdf:resource="http://w3id.org/glosis/model/procedure/cationExchangeCapacitySoilProcedure"/>
    </owl:NamedIndividual>
    


    <!-- http://w3id.org/glosis/model/procedure/cationExchangeCapacitySoilProcedure-CEC_ph8-licl2tea -->


    <owl:NamedIndividual rdf:about="http://w3id.org/glosis/model/procedure/cationExchangeCapacitySoilProcedure-CEC_ph8-licl2tea">
        <rdf:type rdf:resource="http://w3id.org/glosis/model/procedure/CationExchangeCapacitySoilProcedure"/>
        <rdf:type rdf:resource="http://www.w3.org/2004/02/skos/core#Concept"/>
        <skos:definition>CEC buffered at pH 8.0-8.5, in 0.5 M Li-chloride - TEA exchange solution</skos:definition>
        <skos:inScheme rdf:resource="http://w3id.org/glosis/model/procedure/cationExchangeCapacitySoilProcedure"/>
        <skos:notation>CEC_ph8-licl2tea</skos:notation>
        <skos:prefLabel xml:lang="en">CEC_ph8-licl2tea</skos:prefLabel>
        <skos:scopeNote rdf:resource="https://www.isric.org/sites/default/files/isric_report_2014_01.pdf"/>
        <skos:scopeNote>Leenaars J.G.B., A.J.M. van Oostrum and M. Ruiperez Gonzalez, 2014. Africa Soil Profiles Database, Version 1.2. A compilation of georeferenced and standardised legacy soil profile data for Sub-Saharan Africa (with dataset). ISRIC Report 2014/01. Africa Soil Information Service (AfSIS) project and ISRIC - World Soil Information, Wageningen, the Netherlands. See Annex 4.</skos:scopeNote>
        <skos:topConceptOf rdf:resource="http://w3id.org/glosis/model/procedure/cationExchangeCapacitySoilProcedure"/>
    </owl:NamedIndividual>
    


    <!-- http://w3id.org/glosis/model/procedure/cationExchangeCapacitySoilProcedure-CEC_ph8-naoac -->


    <owl:NamedIndividual rdf:about="http://w3id.org/glosis/model/procedure/cationExchangeCapacitySoilProcedure-CEC_ph8-naoac">
        <rdf:type rdf:resource="http://w3id.org/glosis/model/procedure/CationExchangeCapacitySoilProcedure"/>
        <rdf:type rdf:resource="http://www.w3.org/2004/02/skos/core#Concept"/>
        <skos:definition>CEC buffered at pH 8.0-8.5, in 1 M Na-acetate exchange solution</skos:definition>
        <skos:inScheme rdf:resource="http://w3id.org/glosis/model/procedure/cationExchangeCapacitySoilProcedure"/>
        <skos:notation>CEC_ph8-naoac</skos:notation>
        <skos:prefLabel xml:lang="en">CEC_ph8-naoac</skos:prefLabel>
        <skos:scopeNote rdf:resource="https://www.isric.org/sites/default/files/isric_report_2014_01.pdf"/>
        <skos:scopeNote>Leenaars J.G.B., A.J.M. van Oostrum and M. Ruiperez Gonzalez, 2014. Africa Soil Profiles Database, Version 1.2. A compilation of georeferenced and standardised legacy soil profile data for Sub-Saharan Africa (with dataset). ISRIC Report 2014/01. Africa Soil Information Service (AfSIS) project and ISRIC - World Soil Information, Wageningen, the Netherlands. See Annex 4.</skos:scopeNote>
        <skos:topConceptOf rdf:resource="http://w3id.org/glosis/model/procedure/cationExchangeCapacitySoilProcedure"/>
    </owl:NamedIndividual>
    


    <!-- http://w3id.org/glosis/model/procedure/cationExchangeCapacitySoilProcedure-CEC_ph8-nh4oac -->


    <owl:NamedIndividual rdf:about="http://w3id.org/glosis/model/procedure/cationExchangeCapacitySoilProcedure-CEC_ph8-nh4oac">
        <rdf:type rdf:resource="http://w3id.org/glosis/model/procedure/CationExchangeCapacitySoilProcedure"/>
        <rdf:type rdf:resource="http://www.w3.org/2004/02/skos/core#Concept"/>
        <skos:definition>CEC buffered at pH 8.0-8.5, in 1 M NH4-acetate exchange solution (0.25-1.0 M)</skos:definition>
        <skos:inScheme rdf:resource="http://w3id.org/glosis/model/procedure/cationExchangeCapacitySoilProcedure"/>
        <skos:notation>CEC_ph8-nh4oac</skos:notation>
        <skos:prefLabel xml:lang="en">CEC_ph8-nh4oac</skos:prefLabel>
        <skos:scopeNote rdf:resource="https://www.isric.org/sites/default/files/isric_report_2014_01.pdf"/>
        <skos:scopeNote>Leenaars J.G.B., A.J.M. van Oostrum and M. Ruiperez Gonzalez, 2014. Africa Soil Profiles Database, Version 1.2. A compilation of georeferenced and standardised legacy soil profile data for Sub-Saharan Africa (with dataset). ISRIC Report 2014/01. Africa Soil Information Service (AfSIS) project and ISRIC - World Soil Information, Wageningen, the Netherlands. See Annex 4.</skos:scopeNote>
        <skos:topConceptOf rdf:resource="http://w3id.org/glosis/model/procedure/cationExchangeCapacitySoilProcedure"/>
    </owl:NamedIndividual>
    


    <!-- http://w3id.org/glosis/model/procedure/cationExchangeCapacitySoilProcedure-CEC_ph8-unkn -->


    <owl:NamedIndividual rdf:about="http://w3id.org/glosis/model/procedure/cationExchangeCapacitySoilProcedure-CEC_ph8-unkn">
        <rdf:type rdf:resource="http://w3id.org/glosis/model/procedure/CationExchangeCapacitySoilProcedure"/>
        <rdf:type rdf:resource="http://www.w3.org/2004/02/skos/core#Concept"/>
        <skos:definition>CEC buffered at pH 8.0-8.5, in unknown exchange solution</skos:definition>
        <skos:inScheme rdf:resource="http://w3id.org/glosis/model/procedure/cationExchangeCapacitySoilProcedure"/>
        <skos:notation>CEC_ph8-unkn</skos:notation>
        <skos:prefLabel xml:lang="en">CEC_ph8-unk</skos:prefLabel>
        <skos:scopeNote rdf:resource="https://www.isric.org/sites/default/files/isric_report_2014_01.pdf"/>
        <skos:scopeNote>Leenaars J.G.B., A.J.M. van Oostrum and M. Ruiperez Gonzalez, 2014. Africa Soil Profiles Database, Version 1.2. A compilation of georeferenced and standardised legacy soil profile data for Sub-Saharan Africa (with dataset). ISRIC Report 2014/01. Africa Soil Information Service (AfSIS) project and ISRIC - World Soil Information, Wageningen, the Netherlands. See Annex 4.</skos:scopeNote>
        <skos:topConceptOf rdf:resource="http://w3id.org/glosis/model/procedure/cationExchangeCapacitySoilProcedure"/>
    </owl:NamedIndividual>
    


    <!-- http://w3id.org/glosis/model/procedure/coarseFragmentsProcedure -->


    <owl:NamedIndividual rdf:about="http://w3id.org/glosis/model/procedure/coarseFragmentsProcedure">
        <rdf:type rdf:resource="http://www.w3.org/2004/02/skos/core#ConceptScheme"/>
        <rdfs:label xml:lang="en">Code list for coarseFragments analysis procedures - codelist scheme</rdfs:label>
        <rdfs:seeAlso rdf:resource="http://w3id.org/glosis/model/procedure/CoarseFragmentsProcedure"/>
        <skos:definition>AfSP-derived interpretation (RwaSP)</skos:definition>
        <skos:note xml:lang="en">This code list provides analysis procedures for coarseFragments.</skos:note>
        <skos:prefLabel xml:lang="en">Code list for coarseFragments analysis procedures - codelist scheme</skos:prefLabel>
    </owl:NamedIndividual>
    


    <!-- http://w3id.org/glosis/model/procedure/coarseFragmentsProcedure-CrsFrg_fld -->


    <owl:NamedIndividual rdf:about="http://w3id.org/glosis/model/procedure/coarseFragmentsProcedure-CrsFrg_fld">
        <rdf:type rdf:resource="http://w3id.org/glosis/model/procedure/CoarseFragmentsProcedure"/>
        <rdf:type rdf:resource="http://www.w3.org/2004/02/skos/core#Concept"/>
        <skos:definition>Particles &gt; 2 mm observed in the field. May include concretions and very hard aggregates</skos:definition>
        <skos:inScheme rdf:resource="http://w3id.org/glosis/model/procedure/coarseFragmentsProcedure"/>
        <skos:notation>CrsFrg_fld</skos:notation>
        <skos:prefLabel xml:lang="en">CrsFrg_fld</skos:prefLabel>
        <skos:scopeNote rdf:resource="https://www.isric.org/sites/default/files/isric_report_2014_01.pdf"/>
        <skos:scopeNote>Leenaars J.G.B., A.J.M. van Oostrum and M. Ruiperez Gonzalez, 2014. Africa Soil Profiles Database, Version 1.2. A compilation of georeferenced and standardised legacy soil profile data for Sub-Saharan Africa (with dataset). ISRIC Report 2014/01. Africa Soil Information Service (AfSIS) project and ISRIC - World Soil Information, Wageningen, the Netherlands. See Annex 4.</skos:scopeNote>
        <skos:topConceptOf rdf:resource="http://w3id.org/glosis/model/procedure/coarseFragmentsProcedure"/>
    </owl:NamedIndividual>
    


    <!-- http://w3id.org/glosis/model/procedure/coarseFragmentsProcedure-CrsFrg_fldcls -->


    <owl:NamedIndividual rdf:about="http://w3id.org/glosis/model/procedure/coarseFragmentsProcedure-CrsFrg_fldcls">
        <rdf:type rdf:resource="http://w3id.org/glosis/model/procedure/CoarseFragmentsProcedure"/>
        <rdf:type rdf:resource="http://www.w3.org/2004/02/skos/core#Concept"/>
        <skos:definition>Particles &gt; 2 mm observed in the field and calculated from class values. May include concretions and very hard aggregates</skos:definition>
        <skos:inScheme rdf:resource="http://w3id.org/glosis/model/procedure/coarseFragmentsProcedure"/>
        <skos:notation>CrsFrg_fldcls</skos:notation>
        <skos:prefLabel xml:lang="en">CrsFrg_fldcls</skos:prefLabel>
        <skos:scopeNote rdf:resource="https://www.isric.org/sites/default/files/isric_report_2014_01.pdf"/>
        <skos:scopeNote>Leenaars J.G.B., A.J.M. van Oostrum and M. Ruiperez Gonzalez, 2014. Africa Soil Profiles Database, Version 1.2. A compilation of georeferenced and standardised legacy soil profile data for Sub-Saharan Africa (with dataset). ISRIC Report 2014/01. Africa Soil Information Service (AfSIS) project and ISRIC - World Soil Information, Wageningen, the Netherlands. See Annex 4.</skos:scopeNote>
        <skos:topConceptOf rdf:resource="http://w3id.org/glosis/model/procedure/coarseFragmentsProcedure"/>
    </owl:NamedIndividual>
    


    <!-- http://w3id.org/glosis/model/procedure/coarseFragmentsProcedure-CrsFrg_lab -->


    <owl:NamedIndividual rdf:about="http://w3id.org/glosis/model/procedure/coarseFragmentsProcedure-CrsFrg_lab">
        <rdf:type rdf:resource="http://w3id.org/glosis/model/procedure/CoarseFragmentsProcedure"/>
        <rdf:type rdf:resource="http://www.w3.org/2004/02/skos/core#Concept"/>
        <skos:definition>Particles &gt; 2 mm measured in laboratory (sieved after light pounding). May include concretions and very hard aggregates</skos:definition>
        <skos:inScheme rdf:resource="http://w3id.org/glosis/model/procedure/coarseFragmentsProcedure"/>
        <skos:notation>CrsFrg_lab</skos:notation>
        <skos:prefLabel xml:lang="en">CrsFrg_lab</skos:prefLabel>
        <skos:scopeNote rdf:resource="https://www.isric.org/sites/default/files/isric_report_2014_01.pdf"/>
        <skos:scopeNote>Leenaars J.G.B., A.J.M. van Oostrum and M. Ruiperez Gonzalez, 2014. Africa Soil Profiles Database, Version 1.2. A compilation of georeferenced and standardised legacy soil profile data for Sub-Saharan Africa (with dataset). ISRIC Report 2014/01. Africa Soil Information Service (AfSIS) project and ISRIC - World Soil Information, Wageningen, the Netherlands. See Annex 4.</skos:scopeNote>
        <skos:topConceptOf rdf:resource="http://w3id.org/glosis/model/procedure/coarseFragmentsProcedure"/>
    </owl:NamedIndividual>
    


    <!-- http://w3id.org/glosis/model/procedure/effectiveCecProcedure -->


    <owl:NamedIndividual rdf:about="http://w3id.org/glosis/model/procedure/effectiveCecProcedure">
        <rdf:type rdf:resource="http://www.w3.org/2004/02/skos/core#ConceptScheme"/>
        <rdfs:label xml:lang="en">Code list for effectiveCec analysis procedures - codelist scheme</rdfs:label>
        <rdfs:seeAlso rdf:resource="http://w3id.org/glosis/model/procedure/EffectiveCecProcedure"/>
        <skos:definition>AfSP-derived interpretation (RwaSP)</skos:definition>
        <skos:note xml:lang="en">This code list provides analysis procedures for effectiveCec.</skos:note>
        <skos:prefLabel xml:lang="en">Code list for effectiveCec analysis procedures - codelist scheme</skos:prefLabel>
    </owl:NamedIndividual>
    


    <!-- http://w3id.org/glosis/model/procedure/effectiveCecProcedure-EffCEC_calcul-b -->


    <owl:NamedIndividual rdf:about="http://w3id.org/glosis/model/procedure/effectiveCecProcedure-EffCEC_calcul-b">
        <rdf:type rdf:resource="http://w3id.org/glosis/model/procedure/EffectiveCecProcedure"/>
        <rdf:type rdf:resource="http://www.w3.org/2004/02/skos/core#Concept"/>
        <skos:definition>Sum of exchangeable bases (Ca, Mg, K, Na) without exchangeable acidity (H+Al), see ExchBases and ExchAcids for methods</skos:definition>
        <skos:inScheme rdf:resource="http://w3id.org/glosis/model/procedure/effectiveCecProcedure"/>
        <skos:notation>EffCEC_calcul-b</skos:notation>
        <skos:prefLabel xml:lang="en">EffCEC_calcul-b</skos:prefLabel>
        <skos:scopeNote rdf:resource="https://www.isric.org/sites/default/files/isric_report_2014_01.pdf"/>
        <skos:scopeNote>Leenaars J.G.B., A.J.M. van Oostrum and M. Ruiperez Gonzalez, 2014. Africa Soil Profiles Database, Version 1.2. A compilation of georeferenced and standardised legacy soil profile data for Sub-Saharan Africa (with dataset). ISRIC Report 2014/01. Africa Soil Information Service (AfSIS) project and ISRIC - World Soil Information, Wageningen, the Netherlands. See Annex 4.</skos:scopeNote>
        <skos:topConceptOf rdf:resource="http://w3id.org/glosis/model/procedure/effectiveCecProcedure"/>
    </owl:NamedIndividual>
    


    <!-- http://w3id.org/glosis/model/procedure/effectiveCecProcedure-EffCEC_calcul-ba -->


    <owl:NamedIndividual rdf:about="http://w3id.org/glosis/model/procedure/effectiveCecProcedure-EffCEC_calcul-ba">
        <rdf:type rdf:resource="http://w3id.org/glosis/model/procedure/EffectiveCecProcedure"/>
        <rdf:type rdf:resource="http://www.w3.org/2004/02/skos/core#Concept"/>
        <skos:definition>Sum of exchangeable bases (Ca, Mg, K, Na) plus exchangeable acidity (H+Al), see ExchBases and ExchAcids for methods</skos:definition>
        <skos:inScheme rdf:resource="http://w3id.org/glosis/model/procedure/effectiveCecProcedure"/>
        <skos:notation>EffCEC_calcul-ba</skos:notation>
        <skos:prefLabel xml:lang="en">EffCEC_calcul-ba</skos:prefLabel>
        <skos:scopeNote rdf:resource="https://www.isric.org/sites/default/files/isric_report_2014_01.pdf"/>
        <skos:scopeNote>Leenaars J.G.B., A.J.M. van Oostrum and M. Ruiperez Gonzalez, 2014. Africa Soil Profiles Database, Version 1.2. A compilation of georeferenced and standardised legacy soil profile data for Sub-Saharan Africa (with dataset). ISRIC Report 2014/01. Africa Soil Information Service (AfSIS) project and ISRIC - World Soil Information, Wageningen, the Netherlands. See Annex 4.</skos:scopeNote>
        <skos:topConceptOf rdf:resource="http://w3id.org/glosis/model/procedure/effectiveCecProcedure"/>
    </owl:NamedIndividual>
    


    <!-- http://w3id.org/glosis/model/procedure/electricalConductivityProcedure -->


    <owl:NamedIndividual rdf:about="http://w3id.org/glosis/model/procedure/electricalConductivityProcedure">
        <rdf:type rdf:resource="http://www.w3.org/2004/02/skos/core#ConceptScheme"/>
        <rdfs:label xml:lang="en">Code list for electricalConductivity analysis procedures - codelist scheme</rdfs:label>
        <rdfs:seeAlso rdf:resource="http://w3id.org/glosis/model/procedure/ElectricalConductivityProcedure"/>
        <skos:definition>AfSP-derived interpretation (RwaSP)</skos:definition>
        <skos:note xml:lang="en">This code list provides analysis procedures for electricalConductivity.</skos:note>
        <skos:prefLabel xml:lang="en">Code list for electricalConductivity analysis procedures - codelist scheme</skos:prefLabel>
    </owl:NamedIndividual>
    


    <!-- http://w3id.org/glosis/model/procedure/electricalConductivityProcedure-EC_ratio1-1 -->


    <owl:NamedIndividual rdf:about="http://w3id.org/glosis/model/procedure/electricalConductivityProcedure-EC_ratio1-1">
        <rdf:type rdf:resource="http://w3id.org/glosis/model/procedure/ElectricalConductivityProcedure"/>
        <rdf:type rdf:resource="http://www.w3.org/2004/02/skos/core#Concept"/>
        <skos:definition>Elec. conductivity at 1:1 soil/water ratio</skos:definition>
        <skos:inScheme rdf:resource="http://w3id.org/glosis/model/procedure/electricalConductivityProcedure"/>
        <skos:notation>EC_ratio1-1</skos:notation>
        <skos:prefLabel xml:lang="en">EC_ratio1-1</skos:prefLabel>
        <skos:scopeNote rdf:resource="https://www.isric.org/sites/default/files/isric_report_2014_01.pdf"/>
        <skos:scopeNote>Leenaars J.G.B., A.J.M. van Oostrum and M. Ruiperez Gonzalez, 2014. Africa Soil Profiles Database, Version 1.2. A compilation of georeferenced and standardised legacy soil profile data for Sub-Saharan Africa (with dataset). ISRIC Report 2014/01. Africa Soil Information Service (AfSIS) project and ISRIC - World Soil Information, Wageningen, the Netherlands. See Annex 4.</skos:scopeNote>
        <skos:topConceptOf rdf:resource="http://w3id.org/glosis/model/procedure/electricalConductivityProcedure"/>
    </owl:NamedIndividual>
    


    <!-- http://w3id.org/glosis/model/procedure/electricalConductivityProcedure-EC_ratio1-10 -->


    <owl:NamedIndividual rdf:about="http://w3id.org/glosis/model/procedure/electricalConductivityProcedure-EC_ratio1-10">
        <rdf:type rdf:resource="http://w3id.org/glosis/model/procedure/ElectricalConductivityProcedure"/>
        <rdf:type rdf:resource="http://www.w3.org/2004/02/skos/core#Concept"/>
        <skos:definition>Elec. conductivity at 1:10 soil/water ratio</skos:definition>
        <skos:inScheme rdf:resource="http://w3id.org/glosis/model/procedure/electricalConductivityProcedure"/>
        <skos:notation>EC_ratio1-10</skos:notation>
        <skos:prefLabel xml:lang="en">EC_ratio1-10</skos:prefLabel>
        <skos:scopeNote rdf:resource="https://www.isric.org/sites/default/files/isric_report_2014_01.pdf"/>
        <skos:scopeNote>Leenaars J.G.B., A.J.M. van Oostrum and M. Ruiperez Gonzalez, 2014. Africa Soil Profiles Database, Version 1.2. A compilation of georeferenced and standardised legacy soil profile data for Sub-Saharan Africa (with dataset). ISRIC Report 2014/01. Africa Soil Information Service (AfSIS) project and ISRIC - World Soil Information, Wageningen, the Netherlands. See Annex 4.</skos:scopeNote>
        <skos:topConceptOf rdf:resource="http://w3id.org/glosis/model/procedure/electricalConductivityProcedure"/>
    </owl:NamedIndividual>
    


    <!-- http://w3id.org/glosis/model/procedure/electricalConductivityProcedure-EC_ratio1-2 -->


    <owl:NamedIndividual rdf:about="http://w3id.org/glosis/model/procedure/electricalConductivityProcedure-EC_ratio1-2">
        <rdf:type rdf:resource="http://w3id.org/glosis/model/procedure/ElectricalConductivityProcedure"/>
        <rdf:type rdf:resource="http://www.w3.org/2004/02/skos/core#Concept"/>
        <skos:definition>Elec. conductivity at 1:2 soil/water ratio</skos:definition>
        <skos:inScheme rdf:resource="http://w3id.org/glosis/model/procedure/electricalConductivityProcedure"/>
        <skos:notation>EC_ratio1-2</skos:notation>
        <skos:prefLabel xml:lang="en">EC_ratio1-2</skos:prefLabel>
        <skos:scopeNote rdf:resource="https://www.isric.org/sites/default/files/isric_report_2014_01.pdf"/>
        <skos:scopeNote>Leenaars J.G.B., A.J.M. van Oostrum and M. Ruiperez Gonzalez, 2014. Africa Soil Profiles Database, Version 1.2. A compilation of georeferenced and standardised legacy soil profile data for Sub-Saharan Africa (with dataset). ISRIC Report 2014/01. Africa Soil Information Service (AfSIS) project and ISRIC - World Soil Information, Wageningen, the Netherlands. See Annex 4.</skos:scopeNote>
        <skos:topConceptOf rdf:resource="http://w3id.org/glosis/model/procedure/electricalConductivityProcedure"/>
    </owl:NamedIndividual>
    


    <!-- http://w3id.org/glosis/model/procedure/electricalConductivityProcedure-EC_ratio1-2.5 -->


    <owl:NamedIndividual rdf:about="http://w3id.org/glosis/model/procedure/electricalConductivityProcedure-EC_ratio1-2.5">
        <rdf:type rdf:resource="http://w3id.org/glosis/model/procedure/ElectricalConductivityProcedure"/>
        <rdf:type rdf:resource="http://www.w3.org/2004/02/skos/core#Concept"/>
        <skos:definition>Elec. conductivity at 1:2.5 soil/water ratio</skos:definition>
        <skos:inScheme rdf:resource="http://w3id.org/glosis/model/procedure/electricalConductivityProcedure"/>
        <skos:notation>EC_ratio1-2.5</skos:notation>
        <skos:prefLabel xml:lang="en">EC_ratio1-2.5</skos:prefLabel>
        <skos:scopeNote rdf:resource="https://www.isric.org/sites/default/files/isric_report_2014_01.pdf"/>
        <skos:scopeNote>Leenaars J.G.B., A.J.M. van Oostrum and M. Ruiperez Gonzalez, 2014. Africa Soil Profiles Database, Version 1.2. A compilation of georeferenced and standardised legacy soil profile data for Sub-Saharan Africa (with dataset). ISRIC Report 2014/01. Africa Soil Information Service (AfSIS) project and ISRIC - World Soil Information, Wageningen, the Netherlands. See Annex 4.</skos:scopeNote>
        <skos:topConceptOf rdf:resource="http://w3id.org/glosis/model/procedure/electricalConductivityProcedure"/>
    </owl:NamedIndividual>
    


    <!-- http://w3id.org/glosis/model/procedure/electricalConductivityProcedure-EC_ratio1-5 -->


    <owl:NamedIndividual rdf:about="http://w3id.org/glosis/model/procedure/electricalConductivityProcedure-EC_ratio1-5">
        <rdf:type rdf:resource="http://w3id.org/glosis/model/procedure/ElectricalConductivityProcedure"/>
        <rdf:type rdf:resource="http://www.w3.org/2004/02/skos/core#Concept"/>
        <skos:definition>Elec. conductivity at 1:5 soil/water ratio</skos:definition>
        <skos:inScheme rdf:resource="http://w3id.org/glosis/model/procedure/electricalConductivityProcedure"/>
        <skos:notation>EC_ratio1-5</skos:notation>
        <skos:prefLabel xml:lang="en">EC_ratio1-5</skos:prefLabel>
        <skos:scopeNote rdf:resource="https://www.isric.org/sites/default/files/isric_report_2014_01.pdf"/>
        <skos:scopeNote>Leenaars J.G.B., A.J.M. van Oostrum and M. Ruiperez Gonzalez, 2014. Africa Soil Profiles Database, Version 1.2. A compilation of georeferenced and standardised legacy soil profile data for Sub-Saharan Africa (with dataset). ISRIC Report 2014/01. Africa Soil Information Service (AfSIS) project and ISRIC - World Soil Information, Wageningen, the Netherlands. See Annex 4.</skos:scopeNote>
        <skos:topConceptOf rdf:resource="http://w3id.org/glosis/model/procedure/electricalConductivityProcedure"/>
    </owl:NamedIndividual>
    


    <!-- http://w3id.org/glosis/model/procedure/electricalConductivityProcedure-ECe_sat -->


    <owl:NamedIndividual rdf:about="http://w3id.org/glosis/model/procedure/electricalConductivityProcedure-ECe_sat">
        <rdf:type rdf:resource="http://w3id.org/glosis/model/procedure/ElectricalConductivityProcedure"/>
        <rdf:type rdf:resource="http://www.w3.org/2004/02/skos/core#Concept"/>
        <skos:definition>Elec. conductivity in saturated paste (ECe)</skos:definition>
        <skos:inScheme rdf:resource="http://w3id.org/glosis/model/procedure/electricalConductivityProcedure"/>
        <skos:notation>ECe_sat</skos:notation>
        <skos:prefLabel xml:lang="en">ECe_sat</skos:prefLabel>
        <skos:scopeNote rdf:resource="https://www.isric.org/sites/default/files/isric_report_2014_01.pdf"/>
        <skos:scopeNote>Leenaars J.G.B., A.J.M. van Oostrum and M. Ruiperez Gonzalez, 2014. Africa Soil Profiles Database, Version 1.2. A compilation of georeferenced and standardised legacy soil profile data for Sub-Saharan Africa (with dataset). ISRIC Report 2014/01. Africa Soil Information Service (AfSIS) project and ISRIC - World Soil Information, Wageningen, the Netherlands. See Annex 4.</skos:scopeNote>
        <skos:topConceptOf rdf:resource="http://w3id.org/glosis/model/procedure/electricalConductivityProcedure"/>
    </owl:NamedIndividual>
    


    <!-- http://w3id.org/glosis/model/procedure/exchangeableBasesProcedure -->


    <owl:NamedIndividual rdf:about="http://w3id.org/glosis/model/procedure/exchangeableBasesProcedure">
        <rdf:type rdf:resource="http://www.w3.org/2004/02/skos/core#ConceptScheme"/>
        <rdfs:label xml:lang="en">Code list for exchangeableBases analysis procedures - codelist scheme</rdfs:label>
        <rdfs:seeAlso rdf:resource="http://w3id.org/glosis/model/procedure/ExchangeableBasesProcedure"/>
        <skos:definition>AfSP-derived interpretation (RwaSP)</skos:definition>
        <skos:note xml:lang="en">This code list provides analysis procedures for exchangeableBases.</skos:note>
        <skos:prefLabel xml:lang="en">Code list for exchangeableBases analysis procedures - codelist scheme</skos:prefLabel>
    </owl:NamedIndividual>
    


    <!-- http://w3id.org/glosis/model/procedure/exchangeableBasesProcedure-ExchBases_ph-unkn-edta -->


    <owl:NamedIndividual rdf:about="http://w3id.org/glosis/model/procedure/exchangeableBasesProcedure-ExchBases_ph-unkn-edta">
        <rdf:type rdf:resource="http://w3id.org/glosis/model/procedure/ExchangeableBasesProcedure"/>
        <rdf:type rdf:resource="http://www.w3.org/2004/02/skos/core#Concept"/>
        <skos:definition>Exch bases (Ca, Mg, K, Na) unknown buffer, in EDTA solution</skos:definition>
        <skos:inScheme rdf:resource="http://w3id.org/glosis/model/procedure/exchangeableBasesProcedure"/>
        <skos:notation>ExchBases_ph-unkn-edta</skos:notation>
        <skos:prefLabel xml:lang="en">ExchBases_ph-unkn-edta</skos:prefLabel>
        <skos:scopeNote rdf:resource="https://www.isric.org/sites/default/files/isric_report_2014_01.pdf"/>
        <skos:scopeNote>Leenaars J.G.B., A.J.M. van Oostrum and M. Ruiperez Gonzalez, 2014. Africa Soil Profiles Database, Version 1.2. A compilation of georeferenced and standardised legacy soil profile data for Sub-Saharan Africa (with dataset). ISRIC Report 2014/01. Africa Soil Information Service (AfSIS) project and ISRIC - World Soil Information, Wageningen, the Netherlands. See Annex 4.</skos:scopeNote>
        <skos:topConceptOf rdf:resource="http://w3id.org/glosis/model/procedure/exchangeableBasesProcedure"/>
    </owl:NamedIndividual>
    


    <!-- http://w3id.org/glosis/model/procedure/exchangeableBasesProcedure-ExchBases_ph-unkn-m3 -->


    <owl:NamedIndividual rdf:about="http://w3id.org/glosis/model/procedure/exchangeableBasesProcedure-ExchBases_ph-unkn-m3">
        <rdf:type rdf:resource="http://w3id.org/glosis/model/procedure/ExchangeableBasesProcedure"/>
        <rdf:type rdf:resource="http://www.w3.org/2004/02/skos/core#Concept"/>
        <skos:definition>Exch bases (Ca, Mg, K, Na) unknown buffer, in Mehlich3 solution with extractable ppm assumed exchangeable cmolc/kg</skos:definition>
        <skos:inScheme rdf:resource="http://w3id.org/glosis/model/procedure/exchangeableBasesProcedure"/>
        <skos:notation>ExchBases_ph-unkn-m3</skos:notation>
        <skos:prefLabel xml:lang="en">ExchBases_ph-unkn-m3</skos:prefLabel>
        <skos:scopeNote rdf:resource="https://doi.org/10.1080/00103628409367568"/>
        <skos:topConceptOf rdf:resource="http://w3id.org/glosis/model/procedure/exchangeableBasesProcedure"/>
    </owl:NamedIndividual>
    


    <!-- http://w3id.org/glosis/model/procedure/exchangeableBasesProcedure-ExchBases_ph-unkn-m3-spec -->


    <owl:NamedIndividual rdf:about="http://w3id.org/glosis/model/procedure/exchangeableBasesProcedure-ExchBases_ph-unkn-m3-spec">
        <rdf:type rdf:resource="http://w3id.org/glosis/model/procedure/ExchangeableBasesProcedure"/>
        <rdf:type rdf:resource="http://www.w3.org/2004/02/skos/core#Concept"/>
        <skos:definition>Exch bases (Ca, Mg, K, Na) spectrally measured and converted to, unknown buffer, in Mehlich3 solution with extractable ppm assumed exchangeable cmolc/kg</skos:definition>
        <skos:inScheme rdf:resource="http://w3id.org/glosis/model/procedure/exchangeableBasesProcedure"/>
        <skos:notation>ExchBases_ph-unkn-m3-spec</skos:notation>
        <skos:prefLabel xml:lang="en">ExchBases_ph-unkn-m3-spec</skos:prefLabel>
        <skos:scopeNote rdf:resource="https://doi.org/10.1080/00103628409367568"/>
        <skos:topConceptOf rdf:resource="http://w3id.org/glosis/model/procedure/exchangeableBasesProcedure"/>
    </owl:NamedIndividual>
    


    <!-- http://w3id.org/glosis/model/procedure/exchangeableBasesProcedure-ExchBases_ph0-cohex -->


    <owl:NamedIndividual rdf:about="http://w3id.org/glosis/model/procedure/exchangeableBasesProcedure-ExchBases_ph0-cohex">
        <rdf:type rdf:resource="http://w3id.org/glosis/model/procedure/ExchangeableBasesProcedure"/>
        <rdf:type rdf:resource="http://www.w3.org/2004/02/skos/core#Concept"/>
        <skos:definition>Exch bases (Ca, Mg, K, Na) unbuffered, in Cobalt(III) hexamine chloride solution 0,0166M (Cohex) [Co[NH3]6]Cl3 ), ISO 23470 (2007)</skos:definition>
        <skos:inScheme rdf:resource="http://w3id.org/glosis/model/procedure/exchangeableBasesProcedure"/>
        <skos:notation>ExchBases_ph0-cohex</skos:notation>
        <skos:prefLabel xml:lang="en">ExchBases_ph0-cohex</skos:prefLabel>
        <skos:scopeNote rdf:resource="https://www.iso.org/standard/36879.html"/>
        <skos:topConceptOf rdf:resource="http://w3id.org/glosis/model/procedure/exchangeableBasesProcedure"/>
    </owl:NamedIndividual>
    


    <!-- http://w3id.org/glosis/model/procedure/exchangeableBasesProcedure-ExchBases_ph0-nh4cl -->


    <owl:NamedIndividual rdf:about="http://w3id.org/glosis/model/procedure/exchangeableBasesProcedure-ExchBases_ph0-nh4cl">
        <rdf:type rdf:resource="http://w3id.org/glosis/model/procedure/ExchangeableBasesProcedure"/>
        <rdf:type rdf:resource="http://www.w3.org/2004/02/skos/core#Concept"/>
        <skos:definition>Exch bases (Ca, Mg, K, Na) unbuffered, in 1 M NH4Cl (0.05-1.0 m?)</skos:definition>
        <skos:inScheme rdf:resource="http://w3id.org/glosis/model/procedure/exchangeableBasesProcedure"/>
        <skos:notation>ExchBases_ph0-nh4cl</skos:notation>
        <skos:prefLabel xml:lang="en">ExchBases_ph0-nh4cl</skos:prefLabel>
        <skos:scopeNote rdf:resource="https://www.isric.org/sites/default/files/isric_report_2014_01.pdf"/>
        <skos:scopeNote>Leenaars J.G.B., A.J.M. van Oostrum and M. Ruiperez Gonzalez, 2014. Africa Soil Profiles Database, Version 1.2. A compilation of georeferenced and standardised legacy soil profile data for Sub-Saharan Africa (with dataset). ISRIC Report 2014/01. Africa Soil Information Service (AfSIS) project and ISRIC - World Soil Information, Wageningen, the Netherlands. See Annex 4.</skos:scopeNote>
        <skos:topConceptOf rdf:resource="http://w3id.org/glosis/model/procedure/exchangeableBasesProcedure"/>
    </owl:NamedIndividual>
    


    <!-- http://w3id.org/glosis/model/procedure/exchangeableBasesProcedure-ExchBases_ph7-nh4oac -->


    <owl:NamedIndividual rdf:about="http://w3id.org/glosis/model/procedure/exchangeableBasesProcedure-ExchBases_ph7-nh4oac">
        <rdf:type rdf:resource="http://w3id.org/glosis/model/procedure/ExchangeableBasesProcedure"/>
        <rdf:type rdf:resource="http://www.w3.org/2004/02/skos/core#Concept"/>
        <skos:definition>Exch bases (Ca, Mg, K, Na) buffered at pH 7, in 1M NH4OAc</skos:definition>
        <skos:inScheme rdf:resource="http://w3id.org/glosis/model/procedure/exchangeableBasesProcedure"/>
        <skos:notation>ExchBases_ph7-nh4oac</skos:notation>
        <skos:prefLabel xml:lang="en">ExchBases_ph7-nh4oac</skos:prefLabel>
        <skos:scopeNote rdf:resource="https://www.isric.org/sites/default/files/isric_report_2014_01.pdf"/>
        <skos:scopeNote>Leenaars J.G.B., A.J.M. van Oostrum and M. Ruiperez Gonzalez, 2014. Africa Soil Profiles Database, Version 1.2. A compilation of georeferenced and standardised legacy soil profile data for Sub-Saharan Africa (with dataset). ISRIC Report 2014/01. Africa Soil Information Service (AfSIS) project and ISRIC - World Soil Information, Wageningen, the Netherlands. See Annex 4.</skos:scopeNote>
        <skos:topConceptOf rdf:resource="http://w3id.org/glosis/model/procedure/exchangeableBasesProcedure"/>
    </owl:NamedIndividual>
    


    <!-- http://w3id.org/glosis/model/procedure/exchangeableBasesProcedure-ExchBases_ph7-nh4oac-aas -->


    <owl:NamedIndividual rdf:about="http://w3id.org/glosis/model/procedure/exchangeableBasesProcedure-ExchBases_ph7-nh4oac-aas">
        <rdf:type rdf:resource="http://w3id.org/glosis/model/procedure/ExchangeableBasesProcedure"/>
        <rdf:type rdf:resource="http://www.w3.org/2004/02/skos/core#Concept"/>
        <skos:definition>Exch bases (Ca, Mg, K, Na) buffered at pH 7, in 1M NH4OAc, Ca and Mg with AAS (Atomic Absorption Spectrometry)</skos:definition>
        <skos:inScheme rdf:resource="http://w3id.org/glosis/model/procedure/exchangeableBasesProcedure"/>
        <skos:notation>ExchBases_ph7-nh4oac-aas</skos:notation>
        <skos:prefLabel xml:lang="en">ExchBases_ph7-nh4oac-aas</skos:prefLabel>
        <skos:scopeNote rdf:resource="https://www.isric.org/sites/default/files/isric_report_2014_01.pdf"/>
        <skos:scopeNote>Leenaars J.G.B., A.J.M. van Oostrum and M. Ruiperez Gonzalez, 2014. Africa Soil Profiles Database, Version 1.2. A compilation of georeferenced and standardised legacy soil profile data for Sub-Saharan Africa (with dataset). ISRIC Report 2014/01. Africa Soil Information Service (AfSIS) project and ISRIC - World Soil Information, Wageningen, the Netherlands. See Annex 4.</skos:scopeNote>
        <skos:topConceptOf rdf:resource="http://w3id.org/glosis/model/procedure/exchangeableBasesProcedure"/>
    </owl:NamedIndividual>
    


    <!-- http://w3id.org/glosis/model/procedure/exchangeableBasesProcedure-ExchBases_ph7-nh4oac-fp -->


    <owl:NamedIndividual rdf:about="http://w3id.org/glosis/model/procedure/exchangeableBasesProcedure-ExchBases_ph7-nh4oac-fp">
        <rdf:type rdf:resource="http://w3id.org/glosis/model/procedure/ExchangeableBasesProcedure"/>
        <rdf:type rdf:resource="http://www.w3.org/2004/02/skos/core#Concept"/>
        <skos:definition>Exch bases (Ca, Mg, K, Na) buffered at pH 7, in 1M NH4OAc, K and Na with FP (Flame Photometry)</skos:definition>
        <skos:inScheme rdf:resource="http://w3id.org/glosis/model/procedure/exchangeableBasesProcedure"/>
        <skos:notation>ExchBases_ph7-nh4oac-fp</skos:notation>
        <skos:prefLabel xml:lang="en">ExchBases_ph7-nh4oac-fp</skos:prefLabel>
        <skos:scopeNote rdf:resource="https://www.isric.org/sites/default/files/isric_report_2014_01.pdf"/>
        <skos:scopeNote>Leenaars J.G.B., A.J.M. van Oostrum and M. Ruiperez Gonzalez, 2014. Africa Soil Profiles Database, Version 1.2. A compilation of georeferenced and standardised legacy soil profile data for Sub-Saharan Africa (with dataset). ISRIC Report 2014/01. Africa Soil Information Service (AfSIS) project and ISRIC - World Soil Information, Wageningen, the Netherlands. See Annex 4.</skos:scopeNote>
        <skos:topConceptOf rdf:resource="http://w3id.org/glosis/model/procedure/exchangeableBasesProcedure"/>
    </owl:NamedIndividual>
    


    <!-- http://w3id.org/glosis/model/procedure/exchangeableBasesProcedure-ExchBases_ph7-unkn -->


    <owl:NamedIndividual rdf:about="http://w3id.org/glosis/model/procedure/exchangeableBasesProcedure-ExchBases_ph7-unkn">
        <rdf:type rdf:resource="http://w3id.org/glosis/model/procedure/ExchangeableBasesProcedure"/>
        <rdf:type rdf:resource="http://www.w3.org/2004/02/skos/core#Concept"/>
        <skos:definition>Exch bases (Ca, Mg, K, Na) buffered at pH 7, in unknown solution</skos:definition>
        <skos:inScheme rdf:resource="http://w3id.org/glosis/model/procedure/exchangeableBasesProcedure"/>
        <skos:notation>ExchBases_ph7-unkn</skos:notation>
        <skos:prefLabel xml:lang="en">ExchBases_ph7-unk</skos:prefLabel>
        <skos:scopeNote rdf:resource="https://www.isric.org/sites/default/files/WOSISprocedureManual_2020nov17web.pdf#page=70"/>
        <skos:topConceptOf rdf:resource="http://w3id.org/glosis/model/procedure/exchangeableBasesProcedure"/>
    </owl:NamedIndividual>
    


    <!-- http://w3id.org/glosis/model/procedure/exchangeableBasesProcedure-ExchBases_ph8-bacl2tea -->


    <owl:NamedIndividual rdf:about="http://w3id.org/glosis/model/procedure/exchangeableBasesProcedure-ExchBases_ph8-bacl2tea">
        <rdf:type rdf:resource="http://w3id.org/glosis/model/procedure/ExchangeableBasesProcedure"/>
        <rdf:type rdf:resource="http://www.w3.org/2004/02/skos/core#Concept"/>
        <skos:definition>Exch bases (Ca, Mg, K, Na) buffered at pH 8.0-8.5, in 0.5 M BaCl2 - TEA solution</skos:definition>
        <skos:inScheme rdf:resource="http://w3id.org/glosis/model/procedure/exchangeableBasesProcedure"/>
        <skos:notation>ExchBases_ph8-bacl2tea</skos:notation>
        <skos:prefLabel xml:lang="en">ExchBases_ph8-bacl2tea</skos:prefLabel>
        <skos:scopeNote rdf:resource="https://www.isric.org/sites/default/files/isric_report_2014_01.pdf"/>
        <skos:scopeNote>Leenaars J.G.B., A.J.M. van Oostrum and M. Ruiperez Gonzalez, 2014. Africa Soil Profiles Database, Version 1.2. A compilation of georeferenced and standardised legacy soil profile data for Sub-Saharan Africa (with dataset). ISRIC Report 2014/01. Africa Soil Information Service (AfSIS) project and ISRIC - World Soil Information, Wageningen, the Netherlands. See Annex 4.</skos:scopeNote>
        <skos:topConceptOf rdf:resource="http://w3id.org/glosis/model/procedure/exchangeableBasesProcedure"/>
    </owl:NamedIndividual>
    


    <!-- http://w3id.org/glosis/model/procedure/exchangeableBasesProcedure-ExchBases_ph8-unkn -->


    <owl:NamedIndividual rdf:about="http://w3id.org/glosis/model/procedure/exchangeableBasesProcedure-ExchBases_ph8-unkn">
        <rdf:type rdf:resource="http://w3id.org/glosis/model/procedure/ExchangeableBasesProcedure"/>
        <rdf:type rdf:resource="http://www.w3.org/2004/02/skos/core#Concept"/>
        <skos:definition>Exch bases (Ca, Mg, K, Na) buffered at pH 8.0-8.5, in unknown solution</skos:definition>
        <skos:inScheme rdf:resource="http://w3id.org/glosis/model/procedure/exchangeableBasesProcedure"/>
        <skos:notation>ExchBases_ph8-unkn</skos:notation>
        <skos:prefLabel xml:lang="en">ExchBases_ph8-unk</skos:prefLabel>
        <skos:scopeNote rdf:resource="https://www.isric.org/sites/default/files/isric_report_2014_01.pdf"/>
        <skos:scopeNote>Leenaars J.G.B., A.J.M. van Oostrum and M. Ruiperez Gonzalez, 2014. Africa Soil Profiles Database, Version 1.2. A compilation of georeferenced and standardised legacy soil profile data for Sub-Saharan Africa (with dataset). ISRIC Report 2014/01. Africa Soil Information Service (AfSIS) project and ISRIC - World Soil Information, Wageningen, the Netherlands. See Annex 4.</skos:scopeNote>
        <skos:topConceptOf rdf:resource="http://w3id.org/glosis/model/procedure/exchangeableBasesProcedure"/>
    </owl:NamedIndividual>
    


    <!-- http://w3id.org/glosis/model/procedure/extractableElementsProcedure -->


    <owl:NamedIndividual rdf:about="http://w3id.org/glosis/model/procedure/extractableElementsProcedure">
        <rdf:type rdf:resource="http://www.w3.org/2004/02/skos/core#ConceptScheme"/>
        <rdfs:label xml:lang="en">Code list for extractableElements analysis procedures - codelist scheme</rdfs:label>
        <rdfs:seeAlso rdf:resource="http://w3id.org/glosis/model/procedure/ExtractableElementsProcedure"/>
        <skos:definition>AfSP-derived interpretation (RwaSP)</skos:definition>
        <skos:note xml:lang="en">This code list provides analysis procedures for extractableElements.</skos:note>
        <skos:prefLabel xml:lang="en">Code list for extractableElements analysis procedures - codelist scheme</skos:prefLabel>
    </owl:NamedIndividual>
    


    <!-- http://w3id.org/glosis/model/procedure/extractableElementsProcedure-Extr_ap14 -->


    <owl:NamedIndividual rdf:about="http://w3id.org/glosis/model/procedure/extractableElementsProcedure-Extr_ap14">
        <rdf:type rdf:resource="http://w3id.org/glosis/model/procedure/ExtractableElementsProcedure"/>
        <rdf:type rdf:resource="http://www.w3.org/2004/02/skos/core#Concept"/>
        <skos:definition>Method of Saunders and Metelerkamp (anion-exch. resin). Particularly used for available P.</skos:definition>
        <skos:inScheme rdf:resource="http://w3id.org/glosis/model/procedure/extractableElementsProcedure"/>
        <skos:notation>Extr_ap14</skos:notation>
        <skos:prefLabel xml:lang="en">Extr_ap14</skos:prefLabel>
        <skos:scopeNote>Saunders and Metelerkamp</skos:scopeNote>
        <skos:topConceptOf rdf:resource="http://w3id.org/glosis/model/procedure/extractableElementsProcedure"/>
    </owl:NamedIndividual>
    


    <!-- http://w3id.org/glosis/model/procedure/extractableElementsProcedure-Extr_ap15 -->


    <owl:NamedIndividual rdf:about="http://w3id.org/glosis/model/procedure/extractableElementsProcedure-Extr_ap15">
        <rdf:type rdf:resource="http://w3id.org/glosis/model/procedure/ExtractableElementsProcedure"/>
        <rdf:type rdf:resource="http://www.w3.org/2004/02/skos/core#Concept"/>
        <skos:definition>Method of Hunter (1975) modified after ISFEI method. Particularly used for available P.</skos:definition>
        <skos:inScheme rdf:resource="http://w3id.org/glosis/model/procedure/extractableElementsProcedure"/>
        <skos:notation>Extr_ap15</skos:notation>
        <skos:prefLabel xml:lang="en">Extr_ap15</skos:prefLabel>
        <skos:scopeNote>Hunter, A. 1975. New techniques and equipment for routine soil/plant analytical procedures. In: Soil Management in Tropical America. (eds E. Borremiza &amp; A. Alvarado). N.C. State University, Raleigh, NC.</skos:scopeNote>
        <skos:topConceptOf rdf:resource="http://w3id.org/glosis/model/procedure/extractableElementsProcedure"/>
    </owl:NamedIndividual>
    


    <!-- http://w3id.org/glosis/model/procedure/extractableElementsProcedure-Extr_ap20 -->


    <owl:NamedIndividual rdf:about="http://w3id.org/glosis/model/procedure/extractableElementsProcedure-Extr_ap20">
        <rdf:type rdf:resource="http://w3id.org/glosis/model/procedure/ExtractableElementsProcedure"/>
        <rdf:type rdf:resource="http://www.w3.org/2004/02/skos/core#Concept"/>
        <skos:definition>Olsen (not acid soils) resp. Bray I (acid soils). Particularly used for available P.</skos:definition>
        <skos:inScheme rdf:resource="http://w3id.org/glosis/model/procedure/extractableElementsProcedure"/>
        <skos:notation>Extr_ap20</skos:notation>
        <skos:prefLabel xml:lang="en">Extr_ap20</skos:prefLabel>
        <skos:scopeNote rdf:resource="https://www.isric.org/sites/default/files/isric_report_2014_01.pdf"/>
        <skos:scopeNote>Leenaars J.G.B., A.J.M. van Oostrum and M. Ruiperez Gonzalez, 2014. Africa Soil Profiles Database, Version 1.2. A compilation of georeferenced and standardised legacy soil profile data for Sub-Saharan Africa (with dataset). ISRIC Report 2014/01. Africa Soil Information Service (AfSIS) project and ISRIC - World Soil Information, Wageningen, the Netherlands. See Annex 4.</skos:scopeNote>
        <skos:topConceptOf rdf:resource="http://w3id.org/glosis/model/procedure/extractableElementsProcedure"/>
    </owl:NamedIndividual>
    


    <!-- http://w3id.org/glosis/model/procedure/extractableElementsProcedure-Extr_ap21 -->


    <owl:NamedIndividual rdf:about="http://w3id.org/glosis/model/procedure/extractableElementsProcedure-Extr_ap21">
        <rdf:type rdf:resource="http://w3id.org/glosis/model/procedure/ExtractableElementsProcedure"/>
        <rdf:type rdf:resource="http://www.w3.org/2004/02/skos/core#Concept"/>
        <skos:definition>Olsen (if pH &gt; 7) resp. Mehlich (if pH &lt; 7). Particularly used for available P.</skos:definition>
        <skos:inScheme rdf:resource="http://w3id.org/glosis/model/procedure/extractableElementsProcedure"/>
        <skos:notation>Extr_ap21</skos:notation>
        <skos:prefLabel xml:lang="en">Extr_ap21</skos:prefLabel>
        <skos:scopeNote rdf:resource="https://www.isric.org/sites/default/files/isric_report_2014_01.pdf"/>
        <skos:scopeNote>Leenaars J.G.B., A.J.M. van Oostrum and M. Ruiperez Gonzalez, 2014. Africa Soil Profiles Database, Version 1.2. A compilation of georeferenced and standardised legacy soil profile data for Sub-Saharan Africa (with dataset). ISRIC Report 2014/01. Africa Soil Information Service (AfSIS) project and ISRIC - World Soil Information, Wageningen, the Netherlands. See Annex 4.</skos:scopeNote>
        <skos:topConceptOf rdf:resource="http://w3id.org/glosis/model/procedure/extractableElementsProcedure"/>
    </owl:NamedIndividual>
    


    <!-- http://w3id.org/glosis/model/procedure/extractableElementsProcedure-Extr_c6h8o7-reeuwijk -->


    <owl:NamedIndividual rdf:about="http://w3id.org/glosis/model/procedure/extractableElementsProcedure-Extr_c6h8o7-reeuwijk">
        <rdf:type rdf:resource="http://w3id.org/glosis/model/procedure/ExtractableElementsProcedure"/>
        <rdf:type rdf:resource="http://www.w3.org/2004/02/skos/core#Concept"/>
        <skos:definition>Complexation with citric acid (van Reeuwijk). Particularly used for available P.</skos:definition>
        <skos:inScheme rdf:resource="http://w3id.org/glosis/model/procedure/extractableElementsProcedure"/>
        <skos:notation>Extr_c6h8o7-reeuwijk</skos:notation>
        <skos:prefLabel xml:lang="en">Extr_c6h8o7-reeuwijk</skos:prefLabel>
        <skos:scopeNote rdf:resource="https://www.isric.org/documents/document-type/technical-paper-09-procedures-soil-analysis-6th-edition"/>
        <skos:topConceptOf rdf:resource="http://w3id.org/glosis/model/procedure/extractableElementsProcedure"/>
    </owl:NamedIndividual>
    


    <!-- http://w3id.org/glosis/model/procedure/extractableElementsProcedure-Extr_cacl2 -->


    <owl:NamedIndividual rdf:about="http://w3id.org/glosis/model/procedure/extractableElementsProcedure-Extr_cacl2">
        <rdf:type rdf:resource="http://w3id.org/glosis/model/procedure/ExtractableElementsProcedure"/>
        <rdf:type rdf:resource="http://www.w3.org/2004/02/skos/core#Concept"/>
        <skos:definition>CaCl2. Particularly used for soluble P.</skos:definition>
        <skos:inScheme rdf:resource="http://w3id.org/glosis/model/procedure/extractableElementsProcedure"/>
        <skos:notation>Extr_cacl2</skos:notation>
        <skos:prefLabel xml:lang="en">Extr_cacl2</skos:prefLabel>
        <skos:scopeNote rdf:resource="https://www.isric.org/sites/default/files/isric_report_2014_01.pdf"/>
        <skos:scopeNote>Leenaars J.G.B., A.J.M. van Oostrum and M. Ruiperez Gonzalez, 2014. Africa Soil Profiles Database, Version 1.2. A compilation of georeferenced and standardised legacy soil profile data for Sub-Saharan Africa (with dataset). ISRIC Report 2014/01. Africa Soil Information Service (AfSIS) project and ISRIC - World Soil Information, Wageningen, the Netherlands. See Annex 4.</skos:scopeNote>
        <skos:topConceptOf rdf:resource="http://w3id.org/glosis/model/procedure/extractableElementsProcedure"/>
    </owl:NamedIndividual>
    


    <!-- http://w3id.org/glosis/model/procedure/extractableElementsProcedure-Extr_capo4 -->


    <owl:NamedIndividual rdf:about="http://w3id.org/glosis/model/procedure/extractableElementsProcedure-Extr_capo4">
        <rdf:type rdf:resource="http://w3id.org/glosis/model/procedure/ExtractableElementsProcedure"/>
        <rdf:type rdf:resource="http://www.w3.org/2004/02/skos/core#Concept"/>
        <skos:definition>Ca phosphate. Particularly used for available S.</skos:definition>
        <skos:inScheme rdf:resource="http://w3id.org/glosis/model/procedure/extractableElementsProcedure"/>
        <skos:notation>Extr_capo4</skos:notation>
        <skos:prefLabel xml:lang="en">Extr_capo4</skos:prefLabel>
        <skos:scopeNote rdf:resource="https://www.isric.org/sites/default/files/isric_report_2014_01.pdf"/>
        <skos:scopeNote>Leenaars J.G.B., A.J.M. van Oostrum and M. Ruiperez Gonzalez, 2014. Africa Soil Profiles Database, Version 1.2. A compilation of georeferenced and standardised legacy soil profile data for Sub-Saharan Africa (with dataset). ISRIC Report 2014/01. Africa Soil Information Service (AfSIS) project and ISRIC - World Soil Information, Wageningen, the Netherlands. See Annex 4.</skos:scopeNote>
        <skos:topConceptOf rdf:resource="http://w3id.org/glosis/model/procedure/extractableElementsProcedure"/>
    </owl:NamedIndividual>
    


    <!-- http://w3id.org/glosis/model/procedure/extractableElementsProcedure-Extr_dtpa -->


    <owl:NamedIndividual rdf:about="http://w3id.org/glosis/model/procedure/extractableElementsProcedure-Extr_dtpa">
        <rdf:type rdf:resource="http://w3id.org/glosis/model/procedure/ExtractableElementsProcedure"/>
        <rdf:type rdf:resource="http://www.w3.org/2004/02/skos/core#Concept"/>
        <skos:definition>DiethyneleTriaminePentaAcetic acid (DTPA) method</skos:definition>
        <skos:inScheme rdf:resource="http://w3id.org/glosis/model/procedure/extractableElementsProcedure"/>
        <skos:notation>Extr_dtpa</skos:notation>
        <skos:prefLabel xml:lang="en">Extr_dtpa</skos:prefLabel>
        <skos:scopeNote rdf:resource="https://doi.org/10.2136/sssaj1978.03615995004200030009x"/>
        <skos:topConceptOf rdf:resource="http://w3id.org/glosis/model/procedure/extractableElementsProcedure"/>
    </owl:NamedIndividual>
    


    <!-- http://w3id.org/glosis/model/procedure/extractableElementsProcedure-Extr_edta -->


    <owl:NamedIndividual rdf:about="http://w3id.org/glosis/model/procedure/extractableElementsProcedure-Extr_edta">
        <rdf:type rdf:resource="http://w3id.org/glosis/model/procedure/ExtractableElementsProcedure"/>
        <rdf:type rdf:resource="http://www.w3.org/2004/02/skos/core#Concept"/>
        <skos:definition>EthyleneDiamineTetraAcetic acid (EDTA) method</skos:definition>
        <skos:inScheme rdf:resource="http://w3id.org/glosis/model/procedure/extractableElementsProcedure"/>
        <skos:notation>Extr_edta</skos:notation>
        <skos:prefLabel xml:lang="en">Extr_edta</skos:prefLabel>
        <skos:scopeNote rdf:resource="https://journals.lww.com/soilsci/Citation/1954/10000/SOIL_AND_PLANT_STUDIES_WITH_CHELATES_OF.8.aspx"/>
        <skos:topConceptOf rdf:resource="http://w3id.org/glosis/model/procedure/extractableElementsProcedure"/>
    </owl:NamedIndividual>
    


    <!-- http://w3id.org/glosis/model/procedure/extractableElementsProcedure-Extr_h2so4-truog -->


    <owl:NamedIndividual rdf:about="http://w3id.org/glosis/model/procedure/extractableElementsProcedure-Extr_h2so4-truog">
        <rdf:type rdf:resource="http://w3id.org/glosis/model/procedure/ExtractableElementsProcedure"/>
        <rdf:type rdf:resource="http://www.w3.org/2004/02/skos/core#Concept"/>
        <skos:definition>Method of Truog (dilute H2SO4). Particularly used for available P.</skos:definition>
        <skos:inScheme rdf:resource="http://w3id.org/glosis/model/procedure/extractableElementsProcedure"/>
        <skos:notation>Extr_h2so4-truog</skos:notation>
        <skos:prefLabel xml:lang="en">Extr_h2so4-truog</skos:prefLabel>
        <skos:scopeNote rdf:resource="https://doi.org/10.2134/agronj1930.00021962002200100008x"/>
        <skos:topConceptOf rdf:resource="http://w3id.org/glosis/model/procedure/extractableElementsProcedure"/>
    </owl:NamedIndividual>
    


    <!-- http://w3id.org/glosis/model/procedure/extractableElementsProcedure-Extr_hcl-h2so4-nelson -->


    <owl:NamedIndividual rdf:about="http://w3id.org/glosis/model/procedure/extractableElementsProcedure-Extr_hcl-h2so4-nelson">
        <rdf:type rdf:resource="http://w3id.org/glosis/model/procedure/ExtractableElementsProcedure"/>
        <rdf:type rdf:resource="http://www.w3.org/2004/02/skos/core#Concept"/>
        <skos:definition>Method of Nelson (dilute HCl/H2SO4). Particularly used for available P.</skos:definition>
        <skos:inScheme rdf:resource="http://w3id.org/glosis/model/procedure/extractableElementsProcedure"/>
        <skos:notation>Extr_hcl-h2so4-nelson</skos:notation>
        <skos:prefLabel xml:lang="en">Extr_hcl-h2so4-nelso</skos:prefLabel>
        <skos:scopeNote rdf:resource="https://www.isric.org/sites/default/files/isric_report_2014_01.pdf"/>
        <skos:scopeNote>Leenaars J.G.B., A.J.M. van Oostrum and M. Ruiperez Gonzalez, 2014. Africa Soil Profiles Database, Version 1.2. A compilation of georeferenced and standardised legacy soil profile data for Sub-Saharan Africa (with dataset). ISRIC Report 2014/01. Africa Soil Information Service (AfSIS) project and ISRIC - World Soil Information, Wageningen, the Netherlands. See Annex 4.</skos:scopeNote>
        <skos:topConceptOf rdf:resource="http://w3id.org/glosis/model/procedure/extractableElementsProcedure"/>
    </owl:NamedIndividual>
    


    <!-- http://w3id.org/glosis/model/procedure/extractableElementsProcedure-Extr_hcl-nh4f-bray1 -->


    <owl:NamedIndividual rdf:about="http://w3id.org/glosis/model/procedure/extractableElementsProcedure-Extr_hcl-nh4f-bray1">
        <rdf:type rdf:resource="http://w3id.org/glosis/model/procedure/ExtractableElementsProcedure"/>
        <rdf:type rdf:resource="http://www.w3.org/2004/02/skos/core#Concept"/>
        <skos:definition>Method of Bray I  (dilute HCl/NH4F). Particularly used for available P.</skos:definition>
        <skos:inScheme rdf:resource="http://w3id.org/glosis/model/procedure/extractableElementsProcedure"/>
        <skos:notation>Extr_hcl-nh4f-bray1</skos:notation>
        <skos:prefLabel xml:lang="en">Extr_hcl-nh4f-bray1</skos:prefLabel>
        <skos:scopeNote rdf:resource="https://doi.org/10.1097/00010694-194501000-00006"/>
        <skos:topConceptOf rdf:resource="http://w3id.org/glosis/model/procedure/extractableElementsProcedure"/>
    </owl:NamedIndividual>
    


    <!-- http://w3id.org/glosis/model/procedure/extractableElementsProcedure-Extr_hcl-nh4f-bray2 -->


    <owl:NamedIndividual rdf:about="http://w3id.org/glosis/model/procedure/extractableElementsProcedure-Extr_hcl-nh4f-bray2">
        <rdf:type rdf:resource="http://w3id.org/glosis/model/procedure/ExtractableElementsProcedure"/>
        <rdf:type rdf:resource="http://www.w3.org/2004/02/skos/core#Concept"/>
        <skos:definition>Method of Bray II (dilute HCl/NH4F). Particularly used for available P.</skos:definition>
        <skos:inScheme rdf:resource="http://w3id.org/glosis/model/procedure/extractableElementsProcedure"/>
        <skos:notation>Extr_hcl-nh4f-bray2</skos:notation>
        <skos:prefLabel xml:lang="en">Extr_hcl-nh4f-bray2</skos:prefLabel>
        <skos:scopeNote rdf:resource="https://doi.org/10.1097/00010694-194501000-00006"/>
        <skos:topConceptOf rdf:resource="http://w3id.org/glosis/model/procedure/extractableElementsProcedure"/>
    </owl:NamedIndividual>
    


    <!-- http://w3id.org/glosis/model/procedure/extractableElementsProcedure-Extr_hcl-nh4f-kurtz-bray -->


    <owl:NamedIndividual rdf:about="http://w3id.org/glosis/model/procedure/extractableElementsProcedure-Extr_hcl-nh4f-kurtz-bray">
        <rdf:type rdf:resource="http://w3id.org/glosis/model/procedure/ExtractableElementsProcedure"/>
        <rdf:type rdf:resource="http://www.w3.org/2004/02/skos/core#Concept"/>
        <skos:definition>Method of Kurtz-Bray I (0.025 M HCl + 0.03 M NH4F). Particularly used for available P.</skos:definition>
        <skos:inScheme rdf:resource="http://w3id.org/glosis/model/procedure/extractableElementsProcedure"/>
        <skos:notation>Extr_hcl-nh4f-kurtz-bray</skos:notation>
        <skos:prefLabel xml:lang="en">Extr_hcl-nh4f-kurtz-bray</skos:prefLabel>
        <skos:scopeNote rdf:resource="https://doi.org/10.1097/00010694-194501000-00006"/>
        <skos:topConceptOf rdf:resource="http://w3id.org/glosis/model/procedure/extractableElementsProcedure"/>
    </owl:NamedIndividual>
    


    <!-- http://w3id.org/glosis/model/procedure/extractableElementsProcedure-Extr_hno3 -->


    <owl:NamedIndividual rdf:about="http://w3id.org/glosis/model/procedure/extractableElementsProcedure-Extr_hno3">
        <rdf:type rdf:resource="http://w3id.org/glosis/model/procedure/ExtractableElementsProcedure"/>
        <rdf:type rdf:resource="http://www.w3.org/2004/02/skos/core#Concept"/>
        <skos:definition>Nitric acid (HNO3) method</skos:definition>
        <skos:inScheme rdf:resource="http://w3id.org/glosis/model/procedure/extractableElementsProcedure"/>
        <skos:notation>Extr_hno3</skos:notation>
        <skos:prefLabel xml:lang="en">Extr_hno3</skos:prefLabel>
        <skos:scopeNote rdf:resource="https://www.iso.org/standard/60060.html"/>
        <skos:scopeNote>ISO. ISO/DIS 17586 Soil Quality - Extraction of Trace Elements Using Dilute Nitric Acid, 2016; p 14</skos:scopeNote>
        <skos:topConceptOf rdf:resource="http://w3id.org/glosis/model/procedure/extractableElementsProcedure"/>
    </owl:NamedIndividual>
    


    <!-- http://w3id.org/glosis/model/procedure/extractableElementsProcedure-Extr_hotwater -->


    <owl:NamedIndividual rdf:about="http://w3id.org/glosis/model/procedure/extractableElementsProcedure-Extr_hotwater">
        <rdf:type rdf:resource="http://w3id.org/glosis/model/procedure/ExtractableElementsProcedure"/>
        <rdf:type rdf:resource="http://www.w3.org/2004/02/skos/core#Concept"/>
        <skos:definition>Hot water. Particularly used for available B</skos:definition>
        <skos:inScheme rdf:resource="http://w3id.org/glosis/model/procedure/extractableElementsProcedure"/>
        <skos:notation>Extr_hotwater</skos:notation>
        <skos:prefLabel xml:lang="en">Extr_hotwater</skos:prefLabel>
        <skos:scopeNote rdf:resource="https://www.isric.org/sites/default/files/isric_report_2014_01.pdf"/>
        <skos:scopeNote>Leenaars J.G.B., A.J.M. van Oostrum and M. Ruiperez Gonzalez, 2014. Africa Soil Profiles Database, Version 1.2. A compilation of georeferenced and standardised legacy soil profile data for Sub-Saharan Africa (with dataset). ISRIC Report 2014/01. Africa Soil Information Service (AfSIS) project and ISRIC - World Soil Information, Wageningen, the Netherlands. See Annex 4.</skos:scopeNote>
        <skos:topConceptOf rdf:resource="http://w3id.org/glosis/model/procedure/extractableElementsProcedure"/>
    </owl:NamedIndividual>
    


    <!-- http://w3id.org/glosis/model/procedure/extractableElementsProcedure-Extr_m1 -->


    <owl:NamedIndividual rdf:about="http://w3id.org/glosis/model/procedure/extractableElementsProcedure-Extr_m1">
        <rdf:type rdf:resource="http://w3id.org/glosis/model/procedure/ExtractableElementsProcedure"/>
        <rdf:type rdf:resource="http://www.w3.org/2004/02/skos/core#Concept"/>
        <skos:definition>Mehlich1 method</skos:definition>
        <skos:inScheme rdf:resource="http://w3id.org/glosis/model/procedure/extractableElementsProcedure"/>
        <skos:notation>Extr_m1</skos:notation>
        <skos:prefLabel xml:lang="en">Extr_m1</skos:prefLabel>
        <skos:scopeNote rdf:resource="https://www.ncagr.gov/AGRONOMI/pdffiles/mehlich53.pdf"/>
        <skos:topConceptOf rdf:resource="http://w3id.org/glosis/model/procedure/extractableElementsProcedure"/>
    </owl:NamedIndividual>
    


    <!-- http://w3id.org/glosis/model/procedure/extractableElementsProcedure-Extr_m2 -->


    <owl:NamedIndividual rdf:about="http://w3id.org/glosis/model/procedure/extractableElementsProcedure-Extr_m2">
        <rdf:type rdf:resource="http://w3id.org/glosis/model/procedure/ExtractableElementsProcedure"/>
        <rdf:type rdf:resource="http://www.w3.org/2004/02/skos/core#Concept"/>
        <skos:definition>Mehlich2 method</skos:definition>
        <skos:inScheme rdf:resource="http://w3id.org/glosis/model/procedure/extractableElementsProcedure"/>
        <skos:notation>Extr_m2</skos:notation>
        <skos:prefLabel xml:lang="en">Extr_m2</skos:prefLabel>
        <skos:scopeNote rdf:resource="https://doi.org/10.1080/00103627609366673"/>
        <skos:topConceptOf rdf:resource="http://w3id.org/glosis/model/procedure/extractableElementsProcedure"/>
    </owl:NamedIndividual>
    


    <!-- http://w3id.org/glosis/model/procedure/extractableElementsProcedure-Extr_m3 -->


    <owl:NamedIndividual rdf:about="http://w3id.org/glosis/model/procedure/extractableElementsProcedure-Extr_m3">
        <rdf:type rdf:resource="http://w3id.org/glosis/model/procedure/ExtractableElementsProcedure"/>
        <rdf:type rdf:resource="http://www.w3.org/2004/02/skos/core#Concept"/>
        <skos:definition>Mehlich3 method (extractant 0.2 N CH3COOH + 0.25 N NH4NO3 + 0.015 N NH4F + 0.013 N HNO3 + 0.001 M EDTA)</skos:definition>
        <skos:inScheme rdf:resource="http://w3id.org/glosis/model/procedure/extractableElementsProcedure"/>
        <skos:notation>Extr_m3</skos:notation>
        <skos:prefLabel xml:lang="en">Extr_m3</skos:prefLabel>
        <skos:scopeNote rdf:resource="https://doi.org/10.1080/00103628409367568"/>
        <skos:topConceptOf rdf:resource="http://w3id.org/glosis/model/procedure/extractableElementsProcedure"/>
    </owl:NamedIndividual>
    


    <!-- http://w3id.org/glosis/model/procedure/extractableElementsProcedure-Extr_m3-spec -->


    <owl:NamedIndividual rdf:about="http://w3id.org/glosis/model/procedure/extractableElementsProcedure-Extr_m3-spec">
        <rdf:type rdf:resource="http://w3id.org/glosis/model/procedure/ExtractableElementsProcedure"/>
        <rdf:type rdf:resource="http://www.w3.org/2004/02/skos/core#Concept"/>
        <skos:definition>Spectrally measured and converted to Mehlich3 method (extractant 0.2 N CH3COOH + 0.25 N NH4NO3 + 0.015 N NH4F + 0.013 N HNO3 + 0.001 M EDTA)</skos:definition>
        <skos:inScheme rdf:resource="http://w3id.org/glosis/model/procedure/extractableElementsProcedure"/>
        <skos:notation>Extr_m3-spec</skos:notation>
        <skos:prefLabel xml:lang="en">Extr_m3-spec</skos:prefLabel>
        <skos:scopeNote rdf:resource="https://doi.org/10.1080/00103628409367568"/>
        <skos:topConceptOf rdf:resource="http://w3id.org/glosis/model/procedure/extractableElementsProcedure"/>
    </owl:NamedIndividual>
    


    <!-- http://w3id.org/glosis/model/procedure/extractableElementsProcedure-Extr_nahco3-olsen -->


    <owl:NamedIndividual rdf:about="http://w3id.org/glosis/model/procedure/extractableElementsProcedure-Extr_nahco3-olsen">
        <rdf:type rdf:resource="http://w3id.org/glosis/model/procedure/ExtractableElementsProcedure"/>
        <rdf:type rdf:resource="http://www.w3.org/2004/02/skos/core#Concept"/>
        <skos:definition>Method of Olsen (0.5 M Sodium Bicarbonate (NaHCO3) extraction at pH8.5). Particularly used for available P.</skos:definition>
        <skos:inScheme rdf:resource="http://w3id.org/glosis/model/procedure/extractableElementsProcedure"/>
        <skos:notation>Extr_nahco3-olsen</skos:notation>
        <skos:prefLabel xml:lang="en">Extr_nahco3-ols</skos:prefLabel>
        <skos:scopeNote rdf:resource="https://acsess.onlinelibrary.wiley.com/doi/book/10.2134/agronmonogr9.2"/>
        <skos:topConceptOf rdf:resource="http://w3id.org/glosis/model/procedure/extractableElementsProcedure"/>
    </owl:NamedIndividual>
    


    <!-- http://w3id.org/glosis/model/procedure/extractableElementsProcedure-Extr_nahco3-olsen-dabin -->


    <owl:NamedIndividual rdf:about="http://w3id.org/glosis/model/procedure/extractableElementsProcedure-Extr_nahco3-olsen-dabin">
        <rdf:type rdf:resource="http://w3id.org/glosis/model/procedure/ExtractableElementsProcedure"/>
        <rdf:type rdf:resource="http://www.w3.org/2004/02/skos/core#Concept"/>
        <skos:definition>Method of Olsen, modified by Dabin (ORSTOM). Particularly used for available P.</skos:definition>
        <skos:inScheme rdf:resource="http://w3id.org/glosis/model/procedure/extractableElementsProcedure"/>
        <skos:notation>Extr_nahco3-olsen-dabin</skos:notation>
        <skos:prefLabel xml:lang="en">Extr_nahco3-olsen-dabi</skos:prefLabel>
        <skos:scopeNote rdf:resource="https://docplayer.fr/81912854-Application-des-dosages-automatiques-a-l-analyse-des-sols-2e-partie-par.html"/>
        <skos:topConceptOf rdf:resource="http://w3id.org/glosis/model/procedure/extractableElementsProcedure"/>
    </owl:NamedIndividual>
    


    <!-- http://w3id.org/glosis/model/procedure/extractableElementsProcedure-Extr_naoac-morgan -->


    <owl:NamedIndividual rdf:about="http://w3id.org/glosis/model/procedure/extractableElementsProcedure-Extr_naoac-morgan">
        <rdf:type rdf:resource="http://w3id.org/glosis/model/procedure/ExtractableElementsProcedure"/>
        <rdf:type rdf:resource="http://www.w3.org/2004/02/skos/core#Concept"/>
        <skos:definition>Method of Morgan (Na-acetate/acetic acid). Particularly used for available P.</skos:definition>
        <skos:inScheme rdf:resource="http://w3id.org/glosis/model/procedure/extractableElementsProcedure"/>
        <skos:notation>Extr_naoac-morgan</skos:notation>
        <skos:prefLabel xml:lang="en">Extr_naoac-morga</skos:prefLabel>
        <skos:scopeNote rdf:resource="https://portal.ct.gov/-/media/CAES/DOCUMENTS/Publications/Bulletins/B450pdf.pdf?la=en"/>
        <skos:topConceptOf rdf:resource="http://w3id.org/glosis/model/procedure/extractableElementsProcedure"/>
    </owl:NamedIndividual>
    


    <!-- http://w3id.org/glosis/model/procedure/extractableElementsProcedure-Extr_nh4-co3-2-ambic1 -->


    <owl:NamedIndividual rdf:about="http://w3id.org/glosis/model/procedure/extractableElementsProcedure-Extr_nh4-co3-2-ambic1">
        <rdf:type rdf:resource="http://w3id.org/glosis/model/procedure/ExtractableElementsProcedure"/>
        <rdf:type rdf:resource="http://www.w3.org/2004/02/skos/core#Concept"/>
        <skos:definition>Ambic1 method (ammonium bicarbonate) (South Africa). Particularly used for available P.</skos:definition>
        <skos:inScheme rdf:resource="http://w3id.org/glosis/model/procedure/extractableElementsProcedure"/>
        <skos:notation>Extr_nh4-co3-2-ambic1</skos:notation>
        <skos:prefLabel xml:lang="en">Extr_nh4-co3-2-ambic1</skos:prefLabel>
        <skos:scopeNote rdf:resource="https://www.isric.org/sites/default/files/isric_report_2014_01.pdf"/>
        <skos:scopeNote>Leenaars J.G.B., A.J.M. van Oostrum and M. Ruiperez Gonzalez, 2014. Africa Soil Profiles Database, Version 1.2. A compilation of georeferenced and standardised legacy soil profile data for Sub-Saharan Africa (with dataset). ISRIC Report 2014/01. Africa Soil Information Service (AfSIS) project and ISRIC - World Soil Information, Wageningen, the Netherlands. See Annex 4.</skos:scopeNote>
        <skos:topConceptOf rdf:resource="http://w3id.org/glosis/model/procedure/extractableElementsProcedure"/>
    </owl:NamedIndividual>
    


    <!-- http://w3id.org/glosis/model/procedure/extractableElementsProcedure-Extr_nh4ch3ch-oh-cooh-leuven -->


    <owl:NamedIndividual rdf:about="http://w3id.org/glosis/model/procedure/extractableElementsProcedure-Extr_nh4ch3ch-oh-cooh-leuven">
        <rdf:type rdf:resource="http://w3id.org/glosis/model/procedure/ExtractableElementsProcedure"/>
        <rdf:type rdf:resource="http://www.w3.org/2004/02/skos/core#Concept"/>
        <skos:definition>NH4-lactate extraction method (KU-Leuven). Particularly used for available P.</skos:definition>
        <skos:inScheme rdf:resource="http://w3id.org/glosis/model/procedure/extractableElementsProcedure"/>
        <skos:notation>Extr_nh4ch3ch-oh-cooh-leuven</skos:notation>
        <skos:prefLabel xml:lang="en">Extr_nh4ch3ch-oh-cooh-leuv</skos:prefLabel>
        <skos:scopeNote rdf:resource="https://www.isric.org/sites/default/files/isric_report_2014_01.pdf"/>
        <skos:scopeNote>Leenaars J.G.B., A.J.M. van Oostrum and M. Ruiperez Gonzalez, 2014. Africa Soil Profiles Database, Version 1.2. A compilation of georeferenced and standardised legacy soil profile data for Sub-Saharan Africa (with dataset). ISRIC Report 2014/01. Africa Soil Information Service (AfSIS) project and ISRIC - World Soil Information, Wageningen, the Netherlands. See Annex 4.</skos:scopeNote>
        <skos:topConceptOf rdf:resource="http://w3id.org/glosis/model/procedure/extractableElementsProcedure"/>
    </owl:NamedIndividual>
    


    <!-- http://w3id.org/glosis/model/procedure/gypsumProcedure -->


    <owl:NamedIndividual rdf:about="http://w3id.org/glosis/model/procedure/gypsumProcedure">
        <rdf:type rdf:resource="http://www.w3.org/2004/02/skos/core#ConceptScheme"/>
        <rdfs:label xml:lang="en">Code list for gypsum analysis procedures - codelist scheme</rdfs:label>
        <rdfs:seeAlso rdf:resource="http://w3id.org/glosis/model/procedure/GypsumProcedure"/>
        <skos:definition>AfSP-derived interpretation (RwaSP)</skos:definition>
        <skos:note xml:lang="en">This code list provides analysis procedures for gypsum.</skos:note>
        <skos:prefLabel xml:lang="en">Code list for gypsum analysis procedures - codelist scheme</skos:prefLabel>
    </owl:NamedIndividual>
    


    <!-- http://w3id.org/glosis/model/procedure/gypsumProcedure-CaSO4_gy01 -->


    <owl:NamedIndividual rdf:about="http://w3id.org/glosis/model/procedure/gypsumProcedure-CaSO4_gy01">
        <rdf:type rdf:resource="http://w3id.org/glosis/model/procedure/GypsumProcedure"/>
        <rdf:type rdf:resource="http://www.w3.org/2004/02/skos/core#Concept"/>
        <skos:definition>Dissolved in water and precipitated by acetone</skos:definition>
        <skos:inScheme rdf:resource="http://w3id.org/glosis/model/procedure/gypsumProcedure"/>
        <skos:notation>CaSO4_gy01</skos:notation>
        <skos:prefLabel xml:lang="en">CaSO4_gy01</skos:prefLabel>
        <skos:scopeNote rdf:resource="https://www.isric.org/sites/default/files/isric_report_2014_01.pdf"/>
        <skos:scopeNote>Leenaars J.G.B., A.J.M. van Oostrum and M. Ruiperez Gonzalez, 2014. Africa Soil Profiles Database, Version 1.2. A compilation of georeferenced and standardised legacy soil profile data for Sub-Saharan Africa (with dataset). ISRIC Report 2014/01. Africa Soil Information Service (AfSIS) project and ISRIC - World Soil Information, Wageningen, the Netherlands. See Annex 4.</skos:scopeNote>
        <skos:topConceptOf rdf:resource="http://w3id.org/glosis/model/procedure/gypsumProcedure"/>
    </owl:NamedIndividual>
    


    <!-- http://w3id.org/glosis/model/procedure/gypsumProcedure-CaSO4_gy02 -->


    <owl:NamedIndividual rdf:about="http://w3id.org/glosis/model/procedure/gypsumProcedure-CaSO4_gy02">
        <rdf:type rdf:resource="http://w3id.org/glosis/model/procedure/GypsumProcedure"/>
        <rdf:type rdf:resource="http://www.w3.org/2004/02/skos/core#Concept"/>
        <skos:definition>Differ. between Ca-conc. in sat. extr. and Ca-conc. in 1/50 s/w solution</skos:definition>
        <skos:inScheme rdf:resource="http://w3id.org/glosis/model/procedure/gypsumProcedure"/>
        <skos:notation>CaSO4_gy02</skos:notation>
        <skos:prefLabel xml:lang="en">CaSO4_gy02</skos:prefLabel>
        <skos:scopeNote rdf:resource="https://www.isric.org/sites/default/files/isric_report_2014_01.pdf"/>
        <skos:scopeNote>Leenaars J.G.B., A.J.M. van Oostrum and M. Ruiperez Gonzalez, 2014. Africa Soil Profiles Database, Version 1.2. A compilation of georeferenced and standardised legacy soil profile data for Sub-Saharan Africa (with dataset). ISRIC Report 2014/01. Africa Soil Information Service (AfSIS) project and ISRIC - World Soil Information, Wageningen, the Netherlands. See Annex 4.</skos:scopeNote>
        <skos:topConceptOf rdf:resource="http://w3id.org/glosis/model/procedure/gypsumProcedure"/>
    </owl:NamedIndividual>
    


    <!-- http://w3id.org/glosis/model/procedure/gypsumProcedure-CaSO4_gy03 -->


    <owl:NamedIndividual rdf:about="http://w3id.org/glosis/model/procedure/gypsumProcedure-CaSO4_gy03">
        <rdf:type rdf:resource="http://w3id.org/glosis/model/procedure/GypsumProcedure"/>
        <rdf:type rdf:resource="http://www.w3.org/2004/02/skos/core#Concept"/>
        <skos:definition>Calculated from conductivity of successive dilutions</skos:definition>
        <skos:inScheme rdf:resource="http://w3id.org/glosis/model/procedure/gypsumProcedure"/>
        <skos:notation>CaSO4_gy03</skos:notation>
        <skos:prefLabel xml:lang="en">CaSO4_gy03</skos:prefLabel>
        <skos:scopeNote rdf:resource="https://www.isric.org/sites/default/files/isric_report_2014_01.pdf"/>
        <skos:scopeNote>Leenaars J.G.B., A.J.M. van Oostrum and M. Ruiperez Gonzalez, 2014. Africa Soil Profiles Database, Version 1.2. A compilation of georeferenced and standardised legacy soil profile data for Sub-Saharan Africa (with dataset). ISRIC Report 2014/01. Africa Soil Information Service (AfSIS) project and ISRIC - World Soil Information, Wageningen, the Netherlands. See Annex 4.</skos:scopeNote>
        <skos:topConceptOf rdf:resource="http://w3id.org/glosis/model/procedure/gypsumProcedure"/>
    </owl:NamedIndividual>
    


    <!-- http://w3id.org/glosis/model/procedure/gypsumProcedure-CaSO4_gy04 -->


    <owl:NamedIndividual rdf:about="http://w3id.org/glosis/model/procedure/gypsumProcedure-CaSO4_gy04">
        <rdf:type rdf:resource="http://w3id.org/glosis/model/procedure/GypsumProcedure"/>
        <rdf:type rdf:resource="http://www.w3.org/2004/02/skos/core#Concept"/>
        <skos:definition>In 0.1 M Na3-EDTA-/- turbidimetric (Begheijn, 1993)</skos:definition>
        <skos:inScheme rdf:resource="http://w3id.org/glosis/model/procedure/gypsumProcedure"/>
        <skos:notation>CaSO4_gy04</skos:notation>
        <skos:prefLabel xml:lang="en">CaSO4_gy04</skos:prefLabel>
        <skos:scopeNote rdf:resource="https://www.isric.org/sites/default/files/isric_report_2014_01.pdf"/>
        <skos:scopeNote>Leenaars J.G.B., A.J.M. van Oostrum and M. Ruiperez Gonzalez, 2014. Africa Soil Profiles Database, Version 1.2. A compilation of georeferenced and standardised legacy soil profile data for Sub-Saharan Africa (with dataset). ISRIC Report 2014/01. Africa Soil Information Service (AfSIS) project and ISRIC - World Soil Information, Wageningen, the Netherlands. See Annex 4.</skos:scopeNote>
        <skos:topConceptOf rdf:resource="http://w3id.org/glosis/model/procedure/gypsumProcedure"/>
    </owl:NamedIndividual>
    


    <!-- http://w3id.org/glosis/model/procedure/gypsumProcedure-CaSO4_gy05 -->


    <owl:NamedIndividual rdf:about="http://w3id.org/glosis/model/procedure/gypsumProcedure-CaSO4_gy05">
        <rdf:type rdf:resource="http://w3id.org/glosis/model/procedure/GypsumProcedure"/>
        <rdf:type rdf:resource="http://www.w3.org/2004/02/skos/core#Concept"/>
        <skos:definition>Gravimetric after dissolution in 0.2 N HCl (USSR-method)</skos:definition>
        <skos:inScheme rdf:resource="http://w3id.org/glosis/model/procedure/gypsumProcedure"/>
        <skos:notation>CaSO4_gy05</skos:notation>
        <skos:prefLabel xml:lang="en">CaSO4_gy05</skos:prefLabel>
        <skos:scopeNote rdf:resource="https://www.isric.org/sites/default/files/isric_report_2014_01.pdf"/>
        <skos:scopeNote>Leenaars J.G.B., A.J.M. van Oostrum and M. Ruiperez Gonzalez, 2014. Africa Soil Profiles Database, Version 1.2. A compilation of georeferenced and standardised legacy soil profile data for Sub-Saharan Africa (with dataset). ISRIC Report 2014/01. Africa Soil Information Service (AfSIS) project and ISRIC - World Soil Information, Wageningen, the Netherlands. See Annex 4.</skos:scopeNote>
        <skos:topConceptOf rdf:resource="http://w3id.org/glosis/model/procedure/gypsumProcedure"/>
    </owl:NamedIndividual>
    


    <!-- http://w3id.org/glosis/model/procedure/gypsumProcedure-CaSO4_gy06 -->


    <owl:NamedIndividual rdf:about="http://w3id.org/glosis/model/procedure/gypsumProcedure-CaSO4_gy06">
        <rdf:type rdf:resource="http://w3id.org/glosis/model/procedure/GypsumProcedure"/>
        <rdf:type rdf:resource="http://www.w3.org/2004/02/skos/core#Concept"/>
        <skos:definition>Total-S, using LECO furnace, minus easily soluble MgSO4 and Na2SO4</skos:definition>
        <skos:inScheme rdf:resource="http://w3id.org/glosis/model/procedure/gypsumProcedure"/>
        <skos:notation>CaSO4_gy06</skos:notation>
        <skos:prefLabel xml:lang="en">CaSO4_gy06</skos:prefLabel>
        <skos:scopeNote rdf:resource="https://www.isric.org/sites/default/files/isric_report_2014_01.pdf"/>
        <skos:scopeNote>Leenaars J.G.B., A.J.M. van Oostrum and M. Ruiperez Gonzalez, 2014. Africa Soil Profiles Database, Version 1.2. A compilation of georeferenced and standardised legacy soil profile data for Sub-Saharan Africa (with dataset). ISRIC Report 2014/01. Africa Soil Information Service (AfSIS) project and ISRIC - World Soil Information, Wageningen, the Netherlands. See Annex 4.</skos:scopeNote>
        <skos:topConceptOf rdf:resource="http://w3id.org/glosis/model/procedure/gypsumProcedure"/>
    </owl:NamedIndividual>
    


    <!-- http://w3id.org/glosis/model/procedure/gypsumProcedure-CaSO4_gy07 -->


    <owl:NamedIndividual rdf:about="http://w3id.org/glosis/model/procedure/gypsumProcedure-CaSO4_gy07">
        <rdf:type rdf:resource="http://w3id.org/glosis/model/procedure/GypsumProcedure"/>
        <rdf:type rdf:resource="http://www.w3.org/2004/02/skos/core#Concept"/>
        <skos:definition>Schleiff method, electrometric</skos:definition>
        <skos:inScheme rdf:resource="http://w3id.org/glosis/model/procedure/gypsumProcedure"/>
        <skos:notation>CaSO4_gy07</skos:notation>
        <skos:prefLabel xml:lang="en">CaSO4_gy07</skos:prefLabel>
        <skos:scopeNote rdf:resource="https://www.isric.org/sites/default/files/isric_report_2014_01.pdf"/>
        <skos:scopeNote>Leenaars J.G.B., A.J.M. van Oostrum and M. Ruiperez Gonzalez, 2014. Africa Soil Profiles Database, Version 1.2. A compilation of georeferenced and standardised legacy soil profile data for Sub-Saharan Africa (with dataset). ISRIC Report 2014/01. Africa Soil Information Service (AfSIS) project and ISRIC - World Soil Information, Wageningen, the Netherlands. See Annex 4.</skos:scopeNote>
        <skos:topConceptOf rdf:resource="http://w3id.org/glosis/model/procedure/gypsumProcedure"/>
    </owl:NamedIndividual>
    


    <!-- http://w3id.org/glosis/model/procedure/hydraulicConductivityProcedure -->


    <owl:NamedIndividual rdf:about="http://w3id.org/glosis/model/procedure/hydraulicConductivityProcedure">
        <rdf:type rdf:resource="http://www.w3.org/2004/02/skos/core#ConceptScheme"/>
        <rdfs:label xml:lang="en">Code list for hydraulicConductivity analysis procedures - codelist scheme</rdfs:label>
        <rdfs:seeAlso rdf:resource="http://w3id.org/glosis/model/procedure/HydraulicConductivityProcedure"/>
        <skos:definition>AfSP-derived interpretation (RwaSP)</skos:definition>
        <skos:note xml:lang="en">This code list provides analysis procedures for hydraulicConductivity.</skos:note>
        <skos:prefLabel xml:lang="en">Code list for hydraulicConductivity analysis procedures - codelist scheme</skos:prefLabel>
    </owl:NamedIndividual>
    


    <!-- http://w3id.org/glosis/model/procedure/hydraulicConductivityProcedure-KSat_calcul-ptf -->


    <owl:NamedIndividual rdf:about="http://w3id.org/glosis/model/procedure/hydraulicConductivityProcedure-KSat_calcul-ptf">
        <rdf:type rdf:resource="http://w3id.org/glosis/model/procedure/HydraulicConductivityProcedure"/>
        <rdf:type rdf:resource="http://www.w3.org/2004/02/skos/core#Concept"/>
        <skos:definition>Saturated hydraulic conductivity.</skos:definition>
        <skos:inScheme rdf:resource="http://w3id.org/glosis/model/procedure/hydraulicConductivityProcedure"/>
        <skos:notation>KSat_calcul-ptf</skos:notation>
        <skos:prefLabel xml:lang="en">KSat_calcul-ptf</skos:prefLabel>
        <skos:scopeNote rdf:resource="https://www.isric.org/sites/default/files/isric_report_2014_01.pdf"/>
        <skos:scopeNote>Leenaars J.G.B., A.J.M. van Oostrum and M. Ruiperez Gonzalez, 2014. Africa Soil Profiles Database, Version 1.2. A compilation of georeferenced and standardised legacy soil profile data for Sub-Saharan Africa (with dataset). ISRIC Report 2014/01. Africa Soil Information Service (AfSIS) project and ISRIC - World Soil Information, Wageningen, the Netherlands. See Annex 4.</skos:scopeNote>
        <skos:topConceptOf rdf:resource="http://w3id.org/glosis/model/procedure/hydraulicConductivityProcedure"/>
    </owl:NamedIndividual>
    


    <!-- http://w3id.org/glosis/model/procedure/hydraulicConductivityProcedure-KSat_calcul-ptf-genuchten -->


    <owl:NamedIndividual rdf:about="http://w3id.org/glosis/model/procedure/hydraulicConductivityProcedure-KSat_calcul-ptf-genuchten">
        <rdf:type rdf:resource="http://w3id.org/glosis/model/procedure/HydraulicConductivityProcedure"/>
        <rdf:type rdf:resource="http://www.w3.org/2004/02/skos/core#Concept"/>
        <skos:definition>Saturated and not saturated hydraulic conductivity.</skos:definition>
        <skos:inScheme rdf:resource="http://w3id.org/glosis/model/procedure/hydraulicConductivityProcedure"/>
        <skos:notation>KSat_calcul-ptf-genuchten</skos:notation>
        <skos:prefLabel xml:lang="en">KSat_calcul-ptf-genucht</skos:prefLabel>
        <skos:scopeNote rdf:resource="https://www.isric.org/sites/default/files/isric_report_2014_01.pdf"/>
        <skos:scopeNote>Leenaars J.G.B., A.J.M. van Oostrum and M. Ruiperez Gonzalez, 2014. Africa Soil Profiles Database, Version 1.2. A compilation of georeferenced and standardised legacy soil profile data for Sub-Saharan Africa (with dataset). ISRIC Report 2014/01. Africa Soil Information Service (AfSIS) project and ISRIC - World Soil Information, Wageningen, the Netherlands. See Annex 4.</skos:scopeNote>
        <skos:topConceptOf rdf:resource="http://w3id.org/glosis/model/procedure/hydraulicConductivityProcedure"/>
    </owl:NamedIndividual>
    


    <!-- http://w3id.org/glosis/model/procedure/hydraulicConductivityProcedure-KSat_calcul-ptf-saxton -->


    <owl:NamedIndividual rdf:about="http://w3id.org/glosis/model/procedure/hydraulicConductivityProcedure-KSat_calcul-ptf-saxton">
        <rdf:type rdf:resource="http://w3id.org/glosis/model/procedure/HydraulicConductivityProcedure"/>
        <rdf:type rdf:resource="http://www.w3.org/2004/02/skos/core#Concept"/>
        <skos:definition>Saturated hydraulic conductivity.</skos:definition>
        <skos:inScheme rdf:resource="http://w3id.org/glosis/model/procedure/hydraulicConductivityProcedure"/>
        <skos:notation>KSat_calcul-ptf-saxton</skos:notation>
        <skos:prefLabel xml:lang="en">KSat_calcul-ptf-saxto</skos:prefLabel>
        <skos:scopeNote rdf:resource="https://www.isric.org/sites/default/files/isric_report_2014_01.pdf"/>
        <skos:scopeNote>Leenaars J.G.B., A.J.M. van Oostrum and M. Ruiperez Gonzalez, 2014. Africa Soil Profiles Database, Version 1.2. A compilation of georeferenced and standardised legacy soil profile data for Sub-Saharan Africa (with dataset). ISRIC Report 2014/01. Africa Soil Information Service (AfSIS) project and ISRIC - World Soil Information, Wageningen, the Netherlands. See Annex 4.</skos:scopeNote>
        <skos:topConceptOf rdf:resource="http://w3id.org/glosis/model/procedure/hydraulicConductivityProcedure"/>
    </owl:NamedIndividual>
    


    <!-- http://w3id.org/glosis/model/procedure/hydraulicConductivityProcedure-Ksat_bhole -->


    <owl:NamedIndividual rdf:about="http://w3id.org/glosis/model/procedure/hydraulicConductivityProcedure-Ksat_bhole">
        <rdf:type rdf:resource="http://w3id.org/glosis/model/procedure/HydraulicConductivityProcedure"/>
        <rdf:type rdf:resource="http://www.w3.org/2004/02/skos/core#Concept"/>
        <skos:definition>Saturated hydraulic conductivity. Bore hole method</skos:definition>
        <skos:inScheme rdf:resource="http://w3id.org/glosis/model/procedure/hydraulicConductivityProcedure"/>
        <skos:notation>Ksat_bhole</skos:notation>
        <skos:prefLabel xml:lang="en">Ksat_bhol</skos:prefLabel>
        <skos:scopeNote rdf:resource="https://www.isric.org/sites/default/files/isric_report_2014_01.pdf"/>
        <skos:scopeNote>Leenaars J.G.B., A.J.M. van Oostrum and M. Ruiperez Gonzalez, 2014. Africa Soil Profiles Database, Version 1.2. A compilation of georeferenced and standardised legacy soil profile data for Sub-Saharan Africa (with dataset). ISRIC Report 2014/01. Africa Soil Information Service (AfSIS) project and ISRIC - World Soil Information, Wageningen, the Netherlands. See Annex 4.</skos:scopeNote>
        <skos:topConceptOf rdf:resource="http://w3id.org/glosis/model/procedure/hydraulicConductivityProcedure"/>
    </owl:NamedIndividual>
    


    <!-- http://w3id.org/glosis/model/procedure/hydraulicConductivityProcedure-Ksat_column -->


    <owl:NamedIndividual rdf:about="http://w3id.org/glosis/model/procedure/hydraulicConductivityProcedure-Ksat_column">
        <rdf:type rdf:resource="http://w3id.org/glosis/model/procedure/HydraulicConductivityProcedure"/>
        <rdf:type rdf:resource="http://www.w3.org/2004/02/skos/core#Concept"/>
        <skos:definition>Saturated hydraulic conductivity. Permeability in cm/hr determined in column filled with fine earth fraction</skos:definition>
        <skos:inScheme rdf:resource="http://w3id.org/glosis/model/procedure/hydraulicConductivityProcedure"/>
        <skos:notation>Ksat_column</skos:notation>
        <skos:prefLabel xml:lang="en">Ksat_colum</skos:prefLabel>
        <skos:scopeNote rdf:resource="https://www.isric.org/sites/default/files/isric_report_2014_01.pdf"/>
        <skos:scopeNote>Leenaars J.G.B., A.J.M. van Oostrum and M. Ruiperez Gonzalez, 2014. Africa Soil Profiles Database, Version 1.2. A compilation of georeferenced and standardised legacy soil profile data for Sub-Saharan Africa (with dataset). ISRIC Report 2014/01. Africa Soil Information Service (AfSIS) project and ISRIC - World Soil Information, Wageningen, the Netherlands. See Annex 4.</skos:scopeNote>
        <skos:topConceptOf rdf:resource="http://w3id.org/glosis/model/procedure/hydraulicConductivityProcedure"/>
    </owl:NamedIndividual>
    


    <!-- http://w3id.org/glosis/model/procedure/hydraulicConductivityProcedure-Ksat_dblring -->


    <owl:NamedIndividual rdf:about="http://w3id.org/glosis/model/procedure/hydraulicConductivityProcedure-Ksat_dblring">
        <rdf:type rdf:resource="http://w3id.org/glosis/model/procedure/HydraulicConductivityProcedure"/>
        <rdf:type rdf:resource="http://www.w3.org/2004/02/skos/core#Concept"/>
        <skos:definition>Saturated hydraulic conductivity. Double ring method</skos:definition>
        <skos:inScheme rdf:resource="http://w3id.org/glosis/model/procedure/hydraulicConductivityProcedure"/>
        <skos:notation>Ksat_dblring</skos:notation>
        <skos:prefLabel xml:lang="en">Ksat_dblring</skos:prefLabel>
        <skos:scopeNote rdf:resource="https://www.isric.org/sites/default/files/isric_report_2014_01.pdf"/>
        <skos:scopeNote>Leenaars J.G.B., A.J.M. van Oostrum and M. Ruiperez Gonzalez, 2014. Africa Soil Profiles Database, Version 1.2. A compilation of georeferenced and standardised legacy soil profile data for Sub-Saharan Africa (with dataset). ISRIC Report 2014/01. Africa Soil Information Service (AfSIS) project and ISRIC - World Soil Information, Wageningen, the Netherlands. See Annex 4.</skos:scopeNote>
        <skos:topConceptOf rdf:resource="http://w3id.org/glosis/model/procedure/hydraulicConductivityProcedure"/>
    </owl:NamedIndividual>
    


    <!-- http://w3id.org/glosis/model/procedure/hydraulicConductivityProcedure-Ksat_invbhole -->


    <owl:NamedIndividual rdf:about="http://w3id.org/glosis/model/procedure/hydraulicConductivityProcedure-Ksat_invbhole">
        <rdf:type rdf:resource="http://w3id.org/glosis/model/procedure/HydraulicConductivityProcedure"/>
        <rdf:type rdf:resource="http://www.w3.org/2004/02/skos/core#Concept"/>
        <skos:definition>Saturated hydraulic conductivity. Inverse bore hole method</skos:definition>
        <skos:inScheme rdf:resource="http://w3id.org/glosis/model/procedure/hydraulicConductivityProcedure"/>
        <skos:notation>Ksat_invbhole</skos:notation>
        <skos:prefLabel xml:lang="en">Ksat_invbhol</skos:prefLabel>
        <skos:scopeNote rdf:resource="https://www.isric.org/sites/default/files/isric_report_2014_01.pdf"/>
        <skos:scopeNote>Leenaars J.G.B., A.J.M. van Oostrum and M. Ruiperez Gonzalez, 2014. Africa Soil Profiles Database, Version 1.2. A compilation of georeferenced and standardised legacy soil profile data for Sub-Saharan Africa (with dataset). ISRIC Report 2014/01. Africa Soil Information Service (AfSIS) project and ISRIC - World Soil Information, Wageningen, the Netherlands. See Annex 4.</skos:scopeNote>
        <skos:topConceptOf rdf:resource="http://w3id.org/glosis/model/procedure/hydraulicConductivityProcedure"/>
    </owl:NamedIndividual>
    


    <!-- http://w3id.org/glosis/model/procedure/moistureContentProcedure -->


    <owl:NamedIndividual rdf:about="http://w3id.org/glosis/model/procedure/moistureContentProcedure">
        <rdf:type rdf:resource="http://www.w3.org/2004/02/skos/core#ConceptScheme"/>
        <rdfs:label xml:lang="en">Code list for moistureContent analysis procedures - codelist scheme</rdfs:label>
        <rdfs:seeAlso rdf:resource="http://w3id.org/glosis/model/procedure/MoistureContentProcedure"/>
        <skos:definition>AfSP-derived interpretation (RwaSP)</skos:definition>
        <skos:note xml:lang="en">This code list provides analysis procedures for moistureContent.</skos:note>
        <skos:prefLabel xml:lang="en">Code list for moistureContent analysis procedures - codelist scheme</skos:prefLabel>
    </owl:NamedIndividual>
    


    <!-- http://w3id.org/glosis/model/procedure/moistureContentProcedure-VMC_calcul-ptf -->


    <owl:NamedIndividual rdf:about="http://w3id.org/glosis/model/procedure/moistureContentProcedure-VMC_calcul-ptf">
        <rdf:type rdf:resource="http://w3id.org/glosis/model/procedure/MoistureContentProcedure"/>
        <rdf:type rdf:resource="http://www.w3.org/2004/02/skos/core#Concept"/>
        <skos:definition>Calculated by PTF</skos:definition>
        <skos:inScheme rdf:resource="http://w3id.org/glosis/model/procedure/moistureContentProcedure"/>
        <skos:notation>VMC_calcul-ptf</skos:notation>
        <skos:prefLabel xml:lang="en">VMC_calcul-ptf</skos:prefLabel>
        <skos:scopeNote rdf:resource="https://www.isric.org/sites/default/files/isric_report_2014_01.pdf"/>
        <skos:scopeNote>Leenaars J.G.B., A.J.M. van Oostrum and M. Ruiperez Gonzalez, 2014. Africa Soil Profiles Database, Version 1.2. A compilation of georeferenced and standardised legacy soil profile data for Sub-Saharan Africa (with dataset). ISRIC Report 2014/01. Africa Soil Information Service (AfSIS) project and ISRIC - World Soil Information, Wageningen, the Netherlands. See Annex 4.</skos:scopeNote>
        <skos:topConceptOf rdf:resource="http://w3id.org/glosis/model/procedure/moistureContentProcedure"/>
    </owl:NamedIndividual>
    


    <!-- http://w3id.org/glosis/model/procedure/moistureContentProcedure-VMC_calcul-ptf-brookscorey -->


    <owl:NamedIndividual rdf:about="http://w3id.org/glosis/model/procedure/moistureContentProcedure-VMC_calcul-ptf-brookscorey">
        <rdf:type rdf:resource="http://w3id.org/glosis/model/procedure/MoistureContentProcedure"/>
        <rdf:type rdf:resource="http://www.w3.org/2004/02/skos/core#Concept"/>
        <skos:definition>Calculated by PTF of brooks - corey</skos:definition>
        <skos:inScheme rdf:resource="http://w3id.org/glosis/model/procedure/moistureContentProcedure"/>
        <skos:notation>VMC_calcul-ptf-brookscorey</skos:notation>
        <skos:prefLabel xml:lang="en">VMC_calcul-ptf-brookscorey</skos:prefLabel>
        <skos:scopeNote rdf:resource="https://www.isric.org/sites/default/files/isric_report_2014_01.pdf"/>
        <skos:scopeNote>Leenaars J.G.B., A.J.M. van Oostrum and M. Ruiperez Gonzalez, 2014. Africa Soil Profiles Database, Version 1.2. A compilation of georeferenced and standardised legacy soil profile data for Sub-Saharan Africa (with dataset). ISRIC Report 2014/01. Africa Soil Information Service (AfSIS) project and ISRIC - World Soil Information, Wageningen, the Netherlands. See Annex 4.</skos:scopeNote>
        <skos:topConceptOf rdf:resource="http://w3id.org/glosis/model/procedure/moistureContentProcedure"/>
    </owl:NamedIndividual>
    


    <!-- http://w3id.org/glosis/model/procedure/moistureContentProcedure-VMC_d -->


    <owl:NamedIndividual rdf:about="http://w3id.org/glosis/model/procedure/moistureContentProcedure-VMC_d">
        <rdf:type rdf:resource="http://w3id.org/glosis/model/procedure/MoistureContentProcedure"/>
        <rdf:type rdf:resource="http://www.w3.org/2004/02/skos/core#Concept"/>
        <skos:definition>Volumetric moisture content in disturbed samples</skos:definition>
        <skos:inScheme rdf:resource="http://w3id.org/glosis/model/procedure/moistureContentProcedure"/>
        <skos:notation>VMC_d</skos:notation>
        <skos:prefLabel xml:lang="en">VMC_d</skos:prefLabel>
        <skos:scopeNote rdf:resource="https://www.isric.org/sites/default/files/isric_report_2014_01.pdf"/>
        <skos:scopeNote>Leenaars J.G.B., A.J.M. van Oostrum and M. Ruiperez Gonzalez, 2014. Africa Soil Profiles Database, Version 1.2. A compilation of georeferenced and standardised legacy soil profile data for Sub-Saharan Africa (with dataset). ISRIC Report 2014/01. Africa Soil Information Service (AfSIS) project and ISRIC - World Soil Information, Wageningen, the Netherlands. See Annex 4.</skos:scopeNote>
        <skos:topConceptOf rdf:resource="http://w3id.org/glosis/model/procedure/moistureContentProcedure"/>
    </owl:NamedIndividual>
    


    <!-- http://w3id.org/glosis/model/procedure/moistureContentProcedure-VMC_d-cl -->


    <owl:NamedIndividual rdf:about="http://w3id.org/glosis/model/procedure/moistureContentProcedure-VMC_d-cl">
        <rdf:type rdf:resource="http://w3id.org/glosis/model/procedure/MoistureContentProcedure"/>
        <rdf:type rdf:resource="http://www.w3.org/2004/02/skos/core#Concept"/>
        <skos:definition>Pressure-plate extraction, disturbed -clod- samples (wt%) * density</skos:definition>
        <skos:inScheme rdf:resource="http://w3id.org/glosis/model/procedure/moistureContentProcedure"/>
        <skos:notation>VMC_d-cl</skos:notation>
        <skos:prefLabel xml:lang="en">VMC_d-cl</skos:prefLabel>
        <skos:scopeNote rdf:resource="https://www.isric.org/sites/default/files/isric_report_2014_01.pdf"/>
        <skos:scopeNote>Leenaars J.G.B., A.J.M. van Oostrum and M. Ruiperez Gonzalez, 2014. Africa Soil Profiles Database, Version 1.2. A compilation of georeferenced and standardised legacy soil profile data for Sub-Saharan Africa (with dataset). ISRIC Report 2014/01. Africa Soil Information Service (AfSIS) project and ISRIC - World Soil Information, Wageningen, the Netherlands. See Annex 4.</skos:scopeNote>
        <skos:topConceptOf rdf:resource="http://w3id.org/glosis/model/procedure/moistureContentProcedure"/>
    </owl:NamedIndividual>
    


    <!-- http://w3id.org/glosis/model/procedure/moistureContentProcedure-VMC_d-cl-ww -->


    <owl:NamedIndividual rdf:about="http://w3id.org/glosis/model/procedure/moistureContentProcedure-VMC_d-cl-ww">
        <rdf:type rdf:resource="http://w3id.org/glosis/model/procedure/MoistureContentProcedure"/>
        <rdf:type rdf:resource="http://www.w3.org/2004/02/skos/core#Concept"/>
        <skos:definition>Pressure-plate extraction, disturbed -clod- samples (wt%) * density on weight/weight basis; to be converted to v/v (with BD at appropriate humidity)</skos:definition>
        <skos:inScheme rdf:resource="http://w3id.org/glosis/model/procedure/moistureContentProcedure"/>
        <skos:notation>VMC_d-cl-ww</skos:notation>
        <skos:prefLabel xml:lang="en">VMC_d-cl-ww</skos:prefLabel>
        <skos:scopeNote rdf:resource="https://www.isric.org/sites/default/files/isric_report_2014_01.pdf"/>
        <skos:scopeNote>Leenaars J.G.B., A.J.M. van Oostrum and M. Ruiperez Gonzalez, 2014. Africa Soil Profiles Database, Version 1.2. A compilation of georeferenced and standardised legacy soil profile data for Sub-Saharan Africa (with dataset). ISRIC Report 2014/01. Africa Soil Information Service (AfSIS) project and ISRIC - World Soil Information, Wageningen, the Netherlands. See Annex 4.</skos:scopeNote>
        <skos:topConceptOf rdf:resource="http://w3id.org/glosis/model/procedure/moistureContentProcedure"/>
    </owl:NamedIndividual>
    


    <!-- http://w3id.org/glosis/model/procedure/moistureContentProcedure-VMC_d-ww -->


    <owl:NamedIndividual rdf:about="http://w3id.org/glosis/model/procedure/moistureContentProcedure-VMC_d-ww">
        <rdf:type rdf:resource="http://w3id.org/glosis/model/procedure/MoistureContentProcedure"/>
        <rdf:type rdf:resource="http://www.w3.org/2004/02/skos/core#Concept"/>
        <skos:definition>Volumetric moisture content in disturbed samples on weight/weight basis to be converted to v/v (with BD at appropriate humidity)</skos:definition>
        <skos:inScheme rdf:resource="http://w3id.org/glosis/model/procedure/moistureContentProcedure"/>
        <skos:notation>VMC_d-ww</skos:notation>
        <skos:prefLabel xml:lang="en">VMC_d-ww</skos:prefLabel>
        <skos:scopeNote rdf:resource="https://www.isric.org/sites/default/files/isric_report_2014_01.pdf"/>
        <skos:scopeNote>Leenaars J.G.B., A.J.M. van Oostrum and M. Ruiperez Gonzalez, 2014. Africa Soil Profiles Database, Version 1.2. A compilation of georeferenced and standardised legacy soil profile data for Sub-Saharan Africa (with dataset). ISRIC Report 2014/01. Africa Soil Information Service (AfSIS) project and ISRIC - World Soil Information, Wageningen, the Netherlands. See Annex 4.</skos:scopeNote>
        <skos:topConceptOf rdf:resource="http://w3id.org/glosis/model/procedure/moistureContentProcedure"/>
    </owl:NamedIndividual>
    


    <!-- http://w3id.org/glosis/model/procedure/moistureContentProcedure-VMC_ud -->


    <owl:NamedIndividual rdf:about="http://w3id.org/glosis/model/procedure/moistureContentProcedure-VMC_ud">
        <rdf:type rdf:resource="http://w3id.org/glosis/model/procedure/MoistureContentProcedure"/>
        <rdf:type rdf:resource="http://www.w3.org/2004/02/skos/core#Concept"/>
        <skos:definition>Undisturbed samples</skos:definition>
        <skos:inScheme rdf:resource="http://w3id.org/glosis/model/procedure/moistureContentProcedure"/>
        <skos:notation>VMC_ud</skos:notation>
        <skos:prefLabel xml:lang="en">VMC_ud</skos:prefLabel>
        <skos:scopeNote rdf:resource="https://www.isric.org/sites/default/files/isric_report_2014_01.pdf"/>
        <skos:scopeNote>Leenaars J.G.B., A.J.M. van Oostrum and M. Ruiperez Gonzalez, 2014. Africa Soil Profiles Database, Version 1.2. A compilation of georeferenced and standardised legacy soil profile data for Sub-Saharan Africa (with dataset). ISRIC Report 2014/01. Africa Soil Information Service (AfSIS) project and ISRIC - World Soil Information, Wageningen, the Netherlands. See Annex 4.</skos:scopeNote>
        <skos:topConceptOf rdf:resource="http://w3id.org/glosis/model/procedure/moistureContentProcedure"/>
    </owl:NamedIndividual>
    


    <!-- http://w3id.org/glosis/model/procedure/moistureContentProcedure-VMC_ud-cl -->


    <owl:NamedIndividual rdf:about="http://w3id.org/glosis/model/procedure/moistureContentProcedure-VMC_ud-cl">
        <rdf:type rdf:resource="http://w3id.org/glosis/model/procedure/MoistureContentProcedure"/>
        <rdf:type rdf:resource="http://www.w3.org/2004/02/skos/core#Concept"/>
        <skos:definition>Natural clod</skos:definition>
        <skos:inScheme rdf:resource="http://w3id.org/glosis/model/procedure/moistureContentProcedure"/>
        <skos:notation>VMC_ud-cl</skos:notation>
        <skos:prefLabel xml:lang="en">VMC_ud-cl</skos:prefLabel>
        <skos:scopeNote rdf:resource="https://www.isric.org/sites/default/files/isric_report_2014_01.pdf"/>
        <skos:scopeNote>Leenaars J.G.B., A.J.M. van Oostrum and M. Ruiperez Gonzalez, 2014. Africa Soil Profiles Database, Version 1.2. A compilation of georeferenced and standardised legacy soil profile data for Sub-Saharan Africa (with dataset). ISRIC Report 2014/01. Africa Soil Information Service (AfSIS) project and ISRIC - World Soil Information, Wageningen, the Netherlands. See Annex 4.</skos:scopeNote>
        <skos:topConceptOf rdf:resource="http://w3id.org/glosis/model/procedure/moistureContentProcedure"/>
    </owl:NamedIndividual>
    


    <!-- http://w3id.org/glosis/model/procedure/moistureContentProcedure-VMC_ud-co -->


    <owl:NamedIndividual rdf:about="http://w3id.org/glosis/model/procedure/moistureContentProcedure-VMC_ud-co">
        <rdf:type rdf:resource="http://w3id.org/glosis/model/procedure/MoistureContentProcedure"/>
        <rdf:type rdf:resource="http://www.w3.org/2004/02/skos/core#Concept"/>
        <skos:definition>Volumetric moisture content in undisturbed samples (pF rings cores)</skos:definition>
        <skos:inScheme rdf:resource="http://w3id.org/glosis/model/procedure/moistureContentProcedure"/>
        <skos:notation>VMC_ud-co</skos:notation>
        <skos:prefLabel xml:lang="en">VMC_ud-co</skos:prefLabel>
        <skos:scopeNote rdf:resource="https://www.isric.org/sites/default/files/isric_report_2014_01.pdf"/>
        <skos:scopeNote>Leenaars J.G.B., A.J.M. van Oostrum and M. Ruiperez Gonzalez, 2014. Africa Soil Profiles Database, Version 1.2. A compilation of georeferenced and standardised legacy soil profile data for Sub-Saharan Africa (with dataset). ISRIC Report 2014/01. Africa Soil Information Service (AfSIS) project and ISRIC - World Soil Information, Wageningen, the Netherlands. See Annex 4.</skos:scopeNote>
        <skos:topConceptOf rdf:resource="http://w3id.org/glosis/model/procedure/moistureContentProcedure"/>
    </owl:NamedIndividual>
    


    <!-- http://w3id.org/glosis/model/procedure/nitrogenTotalProcedure -->


    <owl:NamedIndividual rdf:about="http://w3id.org/glosis/model/procedure/nitrogenTotalProcedure">
        <rdf:type rdf:resource="http://www.w3.org/2004/02/skos/core#ConceptScheme"/>
        <rdfs:label xml:lang="en">Code list for nitrogenTotal analysis procedures - codelist scheme</rdfs:label>
        <rdfs:seeAlso rdf:resource="http://w3id.org/glosis/model/procedure/NitrogenTotalProcedure"/>
        <skos:definition>AfSP-derived interpretation (RwaSP)</skos:definition>
        <skos:note xml:lang="en">This code list provides analysis procedures for nitrogenTotal.</skos:note>
        <skos:prefLabel xml:lang="en">Code list for nitrogenTotal analysis procedures - codelist scheme</skos:prefLabel>
    </owl:NamedIndividual>
    


    <!-- http://w3id.org/glosis/model/procedure/nitrogenTotalProcedure-TotalN_bremner -->


    <owl:NamedIndividual rdf:about="http://w3id.org/glosis/model/procedure/nitrogenTotalProcedure-TotalN_bremner">
        <rdf:type rdf:resource="http://w3id.org/glosis/model/procedure/NitrogenTotalProcedure"/>
        <rdf:type rdf:resource="http://www.w3.org/2004/02/skos/core#Concept"/>
        <skos:definition>Total N (Bremner, 1965, p. 1162-1164)</skos:definition>
        <skos:inScheme rdf:resource="http://w3id.org/glosis/model/procedure/nitrogenTotalProcedure"/>
        <skos:notation>TotalN_bremner</skos:notation>
        <skos:prefLabel xml:lang="en">TotalN_bremner</skos:prefLabel>
        <skos:scopeNote rdf:resource="https://doi.org/10.2134/agronmonogr9.2.c32"/>
        <skos:scopeNote>Bremner, J. M. 1965. Total Nitrogen. In: C. A. Black (ed.) Methods of soil analysis. Part 2: Chemical and microbial properties. Number 9 in series Agronomy. American Society of Agronomy, Inc. Publisher, Madison, USA. Pp. 1049-1178</skos:scopeNote>
        <skos:topConceptOf rdf:resource="http://w3id.org/glosis/model/procedure/nitrogenTotalProcedure"/>
    </owl:NamedIndividual>
    


    <!-- http://w3id.org/glosis/model/procedure/nitrogenTotalProcedure-TotalN_calcul -->


    <owl:NamedIndividual rdf:about="http://w3id.org/glosis/model/procedure/nitrogenTotalProcedure-TotalN_calcul">
        <rdf:type rdf:resource="http://w3id.org/glosis/model/procedure/NitrogenTotalProcedure"/>
        <rdf:type rdf:resource="http://www.w3.org/2004/02/skos/core#Concept"/>
        <skos:definition>OC * 1.72 / 20 (gives C/N=11.6009)</skos:definition>
        <skos:inScheme rdf:resource="http://w3id.org/glosis/model/procedure/nitrogenTotalProcedure"/>
        <skos:notation>TotalN_calcul</skos:notation>
        <skos:prefLabel xml:lang="en">TotalN_calcul</skos:prefLabel>
        <skos:scopeNote rdf:resource="https://www.isric.org/sites/default/files/isric_report_2014_01.pdf"/>
        <skos:scopeNote>Leenaars J.G.B., A.J.M. van Oostrum and M. Ruiperez Gonzalez, 2014. Africa Soil Profiles Database, Version 1.2. A compilation of georeferenced and standardised legacy soil profile data for Sub-Saharan Africa (with dataset). ISRIC Report 2014/01. Africa Soil Information Service (AfSIS) project and ISRIC - World Soil Information, Wageningen, the Netherlands. See Annex 4.</skos:scopeNote>
        <skos:topConceptOf rdf:resource="http://w3id.org/glosis/model/procedure/nitrogenTotalProcedure"/>
    </owl:NamedIndividual>
    


    <!-- http://w3id.org/glosis/model/procedure/nitrogenTotalProcedure-TotalN_calcul-oc10 -->


    <owl:NamedIndividual rdf:about="http://w3id.org/glosis/model/procedure/nitrogenTotalProcedure-TotalN_calcul-oc10">
        <rdf:type rdf:resource="http://w3id.org/glosis/model/procedure/NitrogenTotalProcedure"/>
        <rdf:type rdf:resource="http://www.w3.org/2004/02/skos/core#Concept"/>
        <skos:definition>Calculated from OrgC and C/N ratio of 10</skos:definition>
        <skos:inScheme rdf:resource="http://w3id.org/glosis/model/procedure/nitrogenTotalProcedure"/>
        <skos:notation>TotalN_calcul-oc10</skos:notation>
        <skos:prefLabel xml:lang="en">TotalN_calcul-oc10</skos:prefLabel>
        <skos:scopeNote rdf:resource="https://www.isric.org/sites/default/files/isric_report_2014_01.pdf"/>
        <skos:scopeNote>Leenaars J.G.B., A.J.M. van Oostrum and M. Ruiperez Gonzalez, 2014. Africa Soil Profiles Database, Version 1.2. A compilation of georeferenced and standardised legacy soil profile data for Sub-Saharan Africa (with dataset). ISRIC Report 2014/01. Africa Soil Information Service (AfSIS) project and ISRIC - World Soil Information, Wageningen, the Netherlands. See Annex 4.</skos:scopeNote>
        <skos:topConceptOf rdf:resource="http://w3id.org/glosis/model/procedure/nitrogenTotalProcedure"/>
    </owl:NamedIndividual>
    


    <!-- http://w3id.org/glosis/model/procedure/nitrogenTotalProcedure-TotalN_dc -->


    <owl:NamedIndividual rdf:about="http://w3id.org/glosis/model/procedure/nitrogenTotalProcedure-TotalN_dc">
        <rdf:type rdf:resource="http://w3id.org/glosis/model/procedure/NitrogenTotalProcedure"/>
        <rdf:type rdf:resource="http://www.w3.org/2004/02/skos/core#Concept"/>
        <skos:definition>Dry combustion</skos:definition>
        <skos:inScheme rdf:resource="http://w3id.org/glosis/model/procedure/nitrogenTotalProcedure"/>
        <skos:narrower rdf:resource="http://w3id.org/glosis/model/procedure/nitrogenTotalProcedure-TotalN_dc-ht-dumas"/>
        <skos:narrower rdf:resource="http://w3id.org/glosis/model/procedure/nitrogenTotalProcedure-TotalN_dc-ht-leco"/>
        <skos:narrower rdf:resource="http://w3id.org/glosis/model/procedure/nitrogenTotalProcedure-TotalN_dc-spec"/>
        <skos:notation>TotalN_dc</skos:notation>
        <skos:prefLabel xml:lang="en">TotalN_dc</skos:prefLabel>
        <skos:scopeNote rdf:resource="https://www.isric.org/sites/default/files/isric_report_2014_01.pdf"/>
        <skos:scopeNote>Leenaars J.G.B., A.J.M. van Oostrum and M. Ruiperez Gonzalez, 2014. Africa Soil Profiles Database, Version 1.2. A compilation of georeferenced and standardised legacy soil profile data for Sub-Saharan Africa (with dataset). ISRIC Report 2014/01. Africa Soil Information Service (AfSIS) project and ISRIC - World Soil Information, Wageningen, the Netherlands. See Annex 4.</skos:scopeNote>
        <skos:topConceptOf rdf:resource="http://w3id.org/glosis/model/procedure/nitrogenTotalProcedure"/>
    </owl:NamedIndividual>
    


    <!-- http://w3id.org/glosis/model/procedure/nitrogenTotalProcedure-TotalN_dc-ht-dumas -->


    <owl:NamedIndividual rdf:about="http://w3id.org/glosis/model/procedure/nitrogenTotalProcedure-TotalN_dc-ht-dumas">
        <rdf:type rdf:resource="http://w3id.org/glosis/model/procedure/NitrogenTotalProcedure"/>
        <rdf:type rdf:resource="http://www.w3.org/2004/02/skos/core#Concept"/>
        <skos:broader rdf:resource="http://w3id.org/glosis/model/procedure/nitrogenTotalProcedure-TotalN_dc"/>
        <skos:definition>Dry combustion at 800-1000 C celcius (Dumas method)</skos:definition>
        <skos:inScheme rdf:resource="http://w3id.org/glosis/model/procedure/nitrogenTotalProcedure"/>
        <skos:notation>TotalN_dc-ht-dumas</skos:notation>
        <skos:prefLabel xml:lang="en">TotalN_dc-ht-dumas</skos:prefLabel>
        <skos:scopeNote rdf:resource="https://www.isric.org/sites/default/files/isric_report_2014_01.pdf"/>
        <skos:scopeNote>Leenaars J.G.B., A.J.M. van Oostrum and M. Ruiperez Gonzalez, 2014. Africa Soil Profiles Database, Version 1.2. A compilation of georeferenced and standardised legacy soil profile data for Sub-Saharan Africa (with dataset). ISRIC Report 2014/01. Africa Soil Information Service (AfSIS) project and ISRIC - World Soil Information, Wageningen, the Netherlands. See Annex 4.</skos:scopeNote>
    </owl:NamedIndividual>
    


    <!-- http://w3id.org/glosis/model/procedure/nitrogenTotalProcedure-TotalN_dc-ht-leco -->


    <owl:NamedIndividual rdf:about="http://w3id.org/glosis/model/procedure/nitrogenTotalProcedure-TotalN_dc-ht-leco">
        <rdf:type rdf:resource="http://w3id.org/glosis/model/procedure/NitrogenTotalProcedure"/>
        <rdf:type rdf:resource="http://www.w3.org/2004/02/skos/core#Concept"/>
        <skos:broader rdf:resource="http://w3id.org/glosis/model/procedure/nitrogenTotalProcedure-TotalN_dc"/>
        <skos:definition>Element analyzer (LECO analyzer), Dry Combustion</skos:definition>
        <skos:inScheme rdf:resource="http://w3id.org/glosis/model/procedure/nitrogenTotalProcedure"/>
        <skos:notation>TotalN_dc-ht-leco</skos:notation>
        <skos:prefLabel xml:lang="en">TotalN_dc-ht-leco</skos:prefLabel>
        <skos:scopeNote rdf:resource="https://www.isric.org/sites/default/files/isric_report_2014_01.pdf"/>
        <skos:scopeNote>Leenaars J.G.B., A.J.M. van Oostrum and M. Ruiperez Gonzalez, 2014. Africa Soil Profiles Database, Version 1.2. A compilation of georeferenced and standardised legacy soil profile data for Sub-Saharan Africa (with dataset). ISRIC Report 2014/01. Africa Soil Information Service (AfSIS) project and ISRIC - World Soil Information, Wageningen, the Netherlands. See Annex 4.</skos:scopeNote>
    </owl:NamedIndividual>
    


    <!-- http://w3id.org/glosis/model/procedure/nitrogenTotalProcedure-TotalN_dc-spec -->


    <owl:NamedIndividual rdf:about="http://w3id.org/glosis/model/procedure/nitrogenTotalProcedure-TotalN_dc-spec">
        <rdf:type rdf:resource="http://w3id.org/glosis/model/procedure/NitrogenTotalProcedure"/>
        <rdf:type rdf:resource="http://www.w3.org/2004/02/skos/core#Concept"/>
        <skos:broader rdf:resource="http://w3id.org/glosis/model/procedure/nitrogenTotalProcedure-TotalN_dc"/>
        <skos:definition>Spectrally measured and converted to N by dry combustion</skos:definition>
        <skos:inScheme rdf:resource="http://w3id.org/glosis/model/procedure/nitrogenTotalProcedure"/>
        <skos:notation>TotalN_dc-spec</skos:notation>
        <skos:prefLabel xml:lang="en">TotalN_dc-spec</skos:prefLabel>
        <skos:scopeNote rdf:resource="https://www.isric.org/sites/default/files/isric_report_2014_01.pdf"/>
        <skos:scopeNote>Leenaars J.G.B., A.J.M. van Oostrum and M. Ruiperez Gonzalez, 2014. Africa Soil Profiles Database, Version 1.2. A compilation of georeferenced and standardised legacy soil profile data for Sub-Saharan Africa (with dataset). ISRIC Report 2014/01. Africa Soil Information Service (AfSIS) project and ISRIC - World Soil Information, Wageningen, the Netherlands. See Annex 4.</skos:scopeNote>
    </owl:NamedIndividual>
    


    <!-- http://w3id.org/glosis/model/procedure/nitrogenTotalProcedure-TotalN_h2so4 -->


    <owl:NamedIndividual rdf:about="http://w3id.org/glosis/model/procedure/nitrogenTotalProcedure-TotalN_h2so4">
        <rdf:type rdf:resource="http://w3id.org/glosis/model/procedure/NitrogenTotalProcedure"/>
        <rdf:type rdf:resource="http://www.w3.org/2004/02/skos/core#Concept"/>
        <skos:definition>H2SO4</skos:definition>
        <skos:inScheme rdf:resource="http://w3id.org/glosis/model/procedure/nitrogenTotalProcedure"/>
        <skos:notation>TotalN_h2so4</skos:notation>
        <skos:prefLabel xml:lang="en">TotalN_h2so4</skos:prefLabel>
        <skos:topConceptOf rdf:resource="http://w3id.org/glosis/model/procedure/nitrogenTotalProcedure"/>
    </owl:NamedIndividual>
    


    <!-- http://w3id.org/glosis/model/procedure/nitrogenTotalProcedure-TotalN_kjeldahl -->


    <owl:NamedIndividual rdf:about="http://w3id.org/glosis/model/procedure/nitrogenTotalProcedure-TotalN_kjeldahl">
        <rdf:type rdf:resource="http://w3id.org/glosis/model/procedure/NitrogenTotalProcedure"/>
        <rdf:type rdf:resource="http://www.w3.org/2004/02/skos/core#Concept"/>
        <skos:definition>Method of Kjeldahl (digestion)</skos:definition>
        <skos:inScheme rdf:resource="http://w3id.org/glosis/model/procedure/nitrogenTotalProcedure"/>
        <skos:notation>TotalN_kjeldahl</skos:notation>
        <skos:prefLabel xml:lang="en">TotalN_kjeldahl</skos:prefLabel>
        <skos:scopeNote rdf:resource="https://en.wikipedia.org/wiki/Kjeldahl_method"/>
        <skos:scopeNote>Kjeldahl, J. (1883) ‘Neue Methode zur Bestimmung des Stickstoffs in organischen Körpern’ (New method for the determination of nitrogen in organic substances), Zeitschrift für analytische Chemie, 22 (1) : 366-383.</skos:scopeNote>
        <skos:topConceptOf rdf:resource="http://w3id.org/glosis/model/procedure/nitrogenTotalProcedure"/>
    </owl:NamedIndividual>
    


    <!-- http://w3id.org/glosis/model/procedure/nitrogenTotalProcedure-TotalN_kjeldahl-nh4 -->


    <owl:NamedIndividual rdf:about="http://w3id.org/glosis/model/procedure/nitrogenTotalProcedure-TotalN_kjeldahl-nh4">
        <rdf:type rdf:resource="http://w3id.org/glosis/model/procedure/NitrogenTotalProcedure"/>
        <rdf:type rdf:resource="http://www.w3.org/2004/02/skos/core#Concept"/>
        <skos:definition>Kjeldahl, and ammonia distillation</skos:definition>
        <skos:inScheme rdf:resource="http://w3id.org/glosis/model/procedure/nitrogenTotalProcedure"/>
        <skos:notation>TotalN_kjeldahl-nh4</skos:notation>
        <skos:prefLabel xml:lang="en">TotalN_kjeldahl-nh4</skos:prefLabel>
        <skos:scopeNote rdf:resource="https://www.isric.org/sites/default/files/isric_report_2014_01.pdf"/>
        <skos:scopeNote>Leenaars J.G.B., A.J.M. van Oostrum and M. Ruiperez Gonzalez, 2014. Africa Soil Profiles Database, Version 1.2. A compilation of georeferenced and standardised legacy soil profile data for Sub-Saharan Africa (with dataset). ISRIC Report 2014/01. Africa Soil Information Service (AfSIS) project and ISRIC - World Soil Information, Wageningen, the Netherlands. See Annex 4.</skos:scopeNote>
        <skos:topConceptOf rdf:resource="http://w3id.org/glosis/model/procedure/nitrogenTotalProcedure"/>
    </owl:NamedIndividual>
    


    <!-- http://w3id.org/glosis/model/procedure/nitrogenTotalProcedure-TotalN_nelson -->


    <owl:NamedIndividual rdf:about="http://w3id.org/glosis/model/procedure/nitrogenTotalProcedure-TotalN_nelson">
        <rdf:type rdf:resource="http://w3id.org/glosis/model/procedure/NitrogenTotalProcedure"/>
        <rdf:type rdf:resource="http://www.w3.org/2004/02/skos/core#Concept"/>
        <skos:definition>Nelson and Sommers, 1980</skos:definition>
        <skos:inScheme rdf:resource="http://w3id.org/glosis/model/procedure/nitrogenTotalProcedure"/>
        <skos:notation>TotalN_nelson</skos:notation>
        <skos:prefLabel xml:lang="en">TotalN_nelso</skos:prefLabel>
        <skos:scopeNote rdf:resource="https://doi.org/10.1093/jaoac/63.4.770"/>
        <skos:scopeNote>Darrell W Nelson, Lee E Sommers, Total Nitrogen Analysis of Soil and Plant Tissues, Journal of Association of Official Analytical Chemists, Volume 63, Issue 4, 1 July 1980, Pages 770–778,</skos:scopeNote>
        <skos:topConceptOf rdf:resource="http://w3id.org/glosis/model/procedure/nitrogenTotalProcedure"/>
    </owl:NamedIndividual>
    


    <!-- http://w3id.org/glosis/model/procedure/nitrogenTotalProcedure-TotalN_tn04 -->


    <owl:NamedIndividual rdf:about="http://w3id.org/glosis/model/procedure/nitrogenTotalProcedure-TotalN_tn04">
        <rdf:type rdf:resource="http://w3id.org/glosis/model/procedure/NitrogenTotalProcedure"/>
        <rdf:type rdf:resource="http://www.w3.org/2004/02/skos/core#Concept"/>
        <skos:definition>Dry combustion using a CN-corder and cobalt oxide or copper oxide as an oxidation accelerator (Tanabe and Araragi, 1970)</skos:definition>
        <skos:inScheme rdf:resource="http://w3id.org/glosis/model/procedure/nitrogenTotalProcedure"/>
        <skos:notation>TotalN_tn04</skos:notation>
        <skos:prefLabel xml:lang="en">TotalN_tn04</skos:prefLabel>
        <skos:scopeNote rdf:resource="https://www.isric.org/sites/default/files/isric_report_2014_01.pdf"/>
        <skos:scopeNote>Leenaars J.G.B., A.J.M. van Oostrum and M. Ruiperez Gonzalez, 2014. Africa Soil Profiles Database, Version 1.2. A compilation of georeferenced and standardised legacy soil profile data for Sub-Saharan Africa (with dataset). ISRIC Report 2014/01. Africa Soil Information Service (AfSIS) project and ISRIC - World Soil Information, Wageningen, the Netherlands. See Annex 4.</skos:scopeNote>
        <skos:topConceptOf rdf:resource="http://w3id.org/glosis/model/procedure/nitrogenTotalProcedure"/>
    </owl:NamedIndividual>
    


    <!-- http://w3id.org/glosis/model/procedure/nitrogenTotalProcedure-TotalN_tn06 -->


    <owl:NamedIndividual rdf:about="http://w3id.org/glosis/model/procedure/nitrogenTotalProcedure-TotalN_tn06">
        <rdf:type rdf:resource="http://w3id.org/glosis/model/procedure/NitrogenTotalProcedure"/>
        <rdf:type rdf:resource="http://www.w3.org/2004/02/skos/core#Concept"/>
        <skos:definition>Continuous flow analyser after digestion with H2SO4/salicyclic acid/H2O2/Se</skos:definition>
        <skos:inScheme rdf:resource="http://w3id.org/glosis/model/procedure/nitrogenTotalProcedure"/>
        <skos:notation>TotalN_tn06</skos:notation>
        <skos:prefLabel xml:lang="en">TotalN_tn06</skos:prefLabel>
        <skos:scopeNote rdf:resource="https://www.isric.org/sites/default/files/isric_report_2014_01.pdf"/>
        <skos:scopeNote>Leenaars J.G.B., A.J.M. van Oostrum and M. Ruiperez Gonzalez, 2014. Africa Soil Profiles Database, Version 1.2. A compilation of georeferenced and standardised legacy soil profile data for Sub-Saharan Africa (with dataset). ISRIC Report 2014/01. Africa Soil Information Service (AfSIS) project and ISRIC - World Soil Information, Wageningen, the Netherlands. See Annex 4.</skos:scopeNote>
        <skos:topConceptOf rdf:resource="http://w3id.org/glosis/model/procedure/nitrogenTotalProcedure"/>
    </owl:NamedIndividual>
    


    <!-- http://w3id.org/glosis/model/procedure/nitrogenTotalProcedure-TotalN_tn08 -->


    <owl:NamedIndividual rdf:about="http://w3id.org/glosis/model/procedure/nitrogenTotalProcedure-TotalN_tn08">
        <rdf:type rdf:resource="http://w3id.org/glosis/model/procedure/NitrogenTotalProcedure"/>
        <rdf:type rdf:resource="http://www.w3.org/2004/02/skos/core#Concept"/>
        <skos:definition>Sample digested by sulphuric acid, distillation of released ammonia, back titration against sulpuric acid</skos:definition>
        <skos:inScheme rdf:resource="http://w3id.org/glosis/model/procedure/nitrogenTotalProcedure"/>
        <skos:notation>TotalN_tn08</skos:notation>
        <skos:prefLabel xml:lang="en">TotalN_tn08</skos:prefLabel>
        <skos:scopeNote rdf:resource="https://www.isric.org/sites/default/files/isric_report_2014_01.pdf"/>
        <skos:scopeNote>Leenaars J.G.B., A.J.M. van Oostrum and M. Ruiperez Gonzalez, 2014. Africa Soil Profiles Database, Version 1.2. A compilation of georeferenced and standardised legacy soil profile data for Sub-Saharan Africa (with dataset). ISRIC Report 2014/01. Africa Soil Information Service (AfSIS) project and ISRIC - World Soil Information, Wageningen, the Netherlands. See Annex 4.</skos:scopeNote>
        <skos:topConceptOf rdf:resource="http://w3id.org/glosis/model/procedure/nitrogenTotalProcedure"/>
    </owl:NamedIndividual>
    


    <!-- http://w3id.org/glosis/model/procedure/organicMatterProcedure -->


    <owl:NamedIndividual rdf:about="http://w3id.org/glosis/model/procedure/organicMatterProcedure">
        <rdf:type rdf:resource="http://www.w3.org/2004/02/skos/core#ConceptScheme"/>
        <rdfs:label xml:lang="en">Code list for organicMatter analysis procedures - codelist scheme</rdfs:label>
        <rdfs:seeAlso rdf:resource="http://w3id.org/glosis/model/procedure/OrganicMatterProcedure"/>
        <skos:definition>AfSP-derived interpretation (RwaSP)</skos:definition>
        <skos:note xml:lang="en">This code list provides analysis procedures for organicMatter.</skos:note>
        <skos:prefLabel xml:lang="en">Code list for organicMatter analysis procedures - codelist scheme</skos:prefLabel>
    </owl:NamedIndividual>
    


    <!-- http://w3id.org/glosis/model/procedure/organicMatterProcedure-FulAcidC_unkn -->


    <owl:NamedIndividual rdf:about="http://w3id.org/glosis/model/procedure/organicMatterProcedure-FulAcidC_unkn">
        <rdf:type rdf:resource="http://w3id.org/glosis/model/procedure/OrganicMatterProcedure"/>
        <rdf:type rdf:resource="http://www.w3.org/2004/02/skos/core#Concept"/>
        <skos:definition>Fulvic acid carbon_unknown method</skos:definition>
        <skos:inScheme rdf:resource="http://w3id.org/glosis/model/procedure/organicMatterProcedure"/>
        <skos:notation>FulAcidC_unkn</skos:notation>
        <skos:prefLabel xml:lang="en">FulAcidC_unk</skos:prefLabel>
        <skos:scopeNote rdf:resource="https://www.isric.org/sites/default/files/isric_report_2014_01.pdf"/>
        <skos:scopeNote>Leenaars J.G.B., A.J.M. van Oostrum and M. Ruiperez Gonzalez, 2014. Africa Soil Profiles Database, Version 1.2. A compilation of georeferenced and standardised legacy soil profile data for Sub-Saharan Africa (with dataset). ISRIC Report 2014/01. Africa Soil Information Service (AfSIS) project and ISRIC - World Soil Information, Wageningen, the Netherlands. See Annex 4.</skos:scopeNote>
        <skos:topConceptOf rdf:resource="http://w3id.org/glosis/model/procedure/organicMatterProcedure"/>
    </owl:NamedIndividual>
    


    <!-- http://w3id.org/glosis/model/procedure/organicMatterProcedure-HumAcidC_unkn -->


    <owl:NamedIndividual rdf:about="http://w3id.org/glosis/model/procedure/organicMatterProcedure-HumAcidC_unkn">
        <rdf:type rdf:resource="http://w3id.org/glosis/model/procedure/OrganicMatterProcedure"/>
        <rdf:type rdf:resource="http://www.w3.org/2004/02/skos/core#Concept"/>
        <skos:definition>Humic acid carbon_unknown method</skos:definition>
        <skos:inScheme rdf:resource="http://w3id.org/glosis/model/procedure/organicMatterProcedure"/>
        <skos:notation>HumAcidC_unkn</skos:notation>
        <skos:prefLabel xml:lang="en">HumAcidC_unk</skos:prefLabel>
        <skos:scopeNote rdf:resource="https://www.isric.org/sites/default/files/isric_report_2014_01.pdf"/>
        <skos:scopeNote>Leenaars J.G.B., A.J.M. van Oostrum and M. Ruiperez Gonzalez, 2014. Africa Soil Profiles Database, Version 1.2. A compilation of georeferenced and standardised legacy soil profile data for Sub-Saharan Africa (with dataset). ISRIC Report 2014/01. Africa Soil Information Service (AfSIS) project and ISRIC - World Soil Information, Wageningen, the Netherlands. See Annex 4.</skos:scopeNote>
        <skos:topConceptOf rdf:resource="http://w3id.org/glosis/model/procedure/organicMatterProcedure"/>
    </owl:NamedIndividual>
    


    <!-- http://w3id.org/glosis/model/procedure/organicMatterProcedure-OrgM_calcul-oc1.73 -->


    <owl:NamedIndividual rdf:about="http://w3id.org/glosis/model/procedure/organicMatterProcedure-OrgM_calcul-oc1.73">
        <rdf:type rdf:resource="http://w3id.org/glosis/model/procedure/OrganicMatterProcedure"/>
        <rdf:type rdf:resource="http://www.w3.org/2004/02/skos/core#Concept"/>
        <skos:definition>Organic carbon * 1,73</skos:definition>
        <skos:inScheme rdf:resource="http://w3id.org/glosis/model/procedure/organicMatterProcedure"/>
        <skos:notation>OrgM_calcul-oc1.73</skos:notation>
        <skos:prefLabel xml:lang="en">OrgM_calcul-oc1.73</skos:prefLabel>
        <skos:scopeNote rdf:resource="https://www.isric.org/sites/default/files/isric_report_2014_01.pdf"/>
        <skos:scopeNote>Leenaars J.G.B., A.J.M. van Oostrum and M. Ruiperez Gonzalez, 2014. Africa Soil Profiles Database, Version 1.2. A compilation of georeferenced and standardised legacy soil profile data for Sub-Saharan Africa (with dataset). ISRIC Report 2014/01. Africa Soil Information Service (AfSIS) project and ISRIC - World Soil Information, Wageningen, the Netherlands. See Annex 4.</skos:scopeNote>
        <skos:topConceptOf rdf:resource="http://w3id.org/glosis/model/procedure/organicMatterProcedure"/>
    </owl:NamedIndividual>
    


    <!-- http://w3id.org/glosis/model/procedure/organicMatterProcedure-TotHumC_unkn -->


    <owl:NamedIndividual rdf:about="http://w3id.org/glosis/model/procedure/organicMatterProcedure-TotHumC_unkn">
        <rdf:type rdf:resource="http://w3id.org/glosis/model/procedure/OrganicMatterProcedure"/>
        <rdf:type rdf:resource="http://www.w3.org/2004/02/skos/core#Concept"/>
        <skos:definition>Total humic carbon_unknown method</skos:definition>
        <skos:inScheme rdf:resource="http://w3id.org/glosis/model/procedure/organicMatterProcedure"/>
        <skos:notation>TotHumC_unkn</skos:notation>
        <skos:prefLabel xml:lang="en">TotHumC_unk</skos:prefLabel>
        <skos:scopeNote rdf:resource="https://www.isric.org/sites/default/files/isric_report_2014_01.pdf"/>
        <skos:scopeNote>Leenaars J.G.B., A.J.M. van Oostrum and M. Ruiperez Gonzalez, 2014. Africa Soil Profiles Database, Version 1.2. A compilation of georeferenced and standardised legacy soil profile data for Sub-Saharan Africa (with dataset). ISRIC Report 2014/01. Africa Soil Information Service (AfSIS) project and ISRIC - World Soil Information, Wageningen, the Netherlands. See Annex 4.</skos:scopeNote>
        <skos:topConceptOf rdf:resource="http://w3id.org/glosis/model/procedure/organicMatterProcedure"/>
    </owl:NamedIndividual>
    


    <!-- http://w3id.org/glosis/model/procedure/pHProcedure -->


    <owl:NamedIndividual rdf:about="http://w3id.org/glosis/model/procedure/pHProcedure">
        <rdf:type rdf:resource="http://www.w3.org/2004/02/skos/core#ConceptScheme"/>
        <rdfs:label xml:lang="en">Code list for pH analysis procedures - codelist scheme</rdfs:label>
        <rdfs:seeAlso rdf:resource="http://w3id.org/glosis/model/procedure/PHProcedure"/>
        <skos:definition>AfSP-derived interpretation (RwaSP)</skos:definition>
        <skos:note xml:lang="en">This code list provides analysis procedures for pH.</skos:note>
        <skos:prefLabel xml:lang="en">Code list for pH analysis procedures - codelist scheme</skos:prefLabel>
    </owl:NamedIndividual>
    


    <!-- http://w3id.org/glosis/model/procedure/pHProcedure-pHCaCl2 -->


    <owl:NamedIndividual rdf:about="http://w3id.org/glosis/model/procedure/pHProcedure-pHCaCl2">
        <rdf:type rdf:resource="http://w3id.org/glosis/model/procedure/PHProcedure"/>
        <rdf:type rdf:resource="http://www.w3.org/2004/02/skos/core#Concept"/>
        <skos:definition>pHCaCl2 (soil reaction) in a soil/CaCl2 solution (0.01-1 M)</skos:definition>
        <skos:inScheme rdf:resource="http://w3id.org/glosis/model/procedure/pHProcedure"/>
        <skos:narrower rdf:resource="http://w3id.org/glosis/model/procedure/pHProcedure-pHCaCl2_ratio1-1"/>
        <skos:narrower rdf:resource="http://w3id.org/glosis/model/procedure/pHProcedure-pHCaCl2_ratio1-10"/>
        <skos:narrower rdf:resource="http://w3id.org/glosis/model/procedure/pHProcedure-pHCaCl2_ratio1-2"/>
        <skos:narrower rdf:resource="http://w3id.org/glosis/model/procedure/pHProcedure-pHCaCl2_ratio1-2.5"/>
        <skos:narrower rdf:resource="http://w3id.org/glosis/model/procedure/pHProcedure-pHCaCl2_ratio1-5"/>
        <skos:narrower rdf:resource="http://w3id.org/glosis/model/procedure/pHProcedure-pHCaCl2_sat"/>
        <skos:notation>pHCaCl2</skos:notation>
        <skos:prefLabel xml:lang="en">pHCaCl2</skos:prefLabel>
        <skos:scopeNote rdf:resource="https://www.isric.org/sites/default/files/isric_report_2014_01.pdf"/>
        <skos:scopeNote>Leenaars J.G.B., A.J.M. van Oostrum and M. Ruiperez Gonzalez, 2014. Africa Soil Profiles Database, Version 1.2. A compilation of georeferenced and standardised legacy soil profile data for Sub-Saharan Africa (with dataset). ISRIC Report 2014/01. Africa Soil Information Service (AfSIS) project and ISRIC - World Soil Information, Wageningen, the Netherlands. See Annex 4.</skos:scopeNote>
        <skos:topConceptOf rdf:resource="http://w3id.org/glosis/model/procedure/pHProcedure"/>
    </owl:NamedIndividual>
    


    <!-- http://w3id.org/glosis/model/procedure/pHProcedure-pHCaCl2_ratio1-1 -->


    <owl:NamedIndividual rdf:about="http://w3id.org/glosis/model/procedure/pHProcedure-pHCaCl2_ratio1-1">
        <rdf:type rdf:resource="http://w3id.org/glosis/model/procedure/PHProcedure"/>
        <rdf:type rdf:resource="http://www.w3.org/2004/02/skos/core#Concept"/>
        <skos:broader rdf:resource="http://w3id.org/glosis/model/procedure/pHProcedure-pHCaCl2"/>
        <skos:definition>pHCaCl2 (soil reaction) in 1:1 soil/1 M CaCl2 solution (1 M)</skos:definition>
        <skos:inScheme rdf:resource="http://w3id.org/glosis/model/procedure/pHProcedure"/>
        <skos:notation>pHCaCl2_ratio1-1</skos:notation>
        <skos:prefLabel xml:lang="en">pHCaCl2_ratio1-1</skos:prefLabel>
        <skos:scopeNote rdf:resource="https://www.isric.org/sites/default/files/isric_report_2014_01.pdf"/>
        <skos:scopeNote>Leenaars J.G.B., A.J.M. van Oostrum and M. Ruiperez Gonzalez, 2014. Africa Soil Profiles Database, Version 1.2. A compilation of georeferenced and standardised legacy soil profile data for Sub-Saharan Africa (with dataset). ISRIC Report 2014/01. Africa Soil Information Service (AfSIS) project and ISRIC - World Soil Information, Wageningen, the Netherlands. See Annex 4.</skos:scopeNote>
    </owl:NamedIndividual>
    


    <!-- http://w3id.org/glosis/model/procedure/pHProcedure-pHCaCl2_ratio1-10 -->


    <owl:NamedIndividual rdf:about="http://w3id.org/glosis/model/procedure/pHProcedure-pHCaCl2_ratio1-10">
        <rdf:type rdf:resource="http://w3id.org/glosis/model/procedure/PHProcedure"/>
        <rdf:type rdf:resource="http://www.w3.org/2004/02/skos/core#Concept"/>
        <skos:broader rdf:resource="http://w3id.org/glosis/model/procedure/pHProcedure-pHCaCl2"/>
        <skos:definition>pHCaCl2 (soil reaction) in 1:10 soil/CaCl2 solution (0.01-1 M)</skos:definition>
        <skos:inScheme rdf:resource="http://w3id.org/glosis/model/procedure/pHProcedure"/>
        <skos:notation>pHCaCl2_ratio1-10</skos:notation>
        <skos:prefLabel xml:lang="en">pHCaCl2_ratio1-10</skos:prefLabel>
        <skos:scopeNote rdf:resource="https://www.isric.org/sites/default/files/isric_report_2014_01.pdf"/>
        <skos:scopeNote>Leenaars J.G.B., A.J.M. van Oostrum and M. Ruiperez Gonzalez, 2014. Africa Soil Profiles Database, Version 1.2. A compilation of georeferenced and standardised legacy soil profile data for Sub-Saharan Africa (with dataset). ISRIC Report 2014/01. Africa Soil Information Service (AfSIS) project and ISRIC - World Soil Information, Wageningen, the Netherlands. See Annex 4.</skos:scopeNote>
    </owl:NamedIndividual>
    


    <!-- http://w3id.org/glosis/model/procedure/pHProcedure-pHCaCl2_ratio1-2 -->


    <owl:NamedIndividual rdf:about="http://w3id.org/glosis/model/procedure/pHProcedure-pHCaCl2_ratio1-2">
        <rdf:type rdf:resource="http://w3id.org/glosis/model/procedure/PHProcedure"/>
        <rdf:type rdf:resource="http://www.w3.org/2004/02/skos/core#Concept"/>
        <skos:broader rdf:resource="http://w3id.org/glosis/model/procedure/pHProcedure-pHCaCl2"/>
        <skos:definition>pHCaCl2 (soil reaction) in 1:2 soil/CaCl2 solution (0.01-1 M)</skos:definition>
        <skos:inScheme rdf:resource="http://w3id.org/glosis/model/procedure/pHProcedure"/>
        <skos:notation>pHCaCl2_ratio1-2</skos:notation>
        <skos:prefLabel xml:lang="en">pHCaCl2_ratio1-2</skos:prefLabel>
        <skos:scopeNote rdf:resource="https://www.isric.org/sites/default/files/isric_report_2014_01.pdf"/>
        <skos:scopeNote>Leenaars J.G.B., A.J.M. van Oostrum and M. Ruiperez Gonzalez, 2014. Africa Soil Profiles Database, Version 1.2. A compilation of georeferenced and standardised legacy soil profile data for Sub-Saharan Africa (with dataset). ISRIC Report 2014/01. Africa Soil Information Service (AfSIS) project and ISRIC - World Soil Information, Wageningen, the Netherlands. See Annex 4.</skos:scopeNote>
    </owl:NamedIndividual>
    


    <!-- http://w3id.org/glosis/model/procedure/pHProcedure-pHCaCl2_ratio1-2.5 -->


    <owl:NamedIndividual rdf:about="http://w3id.org/glosis/model/procedure/pHProcedure-pHCaCl2_ratio1-2.5">
        <rdf:type rdf:resource="http://w3id.org/glosis/model/procedure/PHProcedure"/>
        <rdf:type rdf:resource="http://www.w3.org/2004/02/skos/core#Concept"/>
        <skos:broader rdf:resource="http://w3id.org/glosis/model/procedure/pHProcedure-pHCaCl2"/>
        <skos:definition>pHCaCl2 (soil reaction) in 1:2.5 soil/CaCl2 solution (0.01-1 M)</skos:definition>
        <skos:inScheme rdf:resource="http://w3id.org/glosis/model/procedure/pHProcedure"/>
        <skos:notation>pHCaCl2_ratio1-2.5</skos:notation>
        <skos:prefLabel xml:lang="en">pHCaCl2_ratio1-2.5</skos:prefLabel>
        <skos:scopeNote rdf:resource="https://www.isric.org/sites/default/files/isric_report_2014_01.pdf"/>
        <skos:scopeNote>Leenaars J.G.B., A.J.M. van Oostrum and M. Ruiperez Gonzalez, 2014. Africa Soil Profiles Database, Version 1.2. A compilation of georeferenced and standardised legacy soil profile data for Sub-Saharan Africa (with dataset). ISRIC Report 2014/01. Africa Soil Information Service (AfSIS) project and ISRIC - World Soil Information, Wageningen, the Netherlands. See Annex 4.</skos:scopeNote>
    </owl:NamedIndividual>
    


    <!-- http://w3id.org/glosis/model/procedure/pHProcedure-pHCaCl2_ratio1-5 -->


    <owl:NamedIndividual rdf:about="http://w3id.org/glosis/model/procedure/pHProcedure-pHCaCl2_ratio1-5">
        <rdf:type rdf:resource="http://w3id.org/glosis/model/procedure/PHProcedure"/>
        <rdf:type rdf:resource="http://www.w3.org/2004/02/skos/core#Concept"/>
        <skos:broader rdf:resource="http://w3id.org/glosis/model/procedure/pHProcedure-pHCaCl2"/>
        <skos:definition>pHCaCl2 (soil reaction) in 1:5 soil/CaCl2 solution (0.01-1 M)</skos:definition>
        <skos:inScheme rdf:resource="http://w3id.org/glosis/model/procedure/pHProcedure"/>
        <skos:notation>pHCaCl2_ratio1-5</skos:notation>
        <skos:prefLabel xml:lang="en">pHCaCl2_ratio1-5</skos:prefLabel>
        <skos:scopeNote rdf:resource="https://www.isric.org/sites/default/files/isric_report_2014_01.pdf"/>
        <skos:scopeNote>Leenaars J.G.B., A.J.M. van Oostrum and M. Ruiperez Gonzalez, 2014. Africa Soil Profiles Database, Version 1.2. A compilation of georeferenced and standardised legacy soil profile data for Sub-Saharan Africa (with dataset). ISRIC Report 2014/01. Africa Soil Information Service (AfSIS) project and ISRIC - World Soil Information, Wageningen, the Netherlands. See Annex 4.</skos:scopeNote>
    </owl:NamedIndividual>
    


    <!-- http://w3id.org/glosis/model/procedure/pHProcedure-pHCaCl2_sat -->


    <owl:NamedIndividual rdf:about="http://w3id.org/glosis/model/procedure/pHProcedure-pHCaCl2_sat">
        <rdf:type rdf:resource="http://w3id.org/glosis/model/procedure/PHProcedure"/>
        <rdf:type rdf:resource="http://www.w3.org/2004/02/skos/core#Concept"/>
        <skos:broader rdf:resource="http://w3id.org/glosis/model/procedure/pHProcedure-pHCaCl2"/>
        <skos:definition>pHCaCl2 (soil reaction) in saturated paste</skos:definition>
        <skos:inScheme rdf:resource="http://w3id.org/glosis/model/procedure/pHProcedure"/>
        <skos:notation>pHCaCl2_sat</skos:notation>
        <skos:prefLabel xml:lang="en">pHCaCl2_sat</skos:prefLabel>
        <skos:scopeNote rdf:resource="https://www.isric.org/sites/default/files/isric_report_2014_01.pdf"/>
        <skos:scopeNote>Leenaars J.G.B., A.J.M. van Oostrum and M. Ruiperez Gonzalez, 2014. Africa Soil Profiles Database, Version 1.2. A compilation of georeferenced and standardised legacy soil profile data for Sub-Saharan Africa (with dataset). ISRIC Report 2014/01. Africa Soil Information Service (AfSIS) project and ISRIC - World Soil Information, Wageningen, the Netherlands. See Annex 4.</skos:scopeNote>
    </owl:NamedIndividual>
    


    <!-- http://w3id.org/glosis/model/procedure/pHProcedure-pHH2O -->


    <owl:NamedIndividual rdf:about="http://w3id.org/glosis/model/procedure/pHProcedure-pHH2O">
        <rdf:type rdf:resource="http://w3id.org/glosis/model/procedure/PHProcedure"/>
        <rdf:type rdf:resource="http://www.w3.org/2004/02/skos/core#Concept"/>
        <skos:definition>pHH2O (soil reaction) in a soil/water solution</skos:definition>
        <skos:inScheme rdf:resource="http://w3id.org/glosis/model/procedure/pHProcedure"/>
        <skos:narrower rdf:resource="http://w3id.org/glosis/model/procedure/pHProcedure-pHH2O_ratio1-1"/>
        <skos:narrower rdf:resource="http://w3id.org/glosis/model/procedure/pHProcedure-pHH2O_ratio1-10"/>
        <skos:narrower rdf:resource="http://w3id.org/glosis/model/procedure/pHProcedure-pHH2O_ratio1-2"/>
        <skos:narrower rdf:resource="http://w3id.org/glosis/model/procedure/pHProcedure-pHH2O_ratio1-2.5"/>
        <skos:narrower rdf:resource="http://w3id.org/glosis/model/procedure/pHProcedure-pHH2O_ratio1-5"/>
        <skos:narrower rdf:resource="http://w3id.org/glosis/model/procedure/pHProcedure-pHH2O_sat"/>
        <skos:narrower rdf:resource="http://w3id.org/glosis/model/procedure/pHProcedure-pHH2O_unkn-spec"/>
        <skos:notation>pHH2O</skos:notation>
        <skos:prefLabel xml:lang="en">pHH2O</skos:prefLabel>
        <skos:scopeNote rdf:resource="https://www.isric.org/sites/default/files/isric_report_2014_01.pdf"/>
        <skos:scopeNote>Leenaars J.G.B., A.J.M. van Oostrum and M. Ruiperez Gonzalez, 2014. Africa Soil Profiles Database, Version 1.2. A compilation of georeferenced and standardised legacy soil profile data for Sub-Saharan Africa (with dataset). ISRIC Report 2014/01. Africa Soil Information Service (AfSIS) project and ISRIC - World Soil Information, Wageningen, the Netherlands. See Annex 4.</skos:scopeNote>
        <skos:topConceptOf rdf:resource="http://w3id.org/glosis/model/procedure/pHProcedure"/>
    </owl:NamedIndividual>
    


    <!-- http://w3id.org/glosis/model/procedure/pHProcedure-pHH2O_ratio1-1 -->


    <owl:NamedIndividual rdf:about="http://w3id.org/glosis/model/procedure/pHProcedure-pHH2O_ratio1-1">
        <rdf:type rdf:resource="http://w3id.org/glosis/model/procedure/PHProcedure"/>
        <rdf:type rdf:resource="http://www.w3.org/2004/02/skos/core#Concept"/>
        <skos:broader rdf:resource="http://w3id.org/glosis/model/procedure/pHProcedure-pHH2O"/>
        <skos:definition>pHH2O (soil reaction) in 1:1 soil/water solution</skos:definition>
        <skos:inScheme rdf:resource="http://w3id.org/glosis/model/procedure/pHProcedure"/>
        <skos:notation>pHH2O_ratio1-1</skos:notation>
        <skos:prefLabel xml:lang="en">pHH2O_ratio1-1</skos:prefLabel>
        <skos:scopeNote rdf:resource="https://www.isric.org/sites/default/files/isric_report_2014_01.pdf"/>
        <skos:scopeNote>Leenaars J.G.B., A.J.M. van Oostrum and M. Ruiperez Gonzalez, 2014. Africa Soil Profiles Database, Version 1.2. A compilation of georeferenced and standardised legacy soil profile data for Sub-Saharan Africa (with dataset). ISRIC Report 2014/01. Africa Soil Information Service (AfSIS) project and ISRIC - World Soil Information, Wageningen, the Netherlands. See Annex 4.</skos:scopeNote>
    </owl:NamedIndividual>
    


    <!-- http://w3id.org/glosis/model/procedure/pHProcedure-pHH2O_ratio1-10 -->


    <owl:NamedIndividual rdf:about="http://w3id.org/glosis/model/procedure/pHProcedure-pHH2O_ratio1-10">
        <rdf:type rdf:resource="http://w3id.org/glosis/model/procedure/PHProcedure"/>
        <rdf:type rdf:resource="http://www.w3.org/2004/02/skos/core#Concept"/>
        <skos:broader rdf:resource="http://w3id.org/glosis/model/procedure/pHProcedure-pHH2O"/>
        <skos:definition>pHH2O (soil reaction) in 1:10 soil/water solution</skos:definition>
        <skos:inScheme rdf:resource="http://w3id.org/glosis/model/procedure/pHProcedure"/>
        <skos:notation>pHH2O_ratio1-10</skos:notation>
        <skos:prefLabel xml:lang="en">pHH2O_ratio1-10</skos:prefLabel>
        <skos:scopeNote rdf:resource="https://www.isric.org/sites/default/files/isric_report_2014_01.pdf"/>
        <skos:scopeNote>Leenaars J.G.B., A.J.M. van Oostrum and M. Ruiperez Gonzalez, 2014. Africa Soil Profiles Database, Version 1.2. A compilation of georeferenced and standardised legacy soil profile data for Sub-Saharan Africa (with dataset). ISRIC Report 2014/01. Africa Soil Information Service (AfSIS) project and ISRIC - World Soil Information, Wageningen, the Netherlands. See Annex 4.</skos:scopeNote>
    </owl:NamedIndividual>
    


    <!-- http://w3id.org/glosis/model/procedure/pHProcedure-pHH2O_ratio1-2 -->


    <owl:NamedIndividual rdf:about="http://w3id.org/glosis/model/procedure/pHProcedure-pHH2O_ratio1-2">
        <rdf:type rdf:resource="http://w3id.org/glosis/model/procedure/PHProcedure"/>
        <rdf:type rdf:resource="http://www.w3.org/2004/02/skos/core#Concept"/>
        <skos:broader rdf:resource="http://w3id.org/glosis/model/procedure/pHProcedure-pHH2O"/>
        <skos:definition>pHH2O (soil reaction) in 1:2 soil/water solution</skos:definition>
        <skos:inScheme rdf:resource="http://w3id.org/glosis/model/procedure/pHProcedure"/>
        <skos:notation>pHH2O_ratio1-2</skos:notation>
        <skos:prefLabel xml:lang="en">pHH2O_ratio1-2</skos:prefLabel>
        <skos:scopeNote rdf:resource="https://www.isric.org/sites/default/files/isric_report_2014_01.pdf"/>
        <skos:scopeNote>Leenaars J.G.B., A.J.M. van Oostrum and M. Ruiperez Gonzalez, 2014. Africa Soil Profiles Database, Version 1.2. A compilation of georeferenced and standardised legacy soil profile data for Sub-Saharan Africa (with dataset). ISRIC Report 2014/01. Africa Soil Information Service (AfSIS) project and ISRIC - World Soil Information, Wageningen, the Netherlands. See Annex 4.</skos:scopeNote>
    </owl:NamedIndividual>
    


    <!-- http://w3id.org/glosis/model/procedure/pHProcedure-pHH2O_ratio1-2.5 -->


    <owl:NamedIndividual rdf:about="http://w3id.org/glosis/model/procedure/pHProcedure-pHH2O_ratio1-2.5">
        <rdf:type rdf:resource="http://w3id.org/glosis/model/procedure/PHProcedure"/>
        <rdf:type rdf:resource="http://www.w3.org/2004/02/skos/core#Concept"/>
        <skos:broader rdf:resource="http://w3id.org/glosis/model/procedure/pHProcedure-pHH2O"/>
        <skos:definition>pHH2O (soil reaction) in 1:2.5 soil/water solution</skos:definition>
        <skos:inScheme rdf:resource="http://w3id.org/glosis/model/procedure/pHProcedure"/>
        <skos:notation>pHH2O_ratio1-2.5</skos:notation>
        <skos:prefLabel xml:lang="en">pHH2O_ratio1-2.5</skos:prefLabel>
        <skos:scopeNote rdf:resource="https://www.isric.org/sites/default/files/isric_report_2014_01.pdf"/>
        <skos:scopeNote>Leenaars J.G.B., A.J.M. van Oostrum and M. Ruiperez Gonzalez, 2014. Africa Soil Profiles Database, Version 1.2. A compilation of georeferenced and standardised legacy soil profile data for Sub-Saharan Africa (with dataset). ISRIC Report 2014/01. Africa Soil Information Service (AfSIS) project and ISRIC - World Soil Information, Wageningen, the Netherlands. See Annex 4.</skos:scopeNote>
    </owl:NamedIndividual>
    


    <!-- http://w3id.org/glosis/model/procedure/pHProcedure-pHH2O_ratio1-5 -->


    <owl:NamedIndividual rdf:about="http://w3id.org/glosis/model/procedure/pHProcedure-pHH2O_ratio1-5">
        <rdf:type rdf:resource="http://w3id.org/glosis/model/procedure/PHProcedure"/>
        <rdf:type rdf:resource="http://www.w3.org/2004/02/skos/core#Concept"/>
        <skos:broader rdf:resource="http://w3id.org/glosis/model/procedure/pHProcedure-pHH2O"/>
        <skos:definition>pHH2O (soil reaction) in 1:5 soil/water solution</skos:definition>
        <skos:inScheme rdf:resource="http://w3id.org/glosis/model/procedure/pHProcedure"/>
        <skos:notation>pHH2O_ratio1-5</skos:notation>
        <skos:prefLabel xml:lang="en">pHH2O_ratio1-5</skos:prefLabel>
        <skos:scopeNote rdf:resource="https://www.isric.org/sites/default/files/isric_report_2014_01.pdf"/>
        <skos:scopeNote>Leenaars J.G.B., A.J.M. van Oostrum and M. Ruiperez Gonzalez, 2014. Africa Soil Profiles Database, Version 1.2. A compilation of georeferenced and standardised legacy soil profile data for Sub-Saharan Africa (with dataset). ISRIC Report 2014/01. Africa Soil Information Service (AfSIS) project and ISRIC - World Soil Information, Wageningen, the Netherlands. See Annex 4.</skos:scopeNote>
    </owl:NamedIndividual>
    


    <!-- http://w3id.org/glosis/model/procedure/pHProcedure-pHH2O_sat -->


    <owl:NamedIndividual rdf:about="http://w3id.org/glosis/model/procedure/pHProcedure-pHH2O_sat">
        <rdf:type rdf:resource="http://w3id.org/glosis/model/procedure/PHProcedure"/>
        <rdf:type rdf:resource="http://www.w3.org/2004/02/skos/core#Concept"/>
        <skos:broader rdf:resource="http://w3id.org/glosis/model/procedure/pHProcedure-pHH2O"/>
        <skos:definition>pHH2O (soil reaction) in water saturated paste</skos:definition>
        <skos:inScheme rdf:resource="http://w3id.org/glosis/model/procedure/pHProcedure"/>
        <skos:notation>pHH2O_sat</skos:notation>
        <skos:prefLabel xml:lang="en">pHH2O_sat</skos:prefLabel>
        <skos:scopeNote rdf:resource="https://www.isric.org/sites/default/files/isric_report_2014_01.pdf"/>
        <skos:scopeNote>Leenaars J.G.B., A.J.M. van Oostrum and M. Ruiperez Gonzalez, 2014. Africa Soil Profiles Database, Version 1.2. A compilation of georeferenced and standardised legacy soil profile data for Sub-Saharan Africa (with dataset). ISRIC Report 2014/01. Africa Soil Information Service (AfSIS) project and ISRIC - World Soil Information, Wageningen, the Netherlands. See Annex 4.</skos:scopeNote>
    </owl:NamedIndividual>
    


    <!-- http://w3id.org/glosis/model/procedure/pHProcedure-pHH2O_unkn-spec -->


    <owl:NamedIndividual rdf:about="http://w3id.org/glosis/model/procedure/pHProcedure-pHH2O_unkn-spec">
        <rdf:type rdf:resource="http://w3id.org/glosis/model/procedure/PHProcedure"/>
        <rdf:type rdf:resource="http://www.w3.org/2004/02/skos/core#Concept"/>
        <skos:broader rdf:resource="http://w3id.org/glosis/model/procedure/pHProcedure-pHH2O"/>
        <skos:definition>Spectrally measured and converted to pHH2O (soil reaction) in unknown soil/water solution</skos:definition>
        <skos:inScheme rdf:resource="http://w3id.org/glosis/model/procedure/pHProcedure"/>
        <skos:notation>pHH2O_unkn-spec</skos:notation>
        <skos:prefLabel xml:lang="en">pHH2O_unkn-spec</skos:prefLabel>
        <skos:scopeNote rdf:resource="https://www.isric.org/sites/default/files/isric_report_2014_01.pdf"/>
        <skos:scopeNote>Leenaars J.G.B., A.J.M. van Oostrum and M. Ruiperez Gonzalez, 2014. Africa Soil Profiles Database, Version 1.2. A compilation of georeferenced and standardised legacy soil profile data for Sub-Saharan Africa (with dataset). ISRIC Report 2014/01. Africa Soil Information Service (AfSIS) project and ISRIC - World Soil Information, Wageningen, the Netherlands. See Annex 4.</skos:scopeNote>
    </owl:NamedIndividual>
    


    <!-- http://w3id.org/glosis/model/procedure/pHProcedure-pHKCl -->


    <owl:NamedIndividual rdf:about="http://w3id.org/glosis/model/procedure/pHProcedure-pHKCl">
        <rdf:type rdf:resource="http://w3id.org/glosis/model/procedure/PHProcedure"/>
        <rdf:type rdf:resource="http://www.w3.org/2004/02/skos/core#Concept"/>
        <skos:definition>pHKCl (soil reaction) in a soil/KCl solution (0.01-1 M)</skos:definition>
        <skos:inScheme rdf:resource="http://w3id.org/glosis/model/procedure/pHProcedure"/>
        <skos:narrower rdf:resource="http://w3id.org/glosis/model/procedure/pHProcedure-pHKCl_ratio1-1"/>
        <skos:narrower rdf:resource="http://w3id.org/glosis/model/procedure/pHProcedure-pHKCl_ratio1-10"/>
        <skos:narrower rdf:resource="http://w3id.org/glosis/model/procedure/pHProcedure-pHKCl_ratio1-2"/>
        <skos:narrower rdf:resource="http://w3id.org/glosis/model/procedure/pHProcedure-pHKCl_ratio1-2.5"/>
        <skos:narrower rdf:resource="http://w3id.org/glosis/model/procedure/pHProcedure-pHKCl_ratio1-5"/>
        <skos:notation>pHKCl</skos:notation>
        <skos:prefLabel xml:lang="en">pHKCl</skos:prefLabel>
        <skos:scopeNote rdf:resource="https://www.isric.org/sites/default/files/isric_report_2014_01.pdf"/>
        <skos:scopeNote>Leenaars J.G.B., A.J.M. van Oostrum and M. Ruiperez Gonzalez, 2014. Africa Soil Profiles Database, Version 1.2. A compilation of georeferenced and standardised legacy soil profile data for Sub-Saharan Africa (with dataset). ISRIC Report 2014/01. Africa Soil Information Service (AfSIS) project and ISRIC - World Soil Information, Wageningen, the Netherlands. See Annex 4.</skos:scopeNote>
        <skos:topConceptOf rdf:resource="http://w3id.org/glosis/model/procedure/pHProcedure"/>
    </owl:NamedIndividual>
    


    <!-- http://w3id.org/glosis/model/procedure/pHProcedure-pHKCl_ratio1-1 -->


    <owl:NamedIndividual rdf:about="http://w3id.org/glosis/model/procedure/pHProcedure-pHKCl_ratio1-1">
        <rdf:type rdf:resource="http://w3id.org/glosis/model/procedure/PHProcedure"/>
        <rdf:type rdf:resource="http://www.w3.org/2004/02/skos/core#Concept"/>
        <skos:broader rdf:resource="http://w3id.org/glosis/model/procedure/pHProcedure-pHKCl"/>
        <skos:definition>pHKCl (soil reaction) in 1:1 soil/KCl solution (1 M)</skos:definition>
        <skos:inScheme rdf:resource="http://w3id.org/glosis/model/procedure/pHProcedure"/>
        <skos:notation>pHKCl_ratio1-1</skos:notation>
        <skos:prefLabel xml:lang="en">pHKCl_ratio1-1</skos:prefLabel>
        <skos:scopeNote rdf:resource="https://www.isric.org/sites/default/files/isric_report_2014_01.pdf"/>
        <skos:scopeNote>Leenaars J.G.B., A.J.M. van Oostrum and M. Ruiperez Gonzalez, 2014. Africa Soil Profiles Database, Version 1.2. A compilation of georeferenced and standardised legacy soil profile data for Sub-Saharan Africa (with dataset). ISRIC Report 2014/01. Africa Soil Information Service (AfSIS) project and ISRIC - World Soil Information, Wageningen, the Netherlands. See Annex 4.</skos:scopeNote>
    </owl:NamedIndividual>
    


    <!-- http://w3id.org/glosis/model/procedure/pHProcedure-pHKCl_ratio1-10 -->


    <owl:NamedIndividual rdf:about="http://w3id.org/glosis/model/procedure/pHProcedure-pHKCl_ratio1-10">
        <rdf:type rdf:resource="http://w3id.org/glosis/model/procedure/PHProcedure"/>
        <rdf:type rdf:resource="http://www.w3.org/2004/02/skos/core#Concept"/>
        <skos:broader rdf:resource="http://w3id.org/glosis/model/procedure/pHProcedure-pHKCl"/>
        <skos:definition>pHKCl (soil reaction) in 1:10 soil/KCl solution (0.01-1 M)</skos:definition>
        <skos:inScheme rdf:resource="http://w3id.org/glosis/model/procedure/pHProcedure"/>
        <skos:notation>pHKCl_ratio1-10</skos:notation>
        <skos:prefLabel xml:lang="en">pHKCl_ratio1-10</skos:prefLabel>
        <skos:scopeNote rdf:resource="https://www.isric.org/sites/default/files/isric_report_2014_01.pdf"/>
        <skos:scopeNote>Leenaars J.G.B., A.J.M. van Oostrum and M. Ruiperez Gonzalez, 2014. Africa Soil Profiles Database, Version 1.2. A compilation of georeferenced and standardised legacy soil profile data for Sub-Saharan Africa (with dataset). ISRIC Report 2014/01. Africa Soil Information Service (AfSIS) project and ISRIC - World Soil Information, Wageningen, the Netherlands. See Annex 4.</skos:scopeNote>
    </owl:NamedIndividual>
    


    <!-- http://w3id.org/glosis/model/procedure/pHProcedure-pHKCl_ratio1-2 -->


    <owl:NamedIndividual rdf:about="http://w3id.org/glosis/model/procedure/pHProcedure-pHKCl_ratio1-2">
        <rdf:type rdf:resource="http://w3id.org/glosis/model/procedure/PHProcedure"/>
        <rdf:type rdf:resource="http://www.w3.org/2004/02/skos/core#Concept"/>
        <skos:broader rdf:resource="http://w3id.org/glosis/model/procedure/pHProcedure-pHKCl"/>
        <skos:definition>pHKCl (soil reaction) in 1:2 soil/KCl solution (0.01-1 M)</skos:definition>
        <skos:inScheme rdf:resource="http://w3id.org/glosis/model/procedure/pHProcedure"/>
        <skos:notation>pHKCl_ratio1-2</skos:notation>
        <skos:prefLabel xml:lang="en">pHKCl_ratio1-2</skos:prefLabel>
        <skos:scopeNote rdf:resource="https://www.isric.org/sites/default/files/isric_report_2014_01.pdf"/>
        <skos:scopeNote>Leenaars J.G.B., A.J.M. van Oostrum and M. Ruiperez Gonzalez, 2014. Africa Soil Profiles Database, Version 1.2. A compilation of georeferenced and standardised legacy soil profile data for Sub-Saharan Africa (with dataset). ISRIC Report 2014/01. Africa Soil Information Service (AfSIS) project and ISRIC - World Soil Information, Wageningen, the Netherlands. See Annex 4.</skos:scopeNote>
    </owl:NamedIndividual>
    


    <!-- http://w3id.org/glosis/model/procedure/pHProcedure-pHKCl_ratio1-2.5 -->


    <owl:NamedIndividual rdf:about="http://w3id.org/glosis/model/procedure/pHProcedure-pHKCl_ratio1-2.5">
        <rdf:type rdf:resource="http://w3id.org/glosis/model/procedure/PHProcedure"/>
        <rdf:type rdf:resource="http://www.w3.org/2004/02/skos/core#Concept"/>
        <skos:broader rdf:resource="http://w3id.org/glosis/model/procedure/pHProcedure-pHKCl"/>
        <skos:definition>pHKCl (soil reaction) in 1:2.5 soil/KCl solution (0.01-1 M)</skos:definition>
        <skos:inScheme rdf:resource="http://w3id.org/glosis/model/procedure/pHProcedure"/>
        <skos:notation>pHKCl_ratio1-2.5</skos:notation>
        <skos:prefLabel xml:lang="en">pHKCl_ratio1-2.5</skos:prefLabel>
        <skos:scopeNote rdf:resource="https://www.isric.org/sites/default/files/isric_report_2014_01.pdf"/>
        <skos:scopeNote>Leenaars J.G.B., A.J.M. van Oostrum and M. Ruiperez Gonzalez, 2014. Africa Soil Profiles Database, Version 1.2. A compilation of georeferenced and standardised legacy soil profile data for Sub-Saharan Africa (with dataset). ISRIC Report 2014/01. Africa Soil Information Service (AfSIS) project and ISRIC - World Soil Information, Wageningen, the Netherlands. See Annex 4.</skos:scopeNote>
    </owl:NamedIndividual>
    


    <!-- http://w3id.org/glosis/model/procedure/pHProcedure-pHKCl_ratio1-5 -->


    <owl:NamedIndividual rdf:about="http://w3id.org/glosis/model/procedure/pHProcedure-pHKCl_ratio1-5">
        <rdf:type rdf:resource="http://w3id.org/glosis/model/procedure/PHProcedure"/>
        <rdf:type rdf:resource="http://www.w3.org/2004/02/skos/core#Concept"/>
        <skos:broader rdf:resource="http://w3id.org/glosis/model/procedure/pHProcedure-pHKCl"/>
        <skos:definition>pHKCl (soil reaction) in 1:5 soil/KCl solution (0.01-1 M)</skos:definition>
        <skos:inScheme rdf:resource="http://w3id.org/glosis/model/procedure/pHProcedure"/>
        <skos:notation>pHKCl_ratio1-5</skos:notation>
        <skos:prefLabel xml:lang="en">pHKCl_ratio1-5</skos:prefLabel>
        <skos:scopeNote rdf:resource="https://www.isric.org/sites/default/files/isric_report_2014_01.pdf"/>
        <skos:scopeNote>Leenaars J.G.B., A.J.M. van Oostrum and M. Ruiperez Gonzalez, 2014. Africa Soil Profiles Database, Version 1.2. A compilation of georeferenced and standardised legacy soil profile data for Sub-Saharan Africa (with dataset). ISRIC Report 2014/01. Africa Soil Information Service (AfSIS) project and ISRIC - World Soil Information, Wageningen, the Netherlands. See Annex 4.</skos:scopeNote>
    </owl:NamedIndividual>
    


    <!-- http://w3id.org/glosis/model/procedure/pHProcedure-pHKCl_sat -->


    <owl:NamedIndividual rdf:about="http://w3id.org/glosis/model/procedure/pHProcedure-pHKCl_sat">
        <rdf:type rdf:resource="http://w3id.org/glosis/model/procedure/PHProcedure"/>
        <rdf:type rdf:resource="http://www.w3.org/2004/02/skos/core#Concept"/>
        <skos:definition>pHKCl (soil reaction) in saturated paste</skos:definition>
        <skos:inScheme rdf:resource="http://w3id.org/glosis/model/procedure/pHProcedure"/>
        <skos:notation>pHKCl_sat</skos:notation>
        <skos:prefLabel xml:lang="en">pHKCl_sat</skos:prefLabel>
        <skos:scopeNote rdf:resource="https://www.isric.org/sites/default/files/isric_report_2014_01.pdf"/>
        <skos:scopeNote>Leenaars J.G.B., A.J.M. van Oostrum and M. Ruiperez Gonzalez, 2014. Africa Soil Profiles Database, Version 1.2. A compilation of georeferenced and standardised legacy soil profile data for Sub-Saharan Africa (with dataset). ISRIC Report 2014/01. Africa Soil Information Service (AfSIS) project and ISRIC - World Soil Information, Wageningen, the Netherlands. See Annex 4.</skos:scopeNote>
        <skos:topConceptOf rdf:resource="http://w3id.org/glosis/model/procedure/pHProcedure"/>
    </owl:NamedIndividual>
    


    <!-- http://w3id.org/glosis/model/procedure/pHProcedure-pHNaF -->


    <owl:NamedIndividual rdf:about="http://w3id.org/glosis/model/procedure/pHProcedure-pHNaF">
        <rdf:type rdf:resource="http://w3id.org/glosis/model/procedure/PHProcedure"/>
        <rdf:type rdf:resource="http://www.w3.org/2004/02/skos/core#Concept"/>
        <skos:definition>pHNaF (soil reaction) in a soil/NaF solution (0.01-1 M)</skos:definition>
        <skos:inScheme rdf:resource="http://w3id.org/glosis/model/procedure/pHProcedure"/>
        <skos:narrower rdf:resource="http://w3id.org/glosis/model/procedure/pHProcedure-pHNaF_ratio1-1"/>
        <skos:narrower rdf:resource="http://w3id.org/glosis/model/procedure/pHProcedure-pHNaF_ratio1-10"/>
        <skos:narrower rdf:resource="http://w3id.org/glosis/model/procedure/pHProcedure-pHNaF_ratio1-2"/>
        <skos:narrower rdf:resource="http://w3id.org/glosis/model/procedure/pHProcedure-pHNaF_ratio1-2.5"/>
        <skos:narrower rdf:resource="http://w3id.org/glosis/model/procedure/pHProcedure-pHNaF_ratio1-5"/>
        <skos:narrower rdf:resource="http://w3id.org/glosis/model/procedure/pHProcedure-pHNaF_sat"/>
        <skos:notation>pHNaF</skos:notation>
        <skos:prefLabel xml:lang="en">pHNaF</skos:prefLabel>
        <skos:scopeNote rdf:resource="https://www.isric.org/sites/default/files/isric_report_2014_01.pdf"/>
        <skos:scopeNote>Leenaars J.G.B., A.J.M. van Oostrum and M. Ruiperez Gonzalez, 2014. Africa Soil Profiles Database, Version 1.2. A compilation of georeferenced and standardised legacy soil profile data for Sub-Saharan Africa (with dataset). ISRIC Report 2014/01. Africa Soil Information Service (AfSIS) project and ISRIC - World Soil Information, Wageningen, the Netherlands. See Annex 4.</skos:scopeNote>
        <skos:topConceptOf rdf:resource="http://w3id.org/glosis/model/procedure/pHProcedure"/>
    </owl:NamedIndividual>
    


    <!-- http://w3id.org/glosis/model/procedure/pHProcedure-pHNaF_ratio1-1 -->


    <owl:NamedIndividual rdf:about="http://w3id.org/glosis/model/procedure/pHProcedure-pHNaF_ratio1-1">
        <rdf:type rdf:resource="http://w3id.org/glosis/model/procedure/PHProcedure"/>
        <rdf:type rdf:resource="http://www.w3.org/2004/02/skos/core#Concept"/>
        <skos:broader rdf:resource="http://w3id.org/glosis/model/procedure/pHProcedure-pHNaF"/>
        <skos:definition>pHNaF (soil reaction) in 1:1 soil/NaF solution (1 M)</skos:definition>
        <skos:inScheme rdf:resource="http://w3id.org/glosis/model/procedure/pHProcedure"/>
        <skos:notation>pHNaF_ratio1-1</skos:notation>
        <skos:prefLabel xml:lang="en">pHNaF_ratio1-1</skos:prefLabel>
        <skos:scopeNote rdf:resource="https://www.isric.org/sites/default/files/isric_report_2014_01.pdf"/>
        <skos:scopeNote>Leenaars J.G.B., A.J.M. van Oostrum and M. Ruiperez Gonzalez, 2014. Africa Soil Profiles Database, Version 1.2. A compilation of georeferenced and standardised legacy soil profile data for Sub-Saharan Africa (with dataset). ISRIC Report 2014/01. Africa Soil Information Service (AfSIS) project and ISRIC - World Soil Information, Wageningen, the Netherlands. See Annex 4.</skos:scopeNote>
    </owl:NamedIndividual>
    


    <!-- http://w3id.org/glosis/model/procedure/pHProcedure-pHNaF_ratio1-10 -->


    <owl:NamedIndividual rdf:about="http://w3id.org/glosis/model/procedure/pHProcedure-pHNaF_ratio1-10">
        <rdf:type rdf:resource="http://w3id.org/glosis/model/procedure/PHProcedure"/>
        <rdf:type rdf:resource="http://www.w3.org/2004/02/skos/core#Concept"/>
        <skos:broader rdf:resource="http://w3id.org/glosis/model/procedure/pHProcedure-pHNaF"/>
        <skos:definition>pHNaF (soil reaction) in 1:10 soil/NaF solution (0.01-1 M)</skos:definition>
        <skos:inScheme rdf:resource="http://w3id.org/glosis/model/procedure/pHProcedure"/>
        <skos:notation>pHNaF_ratio1-10</skos:notation>
        <skos:prefLabel xml:lang="en">pHNaF_ratio1-10</skos:prefLabel>
        <skos:scopeNote rdf:resource="https://www.isric.org/sites/default/files/isric_report_2014_01.pdf"/>
        <skos:scopeNote>Leenaars J.G.B., A.J.M. van Oostrum and M. Ruiperez Gonzalez, 2014. Africa Soil Profiles Database, Version 1.2. A compilation of georeferenced and standardised legacy soil profile data for Sub-Saharan Africa (with dataset). ISRIC Report 2014/01. Africa Soil Information Service (AfSIS) project and ISRIC - World Soil Information, Wageningen, the Netherlands. See Annex 4.</skos:scopeNote>
    </owl:NamedIndividual>
    


    <!-- http://w3id.org/glosis/model/procedure/pHProcedure-pHNaF_ratio1-2 -->


    <owl:NamedIndividual rdf:about="http://w3id.org/glosis/model/procedure/pHProcedure-pHNaF_ratio1-2">
        <rdf:type rdf:resource="http://w3id.org/glosis/model/procedure/PHProcedure"/>
        <rdf:type rdf:resource="http://www.w3.org/2004/02/skos/core#Concept"/>
        <skos:broader rdf:resource="http://w3id.org/glosis/model/procedure/pHProcedure-pHNaF"/>
        <skos:definition>pHNaF (soil reaction) in 1:2 soil/NaF solution (0.01-1 M)</skos:definition>
        <skos:inScheme rdf:resource="http://w3id.org/glosis/model/procedure/pHProcedure"/>
        <skos:notation>pHNaF_ratio1-2</skos:notation>
        <skos:prefLabel xml:lang="en">pHNaF_ratio1-2</skos:prefLabel>
        <skos:scopeNote rdf:resource="https://www.isric.org/sites/default/files/isric_report_2014_01.pdf"/>
        <skos:scopeNote>Leenaars J.G.B., A.J.M. van Oostrum and M. Ruiperez Gonzalez, 2014. Africa Soil Profiles Database, Version 1.2. A compilation of georeferenced and standardised legacy soil profile data for Sub-Saharan Africa (with dataset). ISRIC Report 2014/01. Africa Soil Information Service (AfSIS) project and ISRIC - World Soil Information, Wageningen, the Netherlands. See Annex 4.</skos:scopeNote>
    </owl:NamedIndividual>
    


    <!-- http://w3id.org/glosis/model/procedure/pHProcedure-pHNaF_ratio1-2.5 -->


    <owl:NamedIndividual rdf:about="http://w3id.org/glosis/model/procedure/pHProcedure-pHNaF_ratio1-2.5">
        <rdf:type rdf:resource="http://w3id.org/glosis/model/procedure/PHProcedure"/>
        <rdf:type rdf:resource="http://www.w3.org/2004/02/skos/core#Concept"/>
        <skos:broader rdf:resource="http://w3id.org/glosis/model/procedure/pHProcedure-pHNaF"/>
        <skos:definition>pHNaF (soil reaction) in 1:2.5 soil/NaF solution (0.01-1 M)</skos:definition>
        <skos:inScheme rdf:resource="http://w3id.org/glosis/model/procedure/pHProcedure"/>
        <skos:notation>pHNaF_ratio1-2.5</skos:notation>
        <skos:prefLabel xml:lang="en">pHNaF_ratio1-2.5</skos:prefLabel>
        <skos:scopeNote rdf:resource="https://www.isric.org/sites/default/files/isric_report_2014_01.pdf"/>
        <skos:scopeNote>Leenaars J.G.B., A.J.M. van Oostrum and M. Ruiperez Gonzalez, 2014. Africa Soil Profiles Database, Version 1.2. A compilation of georeferenced and standardised legacy soil profile data for Sub-Saharan Africa (with dataset). ISRIC Report 2014/01. Africa Soil Information Service (AfSIS) project and ISRIC - World Soil Information, Wageningen, the Netherlands. See Annex 4.</skos:scopeNote>
    </owl:NamedIndividual>
    


    <!-- http://w3id.org/glosis/model/procedure/pHProcedure-pHNaF_ratio1-5 -->


    <owl:NamedIndividual rdf:about="http://w3id.org/glosis/model/procedure/pHProcedure-pHNaF_ratio1-5">
        <rdf:type rdf:resource="http://w3id.org/glosis/model/procedure/PHProcedure"/>
        <rdf:type rdf:resource="http://www.w3.org/2004/02/skos/core#Concept"/>
        <skos:broader rdf:resource="http://w3id.org/glosis/model/procedure/pHProcedure-pHNaF"/>
        <skos:definition>pHNaF (soil reaction) in 1:5 soil/NaF solution (0.01-1 M)</skos:definition>
        <skos:inScheme rdf:resource="http://w3id.org/glosis/model/procedure/pHProcedure"/>
        <skos:notation>pHNaF_ratio1-5</skos:notation>
        <skos:prefLabel xml:lang="en">pHNaF_ratio1-5</skos:prefLabel>
        <skos:scopeNote rdf:resource="https://www.isric.org/sites/default/files/isric_report_2014_01.pdf"/>
        <skos:scopeNote>Leenaars J.G.B., A.J.M. van Oostrum and M. Ruiperez Gonzalez, 2014. Africa Soil Profiles Database, Version 1.2. A compilation of georeferenced and standardised legacy soil profile data for Sub-Saharan Africa (with dataset). ISRIC Report 2014/01. Africa Soil Information Service (AfSIS) project and ISRIC - World Soil Information, Wageningen, the Netherlands. See Annex 4.</skos:scopeNote>
    </owl:NamedIndividual>
    


    <!-- http://w3id.org/glosis/model/procedure/pHProcedure-pHNaF_sat -->


    <owl:NamedIndividual rdf:about="http://w3id.org/glosis/model/procedure/pHProcedure-pHNaF_sat">
        <rdf:type rdf:resource="http://w3id.org/glosis/model/procedure/PHProcedure"/>
        <rdf:type rdf:resource="http://www.w3.org/2004/02/skos/core#Concept"/>
        <skos:broader rdf:resource="http://w3id.org/glosis/model/procedure/pHProcedure-pHNaF"/>
        <skos:definition>pHNaF (soil reaction) in saturated paste</skos:definition>
        <skos:inScheme rdf:resource="http://w3id.org/glosis/model/procedure/pHProcedure"/>
        <skos:notation>pHNaF_sat</skos:notation>
        <skos:prefLabel xml:lang="en">pHNaF_sat</skos:prefLabel>
        <skos:scopeNote rdf:resource="https://www.isric.org/sites/default/files/isric_report_2014_01.pdf"/>
        <skos:scopeNote>Leenaars J.G.B., A.J.M. van Oostrum and M. Ruiperez Gonzalez, 2014. Africa Soil Profiles Database, Version 1.2. A compilation of georeferenced and standardised legacy soil profile data for Sub-Saharan Africa (with dataset). ISRIC Report 2014/01. Africa Soil Information Service (AfSIS) project and ISRIC - World Soil Information, Wageningen, the Netherlands. See Annex 4.</skos:scopeNote>
    </owl:NamedIndividual>
    


    <!-- http://w3id.org/glosis/model/procedure/pSAProcedure -->


    <owl:NamedIndividual rdf:about="http://w3id.org/glosis/model/procedure/pSAProcedure">
        <rdf:type rdf:resource="http://www.w3.org/2004/02/skos/core#ConceptScheme"/>
        <rdfs:label xml:lang="en">Code list for pSA analysis procedures - codelist scheme</rdfs:label>
        <rdfs:seeAlso rdf:resource="http://w3id.org/glosis/model/procedure/PSAProcedure"/>
        <skos:definition>AfSP-derived interpretation (RwaSP)</skos:definition>
        <skos:note xml:lang="en">This code list provides analysis procedures for pSA.</skos:note>
        <skos:prefLabel xml:lang="en">Code list for pSA analysis procedures - codelist scheme</skos:prefLabel>
    </owl:NamedIndividual>
    


    <!-- http://w3id.org/glosis/model/procedure/pSAProcedure-beaker-disp -->


    <owl:NamedIndividual rdf:about="http://w3id.org/glosis/model/procedure/pSAProcedure-beaker-disp">
        <rdf:type rdf:resource="http://w3id.org/glosis/model/procedure/PSAProcedure"/>
        <rdf:type rdf:resource="http://www.w3.org/2004/02/skos/core#Concept"/>
        <skos:definition>Particle size analysis with beaker method with appropriate dispersion of the primary particles and pretreatment to remove cementing particles (organic matter, carbonates)</skos:definition>
        <skos:inScheme rdf:resource="http://w3id.org/glosis/model/procedure/pSAProcedure"/>
        <skos:notation>beaker-disp</skos:notation>
        <skos:prefLabel xml:lang="en">beaker-dispersion</skos:prefLabel>
        <skos:scopeNote rdf:resource="https://www.isric.org/sites/default/files/isric_report_2014_01.pdf"/>
        <skos:scopeNote>Leenaars J.G.B., A.J.M. van Oostrum and M. Ruiperez Gonzalez, 2014. Africa Soil Profiles Database, Version 1.2. A compilation of georeferenced and standardised legacy soil profile data for Sub-Saharan Africa (with dataset). ISRIC Report 2014/01. Africa Soil Information Service (AfSIS) project and ISRIC - World Soil Information, Wageningen, the Netherlands. See Annex 4.</skos:scopeNote>
        <skos:topConceptOf rdf:resource="http://w3id.org/glosis/model/procedure/pSAProcedure"/>
    </owl:NamedIndividual>
    


    <!-- http://w3id.org/glosis/model/procedure/pSAProcedure-beaker-disp-spec -->


    <owl:NamedIndividual rdf:about="http://w3id.org/glosis/model/procedure/pSAProcedure-beaker-disp-spec">
        <rdf:type rdf:resource="http://w3id.org/glosis/model/procedure/PSAProcedure"/>
        <rdf:type rdf:resource="http://www.w3.org/2004/02/skos/core#Concept"/>
        <skos:definition>Spectrally predicted based on measurments with the beaker method with appropriate dispersion of the primary particles and pretreatment to remove cementing particles (organic matter, carbonates)</skos:definition>
        <skos:inScheme rdf:resource="http://w3id.org/glosis/model/procedure/pSAProcedure"/>
        <skos:notation>beaker-disp-spec</skos:notation>
        <skos:prefLabel xml:lang="en">beaker-dispersion-spectral</skos:prefLabel>
        <skos:scopeNote rdf:resource="https://www.isric.org/sites/default/files/isric_report_2014_01.pdf"/>
        <skos:scopeNote>Leenaars J.G.B., A.J.M. van Oostrum and M. Ruiperez Gonzalez, 2014. Africa Soil Profiles Database, Version 1.2. A compilation of georeferenced and standardised legacy soil profile data for Sub-Saharan Africa (with dataset). ISRIC Report 2014/01. Africa Soil Information Service (AfSIS) project and ISRIC - World Soil Information, Wageningen, the Netherlands. See Annex 4.</skos:scopeNote>
        <skos:topConceptOf rdf:resource="http://w3id.org/glosis/model/procedure/pSAProcedure"/>
    </owl:NamedIndividual>
    


    <!-- http://w3id.org/glosis/model/procedure/pSAProcedure-beaker-nodisp -->


    <owl:NamedIndividual rdf:about="http://w3id.org/glosis/model/procedure/pSAProcedure-beaker-nodisp">
        <rdf:type rdf:resource="http://w3id.org/glosis/model/procedure/PSAProcedure"/>
        <rdf:type rdf:resource="http://www.w3.org/2004/02/skos/core#Concept"/>
        <skos:definition>Particle size analysis with beaker method with no dispersion of the primary particlesand pretreatment to remove cementing particles (organic matter, carbonates)</skos:definition>
        <skos:inScheme rdf:resource="http://w3id.org/glosis/model/procedure/pSAProcedure"/>
        <skos:notation>beaker-nodisp</skos:notation>
        <skos:prefLabel xml:lang="en">beaker-no_dispersion</skos:prefLabel>
        <skos:scopeNote rdf:resource="https://www.isric.org/sites/default/files/isric_report_2014_01.pdf"/>
        <skos:scopeNote>Leenaars J.G.B., A.J.M. van Oostrum and M. Ruiperez Gonzalez, 2014. Africa Soil Profiles Database, Version 1.2. A compilation of georeferenced and standardised legacy soil profile data for Sub-Saharan Africa (with dataset). ISRIC Report 2014/01. Africa Soil Information Service (AfSIS) project and ISRIC - World Soil Information, Wageningen, the Netherlands. See Annex 4.</skos:scopeNote>
        <skos:topConceptOf rdf:resource="http://w3id.org/glosis/model/procedure/pSAProcedure"/>
    </owl:NamedIndividual>
    


    <!-- http://w3id.org/glosis/model/procedure/pSAProcedure-beaker-nodisp-spec -->


    <owl:NamedIndividual rdf:about="http://w3id.org/glosis/model/procedure/pSAProcedure-beaker-nodisp-spec">
        <rdf:type rdf:resource="http://w3id.org/glosis/model/procedure/PSAProcedure"/>
        <rdf:type rdf:resource="http://www.w3.org/2004/02/skos/core#Concept"/>
        <skos:definition>Spectrally predicted based on measurments with the beaker method with no dispersion of the primary particles and pretreatment to remove cementing particles (organic matter, carbonates)</skos:definition>
        <skos:inScheme rdf:resource="http://w3id.org/glosis/model/procedure/pSAProcedure"/>
        <skos:notation>beaker-nodisp-spec</skos:notation>
        <skos:prefLabel xml:lang="en">beaker-no_dispersion-spectral</skos:prefLabel>
        <skos:scopeNote rdf:resource="https://www.isric.org/sites/default/files/isric_report_2014_01.pdf"/>
        <skos:scopeNote>Leenaars J.G.B., A.J.M. van Oostrum and M. Ruiperez Gonzalez, 2014. Africa Soil Profiles Database, Version 1.2. A compilation of georeferenced and standardised legacy soil profile data for Sub-Saharan Africa (with dataset). ISRIC Report 2014/01. Africa Soil Information Service (AfSIS) project and ISRIC - World Soil Information, Wageningen, the Netherlands. See Annex 4.</skos:scopeNote>
        <skos:topConceptOf rdf:resource="http://w3id.org/glosis/model/procedure/pSAProcedure"/>
    </owl:NamedIndividual>
    


    <!-- http://w3id.org/glosis/model/procedure/pSAProcedure-beaker-unkdisp -->


    <owl:NamedIndividual rdf:about="http://w3id.org/glosis/model/procedure/pSAProcedure-beaker-unkdisp">
        <rdf:type rdf:resource="http://w3id.org/glosis/model/procedure/PSAProcedure"/>
        <rdf:type rdf:resource="http://www.w3.org/2004/02/skos/core#Concept"/>
        <skos:definition>Particle size analysis with beaker method unknown dispersion of the primary particles and pretreatment to remove cementing particles (organic matter, carbonates)</skos:definition>
        <skos:inScheme rdf:resource="http://w3id.org/glosis/model/procedure/pSAProcedure"/>
        <skos:notation>beaker-unkdisp</skos:notation>
        <skos:prefLabel xml:lang="en">beaker-unknown_dispersion</skos:prefLabel>
        <skos:scopeNote rdf:resource="https://www.isric.org/sites/default/files/isric_report_2014_01.pdf"/>
        <skos:scopeNote>Leenaars J.G.B., A.J.M. van Oostrum and M. Ruiperez Gonzalez, 2014. Africa Soil Profiles Database, Version 1.2. A compilation of georeferenced and standardised legacy soil profile data for Sub-Saharan Africa (with dataset). ISRIC Report 2014/01. Africa Soil Information Service (AfSIS) project and ISRIC - World Soil Information, Wageningen, the Netherlands. See Annex 4.</skos:scopeNote>
        <skos:topConceptOf rdf:resource="http://w3id.org/glosis/model/procedure/pSAProcedure"/>
    </owl:NamedIndividual>
    


    <!-- http://w3id.org/glosis/model/procedure/pSAProcedure-beaker-unkdisp-spec -->


    <owl:NamedIndividual rdf:about="http://w3id.org/glosis/model/procedure/pSAProcedure-beaker-unkdisp-spec">
        <rdf:type rdf:resource="http://w3id.org/glosis/model/procedure/PSAProcedure"/>
        <rdf:type rdf:resource="http://www.w3.org/2004/02/skos/core#Concept"/>
        <skos:definition>Spectrally predicted based on measurments with the beaker method unknown dispersion of the primary particles and pretreatment to remove cementing particles (organic matter, carbonates)</skos:definition>
        <skos:inScheme rdf:resource="http://w3id.org/glosis/model/procedure/pSAProcedure"/>
        <skos:notation>beaker-unkdisp-spec</skos:notation>
        <skos:prefLabel xml:lang="en">beaker-unknown_dispersion-spectral</skos:prefLabel>
        <skos:scopeNote rdf:resource="https://www.isric.org/sites/default/files/isric_report_2014_01.pdf"/>
        <skos:scopeNote>Leenaars J.G.B., A.J.M. van Oostrum and M. Ruiperez Gonzalez, 2014. Africa Soil Profiles Database, Version 1.2. A compilation of georeferenced and standardised legacy soil profile data for Sub-Saharan Africa (with dataset). ISRIC Report 2014/01. Africa Soil Information Service (AfSIS) project and ISRIC - World Soil Information, Wageningen, the Netherlands. See Annex 4.</skos:scopeNote>
        <skos:topConceptOf rdf:resource="http://w3id.org/glosis/model/procedure/pSAProcedure"/>
    </owl:NamedIndividual>
    


    <!-- http://w3id.org/glosis/model/procedure/pSAProcedure-fldest -->


    <owl:NamedIndividual rdf:about="http://w3id.org/glosis/model/procedure/pSAProcedure-fldest">
        <rdf:type rdf:resource="http://w3id.org/glosis/model/procedure/PSAProcedure"/>
        <rdf:type rdf:resource="http://www.w3.org/2004/02/skos/core#Concept"/>
        <skos:definition>Field estimate of the particle size distribution, typically done by hand</skos:definition>
        <skos:inScheme rdf:resource="http://w3id.org/glosis/model/procedure/pSAProcedure"/>
        <skos:notation>fldest</skos:notation>
        <skos:prefLabel xml:lang="en">field estimate</skos:prefLabel>
        <skos:scopeNote rdf:resource="https://www.isric.org/sites/default/files/isric_report_2014_01.pdf"/>
        <skos:scopeNote>Leenaars J.G.B., A.J.M. van Oostrum and M. Ruiperez Gonzalez, 2014. Africa Soil Profiles Database, Version 1.2. A compilation of georeferenced and standardised legacy soil profile data for Sub-Saharan Africa (with dataset). ISRIC Report 2014/01. Africa Soil Information Service (AfSIS) project and ISRIC - World Soil Information, Wageningen, the Netherlands. See Annex 4.</skos:scopeNote>
        <skos:topConceptOf rdf:resource="http://w3id.org/glosis/model/procedure/pSAProcedure"/>
    </owl:NamedIndividual>
    


    <!-- http://w3id.org/glosis/model/procedure/pSAProcedure-hydrometer-disp -->


    <owl:NamedIndividual rdf:about="http://w3id.org/glosis/model/procedure/pSAProcedure-hydrometer-disp">
        <rdf:type rdf:resource="http://w3id.org/glosis/model/procedure/PSAProcedure"/>
        <rdf:type rdf:resource="http://www.w3.org/2004/02/skos/core#Concept"/>
        <skos:definition>Particle size analysis with hydrometer (bouyoucos) method with appropriate dispersion of the primary particles and pretreatment to remove cementing particles (organic matter, carbonates)</skos:definition>
        <skos:inScheme rdf:resource="http://w3id.org/glosis/model/procedure/pSAProcedure"/>
        <skos:notation>hydrometer-disp</skos:notation>
        <skos:prefLabel xml:lang="en">hydrometer (bouyoucos)-dispersion</skos:prefLabel>
        <skos:scopeNote rdf:resource="https://www.isric.org/sites/default/files/isric_report_2014_01.pdf"/>
        <skos:scopeNote>Leenaars J.G.B., A.J.M. van Oostrum and M. Ruiperez Gonzalez, 2014. Africa Soil Profiles Database, Version 1.2. A compilation of georeferenced and standardised legacy soil profile data for Sub-Saharan Africa (with dataset). ISRIC Report 2014/01. Africa Soil Information Service (AfSIS) project and ISRIC - World Soil Information, Wageningen, the Netherlands. See Annex 4.</skos:scopeNote>
        <skos:topConceptOf rdf:resource="http://w3id.org/glosis/model/procedure/pSAProcedure"/>
    </owl:NamedIndividual>
    


    <!-- http://w3id.org/glosis/model/procedure/pSAProcedure-hydrometer-disp-spec -->


    <owl:NamedIndividual rdf:about="http://w3id.org/glosis/model/procedure/pSAProcedure-hydrometer-disp-spec">
        <rdf:type rdf:resource="http://w3id.org/glosis/model/procedure/PSAProcedure"/>
        <rdf:type rdf:resource="http://www.w3.org/2004/02/skos/core#Concept"/>
        <skos:definition>Spectrally predicted based on measurments with the hydrometer (bouyoucos) method with appropriate dispersion of the primary particles and pretreatment to remove cementing particles (organic matter, carbonates)</skos:definition>
        <skos:inScheme rdf:resource="http://w3id.org/glosis/model/procedure/pSAProcedure"/>
        <skos:notation>hydrometer-disp-spec</skos:notation>
        <skos:prefLabel xml:lang="en">hydrometer (bouyoucos)-dispersion-spectral</skos:prefLabel>
        <skos:scopeNote rdf:resource="https://www.isric.org/sites/default/files/isric_report_2014_01.pdf"/>
        <skos:scopeNote>Leenaars J.G.B., A.J.M. van Oostrum and M. Ruiperez Gonzalez, 2014. Africa Soil Profiles Database, Version 1.2. A compilation of georeferenced and standardised legacy soil profile data for Sub-Saharan Africa (with dataset). ISRIC Report 2014/01. Africa Soil Information Service (AfSIS) project and ISRIC - World Soil Information, Wageningen, the Netherlands. See Annex 4.</skos:scopeNote>
        <skos:topConceptOf rdf:resource="http://w3id.org/glosis/model/procedure/pSAProcedure"/>
    </owl:NamedIndividual>
    


    <!-- http://w3id.org/glosis/model/procedure/pSAProcedure-hydrometer-nodisp -->


    <owl:NamedIndividual rdf:about="http://w3id.org/glosis/model/procedure/pSAProcedure-hydrometer-nodisp">
        <rdf:type rdf:resource="http://w3id.org/glosis/model/procedure/PSAProcedure"/>
        <rdf:type rdf:resource="http://www.w3.org/2004/02/skos/core#Concept"/>
        <skos:definition>Particle size analysis with hydrometer (bouyoucos) method with no dispersion of the primary particles and removal of cementing particles (organic matter, carbonates)</skos:definition>
        <skos:inScheme rdf:resource="http://w3id.org/glosis/model/procedure/pSAProcedure"/>
        <skos:notation>hydrometer-nodisp</skos:notation>
        <skos:prefLabel xml:lang="en">hydrometer (bouyoucos)-no_dispersion</skos:prefLabel>
        <skos:scopeNote rdf:resource="https://www.isric.org/sites/default/files/isric_report_2014_01.pdf"/>
        <skos:scopeNote>Leenaars J.G.B., A.J.M. van Oostrum and M. Ruiperez Gonzalez, 2014. Africa Soil Profiles Database, Version 1.2. A compilation of georeferenced and standardised legacy soil profile data for Sub-Saharan Africa (with dataset). ISRIC Report 2014/01. Africa Soil Information Service (AfSIS) project and ISRIC - World Soil Information, Wageningen, the Netherlands. See Annex 4.</skos:scopeNote>
        <skos:topConceptOf rdf:resource="http://w3id.org/glosis/model/procedure/pSAProcedure"/>
    </owl:NamedIndividual>
    


    <!-- http://w3id.org/glosis/model/procedure/pSAProcedure-hydrometer-nodisp-spec -->


    <owl:NamedIndividual rdf:about="http://w3id.org/glosis/model/procedure/pSAProcedure-hydrometer-nodisp-spec">
        <rdf:type rdf:resource="http://w3id.org/glosis/model/procedure/PSAProcedure"/>
        <rdf:type rdf:resource="http://www.w3.org/2004/02/skos/core#Concept"/>
        <skos:definition>Spectrally predicted based on measurments with the hydrometer (bouyoucos) method with no dispersion of the primary particles and pretreatment to remove cementing particles (organic matter, carbonates)</skos:definition>
        <skos:inScheme rdf:resource="http://w3id.org/glosis/model/procedure/pSAProcedure"/>
        <skos:notation>hydrometer-nodisp-spec</skos:notation>
        <skos:prefLabel xml:lang="en">hydrometer (bouyoucos)-no_dispersion-spectral</skos:prefLabel>
        <skos:scopeNote rdf:resource="https://www.isric.org/sites/default/files/isric_report_2014_01.pdf"/>
        <skos:scopeNote>Leenaars J.G.B., A.J.M. van Oostrum and M. Ruiperez Gonzalez, 2014. Africa Soil Profiles Database, Version 1.2. A compilation of georeferenced and standardised legacy soil profile data for Sub-Saharan Africa (with dataset). ISRIC Report 2014/01. Africa Soil Information Service (AfSIS) project and ISRIC - World Soil Information, Wageningen, the Netherlands. See Annex 4.</skos:scopeNote>
        <skos:topConceptOf rdf:resource="http://w3id.org/glosis/model/procedure/pSAProcedure"/>
    </owl:NamedIndividual>
    


    <!-- http://w3id.org/glosis/model/procedure/pSAProcedure-hydrometer-unkdisp -->


    <owl:NamedIndividual rdf:about="http://w3id.org/glosis/model/procedure/pSAProcedure-hydrometer-unkdisp">
        <rdf:type rdf:resource="http://w3id.org/glosis/model/procedure/PSAProcedure"/>
        <rdf:type rdf:resource="http://www.w3.org/2004/02/skos/core#Concept"/>
        <skos:definition>Particle size analysis with hydrometer (bouyoucos) method unknown dispersion of the primary particles and pretreatment to remove cementing particles (organic matter, carbonates)</skos:definition>
        <skos:inScheme rdf:resource="http://w3id.org/glosis/model/procedure/pSAProcedure"/>
        <skos:notation>hydrometer-unkdisp</skos:notation>
        <skos:prefLabel xml:lang="en">hydrometer (bouyoucos)-unknown_dispersion</skos:prefLabel>
        <skos:scopeNote rdf:resource="https://www.isric.org/sites/default/files/isric_report_2014_01.pdf"/>
        <skos:scopeNote>Leenaars J.G.B., A.J.M. van Oostrum and M. Ruiperez Gonzalez, 2014. Africa Soil Profiles Database, Version 1.2. A compilation of georeferenced and standardised legacy soil profile data for Sub-Saharan Africa (with dataset). ISRIC Report 2014/01. Africa Soil Information Service (AfSIS) project and ISRIC - World Soil Information, Wageningen, the Netherlands. See Annex 4.</skos:scopeNote>
        <skos:topConceptOf rdf:resource="http://w3id.org/glosis/model/procedure/pSAProcedure"/>
    </owl:NamedIndividual>
    


    <!-- http://w3id.org/glosis/model/procedure/pSAProcedure-hydrometer-unkdisp-spec -->


    <owl:NamedIndividual rdf:about="http://w3id.org/glosis/model/procedure/pSAProcedure-hydrometer-unkdisp-spec">
        <rdf:type rdf:resource="http://w3id.org/glosis/model/procedure/PSAProcedure"/>
        <rdf:type rdf:resource="http://www.w3.org/2004/02/skos/core#Concept"/>
        <skos:definition>Spectrally predicted based on measurments with the hydrometer (bouyoucos) method unknown dispersion of the primary particles and pretreatment to remove cementing particles (organic matter, carbonates)</skos:definition>
        <skos:inScheme rdf:resource="http://w3id.org/glosis/model/procedure/pSAProcedure"/>
        <skos:notation>hydrometer-unkdisp-spec</skos:notation>
        <skos:prefLabel xml:lang="en">hydrometer (bouyoucos)-unknown_dispersion-spectral</skos:prefLabel>
        <skos:scopeNote rdf:resource="https://www.isric.org/sites/default/files/isric_report_2014_01.pdf"/>
        <skos:scopeNote>Leenaars J.G.B., A.J.M. van Oostrum and M. Ruiperez Gonzalez, 2014. Africa Soil Profiles Database, Version 1.2. A compilation of georeferenced and standardised legacy soil profile data for Sub-Saharan Africa (with dataset). ISRIC Report 2014/01. Africa Soil Information Service (AfSIS) project and ISRIC - World Soil Information, Wageningen, the Netherlands. See Annex 4.</skos:scopeNote>
        <skos:topConceptOf rdf:resource="http://w3id.org/glosis/model/procedure/pSAProcedure"/>
    </owl:NamedIndividual>
    


    <!-- http://w3id.org/glosis/model/procedure/pSAProcedure-laser-disp -->


    <owl:NamedIndividual rdf:about="http://w3id.org/glosis/model/procedure/pSAProcedure-laser-disp">
        <rdf:type rdf:resource="http://w3id.org/glosis/model/procedure/PSAProcedure"/>
        <rdf:type rdf:resource="http://www.w3.org/2004/02/skos/core#Concept"/>
        <skos:definition>Particle size analysis with laser diffraction with appropriate disperson of the primary particles and pretreatment to remove cementing particles (organic matter, carbonates)</skos:definition>
        <skos:inScheme rdf:resource="http://w3id.org/glosis/model/procedure/pSAProcedure"/>
        <skos:notation>laser-disp</skos:notation>
        <skos:prefLabel xml:lang="en">laser diffraction-dispersion</skos:prefLabel>
        <skos:scopeNote rdf:resource="https://www.isric.org/sites/default/files/isric_report_2014_01.pdf"/>
        <skos:scopeNote>Leenaars J.G.B., A.J.M. van Oostrum and M. Ruiperez Gonzalez, 2014. Africa Soil Profiles Database, Version 1.2. A compilation of georeferenced and standardised legacy soil profile data for Sub-Saharan Africa (with dataset). ISRIC Report 2014/01. Africa Soil Information Service (AfSIS) project and ISRIC - World Soil Information, Wageningen, the Netherlands. See Annex 4.</skos:scopeNote>
        <skos:topConceptOf rdf:resource="http://w3id.org/glosis/model/procedure/pSAProcedure"/>
    </owl:NamedIndividual>
    


    <!-- http://w3id.org/glosis/model/procedure/pSAProcedure-laser-disp-spec -->


    <owl:NamedIndividual rdf:about="http://w3id.org/glosis/model/procedure/pSAProcedure-laser-disp-spec">
        <rdf:type rdf:resource="http://w3id.org/glosis/model/procedure/PSAProcedure"/>
        <rdf:type rdf:resource="http://www.w3.org/2004/02/skos/core#Concept"/>
        <skos:definition>Spectrally predicted based on measurments with laser diffraction analysis with appropriate disperson of the primary particles and pretreatment to remove cementing particles (organic matter, carbonates)</skos:definition>
        <skos:inScheme rdf:resource="http://w3id.org/glosis/model/procedure/pSAProcedure"/>
        <skos:notation>laser-disp-spec</skos:notation>
        <skos:prefLabel xml:lang="en">laser diffraction-dispersion-spectral</skos:prefLabel>
        <skos:scopeNote rdf:resource="https://www.isric.org/sites/default/files/isric_report_2014_01.pdf"/>
        <skos:scopeNote>Leenaars J.G.B., A.J.M. van Oostrum and M. Ruiperez Gonzalez, 2014. Africa Soil Profiles Database, Version 1.2. A compilation of georeferenced and standardised legacy soil profile data for Sub-Saharan Africa (with dataset). ISRIC Report 2014/01. Africa Soil Information Service (AfSIS) project and ISRIC - World Soil Information, Wageningen, the Netherlands. See Annex 4.</skos:scopeNote>
        <skos:topConceptOf rdf:resource="http://w3id.org/glosis/model/procedure/pSAProcedure"/>
    </owl:NamedIndividual>
    


    <!-- http://w3id.org/glosis/model/procedure/pSAProcedure-laser-nodisp -->


    <owl:NamedIndividual rdf:about="http://w3id.org/glosis/model/procedure/pSAProcedure-laser-nodisp">
        <rdf:type rdf:resource="http://w3id.org/glosis/model/procedure/PSAProcedure"/>
        <rdf:type rdf:resource="http://www.w3.org/2004/02/skos/core#Concept"/>
        <skos:definition>Particle size analysis with laser diffraction with no dispersion of the primary particles and pretreatment to remove cementing particles (organic matter, carbonates)</skos:definition>
        <skos:inScheme rdf:resource="http://w3id.org/glosis/model/procedure/pSAProcedure"/>
        <skos:notation>laser-nodisp</skos:notation>
        <skos:prefLabel xml:lang="en">laser diffraction-no_dispersion</skos:prefLabel>
        <skos:scopeNote rdf:resource="https://www.isric.org/sites/default/files/isric_report_2014_01.pdf"/>
        <skos:scopeNote>Leenaars J.G.B., A.J.M. van Oostrum and M. Ruiperez Gonzalez, 2014. Africa Soil Profiles Database, Version 1.2. A compilation of georeferenced and standardised legacy soil profile data for Sub-Saharan Africa (with dataset). ISRIC Report 2014/01. Africa Soil Information Service (AfSIS) project and ISRIC - World Soil Information, Wageningen, the Netherlands. See Annex 4.</skos:scopeNote>
        <skos:topConceptOf rdf:resource="http://w3id.org/glosis/model/procedure/pSAProcedure"/>
    </owl:NamedIndividual>
    


    <!-- http://w3id.org/glosis/model/procedure/pSAProcedure-laser-nodisp-spec -->


    <owl:NamedIndividual rdf:about="http://w3id.org/glosis/model/procedure/pSAProcedure-laser-nodisp-spec">
        <rdf:type rdf:resource="http://w3id.org/glosis/model/procedure/PSAProcedure"/>
        <rdf:type rdf:resource="http://www.w3.org/2004/02/skos/core#Concept"/>
        <skos:definition>Spectrally predicted based on measurments with laser diffraction analysis with no dispersion of the primary particles and pretreatment to remove cementing particles (organic matter, carbonates)</skos:definition>
        <skos:inScheme rdf:resource="http://w3id.org/glosis/model/procedure/pSAProcedure"/>
        <skos:notation>laser-nodisp-spec</skos:notation>
        <skos:prefLabel xml:lang="en">laser diffraction-no_dispersion-spectral</skos:prefLabel>
        <skos:scopeNote rdf:resource="https://www.isric.org/sites/default/files/isric_report_2014_01.pdf"/>
        <skos:scopeNote>Leenaars J.G.B., A.J.M. van Oostrum and M. Ruiperez Gonzalez, 2014. Africa Soil Profiles Database, Version 1.2. A compilation of georeferenced and standardised legacy soil profile data for Sub-Saharan Africa (with dataset). ISRIC Report 2014/01. Africa Soil Information Service (AfSIS) project and ISRIC - World Soil Information, Wageningen, the Netherlands. See Annex 4.</skos:scopeNote>
        <skos:topConceptOf rdf:resource="http://w3id.org/glosis/model/procedure/pSAProcedure"/>
    </owl:NamedIndividual>
    


    <!-- http://w3id.org/glosis/model/procedure/pSAProcedure-laser-unkdisp -->


    <owl:NamedIndividual rdf:about="http://w3id.org/glosis/model/procedure/pSAProcedure-laser-unkdisp">
        <rdf:type rdf:resource="http://w3id.org/glosis/model/procedure/PSAProcedure"/>
        <rdf:type rdf:resource="http://www.w3.org/2004/02/skos/core#Concept"/>
        <skos:definition>Particle size analysis with laser diffraction with unknown dispersion of the primary particles and pretreatment to remove cementing particles (organic matter, carbonates)</skos:definition>
        <skos:inScheme rdf:resource="http://w3id.org/glosis/model/procedure/pSAProcedure"/>
        <skos:notation>laser-unkdisp</skos:notation>
        <skos:prefLabel xml:lang="en">laser diffraction-unknown_dispersion</skos:prefLabel>
        <skos:scopeNote rdf:resource="https://www.isric.org/sites/default/files/isric_report_2014_01.pdf"/>
        <skos:scopeNote>Leenaars J.G.B., A.J.M. van Oostrum and M. Ruiperez Gonzalez, 2014. Africa Soil Profiles Database, Version 1.2. A compilation of georeferenced and standardised legacy soil profile data for Sub-Saharan Africa (with dataset). ISRIC Report 2014/01. Africa Soil Information Service (AfSIS) project and ISRIC - World Soil Information, Wageningen, the Netherlands. See Annex 4.</skos:scopeNote>
        <skos:topConceptOf rdf:resource="http://w3id.org/glosis/model/procedure/pSAProcedure"/>
    </owl:NamedIndividual>
    


    <!-- http://w3id.org/glosis/model/procedure/pSAProcedure-laser-unkdisp-spec -->


    <owl:NamedIndividual rdf:about="http://w3id.org/glosis/model/procedure/pSAProcedure-laser-unkdisp-spec">
        <rdf:type rdf:resource="http://w3id.org/glosis/model/procedure/PSAProcedure"/>
        <rdf:type rdf:resource="http://www.w3.org/2004/02/skos/core#Concept"/>
        <skos:definition>Spectrally predicted based on measurments with laser diffraction analysis with unknown dispersion of the primary particles and pretreatment to remove cementing particles (organic matter, carbonates)</skos:definition>
        <skos:inScheme rdf:resource="http://w3id.org/glosis/model/procedure/pSAProcedure"/>
        <skos:notation>laser-unkdisp-spec</skos:notation>
        <skos:prefLabel xml:lang="en">laser diffraction-unknown_dispersion-spectral</skos:prefLabel>
        <skos:scopeNote rdf:resource="https://www.isric.org/sites/default/files/isric_report_2014_01.pdf"/>
        <skos:scopeNote>Leenaars J.G.B., A.J.M. van Oostrum and M. Ruiperez Gonzalez, 2014. Africa Soil Profiles Database, Version 1.2. A compilation of georeferenced and standardised legacy soil profile data for Sub-Saharan Africa (with dataset). ISRIC Report 2014/01. Africa Soil Information Service (AfSIS) project and ISRIC - World Soil Information, Wageningen, the Netherlands. See Annex 4.</skos:scopeNote>
        <skos:topConceptOf rdf:resource="http://w3id.org/glosis/model/procedure/pSAProcedure"/>
    </owl:NamedIndividual>
    


    <!-- http://w3id.org/glosis/model/procedure/pSAProcedure-pipette-disp -->


    <owl:NamedIndividual rdf:about="http://w3id.org/glosis/model/procedure/pSAProcedure-pipette-disp">
        <rdf:type rdf:resource="http://w3id.org/glosis/model/procedure/PSAProcedure"/>
        <rdf:type rdf:resource="http://www.w3.org/2004/02/skos/core#Concept"/>
        <skos:definition>Particle size analysis with pipette method with appropriate dispersion of the primary particles and pretreatment to remove cementing particles (organic matter, carbonates)</skos:definition>
        <skos:inScheme rdf:resource="http://w3id.org/glosis/model/procedure/pSAProcedure"/>
        <skos:notation>pipette-disp</skos:notation>
        <skos:prefLabel xml:lang="en">pipette-dispersion</skos:prefLabel>
        <skos:scopeNote rdf:resource="https://www.isric.org/sites/default/files/isric_report_2014_01.pdf"/>
        <skos:scopeNote>Leenaars J.G.B., A.J.M. van Oostrum and M. Ruiperez Gonzalez, 2014. Africa Soil Profiles Database, Version 1.2. A compilation of georeferenced and standardised legacy soil profile data for Sub-Saharan Africa (with dataset). ISRIC Report 2014/01. Africa Soil Information Service (AfSIS) project and ISRIC - World Soil Information, Wageningen, the Netherlands. See Annex 4.</skos:scopeNote>
        <skos:topConceptOf rdf:resource="http://w3id.org/glosis/model/procedure/pSAProcedure"/>
    </owl:NamedIndividual>
    


    <!-- http://w3id.org/glosis/model/procedure/pSAProcedure-pipette-disp-spec -->


    <owl:NamedIndividual rdf:about="http://w3id.org/glosis/model/procedure/pSAProcedure-pipette-disp-spec">
        <rdf:type rdf:resource="http://w3id.org/glosis/model/procedure/PSAProcedure"/>
        <rdf:type rdf:resource="http://www.w3.org/2004/02/skos/core#Concept"/>
        <skos:definition>Spectrally predicted based on measurments with the pipette method with appropriate dispersion of the primary particles and pretreatment to remove cementing particles (organic matter, carbonates)</skos:definition>
        <skos:inScheme rdf:resource="http://w3id.org/glosis/model/procedure/pSAProcedure"/>
        <skos:notation>pipette-disp-spec</skos:notation>
        <skos:prefLabel xml:lang="en">pipette-dispersion-spectral</skos:prefLabel>
        <skos:scopeNote rdf:resource="https://www.isric.org/sites/default/files/isric_report_2014_01.pdf"/>
        <skos:scopeNote>Leenaars J.G.B., A.J.M. van Oostrum and M. Ruiperez Gonzalez, 2014. Africa Soil Profiles Database, Version 1.2. A compilation of georeferenced and standardised legacy soil profile data for Sub-Saharan Africa (with dataset). ISRIC Report 2014/01. Africa Soil Information Service (AfSIS) project and ISRIC - World Soil Information, Wageningen, the Netherlands. See Annex 4.</skos:scopeNote>
        <skos:topConceptOf rdf:resource="http://w3id.org/glosis/model/procedure/pSAProcedure"/>
    </owl:NamedIndividual>
    


    <!-- http://w3id.org/glosis/model/procedure/pSAProcedure-pipette-nodisp -->


    <owl:NamedIndividual rdf:about="http://w3id.org/glosis/model/procedure/pSAProcedure-pipette-nodisp">
        <rdf:type rdf:resource="http://w3id.org/glosis/model/procedure/PSAProcedure"/>
        <rdf:type rdf:resource="http://www.w3.org/2004/02/skos/core#Concept"/>
        <skos:definition>Particle size analysis with pipette method with no dispersion of the primary particles and pretreatment to remove cementing particles (organic matter, carbonates)</skos:definition>
        <skos:inScheme rdf:resource="http://w3id.org/glosis/model/procedure/pSAProcedure"/>
        <skos:notation>pipette-nodisp</skos:notation>
        <skos:prefLabel xml:lang="en">pipette-no_dispersion</skos:prefLabel>
        <skos:scopeNote rdf:resource="https://www.isric.org/sites/default/files/isric_report_2014_01.pdf"/>
        <skos:scopeNote>Leenaars J.G.B., A.J.M. van Oostrum and M. Ruiperez Gonzalez, 2014. Africa Soil Profiles Database, Version 1.2. A compilation of georeferenced and standardised legacy soil profile data for Sub-Saharan Africa (with dataset). ISRIC Report 2014/01. Africa Soil Information Service (AfSIS) project and ISRIC - World Soil Information, Wageningen, the Netherlands. See Annex 4.</skos:scopeNote>
        <skos:topConceptOf rdf:resource="http://w3id.org/glosis/model/procedure/pSAProcedure"/>
    </owl:NamedIndividual>
    


    <!-- http://w3id.org/glosis/model/procedure/pSAProcedure-pipette-nodisp-spec -->


    <owl:NamedIndividual rdf:about="http://w3id.org/glosis/model/procedure/pSAProcedure-pipette-nodisp-spec">
        <rdf:type rdf:resource="http://w3id.org/glosis/model/procedure/PSAProcedure"/>
        <rdf:type rdf:resource="http://www.w3.org/2004/02/skos/core#Concept"/>
        <skos:definition>Spectrally predicted based on measurments with the pipette method with no dispersion of the primary particles and pretreatment to remove cementing particles (organic matter, carbonates)</skos:definition>
        <skos:inScheme rdf:resource="http://w3id.org/glosis/model/procedure/pSAProcedure"/>
        <skos:notation>pipette-nodisp-spec</skos:notation>
        <skos:prefLabel xml:lang="en">pipette-no_dispersion-spectral</skos:prefLabel>
        <skos:scopeNote rdf:resource="https://www.isric.org/sites/default/files/isric_report_2014_01.pdf"/>
        <skos:scopeNote>Leenaars J.G.B., A.J.M. van Oostrum and M. Ruiperez Gonzalez, 2014. Africa Soil Profiles Database, Version 1.2. A compilation of georeferenced and standardised legacy soil profile data for Sub-Saharan Africa (with dataset). ISRIC Report 2014/01. Africa Soil Information Service (AfSIS) project and ISRIC - World Soil Information, Wageningen, the Netherlands. See Annex 4.</skos:scopeNote>
        <skos:topConceptOf rdf:resource="http://w3id.org/glosis/model/procedure/pSAProcedure"/>
    </owl:NamedIndividual>
    


    <!-- http://w3id.org/glosis/model/procedure/pSAProcedure-pipette-unkdisp -->


    <owl:NamedIndividual rdf:about="http://w3id.org/glosis/model/procedure/pSAProcedure-pipette-unkdisp">
        <rdf:type rdf:resource="http://w3id.org/glosis/model/procedure/PSAProcedure"/>
        <rdf:type rdf:resource="http://www.w3.org/2004/02/skos/core#Concept"/>
        <skos:definition>Particle size analysis with pipette method unknown dispersion of the primary particles and pretreatment to remove cementing particles (organic matter, carbonates)</skos:definition>
        <skos:inScheme rdf:resource="http://w3id.org/glosis/model/procedure/pSAProcedure"/>
        <skos:notation>pipette-unkdisp</skos:notation>
        <skos:prefLabel xml:lang="en">pipette-unknown_dispersion</skos:prefLabel>
        <skos:scopeNote rdf:resource="https://www.isric.org/sites/default/files/isric_report_2014_01.pdf"/>
        <skos:scopeNote>Leenaars J.G.B., A.J.M. van Oostrum and M. Ruiperez Gonzalez, 2014. Africa Soil Profiles Database, Version 1.2. A compilation of georeferenced and standardised legacy soil profile data for Sub-Saharan Africa (with dataset). ISRIC Report 2014/01. Africa Soil Information Service (AfSIS) project and ISRIC - World Soil Information, Wageningen, the Netherlands. See Annex 4.</skos:scopeNote>
        <skos:topConceptOf rdf:resource="http://w3id.org/glosis/model/procedure/pSAProcedure"/>
    </owl:NamedIndividual>
    


    <!-- http://w3id.org/glosis/model/procedure/pSAProcedure-pipette-unkdisp-spec -->


    <owl:NamedIndividual rdf:about="http://w3id.org/glosis/model/procedure/pSAProcedure-pipette-unkdisp-spec">
        <rdf:type rdf:resource="http://w3id.org/glosis/model/procedure/PSAProcedure"/>
        <rdf:type rdf:resource="http://www.w3.org/2004/02/skos/core#Concept"/>
        <skos:definition>Spectrally predicted based on measurments with the pipette method unknown dispersion of the primary particles and pretreatment to remove cementing particles (organic matter, carbonates)</skos:definition>
        <skos:inScheme rdf:resource="http://w3id.org/glosis/model/procedure/pSAProcedure"/>
        <skos:notation>pipette-unkdisp-spec</skos:notation>
        <skos:prefLabel xml:lang="en">pipette-unknown_dispersion-spectral</skos:prefLabel>
        <skos:scopeNote rdf:resource="https://www.isric.org/sites/default/files/isric_report_2014_01.pdf"/>
        <skos:scopeNote>Leenaars J.G.B., A.J.M. van Oostrum and M. Ruiperez Gonzalez, 2014. Africa Soil Profiles Database, Version 1.2. A compilation of georeferenced and standardised legacy soil profile data for Sub-Saharan Africa (with dataset). ISRIC Report 2014/01. Africa Soil Information Service (AfSIS) project and ISRIC - World Soil Information, Wageningen, the Netherlands. See Annex 4.</skos:scopeNote>
        <skos:topConceptOf rdf:resource="http://w3id.org/glosis/model/procedure/pSAProcedure"/>
    </owl:NamedIndividual>
    


    <!-- http://w3id.org/glosis/model/procedure/phosphorusRetentionProcedure -->


    <owl:NamedIndividual rdf:about="http://w3id.org/glosis/model/procedure/phosphorusRetentionProcedure">
        <rdf:type rdf:resource="http://www.w3.org/2004/02/skos/core#ConceptScheme"/>
        <rdfs:label xml:lang="en">Code list for phosphorusRetention analysis procedures - codelist scheme</rdfs:label>
        <rdfs:seeAlso rdf:resource="http://w3id.org/glosis/model/procedure/PhosphorusRetentionProcedure"/>
        <skos:definition>AfSP-derived interpretation (RwaSP)</skos:definition>
        <skos:note xml:lang="en">This code list provides analysis procedures for phosphorusRetention.</skos:note>
        <skos:prefLabel xml:lang="en">Code list for phosphorusRetention analysis procedures - codelist scheme</skos:prefLabel>
    </owl:NamedIndividual>
    


    <!-- http://w3id.org/glosis/model/procedure/phosphorusRetentionProcedure-RetentP_blakemore -->


    <owl:NamedIndividual rdf:about="http://w3id.org/glosis/model/procedure/phosphorusRetentionProcedure-RetentP_blakemore">
        <rdf:type rdf:resource="http://w3id.org/glosis/model/procedure/PhosphorusRetentionProcedure"/>
        <rdf:type rdf:resource="http://www.w3.org/2004/02/skos/core#Concept"/>
        <skos:definition>P retention at ~pH4.6  (acc. Blakemore 1987)</skos:definition>
        <skos:inScheme rdf:resource="http://w3id.org/glosis/model/procedure/phosphorusRetentionProcedure"/>
        <skos:notation>RetentP_blakemore</skos:notation>
        <skos:prefLabel xml:lang="en">RetentP_blakemor</skos:prefLabel>
        <skos:scopeNote>Blakemore L.C. Searle P.L. and Daly, B.K. (1987) Methods for chemical analysis of soils. NZ Soil Bureau, Lower Hutt, New Zealand.</skos:scopeNote>
        <skos:topConceptOf rdf:resource="http://w3id.org/glosis/model/procedure/phosphorusRetentionProcedure"/>
    </owl:NamedIndividual>
    


    <!-- http://w3id.org/glosis/model/procedure/phosphorusRetentionProcedure-RetentP_unkn-spec -->


    <owl:NamedIndividual rdf:about="http://w3id.org/glosis/model/procedure/phosphorusRetentionProcedure-RetentP_unkn-spec">
        <rdf:type rdf:resource="http://w3id.org/glosis/model/procedure/PhosphorusRetentionProcedure"/>
        <rdf:type rdf:resource="http://www.w3.org/2004/02/skos/core#Concept"/>
        <skos:definition>Spectrally measured and converted to P retention (P buffer index)</skos:definition>
        <skos:inScheme rdf:resource="http://w3id.org/glosis/model/procedure/phosphorusRetentionProcedure"/>
        <skos:notation>RetentP_unkn-spec</skos:notation>
        <skos:prefLabel xml:lang="en">RetentP_unkn-spec</skos:prefLabel>
        <skos:scopeNote rdf:resource="https://www.isric.org/sites/default/files/isric_report_2014_01.pdf"/>
        <skos:scopeNote>Leenaars J.G.B., A.J.M. van Oostrum and M. Ruiperez Gonzalez, 2014. Africa Soil Profiles Database, Version 1.2. A compilation of georeferenced and standardised legacy soil profile data for Sub-Saharan Africa (with dataset). ISRIC Report 2014/01. Africa Soil Information Service (AfSIS) project and ISRIC - World Soil Information, Wageningen, the Netherlands. See Annex 4.</skos:scopeNote>
        <skos:topConceptOf rdf:resource="http://w3id.org/glosis/model/procedure/phosphorusRetentionProcedure"/>
    </owl:NamedIndividual>
    


    <!-- http://w3id.org/glosis/model/procedure/porosityProcedure -->


    <owl:NamedIndividual rdf:about="http://w3id.org/glosis/model/procedure/porosityProcedure">
        <rdf:type rdf:resource="http://www.w3.org/2004/02/skos/core#ConceptScheme"/>
        <rdfs:label xml:lang="en">Code list for porosity analysis procedures - codelist scheme</rdfs:label>
        <rdfs:seeAlso rdf:resource="http://w3id.org/glosis/model/procedure/PorosityProcedure"/>
        <skos:definition>AfSP-derived interpretation (RwaSP)</skos:definition>
        <skos:note xml:lang="en">This code list provides analysis procedures for porosity.</skos:note>
        <skos:prefLabel xml:lang="en">Code list for porosity analysis procedures - codelist scheme</skos:prefLabel>
    </owl:NamedIndividual>
    


    <!-- http://w3id.org/glosis/model/procedure/porosityProcedure-Poros_calcul-pf0 -->


    <owl:NamedIndividual rdf:about="http://w3id.org/glosis/model/procedure/porosityProcedure-Poros_calcul-pf0">
        <rdf:type rdf:resource="http://w3id.org/glosis/model/procedure/PorosityProcedure"/>
        <rdf:type rdf:resource="http://www.w3.org/2004/02/skos/core#Concept"/>
        <skos:definition>Porosity calculated from volumetric moisture content at pF 0 (1 cm)</skos:definition>
        <skos:inScheme rdf:resource="http://w3id.org/glosis/model/procedure/porosityProcedure"/>
        <skos:notation>Poros_calcul-pf0</skos:notation>
        <skos:prefLabel xml:lang="en">Poros_calcul-pf0</skos:prefLabel>
        <skos:scopeNote rdf:resource="https://www.isric.org/sites/default/files/isric_report_2014_01.pdf"/>
        <skos:scopeNote>Leenaars J.G.B., A.J.M. van Oostrum and M. Ruiperez Gonzalez, 2014. Africa Soil Profiles Database, Version 1.2. A compilation of georeferenced and standardised legacy soil profile data for Sub-Saharan Africa (with dataset). ISRIC Report 2014/01. Africa Soil Information Service (AfSIS) project and ISRIC - World Soil Information, Wageningen, the Netherlands. See Annex 4.</skos:scopeNote>
        <skos:topConceptOf rdf:resource="http://w3id.org/glosis/model/procedure/porosityProcedure"/>
    </owl:NamedIndividual>
    


    <!-- http://w3id.org/glosis/model/procedure/solubleSaltsProcedure -->


    <owl:NamedIndividual rdf:about="http://w3id.org/glosis/model/procedure/solubleSaltsProcedure">
        <rdf:type rdf:resource="http://www.w3.org/2004/02/skos/core#ConceptScheme"/>
        <rdfs:label xml:lang="en">Code list for solubleSalts analysis procedures - codelist scheme</rdfs:label>
        <rdfs:seeAlso rdf:resource="http://w3id.org/glosis/model/procedure/SolubleSaltsProcedure"/>
        <skos:definition>AfSP-derived interpretation (RwaSP)</skos:definition>
        <skos:note xml:lang="en">This code list provides analysis procedures for solubleSalts.</skos:note>
        <skos:prefLabel xml:lang="en">Code list for solubleSalts analysis procedures - codelist scheme</skos:prefLabel>
    </owl:NamedIndividual>
    


    <!-- http://w3id.org/glosis/model/procedure/solubleSaltsProcedure-SlbAn_calcul-unkn -->


    <owl:NamedIndividual rdf:about="http://w3id.org/glosis/model/procedure/solubleSaltsProcedure-SlbAn_calcul-unkn">
        <rdf:type rdf:resource="http://w3id.org/glosis/model/procedure/SolubleSaltsProcedure"/>
        <rdf:type rdf:resource="http://www.w3.org/2004/02/skos/core#Concept"/>
        <skos:definition>Sum of soluble anions (Cl, SO4, HCO2, CO3, NO3, F)</skos:definition>
        <skos:inScheme rdf:resource="http://w3id.org/glosis/model/procedure/solubleSaltsProcedure"/>
        <skos:notation>SlbAn_calcul-unkn</skos:notation>
        <skos:prefLabel xml:lang="en">SlbAn_calcul-unk</skos:prefLabel>
        <skos:scopeNote rdf:resource="https://www.isric.org/sites/default/files/isric_report_2014_01.pdf"/>
        <skos:scopeNote>Leenaars J.G.B., A.J.M. van Oostrum and M. Ruiperez Gonzalez, 2014. Africa Soil Profiles Database, Version 1.2. A compilation of georeferenced and standardised legacy soil profile data for Sub-Saharan Africa (with dataset). ISRIC Report 2014/01. Africa Soil Information Service (AfSIS) project and ISRIC - World Soil Information, Wageningen, the Netherlands. See Annex 4.</skos:scopeNote>
        <skos:topConceptOf rdf:resource="http://w3id.org/glosis/model/procedure/solubleSaltsProcedure"/>
    </owl:NamedIndividual>
    


    <!-- http://w3id.org/glosis/model/procedure/solubleSaltsProcedure-SlbCat_calcul-unkn -->


    <owl:NamedIndividual rdf:about="http://w3id.org/glosis/model/procedure/solubleSaltsProcedure-SlbCat_calcul-unkn">
        <rdf:type rdf:resource="http://w3id.org/glosis/model/procedure/SolubleSaltsProcedure"/>
        <rdf:type rdf:resource="http://www.w3.org/2004/02/skos/core#Concept"/>
        <skos:definition>Sum of soluble cations (Ca, Mg, K, Na)</skos:definition>
        <skos:inScheme rdf:resource="http://w3id.org/glosis/model/procedure/solubleSaltsProcedure"/>
        <skos:notation>SlbCat_calcul-unkn</skos:notation>
        <skos:prefLabel xml:lang="en">SlbCat_calcul-unk</skos:prefLabel>
        <skos:scopeNote rdf:resource="https://www.isric.org/sites/default/files/isric_report_2014_01.pdf"/>
        <skos:scopeNote>Leenaars J.G.B., A.J.M. van Oostrum and M. Ruiperez Gonzalez, 2014. Africa Soil Profiles Database, Version 1.2. A compilation of georeferenced and standardised legacy soil profile data for Sub-Saharan Africa (with dataset). ISRIC Report 2014/01. Africa Soil Information Service (AfSIS) project and ISRIC - World Soil Information, Wageningen, the Netherlands. See Annex 4.</skos:scopeNote>
        <skos:topConceptOf rdf:resource="http://w3id.org/glosis/model/procedure/solubleSaltsProcedure"/>
    </owl:NamedIndividual>
    


    <!-- http://w3id.org/glosis/model/procedure/textureSumProcedure -->


    <owl:NamedIndividual rdf:about="http://w3id.org/glosis/model/procedure/textureSumProcedure">
        <rdf:type rdf:resource="http://www.w3.org/2004/02/skos/core#ConceptScheme"/>
        <rdfs:label xml:lang="en">Code list for textureSum analysis procedures - codelist scheme</rdfs:label>
        <rdfs:seeAlso rdf:resource="http://w3id.org/glosis/model/procedure/TextureSumProcedure"/>
        <skos:definition>AfSP-derived interpretation (RwaSP)</skos:definition>
        <skos:note xml:lang="en">This code list provides analysis procedures for textureSum.</skos:note>
        <skos:prefLabel xml:lang="en">Code list for textureSum analysis procedures - codelist scheme</skos:prefLabel>
    </owl:NamedIndividual>
    


    <!-- http://w3id.org/glosis/model/procedure/textureSumProcedure-SumTxtr_calcul -->


    <owl:NamedIndividual rdf:about="http://w3id.org/glosis/model/procedure/textureSumProcedure-SumTxtr_calcul">
        <rdf:type rdf:resource="http://w3id.org/glosis/model/procedure/TextureSumProcedure"/>
        <rdf:type rdf:resource="http://www.w3.org/2004/02/skos/core#Concept"/>
        <skos:definition>Calculated sum of sand, silt and clay fractions</skos:definition>
        <skos:inScheme rdf:resource="http://w3id.org/glosis/model/procedure/textureSumProcedure"/>
        <skos:notation>SumTxtr_calcul</skos:notation>
        <skos:prefLabel xml:lang="en">SumTxtr_calcul</skos:prefLabel>
        <skos:scopeNote rdf:resource="https://www.isric.org/sites/default/files/isric_report_2014_01.pdf"/>
        <skos:scopeNote>Leenaars J.G.B., A.J.M. van Oostrum and M. Ruiperez Gonzalez, 2014. Africa Soil Profiles Database, Version 1.2. A compilation of georeferenced and standardised legacy soil profile data for Sub-Saharan Africa (with dataset). ISRIC Report 2014/01. Africa Soil Information Service (AfSIS) project and ISRIC - World Soil Information, Wageningen, the Netherlands. See Annex 4.</skos:scopeNote>
        <skos:topConceptOf rdf:resource="http://w3id.org/glosis/model/procedure/textureSumProcedure"/>
    </owl:NamedIndividual>
    


    <!-- http://w3id.org/glosis/model/procedure/totalCarbonateEquivalentProcedure -->


    <owl:NamedIndividual rdf:about="http://w3id.org/glosis/model/procedure/totalCarbonateEquivalentProcedure">
        <rdf:type rdf:resource="http://www.w3.org/2004/02/skos/core#ConceptScheme"/>
        <rdfs:label xml:lang="en">Code list for totalCarbonateEquivalent analysis procedures - codelist scheme</rdfs:label>
        <rdfs:seeAlso rdf:resource="http://w3id.org/glosis/model/procedure/TotalCarbonateEquivalentProcedure"/>
        <skos:definition>AfSP-derived interpretation (RwaSP)</skos:definition>
        <skos:note xml:lang="en">This code list provides analysis procedures for totalCarbonateEquivalent.</skos:note>
        <skos:prefLabel xml:lang="en">Code list for totalCarbonateEquivalent analysis procedures - codelist scheme</skos:prefLabel>
    </owl:NamedIndividual>
    


    <!-- http://w3id.org/glosis/model/procedure/totalCarbonateEquivalentProcedure-CaCO3_acid-ch3cooh-dc -->


    <owl:NamedIndividual rdf:about="http://w3id.org/glosis/model/procedure/totalCarbonateEquivalentProcedure-CaCO3_acid-ch3cooh-dc">
        <rdf:type rdf:resource="http://w3id.org/glosis/model/procedure/TotalCarbonateEquivalentProcedure"/>
        <rdf:type rdf:resource="http://www.w3.org/2004/02/skos/core#Concept"/>
        <skos:definition>Dissolution of carbonates by Acetic acid [CH3COOH], external heat (dry combustion)</skos:definition>
        <skos:inScheme rdf:resource="http://w3id.org/glosis/model/procedure/totalCarbonateEquivalentProcedure"/>
        <skos:notation>CaCO3_acid-ch3cooh-dc</skos:notation>
        <skos:prefLabel xml:lang="en">CaCO3_acid-ch3cooh-dc</skos:prefLabel>
        <skos:scopeNote rdf:resource="https://www.isric.org/sites/default/files/isric_report_2014_01.pdf"/>
        <skos:scopeNote>Leenaars J.G.B., A.J.M. van Oostrum and M. Ruiperez Gonzalez, 2014. Africa Soil Profiles Database, Version 1.2. A compilation of georeferenced and standardised legacy soil profile data for Sub-Saharan Africa (with dataset). ISRIC Report 2014/01. Africa Soil Information Service (AfSIS) project and ISRIC - World Soil Information, Wageningen, the Netherlands. See Annex 4.</skos:scopeNote>
        <skos:topConceptOf rdf:resource="http://w3id.org/glosis/model/procedure/totalCarbonateEquivalentProcedure"/>
    </owl:NamedIndividual>
    


    <!-- http://w3id.org/glosis/model/procedure/totalCarbonateEquivalentProcedure-CaCO3_acid-ch3cooh-nodc -->


    <owl:NamedIndividual rdf:about="http://w3id.org/glosis/model/procedure/totalCarbonateEquivalentProcedure-CaCO3_acid-ch3cooh-nodc">
        <rdf:type rdf:resource="http://w3id.org/glosis/model/procedure/TotalCarbonateEquivalentProcedure"/>
        <rdf:type rdf:resource="http://www.w3.org/2004/02/skos/core#Concept"/>
        <skos:definition>Dissolution of carbonates by Acetic acid [CH3COOH], no external (no dry combustion)</skos:definition>
        <skos:inScheme rdf:resource="http://w3id.org/glosis/model/procedure/totalCarbonateEquivalentProcedure"/>
        <skos:notation>CaCO3_acid-ch3cooh-nodc</skos:notation>
        <skos:prefLabel xml:lang="en">CaCO3_acid-ch3cooh-nodc</skos:prefLabel>
        <skos:scopeNote rdf:resource="https://www.isric.org/sites/default/files/isric_report_2014_01.pdf"/>
        <skos:scopeNote>Leenaars J.G.B., A.J.M. van Oostrum and M. Ruiperez Gonzalez, 2014. Africa Soil Profiles Database, Version 1.2. A compilation of georeferenced and standardised legacy soil profile data for Sub-Saharan Africa (with dataset). ISRIC Report 2014/01. Africa Soil Information Service (AfSIS) project and ISRIC - World Soil Information, Wageningen, the Netherlands. See Annex 4.</skos:scopeNote>
        <skos:topConceptOf rdf:resource="http://w3id.org/glosis/model/procedure/totalCarbonateEquivalentProcedure"/>
    </owl:NamedIndividual>
    


    <!-- http://w3id.org/glosis/model/procedure/totalCarbonateEquivalentProcedure-CaCO3_acid-ch3cooh-unkn -->


    <owl:NamedIndividual rdf:about="http://w3id.org/glosis/model/procedure/totalCarbonateEquivalentProcedure-CaCO3_acid-ch3cooh-unkn">
        <rdf:type rdf:resource="http://w3id.org/glosis/model/procedure/TotalCarbonateEquivalentProcedure"/>
        <rdf:type rdf:resource="http://www.w3.org/2004/02/skos/core#Concept"/>
        <skos:definition>Dissolution of carbonates by Acetic acid [CH3COOH], external heat unknown</skos:definition>
        <skos:inScheme rdf:resource="http://w3id.org/glosis/model/procedure/totalCarbonateEquivalentProcedure"/>
        <skos:notation>CaCO3_acid-ch3cooh-unkn</skos:notation>
        <skos:prefLabel xml:lang="en">CaCO3_acid-ch3cooh-unk</skos:prefLabel>
        <skos:scopeNote rdf:resource="https://www.isric.org/sites/default/files/isric_report_2014_01.pdf"/>
        <skos:scopeNote>Leenaars J.G.B., A.J.M. van Oostrum and M. Ruiperez Gonzalez, 2014. Africa Soil Profiles Database, Version 1.2. A compilation of georeferenced and standardised legacy soil profile data for Sub-Saharan Africa (with dataset). ISRIC Report 2014/01. Africa Soil Information Service (AfSIS) project and ISRIC - World Soil Information, Wageningen, the Netherlands. See Annex 4.</skos:scopeNote>
        <skos:topConceptOf rdf:resource="http://w3id.org/glosis/model/procedure/totalCarbonateEquivalentProcedure"/>
    </owl:NamedIndividual>
    


    <!-- http://w3id.org/glosis/model/procedure/totalCarbonateEquivalentProcedure-CaCO3_acid-dc -->


    <owl:NamedIndividual rdf:about="http://w3id.org/glosis/model/procedure/totalCarbonateEquivalentProcedure-CaCO3_acid-dc">
        <rdf:type rdf:resource="http://w3id.org/glosis/model/procedure/TotalCarbonateEquivalentProcedure"/>
        <rdf:type rdf:resource="http://www.w3.org/2004/02/skos/core#Concept"/>
        <skos:definition>Dissolution of carbonates by acid, external heat (dry combustion)</skos:definition>
        <skos:inScheme rdf:resource="http://w3id.org/glosis/model/procedure/totalCarbonateEquivalentProcedure"/>
        <skos:notation>CaCO3_acid-dc</skos:notation>
        <skos:prefLabel xml:lang="en">CaCO3_acid-dc</skos:prefLabel>
        <skos:scopeNote rdf:resource="https://www.isric.org/sites/default/files/isric_report_2014_01.pdf"/>
        <skos:scopeNote>Leenaars J.G.B., A.J.M. van Oostrum and M. Ruiperez Gonzalez, 2014. Africa Soil Profiles Database, Version 1.2. A compilation of georeferenced and standardised legacy soil profile data for Sub-Saharan Africa (with dataset). ISRIC Report 2014/01. Africa Soil Information Service (AfSIS) project and ISRIC - World Soil Information, Wageningen, the Netherlands. See Annex 4.</skos:scopeNote>
        <skos:topConceptOf rdf:resource="http://w3id.org/glosis/model/procedure/totalCarbonateEquivalentProcedure"/>
    </owl:NamedIndividual>
    


    <!-- http://w3id.org/glosis/model/procedure/totalCarbonateEquivalentProcedure-CaCO3_acid-h2so4-dc -->


    <owl:NamedIndividual rdf:about="http://w3id.org/glosis/model/procedure/totalCarbonateEquivalentProcedure-CaCO3_acid-h2so4-dc">
        <rdf:type rdf:resource="http://w3id.org/glosis/model/procedure/TotalCarbonateEquivalentProcedure"/>
        <rdf:type rdf:resource="http://www.w3.org/2004/02/skos/core#Concept"/>
        <skos:definition>Dissolution of carbonates by Sulfuric acid [H2SO4], external heat (dry combustion)</skos:definition>
        <skos:inScheme rdf:resource="http://w3id.org/glosis/model/procedure/totalCarbonateEquivalentProcedure"/>
        <skos:notation>CaCO3_acid-h2so4-dc</skos:notation>
        <skos:prefLabel xml:lang="en">CaCO3_acid-h2so4-dc</skos:prefLabel>
        <skos:scopeNote rdf:resource="https://www.isric.org/sites/default/files/isric_report_2014_01.pdf"/>
        <skos:scopeNote>Leenaars J.G.B., A.J.M. van Oostrum and M. Ruiperez Gonzalez, 2014. Africa Soil Profiles Database, Version 1.2. A compilation of georeferenced and standardised legacy soil profile data for Sub-Saharan Africa (with dataset). ISRIC Report 2014/01. Africa Soil Information Service (AfSIS) project and ISRIC - World Soil Information, Wageningen, the Netherlands. See Annex 4.</skos:scopeNote>
        <skos:topConceptOf rdf:resource="http://w3id.org/glosis/model/procedure/totalCarbonateEquivalentProcedure"/>
    </owl:NamedIndividual>
    


    <!-- http://w3id.org/glosis/model/procedure/totalCarbonateEquivalentProcedure-CaCO3_acid-h2so4-nodc -->


    <owl:NamedIndividual rdf:about="http://w3id.org/glosis/model/procedure/totalCarbonateEquivalentProcedure-CaCO3_acid-h2so4-nodc">
        <rdf:type rdf:resource="http://w3id.org/glosis/model/procedure/TotalCarbonateEquivalentProcedure"/>
        <rdf:type rdf:resource="http://www.w3.org/2004/02/skos/core#Concept"/>
        <skos:definition>Dissolution of carbonates by Sulfuric acid [H2SO4], no external (no dry combustion)</skos:definition>
        <skos:inScheme rdf:resource="http://w3id.org/glosis/model/procedure/totalCarbonateEquivalentProcedure"/>
        <skos:notation>CaCO3_acid-h2so4-nodc</skos:notation>
        <skos:prefLabel xml:lang="en">CaCO3_acid-h2so4-nodc</skos:prefLabel>
        <skos:scopeNote rdf:resource="https://www.isric.org/sites/default/files/isric_report_2014_01.pdf"/>
        <skos:scopeNote>Leenaars J.G.B., A.J.M. van Oostrum and M. Ruiperez Gonzalez, 2014. Africa Soil Profiles Database, Version 1.2. A compilation of georeferenced and standardised legacy soil profile data for Sub-Saharan Africa (with dataset). ISRIC Report 2014/01. Africa Soil Information Service (AfSIS) project and ISRIC - World Soil Information, Wageningen, the Netherlands. See Annex 4.</skos:scopeNote>
        <skos:topConceptOf rdf:resource="http://w3id.org/glosis/model/procedure/totalCarbonateEquivalentProcedure"/>
    </owl:NamedIndividual>
    


    <!-- http://w3id.org/glosis/model/procedure/totalCarbonateEquivalentProcedure-CaCO3_acid-h2so4-unkn -->


    <owl:NamedIndividual rdf:about="http://w3id.org/glosis/model/procedure/totalCarbonateEquivalentProcedure-CaCO3_acid-h2so4-unkn">
        <rdf:type rdf:resource="http://w3id.org/glosis/model/procedure/TotalCarbonateEquivalentProcedure"/>
        <rdf:type rdf:resource="http://www.w3.org/2004/02/skos/core#Concept"/>
        <skos:definition>Dissolution of carbonates by Sulfuric acid [H2SO4], external heat unknown</skos:definition>
        <skos:inScheme rdf:resource="http://w3id.org/glosis/model/procedure/totalCarbonateEquivalentProcedure"/>
        <skos:notation>CaCO3_acid-h2so4-unkn</skos:notation>
        <skos:prefLabel xml:lang="en">CaCO3_acid-h2so4-unk</skos:prefLabel>
        <skos:scopeNote rdf:resource="https://www.isric.org/sites/default/files/isric_report_2014_01.pdf"/>
        <skos:scopeNote>Leenaars J.G.B., A.J.M. van Oostrum and M. Ruiperez Gonzalez, 2014. Africa Soil Profiles Database, Version 1.2. A compilation of georeferenced and standardised legacy soil profile data for Sub-Saharan Africa (with dataset). ISRIC Report 2014/01. Africa Soil Information Service (AfSIS) project and ISRIC - World Soil Information, Wageningen, the Netherlands. See Annex 4.</skos:scopeNote>
        <skos:topConceptOf rdf:resource="http://w3id.org/glosis/model/procedure/totalCarbonateEquivalentProcedure"/>
    </owl:NamedIndividual>
    


    <!-- http://w3id.org/glosis/model/procedure/totalCarbonateEquivalentProcedure-CaCO3_acid-h3po4-dc -->


    <owl:NamedIndividual rdf:about="http://w3id.org/glosis/model/procedure/totalCarbonateEquivalentProcedure-CaCO3_acid-h3po4-dc">
        <rdf:type rdf:resource="http://w3id.org/glosis/model/procedure/TotalCarbonateEquivalentProcedure"/>
        <rdf:type rdf:resource="http://www.w3.org/2004/02/skos/core#Concept"/>
        <skos:definition>Dissolution of carbonates by Phosphoric acid [H3PO4], external heat (dry combustion)</skos:definition>
        <skos:inScheme rdf:resource="http://w3id.org/glosis/model/procedure/totalCarbonateEquivalentProcedure"/>
        <skos:notation>CaCO3_acid-h3po4-dc</skos:notation>
        <skos:prefLabel xml:lang="en">CaCO3_acid-h3po4-dc</skos:prefLabel>
        <skos:scopeNote rdf:resource="https://www.isric.org/sites/default/files/isric_report_2014_01.pdf"/>
        <skos:scopeNote>Leenaars J.G.B., A.J.M. van Oostrum and M. Ruiperez Gonzalez, 2014. Africa Soil Profiles Database, Version 1.2. A compilation of georeferenced and standardised legacy soil profile data for Sub-Saharan Africa (with dataset). ISRIC Report 2014/01. Africa Soil Information Service (AfSIS) project and ISRIC - World Soil Information, Wageningen, the Netherlands. See Annex 4.</skos:scopeNote>
        <skos:topConceptOf rdf:resource="http://w3id.org/glosis/model/procedure/totalCarbonateEquivalentProcedure"/>
    </owl:NamedIndividual>
    


    <!-- http://w3id.org/glosis/model/procedure/totalCarbonateEquivalentProcedure-CaCO3_acid-h3po4-nodc -->


    <owl:NamedIndividual rdf:about="http://w3id.org/glosis/model/procedure/totalCarbonateEquivalentProcedure-CaCO3_acid-h3po4-nodc">
        <rdf:type rdf:resource="http://w3id.org/glosis/model/procedure/TotalCarbonateEquivalentProcedure"/>
        <rdf:type rdf:resource="http://www.w3.org/2004/02/skos/core#Concept"/>
        <skos:definition>Dissolution of carbonates by Phosphoric acid [H3PO4], no external (no dry combustion)</skos:definition>
        <skos:inScheme rdf:resource="http://w3id.org/glosis/model/procedure/totalCarbonateEquivalentProcedure"/>
        <skos:notation>CaCO3_acid-h3po4-nodc</skos:notation>
        <skos:prefLabel xml:lang="en">CaCO3_acid-h3po4-nodc</skos:prefLabel>
        <skos:scopeNote rdf:resource="https://www.isric.org/sites/default/files/isric_report_2014_01.pdf"/>
        <skos:scopeNote>Leenaars J.G.B., A.J.M. van Oostrum and M. Ruiperez Gonzalez, 2014. Africa Soil Profiles Database, Version 1.2. A compilation of georeferenced and standardised legacy soil profile data for Sub-Saharan Africa (with dataset). ISRIC Report 2014/01. Africa Soil Information Service (AfSIS) project and ISRIC - World Soil Information, Wageningen, the Netherlands. See Annex 4.</skos:scopeNote>
        <skos:topConceptOf rdf:resource="http://w3id.org/glosis/model/procedure/totalCarbonateEquivalentProcedure"/>
    </owl:NamedIndividual>
    


    <!-- http://w3id.org/glosis/model/procedure/totalCarbonateEquivalentProcedure-CaCO3_acid-h3po4-unkn -->


    <owl:NamedIndividual rdf:about="http://w3id.org/glosis/model/procedure/totalCarbonateEquivalentProcedure-CaCO3_acid-h3po4-unkn">
        <rdf:type rdf:resource="http://w3id.org/glosis/model/procedure/TotalCarbonateEquivalentProcedure"/>
        <rdf:type rdf:resource="http://www.w3.org/2004/02/skos/core#Concept"/>
        <skos:definition>Dissolution of carbonates by Phosphoric acid [H3PO4], external heat unknown</skos:definition>
        <skos:inScheme rdf:resource="http://w3id.org/glosis/model/procedure/totalCarbonateEquivalentProcedure"/>
        <skos:notation>CaCO3_acid-h3po4-unkn</skos:notation>
        <skos:prefLabel xml:lang="en">CaCO3_acid-h3po4-unk</skos:prefLabel>
        <skos:scopeNote rdf:resource="https://www.isric.org/sites/default/files/isric_report_2014_01.pdf"/>
        <skos:scopeNote>Leenaars J.G.B., A.J.M. van Oostrum and M. Ruiperez Gonzalez, 2014. Africa Soil Profiles Database, Version 1.2. A compilation of georeferenced and standardised legacy soil profile data for Sub-Saharan Africa (with dataset). ISRIC Report 2014/01. Africa Soil Information Service (AfSIS) project and ISRIC - World Soil Information, Wageningen, the Netherlands. See Annex 4.</skos:scopeNote>
        <skos:topConceptOf rdf:resource="http://w3id.org/glosis/model/procedure/totalCarbonateEquivalentProcedure"/>
    </owl:NamedIndividual>
    


    <!-- http://w3id.org/glosis/model/procedure/totalCarbonateEquivalentProcedure-CaCO3_acid-hcl-dc -->


    <owl:NamedIndividual rdf:about="http://w3id.org/glosis/model/procedure/totalCarbonateEquivalentProcedure-CaCO3_acid-hcl-dc">
        <rdf:type rdf:resource="http://w3id.org/glosis/model/procedure/TotalCarbonateEquivalentProcedure"/>
        <rdf:type rdf:resource="http://www.w3.org/2004/02/skos/core#Concept"/>
        <skos:definition>Dissolution of carbonates by Hydrochloric acid [HCl], or Perchloric acid [HClO4], external heat (dry combustion)</skos:definition>
        <skos:inScheme rdf:resource="http://w3id.org/glosis/model/procedure/totalCarbonateEquivalentProcedure"/>
        <skos:notation>CaCO3_acid-hcl-dc</skos:notation>
        <skos:prefLabel xml:lang="en">CaCO3_acid-hcl-dc</skos:prefLabel>
        <skos:scopeNote rdf:resource="https://www.isric.org/sites/default/files/isric_report_2014_01.pdf"/>
        <skos:scopeNote>Leenaars J.G.B., A.J.M. van Oostrum and M. Ruiperez Gonzalez, 2014. Africa Soil Profiles Database, Version 1.2. A compilation of georeferenced and standardised legacy soil profile data for Sub-Saharan Africa (with dataset). ISRIC Report 2014/01. Africa Soil Information Service (AfSIS) project and ISRIC - World Soil Information, Wageningen, the Netherlands. See Annex 4.</skos:scopeNote>
        <skos:topConceptOf rdf:resource="http://w3id.org/glosis/model/procedure/totalCarbonateEquivalentProcedure"/>
    </owl:NamedIndividual>
    


    <!-- http://w3id.org/glosis/model/procedure/totalCarbonateEquivalentProcedure-CaCO3_acid-hcl-nodc -->


    <owl:NamedIndividual rdf:about="http://w3id.org/glosis/model/procedure/totalCarbonateEquivalentProcedure-CaCO3_acid-hcl-nodc">
        <rdf:type rdf:resource="http://w3id.org/glosis/model/procedure/TotalCarbonateEquivalentProcedure"/>
        <rdf:type rdf:resource="http://www.w3.org/2004/02/skos/core#Concept"/>
        <skos:definition>Dissolution of carbonates by Hydrochloric acid [HCl], or Perchloric acid [HClO4], no external (no dry combustion)</skos:definition>
        <skos:inScheme rdf:resource="http://w3id.org/glosis/model/procedure/totalCarbonateEquivalentProcedure"/>
        <skos:notation>CaCO3_acid-hcl-nodc</skos:notation>
        <skos:prefLabel xml:lang="en">CaCO3_acid-hcl-nodc</skos:prefLabel>
        <skos:scopeNote rdf:resource="https://www.isric.org/sites/default/files/isric_report_2014_01.pdf"/>
        <skos:scopeNote>Leenaars J.G.B., A.J.M. van Oostrum and M. Ruiperez Gonzalez, 2014. Africa Soil Profiles Database, Version 1.2. A compilation of georeferenced and standardised legacy soil profile data for Sub-Saharan Africa (with dataset). ISRIC Report 2014/01. Africa Soil Information Service (AfSIS) project and ISRIC - World Soil Information, Wageningen, the Netherlands. See Annex 4.</skos:scopeNote>
        <skos:topConceptOf rdf:resource="http://w3id.org/glosis/model/procedure/totalCarbonateEquivalentProcedure"/>
    </owl:NamedIndividual>
    


    <!-- http://w3id.org/glosis/model/procedure/totalCarbonateEquivalentProcedure-CaCO3_acid-hcl-unkn -->


    <owl:NamedIndividual rdf:about="http://w3id.org/glosis/model/procedure/totalCarbonateEquivalentProcedure-CaCO3_acid-hcl-unkn">
        <rdf:type rdf:resource="http://w3id.org/glosis/model/procedure/TotalCarbonateEquivalentProcedure"/>
        <rdf:type rdf:resource="http://www.w3.org/2004/02/skos/core#Concept"/>
        <skos:definition>Dissolution of carbonates by Hydrochloric acid [HCl], or Perchloric acid [HClO4], external heat unknown</skos:definition>
        <skos:inScheme rdf:resource="http://w3id.org/glosis/model/procedure/totalCarbonateEquivalentProcedure"/>
        <skos:notation>CaCO3_acid-hcl-unkn</skos:notation>
        <skos:prefLabel xml:lang="en">CaCO3_acid-hcl-unk</skos:prefLabel>
        <skos:scopeNote rdf:resource="https://www.isric.org/sites/default/files/isric_report_2014_01.pdf"/>
        <skos:scopeNote>Leenaars J.G.B., A.J.M. van Oostrum and M. Ruiperez Gonzalez, 2014. Africa Soil Profiles Database, Version 1.2. A compilation of georeferenced and standardised legacy soil profile data for Sub-Saharan Africa (with dataset). ISRIC Report 2014/01. Africa Soil Information Service (AfSIS) project and ISRIC - World Soil Information, Wageningen, the Netherlands. See Annex 4.</skos:scopeNote>
        <skos:topConceptOf rdf:resource="http://w3id.org/glosis/model/procedure/totalCarbonateEquivalentProcedure"/>
    </owl:NamedIndividual>
    


    <!-- http://w3id.org/glosis/model/procedure/totalCarbonateEquivalentProcedure-CaCO3_acid-nodc -->


    <owl:NamedIndividual rdf:about="http://w3id.org/glosis/model/procedure/totalCarbonateEquivalentProcedure-CaCO3_acid-nodc">
        <rdf:type rdf:resource="http://w3id.org/glosis/model/procedure/TotalCarbonateEquivalentProcedure"/>
        <rdf:type rdf:resource="http://www.w3.org/2004/02/skos/core#Concept"/>
        <skos:definition>Dissolution of carbonates by acid, no external (no dry combustion)</skos:definition>
        <skos:inScheme rdf:resource="http://w3id.org/glosis/model/procedure/totalCarbonateEquivalentProcedure"/>
        <skos:notation>CaCO3_acid-nodc</skos:notation>
        <skos:prefLabel xml:lang="en">CaCO3_acid-nodc</skos:prefLabel>
        <skos:scopeNote rdf:resource="https://www.isric.org/sites/default/files/isric_report_2014_01.pdf"/>
        <skos:scopeNote>Leenaars J.G.B., A.J.M. van Oostrum and M. Ruiperez Gonzalez, 2014. Africa Soil Profiles Database, Version 1.2. A compilation of georeferenced and standardised legacy soil profile data for Sub-Saharan Africa (with dataset). ISRIC Report 2014/01. Africa Soil Information Service (AfSIS) project and ISRIC - World Soil Information, Wageningen, the Netherlands. See Annex 4.</skos:scopeNote>
        <skos:topConceptOf rdf:resource="http://w3id.org/glosis/model/procedure/totalCarbonateEquivalentProcedure"/>
    </owl:NamedIndividual>
    


    <!-- http://w3id.org/glosis/model/procedure/totalCarbonateEquivalentProcedure-CaCO3_acid-unkn -->


    <owl:NamedIndividual rdf:about="http://w3id.org/glosis/model/procedure/totalCarbonateEquivalentProcedure-CaCO3_acid-unkn">
        <rdf:type rdf:resource="http://w3id.org/glosis/model/procedure/TotalCarbonateEquivalentProcedure"/>
        <rdf:type rdf:resource="http://www.w3.org/2004/02/skos/core#Concept"/>
        <skos:definition>Dissolution of carbonates by acid, external heat unknown</skos:definition>
        <skos:inScheme rdf:resource="http://w3id.org/glosis/model/procedure/totalCarbonateEquivalentProcedure"/>
        <skos:notation>CaCO3_acid-unkn</skos:notation>
        <skos:prefLabel xml:lang="en">CaCO3_acid-unk</skos:prefLabel>
        <skos:scopeNote rdf:resource="https://www.isric.org/sites/default/files/isric_report_2014_01.pdf"/>
        <skos:scopeNote>Leenaars J.G.B., A.J.M. van Oostrum and M. Ruiperez Gonzalez, 2014. Africa Soil Profiles Database, Version 1.2. A compilation of georeferenced and standardised legacy soil profile data for Sub-Saharan Africa (with dataset). ISRIC Report 2014/01. Africa Soil Information Service (AfSIS) project and ISRIC - World Soil Information, Wageningen, the Netherlands. See Annex 4.</skos:scopeNote>
        <skos:topConceptOf rdf:resource="http://w3id.org/glosis/model/procedure/totalCarbonateEquivalentProcedure"/>
    </owl:NamedIndividual>
    


    <!-- http://w3id.org/glosis/model/procedure/totalCarbonateEquivalentProcedure-CaCO3_ca01 -->


    <owl:NamedIndividual rdf:about="http://w3id.org/glosis/model/procedure/totalCarbonateEquivalentProcedure-CaCO3_ca01">
        <rdf:type rdf:resource="http://w3id.org/glosis/model/procedure/TotalCarbonateEquivalentProcedure"/>
        <rdf:type rdf:resource="http://www.w3.org/2004/02/skos/core#Concept"/>
        <skos:definition>Method of Scheibler (volumetric)</skos:definition>
        <skos:inScheme rdf:resource="http://w3id.org/glosis/model/procedure/totalCarbonateEquivalentProcedure"/>
        <skos:notation>CaCO3_ca01</skos:notation>
        <skos:prefLabel xml:lang="en">CaCO3_ca01</skos:prefLabel>
        <skos:scopeNote>ON L 1084-99 (1999) Chemical analyses of soils—determination of carbonate. In: Austrian Standards Institute (ed) O‹ NORM L 1084. Austrian Standards Institute, Vienna</skos:scopeNote>
        <skos:topConceptOf rdf:resource="http://w3id.org/glosis/model/procedure/totalCarbonateEquivalentProcedure"/>
    </owl:NamedIndividual>
    


    <!-- http://w3id.org/glosis/model/procedure/totalCarbonateEquivalentProcedure-CaCO3_ca02 -->


    <owl:NamedIndividual rdf:about="http://w3id.org/glosis/model/procedure/totalCarbonateEquivalentProcedure-CaCO3_ca02">
        <rdf:type rdf:resource="http://w3id.org/glosis/model/procedure/TotalCarbonateEquivalentProcedure"/>
        <rdf:type rdf:resource="http://www.w3.org/2004/02/skos/core#Concept"/>
        <skos:definition>Method of Wesemael</skos:definition>
        <skos:inScheme rdf:resource="http://w3id.org/glosis/model/procedure/totalCarbonateEquivalentProcedure"/>
        <skos:notation>CaCO3_ca02</skos:notation>
        <skos:prefLabel xml:lang="en">CaCO3_ca02</skos:prefLabel>
        <skos:scopeNote>Wesemael, J.C., 1955. De bepaling van van calciumcarbonaatgehalte van gronden. Chemisch Weekblad 51, 35-36.</skos:scopeNote>
        <skos:topConceptOf rdf:resource="http://w3id.org/glosis/model/procedure/totalCarbonateEquivalentProcedure"/>
    </owl:NamedIndividual>
    


    <!-- http://w3id.org/glosis/model/procedure/totalCarbonateEquivalentProcedure-CaCO3_ca03 -->


    <owl:NamedIndividual rdf:about="http://w3id.org/glosis/model/procedure/totalCarbonateEquivalentProcedure-CaCO3_ca03">
        <rdf:type rdf:resource="http://w3id.org/glosis/model/procedure/TotalCarbonateEquivalentProcedure"/>
        <rdf:type rdf:resource="http://www.w3.org/2004/02/skos/core#Concept"/>
        <skos:definition>Method of Piper (HCl)</skos:definition>
        <skos:inScheme rdf:resource="http://w3id.org/glosis/model/procedure/totalCarbonateEquivalentProcedure"/>
        <skos:notation>CaCO3_ca03</skos:notation>
        <skos:prefLabel xml:lang="en">CaCO3_ca03</skos:prefLabel>
        <skos:scopeNote rdf:resource="https://www.isric.org/sites/default/files/isric_report_2014_01.pdf"/>
        <skos:scopeNote>Leenaars J.G.B., A.J.M. van Oostrum and M. Ruiperez Gonzalez, 2014. Africa Soil Profiles Database, Version 1.2. A compilation of georeferenced and standardised legacy soil profile data for Sub-Saharan Africa (with dataset). ISRIC Report 2014/01. Africa Soil Information Service (AfSIS) project and ISRIC - World Soil Information, Wageningen, the Netherlands. See Annex 4.</skos:scopeNote>
        <skos:topConceptOf rdf:resource="http://w3id.org/glosis/model/procedure/totalCarbonateEquivalentProcedure"/>
    </owl:NamedIndividual>
    


    <!-- http://w3id.org/glosis/model/procedure/totalCarbonateEquivalentProcedure-CaCO3_ca04 -->


    <owl:NamedIndividual rdf:about="http://w3id.org/glosis/model/procedure/totalCarbonateEquivalentProcedure-CaCO3_ca04">
        <rdf:type rdf:resource="http://w3id.org/glosis/model/procedure/TotalCarbonateEquivalentProcedure"/>
        <rdf:type rdf:resource="http://www.w3.org/2004/02/skos/core#Concept"/>
        <skos:definition>Calcimeter method (volumetric after adition of dilute acid)</skos:definition>
        <skos:inScheme rdf:resource="http://w3id.org/glosis/model/procedure/totalCarbonateEquivalentProcedure"/>
        <skos:notation>CaCO3_ca04</skos:notation>
        <skos:prefLabel xml:lang="en">CaCO3_ca04</skos:prefLabel>
        <skos:scopeNote rdf:resource="https://www.isric.org/sites/default/files/isric_report_2014_01.pdf"/>
        <skos:scopeNote>Leenaars J.G.B., A.J.M. van Oostrum and M. Ruiperez Gonzalez, 2014. Africa Soil Profiles Database, Version 1.2. A compilation of georeferenced and standardised legacy soil profile data for Sub-Saharan Africa (with dataset). ISRIC Report 2014/01. Africa Soil Information Service (AfSIS) project and ISRIC - World Soil Information, Wageningen, the Netherlands. See Annex 4.</skos:scopeNote>
        <skos:topConceptOf rdf:resource="http://w3id.org/glosis/model/procedure/totalCarbonateEquivalentProcedure"/>
    </owl:NamedIndividual>
    


    <!-- http://w3id.org/glosis/model/procedure/totalCarbonateEquivalentProcedure-CaCO3_ca05 -->


    <owl:NamedIndividual rdf:about="http://w3id.org/glosis/model/procedure/totalCarbonateEquivalentProcedure-CaCO3_ca05">
        <rdf:type rdf:resource="http://w3id.org/glosis/model/procedure/TotalCarbonateEquivalentProcedure"/>
        <rdf:type rdf:resource="http://www.w3.org/2004/02/skos/core#Concept"/>
        <skos:definition>Gravimetric (USDA Agr. Hdbk 60-/- method Richards et al., 1954)</skos:definition>
        <skos:inScheme rdf:resource="http://w3id.org/glosis/model/procedure/totalCarbonateEquivalentProcedure"/>
        <skos:notation>CaCO3_ca05</skos:notation>
        <skos:prefLabel xml:lang="en">CaCO3_ca05</skos:prefLabel>
        <skos:scopeNote rdf:resource="https://www.isric.org/sites/default/files/isric_report_2014_01.pdf"/>
        <skos:scopeNote>Leenaars J.G.B., A.J.M. van Oostrum and M. Ruiperez Gonzalez, 2014. Africa Soil Profiles Database, Version 1.2. A compilation of georeferenced and standardised legacy soil profile data for Sub-Saharan Africa (with dataset). ISRIC Report 2014/01. Africa Soil Information Service (AfSIS) project and ISRIC - World Soil Information, Wageningen, the Netherlands. See Annex 4.</skos:scopeNote>
        <skos:topConceptOf rdf:resource="http://w3id.org/glosis/model/procedure/totalCarbonateEquivalentProcedure"/>
    </owl:NamedIndividual>
    


    <!-- http://w3id.org/glosis/model/procedure/totalCarbonateEquivalentProcedure-CaCO3_ca06 -->


    <owl:NamedIndividual rdf:about="http://w3id.org/glosis/model/procedure/totalCarbonateEquivalentProcedure-CaCO3_ca06">
        <rdf:type rdf:resource="http://w3id.org/glosis/model/procedure/TotalCarbonateEquivalentProcedure"/>
        <rdf:type rdf:resource="http://www.w3.org/2004/02/skos/core#Concept"/>
        <skos:definition>H3PO4 acid at 80C, conductometric in NaOH (Schlichting &amp; Blume, 1966)</skos:definition>
        <skos:inScheme rdf:resource="http://w3id.org/glosis/model/procedure/totalCarbonateEquivalentProcedure"/>
        <skos:notation>CaCO3_ca06</skos:notation>
        <skos:prefLabel xml:lang="en">CaCO3_ca06</skos:prefLabel>
        <skos:scopeNote rdf:resource="https://www.isric.org/sites/default/files/isric_report_2014_01.pdf"/>
        <skos:scopeNote>Leenaars J.G.B., A.J.M. van Oostrum and M. Ruiperez Gonzalez, 2014. Africa Soil Profiles Database, Version 1.2. A compilation of georeferenced and standardised legacy soil profile data for Sub-Saharan Africa (with dataset). ISRIC Report 2014/01. Africa Soil Information Service (AfSIS) project and ISRIC - World Soil Information, Wageningen, the Netherlands. See Annex 4.</skos:scopeNote>
        <skos:topConceptOf rdf:resource="http://w3id.org/glosis/model/procedure/totalCarbonateEquivalentProcedure"/>
    </owl:NamedIndividual>
    


    <!-- http://w3id.org/glosis/model/procedure/totalCarbonateEquivalentProcedure-CaCO3_ca07 -->


    <owl:NamedIndividual rdf:about="http://w3id.org/glosis/model/procedure/totalCarbonateEquivalentProcedure-CaCO3_ca07">
        <rdf:type rdf:resource="http://w3id.org/glosis/model/procedure/TotalCarbonateEquivalentProcedure"/>
        <rdf:type rdf:resource="http://www.w3.org/2004/02/skos/core#Concept"/>
        <skos:definition>Pressure calcimeter (Nelson, 1982)</skos:definition>
        <skos:inScheme rdf:resource="http://w3id.org/glosis/model/procedure/totalCarbonateEquivalentProcedure"/>
        <skos:notation>CaCO3_ca07</skos:notation>
        <skos:prefLabel xml:lang="en">CaCO3_ca07</skos:prefLabel>
        <skos:scopeNote rdf:resource="https://acsess.onlinelibrary.wiley.com/doi/book/10.2134/agronmonogr9.2.2ed"/>
        <skos:scopeNote>Nelson, D.W., and L.E. Sommers. 1982. Total carbon, organic carbon and organic matter. p. 539-579. In A.L. Page (ed.), 1983. Methods of soil analysis. Part 2. 2nd ed. Agron. Monogr. 9. ASA and SSSA, Madison, WI.</skos:scopeNote>
        <skos:topConceptOf rdf:resource="http://w3id.org/glosis/model/procedure/totalCarbonateEquivalentProcedure"/>
    </owl:NamedIndividual>
    


    <!-- http://w3id.org/glosis/model/procedure/totalCarbonateEquivalentProcedure-CaCO3_ca08 -->


    <owl:NamedIndividual rdf:about="http://w3id.org/glosis/model/procedure/totalCarbonateEquivalentProcedure-CaCO3_ca08">
        <rdf:type rdf:resource="http://w3id.org/glosis/model/procedure/TotalCarbonateEquivalentProcedure"/>
        <rdf:type rdf:resource="http://www.w3.org/2004/02/skos/core#Concept"/>
        <skos:definition>Bernard calcimeter (Total CaCO3)</skos:definition>
        <skos:inScheme rdf:resource="http://w3id.org/glosis/model/procedure/totalCarbonateEquivalentProcedure"/>
        <skos:notation>CaCO3_ca08</skos:notation>
        <skos:prefLabel xml:lang="en">CaCO3_ca08</skos:prefLabel>
        <skos:scopeNote rdf:resource="https://www.isric.org/sites/default/files/isric_report_2014_01.pdf"/>
        <skos:scopeNote>Leenaars J.G.B., A.J.M. van Oostrum and M. Ruiperez Gonzalez, 2014. Africa Soil Profiles Database, Version 1.2. A compilation of georeferenced and standardised legacy soil profile data for Sub-Saharan Africa (with dataset). ISRIC Report 2014/01. Africa Soil Information Service (AfSIS) project and ISRIC - World Soil Information, Wageningen, the Netherlands. See Annex 4.</skos:scopeNote>
        <skos:topConceptOf rdf:resource="http://w3id.org/glosis/model/procedure/totalCarbonateEquivalentProcedure"/>
    </owl:NamedIndividual>
    


    <!-- http://w3id.org/glosis/model/procedure/totalCarbonateEquivalentProcedure-CaCO3_ca09 -->


    <owl:NamedIndividual rdf:about="http://w3id.org/glosis/model/procedure/totalCarbonateEquivalentProcedure-CaCO3_ca09">
        <rdf:type rdf:resource="http://w3id.org/glosis/model/procedure/TotalCarbonateEquivalentProcedure"/>
        <rdf:type rdf:resource="http://www.w3.org/2004/02/skos/core#Concept"/>
        <skos:definition>Carbonates: H3PO4 treatment at 80 deg. C and CO2 measurement like TOC (OC13), transformation into CaCO3 (Schlichting et al. 1995)</skos:definition>
        <skos:inScheme rdf:resource="http://w3id.org/glosis/model/procedure/totalCarbonateEquivalentProcedure"/>
        <skos:notation>CaCO3_ca09</skos:notation>
        <skos:prefLabel xml:lang="en">CaCO3_ca09</skos:prefLabel>
        <skos:scopeNote rdf:resource="https://www.isric.org/sites/default/files/isric_report_2014_01.pdf"/>
        <skos:scopeNote>Leenaars J.G.B., A.J.M. van Oostrum and M. Ruiperez Gonzalez, 2014. Africa Soil Profiles Database, Version 1.2. A compilation of georeferenced and standardised legacy soil profile data for Sub-Saharan Africa (with dataset). ISRIC Report 2014/01. Africa Soil Information Service (AfSIS) project and ISRIC - World Soil Information, Wageningen, the Netherlands. See Annex 4.</skos:scopeNote>
        <skos:topConceptOf rdf:resource="http://w3id.org/glosis/model/procedure/totalCarbonateEquivalentProcedure"/>
    </owl:NamedIndividual>
    


    <!-- http://w3id.org/glosis/model/procedure/totalCarbonateEquivalentProcedure-CaCO3_ca10 -->


    <owl:NamedIndividual rdf:about="http://w3id.org/glosis/model/procedure/totalCarbonateEquivalentProcedure-CaCO3_ca10">
        <rdf:type rdf:resource="http://w3id.org/glosis/model/procedure/TotalCarbonateEquivalentProcedure"/>
        <rdf:type rdf:resource="http://www.w3.org/2004/02/skos/core#Concept"/>
        <skos:definition>CaCO3 Equivalent, CO2 evolution after HCl treatment. Gravimetric</skos:definition>
        <skos:inScheme rdf:resource="http://w3id.org/glosis/model/procedure/totalCarbonateEquivalentProcedure"/>
        <skos:notation>CaCO3_ca10</skos:notation>
        <skos:prefLabel xml:lang="en">CaCO3_ca10</skos:prefLabel>
        <skos:scopeNote rdf:resource="https://www.isric.org/sites/default/files/isric_report_2014_01.pdf"/>
        <skos:scopeNote>Leenaars J.G.B., A.J.M. van Oostrum and M. Ruiperez Gonzalez, 2014. Africa Soil Profiles Database, Version 1.2. A compilation of georeferenced and standardised legacy soil profile data for Sub-Saharan Africa (with dataset). ISRIC Report 2014/01. Africa Soil Information Service (AfSIS) project and ISRIC - World Soil Information, Wageningen, the Netherlands. See Annex 4.</skos:scopeNote>
        <skos:topConceptOf rdf:resource="http://w3id.org/glosis/model/procedure/totalCarbonateEquivalentProcedure"/>
    </owl:NamedIndividual>
    


    <!-- http://w3id.org/glosis/model/procedure/totalCarbonateEquivalentProcedure-CaCO3_ca11 -->


    <owl:NamedIndividual rdf:about="http://w3id.org/glosis/model/procedure/totalCarbonateEquivalentProcedure-CaCO3_ca11">
        <rdf:type rdf:resource="http://w3id.org/glosis/model/procedure/TotalCarbonateEquivalentProcedure"/>
        <rdf:type rdf:resource="http://www.w3.org/2004/02/skos/core#Concept"/>
        <skos:definition>Black, 1965-HCl</skos:definition>
        <skos:inScheme rdf:resource="http://w3id.org/glosis/model/procedure/totalCarbonateEquivalentProcedure"/>
        <skos:notation>CaCO3_ca11</skos:notation>
        <skos:prefLabel xml:lang="en">CaCO3_ca11</skos:prefLabel>
        <skos:scopeNote rdf:resource="https://www.isric.org/sites/default/files/isric_report_2014_01.pdf"/>
        <skos:scopeNote>Leenaars J.G.B., A.J.M. van Oostrum and M. Ruiperez Gonzalez, 2014. Africa Soil Profiles Database, Version 1.2. A compilation of georeferenced and standardised legacy soil profile data for Sub-Saharan Africa (with dataset). ISRIC Report 2014/01. Africa Soil Information Service (AfSIS) project and ISRIC - World Soil Information, Wageningen, the Netherlands. See Annex 4.</skos:scopeNote>
        <skos:topConceptOf rdf:resource="http://w3id.org/glosis/model/procedure/totalCarbonateEquivalentProcedure"/>
    </owl:NamedIndividual>
    


    <!-- http://w3id.org/glosis/model/procedure/totalCarbonateEquivalentProcedure-CaCO3_ca12 -->


    <owl:NamedIndividual rdf:about="http://w3id.org/glosis/model/procedure/totalCarbonateEquivalentProcedure-CaCO3_ca12">
        <rdf:type rdf:resource="http://w3id.org/glosis/model/procedure/TotalCarbonateEquivalentProcedure"/>
        <rdf:type rdf:resource="http://www.w3.org/2004/02/skos/core#Concept"/>
        <skos:definition>Treatment with H2SO4 N/2 acid followed by titration with NaOH N/2 in presence of an indicator</skos:definition>
        <skos:inScheme rdf:resource="http://w3id.org/glosis/model/procedure/totalCarbonateEquivalentProcedure"/>
        <skos:notation>CaCO3_ca12</skos:notation>
        <skos:prefLabel xml:lang="en">CaCO3_ca12</skos:prefLabel>
        <skos:scopeNote rdf:resource="https://www.isric.org/sites/default/files/isric_report_2014_01.pdf"/>
        <skos:scopeNote>Leenaars J.G.B., A.J.M. van Oostrum and M. Ruiperez Gonzalez, 2014. Africa Soil Profiles Database, Version 1.2. A compilation of georeferenced and standardised legacy soil profile data for Sub-Saharan Africa (with dataset). ISRIC Report 2014/01. Africa Soil Information Service (AfSIS) project and ISRIC - World Soil Information, Wageningen, the Netherlands. See Annex 4.</skos:scopeNote>
        <skos:topConceptOf rdf:resource="http://w3id.org/glosis/model/procedure/totalCarbonateEquivalentProcedure"/>
    </owl:NamedIndividual>
    


    <!-- http://w3id.org/glosis/model/procedure/totalCarbonateEquivalentProcedure-CaCO3_calcul-tc-oc -->


    <owl:NamedIndividual rdf:about="http://w3id.org/glosis/model/procedure/totalCarbonateEquivalentProcedure-CaCO3_calcul-tc-oc">
        <rdf:type rdf:resource="http://w3id.org/glosis/model/procedure/TotalCarbonateEquivalentProcedure"/>
        <rdf:type rdf:resource="http://www.w3.org/2004/02/skos/core#Concept"/>
        <skos:definition>Indirect estimate: inorganic carbon divided by 0.12 (computed as total carbon minus organic carbon)</skos:definition>
        <skos:inScheme rdf:resource="http://w3id.org/glosis/model/procedure/totalCarbonateEquivalentProcedure"/>
        <skos:notation>CaCO3_calcul-tc-oc</skos:notation>
        <skos:prefLabel xml:lang="en">CaCO3_calcul-tc-oc</skos:prefLabel>
        <skos:scopeNote rdf:resource="https://www.isric.org/sites/default/files/isric_report_2014_01.pdf"/>
        <skos:scopeNote>Leenaars J.G.B., A.J.M. van Oostrum and M. Ruiperez Gonzalez, 2014. Africa Soil Profiles Database, Version 1.2. A compilation of georeferenced and standardised legacy soil profile data for Sub-Saharan Africa (with dataset). ISRIC Report 2014/01. Africa Soil Information Service (AfSIS) project and ISRIC - World Soil Information, Wageningen, the Netherlands. See Annex 4.</skos:scopeNote>
        <skos:topConceptOf rdf:resource="http://w3id.org/glosis/model/procedure/totalCarbonateEquivalentProcedure"/>
    </owl:NamedIndividual>
    


    <!-- http://w3id.org/glosis/model/procedure/totalElementsProcedure -->


    <owl:NamedIndividual rdf:about="http://w3id.org/glosis/model/procedure/totalElementsProcedure">
        <rdf:type rdf:resource="http://www.w3.org/2004/02/skos/core#ConceptScheme"/>
        <rdfs:label xml:lang="en">Code list for totalElements analysis procedures - codelist scheme</rdfs:label>
        <rdfs:seeAlso rdf:resource="http://w3id.org/glosis/model/procedure/TotalElementsProcedure"/>
        <skos:definition>AfSP-derived interpretation (RwaSP)</skos:definition>
        <skos:note xml:lang="en">This code list provides analysis procedures for totalElements.</skos:note>
        <skos:prefLabel xml:lang="en">Code list for totalElements analysis procedures - codelist scheme</skos:prefLabel>
    </owl:NamedIndividual>
    


    <!-- http://w3id.org/glosis/model/procedure/totalElementsProcedure-Total_h2so4 -->


    <owl:NamedIndividual rdf:about="http://w3id.org/glosis/model/procedure/totalElementsProcedure-Total_h2so4">
        <rdf:type rdf:resource="http://w3id.org/glosis/model/procedure/TotalElementsProcedure"/>
        <rdf:type rdf:resource="http://www.w3.org/2004/02/skos/core#Concept"/>
        <skos:definition>Total P-/- colorimetric in H2SO4-Se-Salicylic acid digest( sulfuric acid) Particularly used for Total P.</skos:definition>
        <skos:inScheme rdf:resource="http://w3id.org/glosis/model/procedure/totalElementsProcedure"/>
        <skos:notation>Total_h2so4</skos:notation>
        <skos:prefLabel xml:lang="en">Total_h2so4</skos:prefLabel>
        <skos:scopeNote rdf:resource="https://www.isric.org/sites/default/files/isric_report_2014_01.pdf"/>
        <skos:scopeNote>Leenaars J.G.B., A.J.M. van Oostrum and M. Ruiperez Gonzalez, 2014. Africa Soil Profiles Database, Version 1.2. A compilation of georeferenced and standardised legacy soil profile data for Sub-Saharan Africa (with dataset). ISRIC Report 2014/01. Africa Soil Information Service (AfSIS) project and ISRIC - World Soil Information, Wageningen, the Netherlands. See Annex 4.</skos:scopeNote>
        <skos:topConceptOf rdf:resource="http://w3id.org/glosis/model/procedure/totalElementsProcedure"/>
    </owl:NamedIndividual>
    


    <!-- http://w3id.org/glosis/model/procedure/totalElementsProcedure-Total_hcl -->


    <owl:NamedIndividual rdf:about="http://w3id.org/glosis/model/procedure/totalElementsProcedure-Total_hcl">
        <rdf:type rdf:resource="http://w3id.org/glosis/model/procedure/TotalElementsProcedure"/>
        <rdf:type rdf:resource="http://www.w3.org/2004/02/skos/core#Concept"/>
        <skos:definition>HCl extraction. Particularly used for Total P.</skos:definition>
        <skos:inScheme rdf:resource="http://w3id.org/glosis/model/procedure/totalElementsProcedure"/>
        <skos:notation>Total_hcl</skos:notation>
        <skos:prefLabel xml:lang="en">Total_hcl</skos:prefLabel>
        <skos:scopeNote rdf:resource="https://www.isric.org/sites/default/files/isric_report_2014_01.pdf"/>
        <skos:scopeNote>Leenaars J.G.B., A.J.M. van Oostrum and M. Ruiperez Gonzalez, 2014. Africa Soil Profiles Database, Version 1.2. A compilation of georeferenced and standardised legacy soil profile data for Sub-Saharan Africa (with dataset). ISRIC Report 2014/01. Africa Soil Information Service (AfSIS) project and ISRIC - World Soil Information, Wageningen, the Netherlands. See Annex 4.</skos:scopeNote>
        <skos:topConceptOf rdf:resource="http://w3id.org/glosis/model/procedure/totalElementsProcedure"/>
    </owl:NamedIndividual>
    


    <!-- http://w3id.org/glosis/model/procedure/totalElementsProcedure-Total_hcl-aquaregia -->


    <owl:NamedIndividual rdf:about="http://w3id.org/glosis/model/procedure/totalElementsProcedure-Total_hcl-aquaregia">
        <rdf:type rdf:resource="http://w3id.org/glosis/model/procedure/TotalElementsProcedure"/>
        <rdf:type rdf:resource="http://www.w3.org/2004/02/skos/core#Concept"/>
        <skos:definition>Hydrocloric (HCl) extraction in nitric/perchloric acid mixture (totals) aqua regia</skos:definition>
        <skos:inScheme rdf:resource="http://w3id.org/glosis/model/procedure/totalElementsProcedure"/>
        <skos:notation>Total_hcl-aquaregia</skos:notation>
        <skos:prefLabel xml:lang="en">Total_hcl-aquaregia</skos:prefLabel>
        <skos:scopeNote rdf:resource="https://www.isric.org/sites/default/files/isric_report_2014_01.pdf"/>
        <skos:scopeNote>Leenaars J.G.B., A.J.M. van Oostrum and M. Ruiperez Gonzalez, 2014. Africa Soil Profiles Database, Version 1.2. A compilation of georeferenced and standardised legacy soil profile data for Sub-Saharan Africa (with dataset). ISRIC Report 2014/01. Africa Soil Information Service (AfSIS) project and ISRIC - World Soil Information, Wageningen, the Netherlands. See Annex 4.</skos:scopeNote>
        <skos:topConceptOf rdf:resource="http://w3id.org/glosis/model/procedure/totalElementsProcedure"/>
    </owl:NamedIndividual>
    


    <!-- http://w3id.org/glosis/model/procedure/totalElementsProcedure-Total_hclo4 -->


    <owl:NamedIndividual rdf:about="http://w3id.org/glosis/model/procedure/totalElementsProcedure-Total_hclo4">
        <rdf:type rdf:resource="http://w3id.org/glosis/model/procedure/TotalElementsProcedure"/>
        <rdf:type rdf:resource="http://www.w3.org/2004/02/skos/core#Concept"/>
        <skos:definition>Perchloric acid percolation. Particularly used for Total P.</skos:definition>
        <skos:inScheme rdf:resource="http://w3id.org/glosis/model/procedure/totalElementsProcedure"/>
        <skos:notation>Total_hclo4</skos:notation>
        <skos:prefLabel xml:lang="en">Total_hclo4</skos:prefLabel>
        <skos:scopeNote rdf:resource="https://www.isric.org/sites/default/files/isric_report_2014_01.pdf"/>
        <skos:scopeNote>Leenaars J.G.B., A.J.M. van Oostrum and M. Ruiperez Gonzalez, 2014. Africa Soil Profiles Database, Version 1.2. A compilation of georeferenced and standardised legacy soil profile data for Sub-Saharan Africa (with dataset). ISRIC Report 2014/01. Africa Soil Information Service (AfSIS) project and ISRIC - World Soil Information, Wageningen, the Netherlands. See Annex 4.</skos:scopeNote>
        <skos:topConceptOf rdf:resource="http://w3id.org/glosis/model/procedure/totalElementsProcedure"/>
    </owl:NamedIndividual>
    


    <!-- http://w3id.org/glosis/model/procedure/totalElementsProcedure-Total_hno3-aquafortis -->


    <owl:NamedIndividual rdf:about="http://w3id.org/glosis/model/procedure/totalElementsProcedure-Total_hno3-aquafortis">
        <rdf:type rdf:resource="http://w3id.org/glosis/model/procedure/TotalElementsProcedure"/>
        <rdf:type rdf:resource="http://www.w3.org/2004/02/skos/core#Concept"/>
        <skos:definition>Nitric acid attack. Particularly used for Total P.</skos:definition>
        <skos:inScheme rdf:resource="http://w3id.org/glosis/model/procedure/totalElementsProcedure"/>
        <skos:notation>Total_hno3-aquafortis</skos:notation>
        <skos:prefLabel xml:lang="en">Total_hno3-aquafortis</skos:prefLabel>
        <skos:scopeNote rdf:resource="https://www.isric.org/sites/default/files/isric_report_2014_01.pdf"/>
        <skos:scopeNote>Leenaars J.G.B., A.J.M. van Oostrum and M. Ruiperez Gonzalez, 2014. Africa Soil Profiles Database, Version 1.2. A compilation of georeferenced and standardised legacy soil profile data for Sub-Saharan Africa (with dataset). ISRIC Report 2014/01. Africa Soil Information Service (AfSIS) project and ISRIC - World Soil Information, Wageningen, the Netherlands. See Annex 4.</skos:scopeNote>
        <skos:topConceptOf rdf:resource="http://w3id.org/glosis/model/procedure/totalElementsProcedure"/>
    </owl:NamedIndividual>
    


    <!-- http://w3id.org/glosis/model/procedure/totalElementsProcedure-Total_nh4-6mo7o24 -->


    <owl:NamedIndividual rdf:about="http://w3id.org/glosis/model/procedure/totalElementsProcedure-Total_nh4-6mo7o24">
        <rdf:type rdf:resource="http://w3id.org/glosis/model/procedure/TotalElementsProcedure"/>
        <rdf:type rdf:resource="http://www.w3.org/2004/02/skos/core#Concept"/>
        <skos:definition>COLORIMETRIC VANADATE MOLYBDATE. Particularly used for Total P.</skos:definition>
        <skos:inScheme rdf:resource="http://w3id.org/glosis/model/procedure/totalElementsProcedure"/>
        <skos:notation>Total_nh4-6mo7o24</skos:notation>
        <skos:prefLabel xml:lang="en">Total_nh4-6mo7o24</skos:prefLabel>
        <skos:scopeNote rdf:resource="https://www.isric.org/sites/default/files/isric_report_2014_01.pdf"/>
        <skos:scopeNote>Leenaars J.G.B., A.J.M. van Oostrum and M. Ruiperez Gonzalez, 2014. Africa Soil Profiles Database, Version 1.2. A compilation of georeferenced and standardised legacy soil profile data for Sub-Saharan Africa (with dataset). ISRIC Report 2014/01. Africa Soil Information Service (AfSIS) project and ISRIC - World Soil Information, Wageningen, the Netherlands. See Annex 4.</skos:scopeNote>
        <skos:topConceptOf rdf:resource="http://w3id.org/glosis/model/procedure/totalElementsProcedure"/>
    </owl:NamedIndividual>
    


    <!-- http://w3id.org/glosis/model/procedure/totalElementsProcedure-Total_tp03 -->


    <owl:NamedIndividual rdf:about="http://w3id.org/glosis/model/procedure/totalElementsProcedure-Total_tp03">
        <rdf:type rdf:resource="http://w3id.org/glosis/model/procedure/TotalElementsProcedure"/>
        <rdf:type rdf:resource="http://www.w3.org/2004/02/skos/core#Concept"/>
        <skos:definition>reagent of Baeyens. Precipitation in form of Phosphomolybdate. Particularly used for Total P.</skos:definition>
        <skos:inScheme rdf:resource="http://w3id.org/glosis/model/procedure/totalElementsProcedure"/>
        <skos:notation>Total_tp03</skos:notation>
        <skos:prefLabel xml:lang="en">Total_tp03</skos:prefLabel>
        <skos:scopeNote rdf:resource="https://www.isric.org/sites/default/files/isric_report_2014_01.pdf"/>
        <skos:scopeNote>Leenaars J.G.B., A.J.M. van Oostrum and M. Ruiperez Gonzalez, 2014. Africa Soil Profiles Database, Version 1.2. A compilation of georeferenced and standardised legacy soil profile data for Sub-Saharan Africa (with dataset). ISRIC Report 2014/01. Africa Soil Information Service (AfSIS) project and ISRIC - World Soil Information, Wageningen, the Netherlands. See Annex 4.</skos:scopeNote>
        <skos:topConceptOf rdf:resource="http://w3id.org/glosis/model/procedure/totalElementsProcedure"/>
    </owl:NamedIndividual>
    


    <!-- http://w3id.org/glosis/model/procedure/totalElementsProcedure-Total_tp04 -->


    <owl:NamedIndividual rdf:about="http://w3id.org/glosis/model/procedure/totalElementsProcedure-Total_tp04">
        <rdf:type rdf:resource="http://w3id.org/glosis/model/procedure/TotalElementsProcedure"/>
        <rdf:type rdf:resource="http://www.w3.org/2004/02/skos/core#Concept"/>
        <skos:definition>acid fleischman. Particularly used for Total P.</skos:definition>
        <skos:inScheme rdf:resource="http://w3id.org/glosis/model/procedure/totalElementsProcedure"/>
        <skos:notation>Total_tp04</skos:notation>
        <skos:prefLabel xml:lang="en">Total_tp04</skos:prefLabel>
        <skos:scopeNote rdf:resource="https://www.isric.org/sites/default/files/isric_report_2014_01.pdf"/>
        <skos:scopeNote>Leenaars J.G.B., A.J.M. van Oostrum and M. Ruiperez Gonzalez, 2014. Africa Soil Profiles Database, Version 1.2. A compilation of georeferenced and standardised legacy soil profile data for Sub-Saharan Africa (with dataset). ISRIC Report 2014/01. Africa Soil Information Service (AfSIS) project and ISRIC - World Soil Information, Wageningen, the Netherlands. See Annex 4.</skos:scopeNote>
        <skos:topConceptOf rdf:resource="http://w3id.org/glosis/model/procedure/totalElementsProcedure"/>
    </owl:NamedIndividual>
    


    <!-- http://w3id.org/glosis/model/procedure/totalElementsProcedure-Total_tp05 -->


    <owl:NamedIndividual rdf:about="http://w3id.org/glosis/model/procedure/totalElementsProcedure-Total_tp05">
        <rdf:type rdf:resource="http://w3id.org/glosis/model/procedure/TotalElementsProcedure"/>
        <rdf:type rdf:resource="http://www.w3.org/2004/02/skos/core#Concept"/>
        <skos:definition>8 M HCl extraction. Particularly used for Total P.</skos:definition>
        <skos:inScheme rdf:resource="http://w3id.org/glosis/model/procedure/totalElementsProcedure"/>
        <skos:notation>Total_tp05</skos:notation>
        <skos:prefLabel xml:lang="en">Total_tp05</skos:prefLabel>
        <skos:scopeNote rdf:resource="https://www.isric.org/sites/default/files/isric_report_2014_01.pdf"/>
        <skos:scopeNote>Leenaars J.G.B., A.J.M. van Oostrum and M. Ruiperez Gonzalez, 2014. Africa Soil Profiles Database, Version 1.2. A compilation of georeferenced and standardised legacy soil profile data for Sub-Saharan Africa (with dataset). ISRIC Report 2014/01. Africa Soil Information Service (AfSIS) project and ISRIC - World Soil Information, Wageningen, the Netherlands. See Annex 4.</skos:scopeNote>
        <skos:topConceptOf rdf:resource="http://w3id.org/glosis/model/procedure/totalElementsProcedure"/>
    </owl:NamedIndividual>
    


    <!-- http://w3id.org/glosis/model/procedure/totalElementsProcedure-Total_tp06 -->


    <owl:NamedIndividual rdf:about="http://w3id.org/glosis/model/procedure/totalElementsProcedure-Total_tp06">
        <rdf:type rdf:resource="http://w3id.org/glosis/model/procedure/TotalElementsProcedure"/>
        <rdf:type rdf:resource="http://www.w3.org/2004/02/skos/core#Concept"/>
        <skos:definition>Molybdenum blue method, using ascorbic acid as reductant after heating of soil to 550 C and extraction with 6M sulphuric acid. Particularly used for Total P.</skos:definition>
        <skos:inScheme rdf:resource="http://w3id.org/glosis/model/procedure/totalElementsProcedure"/>
        <skos:notation>Total_tp06</skos:notation>
        <skos:prefLabel xml:lang="en">Total_tp06</skos:prefLabel>
        <skos:scopeNote rdf:resource="https://www.isric.org/sites/default/files/isric_report_2014_01.pdf"/>
        <skos:scopeNote>Leenaars J.G.B., A.J.M. van Oostrum and M. Ruiperez Gonzalez, 2014. Africa Soil Profiles Database, Version 1.2. A compilation of georeferenced and standardised legacy soil profile data for Sub-Saharan Africa (with dataset). ISRIC Report 2014/01. Africa Soil Information Service (AfSIS) project and ISRIC - World Soil Information, Wageningen, the Netherlands. See Annex 4.</skos:scopeNote>
        <skos:topConceptOf rdf:resource="http://w3id.org/glosis/model/procedure/totalElementsProcedure"/>
    </owl:NamedIndividual>
    


    <!-- http://w3id.org/glosis/model/procedure/totalElementsProcedure-Total_tp07 -->


    <owl:NamedIndividual rdf:about="http://w3id.org/glosis/model/procedure/totalElementsProcedure-Total_tp07">
        <rdf:type rdf:resource="http://w3id.org/glosis/model/procedure/TotalElementsProcedure"/>
        <rdf:type rdf:resource="http://www.w3.org/2004/02/skos/core#Concept"/>
        <skos:definition>1:1 H2SO4 : HNO3. Particularly used for Total P.</skos:definition>
        <skos:inScheme rdf:resource="http://w3id.org/glosis/model/procedure/totalElementsProcedure"/>
        <skos:notation>Total_tp07</skos:notation>
        <skos:prefLabel xml:lang="en">Total_tp07</skos:prefLabel>
        <skos:scopeNote rdf:resource="https://www.isric.org/sites/default/files/isric_report_2014_01.pdf"/>
        <skos:scopeNote>Leenaars J.G.B., A.J.M. van Oostrum and M. Ruiperez Gonzalez, 2014. Africa Soil Profiles Database, Version 1.2. A compilation of georeferenced and standardised legacy soil profile data for Sub-Saharan Africa (with dataset). ISRIC Report 2014/01. Africa Soil Information Service (AfSIS) project and ISRIC - World Soil Information, Wageningen, the Netherlands. See Annex 4.</skos:scopeNote>
        <skos:topConceptOf rdf:resource="http://w3id.org/glosis/model/procedure/totalElementsProcedure"/>
    </owl:NamedIndividual>
    


    <!-- http://w3id.org/glosis/model/procedure/totalElementsProcedure-Total_tp08 -->


    <owl:NamedIndividual rdf:about="http://w3id.org/glosis/model/procedure/totalElementsProcedure-Total_tp08">
        <rdf:type rdf:resource="http://w3id.org/glosis/model/procedure/TotalElementsProcedure"/>
        <rdf:type rdf:resource="http://www.w3.org/2004/02/skos/core#Concept"/>
        <skos:definition>After Nitric acid attack (boiling with HNO3), colometric determination (method of Duval).. Particularly used for Total P.</skos:definition>
        <skos:inScheme rdf:resource="http://w3id.org/glosis/model/procedure/totalElementsProcedure"/>
        <skos:notation>Total_tp08</skos:notation>
        <skos:prefLabel xml:lang="en">Total_tp08</skos:prefLabel>
        <skos:scopeNote rdf:resource="https://www.isric.org/sites/default/files/isric_report_2014_01.pdf"/>
        <skos:scopeNote>Leenaars J.G.B., A.J.M. van Oostrum and M. Ruiperez Gonzalez, 2014. Africa Soil Profiles Database, Version 1.2. A compilation of georeferenced and standardised legacy soil profile data for Sub-Saharan Africa (with dataset). ISRIC Report 2014/01. Africa Soil Information Service (AfSIS) project and ISRIC - World Soil Information, Wageningen, the Netherlands. See Annex 4.</skos:scopeNote>
        <skos:topConceptOf rdf:resource="http://w3id.org/glosis/model/procedure/totalElementsProcedure"/>
    </owl:NamedIndividual>
    


    <!-- http://w3id.org/glosis/model/procedure/totalElementsProcedure-Total_tp09 -->


    <owl:NamedIndividual rdf:about="http://w3id.org/glosis/model/procedure/totalElementsProcedure-Total_tp09">
        <rdf:type rdf:resource="http://w3id.org/glosis/model/procedure/TotalElementsProcedure"/>
        <rdf:type rdf:resource="http://www.w3.org/2004/02/skos/core#Concept"/>
        <skos:definition>Walker and Adams, 1958. Particularly used for Total P.</skos:definition>
        <skos:inScheme rdf:resource="http://w3id.org/glosis/model/procedure/totalElementsProcedure"/>
        <skos:notation>Total_tp09</skos:notation>
        <skos:prefLabel xml:lang="en">Total_tp09</skos:prefLabel>
        <skos:scopeNote>WALKER, T. W., AND A. F. R. ADAMS. 1958. Studies on soil organic matter. I. Soil Sci. 85: 307-318. </skos:scopeNote>
        <skos:topConceptOf rdf:resource="http://w3id.org/glosis/model/procedure/totalElementsProcedure"/>
    </owl:NamedIndividual>
    


    <!-- http://w3id.org/glosis/model/procedure/totalElementsProcedure-Total_tp10 -->


    <owl:NamedIndividual rdf:about="http://w3id.org/glosis/model/procedure/totalElementsProcedure-Total_tp10">
        <rdf:type rdf:resource="http://w3id.org/glosis/model/procedure/TotalElementsProcedure"/>
        <rdf:type rdf:resource="http://www.w3.org/2004/02/skos/core#Concept"/>
        <skos:definition>Colorimetric, unspecified extract</skos:definition>
        <skos:inScheme rdf:resource="http://w3id.org/glosis/model/procedure/totalElementsProcedure"/>
        <skos:notation>Total_tp10</skos:notation>
        <skos:prefLabel xml:lang="en">Total_tp10</skos:prefLabel>
        <skos:scopeNote rdf:resource="https://www.isric.org/sites/default/files/isric_report_2014_01.pdf"/>
        <skos:scopeNote>Leenaars J.G.B., A.J.M. van Oostrum and M. Ruiperez Gonzalez, 2014. Africa Soil Profiles Database, Version 1.2. A compilation of georeferenced and standardised legacy soil profile data for Sub-Saharan Africa (with dataset). ISRIC Report 2014/01. Africa Soil Information Service (AfSIS) project and ISRIC - World Soil Information, Wageningen, the Netherlands. See Annex 4.</skos:scopeNote>
        <skos:topConceptOf rdf:resource="http://w3id.org/glosis/model/procedure/totalElementsProcedure"/>
    </owl:NamedIndividual>
    


    <!-- http://w3id.org/glosis/model/procedure/totalElementsProcedure-Total_unkn -->


    <owl:NamedIndividual rdf:about="http://w3id.org/glosis/model/procedure/totalElementsProcedure-Total_unkn">
        <rdf:type rdf:resource="http://w3id.org/glosis/model/procedure/TotalElementsProcedure"/>
        <rdf:type rdf:resource="http://www.w3.org/2004/02/skos/core#Concept"/>
        <skos:definition>Unspecified method</skos:definition>
        <skos:inScheme rdf:resource="http://w3id.org/glosis/model/procedure/totalElementsProcedure"/>
        <skos:notation>Total_unkn</skos:notation>
        <skos:prefLabel xml:lang="en">Total_unk</skos:prefLabel>
        <skos:scopeNote rdf:resource="https://www.isric.org/sites/default/files/isric_report_2014_01.pdf"/>
        <skos:scopeNote>Leenaars J.G.B., A.J.M. van Oostrum and M. Ruiperez Gonzalez, 2014. Africa Soil Profiles Database, Version 1.2. A compilation of georeferenced and standardised legacy soil profile data for Sub-Saharan Africa (with dataset). ISRIC Report 2014/01. Africa Soil Information Service (AfSIS) project and ISRIC - World Soil Information, Wageningen, the Netherlands. See Annex 4.</skos:scopeNote>
        <skos:topConceptOf rdf:resource="http://w3id.org/glosis/model/procedure/totalElementsProcedure"/>
    </owl:NamedIndividual>
    


    <!-- http://w3id.org/glosis/model/procedure/totalElementsProcedure-Total_xrd -->


    <owl:NamedIndividual rdf:about="http://w3id.org/glosis/model/procedure/totalElementsProcedure-Total_xrd">
        <rdf:type rdf:resource="http://w3id.org/glosis/model/procedure/TotalElementsProcedure"/>
        <rdf:type rdf:resource="http://www.w3.org/2004/02/skos/core#Concept"/>
        <skos:definition>XRD</skos:definition>
        <skos:inScheme rdf:resource="http://w3id.org/glosis/model/procedure/totalElementsProcedure"/>
        <skos:notation>Total_xrd</skos:notation>
        <skos:prefLabel xml:lang="en">Total_xrd</skos:prefLabel>
        <skos:scopeNote rdf:resource="https://www.isric.org/sites/default/files/isric_report_2014_01.pdf"/>
        <skos:scopeNote>Leenaars J.G.B., A.J.M. van Oostrum and M. Ruiperez Gonzalez, 2014. Africa Soil Profiles Database, Version 1.2. A compilation of georeferenced and standardised legacy soil profile data for Sub-Saharan Africa (with dataset). ISRIC Report 2014/01. Africa Soil Information Service (AfSIS) project and ISRIC - World Soil Information, Wageningen, the Netherlands. See Annex 4.</skos:scopeNote>
        <skos:topConceptOf rdf:resource="http://w3id.org/glosis/model/procedure/totalElementsProcedure"/>
    </owl:NamedIndividual>
    


    <!-- http://w3id.org/glosis/model/procedure/totalElementsProcedure-Total_xrf -->


    <owl:NamedIndividual rdf:about="http://w3id.org/glosis/model/procedure/totalElementsProcedure-Total_xrf">
        <rdf:type rdf:resource="http://w3id.org/glosis/model/procedure/TotalElementsProcedure"/>
        <rdf:type rdf:resource="http://www.w3.org/2004/02/skos/core#Concept"/>
        <skos:definition>XRF</skos:definition>
        <skos:inScheme rdf:resource="http://w3id.org/glosis/model/procedure/totalElementsProcedure"/>
        <skos:notation>Total_xrf</skos:notation>
        <skos:prefLabel xml:lang="en">Total_xrf</skos:prefLabel>
        <skos:scopeNote rdf:resource="https://www.isric.org/sites/default/files/isric_report_2014_01.pdf"/>
        <skos:scopeNote>Leenaars J.G.B., A.J.M. van Oostrum and M. Ruiperez Gonzalez, 2014. Africa Soil Profiles Database, Version 1.2. A compilation of georeferenced and standardised legacy soil profile data for Sub-Saharan Africa (with dataset). ISRIC Report 2014/01. Africa Soil Information Service (AfSIS) project and ISRIC - World Soil Information, Wageningen, the Netherlands. See Annex 4.</skos:scopeNote>
        <skos:topConceptOf rdf:resource="http://w3id.org/glosis/model/procedure/totalElementsProcedure"/>
    </owl:NamedIndividual>
    


    <!-- http://w3id.org/glosis/model/procedure/totalElementsProcedure-Total_xrf-p -->


    <owl:NamedIndividual rdf:about="http://w3id.org/glosis/model/procedure/totalElementsProcedure-Total_xrf-p">
        <rdf:type rdf:resource="http://w3id.org/glosis/model/procedure/TotalElementsProcedure"/>
        <rdf:type rdf:resource="http://www.w3.org/2004/02/skos/core#Concept"/>
        <skos:definition>PXRF</skos:definition>
        <skos:inScheme rdf:resource="http://w3id.org/glosis/model/procedure/totalElementsProcedure"/>
        <skos:notation>Total_xrf-p</skos:notation>
        <skos:prefLabel xml:lang="en">Total_xrf-p</skos:prefLabel>
        <skos:scopeNote rdf:resource="https://www.isric.org/sites/default/files/isric_report_2014_01.pdf"/>
        <skos:scopeNote>Leenaars J.G.B., A.J.M. van Oostrum and M. Ruiperez Gonzalez, 2014. Africa Soil Profiles Database, Version 1.2. A compilation of georeferenced and standardised legacy soil profile data for Sub-Saharan Africa (with dataset). ISRIC Report 2014/01. Africa Soil Information Service (AfSIS) project and ISRIC - World Soil Information, Wageningen, the Netherlands. See Annex 4.</skos:scopeNote>
        <skos:topConceptOf rdf:resource="http://w3id.org/glosis/model/procedure/totalElementsProcedure"/>
    </owl:NamedIndividual>
    


    <!-- http://w3id.org/glosis/model/procedure/totalElementsProcedure-Total_xtf-t -->


    <owl:NamedIndividual rdf:about="http://w3id.org/glosis/model/procedure/totalElementsProcedure-Total_xtf-t">
        <rdf:type rdf:resource="http://w3id.org/glosis/model/procedure/TotalElementsProcedure"/>
        <rdf:type rdf:resource="http://www.w3.org/2004/02/skos/core#Concept"/>
        <skos:definition>TXRF</skos:definition>
        <skos:inScheme rdf:resource="http://w3id.org/glosis/model/procedure/totalElementsProcedure"/>
        <skos:notation>Total_xtf-t</skos:notation>
        <skos:prefLabel xml:lang="en">Total_xtf-t</skos:prefLabel>
        <skos:scopeNote rdf:resource="https://www.isric.org/sites/default/files/isric_report_2014_01.pdf"/>
        <skos:scopeNote>Leenaars J.G.B., A.J.M. van Oostrum and M. Ruiperez Gonzalez, 2014. Africa Soil Profiles Database, Version 1.2. A compilation of georeferenced and standardised legacy soil profile data for Sub-Saharan Africa (with dataset). ISRIC Report 2014/01. Africa Soil Information Service (AfSIS) project and ISRIC - World Soil Information, Wageningen, the Netherlands. See Annex 4.</skos:scopeNote>
        <skos:topConceptOf rdf:resource="http://w3id.org/glosis/model/procedure/totalElementsProcedure"/>
    </owl:NamedIndividual>
</rdf:RDF>



<!-- Generated by the OWL API (version 5.1.18) https://github.com/owlcs/owlapi/ -->


